<?xml version="1.0" encoding="UTF-8"?>
<rdf:RDF
	xmlns:skos="http://www.w3.org/2004/02/skos/core#"
	xmlns:dc="http://purl.org/dc/elements/1.1/"
	xmlns:dcterms="http://purl.org/dc/terms/"
	xmlns:geo="http://www.w3.org/2003/01/geo/wgs84_pos#"
	xmlns:iso-thes="http://purl.org/iso25964/skos-thes#"
	xmlns:opentheso="http://purl.org/umu/uneskos#"
	xmlns:foaf="http://xmlns.com/foaf/0.1/"
	xmlns:owl="http://www.w3.org/2002/07/owl#"
	xmlns:wdt="http://www.opengis.net/ont/geosparql#"
	xmlns:rdf="http://www.w3.org/1999/02/22-rdf-syntax-ns#">

<rdf:Description rdf:about="https://ark.frantiq.fr/ark:/26678/TH_1">
	<rdf:type rdf:resource="http://www.w3.org/2004/02/skos/core#ConceptScheme"/>
	<skos:prefLabel xml:lang="ar">pactols_2</skos:prefLabel>
	<skos:prefLabel xml:lang="fr">Pactols_Sujets</skos:prefLabel>
	<skos:prefLabel xml:lang="de">Pactols_Themen</skos:prefLabel>
	<skos:prefLabel xml:lang="es">Pactols_Temas</skos:prefLabel>
	<skos:prefLabel xml:lang="nl">Pactols_Topics</skos:prefLabel>
	<skos:prefLabel xml:lang="ru">Pactols_Tema</skos:prefLabel>
	<skos:prefLabel xml:lang="it">Pactols_Temi</skos:prefLabel>
	<skos:prefLabel xml:lang="en">Pactols_Subjects</skos:prefLabel>
	<skos:prefLabel xml:lang="el">Pactols_Topics</skos:prefLabel>
	<skos:prefLabel xml:lang="he">Pactols_Subjects</skos:prefLabel>
	<skos:hasTopConcept rdf:resource="https://ark.frantiq.fr/ark:/26678/pcrtgSbjUSVUr8"/>
	<skos:hasTopConcept rdf:resource="https://ark.frantiq.fr/ark:/26678/pcrt8n40q9ng1p"/>
	<skos:hasTopConcept rdf:resource="https://ark.frantiq.fr/ark:/26678/pcrtIMsuG0RWTs"/>
	<skos:hasTopConcept rdf:resource="https://ark.frantiq.fr/ark:/26678/pcrtqOnvbkSUvu"/>
	<skos:hasTopConcept rdf:resource="https://ark.frantiq.fr/ark:/26678/pcrtnQFBp7vRwb"/>
	<skos:hasTopConcept rdf:resource="https://ark.frantiq.fr/ark:/26678/pcrtb8pL8xI1LB"/>
	<skos:hasTopConcept rdf:resource="https://ark.frantiq.fr/ark:/26678/pcrtGrTrckrNHZ"/>
	<skos:hasTopConcept rdf:resource="https://ark.frantiq.fr/ark:/26678/pcrt1GPZLeLDoN"/>
	<skos:hasTopConcept rdf:resource="https://ark.frantiq.fr/ark:/26678/pcrtx7DI4bZtuR"/>
	<skos:hasTopConcept rdf:resource="https://ark.frantiq.fr/ark:/26678/pcrtYXEBytBn39"/>
	<skos:hasTopConcept rdf:resource="https://ark.frantiq.fr/ark:/26678/pcrt73REVYeFXQ"/>
	<skos:hasTopConcept rdf:resource="https://ark.frantiq.fr/ark:/26678/pcrtmvnhq9hpgb"/>
	<skos:hasTopConcept rdf:resource="https://ark.frantiq.fr/ark:/26678/pcrtu1uuSJeF5V"/>
	<dcterms:created rdf:datatype="http://www.w3.org/2001/XMLSchema#date">2014-10-06</dcterms:created>
	<dcterms:modified rdf:datatype="http://www.w3.org/2001/XMLSchema#date">2014-10-06</dcterms:modified>
	<dcterms:creator>blandine.nouvel</dcterms:creator>
	<dcterms:contributor>blandine.nouvel</dcterms:contributor>
	<dcterms:title>Pactols_Subjects</dcterms:title>
	<dcterms:language>he</dcterms:language>
	<dcterms:contributor xml:lang="en">Pactols Working Group</dcterms:contributor>
	<dcterms:publisher xml:lang="fr">Centre national de la recherche scientifique (CNRS)</dcterms:publisher>
	<dcterms:contributor xml:lang="fr">Groupe de travail Pactols</dcterms:contributor>
	<dcterms:format>SKOS</dcterms:format>
	<dcterms:language>fr</dcterms:language>
	<dcterms:language>en</dcterms:language>
	<dcterms:language>it</dcterms:language>
	<dcterms:language>es</dcterms:language>
	<dcterms:language>de</dcterms:language>
	<dcterms:language>nl</dcterms:language>
	<dcterms:language>ar</dcterms:language>
	<dcterms:created rdf:datatype="http://www.w3.org/2001/XMLSchema#date">1987</dcterms:created>
	<dcterms:rightsHolder>CNRS-Frantiq</dcterms:rightsHolder>
	<dcterms:license>OdBL</dcterms:license>
	<dcterms:title xml:lang="fr">Pactols Sujets</dcterms:title>
	<dcterms:creator xml:lang="fr">Pactols Sujets</dcterms:creator>
	<dcterms:type xml:lang="en">thesaurus</dcterms:type>
	<dcterms:creator xml:lang="fr">Fédération et Ressources sur l'Antiquité (Frantiq)</dcterms:creator>
	<dcterms:description xml:lang="fr">Thésaurus sur l'archéologie, depuis la Préhistoire jusqu'à la période contemporaine, et sur les sciences de l'Antiquité</dcterms:description>
	<dcterms:description xml:lang="en">Thesaurus about archaeology, from Prehistory to the contemporary period, and about classical studies</dcterms:description>
	<dcterms:modified rdf:datatype="http://www.w3.org/2001/XMLSchema#date">2022-09-21</dcterms:modified>
	<dcterms:subject>archéologie</dcterms:subject>
	<dcterms:subject>archaeology</dcterms:subject>
	<dcterms:identifier rdf:resource="https://pactols.frantiq.fr/opentheso/?idt=TH_1"/>
	<dcterms:contributor>Juliette Testard</dcterms:contributor>
	<dcterms:contributor>Guillaume Reich</dcterms:contributor>
	<dcterms:title>Patricia Moitrel</dcterms:title>
	<dcterms:creator>Patricia Moitrel</dcterms:creator>
	<dcterms:contributor>Christelle Molinié</dcterms:contributor>
	<dcterms:contributor>Emmanuelle Bryas</dcterms:contributor>
	<dcterms:contributor>Rémi Ancel</dcterms:contributor>
	<dcterms:contributor>Sophie Kielwasser</dcterms:contributor>
	<dcterms:contributor>Justine Vincent</dcterms:contributor>
	<dcterms:contributor>Evelyne Sinigaglia</dcterms:contributor>
	<dcterms:contributor>Blandine Nouvel</dcterms:contributor>
	<dcterms:subject>classics</dcterms:subject>
	<dcterms:subject xml:lang="fr">science de l'Antiquité</dcterms:subject>
</rdf:Description>

<rdf:Description rdf:about="https://ark.frantiq.fr/ark:/26678/pcrtv66rn9cbv1">
	<rdf:type rdf:resource="http://www.w3.org/2004/02/skos/core#Collection"/>
	<skos:prefLabel xml:lang="en">Facet : Materials</skos:prefLabel>
	<skos:prefLabel xml:lang="fr">P2-MATÉRIAUX</skos:prefLabel>
	<iso-thes:microThesaurusOf rdf:resource="https://ark.frantiq.fr/ark:/26678/pcrtv66rn9cbv1"/>
	<skos:member rdf:resource="https://ark.frantiq.fr/ark:/26678/pcrt3KtdnXPGUg"/>
	<skos:member rdf:resource="https://ark.frantiq.fr/ark:/26678/pcrthELuSjXqGH"/>
	<skos:member rdf:resource="https://ark.frantiq.fr/ark:/26678/pcrtqmXRwn2Az6"/>
	<skos:member rdf:resource="https://ark.frantiq.fr/ark:/26678/pcrtyJc250eY3m"/>
	<skos:member rdf:resource="https://ark.frantiq.fr/ark:/26678/pcrtgcn5U8laUN"/>
	<skos:member rdf:resource="https://ark.frantiq.fr/ark:/26678/pcrtzcGlM17go5"/>
	<skos:member rdf:resource="https://ark.frantiq.fr/ark:/26678/pcrtuV4RYc06TP"/>
	<skos:member rdf:resource="https://ark.frantiq.fr/ark:/26678/pcrtSiQAzZxXsv"/>
	<skos:member rdf:resource="https://ark.frantiq.fr/ark:/26678/pcrt0IaUrrrmF5"/>
	<skos:member rdf:resource="https://ark.frantiq.fr/ark:/26678/pcrtcWoSlbWLE0"/>
	<skos:member rdf:resource="https://ark.frantiq.fr/ark:/26678/pcrto44p1SaKFn"/>
	<skos:member rdf:resource="https://ark.frantiq.fr/ark:/26678/pcrtgjwqPbWjHa"/>
	<skos:member rdf:resource="https://ark.frantiq.fr/ark:/26678/pcrt5mFxzmQ9rX"/>
	<skos:member rdf:resource="https://ark.frantiq.fr/ark:/26678/pcrtctuE9VNJOc"/>
	<skos:member rdf:resource="https://ark.frantiq.fr/ark:/26678/pcrtnsH1xdYgZe"/>
	<skos:member rdf:resource="https://ark.frantiq.fr/ark:/26678/pcrt3nBjHrcDGM"/>
	<skos:member rdf:resource="https://ark.frantiq.fr/ark:/26678/pcrtMr3tb79bV8"/>
	<skos:member rdf:resource="https://ark.frantiq.fr/ark:/26678/pcrtI4g8pXkSSJ"/>
	<skos:member rdf:resource="https://ark.frantiq.fr/ark:/26678/pcrtTbldUhfb1h"/>
	<skos:member rdf:resource="https://ark.frantiq.fr/ark:/26678/pcrtmmQBSGulBN"/>
	<skos:member rdf:resource="https://ark.frantiq.fr/ark:/26678/pcrtgx1nQuifPW"/>
	<skos:member rdf:resource="https://ark.frantiq.fr/ark:/26678/pcrt6z097U6IUf"/>
	<skos:member rdf:resource="https://ark.frantiq.fr/ark:/26678/pcrtjzKlry0LZi"/>
	<skos:member rdf:resource="https://ark.frantiq.fr/ark:/26678/pcrtalmpL9IBGx"/>
	<skos:member rdf:resource="https://ark.frantiq.fr/ark:/26678/pcrtc1Ueky7Zpg"/>
	<skos:member rdf:resource="https://ark.frantiq.fr/ark:/26678/pcrtOBWTai2Xms"/>
	<skos:member rdf:resource="https://ark.frantiq.fr/ark:/26678/pcrtaJLEkei5LQ"/>
	<skos:member rdf:resource="https://ark.frantiq.fr/ark:/26678/pcrtERMm8Q0wYw"/>
	<skos:member rdf:resource="https://ark.frantiq.fr/ark:/26678/pcrtaOHvUS4rT6"/>
	<skos:member rdf:resource="https://ark.frantiq.fr/ark:/26678/pcrtbTb5hPcQEn"/>
	<skos:member rdf:resource="https://ark.frantiq.fr/ark:/26678/pcrtO40ZLI4giK"/>
	<skos:member rdf:resource="https://ark.frantiq.fr/ark:/26678/pcrtUTZqItd8SL"/>
	<skos:member rdf:resource="https://ark.frantiq.fr/ark:/26678/pcrtGg8L8TLNtc"/>
	<skos:member rdf:resource="https://ark.frantiq.fr/ark:/26678/pcrtQuZiT5nYY2"/>
	<skos:member rdf:resource="https://ark.frantiq.fr/ark:/26678/pcrtknhh7n1sa3"/>
	<skos:member rdf:resource="https://ark.frantiq.fr/ark:/26678/pcrtVtHSyKSdbh"/>
	<skos:member rdf:resource="https://ark.frantiq.fr/ark:/26678/pcrtU6YoUalie6"/>
	<skos:member rdf:resource="https://ark.frantiq.fr/ark:/26678/pcrtLpvrsa9RIz"/>
	<skos:member rdf:resource="https://ark.frantiq.fr/ark:/26678/pcrtKvRuuvDNp2"/>
	<skos:member rdf:resource="https://ark.frantiq.fr/ark:/26678/pcrtn5zR6bBN39"/>
	<skos:member rdf:resource="https://ark.frantiq.fr/ark:/26678/pcrt16pnvNar4g"/>
	<skos:member rdf:resource="https://ark.frantiq.fr/ark:/26678/pcrt1DMOWvDF4j"/>
	<skos:member rdf:resource="https://ark.frantiq.fr/ark:/26678/pcrtho8l95no0j"/>
	<skos:member rdf:resource="https://ark.frantiq.fr/ark:/26678/pcrtcTqKm5ufUF"/>
	<skos:member rdf:resource="https://ark.frantiq.fr/ark:/26678/pcrtIxUJc35jSS"/>
	<skos:member rdf:resource="https://ark.frantiq.fr/ark:/26678/pcrtuxpF5YgM3S"/>
	<skos:member rdf:resource="https://ark.frantiq.fr/ark:/26678/pcrtWANqEEARhN"/>
	<skos:member rdf:resource="https://ark.frantiq.fr/ark:/26678/pcrtJYawSTtElG"/>
	<skos:member rdf:resource="https://ark.frantiq.fr/ark:/26678/pcrto2Udjh8XSP"/>
	<skos:member rdf:resource="https://ark.frantiq.fr/ark:/26678/pcrtXgoFDoG7xA"/>
	<skos:member rdf:resource="https://ark.frantiq.fr/ark:/26678/pcrtZFMkWp7vRA"/>
	<skos:member rdf:resource="https://ark.frantiq.fr/ark:/26678/pcrtqHWkorsw9D"/>
	<skos:member rdf:resource="https://ark.frantiq.fr/ark:/26678/pcrtJWWucnutA0"/>
	<skos:member rdf:resource="https://ark.frantiq.fr/ark:/26678/pcrtTcvLDTNT86"/>
	<skos:member rdf:resource="https://ark.frantiq.fr/ark:/26678/pcrtVWVfmfl1T2"/>
	<skos:member rdf:resource="https://ark.frantiq.fr/ark:/26678/pcrtTgttY2SfBr"/>
	<skos:member rdf:resource="https://ark.frantiq.fr/ark:/26678/pcrtDISmiAdvys"/>
	<skos:member rdf:resource="https://ark.frantiq.fr/ark:/26678/pcrth6l0mevtSJ"/>
	<skos:member rdf:resource="https://ark.frantiq.fr/ark:/26678/pcrt8yYh5xgMeO"/>
	<skos:member rdf:resource="https://ark.frantiq.fr/ark:/26678/pcrtikYi5ORdK4"/>
	<skos:member rdf:resource="https://ark.frantiq.fr/ark:/26678/pcrt3pmFUqt27w"/>
	<skos:member rdf:resource="https://ark.frantiq.fr/ark:/26678/pcrtDnenSUMjFl"/>
	<skos:member rdf:resource="https://ark.frantiq.fr/ark:/26678/pcrtVLPx3sY5Ku"/>
	<skos:member rdf:resource="https://ark.frantiq.fr/ark:/26678/pcrtR1s94Zuaul"/>
	<skos:member rdf:resource="https://ark.frantiq.fr/ark:/26678/pcrttcRKMp4QdV"/>
	<skos:member rdf:resource="https://ark.frantiq.fr/ark:/26678/pcrtkdetSDq0bj"/>
	<skos:member rdf:resource="https://ark.frantiq.fr/ark:/26678/pcrtm6uoPROlPN"/>
	<skos:member rdf:resource="https://ark.frantiq.fr/ark:/26678/pcrt52tibSvTjT"/>
	<skos:member rdf:resource="https://ark.frantiq.fr/ark:/26678/pcrtJt3ZKiNEFK"/>
	<skos:member rdf:resource="https://ark.frantiq.fr/ark:/26678/pcrtDoEeaZ6VcU"/>
	<skos:member rdf:resource="https://ark.frantiq.fr/ark:/26678/pcrtKiepgzdXSQ"/>
	<skos:member rdf:resource="https://ark.frantiq.fr/ark:/26678/pcrtp5MND6qfnb"/>
	<skos:member rdf:resource="https://ark.frantiq.fr/ark:/26678/pcrtsEgKPlBjWE"/>
	<skos:member rdf:resource="https://ark.frantiq.fr/ark:/26678/pcrttvE2YZwZu6"/>
	<skos:member rdf:resource="https://ark.frantiq.fr/ark:/26678/pcrttEcSiJ6kNe"/>
	<skos:member rdf:resource="https://ark.frantiq.fr/ark:/26678/pcrtuFMPNUEKWb"/>
	<skos:member rdf:resource="https://ark.frantiq.fr/ark:/26678/pcrt1zVFrqhSh2"/>
	<skos:member rdf:resource="https://ark.frantiq.fr/ark:/26678/pcrt7pgeXjaSI8"/>
	<skos:member rdf:resource="https://ark.frantiq.fr/ark:/26678/pcrtDfHvvnBWz7"/>
	<skos:member rdf:resource="https://ark.frantiq.fr/ark:/26678/pcrtlSaqkoJ8gu"/>
	<skos:member rdf:resource="https://ark.frantiq.fr/ark:/26678/pcrtFUux6JWTnV"/>
	<skos:member rdf:resource="https://ark.frantiq.fr/ark:/26678/pcrt9rIFPQ997Q"/>
	<skos:member rdf:resource="https://ark.frantiq.fr/ark:/26678/pcrt2vlSZd64Zk"/>
	<skos:member rdf:resource="https://ark.frantiq.fr/ark:/26678/pcrtSIsVZPQG1t"/>
	<skos:member rdf:resource="https://ark.frantiq.fr/ark:/26678/pcrtQe4n9vGjl0"/>
	<skos:member rdf:resource="https://ark.frantiq.fr/ark:/26678/pcrtevBDzau7qe"/>
	<skos:member rdf:resource="https://ark.frantiq.fr/ark:/26678/pcrt1pRQD1Ircr"/>
	<skos:member rdf:resource="https://ark.frantiq.fr/ark:/26678/pcrtEstKLNLE1q"/>
	<skos:member rdf:resource="https://ark.frantiq.fr/ark:/26678/crtSPE6Lx4cPI"/>
	<skos:member rdf:resource="https://ark.frantiq.fr/ark:/26678/pcrtSkipOsBGML"/>
	<skos:member rdf:resource="https://ark.frantiq.fr/ark:/26678/pcrtFxTmoqh7a3"/>
	<skos:member rdf:resource="https://ark.frantiq.fr/ark:/26678/crtHmI38AHBYS"/>
	<skos:member rdf:resource="https://ark.frantiq.fr/ark:/26678/pcrtwvFLgSQRs5"/>
	<skos:member rdf:resource="https://ark.frantiq.fr/ark:/26678/pcrtIMsuG0RWTs"/>
	<skos:member rdf:resource="https://ark.frantiq.fr/ark:/26678/pcrtyx3UIr91zi"/>
	<skos:member rdf:resource="https://ark.frantiq.fr/ark:/26678/pcrtsPauzzRS5z"/>
	<skos:member rdf:resource="https://ark.frantiq.fr/ark:/26678/pcrt5bIL1UtwcT"/>
	<skos:member rdf:resource="https://ark.frantiq.fr/ark:/26678/pcrtEWWJvOVoh5"/>
	<skos:member rdf:resource="https://ark.frantiq.fr/ark:/26678/pcrtkn1hAXHveS"/>
	<skos:member rdf:resource="https://ark.frantiq.fr/ark:/26678/pcrtgefwJa13yZ"/>
	<skos:member rdf:resource="https://ark.frantiq.fr/ark:/26678/pcrttnySGIGsj6"/>
	<skos:member rdf:resource="https://ark.frantiq.fr/ark:/26678/pcrtiaewgLXnZc"/>
	<skos:member rdf:resource="https://ark.frantiq.fr/ark:/26678/pcrtbZkzVXTkJI"/>
	<skos:member rdf:resource="https://ark.frantiq.fr/ark:/26678/pcrtjyrVAHv1m8"/>
	<skos:member rdf:resource="https://ark.frantiq.fr/ark:/26678/pcrt0zhHI6jOVx"/>
	<skos:member rdf:resource="https://ark.frantiq.fr/ark:/26678/pcrtuihSl3eSnW"/>
	<skos:member rdf:resource="https://ark.frantiq.fr/ark:/26678/pcrt448yYmVDuT"/>
	<skos:member rdf:resource="https://ark.frantiq.fr/ark:/26678/pcrtDr6Oi6lHM6"/>
	<skos:member rdf:resource="https://ark.frantiq.fr/ark:/26678/pcrtMt1immB5H5"/>
	<skos:member rdf:resource="https://ark.frantiq.fr/ark:/26678/pcrtOM6tMh4qpF"/>
	<skos:member rdf:resource="https://ark.frantiq.fr/ark:/26678/pcrtnlpDSw0du4"/>
	<skos:member rdf:resource="https://ark.frantiq.fr/ark:/26678/pcrtzVuPZeWdAP"/>
	<skos:member rdf:resource="https://ark.frantiq.fr/ark:/26678/pcrtGzQPnntJa1"/>
	<skos:member rdf:resource="https://ark.frantiq.fr/ark:/26678/pcrtlZ7VYeGKO3"/>
	<skos:member rdf:resource="https://ark.frantiq.fr/ark:/26678/pcrtbLhpWhz8H6"/>
	<skos:member rdf:resource="https://ark.frantiq.fr/ark:/26678/pcrtEpGlZykUTy"/>
	<skos:member rdf:resource="https://ark.frantiq.fr/ark:/26678/pcrtxVPISFTEr6"/>
	<skos:member rdf:resource="https://ark.frantiq.fr/ark:/26678/pcrtkbJMkYrMF6"/>
	<skos:member rdf:resource="https://ark.frantiq.fr/ark:/26678/pcrtDffxD420gS"/>
	<skos:member rdf:resource="https://ark.frantiq.fr/ark:/26678/pcrtZETJwE7RTQ"/>
	<skos:member rdf:resource="https://ark.frantiq.fr/ark:/26678/pcrtDwe0cp16nl"/>
	<skos:member rdf:resource="https://ark.frantiq.fr/ark:/26678/pcrtSVdwKcS3MI"/>
	<skos:member rdf:resource="https://ark.frantiq.fr/ark:/26678/pcrtxybfLE1dkn"/>
	<skos:member rdf:resource="https://ark.frantiq.fr/ark:/26678/pcrt4N9jrETRto"/>
	<skos:member rdf:resource="https://ark.frantiq.fr/ark:/26678/pcrtrxL50B7yNx"/>
	<skos:member rdf:resource="https://ark.frantiq.fr/ark:/26678/pcrt82lj1bBlxj"/>
	<skos:member rdf:resource="https://ark.frantiq.fr/ark:/26678/pcrtImRXTwOx0B"/>
	<skos:member rdf:resource="https://ark.frantiq.fr/ark:/26678/pcrthmVBQESXy2"/>
	<skos:member rdf:resource="https://ark.frantiq.fr/ark:/26678/pcrtT7b3IVuYxG"/>
	<skos:member rdf:resource="https://ark.frantiq.fr/ark:/26678/pcrtIzSUofuocv"/>
	<skos:member rdf:resource="https://ark.frantiq.fr/ark:/26678/pcrttxsm3xSsiz"/>
	<skos:member rdf:resource="https://ark.frantiq.fr/ark:/26678/pcrt6TSfpXkNW6"/>
	<skos:member rdf:resource="https://ark.frantiq.fr/ark:/26678/pcrtsIGcaQ8O7x"/>
	<skos:member rdf:resource="https://ark.frantiq.fr/ark:/26678/pcrt9SkpOgSbXw"/>
	<skos:member rdf:resource="https://ark.frantiq.fr/ark:/26678/pcrtnpv5KJIXTy"/>
	<skos:member rdf:resource="https://ark.frantiq.fr/ark:/26678/pcrt1wEGrR9DT3"/>
	<skos:member rdf:resource="https://ark.frantiq.fr/ark:/26678/pcrtfx4s0yvSLj"/>
	<skos:member rdf:resource="https://ark.frantiq.fr/ark:/26678/pcrthAOjGBEfZk"/>
	<skos:member rdf:resource="https://ark.frantiq.fr/ark:/26678/pcrtqGQOorLDxx"/>
	<skos:member rdf:resource="https://ark.frantiq.fr/ark:/26678/pcrtK8tO0rlQlM"/>
	<skos:member rdf:resource="https://ark.frantiq.fr/ark:/26678/pcrtv3md53Ugxj"/>
	<skos:member rdf:resource="https://ark.frantiq.fr/ark:/26678/pcrttS4bFv2ezb"/>
	<skos:member rdf:resource="https://ark.frantiq.fr/ark:/26678/pcrt065IhLltVk"/>
	<skos:member rdf:resource="https://ark.frantiq.fr/ark:/26678/pcrtJXS9PmPlFX"/>
	<skos:member rdf:resource="https://ark.frantiq.fr/ark:/26678/pcrt4GqimUgoOq"/>
	<skos:member rdf:resource="https://ark.frantiq.fr/ark:/26678/pcrtOPqdpwj043"/>
	<skos:member rdf:resource="https://ark.frantiq.fr/ark:/26678/pcrt3mTg9h3RFE"/>
	<skos:member rdf:resource="https://ark.frantiq.fr/ark:/26678/pcrtAhu8O29Xb2"/>
	<skos:member rdf:resource="https://ark.frantiq.fr/ark:/26678/pcrtAHm0qJl9tq"/>
	<skos:member rdf:resource="https://ark.frantiq.fr/ark:/26678/pcrt6d15xRmV8x"/>
	<skos:member rdf:resource="https://ark.frantiq.fr/ark:/26678/pcrtmbhTSRIoYb"/>
	<skos:member rdf:resource="https://ark.frantiq.fr/ark:/26678/pcrt0TJJTrHkN1"/>
	<skos:member rdf:resource="https://ark.frantiq.fr/ark:/26678/pcrtGpmPNJ0jRl"/>
	<skos:member rdf:resource="https://ark.frantiq.fr/ark:/26678/crtL2Kjt70xql"/>
	<skos:member rdf:resource="https://ark.frantiq.fr/ark:/26678/crtXiS7pEzMh1"/>
	<skos:member rdf:resource="https://ark.frantiq.fr/ark:/26678/crtnOhKKcaFEI"/>
	<skos:member rdf:resource="https://ark.frantiq.fr/ark:/26678/crt9EjSUc0WRF"/>
	<skos:member rdf:resource="https://ark.frantiq.fr/ark:/26678/crtAzyiJhxOQN"/>
	<skos:member rdf:resource="https://ark.frantiq.fr/ark:/26678/crtqg6iAF3rS7"/>
	<skos:member rdf:resource="https://ark.frantiq.fr/ark:/26678/crtXXzLndpZbJ"/>
	<skos:member rdf:resource="https://ark.frantiq.fr/ark:/26678/crtiorG06KeFt"/>
	<skos:member rdf:resource="https://ark.frantiq.fr/ark:/26678/pcrtPEGVkSl8Hk"/>
	<skos:member rdf:resource="https://ark.frantiq.fr/ark:/26678/pcrtLgpv98vu4P"/>
	<skos:member rdf:resource="https://ark.frantiq.fr/ark:/26678/pcrtPLs10mF9zI"/>
	<skos:member rdf:resource="https://ark.frantiq.fr/ark:/26678/pcrtp45jEJloXR"/>
	<skos:member rdf:resource="https://ark.frantiq.fr/ark:/26678/crtG26Pkhb07S"/>
	<skos:member rdf:resource="https://ark.frantiq.fr/ark:/26678/pcrtaUOSeoPg5g"/>
	<skos:member rdf:resource="https://ark.frantiq.fr/ark:/26678/pcrtK43haeM3e3"/>
	<skos:member rdf:resource="https://ark.frantiq.fr/ark:/26678/pcrty2mcsksa6s"/>
	<skos:member rdf:resource="https://ark.frantiq.fr/ark:/26678/pcrtj3ZcwkArSR"/>
	<skos:member rdf:resource="https://ark.frantiq.fr/ark:/26678/pcrtDhZmKFAlZa"/>
	<skos:member rdf:resource="https://ark.frantiq.fr/ark:/26678/pcrtQAl1Zjr5KF"/>
	<skos:member rdf:resource="https://ark.frantiq.fr/ark:/26678/pcrt3PUAhlWubZ"/>
	<skos:member rdf:resource="https://ark.frantiq.fr/ark:/26678/pcrtX9DGL4v9Ko"/>
	<skos:member rdf:resource="https://ark.frantiq.fr/ark:/26678/pcrt6BEybyEAjN"/>
	<skos:member rdf:resource="https://ark.frantiq.fr/ark:/26678/pcrtmxvuuXHSTS"/>
	<skos:member rdf:resource="https://ark.frantiq.fr/ark:/26678/pcrtt7G9pnQlu1"/>
	<skos:member rdf:resource="https://ark.frantiq.fr/ark:/26678/pcrtQqTsG6TEFy"/>
	<skos:member rdf:resource="https://ark.frantiq.fr/ark:/26678/pcrt9JSk28suqb"/>
	<skos:member rdf:resource="https://ark.frantiq.fr/ark:/26678/pcrtc6RmFQxFuS"/>
	<skos:member rdf:resource="https://ark.frantiq.fr/ark:/26678/pcrtolrabjfp2T"/>
	<skos:member rdf:resource="https://ark.frantiq.fr/ark:/26678/pcrtOJj49Pe6Vb"/>
	<skos:member rdf:resource="https://ark.frantiq.fr/ark:/26678/pcrtRT5qpNmDqE"/>
	<skos:member rdf:resource="https://ark.frantiq.fr/ark:/26678/pcrt2nbSAPPSwB"/>
	<skos:member rdf:resource="https://ark.frantiq.fr/ark:/26678/pcrtF8Wf7AekK2"/>
	<skos:member rdf:resource="https://ark.frantiq.fr/ark:/26678/pcrtc2SkvG29we"/>
	<skos:member rdf:resource="https://ark.frantiq.fr/ark:/26678/pcrtkgSlgXZbNa"/>
	<skos:member rdf:resource="https://ark.frantiq.fr/ark:/26678/pcrtEU8K1oF2Eh"/>
	<skos:member rdf:resource="https://ark.frantiq.fr/ark:/26678/pcrth18FOY3yYX"/>
	<skos:member rdf:resource="https://ark.frantiq.fr/ark:/26678/pcrtgg4KWVZk74"/>
	<skos:member rdf:resource="https://ark.frantiq.fr/ark:/26678/pcrt4Jy2JE8F3U"/>
	<skos:member rdf:resource="https://ark.frantiq.fr/ark:/26678/crtSfObTEvbdn"/>
	<skos:member rdf:resource="https://ark.frantiq.fr/ark:/26678/pcrtHJ3vzShqFy"/>
	<skos:member rdf:resource="https://ark.frantiq.fr/ark:/26678/pcrtmxoAFl0eWR"/>
	<skos:member rdf:resource="https://ark.frantiq.fr/ark:/26678/pcrtRiKgPqvJQO"/>
	<skos:member rdf:resource="https://ark.frantiq.fr/ark:/26678/pcrt0gJ3NT8WlW"/>
	<skos:member rdf:resource="https://ark.frantiq.fr/ark:/26678/pcrte3NbmKEKON"/>
	<skos:member rdf:resource="https://ark.frantiq.fr/ark:/26678/pcrt4KRB12RYGv"/>
	<skos:member rdf:resource="https://ark.frantiq.fr/ark:/26678/pcrtnR5ePytFhO"/>
	<skos:member rdf:resource="https://ark.frantiq.fr/ark:/26678/pcrteWLSy9aARp"/>
	<skos:member rdf:resource="https://ark.frantiq.fr/ark:/26678/pcrtSpItdjR86k"/>
	<skos:member rdf:resource="https://ark.frantiq.fr/ark:/26678/pcrtQhjRUa1GV8"/>
	<skos:member rdf:resource="https://ark.frantiq.fr/ark:/26678/pcrt4nvgWBQ59k"/>
	<skos:member rdf:resource="https://ark.frantiq.fr/ark:/26678/pcrtGAARv5y4t4"/>
	<skos:member rdf:resource="https://ark.frantiq.fr/ark:/26678/pcrt4dfh8e5Dpz"/>
	<skos:member rdf:resource="https://ark.frantiq.fr/ark:/26678/pcrtnHxyjOkhJw"/>
	<skos:member rdf:resource="https://ark.frantiq.fr/ark:/26678/pcrt8ZW1DEoUSn"/>
	<skos:member rdf:resource="https://ark.frantiq.fr/ark:/26678/pcrtGET4B08135"/>
	<skos:member rdf:resource="https://ark.frantiq.fr/ark:/26678/pcrtakOKgw0Q9M"/>
	<skos:member rdf:resource="https://ark.frantiq.fr/ark:/26678/pcrt30jDOWeS57"/>
	<skos:member rdf:resource="https://ark.frantiq.fr/ark:/26678/pcrtIDUn8EY3Bx"/>
	<skos:member rdf:resource="https://ark.frantiq.fr/ark:/26678/pcrtMBkRt9d0we"/>
	<skos:member rdf:resource="https://ark.frantiq.fr/ark:/26678/pcrtQ3dQ0kEMW9"/>
	<skos:member rdf:resource="https://ark.frantiq.fr/ark:/26678/pcrtvMpoEaUF3q"/>
	<skos:member rdf:resource="https://ark.frantiq.fr/ark:/26678/pcrtjGSMcDpz8A"/>
	<skos:member rdf:resource="https://ark.frantiq.fr/ark:/26678/pcrtahNd1oALhh"/>
	<skos:member rdf:resource="https://ark.frantiq.fr/ark:/26678/pcrtSd50sRXgiH"/>
	<skos:member rdf:resource="https://ark.frantiq.fr/ark:/26678/pcrtFEZaa6oTIS"/>
	<skos:member rdf:resource="https://ark.frantiq.fr/ark:/26678/pcrtaSs5GKhSA7"/>
	<skos:member rdf:resource="https://ark.frantiq.fr/ark:/26678/pcrtzJhR1OwU8P"/>
	<skos:member rdf:resource="https://ark.frantiq.fr/ark:/26678/pcrthKDSnMjAR9"/>
	<skos:member rdf:resource="https://ark.frantiq.fr/ark:/26678/pcrthu1vFbVQHO"/>
	<skos:member rdf:resource="https://ark.frantiq.fr/ark:/26678/pcrtgym8WF8J02"/>
	<skos:member rdf:resource="https://ark.frantiq.fr/ark:/26678/pcrtvmZ325vcRc"/>
	<skos:member rdf:resource="https://ark.frantiq.fr/ark:/26678/pcrtPkEBaAzwGn"/>
	<skos:member rdf:resource="https://ark.frantiq.fr/ark:/26678/pcrtMStphi4T4j"/>
	<skos:member rdf:resource="https://ark.frantiq.fr/ark:/26678/pcrttQ1swNeBVe"/>
	<skos:member rdf:resource="https://ark.frantiq.fr/ark:/26678/pcrtMj9v33qudS"/>
	<skos:member rdf:resource="https://ark.frantiq.fr/ark:/26678/pcrtbKNE16SNWh"/>
	<skos:member rdf:resource="https://ark.frantiq.fr/ark:/26678/pcrtcyhN8uK1oY"/>
	<skos:member rdf:resource="https://ark.frantiq.fr/ark:/26678/pcrtZWUH1HnqXo"/>
	<skos:member rdf:resource="https://ark.frantiq.fr/ark:/26678/pcrtM0mkbZiNnN"/>
	<skos:member rdf:resource="https://ark.frantiq.fr/ark:/26678/pcrt6BaMGq7zE1"/>
	<skos:member rdf:resource="https://ark.frantiq.fr/ark:/26678/pcrtmoM3SzhDcB"/>
	<skos:member rdf:resource="https://ark.frantiq.fr/ark:/26678/pcrt2xkdh2n373"/>
	<skos:member rdf:resource="https://ark.frantiq.fr/ark:/26678/pcrt6v8xrc8qrd"/>
	<skos:member rdf:resource="https://ark.frantiq.fr/ark:/26678/pcrtg0xc91xffk"/>
	<skos:member rdf:resource="https://ark.frantiq.fr/ark:/26678/pcrtzOFeK4FZEf"/>
	<skos:member rdf:resource="https://ark.frantiq.fr/ark:/26678/pcrtr5vk7w9vdz"/>
	<skos:member rdf:resource="https://ark.frantiq.fr/ark:/26678/pcrtfkw4vc3pc5"/>
	<skos:member rdf:resource="https://ark.frantiq.fr/ark:/26678/pcrt5cdhzck93d"/>
	<skos:member rdf:resource="https://ark.frantiq.fr/ark:/26678/pcrtz14gcmpgjh"/>
	<skos:member rdf:resource="https://ark.frantiq.fr/ark:/26678/pcrt218fx7941b"/>
	<skos:member rdf:resource="https://ark.frantiq.fr/ark:/26678/pcrtvn284hkmw0"/>
	<skos:member rdf:resource="https://ark.frantiq.fr/ark:/26678/pcrtb1vvxk8fp3"/>
	<skos:member rdf:resource="https://ark.frantiq.fr/ark:/26678/pcrt73gjdrz4rx"/>
	<skos:member rdf:resource="https://ark.frantiq.fr/ark:/26678/pcrtbbqj7zgqnn"/>
	<skos:member rdf:resource="https://ark.frantiq.fr/ark:/26678/pcrt518w0nr5tf"/>
	<skos:member rdf:resource="https://ark.frantiq.fr/ark:/26678/pcrtrdsp44jvsk0qqqkndb9g"/>
	<skos:member rdf:resource="https://ark.frantiq.fr/ark:/26678/pcrt0k0f3qbw4r"/>
	<skos:member rdf:resource="https://ark.frantiq.fr/ark:/26678/pcrtsxjtz27508"/>
	<skos:member rdf:resource="https://ark.frantiq.fr/ark:/26678/pcrtbhbct8gbhn"/>
	<skos:member rdf:resource="https://ark.frantiq.fr/ark:/26678/pcrtkf9tnv3kc1"/>
	<skos:member rdf:resource="https://ark.frantiq.fr/ark:/26678/pcrtw8nqd0wpmc"/>
	<skos:member rdf:resource="https://ark.frantiq.fr/ark:/26678/pcrtv3pfn44gc4"/>
	<skos:member rdf:resource="https://ark.frantiq.fr/ark:/26678/pcrtvm1c7n58sx"/>
	<skos:member rdf:resource="https://ark.frantiq.fr/ark:/26678/pcrtk3njjx5659"/>
	<skos:member rdf:resource="https://ark.frantiq.fr/ark:/26678/pcrt33sf88d6jh"/>
	<skos:member rdf:resource="https://ark.frantiq.fr/ark:/26678/pcrtckknjb3bj0"/>
	<skos:member rdf:resource="https://ark.frantiq.fr/ark:/26678/pcrthqg1d2ks27"/>
	<skos:member rdf:resource="https://ark.frantiq.fr/ark:/26678/pcrtbpgr0h35bn"/>
	<skos:member rdf:resource="https://ark.frantiq.fr/ark:/26678/pcrtn97gqkmvfx"/>
	<skos:member rdf:resource="https://ark.frantiq.fr/ark:/26678/pcrt58n6q7897s"/>
	<skos:member rdf:resource="https://ark.frantiq.fr/ark:/26678/pcrtrmhr3gdwhf"/>
	<skos:member rdf:resource="https://ark.frantiq.fr/ark:/26678/pcrtp8m4m99q9m"/>
	<skos:member rdf:resource="https://ark.frantiq.fr/ark:/26678/pcrt5fm9qtbrwv"/>
	<skos:member rdf:resource="https://ark.frantiq.fr/ark:/26678/pcrtf4mt37h0q8"/>
	<skos:member rdf:resource="https://ark.frantiq.fr/ark:/26678/pcrt6867pw8dnx"/>
	<skos:member rdf:resource="https://ark.frantiq.fr/ark:/26678/pcrtrsjrghq6f8"/>
	<skos:member rdf:resource="https://ark.frantiq.fr/ark:/26678/pcrtbn5hw6ktqk"/>
	<skos:member rdf:resource="https://ark.frantiq.fr/ark:/26678/pcrtcvphm3f016"/>
	<skos:member rdf:resource="https://ark.frantiq.fr/ark:/26678/pcrtrb58t07tzv"/>
	<skos:member rdf:resource="https://ark.frantiq.fr/ark:/26678/pcrt1z89xc4r6g"/>
	<skos:member rdf:resource="https://ark.frantiq.fr/ark:/26678/pcrt36f77fdd1n"/>
	<skos:member rdf:resource="https://ark.frantiq.fr/ark:/26678/pcrtk20v37cf0s"/>
	<skos:member rdf:resource="https://ark.frantiq.fr/ark:/26678/pcrtd94cn7xznh"/>
	<skos:member rdf:resource="https://ark.frantiq.fr/ark:/26678/pcrt094rdqsfbv"/>
	<skos:member rdf:resource="https://ark.frantiq.fr/ark:/26678/pcrt21v5j62zkd"/>
	<skos:member rdf:resource="https://ark.frantiq.fr/ark:/26678/pcrtj8kv2v5jz0"/>
	<skos:member rdf:resource="https://ark.frantiq.fr/ark:/26678/pcrtc64m697d3t"/>
	<skos:member rdf:resource="https://ark.frantiq.fr/ark:/26678/pcrt9s23ncq2q9"/>
	<skos:member rdf:resource="https://ark.frantiq.fr/ark:/26678/pcrt074z9q8ng3"/>
	<skos:member rdf:resource="https://ark.frantiq.fr/ark:/26678/pcrtkwk6bz94r3"/>
	<skos:member rdf:resource="https://ark.frantiq.fr/ark:/26678/pcrtqc4b4zzzmw"/>
	<skos:member rdf:resource="https://ark.frantiq.fr/ark:/26678/pcrt40qs0fvnxg"/>
	<skos:member rdf:resource="https://ark.frantiq.fr/ark:/26678/pcrtsvkcb5mv2t"/>
	<skos:member rdf:resource="https://ark.frantiq.fr/ark:/26678/pcrt5m5pftg21t"/>
	<skos:member rdf:resource="https://ark.frantiq.fr/ark:/26678/pcrt0kvts48fht"/>
	<skos:member rdf:resource="https://ark.frantiq.fr/ark:/26678/pcrt7fsrb8ggkp"/>
	<skos:member rdf:resource="https://ark.frantiq.fr/ark:/26678/pcrtx3bv9c7050"/>
	<skos:member rdf:resource="https://ark.frantiq.fr/ark:/26678/pcrtv0rphqt1h8"/>
	<skos:member rdf:resource="https://ark.frantiq.fr/ark:/26678/pcrtvh6k2wqhg6"/>
	<skos:member rdf:resource="https://ark.frantiq.fr/ark:/26678/pcrt969pbxxbzt"/>
	<skos:member rdf:resource="https://ark.frantiq.fr/ark:/26678/pcrt2kpf55zh14"/>
	<skos:member rdf:resource="https://ark.frantiq.fr/ark:/26678/pcrtndt9zrpjjk"/>
	<skos:member rdf:resource="https://ark.frantiq.fr/ark:/26678/pcrtfv2krrfh1d"/>
	<skos:member rdf:resource="https://ark.frantiq.fr/ark:/26678/pcrtknmwxc5x5s"/>
	<skos:member rdf:resource="https://ark.frantiq.fr/ark:/26678/pcrtrwdpzch5wh"/>
	<skos:member rdf:resource="https://ark.frantiq.fr/ark:/26678/pcrth30k691qrk"/>
	<skos:member rdf:resource="https://ark.frantiq.fr/ark:/26678/pcrtkgmbfz0x3s"/>
	<skos:member rdf:resource="https://ark.frantiq.fr/ark:/26678/pcrtkrm9q3htcj"/>
	<skos:member rdf:resource="https://ark.frantiq.fr/ark:/26678/pcrtq764j7snt5"/>
	<skos:member rdf:resource="https://ark.frantiq.fr/ark:/26678/pcrtfvk3mp3dhk"/>
	<skos:member rdf:resource="https://ark.frantiq.fr/ark:/26678/pcrt3tmh056368"/>
	<skos:member rdf:resource="https://ark.frantiq.fr/ark:/26678/pcrtfz97ktt9qf"/>
	<skos:member rdf:resource="https://ark.frantiq.fr/ark:/26678/pcrt5bd4f5dv7r"/>
	<skos:member rdf:resource="https://ark.frantiq.fr/ark:/26678/pcrt5ddg241ccv"/>
	<skos:member rdf:resource="https://ark.frantiq.fr/ark:/26678/pcrtjmqpnw74z9"/>
	<skos:member rdf:resource="https://ark.frantiq.fr/ark:/26678/pcrt6pvhc29pfv"/>
	<skos:member rdf:resource="https://ark.frantiq.fr/ark:/26678/pcrtk8c4vv2tw8"/>
	<skos:member rdf:resource="https://ark.frantiq.fr/ark:/26678/pcrt5nd65vnw7p"/>
	<skos:member rdf:resource="https://ark.frantiq.fr/ark:/26678/pcrt24wcqp2cfz"/>
	<skos:member rdf:resource="https://ark.frantiq.fr/ark:/26678/pcrt9qq3x37vt0"/>
	<skos:member rdf:resource="https://ark.frantiq.fr/ark:/26678/pcrtr06vz24nj3"/>
	<skos:member rdf:resource="https://ark.frantiq.fr/ark:/26678/pcrt2fhx0kftpg"/>
	<skos:member rdf:resource="https://ark.frantiq.fr/ark:/26678/pcrt1tm77xkqbd"/>
	<skos:member rdf:resource="https://ark.frantiq.fr/ark:/26678/pcrt6xvrhrkjz8"/>
	<skos:member rdf:resource="https://ark.frantiq.fr/ark:/26678/pcrtwz8jzr2ttd"/>
	<skos:member rdf:resource="https://ark.frantiq.fr/ark:/26678/pcrt4rsdrmfk1b"/>
	<skos:member rdf:resource="https://ark.frantiq.fr/ark:/26678/pcrtjwwb1xztxh"/>
	<skos:member rdf:resource="https://ark.frantiq.fr/ark:/26678/pcrt1kjsnnvmzh"/>
	<skos:member rdf:resource="https://ark.frantiq.fr/ark:/26678/pcrt21f986h3tk"/>
	<skos:member rdf:resource="https://ark.frantiq.fr/ark:/26678/pcrtqmm7q566vh"/>
	<skos:member rdf:resource="https://ark.frantiq.fr/ark:/26678/pcrtv3f379sr9v"/>
	<skos:member rdf:resource="https://ark.frantiq.fr/ark:/26678/pcrtb689mtdsz6"/>
	<skos:member rdf:resource="https://ark.frantiq.fr/ark:/26678/pcrt8c26426vth"/>
	<skos:member rdf:resource="https://ark.frantiq.fr/ark:/26678/pcrtjg8pxcjgdt"/>
	<skos:member rdf:resource="https://ark.frantiq.fr/ark:/26678/pcrt7qtb4j1twt"/>
	<skos:member rdf:resource="https://ark.frantiq.fr/ark:/26678/pcrtqjn0rqg305"/>
	<skos:member rdf:resource="https://ark.frantiq.fr/ark:/26678/pcrtjts6bfc4zq"/>
	<skos:member rdf:resource="https://ark.frantiq.fr/ark:/26678/pcrtzpd0t7gbgz"/>
	<skos:member rdf:resource="https://ark.frantiq.fr/ark:/26678/pcrtvq05vjv1z6"/>
	<skos:member rdf:resource="https://ark.frantiq.fr/ark:/26678/pcrt02hj78whx8"/>
	<skos:member rdf:resource="https://ark.frantiq.fr/ark:/26678/pcrt96jkm5cgpf"/>
	<skos:member rdf:resource="https://ark.frantiq.fr/ark:/26678/pcrt776pzvkdkn"/>
	<skos:member rdf:resource="https://ark.frantiq.fr/ark:/26678/pcrtv9c4m3q53k"/>
	<skos:member rdf:resource="https://ark.frantiq.fr/ark:/26678/pcrt4n7gjb1qfh"/>
	<skos:member rdf:resource="https://ark.frantiq.fr/ark:/26678/pcrttkxc1k68td"/>
	<skos:member rdf:resource="https://ark.frantiq.fr/ark:/26678/pcrt73m1tx29mm"/>
	<skos:member rdf:resource="https://ark.frantiq.fr/ark:/26678/pcrtpsrh8ptqjf"/>
	<skos:member rdf:resource="https://ark.frantiq.fr/ark:/26678/pcrtvq01hkvvn3"/>
	<skos:member rdf:resource="https://ark.frantiq.fr/ark:/26678/pcrt11wm5hjnm3"/>
	<skos:member rdf:resource="https://ark.frantiq.fr/ark:/26678/pcrt375srxkn5s"/>
	<skos:member rdf:resource="https://ark.frantiq.fr/ark:/26678/pcrtqh6z41brjd"/>
	<skos:member rdf:resource="https://ark.frantiq.fr/ark:/26678/pcrt1qsxtkgq0f"/>
	<skos:member rdf:resource="https://ark.frantiq.fr/ark:/26678/pcrtj6wgmdnp4k"/>
	<skos:member rdf:resource="https://ark.frantiq.fr/ark:/26678/pcrtq9kn0538k0"/>
	<skos:member rdf:resource="https://ark.frantiq.fr/ark:/26678/pcrtvd560z43dq"/>
	<skos:member rdf:resource="https://ark.frantiq.fr/ark:/26678/pcrt9bqtk5n9vs"/>
	<skos:member rdf:resource="https://ark.frantiq.fr/ark:/26678/pcrtc1qqps1k4g"/>
	<skos:member rdf:resource="https://ark.frantiq.fr/ark:/26678/pcrtcfbz4mzqtc"/>
	<skos:member rdf:resource="https://ark.frantiq.fr/ark:/26678/pcrtxt48rvckxp"/>
	<skos:member rdf:resource="https://ark.frantiq.fr/ark:/26678/pcrt1pj0md5g5q"/>
	<skos:member rdf:resource="https://ark.frantiq.fr/ark:/26678/pcrt78g8rrd958"/>
	<skos:member rdf:resource="https://ark.frantiq.fr/ark:/26678/pcrt12db2x701r"/>
	<skos:member rdf:resource="https://ark.frantiq.fr/ark:/26678/pcrtnc6zr3n8dr"/>
	<skos:member rdf:resource="https://ark.frantiq.fr/ark:/26678/pcrt277j912tkp"/>
	<skos:member rdf:resource="https://ark.frantiq.fr/ark:/26678/pcrtg4q8hhzgqb"/>
	<skos:member rdf:resource="https://ark.frantiq.fr/ark:/26678/pcrt558wf1f6dg"/>
	<skos:member rdf:resource="https://ark.frantiq.fr/ark:/26678/pcrt11g9hx0p5s"/>
	<skos:member rdf:resource="https://ark.frantiq.fr/ark:/26678/pcrtz6cz5t6ngd"/>
	<skos:member rdf:resource="https://ark.frantiq.fr/ark:/26678/pcrtdn47j0pbjt"/>
	<skos:member rdf:resource="https://ark.frantiq.fr/ark:/26678/pcrtmk1p11fm4k"/>
	<skos:member rdf:resource="https://ark.frantiq.fr/ark:/26678/pcrtq7hgb8vqh2"/>
	<skos:member rdf:resource="https://ark.frantiq.fr/ark:/26678/pcrtxrcv4dz28t"/>
	<skos:member rdf:resource="https://ark.frantiq.fr/ark:/26678/pcrtzwhr6nrsvxm73pzkq2dq"/>
	<skos:member rdf:resource="https://ark.frantiq.fr/ark:/26678/pcrtjbpmw8qvrn"/>
	<skos:member rdf:resource="https://ark.frantiq.fr/ark:/26678/pcrt0712c8ws62"/>
	<skos:member rdf:resource="https://ark.frantiq.fr/ark:/26678/pcrtxn3nfsg0pd"/>
	<skos:member rdf:resource="https://ark.frantiq.fr/ark:/26678/pcrt11zbr3964m"/>
	<skos:member rdf:resource="https://ark.frantiq.fr/ark:/26678/pcrtb8qzpwp7ck"/>
	<skos:member rdf:resource="https://ark.frantiq.fr/ark:/26678/pcrtspv238x81q"/>
	<skos:member rdf:resource="https://ark.frantiq.fr/ark:/26678/pcrtt42zqnhf10"/>
	<skos:member rdf:resource="https://ark.frantiq.fr/ark:/26678/pcrtx37ph91cww"/>
	<skos:member rdf:resource="https://ark.frantiq.fr/ark:/26678/pcrtszp2f0j63w"/>
	<skos:member rdf:resource="https://ark.frantiq.fr/ark:/26678/pcrtdpxq48r9pj"/>
	<skos:member rdf:resource="https://ark.frantiq.fr/ark:/26678/pcrt9bvd56q20k"/>
	<skos:member rdf:resource="https://ark.frantiq.fr/ark:/26678/pcrtcxvd08cn0d"/>
	<skos:member rdf:resource="https://ark.frantiq.fr/ark:/26678/pcrtm3j41zv11k"/>
	<skos:member rdf:resource="https://ark.frantiq.fr/ark:/26678/pcrtf80pqj28pw"/>
	<skos:member rdf:resource="https://ark.frantiq.fr/ark:/26678/pcrt38v8df6d4c"/>
	<skos:member rdf:resource="https://ark.frantiq.fr/ark:/26678/pcrtv4jtvchmgm"/>
	<skos:member rdf:resource="https://ark.frantiq.fr/ark:/26678/pcrtqnzx9qwkt5"/>
	<skos:member rdf:resource="https://ark.frantiq.fr/ark:/26678/pcrtk5md9510q7"/>
	<skos:member rdf:resource="https://ark.frantiq.fr/ark:/26678/pcrtgb1xs84qs8"/>
	<skos:member rdf:resource="https://ark.frantiq.fr/ark:/26678/pcrtfpt7p2xkdf"/>
	<skos:member rdf:resource="https://ark.frantiq.fr/ark:/26678/pcrt01dd8jnk9r"/>
	<skos:member rdf:resource="https://ark.frantiq.fr/ark:/26678/pcrtbrv3wp92hn"/>
	<skos:member rdf:resource="https://ark.frantiq.fr/ark:/26678/pcrtpp27tm32r2"/>
	<skos:member rdf:resource="https://ark.frantiq.fr/ark:/26678/pcrttr8kcz7mgd"/>
	<skos:member rdf:resource="https://ark.frantiq.fr/ark:/26678/pcrtjrbdhj75z0"/>
	<skos:member rdf:resource="https://ark.frantiq.fr/ark:/26678/pcrtcb7qm82cts"/>
	<skos:member rdf:resource="https://ark.frantiq.fr/ark:/26678/pcrtc02b47wn5t"/>
	<skos:member rdf:resource="https://ark.frantiq.fr/ark:/26678/pcrtt9jqbj1ghk"/>
	<skos:member rdf:resource="https://ark.frantiq.fr/ark:/26678/pcrtm4r7mvsvrw"/>
	<skos:member rdf:resource="https://ark.frantiq.fr/ark:/26678/pcrt45bjq160pt"/>
	<skos:member rdf:resource="https://ark.frantiq.fr/ark:/26678/pcrttmkgbwr8c7"/>
	<skos:member rdf:resource="https://ark.frantiq.fr/ark:/26678/pcrtqh9bhz6xcr"/>
	<skos:member rdf:resource="https://ark.frantiq.fr/ark:/26678/pcrtsrWeYcRkNg"/>
	<skos:member rdf:resource="https://ark.frantiq.fr/ark:/26678/pcrtStScmr2cmH"/>
	<skos:member rdf:resource="https://ark.frantiq.fr/ark:/26678/pcrt1asKmbn9q8"/>
	<skos:member rdf:resource="https://ark.frantiq.fr/ark:/26678/pcrtbnBhdnlQrL"/>
	<skos:member rdf:resource="https://ark.frantiq.fr/ark:/26678/pcrtAoNmnP9BYF"/>
	<skos:member rdf:resource="https://ark.frantiq.fr/ark:/26678/pcrt1jTyJEx22Y"/>
	<skos:member rdf:resource="https://ark.frantiq.fr/ark:/26678/pcrtOF9oqZo0Pd"/>
	<skos:member rdf:resource="https://ark.frantiq.fr/ark:/26678/pcrtslVSzVnfeg"/>
	<skos:member rdf:resource="https://ark.frantiq.fr/ark:/26678/pcrtV3BZNic1DR"/>
	<skos:member rdf:resource="https://ark.frantiq.fr/ark:/26678/pcrtAWl3eAUQlA"/>
	<skos:member rdf:resource="https://ark.frantiq.fr/ark:/26678/pcrtvKH7mF2Oas"/>
	<skos:member rdf:resource="https://ark.frantiq.fr/ark:/26678/pcrtFpNU7SZgo7"/>
	<skos:member rdf:resource="https://ark.frantiq.fr/ark:/26678/pcrtKcuT7Kh6vX"/>
	<skos:member rdf:resource="https://ark.frantiq.fr/ark:/26678/pcrtW8Uu5SMsQy"/>
	<skos:member rdf:resource="https://ark.frantiq.fr/ark:/26678/pcrtf97bQHDGEd"/>
	<skos:member rdf:resource="https://ark.frantiq.fr/ark:/26678/pcrtXVZBob53by"/>
	<skos:member rdf:resource="https://ark.frantiq.fr/ark:/26678/pcrtfx2fwztQ8p"/>
	<skos:member rdf:resource="https://ark.frantiq.fr/ark:/26678/pcrtSdKu9rjDHO"/>
	<skos:member rdf:resource="https://ark.frantiq.fr/ark:/26678/pcrtd1cZp0yBER"/>
	<skos:member rdf:resource="https://ark.frantiq.fr/ark:/26678/pcrt0HFzFNNK1N"/>
	<skos:member rdf:resource="https://ark.frantiq.fr/ark:/26678/pcrtxGxOl1KuZz"/>
	<skos:member rdf:resource="https://ark.frantiq.fr/ark:/26678/pcrt5A1NAN3NE3"/>
	<skos:member rdf:resource="https://ark.frantiq.fr/ark:/26678/pcrtgkVy7lK4lN"/>
	<skos:member rdf:resource="https://ark.frantiq.fr/ark:/26678/pcrt8brfm4pd4t"/>
	<skos:member rdf:resource="https://ark.frantiq.fr/ark:/26678/pcrtjs2wjn65hq"/>
	<skos:member rdf:resource="https://ark.frantiq.fr/ark:/26678/pcrtqvm3ztp4h8"/>
	<skos:member rdf:resource="https://ark.frantiq.fr/ark:/26678/pcrt9c0c2gpn8g"/>
	<skos:member rdf:resource="https://ark.frantiq.fr/ark:/26678/pcrtzzdfgbqjgxghdgkrghbq"/>
	<skos:member rdf:resource="https://ark.frantiq.fr/ark:/26678/pcrt3344f5f89w8bjkpfp2zz"/>
	<skos:member rdf:resource="https://ark.frantiq.fr/ark:/26678/pcrtSHAq8xiG3F"/>
	<skos:member rdf:resource="https://ark.frantiq.fr/ark:/26678/pcrtwWYB6o5QwM"/>
	<skos:member rdf:resource="https://ark.frantiq.fr/ark:/26678/pcrtp201sc1d5bd93jj7mm27"/>
	<skos:member rdf:resource="https://ark.frantiq.fr/ark:/26678/pcrtbxntxs7hfz99qvswk8k1"/>
	<skos:member rdf:resource="https://ark.frantiq.fr/ark:/26678/pcrtsr9r0hqdgqcdmw5mds91"/>
	<skos:member rdf:resource="https://ark.frantiq.fr/ark:/26678/pcrtvhmknj8n0n92z5x2xqqk"/>
	<skos:member rdf:resource="https://ark.frantiq.fr/ark:/26678/pcrttk3hqkx8s7049j925sxn"/>
	<skos:member rdf:resource="https://ark.frantiq.fr/ark:/26678/pcrtb4mt1w9s876tsx2cxf61"/>
	<skos:member rdf:resource="https://ark.frantiq.fr/ark:/26678/pcrtB8FNASjQrB"/>
	<skos:member rdf:resource="https://ark.frantiq.fr/ark:/26678/pcrtskMRAe4usI"/>
	<skos:member rdf:resource="https://ark.frantiq.fr/ark:/26678/pcrtpNOweZVSSH"/>
	<skos:member rdf:resource="https://ark.frantiq.fr/ark:/26678/pcrtp0jS51rXL1"/>
	<skos:member rdf:resource="https://ark.frantiq.fr/ark:/26678/pcrtsTcJvHR17f"/>
	<skos:member rdf:resource="https://ark.frantiq.fr/ark:/26678/pcrtjzpz0bA7Mx"/>
	<skos:member rdf:resource="https://ark.frantiq.fr/ark:/26678/pcrtL9hSYO73pS"/>
	<skos:member rdf:resource="https://ark.frantiq.fr/ark:/26678/pcrt5SnWt4iSF2"/>
	<skos:member rdf:resource="https://ark.frantiq.fr/ark:/26678/pcrt2ozTOWS5f0"/>
	<skos:member rdf:resource="https://ark.frantiq.fr/ark:/26678/pcrt9lQWQXyMXK"/>
	<skos:member rdf:resource="https://ark.frantiq.fr/ark:/26678/pcrtIq9NE61BMc"/>
	<skos:member rdf:resource="https://ark.frantiq.fr/ark:/26678/pcrtKASHLmba7X"/>
	<skos:member rdf:resource="https://ark.frantiq.fr/ark:/26678/pcrt7kSfnJElvj"/>
	<skos:member rdf:resource="https://ark.frantiq.fr/ark:/26678/pcrtjSXU4udrfP"/>
	<skos:member rdf:resource="https://ark.frantiq.fr/ark:/26678/pcrterNa8OcooH"/>
	<skos:member rdf:resource="https://ark.frantiq.fr/ark:/26678/pcrtbRoB6J1AY7"/>
	<skos:member rdf:resource="https://ark.frantiq.fr/ark:/26678/pcrtZ6enHsm9bu"/>
	<skos:member rdf:resource="https://ark.frantiq.fr/ark:/26678/pcrttAmNtvNqnf"/>
	<skos:member rdf:resource="https://ark.frantiq.fr/ark:/26678/pcrtu714SnuAFj"/>
	<skos:member rdf:resource="https://ark.frantiq.fr/ark:/26678/pcrtupN3PAxWw0"/>
	<skos:member rdf:resource="https://ark.frantiq.fr/ark:/26678/pcrtK2sVvLapYR"/>
	<skos:member rdf:resource="https://ark.frantiq.fr/ark:/26678/pcrtFwQpNgFwZo"/>
	<skos:member rdf:resource="https://ark.frantiq.fr/ark:/26678/pcrta0mEYU6AUY"/>
	<skos:member rdf:resource="https://ark.frantiq.fr/ark:/26678/pcrtbjSdl4I8Mo"/>
	<skos:notation>007</skos:notation>
</rdf:Description>

<rdf:Description rdf:about="https://pactols.frantiq.fr/?idf=F99&amp;idt=TH_1">
	<rdf:type rdf:resource="http://purl.org/iso25964/skos-thes#ThesaurusArray"/>
	<iso-thes:superOrdinate rdf:resource="https://ark.frantiq.fr/ark:/26678/pcrtgcn5U8laUN"/>
	<skos:member rdf:resource="https://ark.frantiq.fr/ark:/26678/pcrtikYi5ORdK4"/>
	<skos:member rdf:resource="https://ark.frantiq.fr/ark:/26678/pcrttcRKMp4QdV"/>
	<skos:member rdf:resource="https://ark.frantiq.fr/ark:/26678/pcrtKiepgzdXSQ"/>
	<skos:member rdf:resource="https://ark.frantiq.fr/ark:/26678/pcrtiaewgLXnZc"/>
	<skos:member rdf:resource="https://ark.frantiq.fr/ark:/26678/pcrtsxjtz27508"/>
	<skos:member rdf:resource="https://ark.frantiq.fr/ark:/26678/pcrtbhbct8gbhn"/>
	<skos:prefLabel xml:lang="en">fruit and seed</skos:prefLabel>
	<dcterms:created rdf:datatype="http://www.w3.org/2001/XMLSchema#date">2021-08-18 17:38:45.929946+02</dcterms:created>
	<dcterms:modified rdf:datatype="http://www.w3.org/2001/XMLSchema#date">2021-08-18 17:38:45.929946+02</dcterms:modified>
	<skos:prefLabel xml:lang="de">Früchte und Samen</skos:prefLabel>
	<dcterms:created rdf:datatype="http://www.w3.org/2001/XMLSchema#date">2021-08-18 17:39:44.733379+02</dcterms:created>
	<dcterms:modified rdf:datatype="http://www.w3.org/2001/XMLSchema#date">2021-08-18 17:39:44.733379+02</dcterms:modified>
	<skos:prefLabel xml:lang="es">fruta y semilla</skos:prefLabel>
	<dcterms:created rdf:datatype="http://www.w3.org/2001/XMLSchema#date">2021-08-18 17:40:13.660419+02</dcterms:created>
	<dcterms:modified rdf:datatype="http://www.w3.org/2001/XMLSchema#date">2021-08-18 17:40:13.660419+02</dcterms:modified>
	<skos:prefLabel xml:lang="it">frutta e semi</skos:prefLabel>
	<dcterms:created rdf:datatype="http://www.w3.org/2001/XMLSchema#date">2021-08-18 17:40:41.233201+02</dcterms:created>
	<dcterms:modified rdf:datatype="http://www.w3.org/2001/XMLSchema#date">2021-08-18 17:40:41.233201+02</dcterms:modified>
	<skos:prefLabel xml:lang="nl">vruchten en zaden</skos:prefLabel>
	<dcterms:created rdf:datatype="http://www.w3.org/2001/XMLSchema#date">2021-08-18 17:41:07.415355+02</dcterms:created>
	<dcterms:modified rdf:datatype="http://www.w3.org/2001/XMLSchema#date">2021-08-18 17:41:07.415355+02</dcterms:modified>
	<skos:prefLabel xml:lang="fr">graines et fruits</skos:prefLabel>
	<dcterms:created rdf:datatype="http://www.w3.org/2001/XMLSchema#date">2021-08-18 17:11:11.480453+02</dcterms:created>
	<dcterms:modified rdf:datatype="http://www.w3.org/2001/XMLSchema#date">2021-08-18 17:11:11.480453+02</dcterms:modified>
</rdf:Description>

<rdf:Description rdf:about="https://pactols.frantiq.fr/?idf=F425&amp;idt=TH_1">
	<rdf:type rdf:resource="http://purl.org/iso25964/skos-thes#ThesaurusArray"/>
	<iso-thes:superOrdinate rdf:resource="https://ark.frantiq.fr/ark:/26678/pcrt40qs0fvnxg"/>
	<skos:member rdf:resource="https://ark.frantiq.fr/ark:/26678/pcrt24wcqp2cfz"/>
	<skos:member rdf:resource="https://ark.frantiq.fr/ark:/26678/pcrt9qq3x37vt0"/>
	<skos:member rdf:resource="https://ark.frantiq.fr/ark:/26678/pcrtr06vz24nj3"/>
	<skos:member rdf:resource="https://ark.frantiq.fr/ark:/26678/pcrt2fhx0kftpg"/>
	<skos:member rdf:resource="https://ark.frantiq.fr/ark:/26678/pcrt1tm77xkqbd"/>
	<skos:member rdf:resource="https://ark.frantiq.fr/ark:/26678/pcrt6xvrhrkjz8"/>
	<skos:member rdf:resource="https://ark.frantiq.fr/ark:/26678/pcrtwz8jzr2ttd"/>
	<skos:member rdf:resource="https://ark.frantiq.fr/ark:/26678/pcrt4rsdrmfk1b"/>
	<skos:member rdf:resource="https://ark.frantiq.fr/ark:/26678/pcrtjwwb1xztxh"/>
	<skos:prefLabel xml:lang="fr">allochèmes par classe</skos:prefLabel>
	<dcterms:created rdf:datatype="http://www.w3.org/2001/XMLSchema#date">2022-08-23 14:57:54.333543+02</dcterms:created>
	<dcterms:modified rdf:datatype="http://www.w3.org/2001/XMLSchema#date">2022-08-23 14:57:54.333543+02</dcterms:modified>
</rdf:Description>

<rdf:Description rdf:about="https://pactols.frantiq.fr/?idf=F427&amp;idt=TH_1">
	<rdf:type rdf:resource="http://purl.org/iso25964/skos-thes#ThesaurusArray"/>
	<iso-thes:superOrdinate rdf:resource="https://ark.frantiq.fr/ark:/26678/pcrt40qs0fvnxg"/>
	<skos:member rdf:resource="https://ark.frantiq.fr/ark:/26678/pcrt1kjsnnvmzh"/>
	<skos:member rdf:resource="https://ark.frantiq.fr/ark:/26678/pcrt21f986h3tk"/>
	<skos:member rdf:resource="https://ark.frantiq.fr/ark:/26678/pcrtqmm7q566vh"/>
	<skos:member rdf:resource="https://ark.frantiq.fr/ark:/26678/pcrtv3f379sr9v"/>
	<skos:member rdf:resource="https://ark.frantiq.fr/ark:/26678/pcrtb689mtdsz6"/>
	<skos:member rdf:resource="https://ark.frantiq.fr/ark:/26678/pcrt8c26426vth"/>
	<skos:prefLabel xml:lang="fr">allochèmes par répartition</skos:prefLabel>
	<dcterms:created rdf:datatype="http://www.w3.org/2001/XMLSchema#date">2022-08-23 14:58:17.356664+02</dcterms:created>
	<dcterms:modified rdf:datatype="http://www.w3.org/2001/XMLSchema#date">2022-08-23 14:58:17.356664+02</dcterms:modified>
</rdf:Description>

<rdf:Description rdf:about="https://pactols.frantiq.fr/?idf=F795&amp;idt=TH_1">
	<rdf:type rdf:resource="http://purl.org/iso25964/skos-thes#ThesaurusArray"/>
	<iso-thes:superOrdinate rdf:resource="https://ark.frantiq.fr/ark:/26678/pcrtfx4s0yvSLj"/>
	<skos:member rdf:resource="https://ark.frantiq.fr/ark:/26678/pcrtK43haeM3e3"/>
	<skos:member rdf:resource="https://ark.frantiq.fr/ark:/26678/pcrtnR5ePytFhO"/>
	<skos:member rdf:resource="https://ark.frantiq.fr/ark:/26678/pcrt1asKmbn9q8"/>
	<skos:prefLabel xml:lang="fr">terre cuite par revêtement</skos:prefLabel>
	<dcterms:created rdf:datatype="http://www.w3.org/2001/XMLSchema#date">2023-05-30 14:22:28.810644+02</dcterms:created>
	<dcterms:modified rdf:datatype="http://www.w3.org/2001/XMLSchema#date">2023-05-30 14:22:28.810644+02</dcterms:modified>
</rdf:Description>

<rdf:Description rdf:about="https://ark.frantiq.fr/ark:/26678/pcrt3KtdnXPGUg">
	<rdf:type rdf:resource="http://www.w3.org/2004/02/skos/core#Concept"/>
	<skos:prefLabel xml:lang="it">acciaio</skos:prefLabel>
	<skos:prefLabel xml:lang="es">acero</skos:prefLabel>
	<skos:prefLabel xml:lang="fr">acier</skos:prefLabel>
	<skos:prefLabel xml:lang="nl">staal</skos:prefLabel>
	<skos:prefLabel xml:lang="de">Stahl</skos:prefLabel>
	<skos:prefLabel xml:lang="en">steel</skos:prefLabel>
	<skos:prefLabel xml:lang="ar">فولاذ</skos:prefLabel>
	<skos:broader rdf:resource="https://ark.frantiq.fr/ark:/26678/pcrtzcGlM17go5"/>
	<skos:inScheme rdf:resource="https://ark.frantiq.fr/ark:/26678/TH_1"/>
	<opentheso:memberOf rdf:resource="https://ark.frantiq.fr/ark:/26678/pcrtv66rn9cbv1"/>
	<opentheso:memberOf rdf:resource="https://ark.frantiq.fr/ark:/26678/pcrtnbDLi2FkAj"/>
	<opentheso:memberOf rdf:resource="https://ark.frantiq.fr/ark:/26678/pcrtv0jq332vcq3gxt5m13d5"/>
	<skos:exactMatch rdf:resource="https://catalogue.bnf.fr/ark:/12148/cb119418662"/>
	<skos:exactMatch rdf:resource="https://www.wikidata.org/wiki/Q11427"/>
	<skos:exactMatch rdf:resource="http://vocab.getty.edu/aat/300133751"/>
	<dcterms:created rdf:datatype="http://www.w3.org/2001/XMLSchema#date">2007-02-08</dcterms:created>
	<dcterms:modified rdf:datatype="http://www.w3.org/2001/XMLSchema#date">2024-03-21</dcterms:modified>
	<dcterms:identifier>13091</dcterms:identifier>
	<dcterms:contributor>blandine.nouvel</dcterms:contributor>
	<dcterms:contributor>irene.weis</dcterms:contributor>
	<skos:definition xml:lang="en">An alloy of iron and carbon containing less than 1.8% carbon, capable of acquiring a wide variety of properties by mechanical and heat treatment. (Larousse)</skos:definition>
	<skos:definition xml:lang="fr">Alliage de fer et de carbone contenant moins de 1,8 % de carbone, susceptible d'acquérir, par traitement mécanique et thermique, des propriétés très variées. (Larousse)</skos:definition>
</rdf:Description>

<rdf:Description rdf:about="https://ark.frantiq.fr/ark:/26678/pcrthELuSjXqGH">
	<rdf:type rdf:resource="http://www.w3.org/2004/02/skos/core#Concept"/>
	<skos:prefLabel xml:lang="en">adobe</skos:prefLabel>
	<skos:prefLabel xml:lang="es">adobe</skos:prefLabel>
	<skos:prefLabel xml:lang="fr">adobe</skos:prefLabel>
	<skos:prefLabel xml:lang="nl">adobe</skos:prefLabel>
	<skos:prefLabel xml:lang="de">Lehmziegel</skos:prefLabel>
	<skos:prefLabel xml:lang="it">mattone crudo</skos:prefLabel>
	<skos:prefLabel xml:lang="ar">طوب</skos:prefLabel>
	<skos:altLabel xml:lang="it">adobe</skos:altLabel>
	<skos:altLabel xml:lang="fr">banco</skos:altLabel>
	<skos:altLabel xml:lang="fr">brique crue</skos:altLabel>
	<skos:altLabel xml:lang="de">luftgetrockneter Ziegel</skos:altLabel>
	<skos:altLabel xml:lang="en">mudbrick</skos:altLabel>
	<skos:altLabel xml:lang="ar">لِبن</skos:altLabel>
	<skos:related rdf:resource="https://ark.frantiq.fr/ark:/26678/pcrto44p1SaKFn"/>
	<skos:related rdf:resource="https://ark.frantiq.fr/ark:/26678/pcrtW9mUFwQABF"/>
	<skos:related rdf:resource="https://ark.frantiq.fr/ark:/26678/pcrtOI9SLqb5uI"/>
	<skos:broader rdf:resource="https://ark.frantiq.fr/ark:/26678/pcrtm6uoPROlPN"/>
	<skos:inScheme rdf:resource="https://ark.frantiq.fr/ark:/26678/TH_1"/>
	<opentheso:memberOf rdf:resource="https://ark.frantiq.fr/ark:/26678/pcrtv66rn9cbv1"/>
	<opentheso:memberOf rdf:resource="https://ark.frantiq.fr/ark:/26678/pcrtnbDLi2FkAj"/>
	<opentheso:memberOf rdf:resource="https://ark.frantiq.fr/ark:/26678/pcrtv0jq332vcq3gxt5m13d5"/>
	<skos:exactMatch rdf:resource="https://www.wikidata.org/wiki/Q183496"/>
	<skos:exactMatch rdf:resource="https://www.wikidata.org/wiki/Q49617371"/>
	<skos:exactMatch rdf:resource="http://vocab.getty.edu/aat/300081138"/>
	<dcterms:created rdf:datatype="http://www.w3.org/2001/XMLSchema#date">2007-02-08</dcterms:created>
	<dcterms:modified rdf:datatype="http://www.w3.org/2001/XMLSchema#date">2024-11-15</dcterms:modified>
	<dcterms:identifier>13103</dcterms:identifier>
	<dcterms:contributor>blandine.nouvel</dcterms:contributor>
	<dcterms:contributor>irene.weis</dcterms:contributor>
	<dcterms:contributor>justine.vincent</dcterms:contributor>
	<skos:definition xml:lang="fr">Argile qui, mélangée d'eau et d'une faible quantité de paille hachée ou d'un autre liant, peut être façonnée en briques séchées au soleil. (CNTRL)</skos:definition>
	<skos:definition xml:lang="en">Clay which, when mixed with water and a small quantity of chopped straw or another binder, can be shaped into sun-dried bricks (CNTRL).</skos:definition>
</rdf:Description>

<rdf:Description rdf:about="https://ark.frantiq.fr/ark:/26678/pcrtqmXRwn2Az6">
	<rdf:type rdf:resource="http://www.w3.org/2004/02/skos/core#Concept"/>
	<skos:prefLabel xml:lang="de">Achat</skos:prefLabel>
	<skos:prefLabel xml:lang="nl">agaat</skos:prefLabel>
	<skos:prefLabel xml:lang="it">agata</skos:prefLabel>
	<skos:prefLabel xml:lang="es">ágata</skos:prefLabel>
	<skos:prefLabel xml:lang="en">agate</skos:prefLabel>
	<skos:prefLabel xml:lang="fr">agate</skos:prefLabel>
	<skos:prefLabel xml:lang="ar">عقيق</skos:prefLabel>
	<skos:related rdf:resource="https://ark.frantiq.fr/ark:/26678/pcrtJt3ZKiNEFK"/>
	<skos:broader rdf:resource="https://ark.frantiq.fr/ark:/26678/pcrtOBWTai2Xms"/>
	<skos:inScheme rdf:resource="https://ark.frantiq.fr/ark:/26678/TH_1"/>
	<opentheso:memberOf rdf:resource="https://ark.frantiq.fr/ark:/26678/pcrtv66rn9cbv1"/>
	<opentheso:memberOf rdf:resource="https://ark.frantiq.fr/ark:/26678/pcrtnbDLi2FkAj"/>
	<skos:exactMatch rdf:resource="https://www.wikidata.org/wiki/Q123314"/>
	<skos:exactMatch rdf:resource="http://vocab.getty.edu/aat/300011135"/>
	<dcterms:created rdf:datatype="http://www.w3.org/2001/XMLSchema#date">2007-02-08</dcterms:created>
	<dcterms:modified rdf:datatype="http://www.w3.org/2001/XMLSchema#date">2023-08-02</dcterms:modified>
	<dcterms:identifier>13122</dcterms:identifier>
	<dcterms:contributor>blandine.nouvel</dcterms:contributor>
	<skos:definition xml:lang="fr">Variété de calcédoine qui se caractérise par des dépôts successifs de couleurs ou de tons différents, c'est une pierre fine. (wp)</skos:definition>
</rdf:Description>

<rdf:Description rdf:about="https://ark.frantiq.fr/ark:/26678/pcrtyJc250eY3m">
	<rdf:type rdf:resource="http://www.w3.org/2004/02/skos/core#Concept"/>
	<skos:prefLabel xml:lang="en">alabaster</skos:prefLabel>
	<skos:prefLabel xml:lang="de">Alabaster</skos:prefLabel>
	<skos:prefLabel xml:lang="es">alabastro</skos:prefLabel>
	<skos:prefLabel xml:lang="it">alabastro</skos:prefLabel>
	<skos:prefLabel xml:lang="nl">albast</skos:prefLabel>
	<skos:prefLabel xml:lang="fr">albâtre calcaire</skos:prefLabel>
	<skos:prefLabel xml:lang="ar">بِصْر</skos:prefLabel>
	<skos:altLabel xml:lang="fr">albâtre de la Bible</skos:altLabel>
	<skos:altLabel xml:lang="fr">albâtre égyptien</skos:altLabel>
	<skos:altLabel xml:lang="fr">albâtre oriental</skos:altLabel>
	<skos:altLabel xml:lang="fr">marbre onyx</skos:altLabel>
	<skos:related rdf:resource="https://ark.frantiq.fr/ark:/26678/pcrtzwhr6nrsvxm73pzkq2dq"/>
	<skos:broader rdf:resource="https://ark.frantiq.fr/ark:/26678/pcrtc1Ueky7Zpg"/>
	<skos:inScheme rdf:resource="https://ark.frantiq.fr/ark:/26678/TH_1"/>
	<opentheso:memberOf rdf:resource="https://ark.frantiq.fr/ark:/26678/pcrtv66rn9cbv1"/>
	<opentheso:memberOf rdf:resource="https://ark.frantiq.fr/ark:/26678/pcrtnbDLi2FkAj"/>
	<opentheso:memberOf rdf:resource="https://ark.frantiq.fr/ark:/26678/pcrtv0jq332vcq3gxt5m13d5"/>
	<skos:exactMatch rdf:resource="https://www.wikidata.org/wiki/Q143447"/>
	<skos:exactMatch rdf:resource="http://vocab.getty.edu/aat/300011101"/>
	<dcterms:created rdf:datatype="http://www.w3.org/2001/XMLSchema#date">2007-02-08</dcterms:created>
	<dcterms:modified rdf:datatype="http://www.w3.org/2001/XMLSchema#date">2024-09-06</dcterms:modified>
	<dcterms:identifier>13144</dcterms:identifier>
	<dcterms:contributor>blandine.nouvel</dcterms:contributor>
	<dcterms:contributor>patricia.moitrel</dcterms:contributor>
	<skos:definition xml:lang="fr">Variété de gypse très finement cristallisé blanc et translucide. Par extension, désigne aussi diverses variétés de calcaires blancs et parfois veinés par divers oxydes. (Lozet &amp;amp; Mathieu, Dictionnaire de science du sol. Ed. Technique et Documentation Lavoisier)</skos:definition>
</rdf:Description>

<rdf:Description rdf:about="https://ark.frantiq.fr/ark:/26678/pcrtgcn5U8laUN">
	<rdf:type rdf:resource="http://www.w3.org/2004/02/skos/core#Concept"/>
	<skos:prefLabel xml:lang="fr">aliment</skos:prefLabel>
	<skos:prefLabel xml:lang="es">alimento</skos:prefLabel>
	<skos:prefLabel xml:lang="it">alimento</skos:prefLabel>
	<skos:prefLabel xml:lang="en">food</skos:prefLabel>
	<skos:prefLabel xml:lang="de">Nahrungsmittel</skos:prefLabel>
	<skos:prefLabel xml:lang="nl">voedingsmiddelen</skos:prefLabel>
	<skos:prefLabel xml:lang="ar">غذاء</skos:prefLabel>
	<skos:altLabel xml:lang="it">cibo</skos:altLabel>
	<skos:altLabel xml:lang="es">comida</skos:altLabel>
	<skos:altLabel xml:lang="en">foodstuff</skos:altLabel>
	<skos:altLabel xml:lang="en">nourishment</skos:altLabel>
	<skos:altLabel xml:lang="fr">nourriture</skos:altLabel>
	<skos:related rdf:resource="https://ark.frantiq.fr/ark:/26678/pcrtos8skSB1bj"/>
	<skos:related rdf:resource="https://ark.frantiq.fr/ark:/26678/pcrtDFvOrje3j0"/>
	<skos:related rdf:resource="https://ark.frantiq.fr/ark:/26678/pcrtATL3ZnpSP5"/>
	<skos:related rdf:resource="https://ark.frantiq.fr/ark:/26678/pcrtzQPQ7iuHVL"/>
	<skos:narrower rdf:resource="https://ark.frantiq.fr/ark:/26678/pcrtUTZqItd8SL"/>
	<skos:narrower rdf:resource="https://ark.frantiq.fr/ark:/26678/pcrtVWVfmfl1T2"/>
	<skos:narrower rdf:resource="https://ark.frantiq.fr/ark:/26678/pcrtikYi5ORdK4"/>
	<skos:narrower rdf:resource="https://ark.frantiq.fr/ark:/26678/pcrttcRKMp4QdV"/>
	<skos:narrower rdf:resource="https://ark.frantiq.fr/ark:/26678/pcrtKiepgzdXSQ"/>
	<skos:narrower rdf:resource="https://ark.frantiq.fr/ark:/26678/pcrtiaewgLXnZc"/>
	<skos:narrower rdf:resource="https://ark.frantiq.fr/ark:/26678/pcrtDr6Oi6lHM6"/>
	<skos:narrower rdf:resource="https://ark.frantiq.fr/ark:/26678/pcrt82lj1bBlxj"/>
	<skos:narrower rdf:resource="https://ark.frantiq.fr/ark:/26678/pcrtOPqdpwj043"/>
	<skos:narrower rdf:resource="https://ark.frantiq.fr/ark:/26678/pcrtzOFeK4FZEf"/>
	<skos:narrower rdf:resource="https://ark.frantiq.fr/ark:/26678/pcrtsxjtz27508"/>
	<skos:narrower rdf:resource="https://ark.frantiq.fr/ark:/26678/pcrtbhbct8gbhn"/>
	<skos:narrower rdf:resource="https://ark.frantiq.fr/ark:/26678/pcrtjs2wjn65hq"/>
	<skos:broader rdf:resource="https://ark.frantiq.fr/ark:/26678/pcrtIMsuG0RWTs"/>
	<skos:inScheme rdf:resource="https://ark.frantiq.fr/ark:/26678/TH_1"/>
	<opentheso:memberOf rdf:resource="https://ark.frantiq.fr/ark:/26678/pcrtv66rn9cbv1"/>
	<opentheso:memberOf rdf:resource="https://ark.frantiq.fr/ark:/26678/pcrtnbDLi2FkAj"/>
	<iso-thes:subordinateArray rdf:resource="https://pactols.frantiq.fr/?idf=F99&amp;idt=TH_1"/>
	<skos:exactMatch rdf:resource="https://www.wikidata.org/wiki/Q2095"/>
	<skos:exactMatch rdf:resource="http://vocab.getty.edu/aat/300254496"/>
	<dcterms:created rdf:datatype="http://www.w3.org/2001/XMLSchema#date">2007-02-08</dcterms:created>
	<dcterms:modified rdf:datatype="http://www.w3.org/2001/XMLSchema#date">2023-08-02</dcterms:modified>
	<dcterms:identifier>13150</dcterms:identifier>
	<dcterms:contributor>blandine.nouvel</dcterms:contributor>
	<skos:definition xml:lang="en">Substances suitable for consumption as food. (OED)</skos:definition>
	<skos:definition xml:lang="fr">Toute substance susceptible de fournir aux êtres vivants les éléments nécessaires à leur croissance ou à leur conservation (cnrtl)</skos:definition>
</rdf:Description>

<rdf:Description rdf:about="https://ark.frantiq.fr/ark:/26678/pcrtzcGlM17go5">
	<rdf:type rdf:resource="http://www.w3.org/2004/02/skos/core#Concept"/>
	<skos:prefLabel xml:lang="es">aleación</skos:prefLabel>
	<skos:prefLabel xml:lang="fr">alliage</skos:prefLabel>
	<skos:prefLabel xml:lang="en">alloy</skos:prefLabel>
	<skos:prefLabel xml:lang="it">lega (metallurgia)</skos:prefLabel>
	<skos:prefLabel xml:lang="nl">legering</skos:prefLabel>
	<skos:prefLabel xml:lang="de">Legierungen</skos:prefLabel>
	<skos:prefLabel xml:lang="ar">أُشابة</skos:prefLabel>
	<skos:altLabel xml:lang="it">lega metallica</skos:altLabel>
	<skos:altLabel xml:lang="ar">خليط معدني</skos:altLabel>
	<skos:narrower rdf:resource="https://ark.frantiq.fr/ark:/26678/pcrt3KtdnXPGUg"/>
	<skos:narrower rdf:resource="https://ark.frantiq.fr/ark:/26678/pcrtjzKlry0LZi"/>
	<skos:narrower rdf:resource="https://ark.frantiq.fr/ark:/26678/pcrtTcvLDTNT86"/>
	<skos:narrower rdf:resource="https://ark.frantiq.fr/ark:/26678/pcrtlSaqkoJ8gu"/>
	<skos:narrower rdf:resource="https://ark.frantiq.fr/ark:/26678/pcrtkbJMkYrMF6"/>
	<skos:narrower rdf:resource="https://ark.frantiq.fr/ark:/26678/pcrt6d15xRmV8x"/>
	<skos:broader rdf:resource="https://ark.frantiq.fr/ark:/26678/pcrtkn1hAXHveS"/>
	<skos:inScheme rdf:resource="https://ark.frantiq.fr/ark:/26678/TH_1"/>
	<opentheso:memberOf rdf:resource="https://ark.frantiq.fr/ark:/26678/pcrtv66rn9cbv1"/>
	<opentheso:memberOf rdf:resource="https://ark.frantiq.fr/ark:/26678/pcrtnbDLi2FkAj"/>
	<skos:exactMatch rdf:resource="https://catalogue.bnf.fr/ark:/12148/cb119579618"/>
	<skos:exactMatch rdf:resource="https://www.wikidata.org/wiki/Q37756"/>
	<skos:exactMatch rdf:resource="http://vocab.getty.edu/aat/300010902"/>
	<dcterms:created rdf:datatype="http://www.w3.org/2001/XMLSchema#date">2007-02-08</dcterms:created>
	<dcterms:modified rdf:datatype="http://www.w3.org/2001/XMLSchema#date">2023-08-02</dcterms:modified>
	<dcterms:identifier>13153</dcterms:identifier>
	<dcterms:contributor>blandine.nouvel</dcterms:contributor>
	<skos:definition xml:lang="en">Metallurgical product resulting from the incorporation into a metal of one or more elements (metallic or non-metallic), carried out with the aim of modifying some of its properties or even conferring new properties on it. (Larousse)</skos:definition>
	<skos:definition xml:lang="fr">Produit métallurgique résultant de l'incorporation à un métal d'un ou de plusieurs éléments (métalliques ou non), effectuée dans le but de modifier certaines de ses propriétés ou même de lui conférer des propriétés nouvelles. (Larousse)</skos:definition>
</rdf:Description>

<rdf:Description rdf:about="https://ark.frantiq.fr/ark:/26678/pcrtuV4RYc06TP">
	<rdf:type rdf:resource="http://www.w3.org/2004/02/skos/core#Concept"/>
	<skos:prefLabel xml:lang="it">alluminio</skos:prefLabel>
	<skos:prefLabel xml:lang="es">aluminio</skos:prefLabel>
	<skos:prefLabel xml:lang="en">aluminium</skos:prefLabel>
	<skos:prefLabel xml:lang="fr">aluminium</skos:prefLabel>
	<skos:prefLabel xml:lang="nl">aluminium</skos:prefLabel>
	<skos:prefLabel xml:lang="de">Aluminium</skos:prefLabel>
	<skos:prefLabel xml:lang="ar">ألومنيوم</skos:prefLabel>
	<skos:broader rdf:resource="https://ark.frantiq.fr/ark:/26678/pcrtkn1hAXHveS"/>
	<skos:inScheme rdf:resource="https://ark.frantiq.fr/ark:/26678/TH_1"/>
	<opentheso:memberOf rdf:resource="https://ark.frantiq.fr/ark:/26678/pcrtv66rn9cbv1"/>
	<opentheso:memberOf rdf:resource="https://ark.frantiq.fr/ark:/26678/pcrtnbDLi2FkAj"/>
	<opentheso:memberOf rdf:resource="https://ark.frantiq.fr/ark:/26678/pcrtv0jq332vcq3gxt5m13d5"/>
	<skos:exactMatch rdf:resource="https://catalogue.bnf.fr/ark:/12148/cb11976300k"/>
	<skos:exactMatch rdf:resource="https://www.wikidata.org/wiki/Q663"/>
	<skos:exactMatch rdf:resource="http://vocab.getty.edu/aat/300011015"/>
	<skos:exactMatch rdf:resource="http://www.wikidata.org/entity/Q3612663"/>
	<dcterms:created rdf:datatype="http://www.w3.org/2001/XMLSchema#date">2007-02-08</dcterms:created>
	<dcterms:modified rdf:datatype="http://www.w3.org/2001/XMLSchema#date">2024-11-15</dcterms:modified>
	<dcterms:identifier>13159</dcterms:identifier>
	<dcterms:contributor>blandine.nouvel</dcterms:contributor>
	<dcterms:contributor>irene.weis</dcterms:contributor>
	<dcterms:contributor>justine.vincent</dcterms:contributor>
	<skos:definition xml:lang="en">Mineral species, simple metallic body with the chemical formula Al, corresponding mainly to the chemical element aluminium. (wp)</skos:definition>
	<skos:definition xml:lang="fr">Espèce minérale, corps simple métallique de formule chimique Al correspondant principalement à l'élément chimique aluminium. (wp)</skos:definition>
	<skos:historyNote xml:lang="fr">2024-11-15 : modification de la définition.</skos:historyNote>
</rdf:Description>

<rdf:Description rdf:about="https://ark.frantiq.fr/ark:/26678/pcrtSiQAzZxXsv">
	<rdf:type rdf:resource="http://www.w3.org/2004/02/skos/core#Concept"/>
	<skos:prefLabel xml:lang="es">ámbar</skos:prefLabel>
	<skos:prefLabel xml:lang="en">amber</skos:prefLabel>
	<skos:prefLabel xml:lang="it">ambra</skos:prefLabel>
	<skos:prefLabel xml:lang="fr">ambre</skos:prefLabel>
	<skos:prefLabel xml:lang="nl">barnsteen</skos:prefLabel>
	<skos:prefLabel xml:lang="de">Bernstein</skos:prefLabel>
	<skos:prefLabel xml:lang="ar">عنبر</skos:prefLabel>
	<skos:altLabel xml:lang="fr">ambre jaune</skos:altLabel>
	<skos:related rdf:resource="https://ark.frantiq.fr/ark:/26678/pcrtDoEeaZ6VcU"/>
	<skos:related rdf:resource="https://ark.frantiq.fr/ark:/26678/pcrtzORYwll8NI"/>
	<skos:broader rdf:resource="https://ark.frantiq.fr/ark:/26678/pcrtrxL50B7yNx"/>
	<skos:inScheme rdf:resource="https://ark.frantiq.fr/ark:/26678/TH_1"/>
	<opentheso:memberOf rdf:resource="https://ark.frantiq.fr/ark:/26678/pcrtv66rn9cbv1"/>
	<opentheso:memberOf rdf:resource="https://ark.frantiq.fr/ark:/26678/pcrtnbDLi2FkAj"/>
	<skos:exactMatch rdf:resource="https://www.wikidata.org/wiki/Q25381"/>
	<skos:exactMatch rdf:resource="http://vocab.getty.edu/aat/300012934"/>
	<dcterms:created rdf:datatype="http://www.w3.org/2001/XMLSchema#date">2007-02-08</dcterms:created>
	<dcterms:modified rdf:datatype="http://www.w3.org/2001/XMLSchema#date">2024-10-18</dcterms:modified>
	<dcterms:identifier>13166</dcterms:identifier>
	<dcterms:contributor>blandine.nouvel</dcterms:contributor>
	<dcterms:contributor>patricia.moitrel</dcterms:contributor>
	<skos:definition xml:lang="en">Fossilised, hard, transparent oleoresin, also known as yellow amber (Dict. Robert).</skos:definition>
	<skos:definition xml:lang="fr">Oléorésine fossilisée, dure et transparente, également appelée ambre jaune (Dict. Robert).</skos:definition>
	<skos:scopeNote xml:lang="en">Do not use to index ambergris secreted by sperm whales.</skos:scopeNote>
	<skos:scopeNote xml:lang="fr">Ne pas utiliser pour indexer l'ambre gris sécrété par les cachalots.</skos:scopeNote>
</rdf:Description>

<rdf:Description rdf:about="https://ark.frantiq.fr/ark:/26678/pcrt0IaUrrrmF5">
	<rdf:type rdf:resource="http://www.w3.org/2004/02/skos/core#Concept"/>
	<skos:prefLabel xml:lang="es">amatista</skos:prefLabel>
	<skos:prefLabel xml:lang="nl">amethist</skos:prefLabel>
	<skos:prefLabel xml:lang="en">amethyst</skos:prefLabel>
	<skos:prefLabel xml:lang="de">Amethyst</skos:prefLabel>
	<skos:prefLabel xml:lang="fr">améthyste</skos:prefLabel>
	<skos:prefLabel xml:lang="it">ametista</skos:prefLabel>
	<skos:prefLabel xml:lang="ar">جَمَشت</skos:prefLabel>
	<skos:broader rdf:resource="https://ark.frantiq.fr/ark:/26678/pcrtJt3ZKiNEFK"/>
	<skos:inScheme rdf:resource="https://ark.frantiq.fr/ark:/26678/TH_1"/>
	<opentheso:memberOf rdf:resource="https://ark.frantiq.fr/ark:/26678/pcrtv66rn9cbv1"/>
	<opentheso:memberOf rdf:resource="https://ark.frantiq.fr/ark:/26678/pcrtnbDLi2FkAj"/>
	<skos:exactMatch rdf:resource="https://www.wikidata.org/wiki/Q79058"/>
	<skos:exactMatch rdf:resource="http://vocab.getty.edu/aat/300011133"/>
	<dcterms:created rdf:datatype="http://www.w3.org/2001/XMLSchema#date">2007-02-08</dcterms:created>
	<dcterms:modified rdf:datatype="http://www.w3.org/2001/XMLSchema#date">2024-03-20</dcterms:modified>
	<dcterms:identifier>13196</dcterms:identifier>
	<dcterms:contributor>blandine.nouvel</dcterms:contributor>
	<dcterms:contributor>justine.vincent</dcterms:contributor>
	<skos:definition xml:lang="en">A variety of diaphanous to translucent violet quartz (silicon dioxide), whose hue is due to traces of iron (wikipedia).</skos:definition>
	<skos:definition xml:lang="ar">كوارتز بنفسجي</skos:definition>
	<skos:definition xml:lang="fr">Variété de quartz violet (dioxyde de silicium), de diaphane à translucide, dont la teinte est due aux traces de fer. (wikipedia)</skos:definition>
</rdf:Description>

<rdf:Description rdf:about="https://ark.frantiq.fr/ark:/26678/pcrtcWoSlbWLE0">
	<rdf:type rdf:resource="http://www.w3.org/2004/02/skos/core#Concept"/>
	<skos:prefLabel xml:lang="fr">argent</skos:prefLabel>
	<skos:prefLabel xml:lang="it">argento</skos:prefLabel>
	<skos:prefLabel xml:lang="es">plata</skos:prefLabel>
	<skos:prefLabel xml:lang="de">Silber</skos:prefLabel>
	<skos:prefLabel xml:lang="en">silver</skos:prefLabel>
	<skos:prefLabel xml:lang="nl">zilver</skos:prefLabel>
	<skos:prefLabel xml:lang="ar">فضة</skos:prefLabel>
	<skos:altLabel xml:lang="fr">argent (métal)</skos:altLabel>
	<skos:related rdf:resource="https://ark.frantiq.fr/ark:/26678/crt5Bzhnbs4Vb"/>
	<skos:related rdf:resource="https://ark.frantiq.fr/ark:/26678/crttYXJnmIA72"/>
	<skos:broader rdf:resource="https://ark.frantiq.fr/ark:/26678/pcrtkn1hAXHveS"/>
	<skos:inScheme rdf:resource="https://ark.frantiq.fr/ark:/26678/TH_1"/>
	<opentheso:memberOf rdf:resource="https://ark.frantiq.fr/ark:/26678/pcrtv66rn9cbv1"/>
	<opentheso:memberOf rdf:resource="https://ark.frantiq.fr/ark:/26678/pcrtnbDLi2FkAj"/>
	<opentheso:memberOf rdf:resource="https://ark.frantiq.fr/ark:/26678/pcrtv0jq332vcq3gxt5m13d5"/>
	<skos:exactMatch rdf:resource="https://catalogue.bnf.fr/ark:/12148/cb11959564p"/>
	<skos:exactMatch rdf:resource="https://www.wikidata.org/wiki/Q1090"/>
	<skos:exactMatch rdf:resource="http://vocab.getty.edu/aat/300011029"/>
	<dcterms:created rdf:datatype="http://www.w3.org/2001/XMLSchema#date">2007-02-08</dcterms:created>
	<dcterms:modified rdf:datatype="http://www.w3.org/2001/XMLSchema#date">2024-11-15</dcterms:modified>
	<dcterms:identifier>13338</dcterms:identifier>
	<dcterms:contributor>blandine.nouvel</dcterms:contributor>
	<dcterms:contributor>justine.vincent</dcterms:contributor>
	<dcterms:contributor>patricia.moitrel</dcterms:contributor>
	<skos:definition xml:lang="fr">Métal d'un blanc brillant, très ductile et malléable, inoxydable, corps simple de symbole Ag. (CNRTL)</skos:definition>
	<skos:definition xml:lang="en">Shiny white metal, very ductile and malleable, stainless, simple body with Ag symbol. (CNRTL)</skos:definition>
	<skos:scopeNote xml:lang="fr">Ne pas l'utiliser pour la monnaie, sauf pour spécifier la matière (BL)</skos:scopeNote>
	<skos:historyNote xml:lang="fr">2024-10-16 : ajout d'une note d'application et modification de la définition.</skos:historyNote>
</rdf:Description>

<rdf:Description rdf:about="https://ark.frantiq.fr/ark:/26678/pcrto44p1SaKFn">
	<rdf:type rdf:resource="http://www.w3.org/2004/02/skos/core#Concept"/>
	<skos:prefLabel xml:lang="es">arcilla</skos:prefLabel>
	<skos:prefLabel xml:lang="fr">argile</skos:prefLabel>
	<skos:prefLabel xml:lang="it">argilla</skos:prefLabel>
	<skos:prefLabel xml:lang="en">clay</skos:prefLabel>
	<skos:prefLabel xml:lang="nl">klei</skos:prefLabel>
	<skos:prefLabel xml:lang="de">Ton</skos:prefLabel>
	<skos:prefLabel xml:lang="ar">صلصال</skos:prefLabel>
	<skos:related rdf:resource="https://ark.frantiq.fr/ark:/26678/pcrthELuSjXqGH"/>
	<skos:related rdf:resource="https://ark.frantiq.fr/ark:/26678/pcrtdZsvpNrnWI"/>
	<skos:related rdf:resource="https://ark.frantiq.fr/ark:/26678/pcrtZETJwE7RTQ"/>
	<skos:related rdf:resource="https://ark.frantiq.fr/ark:/26678/pcrtfx4s0yvSLj"/>
	<skos:related rdf:resource="https://ark.frantiq.fr/ark:/26678/pcrttqRMDTN4VE"/>
	<skos:narrower rdf:resource="https://ark.frantiq.fr/ark:/26678/pcrtgjwqPbWjHa"/>
	<skos:narrower rdf:resource="https://ark.frantiq.fr/ark:/26678/pcrttnySGIGsj6"/>
	<skos:narrower rdf:resource="https://ark.frantiq.fr/ark:/26678/pcrtB8FNASjQrB"/>
	<skos:narrower rdf:resource="https://ark.frantiq.fr/ark:/26678/pcrtskMRAe4usI"/>
	<skos:broader rdf:resource="https://ark.frantiq.fr/ark:/26678/pcrtRiKgPqvJQO"/>
	<skos:inScheme rdf:resource="https://ark.frantiq.fr/ark:/26678/TH_1"/>
	<opentheso:memberOf rdf:resource="https://ark.frantiq.fr/ark:/26678/pcrtv66rn9cbv1"/>
	<opentheso:memberOf rdf:resource="https://ark.frantiq.fr/ark:/26678/pcrtnbDLi2FkAj"/>
	<opentheso:memberOf rdf:resource="https://ark.frantiq.fr/ark:/26678/pcrtv0jq332vcq3gxt5m13d5"/>
	<skos:exactMatch rdf:resource="https://catalogue.bnf.fr/ark:/12148/cb11934795w"/>
	<skos:exactMatch rdf:resource="https://www.wikidata.org/wiki/Q42302"/>
	<skos:exactMatch rdf:resource="http://vocab.getty.edu/aat/300010439"/>
	<dcterms:created rdf:datatype="http://www.w3.org/2001/XMLSchema#date">2007-02-08</dcterms:created>
	<dcterms:modified rdf:datatype="http://www.w3.org/2001/XMLSchema#date">2024-09-06</dcterms:modified>
	<dcterms:identifier>13342</dcterms:identifier>
	<dcterms:contributor>blandine.nouvel</dcterms:contributor>
	<dcterms:contributor>patricia.moitrel</dcterms:contributor>
	<skos:definition xml:lang="fr">Matière rocheuse naturelle à base de silicates ou d'aluminosilicates hydratés de structure lamellaire, provenant en général de l'altération de silicates à charpente tridimensionnelle, tels que les feldspaths (Wikipedia).</skos:definition>
</rdf:Description>

<rdf:Description rdf:about="https://ark.frantiq.fr/ark:/26678/pcrtgjwqPbWjHa">
	<rdf:type rdf:resource="http://www.w3.org/2004/02/skos/core#Concept"/>
	<skos:prefLabel xml:lang="es">arcilla roja</skos:prefLabel>
	<skos:prefLabel xml:lang="fr">argile rouge</skos:prefLabel>
	<skos:prefLabel xml:lang="it">argilla rossa</skos:prefLabel>
	<skos:prefLabel xml:lang="en">red clay</skos:prefLabel>
	<skos:prefLabel xml:lang="nl">rode klei</skos:prefLabel>
	<skos:prefLabel xml:lang="de">Rotlehm</skos:prefLabel>
	<skos:prefLabel xml:lang="ar">صلصال أحمر</skos:prefLabel>
	<skos:broader rdf:resource="https://ark.frantiq.fr/ark:/26678/pcrto44p1SaKFn"/>
	<skos:inScheme rdf:resource="https://ark.frantiq.fr/ark:/26678/TH_1"/>
	<opentheso:memberOf rdf:resource="https://ark.frantiq.fr/ark:/26678/pcrtv66rn9cbv1"/>
	<opentheso:memberOf rdf:resource="https://ark.frantiq.fr/ark:/26678/pcrtnbDLi2FkAj"/>
	<dcterms:created rdf:datatype="http://www.w3.org/2001/XMLSchema#date">2007-02-08</dcterms:created>
	<dcterms:modified rdf:datatype="http://www.w3.org/2001/XMLSchema#date">2023-08-02</dcterms:modified>
	<dcterms:identifier>13349</dcterms:identifier>
	<dcterms:contributor>blandine.nouvel</dcterms:contributor>
	<skos:definition xml:lang="fr">Dépôt marin des grandes profondeurs. (Lar.)</skos:definition>
</rdf:Description>

<rdf:Description rdf:about="https://ark.frantiq.fr/ark:/26678/pcrt5mFxzmQ9rX">
	<rdf:type rdf:resource="http://www.w3.org/2004/02/skos/core#Concept"/>
	<skos:prefLabel xml:lang="nl">arseen</skos:prefLabel>
	<skos:prefLabel xml:lang="de">Arsen</skos:prefLabel>
	<skos:prefLabel xml:lang="en">arsenic</skos:prefLabel>
	<skos:prefLabel xml:lang="fr">arsenic</skos:prefLabel>
	<skos:prefLabel xml:lang="it">arsenico</skos:prefLabel>
	<skos:prefLabel xml:lang="es">arsénico</skos:prefLabel>
	<skos:prefLabel xml:lang="ar">زِرْنيخ</skos:prefLabel>
	<skos:broader rdf:resource="https://ark.frantiq.fr/ark:/26678/pcrty2mcsksa6s"/>
	<skos:inScheme rdf:resource="https://ark.frantiq.fr/ark:/26678/TH_1"/>
	<opentheso:memberOf rdf:resource="https://ark.frantiq.fr/ark:/26678/pcrtv66rn9cbv1"/>
	<opentheso:memberOf rdf:resource="https://ark.frantiq.fr/ark:/26678/pcrtnbDLi2FkAj"/>
	<opentheso:memberOf rdf:resource="https://ark.frantiq.fr/ark:/26678/pcrtv0jq332vcq3gxt5m13d5"/>
	<skos:exactMatch rdf:resource="https://catalogue.bnf.fr/ark:/12148/cb11971740q"/>
	<skos:exactMatch rdf:resource="https://www.wikidata.org/wiki/Q871"/>
	<dcterms:created rdf:datatype="http://www.w3.org/2001/XMLSchema#date">2007-02-08</dcterms:created>
	<dcterms:modified rdf:datatype="http://www.w3.org/2001/XMLSchema#date">2024-11-18</dcterms:modified>
	<dcterms:identifier>13369</dcterms:identifier>
	<dcterms:contributor>blandine.nouvel</dcterms:contributor>
	<dcterms:contributor>irene.weis</dcterms:contributor>
	<dcterms:contributor>justine.vincent</dcterms:contributor>
	<skos:definition xml:lang="fr">Corps simple d'apparence métallique, très répandu dans les minerais métalliques. (Larousse)</skos:definition>
	<skos:definition xml:lang="en">A simple body of metallic appearance, very common in metal ores. (Larousse)</skos:definition>
	<skos:historyNote xml:lang="fr">2024-11-18 : modification de la définition.</skos:historyNote>
</rdf:Description>

<rdf:Description rdf:about="https://ark.frantiq.fr/ark:/26678/pcrtctuE9VNJOc">
	<rdf:type rdf:resource="http://www.w3.org/2004/02/skos/core#Concept"/>
	<skos:prefLabel xml:lang="en">basalt</skos:prefLabel>
	<skos:prefLabel xml:lang="nl">basalt</skos:prefLabel>
	<skos:prefLabel xml:lang="de">Basalt</skos:prefLabel>
	<skos:prefLabel xml:lang="fr">basalte</skos:prefLabel>
	<skos:prefLabel xml:lang="es">basalto</skos:prefLabel>
	<skos:prefLabel xml:lang="it">basalto</skos:prefLabel>
	<skos:prefLabel xml:lang="ar">بازلت</skos:prefLabel>
	<skos:altLabel xml:lang="ar">نَسَفَة</skos:altLabel>
	<skos:broader rdf:resource="https://ark.frantiq.fr/ark:/26678/pcrtmxvuuXHSTS"/>
	<skos:inScheme rdf:resource="https://ark.frantiq.fr/ark:/26678/TH_1"/>
	<opentheso:memberOf rdf:resource="https://ark.frantiq.fr/ark:/26678/pcrtv66rn9cbv1"/>
	<opentheso:memberOf rdf:resource="https://ark.frantiq.fr/ark:/26678/pcrtnbDLi2FkAj"/>
	<skos:exactMatch rdf:resource="https://catalogue.bnf.fr/ark:/12148/cb11964786j"/>
	<skos:exactMatch rdf:resource="https://www.wikidata.org/wiki/Q43338"/>
	<skos:exactMatch rdf:resource="http://vocab.getty.edu/aat/300011222"/>
	<dcterms:created rdf:datatype="http://www.w3.org/2001/XMLSchema#date">2007-02-08</dcterms:created>
	<dcterms:modified rdf:datatype="http://www.w3.org/2001/XMLSchema#date">2024-11-14</dcterms:modified>
	<dcterms:identifier>13541</dcterms:identifier>
	<dcterms:contributor>blandine.nouvel</dcterms:contributor>
	<dcterms:contributor>justine.vincent</dcterms:contributor>
	<skos:definition xml:lang="en">Compact or vacuolated microlithic eruptive magmatic rock composed of feldspars, pyroxenes, olivine, augite, magnetite, micas, etc. (Lozet &amp;amp; Mathieu, Dictionnaire de science du sol. Ed. Technique et Documentation Lavoisier)</skos:definition>
	<skos:definition xml:lang="fr">Roche magmatique éruptive microlithique compacte ou vacuolaire composée de feldspaths, pyroxènes, olivine, augite, magnétite, micas etc. (Lozet &amp;amp; Mathieu, Dictionnaire de science du sol. Ed. Technique et Documentation Lavoisier)</skos:definition>
</rdf:Description>

<rdf:Description rdf:about="https://ark.frantiq.fr/ark:/26678/pcrtnsH1xdYgZe">
	<rdf:type rdf:resource="http://www.w3.org/2004/02/skos/core#Concept"/>
	<skos:prefLabel xml:lang="es">betún</skos:prefLabel>
	<skos:prefLabel xml:lang="fr">bitume</skos:prefLabel>
	<skos:prefLabel xml:lang="it">bitume</skos:prefLabel>
	<skos:prefLabel xml:lang="en">bitumen</skos:prefLabel>
	<skos:prefLabel xml:lang="nl">bitumen</skos:prefLabel>
	<skos:prefLabel xml:lang="de">Bitumen</skos:prefLabel>
	<skos:prefLabel xml:lang="el">Άσφαλτος</skos:prefLabel>
	<skos:prefLabel xml:lang="ru">битум</skos:prefLabel>
	<skos:prefLabel xml:lang="he">אספלט</skos:prefLabel>
	<skos:prefLabel xml:lang="ar">أسفلت</skos:prefLabel>
	<skos:altLabel xml:lang="es">asfalto</skos:altLabel>
	<skos:altLabel xml:lang="en">asphalt</skos:altLabel>
	<skos:altLabel xml:lang="es">bitumen</skos:altLabel>
	<skos:altLabel xml:lang="de">Erdpech</skos:altLabel>
	<skos:broader rdf:resource="https://ark.frantiq.fr/ark:/26678/pcrtx37ph91cww"/>
	<skos:inScheme rdf:resource="https://ark.frantiq.fr/ark:/26678/TH_1"/>
	<opentheso:memberOf rdf:resource="https://ark.frantiq.fr/ark:/26678/pcrtv66rn9cbv1"/>
	<opentheso:memberOf rdf:resource="https://ark.frantiq.fr/ark:/26678/pcrtnbDLi2FkAj"/>
	<skos:exactMatch rdf:resource="https://www.wikidata.org/wiki/Q167510"/>
	<skos:exactMatch rdf:resource="http://vocab.getty.edu/aat/300012966"/>
	<dcterms:created rdf:datatype="http://www.w3.org/2001/XMLSchema#date">2007-02-08</dcterms:created>
	<dcterms:modified rdf:datatype="http://www.w3.org/2001/XMLSchema#date">2023-08-02</dcterms:modified>
	<dcterms:identifier>13581</dcterms:identifier>
	<dcterms:contributor>blandine.nouvel</dcterms:contributor>
	<skos:definition xml:lang="de">zähes, schwarzes Endprodukt der Erdöldestillation (Wikidata)</skos:definition>
	<skos:definition xml:lang="en">highly viscous, black material obtained from the destillation of petroleum (Wikidata)</skos:definition>
	<skos:definition xml:lang="he">נוזל צמיג שמופיע באופן טבעי בנפט גולמי (Wikidata)</skos:definition>
	<skos:definition xml:lang="it">miscela di idrocarburi naturali o residuati derivanti dalla distillazione o raffinazione del greggio (Wikidata)</skos:definition>
	<skos:definition xml:lang="ru">твёрдые или смолоподобные продукты, представляющие собой смесь углеводородов и их производных (Wikidata)</skos:definition>
	<skos:definition xml:lang="fr">Terme regroupant les produits hydrocarbonés dérivant de la matière organique  où les distinctions sont fondées sur les compositions chimiques, les solubilités, la fluorescence… (Raoult et Foucault, 2005).</skos:definition>
</rdf:Description>

<rdf:Description rdf:about="https://ark.frantiq.fr/ark:/26678/pcrt3nBjHrcDGM">
	<rdf:type rdf:resource="http://www.w3.org/2004/02/skos/core#Concept"/>
	<skos:prefLabel xml:lang="en">beer</skos:prefLabel>
	<skos:prefLabel xml:lang="nl">bier</skos:prefLabel>
	<skos:prefLabel xml:lang="de">Bier</skos:prefLabel>
	<skos:prefLabel xml:lang="fr">bière</skos:prefLabel>
	<skos:prefLabel xml:lang="it">birra</skos:prefLabel>
	<skos:prefLabel xml:lang="es">cerveza</skos:prefLabel>
	<skos:prefLabel xml:lang="ar">جِعة</skos:prefLabel>
	<skos:broader rdf:resource="https://ark.frantiq.fr/ark:/26678/pcrt6z097U6IUf"/>
	<skos:inScheme rdf:resource="https://ark.frantiq.fr/ark:/26678/TH_1"/>
	<opentheso:memberOf rdf:resource="https://ark.frantiq.fr/ark:/26678/pcrtv66rn9cbv1"/>
	<opentheso:memberOf rdf:resource="https://ark.frantiq.fr/ark:/26678/pcrtnbDLi2FkAj"/>
	<skos:exactMatch rdf:resource="https://catalogue.bnf.fr/ark:/12148/cb11965887d"/>
	<skos:exactMatch rdf:resource="https://www.wikidata.org/wiki/Q44"/>
	<dcterms:created rdf:datatype="http://www.w3.org/2001/XMLSchema#date">2007-02-08</dcterms:created>
	<dcterms:modified rdf:datatype="http://www.w3.org/2001/XMLSchema#date">2023-08-02</dcterms:modified>
	<dcterms:identifier>13582</dcterms:identifier>
	<dcterms:contributor>blandine.nouvel</dcterms:contributor>
	<skos:definition xml:lang="en">Fermented beverage prepared from sprouted cereals (Lar.)</skos:definition>
	<skos:definition xml:lang="fr">Boisson fermentée préparée à partir de céréales germées (Lar.)</skos:definition>
</rdf:Description>

<rdf:Description rdf:about="https://ark.frantiq.fr/ark:/26678/pcrtMr3tb79bV8">
	<rdf:type rdf:resource="http://www.w3.org/2004/02/skos/core#Concept"/>
	<skos:prefLabel xml:lang="fr">bois</skos:prefLabel>
	<skos:prefLabel xml:lang="de">Holz</skos:prefLabel>
	<skos:prefLabel xml:lang="nl">hout</skos:prefLabel>
	<skos:prefLabel xml:lang="it">legno</skos:prefLabel>
	<skos:prefLabel xml:lang="es">madera</skos:prefLabel>
	<skos:prefLabel xml:lang="en">wood</skos:prefLabel>
	<skos:prefLabel xml:lang="ar">خشب</skos:prefLabel>
	<skos:related rdf:resource="https://ark.frantiq.fr/ark:/26678/pcrtI4g8pXkSSJ"/>
	<skos:related rdf:resource="https://ark.frantiq.fr/ark:/26678/pcrtO40ZLI4giK"/>
	<skos:related rdf:resource="https://ark.frantiq.fr/ark:/26678/pcrteFHjryOQqT"/>
	<skos:related rdf:resource="https://ark.frantiq.fr/ark:/26678/pcrtYgu4jWtWru"/>
	<skos:related rdf:resource="https://ark.frantiq.fr/ark:/26678/pcrt1SyNG9SDq7"/>
	<skos:related rdf:resource="https://ark.frantiq.fr/ark:/26678/pcrtUdAqTSVpc7"/>
	<skos:related rdf:resource="https://ark.frantiq.fr/ark:/26678/pcrt4OanARQmgf"/>
	<skos:related rdf:resource="https://ark.frantiq.fr/ark:/26678/pcrtRLO9hnk9oV"/>
	<skos:broader rdf:resource="https://ark.frantiq.fr/ark:/26678/pcrtnHxyjOkhJw"/>
	<skos:inScheme rdf:resource="https://ark.frantiq.fr/ark:/26678/TH_1"/>
	<opentheso:memberOf rdf:resource="https://ark.frantiq.fr/ark:/26678/pcrtv66rn9cbv1"/>
	<opentheso:memberOf rdf:resource="https://ark.frantiq.fr/ark:/26678/pcrtnbDLi2FkAj"/>
	<opentheso:memberOf rdf:resource="https://ark.frantiq.fr/ark:/26678/pcrtv0jq332vcq3gxt5m13d5"/>
	<skos:exactMatch rdf:resource="https://catalogue.bnf.fr/ark:/12148/cb11976008h"/>
	<skos:exactMatch rdf:resource="https://www.wikidata.org/wiki/Q287"/>
	<skos:exactMatch rdf:resource="http://vocab.getty.edu/aat/300011914"/>
	<dcterms:created rdf:datatype="http://www.w3.org/2001/XMLSchema#date">2007-02-08</dcterms:created>
	<dcterms:modified rdf:datatype="http://www.w3.org/2001/XMLSchema#date">2024-11-15</dcterms:modified>
	<dcterms:identifier>13589</dcterms:identifier>
	<dcterms:contributor>blandine.nouvel</dcterms:contributor>
	<dcterms:contributor>irene.weis</dcterms:contributor>
	<dcterms:contributor>justine.vincent</dcterms:contributor>
	<skos:definition xml:lang="en">Plant tissue corresponding to the secondary xylem, making up most of the trunk of woody plants (Wikipedia).</skos:definition>
	<skos:definition xml:lang="fr">Tissu végétal correspondant au xylème secondaire, constituant la plus grande partie du tronc des plantes ligneuses. (Wikipédia)</skos:definition>
</rdf:Description>

<rdf:Description rdf:about="https://ark.frantiq.fr/ark:/26678/pcrtI4g8pXkSSJ">
	<rdf:type rdf:resource="http://www.w3.org/2004/02/skos/core#Concept"/>
	<skos:prefLabel xml:lang="de">Bauholz</skos:prefLabel>
	<skos:prefLabel xml:lang="fr">bois d'oeuvre</skos:prefLabel>
	<skos:prefLabel xml:lang="it">legname</skos:prefLabel>
	<skos:prefLabel xml:lang="es">madera de obra</skos:prefLabel>
	<skos:prefLabel xml:lang="en">timber</skos:prefLabel>
	<skos:prefLabel xml:lang="nl">timmerhout</skos:prefLabel>
	<skos:prefLabel xml:lang="ar">خشب البناء</skos:prefLabel>
	<skos:altLabel xml:lang="fr">bois de construction</skos:altLabel>
	<skos:altLabel xml:lang="en">lumber</skos:altLabel>
	<skos:altLabel xml:lang="es">madera aserrada</skos:altLabel>
	<skos:altLabel xml:lang="es">madera para la construcción</skos:altLabel>
	<skos:related rdf:resource="https://ark.frantiq.fr/ark:/26678/pcrtMr3tb79bV8"/>
	<skos:related rdf:resource="https://ark.frantiq.fr/ark:/26678/pcrtLnVNH2ynJc"/>
	<skos:related rdf:resource="https://ark.frantiq.fr/ark:/26678/pcrtUZnNTQzQyu"/>
	<skos:related rdf:resource="https://ark.frantiq.fr/ark:/26678/crtOIK9VeDfzl"/>
	<skos:related rdf:resource="https://ark.frantiq.fr/ark:/26678/pcrtcpt47mgkbg"/>
	<skos:related rdf:resource="https://ark.frantiq.fr/ark:/26678/pcrttknrrfxbnb"/>
	<skos:broader rdf:resource="https://ark.frantiq.fr/ark:/26678/pcrtQuZiT5nYY2"/>
	<skos:inScheme rdf:resource="https://ark.frantiq.fr/ark:/26678/TH_1"/>
	<opentheso:memberOf rdf:resource="https://ark.frantiq.fr/ark:/26678/pcrtv66rn9cbv1"/>
	<opentheso:memberOf rdf:resource="https://ark.frantiq.fr/ark:/26678/pcrtnbDLi2FkAj"/>
	<opentheso:memberOf rdf:resource="https://ark.frantiq.fr/ark:/26678/pcrtv0jq332vcq3gxt5m13d5"/>
	<skos:exactMatch rdf:resource="https://www.wikidata.org/wiki/Q1370714"/>
	<skos:exactMatch rdf:resource="http://vocab.getty.edu/aat/300012785"/>
	<skos:exactMatch rdf:resource="http://vocab.getty.edu/aat/300012827"/>
	<dcterms:created rdf:datatype="http://www.w3.org/2001/XMLSchema#date">2007-02-08</dcterms:created>
	<dcterms:modified rdf:datatype="http://www.w3.org/2001/XMLSchema#date">2024-09-27</dcterms:modified>
	<dcterms:identifier>13590</dcterms:identifier>
	<dcterms:contributor>blandine.nouvel</dcterms:contributor>
	<dcterms:contributor>emmanuelle.bryas</dcterms:contributor>
	<skos:definition xml:lang="en">In the past, wood suitable for civil and naval construction; today, parts of felled trees suitable for sawing, peeling or slicing. (Lar.)</skos:definition>
	<skos:definition xml:lang="fr">Autrefois, bois propre aux constructions civiles et navales ; aujourd'hui, parties des arbres abattus aptes au sciage, au déroulage ou au tranchage. (Lar.)</skos:definition>
</rdf:Description>

<rdf:Description rdf:about="https://ark.frantiq.fr/ark:/26678/pcrtTbldUhfb1h">
	<rdf:type rdf:resource="http://www.w3.org/2004/02/skos/core#Concept"/>
	<skos:prefLabel xml:lang="es">asta de ciervo</skos:prefLabel>
	<skos:prefLabel xml:lang="fr">bois de cerf</skos:prefLabel>
	<skos:prefLabel xml:lang="it">corna di cervo</skos:prefLabel>
	<skos:prefLabel xml:lang="nl">hertengewei</skos:prefLabel>
	<skos:prefLabel xml:lang="de">Hirschgeweih</skos:prefLabel>
	<skos:prefLabel xml:lang="en">red deer antler</skos:prefLabel>
	<skos:prefLabel xml:lang="ar">قرون الأيل</skos:prefLabel>
	<skos:altLabel xml:lang="it">palchi (cervo)</skos:altLabel>
	<skos:broader rdf:resource="https://ark.frantiq.fr/ark:/26678/pcrtmmQBSGulBN"/>
	<skos:inScheme rdf:resource="https://ark.frantiq.fr/ark:/26678/TH_1"/>
	<opentheso:memberOf rdf:resource="https://ark.frantiq.fr/ark:/26678/pcrtv66rn9cbv1"/>
	<opentheso:memberOf rdf:resource="https://ark.frantiq.fr/ark:/26678/pcrtnbDLi2FkAj"/>
	<skos:exactMatch rdf:resource="https://www.wikidata.org/wiki/Q834007"/>
	<skos:exactMatch rdf:resource="http://vocab.getty.edu/aat/300395687"/>
	<dcterms:created rdf:datatype="http://www.w3.org/2001/XMLSchema#date">2007-02-08</dcterms:created>
	<dcterms:modified rdf:datatype="http://www.w3.org/2001/XMLSchema#date">2024-11-15</dcterms:modified>
	<dcterms:identifier>13591</dcterms:identifier>
	<dcterms:contributor>blandine.nouvel</dcterms:contributor>
	<dcterms:contributor>justine.vincent</dcterms:contributor>
	<skos:definition xml:lang="en">A bone formation that develops each year on the skull of a deer and falls off at the end of the growth cycle during moulting, present only in males (Averbouh, 2000).</skos:definition>
	<skos:definition xml:lang="fr">Formation osseuse se développant chaque année sur le crâne des cerf pour tomber à la fin du cycle de pousse lors de la mue, présent seulement chez le mâle (Averbouh, 2000).</skos:definition>
</rdf:Description>

<rdf:Description rdf:about="https://ark.frantiq.fr/ark:/26678/pcrtmmQBSGulBN">
	<rdf:type rdf:resource="http://www.w3.org/2004/02/skos/core#Concept"/>
	<skos:prefLabel xml:lang="en">antler</skos:prefLabel>
	<skos:prefLabel xml:lang="es">asta de cérvido</skos:prefLabel>
	<skos:prefLabel xml:lang="fr">bois de cervidé</skos:prefLabel>
	<skos:prefLabel xml:lang="it">corna di cervidi</skos:prefLabel>
	<skos:prefLabel xml:lang="nl">gewei</skos:prefLabel>
	<skos:prefLabel xml:lang="de">Geweih</skos:prefLabel>
	<skos:prefLabel xml:lang="ar">قرون أيليات</skos:prefLabel>
	<skos:altLabel xml:lang="en">deer antler</skos:altLabel>
	<skos:altLabel xml:lang="it">palchi (cervidi)</skos:altLabel>
	<skos:related rdf:resource="https://ark.frantiq.fr/ark:/26678/pcrte3arlcUhzY"/>
	<skos:related rdf:resource="https://ark.frantiq.fr/ark:/26678/pcrtg7SA6wBfLD"/>
	<skos:narrower rdf:resource="https://ark.frantiq.fr/ark:/26678/pcrtTbldUhfb1h"/>
	<skos:narrower rdf:resource="https://ark.frantiq.fr/ark:/26678/pcrtgx1nQuifPW"/>
	<skos:narrower rdf:resource="https://ark.frantiq.fr/ark:/26678/pcrt8ZW1DEoUSn"/>
	<skos:narrower rdf:resource="https://ark.frantiq.fr/ark:/26678/pcrtIDUn8EY3Bx"/>
	<skos:narrower rdf:resource="https://ark.frantiq.fr/ark:/26678/pcrtMBkRt9d0we"/>
	<skos:narrower rdf:resource="https://ark.frantiq.fr/ark:/26678/pcrtQ3dQ0kEMW9"/>
	<skos:narrower rdf:resource="https://ark.frantiq.fr/ark:/26678/pcrtvMpoEaUF3q"/>
	<skos:narrower rdf:resource="https://ark.frantiq.fr/ark:/26678/pcrtjGSMcDpz8A"/>
	<skos:narrower rdf:resource="https://ark.frantiq.fr/ark:/26678/pcrtahNd1oALhh"/>
	<skos:narrower rdf:resource="https://ark.frantiq.fr/ark:/26678/pcrtSd50sRXgiH"/>
	<skos:narrower rdf:resource="https://ark.frantiq.fr/ark:/26678/pcrtFEZaa6oTIS"/>
	<skos:narrower rdf:resource="https://ark.frantiq.fr/ark:/26678/pcrtaSs5GKhSA7"/>
	<skos:narrower rdf:resource="https://ark.frantiq.fr/ark:/26678/pcrtzJhR1OwU8P"/>
	<skos:narrower rdf:resource="https://ark.frantiq.fr/ark:/26678/pcrthKDSnMjAR9"/>
	<skos:narrower rdf:resource="https://ark.frantiq.fr/ark:/26678/pcrthu1vFbVQHO"/>
	<skos:narrower rdf:resource="https://ark.frantiq.fr/ark:/26678/pcrtgym8WF8J02"/>
	<skos:narrower rdf:resource="https://ark.frantiq.fr/ark:/26678/pcrtvmZ325vcRc"/>
	<skos:narrower rdf:resource="https://ark.frantiq.fr/ark:/26678/pcrtPkEBaAzwGn"/>
	<skos:narrower rdf:resource="https://ark.frantiq.fr/ark:/26678/pcrtMStphi4T4j"/>
	<skos:narrower rdf:resource="https://ark.frantiq.fr/ark:/26678/pcrt8brfm4pd4t"/>
	<skos:broader rdf:resource="https://ark.frantiq.fr/ark:/26678/pcrtf97bQHDGEd"/>
	<skos:inScheme rdf:resource="https://ark.frantiq.fr/ark:/26678/TH_1"/>
	<opentheso:memberOf rdf:resource="https://ark.frantiq.fr/ark:/26678/pcrtv66rn9cbv1"/>
	<opentheso:memberOf rdf:resource="https://ark.frantiq.fr/ark:/26678/pcrtnbDLi2FkAj"/>
	<skos:exactMatch rdf:resource="https://www.wikidata.org/wiki/Q834007"/>
	<skos:exactMatch rdf:resource="http://vocab.getty.edu/aat/300395687"/>
	<dcterms:created rdf:datatype="http://www.w3.org/2001/XMLSchema#date">2007-02-08</dcterms:created>
	<dcterms:modified rdf:datatype="http://www.w3.org/2001/XMLSchema#date">2023-08-02</dcterms:modified>
	<dcterms:identifier>13592</dcterms:identifier>
	<dcterms:contributor>blandine.nouvel</dcterms:contributor>
	<skos:definition xml:lang="en">Vascularised, deciduous bone organs of deer, which fall and grow back each year, used as material for artefacts.</skos:definition>
	<skos:definition xml:lang="fr">&lt;p&gt;Organes osseux vascularisés et caducs des cervidés, qui tombent et repoussent chaque année, utilisés comme matière à la confection d'artefacts.&lt;/p&gt;</skos:definition>
</rdf:Description>

<rdf:Description rdf:about="https://ark.frantiq.fr/ark:/26678/pcrtgx1nQuifPW">
	<rdf:type rdf:resource="http://www.w3.org/2004/02/skos/core#Concept"/>
	<skos:prefLabel xml:lang="es">asta de reno</skos:prefLabel>
	<skos:prefLabel xml:lang="fr">bois de renne</skos:prefLabel>
	<skos:prefLabel xml:lang="it">corna di renna</skos:prefLabel>
	<skos:prefLabel xml:lang="en">reindeer antler</skos:prefLabel>
	<skos:prefLabel xml:lang="nl">rendiergewei</skos:prefLabel>
	<skos:prefLabel xml:lang="de">Rengeweih</skos:prefLabel>
	<skos:prefLabel xml:lang="ar">قرون الرنَّة</skos:prefLabel>
	<skos:altLabel xml:lang="it">palchi (renna)</skos:altLabel>
	<skos:broader rdf:resource="https://ark.frantiq.fr/ark:/26678/pcrtmmQBSGulBN"/>
	<skos:inScheme rdf:resource="https://ark.frantiq.fr/ark:/26678/TH_1"/>
	<opentheso:memberOf rdf:resource="https://ark.frantiq.fr/ark:/26678/pcrtv66rn9cbv1"/>
	<opentheso:memberOf rdf:resource="https://ark.frantiq.fr/ark:/26678/pcrtnbDLi2FkAj"/>
	<skos:exactMatch rdf:resource="https://www.wikidata.org/wiki/Q834007"/>
	<skos:exactMatch rdf:resource="http://vocab.getty.edu/aat/300395687"/>
	<dcterms:created rdf:datatype="http://www.w3.org/2001/XMLSchema#date">2007-02-08</dcterms:created>
	<dcterms:modified rdf:datatype="http://www.w3.org/2001/XMLSchema#date">2023-08-02</dcterms:modified>
	<dcterms:identifier>13594</dcterms:identifier>
	<dcterms:contributor>blandine.nouvel</dcterms:contributor>
	<skos:definition xml:lang="en">Bone formation that develops each year on the skull of reindeer and falls off at the end of the growth cycle during moulting (Averbouh, 2000).</skos:definition>
	<skos:definition xml:lang="fr">Formation osseuse se développant chaque année sur le crâne des rennes pour tomber à la fin du cycle de pousse lors de la mue (Averbouh, 2000).</skos:definition>
</rdf:Description>

<rdf:Description rdf:about="https://ark.frantiq.fr/ark:/26678/pcrt6z097U6IUf">
	<rdf:type rdf:resource="http://www.w3.org/2004/02/skos/core#Concept"/>
	<skos:prefLabel xml:lang="es">bebida</skos:prefLabel>
	<skos:prefLabel xml:lang="it">bevanda</skos:prefLabel>
	<skos:prefLabel xml:lang="en">beverage</skos:prefLabel>
	<skos:prefLabel xml:lang="fr">boisson</skos:prefLabel>
	<skos:prefLabel xml:lang="nl">drank</skos:prefLabel>
	<skos:prefLabel xml:lang="de">Getränk</skos:prefLabel>
	<skos:prefLabel xml:lang="ar">مشروب</skos:prefLabel>
	<skos:altLabel xml:lang="en">drink</skos:altLabel>
	<skos:altLabel xml:lang="en">refreshment</skos:altLabel>
	<skos:related rdf:resource="https://ark.frantiq.fr/ark:/26678/pcrtDhyReVc4t3"/>
	<skos:related rdf:resource="https://ark.frantiq.fr/ark:/26678/crtPqi2WY4okg"/>
	<skos:related rdf:resource="https://ark.frantiq.fr/ark:/26678/pcrt6f09bbjj37"/>
	<skos:related rdf:resource="https://ark.frantiq.fr/ark:/26678/pcrtwSzUhGR8vO"/>
	<skos:narrower rdf:resource="https://ark.frantiq.fr/ark:/26678/pcrt3nBjHrcDGM"/>
	<skos:narrower rdf:resource="https://ark.frantiq.fr/ark:/26678/pcrttEcSiJ6kNe"/>
	<skos:narrower rdf:resource="https://ark.frantiq.fr/ark:/26678/pcrt3mTg9h3RFE"/>
	<skos:narrower rdf:resource="https://ark.frantiq.fr/ark:/26678/crtSfObTEvbdn"/>
	<skos:narrower rdf:resource="https://ark.frantiq.fr/ark:/26678/pcrtAWl3eAUQlA"/>
	<skos:broader rdf:resource="https://ark.frantiq.fr/ark:/26678/pcrtIMsuG0RWTs"/>
	<skos:inScheme rdf:resource="https://ark.frantiq.fr/ark:/26678/TH_1"/>
	<opentheso:memberOf rdf:resource="https://ark.frantiq.fr/ark:/26678/pcrtv66rn9cbv1"/>
	<opentheso:memberOf rdf:resource="https://ark.frantiq.fr/ark:/26678/pcrtnbDLi2FkAj"/>
	<skos:exactMatch rdf:resource="https://catalogue.bnf.fr/ark:/12148/cb119763597"/>
	<skos:exactMatch rdf:resource="https://www.wikidata.org/wiki/Q40050"/>
	<skos:exactMatch rdf:resource="http://vocab.getty.edu/aat/300389821"/>
	<dcterms:created rdf:datatype="http://www.w3.org/2001/XMLSchema#date">2007-02-08</dcterms:created>
	<dcterms:modified rdf:datatype="http://www.w3.org/2001/XMLSchema#date">2023-08-02</dcterms:modified>
	<dcterms:identifier>13596</dcterms:identifier>
	<dcterms:contributor>blandine.nouvel</dcterms:contributor>
	<skos:definition xml:lang="en">Liquid intended for consumption.</skos:definition>
	<skos:definition xml:lang="fr">Liquide destiné à la consommation.</skos:definition>
</rdf:Description>

<rdf:Description rdf:about="https://ark.frantiq.fr/ark:/26678/pcrtjzKlry0LZi">
	<rdf:type rdf:resource="http://www.w3.org/2004/02/skos/core#Concept"/>
	<skos:prefLabel xml:lang="es">bronce</skos:prefLabel>
	<skos:prefLabel xml:lang="nl">brons</skos:prefLabel>
	<skos:prefLabel xml:lang="en">bronze</skos:prefLabel>
	<skos:prefLabel xml:lang="fr">bronze</skos:prefLabel>
	<skos:prefLabel xml:lang="de">Bronze</skos:prefLabel>
	<skos:prefLabel xml:lang="it">bronzo</skos:prefLabel>
	<skos:prefLabel xml:lang="ar">برونز</skos:prefLabel>
	<skos:altLabel xml:lang="fr">airain</skos:altLabel>
	<skos:altLabel xml:lang="fr">bronze (alliage)</skos:altLabel>
	<skos:altLabel xml:lang="fr">bronze (métal)</skos:altLabel>
	<skos:related rdf:resource="https://ark.frantiq.fr/ark:/26678/pcrttls2ZeQkKE"/>
	<skos:related rdf:resource="https://ark.frantiq.fr/ark:/26678/pcrtiWltizHDZb"/>
	<skos:related rdf:resource="https://ark.frantiq.fr/ark:/26678/pcrttw20c2DxV5"/>
	<skos:related rdf:resource="https://ark.frantiq.fr/ark:/26678/pcrtibXdLTUhhT"/>
	<skos:related rdf:resource="https://ark.frantiq.fr/ark:/26678/pcrtHIT0hSPFsR"/>
	<skos:related rdf:resource="https://ark.frantiq.fr/ark:/26678/pcrtfl2epc7gJw"/>
	<skos:related rdf:resource="https://ark.frantiq.fr/ark:/26678/pcrtD8bo5lH0H4"/>
	<skos:related rdf:resource="https://ark.frantiq.fr/ark:/26678/pcrtqiiVth9tfA"/>
	<skos:related rdf:resource="https://ark.frantiq.fr/ark:/26678/crtKTYDe28wHh"/>
	<skos:related rdf:resource="https://ark.frantiq.fr/ark:/26678/crtjc88mqo6rf"/>
	<skos:related rdf:resource="https://ark.frantiq.fr/ark:/26678/pcrtproEe0mnKx"/>
	<skos:related rdf:resource="https://ark.frantiq.fr/ark:/26678/pcrt7qcjYosTs3"/>
	<skos:broader rdf:resource="https://ark.frantiq.fr/ark:/26678/pcrtzcGlM17go5"/>
	<skos:inScheme rdf:resource="https://ark.frantiq.fr/ark:/26678/TH_1"/>
	<opentheso:memberOf rdf:resource="https://ark.frantiq.fr/ark:/26678/pcrtv66rn9cbv1"/>
	<opentheso:memberOf rdf:resource="https://ark.frantiq.fr/ark:/26678/pcrtnbDLi2FkAj"/>
	<opentheso:memberOf rdf:resource="https://ark.frantiq.fr/ark:/26678/pcrtv0jq332vcq3gxt5m13d5"/>
	<skos:exactMatch rdf:resource="https://catalogue.bnf.fr/ark:/12148/cb11976193v"/>
	<skos:exactMatch rdf:resource="https://www.wikidata.org/wiki/Q34095"/>
	<skos:exactMatch rdf:resource="http://vocab.getty.edu/aat/300010957"/>
	<dcterms:created rdf:datatype="http://www.w3.org/2001/XMLSchema#date">2007-02-08</dcterms:created>
	<dcterms:modified rdf:datatype="http://www.w3.org/2001/XMLSchema#date">2024-03-21</dcterms:modified>
	<dcterms:identifier>13652</dcterms:identifier>
	<dcterms:contributor>blandine.nouvel</dcterms:contributor>
	<dcterms:contributor>irene.weis</dcterms:contributor>
	<skos:definition xml:lang="en">An alloy of copper and tin with a high copper content (usually more than 80%), which lends itself easily to shaping by casting (Larousse).</skos:definition>
	<skos:definition xml:lang="fr">Alliage de cuivre et d'étain à forte teneur en cuivre (le plus souvent supérieure à 80 %), se prêtant facilement à la mise en forme par fonderie. (Larousse)</skos:definition>
</rdf:Description>

<rdf:Description rdf:about="https://ark.frantiq.fr/ark:/26678/pcrtalmpL9IBGx">
	<rdf:type rdf:resource="http://www.w3.org/2004/02/skos/core#Concept"/>
	<skos:prefLabel xml:lang="fr">cailloutis</skos:prefLabel>
	<skos:prefLabel xml:lang="it">ghiaia</skos:prefLabel>
	<skos:prefLabel xml:lang="es">grava</skos:prefLabel>
	<skos:prefLabel xml:lang="en">gravel</skos:prefLabel>
	<skos:prefLabel xml:lang="nl">grind</skos:prefLabel>
	<skos:prefLabel xml:lang="de">Schotter</skos:prefLabel>
	<skos:prefLabel xml:lang="ar">حصى</skos:prefLabel>
	<skos:altLabel xml:lang="it">brecciame</skos:altLabel>
	<skos:altLabel xml:lang="it">breccino</skos:altLabel>
	<skos:altLabel xml:lang="en">crushed stone</skos:altLabel>
	<skos:altLabel xml:lang="en">gravel-stones</skos:altLabel>
	<skos:related rdf:resource="https://ark.frantiq.fr/ark:/26678/pcrtEklsyTYoVi"/>
	<skos:broader rdf:resource="https://ark.frantiq.fr/ark:/26678/pcrtQuZiT5nYY2"/>
	<skos:inScheme rdf:resource="https://ark.frantiq.fr/ark:/26678/TH_1"/>
	<opentheso:memberOf rdf:resource="https://ark.frantiq.fr/ark:/26678/pcrtv66rn9cbv1"/>
	<opentheso:memberOf rdf:resource="https://ark.frantiq.fr/ark:/26678/pcrtnbDLi2FkAj"/>
	<skos:exactMatch rdf:resource="https://www.wikidata.org/wiki/Q85947802"/>
	<dcterms:created rdf:datatype="http://www.w3.org/2001/XMLSchema#date">2007-02-08</dcterms:created>
	<dcterms:modified rdf:datatype="http://www.w3.org/2001/XMLSchema#date">2024-11-15</dcterms:modified>
	<dcterms:identifier>13700</dcterms:identifier>
	<dcterms:contributor>blandine.nouvel</dcterms:contributor>
	<dcterms:contributor>justine.vincent</dcterms:contributor>
	<skos:definition xml:lang="fr">Cailloux concassés pour l'empierrement des routes et des chemins. (ATLIF)</skos:definition>
	<skos:definition xml:lang="en">Crushed pebbles for gravelling roads and paths (ATLIF)</skos:definition>
</rdf:Description>

<rdf:Description rdf:about="https://ark.frantiq.fr/ark:/26678/pcrtc1Ueky7Zpg">
	<rdf:type rdf:resource="http://www.w3.org/2004/02/skos/core#Concept"/>
	<skos:prefLabel xml:lang="fr">calcaire</skos:prefLabel>
	<skos:prefLabel xml:lang="it">calcare</skos:prefLabel>
	<skos:prefLabel xml:lang="es">caliza</skos:prefLabel>
	<skos:prefLabel xml:lang="nl">kalksteen</skos:prefLabel>
	<skos:prefLabel xml:lang="de">Kalkstein</skos:prefLabel>
	<skos:prefLabel xml:lang="en">limestone</skos:prefLabel>
	<skos:prefLabel xml:lang="ar">حجر جيري</skos:prefLabel>
	<skos:altLabel xml:lang="fr">calcaire dur</skos:altLabel>
	<skos:altLabel xml:lang="es">piedra caliza</skos:altLabel>
	<skos:altLabel xml:lang="it">roccia calcarea</skos:altLabel>
	<skos:altLabel xml:lang="fr">roche calcaire</skos:altLabel>
	<skos:altLabel xml:lang="fr">roche carbonatée</skos:altLabel>
	<skos:narrower rdf:resource="https://ark.frantiq.fr/ark:/26678/pcrtyJc250eY3m"/>
	<skos:narrower rdf:resource="https://ark.frantiq.fr/ark:/26678/crt9EjSUc0WRF"/>
	<skos:narrower rdf:resource="https://ark.frantiq.fr/ark:/26678/pcrtkgSlgXZbNa"/>
	<skos:narrower rdf:resource="https://ark.frantiq.fr/ark:/26678/pcrtxn3nfsg0pd"/>
	<skos:broader rdf:resource="https://ark.frantiq.fr/ark:/26678/pcrtm4r7mvsvrw"/>
	<skos:inScheme rdf:resource="https://ark.frantiq.fr/ark:/26678/TH_1"/>
	<opentheso:memberOf rdf:resource="https://ark.frantiq.fr/ark:/26678/pcrtv66rn9cbv1"/>
	<opentheso:memberOf rdf:resource="https://ark.frantiq.fr/ark:/26678/pcrtnbDLi2FkAj"/>
	<opentheso:memberOf rdf:resource="https://ark.frantiq.fr/ark:/26678/pcrtv0jq332vcq3gxt5m13d5"/>
	<skos:exactMatch rdf:resource="https://catalogue.bnf.fr/ark:/12148/cb11938314x"/>
	<skos:exactMatch rdf:resource="https://www.wikidata.org/wiki/Q23757"/>
	<skos:exactMatch rdf:resource="http://vocab.getty.edu/aat/300011286"/>
	<dcterms:created rdf:datatype="http://www.w3.org/2001/XMLSchema#date">2007-02-08</dcterms:created>
	<dcterms:modified rdf:datatype="http://www.w3.org/2001/XMLSchema#date">2024-03-21</dcterms:modified>
	<dcterms:identifier>13704</dcterms:identifier>
	<dcterms:contributor>blandine.nouvel</dcterms:contributor>
	<dcterms:contributor>irene.weis</dcterms:contributor>
	<dcterms:contributor>justine.vincent</dcterms:contributor>
	<skos:definition xml:lang="fr">Carbonate de calcium, pur ou mélangé à d'autres minéraux ; roche à dominante de carbonate de calcium. (Lozet &amp;amp; Mathieu, Dictionnaire de science du sol. Ed. Technique et Documentation Lavoisier)</skos:definition>
</rdf:Description>

<rdf:Description rdf:about="https://ark.frantiq.fr/ark:/26678/pcrtOBWTai2Xms">
	<rdf:type rdf:resource="http://www.w3.org/2004/02/skos/core#Concept"/>
	<skos:prefLabel xml:lang="fr">calcédoine</skos:prefLabel>
	<skos:prefLabel xml:lang="es">calcedonia</skos:prefLabel>
	<skos:prefLabel xml:lang="it">calcedonio</skos:prefLabel>
	<skos:prefLabel xml:lang="nl">chalcedon</skos:prefLabel>
	<skos:prefLabel xml:lang="de">Chalcedon</skos:prefLabel>
	<skos:prefLabel xml:lang="en">chalcedony</skos:prefLabel>
	<skos:prefLabel xml:lang="ar">خَلقيدونية</skos:prefLabel>
	<skos:altLabel xml:lang="ar">حجر يمَان</skos:altLabel>
	<skos:related rdf:resource="https://ark.frantiq.fr/ark:/26678/pcrtcb7qm82cts"/>
	<skos:narrower rdf:resource="https://ark.frantiq.fr/ark:/26678/pcrtqmXRwn2Az6"/>
	<skos:narrower rdf:resource="https://ark.frantiq.fr/ark:/26678/pcrtVtHSyKSdbh"/>
	<skos:narrower rdf:resource="https://ark.frantiq.fr/ark:/26678/pcrtQAl1Zjr5KF"/>
	<skos:broader rdf:resource="https://ark.frantiq.fr/ark:/26678/pcrt4N9jrETRto"/>
	<skos:inScheme rdf:resource="https://ark.frantiq.fr/ark:/26678/TH_1"/>
	<opentheso:memberOf rdf:resource="https://ark.frantiq.fr/ark:/26678/pcrtv66rn9cbv1"/>
	<opentheso:memberOf rdf:resource="https://ark.frantiq.fr/ark:/26678/pcrtnbDLi2FkAj"/>
	<skos:exactMatch rdf:resource="https://www.wikidata.org/wiki/Q170448"/>
	<skos:exactMatch rdf:resource="http://vocab.getty.edu/aat/300011134"/>
	<dcterms:created rdf:datatype="http://www.w3.org/2001/XMLSchema#date">2007-02-08</dcterms:created>
	<dcterms:modified rdf:datatype="http://www.w3.org/2001/XMLSchema#date">2023-08-02</dcterms:modified>
	<dcterms:identifier>13706</dcterms:identifier>
	<dcterms:contributor>blandine.nouvel</dcterms:contributor>
	<skos:definition xml:lang="fr">Roche composée de cristallites de quartz, dont la taille est comprise entre 50 et 100 nm3, agencées en fibres. Il s'agit d'une phase de la silice. Elle présente plusieurs variétés utilisées en gemmologie, dont l'agate, la cornaline, le jaspe, l'onyx,... (Wikipedia)</skos:definition>
</rdf:Description>

<rdf:Description rdf:about="https://ark.frantiq.fr/ark:/26678/pcrtaJLEkei5LQ">
	<rdf:type rdf:resource="http://www.w3.org/2004/02/skos/core#Concept"/>
	<skos:prefLabel xml:lang="it">calaite</skos:prefLabel>
	<skos:prefLabel xml:lang="es">callais</skos:prefLabel>
	<skos:prefLabel xml:lang="en">callaïs</skos:prefLabel>
	<skos:prefLabel xml:lang="fr">callaïs</skos:prefLabel>
	<skos:prefLabel xml:lang="nl">callaïs</skos:prefLabel>
	<skos:prefLabel xml:lang="de">Callaïs</skos:prefLabel>
	<skos:prefLabel xml:lang="ar">يشميات</skos:prefLabel>
	<skos:altLabel xml:lang="es">callaïs</skos:altLabel>
	<skos:altLabel xml:lang="it">callaite</skos:altLabel>
	<skos:related rdf:resource="https://ark.frantiq.fr/ark:/26678/pcrtv3md53Ugxj"/>
	<skos:related rdf:resource="https://ark.frantiq.fr/ark:/26678/crtL2Kjt70xql"/>
	<skos:broader rdf:resource="https://ark.frantiq.fr/ark:/26678/pcrtJt3ZKiNEFK"/>
	<skos:inScheme rdf:resource="https://ark.frantiq.fr/ark:/26678/TH_1"/>
	<opentheso:memberOf rdf:resource="https://ark.frantiq.fr/ark:/26678/pcrtv66rn9cbv1"/>
	<opentheso:memberOf rdf:resource="https://ark.frantiq.fr/ark:/26678/pcrtnbDLi2FkAj"/>
	<skos:exactMatch rdf:resource="https://www.wikidata.org/wiki/Q1027178"/>
	<dcterms:created rdf:datatype="http://www.w3.org/2001/XMLSchema#date">2007-02-08</dcterms:created>
	<dcterms:modified rdf:datatype="http://www.w3.org/2001/XMLSchema#date">2024-03-20</dcterms:modified>
	<dcterms:identifier>13711</dcterms:identifier>
	<dcterms:contributor>blandine.nouvel</dcterms:contributor>
	<dcterms:contributor>justine.vincent</dcterms:contributor>
	<skos:definition xml:lang="fr">Minéraux verts ou bleus (&lt;span style= background-color: rgb(255, 255, 255); &gt;variscites, néphrites, turquoises ou malachites)&lt;/span&gt; utilisés pour produire des perles à la fin du Néolithique et au début de l'âge du bronze en Europe. (d'après Wikipédia)</skos:definition>
	<skos:definition xml:lang="en">Green or blue minerals (variscites, nephrites, turquoises or malachites) used to produce beads in late Neolithic and early Bronze Age Europe. (from Wikipedia)</skos:definition>
	<skos:definition xml:lang="ar">أحجار فيروزية اللون</skos:definition>
</rdf:Description>

<rdf:Description rdf:about="https://ark.frantiq.fr/ark:/26678/pcrtERMm8Q0wYw">
	<rdf:type rdf:resource="http://www.w3.org/2004/02/skos/core#Concept"/>
	<skos:prefLabel xml:lang="es">cal</skos:prefLabel>
	<skos:prefLabel xml:lang="it">calce</skos:prefLabel>
	<skos:prefLabel xml:lang="fr">chaux</skos:prefLabel>
	<skos:prefLabel xml:lang="nl">kalk</skos:prefLabel>
	<skos:prefLabel xml:lang="de">Kalk</skos:prefLabel>
	<skos:prefLabel xml:lang="en">lime</skos:prefLabel>
	<skos:prefLabel xml:lang="ar">كِلس</skos:prefLabel>
	<skos:related rdf:resource="https://ark.frantiq.fr/ark:/26678/pcrteATef2dHLg"/>
	<skos:related rdf:resource="https://ark.frantiq.fr/ark:/26678/pcrtsIGcaQ8O7x"/>
	<skos:broader rdf:resource="https://ark.frantiq.fr/ark:/26678/pcrtQuZiT5nYY2"/>
	<skos:inScheme rdf:resource="https://ark.frantiq.fr/ark:/26678/TH_1"/>
	<opentheso:memberOf rdf:resource="https://ark.frantiq.fr/ark:/26678/pcrtv66rn9cbv1"/>
	<opentheso:memberOf rdf:resource="https://ark.frantiq.fr/ark:/26678/pcrtnbDLi2FkAj"/>
	<skos:exactMatch rdf:resource="https://www.wikidata.org/wiki/Q250423"/>
	<skos:exactMatch rdf:resource="http://vocab.getty.edu/aat/300011740"/>
	<dcterms:created rdf:datatype="http://www.w3.org/2001/XMLSchema#date">2007-02-08</dcterms:created>
	<dcterms:modified rdf:datatype="http://www.w3.org/2001/XMLSchema#date">2024-11-15</dcterms:modified>
	<dcterms:identifier>13847</dcterms:identifier>
	<dcterms:contributor>blandine.nouvel</dcterms:contributor>
	<dcterms:contributor>justine.vincent</dcterms:contributor>
	<skos:definition xml:lang="en">Name given to a material obtained by burning limestone. (Wikipedia)</skos:definition>
	<skos:definition xml:lang="fr">Nom donné à une matière obtenue par combustion du calcaire. (Wikipédia)</skos:definition>
</rdf:Description>

<rdf:Description rdf:about="https://ark.frantiq.fr/ark:/26678/pcrtaOHvUS4rT6">
	<rdf:type rdf:resource="http://www.w3.org/2004/02/skos/core#Concept"/>
	<skos:prefLabel xml:lang="es">colágeno</skos:prefLabel>
	<skos:prefLabel xml:lang="nl">collageen</skos:prefLabel>
	<skos:prefLabel xml:lang="en">collagen</skos:prefLabel>
	<skos:prefLabel xml:lang="it">collagene</skos:prefLabel>
	<skos:prefLabel xml:lang="fr">collagène</skos:prefLabel>
	<skos:prefLabel xml:lang="de">Kollagen</skos:prefLabel>
	<skos:prefLabel xml:lang="ar">كولاجين</skos:prefLabel>
	<skos:broader rdf:resource="https://ark.frantiq.fr/ark:/26678/pcrtGg8L8TLNtc"/>
	<skos:inScheme rdf:resource="https://ark.frantiq.fr/ark:/26678/TH_1"/>
	<opentheso:memberOf rdf:resource="https://ark.frantiq.fr/ark:/26678/pcrtv66rn9cbv1"/>
	<opentheso:memberOf rdf:resource="https://ark.frantiq.fr/ark:/26678/pcrtnbDLi2FkAj"/>
	<skos:exactMatch rdf:resource="https://www.wikidata.org/wiki/Q26868"/>
	<skos:exactMatch rdf:resource="http://vocab.getty.edu/aat/300192948"/>
	<dcterms:created rdf:datatype="http://www.w3.org/2001/XMLSchema#date">2007-02-08</dcterms:created>
	<dcterms:modified rdf:datatype="http://www.w3.org/2001/XMLSchema#date">2023-08-02</dcterms:modified>
	<dcterms:identifier>13953</dcterms:identifier>
	<dcterms:contributor>blandine.nouvel</dcterms:contributor>
	<skos:definition xml:lang="en">Fibrous protein of connective tissue. (Le Robert)</skos:definition>
	<skos:definition xml:lang="fr">Protéine fibreuse du tissu conjonctif. (Le Robert)</skos:definition>
</rdf:Description>

<rdf:Description rdf:about="https://ark.frantiq.fr/ark:/26678/pcrtbTb5hPcQEn">
	<rdf:type rdf:resource="http://www.w3.org/2004/02/skos/core#Concept"/>
	<skos:prefLabel xml:lang="en">coiling</skos:prefLabel>
	<skos:prefLabel xml:lang="fr">colombin</skos:prefLabel>
	<skos:prefLabel xml:lang="it">colombino</skos:prefLabel>
	<skos:prefLabel xml:lang="es">enrollado</skos:prefLabel>
	<skos:prefLabel xml:lang="nl">opbouwen met kleiworsten</skos:prefLabel>
	<skos:prefLabel xml:lang="de">Wulsttechnik</skos:prefLabel>
	<skos:prefLabel xml:lang="ar">فتائل</skos:prefLabel>
	<skos:altLabel xml:lang="es">adujado</skos:altLabel>
	<skos:altLabel xml:lang="es">churros</skos:altLabel>
	<skos:altLabel xml:lang="en">coiling technique</skos:altLabel>
	<skos:altLabel xml:lang="es">colombín</skos:altLabel>
	<skos:altLabel xml:lang="it">montaggio a colombino</skos:altLabel>
	<skos:altLabel xml:lang="it">tecnica a colombino</skos:altLabel>
	<skos:related rdf:resource="https://ark.frantiq.fr/ark:/26678/pcrt9ckxv35x9x"/>
	<skos:related rdf:resource="https://ark.frantiq.fr/ark:/26678/pcrtffmf123fvr"/>
	<skos:broader rdf:resource="https://ark.frantiq.fr/ark:/26678/pcrtZETJwE7RTQ"/>
	<skos:inScheme rdf:resource="https://ark.frantiq.fr/ark:/26678/TH_1"/>
	<opentheso:memberOf rdf:resource="https://ark.frantiq.fr/ark:/26678/pcrtv66rn9cbv1"/>
	<opentheso:memberOf rdf:resource="https://ark.frantiq.fr/ark:/26678/pcrtnbDLi2FkAj"/>
	<skos:exactMatch rdf:resource="https://www.wikidata.org/wiki/Q770007"/>
	<dcterms:created rdf:datatype="http://www.w3.org/2001/XMLSchema#date">2007-02-08</dcterms:created>
	<dcterms:modified rdf:datatype="http://www.w3.org/2001/XMLSchema#date">2024-11-18</dcterms:modified>
	<dcterms:identifier>13963</dcterms:identifier>
	<dcterms:contributor>blandine.nouvel</dcterms:contributor>
	<dcterms:contributor>justine.vincent</dcterms:contributor>
	<skos:definition xml:lang="en">A lump of clay used to shape ceramics without using a wheel (Lar.)</skos:definition>
	<skos:definition xml:lang="fr">Boudin de pâte argileuse servant à façonner des céramiques sans utiliser le tour. (Lar.)</skos:definition>
	<skos:historyNote xml:lang="fr">2024-18-11 : modification de la définition.</skos:historyNote>
</rdf:Description>

<rdf:Description rdf:about="https://ark.frantiq.fr/ark:/26678/pcrtO40ZLI4giK">
	<rdf:type rdf:resource="http://www.w3.org/2004/02/skos/core#Concept"/>
	<skos:prefLabel xml:lang="nl">brandstof</skos:prefLabel>
	<skos:prefLabel xml:lang="de">Brennstoff</skos:prefLabel>
	<skos:prefLabel xml:lang="it">combustibile</skos:prefLabel>
	<skos:prefLabel xml:lang="es">combustible</skos:prefLabel>
	<skos:prefLabel xml:lang="fr">combustible</skos:prefLabel>
	<skos:prefLabel xml:lang="en">fuel</skos:prefLabel>
	<skos:prefLabel xml:lang="ar">محروقات</skos:prefLabel>
	<skos:altLabel xml:lang="fr">combustible organique</skos:altLabel>
	<skos:altLabel xml:lang="fr">matière combustible</skos:altLabel>
	<skos:related rdf:resource="https://ark.frantiq.fr/ark:/26678/pcrtMr3tb79bV8"/>
	<skos:related rdf:resource="https://ark.frantiq.fr/ark:/26678/pcrt4GtjAItlOn"/>
	<skos:related rdf:resource="https://ark.frantiq.fr/ark:/26678/pcrt9rIFPQ997Q"/>
	<skos:related rdf:resource="https://ark.frantiq.fr/ark:/26678/pcrtQhjRUa1GV8"/>
	<skos:broader rdf:resource="https://ark.frantiq.fr/ark:/26678/pcrtIMsuG0RWTs"/>
	<skos:inScheme rdf:resource="https://ark.frantiq.fr/ark:/26678/TH_1"/>
	<opentheso:memberOf rdf:resource="https://ark.frantiq.fr/ark:/26678/pcrtv66rn9cbv1"/>
	<opentheso:memberOf rdf:resource="https://ark.frantiq.fr/ark:/26678/pcrtnbDLi2FkAj"/>
	<skos:exactMatch rdf:resource="https://catalogue.bnf.fr/ark:/12148/cb119763148"/>
	<skos:exactMatch rdf:resource="https://www.wikidata.org/wiki/Q42501"/>
	<skos:exactMatch rdf:resource="http://vocab.getty.edu/aat/300015139"/>
	<dcterms:created rdf:datatype="http://www.w3.org/2001/XMLSchema#date">2007-02-08</dcterms:created>
	<dcterms:modified rdf:datatype="http://www.w3.org/2001/XMLSchema#date">2023-08-02</dcterms:modified>
	<dcterms:identifier>13988</dcterms:identifier>
	<dcterms:contributor>blandine.nouvel</dcterms:contributor>
	<skos:definition xml:lang="en">A substance that has the property of burning and releasing usable heat (CNRTL).</skos:definition>
	<skos:definition xml:lang="fr">Substance qui a la propriété d'entrer en combustion et de dégager de la chaleur utilisable (CNRTL).</skos:definition>
</rdf:Description>

<rdf:Description rdf:about="https://ark.frantiq.fr/ark:/26678/pcrtUTZqItd8SL">
	<rdf:type rdf:resource="http://www.w3.org/2004/02/skos/core#Concept"/>
	<skos:prefLabel xml:lang="en">condiment</skos:prefLabel>
	<skos:prefLabel xml:lang="fr">condiment</skos:prefLabel>
	<skos:prefLabel xml:lang="es">condimento</skos:prefLabel>
	<skos:prefLabel xml:lang="it">condimento</skos:prefLabel>
	<skos:prefLabel xml:lang="nl">specerij</skos:prefLabel>
	<skos:prefLabel xml:lang="de">Würzsauce</skos:prefLabel>
	<skos:prefLabel xml:lang="ar">بهار</skos:prefLabel>
	<skos:related rdf:resource="https://ark.frantiq.fr/ark:/26678/pcrtOGcpENB4R9"/>
	<skos:related rdf:resource="https://ark.frantiq.fr/ark:/26678/pcrttvE2YZwZu6"/>
	<skos:related rdf:resource="https://ark.frantiq.fr/ark:/26678/pcrt0TJJTrHkN1"/>
	<skos:narrower rdf:resource="https://ark.frantiq.fr/ark:/26678/pcrtsPauzzRS5z"/>
	<skos:narrower rdf:resource="https://ark.frantiq.fr/ark:/26678/pcrthmVBQESXy2"/>
	<skos:narrower rdf:resource="https://ark.frantiq.fr/ark:/26678/pcrt1wEGrR9DT3"/>
	<iso-thes:narrowerPartitive rdf:resource="https://ark.frantiq.fr/ark:/26678/pcrth6l0mevtSJ"/>
	<skos:broader rdf:resource="https://ark.frantiq.fr/ark:/26678/pcrtgcn5U8laUN"/>
	<skos:inScheme rdf:resource="https://ark.frantiq.fr/ark:/26678/TH_1"/>
	<opentheso:memberOf rdf:resource="https://ark.frantiq.fr/ark:/26678/pcrtv66rn9cbv1"/>
	<opentheso:memberOf rdf:resource="https://ark.frantiq.fr/ark:/26678/pcrtnbDLi2FkAj"/>
	<skos:exactMatch rdf:resource="https://catalogue.bnf.fr/ark:/12148/cb119364152"/>
	<skos:exactMatch rdf:resource="https://www.wikidata.org/wiki/Q2596997"/>
	<dcterms:created rdf:datatype="http://www.w3.org/2001/XMLSchema#date">2007-02-08</dcterms:created>
	<dcterms:modified rdf:datatype="http://www.w3.org/2001/XMLSchema#date">2024-03-20</dcterms:modified>
	<dcterms:identifier>14024</dcterms:identifier>
	<dcterms:contributor>blandine.nouvel</dcterms:contributor>
	<dcterms:contributor>justine.vincent</dcterms:contributor>
	<skos:definition xml:lang="en">Substance of vegetable or animal origin, intended as a seasoning, but which may also be eaten as a vegetable, which enhances the flavour of culinary preparations, particularly sauces (Wikipedia).</skos:definition>
	<skos:definition xml:lang="fr">Substance d'origine végétale ou animale, destinée à assaisonner, mais pouvant éventuellement être consommée en légume, qui relève la saveur des préparations culinaires, notamment des sauces. (Wikipedia)</skos:definition>
</rdf:Description>

<rdf:Description rdf:about="https://ark.frantiq.fr/ark:/26678/pcrtGg8L8TLNtc">
	<rdf:type rdf:resource="http://www.w3.org/2004/02/skos/core#Concept"/>
	<skos:prefLabel xml:lang="es">composición del hueso</skos:prefLabel>
	<skos:prefLabel xml:lang="fr">composition de l'os</skos:prefLabel>
	<skos:prefLabel xml:lang="en">composition of bone</skos:prefLabel>
	<skos:prefLabel xml:lang="it">costituente dell'osso</skos:prefLabel>
	<skos:prefLabel xml:lang="de">Knochenaufbau</skos:prefLabel>
	<skos:prefLabel xml:lang="nl">samenstelling van been</skos:prefLabel>
	<skos:prefLabel xml:lang="ar">مكونات العظام</skos:prefLabel>
	<skos:altLabel xml:lang="en">bone composition</skos:altLabel>
	<skos:altLabel xml:lang="fr">constituant de l'os</skos:altLabel>
	<skos:related rdf:resource="https://ark.frantiq.fr/ark:/26678/pcrtEfcf8rSZvm"/>
	<skos:narrower rdf:resource="https://ark.frantiq.fr/ark:/26678/pcrtaOHvUS4rT6"/>
	<skos:narrower rdf:resource="https://ark.frantiq.fr/ark:/26678/pcrtcyhN8uK1oY"/>
	<skos:narrower rdf:resource="https://ark.frantiq.fr/ark:/26678/pcrtZWUH1HnqXo"/>
	<skos:broader rdf:resource="https://ark.frantiq.fr/ark:/26678/pcrt448yYmVDuT"/>
	<skos:inScheme rdf:resource="https://ark.frantiq.fr/ark:/26678/TH_1"/>
	<opentheso:memberOf rdf:resource="https://ark.frantiq.fr/ark:/26678/pcrtv66rn9cbv1"/>
	<opentheso:memberOf rdf:resource="https://ark.frantiq.fr/ark:/26678/pcrtnbDLi2FkAj"/>
	<skos:exactMatch rdf:resource="https://www.wikidata.org/wiki/Q16783212"/>
	<dcterms:created rdf:datatype="http://www.w3.org/2001/XMLSchema#date">2007-02-08</dcterms:created>
	<dcterms:modified rdf:datatype="http://www.w3.org/2001/XMLSchema#date">2024-11-15</dcterms:modified>
	<dcterms:identifier>14067</dcterms:identifier>
	<dcterms:contributor>blandine.nouvel</dcterms:contributor>
	<dcterms:contributor>justine.vincent</dcterms:contributor>
	<skos:definition xml:lang="fr">Composition chimique et tissu osseu constituant un os.</skos:definition>
	<skos:definition xml:lang="en">Chemical composition and bone tissue making up a bone.</skos:definition>
	<skos:historyNote xml:lang="fr">2024-11-15 : modification de la définition.</skos:historyNote>
</rdf:Description>

<rdf:Description rdf:about="https://ark.frantiq.fr/ark:/26678/pcrtQuZiT5nYY2">
	<rdf:type rdf:resource="http://www.w3.org/2004/02/skos/core#Concept"/>
	<skos:prefLabel xml:lang="de">Baumaterialien</skos:prefLabel>
	<skos:prefLabel xml:lang="nl">bouwmaterialen</skos:prefLabel>
	<skos:prefLabel xml:lang="en">building materials</skos:prefLabel>
	<skos:prefLabel xml:lang="it">materiale da costruzione</skos:prefLabel>
	<skos:prefLabel xml:lang="es">materiales de construcción</skos:prefLabel>
	<skos:prefLabel xml:lang="fr">matériau de construction</skos:prefLabel>
	<skos:prefLabel xml:lang="ar">مواد بناء</skos:prefLabel>
	<skos:altLabel xml:lang="de">Baustoff</skos:altLabel>
	<skos:altLabel xml:lang="en">construction materials</skos:altLabel>
	<skos:altLabel xml:lang="fr">construction matériaux</skos:altLabel>
	<skos:altLabel xml:lang="es">materiales para la construcción</skos:altLabel>
	<skos:altLabel xml:lang="it">materiali da costruzione</skos:altLabel>
	<skos:altLabel xml:lang="fr">matériau de construction</skos:altLabel>
	<skos:related rdf:resource="https://ark.frantiq.fr/ark:/26678/pcrtPEkp3Yydb2"/>
	<skos:related rdf:resource="https://ark.frantiq.fr/ark:/26678/pcrtSkipOsBGML"/>
	<skos:related rdf:resource="https://ark.frantiq.fr/ark:/26678/pcrttqRMDTN4VE"/>
	<skos:related rdf:resource="https://ark.frantiq.fr/ark:/26678/crtfEfQa67rEb"/>
	<skos:related rdf:resource="https://ark.frantiq.fr/ark:/26678/crt3JnkclEfDF"/>
	<skos:related rdf:resource="https://ark.frantiq.fr/ark:/26678/pcrtXA9T44IwP1"/>
	<skos:narrower rdf:resource="https://ark.frantiq.fr/ark:/26678/pcrtI4g8pXkSSJ"/>
	<skos:narrower rdf:resource="https://ark.frantiq.fr/ark:/26678/pcrtalmpL9IBGx"/>
	<skos:narrower rdf:resource="https://ark.frantiq.fr/ark:/26678/pcrtERMm8Q0wYw"/>
	<skos:narrower rdf:resource="https://ark.frantiq.fr/ark:/26678/pcrtm6uoPROlPN"/>
	<skos:narrower rdf:resource="https://ark.frantiq.fr/ark:/26678/pcrtFxTmoqh7a3"/>
	<skos:narrower rdf:resource="https://ark.frantiq.fr/ark:/26678/pcrtEWWJvOVoh5"/>
	<skos:narrower rdf:resource="https://ark.frantiq.fr/ark:/26678/pcrtxVPISFTEr6"/>
	<skos:narrower rdf:resource="https://ark.frantiq.fr/ark:/26678/pcrt9JSk28suqb"/>
	<skos:narrower rdf:resource="https://ark.frantiq.fr/ark:/26678/pcrt4KRB12RYGv"/>
	<skos:narrower rdf:resource="https://ark.frantiq.fr/ark:/26678/pcrt6BaMGq7zE1"/>
	<skos:narrower rdf:resource="https://ark.frantiq.fr/ark:/26678/pcrtrdsp44jvsk0qqqkndb9g"/>
	<skos:broader rdf:resource="https://ark.frantiq.fr/ark:/26678/pcrtIMsuG0RWTs"/>
	<skos:inScheme rdf:resource="https://ark.frantiq.fr/ark:/26678/TH_1"/>
	<opentheso:memberOf rdf:resource="https://ark.frantiq.fr/ark:/26678/pcrtv66rn9cbv1"/>
	<opentheso:memberOf rdf:resource="https://ark.frantiq.fr/ark:/26678/pcrtnbDLi2FkAj"/>
	<skos:exactMatch rdf:resource="https://catalogue.bnf.fr/ark:/12148/cb119317804"/>
	<skos:exactMatch rdf:resource="https://www.wikidata.org/wiki/Q206615"/>
	<skos:exactMatch rdf:resource="http://vocab.getty.edu/aat/300014857"/>
	<dcterms:created rdf:datatype="http://www.w3.org/2001/XMLSchema#date">2007-02-08</dcterms:created>
	<dcterms:modified rdf:datatype="http://www.w3.org/2001/XMLSchema#date">2024-11-15</dcterms:modified>
	<dcterms:identifier>14070</dcterms:identifier>
	<dcterms:contributor>blandine.nouvel</dcterms:contributor>
	<dcterms:contributor>justine.vincent</dcterms:contributor>
	<skos:definition xml:lang="en">Natural and non-natural materials used in the construction industry.</skos:definition>
	<skos:definition xml:lang="fr">Matière d'origine naturelle ou non, utilisés dans les secteurs de la construction.</skos:definition>
	<skos:historyNote xml:lang="fr">2024-11-15 : modification de la définition.</skos:historyNote>
</rdf:Description>

<rdf:Description rdf:about="https://ark.frantiq.fr/ark:/26678/pcrtknhh7n1sa3">
	<rdf:type rdf:resource="http://www.w3.org/2004/02/skos/core#Concept"/>
	<skos:prefLabel xml:lang="fr">corail</skos:prefLabel>
	<skos:prefLabel xml:lang="en">coral</skos:prefLabel>
	<skos:prefLabel xml:lang="es">coral</skos:prefLabel>
	<skos:prefLabel xml:lang="it">corallo</skos:prefLabel>
	<skos:prefLabel xml:lang="nl">koraal</skos:prefLabel>
	<skos:prefLabel xml:lang="de">Koralle</skos:prefLabel>
	<skos:prefLabel xml:lang="el">Κοράλλι</skos:prefLabel>
	<skos:prefLabel xml:lang="ru">коралл</skos:prefLabel>
	<skos:prefLabel xml:lang="he">אלמוגים</skos:prefLabel>
	<skos:prefLabel xml:lang="ar">مرجان</skos:prefLabel>
	<skos:related rdf:resource="https://ark.frantiq.fr/ark:/26678/pcrtDoEeaZ6VcU"/>
	<skos:related rdf:resource="https://ark.frantiq.fr/ark:/26678/pcrtkjt4md8w6p"/>
	<skos:broader rdf:resource="https://ark.frantiq.fr/ark:/26678/pcrtf97bQHDGEd"/>
	<skos:inScheme rdf:resource="https://ark.frantiq.fr/ark:/26678/TH_1"/>
	<opentheso:memberOf rdf:resource="https://ark.frantiq.fr/ark:/26678/pcrtv66rn9cbv1"/>
	<opentheso:memberOf rdf:resource="https://ark.frantiq.fr/ark:/26678/pcrtnbDLi2FkAj"/>
	<skos:exactMatch rdf:resource="https://catalogue.bnf.fr/ark:/12148/cb11977101m"/>
	<skos:exactMatch rdf:resource="https://www.wikidata.org/wiki/Q171446"/>
	<skos:exactMatch rdf:resource="http://vocab.getty.edu/aat/300250925"/>
	<dcterms:created rdf:datatype="http://www.w3.org/2001/XMLSchema#date">2007-02-08</dcterms:created>
	<dcterms:modified rdf:datatype="http://www.w3.org/2001/XMLSchema#date">2024-11-15</dcterms:modified>
	<dcterms:identifier>14104</dcterms:identifier>
	<dcterms:contributor>blandine.nouvel</dcterms:contributor>
	<dcterms:contributor>justine.vincent</dcterms:contributor>
	<skos:definition xml:lang="de">koloniebildene Nesseltiere (Wikidata)</skos:definition>
	<skos:definition xml:lang="he">מחלקה של בעלי חיים חסרי חוליות ימיים המשתייכים למערכת הצורבים (Wikidata)</skos:definition>
	<skos:definition xml:lang="nl">zoölogie (Wikidata)</skos:definition>
	<skos:definition xml:lang="ru">материал скелета колонии коралловых полипов (Wikidata)</skos:definition>
	<skos:definition xml:lang="es">animal invertebrado marino que vive bajo del mar (Wikidata)</skos:definition>
	<skos:definition xml:lang="fr">Squelette d'un animal invertébré marin de l'embranchement des Cnidaires utilisé dans la joaillerie. (d'après Wikidata)</skos:definition>
	<skos:definition xml:lang="en">Skeleton of a marine invertebrate animal from the Cnidaria phylum used in jewellery (from Wikidata)</skos:definition>
</rdf:Description>

<rdf:Description rdf:about="https://ark.frantiq.fr/ark:/26678/pcrtVtHSyKSdbh">
	<rdf:type rdf:resource="http://www.w3.org/2004/02/skos/core#Concept"/>
	<skos:prefLabel xml:lang="en">carnelian</skos:prefLabel>
	<skos:prefLabel xml:lang="es">cornalina</skos:prefLabel>
	<skos:prefLabel xml:lang="fr">cornaline</skos:prefLabel>
	<skos:prefLabel xml:lang="it">corniola</skos:prefLabel>
	<skos:prefLabel xml:lang="de">Karneol</skos:prefLabel>
	<skos:prefLabel xml:lang="nl">kornalijn</skos:prefLabel>
	<skos:prefLabel xml:lang="ar">يَنَع</skos:prefLabel>
	<skos:altLabel xml:lang="es">alaqueca</skos:altLabel>
	<skos:altLabel xml:lang="es">carneola</skos:altLabel>
	<skos:altLabel xml:lang="it">cornalina</skos:altLabel>
	<skos:altLabel xml:lang="en">cornelian</skos:altLabel>
	<skos:altLabel xml:lang="ar">عقيق أحمر</skos:altLabel>
	<skos:related rdf:resource="https://ark.frantiq.fr/ark:/26678/pcrtJt3ZKiNEFK"/>
	<skos:broader rdf:resource="https://ark.frantiq.fr/ark:/26678/pcrtOBWTai2Xms"/>
	<skos:inScheme rdf:resource="https://ark.frantiq.fr/ark:/26678/TH_1"/>
	<opentheso:memberOf rdf:resource="https://ark.frantiq.fr/ark:/26678/pcrtv66rn9cbv1"/>
	<opentheso:memberOf rdf:resource="https://ark.frantiq.fr/ark:/26678/pcrtnbDLi2FkAj"/>
	<skos:exactMatch rdf:resource="https://www.wikidata.org/wiki/Q324369"/>
	<skos:exactMatch rdf:resource="http://vocab.getty.edu/aat/300133223"/>
	<dcterms:created rdf:datatype="http://www.w3.org/2001/XMLSchema#date">2007-02-08</dcterms:created>
	<dcterms:modified rdf:datatype="http://www.w3.org/2001/XMLSchema#date">2023-08-02</dcterms:modified>
	<dcterms:identifier>14109</dcterms:identifier>
	<dcterms:contributor>blandine.nouvel</dcterms:contributor>
	<skos:definition xml:lang="fr">Variété de calcédoines rouges. Elle est principalement utilisée pour la bijouterie. (wp)</skos:definition>
</rdf:Description>

<rdf:Description rdf:about="https://ark.frantiq.fr/ark:/26678/pcrtU6YoUalie6">
	<rdf:type rdf:resource="http://www.w3.org/2004/02/skos/core#Concept"/>
	<skos:prefLabel xml:lang="fr">corne (matière)</skos:prefLabel>
	<skos:prefLabel xml:lang="it">corno</skos:prefLabel>
	<skos:prefLabel xml:lang="es">cuerno</skos:prefLabel>
	<skos:prefLabel xml:lang="nl">hoorn</skos:prefLabel>
	<skos:prefLabel xml:lang="en">horn</skos:prefLabel>
	<skos:prefLabel xml:lang="de">Horn</skos:prefLabel>
	<skos:prefLabel xml:lang="ar">قرن</skos:prefLabel>
	<skos:related rdf:resource="https://ark.frantiq.fr/ark:/26678/pcrthstz3w0h8t"/>
	<skos:narrower rdf:resource="https://ark.frantiq.fr/ark:/26678/pcrtbKNE16SNWh"/>
	<skos:narrower rdf:resource="https://ark.frantiq.fr/ark:/26678/pcrt9c0c2gpn8g"/>
	<skos:broader rdf:resource="https://ark.frantiq.fr/ark:/26678/pcrtf97bQHDGEd"/>
	<skos:inScheme rdf:resource="https://ark.frantiq.fr/ark:/26678/TH_1"/>
	<opentheso:memberOf rdf:resource="https://ark.frantiq.fr/ark:/26678/pcrtv66rn9cbv1"/>
	<opentheso:memberOf rdf:resource="https://ark.frantiq.fr/ark:/26678/pcrtnbDLi2FkAj"/>
	<skos:exactMatch rdf:resource="https://www.wikidata.org/wiki/Q355445"/>
	<dcterms:created rdf:datatype="http://www.w3.org/2001/XMLSchema#date">2007-02-08</dcterms:created>
	<dcterms:modified rdf:datatype="http://www.w3.org/2001/XMLSchema#date">2024-11-15</dcterms:modified>
	<dcterms:identifier>14110</dcterms:identifier>
	<dcterms:contributor>blandine.nouvel</dcterms:contributor>
	<dcterms:contributor>justine.vincent</dcterms:contributor>
	<skos:definition xml:lang="en">Keratin-based substance that makes up animal horn (cnrtl)</skos:definition>
	<skos:definition xml:lang="fr">Substance, à base de kératine, dont est constituée la corne des animaux. (cnrtl)</skos:definition>
</rdf:Description>

<rdf:Description rdf:about="https://ark.frantiq.fr/ark:/26678/pcrtLpvrsa9RIz">
	<rdf:type rdf:resource="http://www.w3.org/2004/02/skos/core#Concept"/>
	<skos:prefLabel xml:lang="it">cosmesi</skos:prefLabel>
	<skos:prefLabel xml:lang="en">cosmetic</skos:prefLabel>
	<skos:prefLabel xml:lang="nl">cosmetica</skos:prefLabel>
	<skos:prefLabel xml:lang="es">cosmética</skos:prefLabel>
	<skos:prefLabel xml:lang="fr">cosmétique</skos:prefLabel>
	<skos:prefLabel xml:lang="de">Kosmetik</skos:prefLabel>
	<skos:prefLabel xml:lang="ar">مستحضر تجميل</skos:prefLabel>
	<skos:related rdf:resource="https://ark.frantiq.fr/ark:/26678/pcrtXiL6nBw86Y"/>
	<skos:related rdf:resource="https://ark.frantiq.fr/ark:/26678/pcrtEEqtsQiaZ3"/>
	<skos:narrower rdf:resource="https://ark.frantiq.fr/ark:/26678/pcrtZFMkWp7vRA"/>
	<skos:narrower rdf:resource="https://ark.frantiq.fr/ark:/26678/pcrtOM6tMh4qpF"/>
	<skos:broader rdf:resource="https://ark.frantiq.fr/ark:/26678/pcrtIMsuG0RWTs"/>
	<skos:inScheme rdf:resource="https://ark.frantiq.fr/ark:/26678/TH_1"/>
	<opentheso:memberOf rdf:resource="https://ark.frantiq.fr/ark:/26678/pcrtv66rn9cbv1"/>
	<opentheso:memberOf rdf:resource="https://ark.frantiq.fr/ark:/26678/pcrtnbDLi2FkAj"/>
	<skos:exactMatch rdf:resource="https://catalogue.bnf.fr/ark:/12148/cb119324153"/>
	<skos:exactMatch rdf:resource="https://www.wikidata.org/wiki/Q131207"/>
	<skos:exactMatch rdf:resource="http://vocab.getty.edu/aat/300236306"/>
	<dcterms:created rdf:datatype="http://www.w3.org/2001/XMLSchema#date">2007-02-08</dcterms:created>
	<dcterms:modified rdf:datatype="http://www.w3.org/2001/XMLSchema#date">2024-03-20</dcterms:modified>
	<dcterms:identifier>14126</dcterms:identifier>
	<dcterms:contributor>blandine.nouvel</dcterms:contributor>
	<dcterms:contributor>justine.vincent</dcterms:contributor>
	<skos:definition xml:lang="en">Substance or mixture used to maintain beauty, embellish the skin and hair (d'ap. cnrtl)</skos:definition>
	<skos:definition xml:lang="fr">Substance ou mélange qui sert à entretenir la beauté, à embellir la peau, les cheveux. (d'ap. cnrtl)</skos:definition>
</rdf:Description>

<rdf:Description rdf:about="https://ark.frantiq.fr/ark:/26678/pcrtKvRuuvDNp2">
	<rdf:type rdf:resource="http://www.w3.org/2004/02/skos/core#Concept"/>
	<skos:prefLabel xml:lang="it">arricciato</skos:prefLabel>
	<skos:prefLabel xml:lang="fr">crépi</skos:prefLabel>
	<skos:prefLabel xml:lang="es">enlucido</skos:prefLabel>
	<skos:prefLabel xml:lang="nl">pleisterkalk</skos:prefLabel>
	<skos:prefLabel xml:lang="de">Unterputz</skos:prefLabel>
	<skos:prefLabel xml:lang="en">wall plaster</skos:prefLabel>
	<skos:prefLabel xml:lang="ar">طلاء من الملاط</skos:prefLabel>
	<skos:altLabel xml:lang="it">arricciatura</skos:altLabel>
	<skos:altLabel xml:lang="it">arriccio</skos:altLabel>
	<skos:altLabel xml:lang="es">enlucido rugoso</skos:altLabel>
	<skos:altLabel xml:lang="en">roughcast</skos:altLabel>
	<skos:broader rdf:resource="https://ark.frantiq.fr/ark:/26678/pcrt4KRB12RYGv"/>
	<skos:inScheme rdf:resource="https://ark.frantiq.fr/ark:/26678/TH_1"/>
	<opentheso:memberOf rdf:resource="https://ark.frantiq.fr/ark:/26678/pcrtv66rn9cbv1"/>
	<opentheso:memberOf rdf:resource="https://ark.frantiq.fr/ark:/26678/pcrtnbDLi2FkAj"/>
	<skos:exactMatch rdf:resource="https://www.wikidata.org/wiki/Q9068497"/>
	<skos:exactMatch rdf:resource="http://www.wikidata.org/entity/Q3006287"/>
	<dcterms:created rdf:datatype="http://www.w3.org/2001/XMLSchema#date">2007-02-08</dcterms:created>
	<dcterms:modified rdf:datatype="http://www.w3.org/2001/XMLSchema#date">2023-08-02</dcterms:modified>
	<dcterms:identifier>14188</dcterms:identifier>
	<dcterms:contributor>blandine.nouvel</dcterms:contributor>
	<skos:definition xml:lang="en">A coating of mortar whipped against the walls of a structure. (Lar.)</skos:definition>
	<skos:definition xml:lang="fr">Enduit de mortier fouetté contre les parois d'un ouvrage. (Lar.)</skos:definition>
</rdf:Description>

<rdf:Description rdf:about="https://ark.frantiq.fr/ark:/26678/pcrtn5zR6bBN39">
	<rdf:type rdf:resource="http://www.w3.org/2004/02/skos/core#Concept"/>
	<skos:prefLabel xml:lang="es">cuero</skos:prefLabel>
	<skos:prefLabel xml:lang="fr">cuir</skos:prefLabel>
	<skos:prefLabel xml:lang="it">cuoio</skos:prefLabel>
	<skos:prefLabel xml:lang="en">leather</skos:prefLabel>
	<skos:prefLabel xml:lang="de">Leder</skos:prefLabel>
	<skos:prefLabel xml:lang="nl">leer</skos:prefLabel>
	<skos:prefLabel xml:lang="ar">جِلد</skos:prefLabel>
	<skos:altLabel xml:lang="en">tanned animal hide</skos:altLabel>
	<skos:related rdf:resource="https://ark.frantiq.fr/ark:/26678/pcrtJYVdVvsoOK"/>
	<skos:related rdf:resource="https://ark.frantiq.fr/ark:/26678/pcrtyBKU8jSiGp"/>
	<skos:related rdf:resource="https://ark.frantiq.fr/ark:/26678/pcrt6RVUI8RJMJ"/>
	<skos:related rdf:resource="https://ark.frantiq.fr/ark:/26678/pcrtnvdQmt8WEf"/>
	<skos:related rdf:resource="https://ark.frantiq.fr/ark:/26678/crtZFzipjOlgB"/>
	<skos:broader rdf:resource="https://ark.frantiq.fr/ark:/26678/pcrtW8Uu5SMsQy"/>
	<skos:inScheme rdf:resource="https://ark.frantiq.fr/ark:/26678/TH_1"/>
	<opentheso:memberOf rdf:resource="https://ark.frantiq.fr/ark:/26678/pcrtv66rn9cbv1"/>
	<opentheso:memberOf rdf:resource="https://ark.frantiq.fr/ark:/26678/pcrtnbDLi2FkAj"/>
	<opentheso:memberOf rdf:resource="https://ark.frantiq.fr/ark:/26678/pcrtv0jq332vcq3gxt5m13d5"/>
	<skos:exactMatch rdf:resource="https://catalogue.bnf.fr/ark:/12148/cb119766770"/>
	<skos:exactMatch rdf:resource="https://www.wikidata.org/wiki/Q286"/>
	<skos:exactMatch rdf:resource="http://vocab.getty.edu/aat/300011845"/>
	<dcterms:created rdf:datatype="http://www.w3.org/2001/XMLSchema#date">2007-02-08</dcterms:created>
	<dcterms:modified rdf:datatype="http://www.w3.org/2001/XMLSchema#date">2024-03-21</dcterms:modified>
	<dcterms:identifier>14196</dcterms:identifier>
	<dcterms:contributor>blandine.nouvel</dcterms:contributor>
	<dcterms:contributor>irene.weis</dcterms:contributor>
	<skos:definition xml:lang="en">Material prepared from the skin of an animal, mainly used in clothing and decoration in a wide variety of forms (wp)</skos:definition>
	<skos:definition xml:lang="fr">Matériau préparé à partir de la peau d'un animal, principalement utilisé dans l'habillement et la décoration sous un grand nombre de formes. (wp)</skos:definition>
</rdf:Description>

<rdf:Description rdf:about="https://ark.frantiq.fr/ark:/26678/pcrt16pnvNar4g">
	<rdf:type rdf:resource="http://www.w3.org/2004/02/skos/core#Concept"/>
	<skos:prefLabel xml:lang="es">cobre</skos:prefLabel>
	<skos:prefLabel xml:lang="en">copper</skos:prefLabel>
	<skos:prefLabel xml:lang="fr">cuivre</skos:prefLabel>
	<skos:prefLabel xml:lang="nl">koper</skos:prefLabel>
	<skos:prefLabel xml:lang="de">Kupfer</skos:prefLabel>
	<skos:prefLabel xml:lang="it">rame</skos:prefLabel>
	<skos:prefLabel xml:lang="ar">نحاس</skos:prefLabel>
	<skos:altLabel xml:lang="fr">Cu</skos:altLabel>
	<skos:altLabel xml:lang="fr">cuivre (métal)</skos:altLabel>
	<skos:related rdf:resource="https://ark.frantiq.fr/ark:/26678/crtpHLFa2qA9D"/>
	<skos:related rdf:resource="https://ark.frantiq.fr/ark:/26678/pcrt6v7rFwj0do"/>
	<skos:broader rdf:resource="https://ark.frantiq.fr/ark:/26678/pcrtkn1hAXHveS"/>
	<skos:inScheme rdf:resource="https://ark.frantiq.fr/ark:/26678/TH_1"/>
	<opentheso:memberOf rdf:resource="https://ark.frantiq.fr/ark:/26678/pcrtv66rn9cbv1"/>
	<opentheso:memberOf rdf:resource="https://ark.frantiq.fr/ark:/26678/pcrtnbDLi2FkAj"/>
	<opentheso:memberOf rdf:resource="https://ark.frantiq.fr/ark:/26678/pcrtv0jq332vcq3gxt5m13d5"/>
	<skos:exactMatch rdf:resource="https://catalogue.bnf.fr/ark:/12148/cb119470591"/>
	<skos:exactMatch rdf:resource="https://www.wikidata.org/wiki/Q753"/>
	<skos:exactMatch rdf:resource="http://vocab.getty.edu/aat/300011020"/>
	<dcterms:created rdf:datatype="http://www.w3.org/2001/XMLSchema#date">2007-02-08</dcterms:created>
	<dcterms:modified rdf:datatype="http://www.w3.org/2001/XMLSchema#date">2024-11-15</dcterms:modified>
	<dcterms:identifier>14200</dcterms:identifier>
	<dcterms:contributor>blandine.nouvel</dcterms:contributor>
	<dcterms:contributor>irene.weis</dcterms:contributor>
	<dcterms:contributor>justine.vincent</dcterms:contributor>
	<skos:definition xml:lang="en">Red-brown metal, ductile and malleable, good conductor of electricity, symbol Cu.</skos:definition>
	<skos:definition xml:lang="fr">Métal de couleur rouge-brun, ductile et malléable, bon conducteur de l'électricité, de symbole Cu. (CNRTL)</skos:definition>
	<skos:historyNote xml:lang="fr">2024-11-15 : modification de la définition</skos:historyNote>
</rdf:Description>

<rdf:Description rdf:about="https://ark.frantiq.fr/ark:/26678/pcrt1DMOWvDF4j">
	<rdf:type rdf:resource="http://www.w3.org/2004/02/skos/core#Concept"/>
	<skos:prefLabel xml:lang="it">ceramica</skos:prefLabel>
	<skos:prefLabel xml:lang="es">cerámica</skos:prefLabel>
	<skos:prefLabel xml:lang="fr">céramique (matériau)</skos:prefLabel>
	<skos:prefLabel xml:lang="nl">keramiek</skos:prefLabel>
	<skos:prefLabel xml:lang="de">Keramik</skos:prefLabel>
	<skos:prefLabel xml:lang="en">pottery</skos:prefLabel>
	<skos:prefLabel xml:lang="ar">خَزَف</skos:prefLabel>
	<skos:altLabel xml:lang="en">ceramic</skos:altLabel>
	<skos:altLabel xml:lang="en">ceramics</skos:altLabel>
	<skos:altLabel xml:lang="fr">céramique</skos:altLabel>
	<skos:altLabel xml:lang="es">vasija de cerámica</skos:altLabel>
	<skos:altLabel xml:lang="it">vaso di ceramica</skos:altLabel>
	<skos:altLabel xml:lang="en">wares</skos:altLabel>
	<skos:related rdf:resource="https://ark.frantiq.fr/ark:/26678/pcrtBOEN87D6dV"/>
	<skos:related rdf:resource="https://ark.frantiq.fr/ark:/26678/pcrtXpeIEtqsSk"/>
	<skos:related rdf:resource="https://ark.frantiq.fr/ark:/26678/crtLsb4JNRGOS"/>
	<skos:related rdf:resource="https://ark.frantiq.fr/ark:/26678/pcrtfvFEM5jWpL"/>
	<skos:related rdf:resource="https://ark.frantiq.fr/ark:/26678/pcrtfv4IrNiWE8"/>
	<skos:related rdf:resource="https://ark.frantiq.fr/ark:/26678/crt9ey83pmtqt"/>
	<skos:related rdf:resource="https://ark.frantiq.fr/ark:/26678/pcrts3pxwjw4dq"/>
	<skos:related rdf:resource="https://ark.frantiq.fr/ark:/26678/pcrtr3hwptzwvv"/>
	<skos:broader rdf:resource="https://ark.frantiq.fr/ark:/26678/pcrtfx4s0yvSLj"/>
	<skos:inScheme rdf:resource="https://ark.frantiq.fr/ark:/26678/TH_1"/>
	<opentheso:memberOf rdf:resource="https://ark.frantiq.fr/ark:/26678/pcrtv66rn9cbv1"/>
	<opentheso:memberOf rdf:resource="https://ark.frantiq.fr/ark:/26678/pcrtnbDLi2FkAj"/>
	<skos:exactMatch rdf:resource="https://catalogue.bnf.fr/ark:/12148/cb11935435f"/>
	<skos:exactMatch rdf:resource="https://www.wikidata.org/wiki/Q45621"/>
	<skos:exactMatch rdf:resource="http://vocab.getty.edu/aat/300235507"/>
	<dcterms:created rdf:datatype="http://www.w3.org/2001/XMLSchema#date">2007-02-08</dcterms:created>
	<dcterms:modified rdf:datatype="http://www.w3.org/2001/XMLSchema#date">2023-08-02</dcterms:modified>
	<dcterms:identifier>14255</dcterms:identifier>
	<dcterms:contributor>blandine.nouvel</dcterms:contributor>
	<skos:definition xml:lang="en">Material obtained by firing clay.</skos:definition>
	<skos:definition xml:lang="fr">Matériau obtenu par cuisson de l'argile.</skos:definition>
	<skos:scopeNote xml:lang="fr">&lt;p&gt;Ce concept est générique et ne concerne que le matériau et les études qui s'y attachent. Pour les objets en céramique, préférer poterie, terre cuite architecturale ou tout autre concept plus précis.&lt;/p&gt;</skos:scopeNote>
</rdf:Description>

<rdf:Description rdf:about="https://ark.frantiq.fr/ark:/26678/pcrtho8l95no0j">
	<rdf:type rdf:resource="http://www.w3.org/2004/02/skos/core#Concept"/>
	<skos:prefLabel xml:lang="es">cerámica común</skos:prefLabel>
	<skos:prefLabel xml:lang="it">ceramica comune</skos:prefLabel>
	<skos:prefLabel xml:lang="fr">céramique commune</skos:prefLabel>
	<skos:prefLabel xml:lang="en">common ware</skos:prefLabel>
	<skos:prefLabel xml:lang="de">Gebrauchsware</skos:prefLabel>
	<skos:prefLabel xml:lang="nl">gebruiksaardewerk</skos:prefLabel>
	<skos:prefLabel xml:lang="ar">خزف عام</skos:prefLabel>
	<skos:altLabel xml:lang="en">coarse pottery</skos:altLabel>
	<skos:related rdf:resource="https://ark.frantiq.fr/ark:/26678/pcrtnf5w87prg0"/>
	<skos:narrower rdf:resource="https://ark.frantiq.fr/ark:/26678/crtG26Pkhb07S"/>
	<skos:narrower rdf:resource="https://ark.frantiq.fr/ark:/26678/pcrtfkw4vc3pc5"/>
	<skos:narrower rdf:resource="https://ark.frantiq.fr/ark:/26678/pcrt5cdhzck93d"/>
	<skos:narrower rdf:resource="https://ark.frantiq.fr/ark:/26678/pcrtz14gcmpgjh"/>
	<skos:narrower rdf:resource="https://ark.frantiq.fr/ark:/26678/pcrt218fx7941b"/>
	<skos:narrower rdf:resource="https://ark.frantiq.fr/ark:/26678/pcrtvn284hkmw0"/>
	<skos:narrower rdf:resource="https://ark.frantiq.fr/ark:/26678/pcrtb1vvxk8fp3"/>
	<skos:narrower rdf:resource="https://ark.frantiq.fr/ark:/26678/pcrta0mEYU6AUY"/>
	<skos:broader rdf:resource="https://ark.frantiq.fr/ark:/26678/pcrtfx4s0yvSLj"/>
	<skos:inScheme rdf:resource="https://ark.frantiq.fr/ark:/26678/TH_1"/>
	<opentheso:memberOf rdf:resource="https://ark.frantiq.fr/ark:/26678/pcrtv66rn9cbv1"/>
	<opentheso:memberOf rdf:resource="https://ark.frantiq.fr/ark:/26678/pcrtnbDLi2FkAj"/>
	<skos:exactMatch rdf:resource="https://www.wikidata.org/wiki/Q99743238"/>
	<dcterms:created rdf:datatype="http://www.w3.org/2001/XMLSchema#date">2007-02-08</dcterms:created>
	<dcterms:modified rdf:datatype="http://www.w3.org/2001/XMLSchema#date">2024-10-18</dcterms:modified>
	<dcterms:identifier>14268</dcterms:identifier>
	<dcterms:contributor>blandine.nouvel</dcterms:contributor>
	<dcterms:contributor>justine.vincent</dcterms:contributor>
	<skos:definition xml:lang="fr">Céramique ordinaire sans vernis grésé et généralement sans décor, à pâte parfois grossière, qui peut être produite à une échelle très locale, si bien qu'il n'est pas possible de déterminer un atelier de production. &lt;span style= background-color: rgb(255, 255, 255); &gt;(Bats).&lt;/span&gt;</skos:definition>
	<skos:definition xml:lang="en">Ordinary ceramic without a grey glaze and generally without decoration, with a sometimes coarse paste, which can be produced on a very local scale, so that it is not possible to determine a production workshop (Bats).</skos:definition>
	<skos:historyNote xml:lang="fr">2024-10-18 : modification de la définition.</skos:historyNote>
</rdf:Description>

<rdf:Description rdf:about="https://ark.frantiq.fr/ark:/26678/pcrtcTqKm5ufUF">
	<rdf:type rdf:resource="http://www.w3.org/2004/02/skos/core#Concept"/>
	<skos:prefLabel xml:lang="fr">diamant</skos:prefLabel>
	<skos:prefLabel xml:lang="nl">diamant</skos:prefLabel>
	<skos:prefLabel xml:lang="de">Diamant</skos:prefLabel>
	<skos:prefLabel xml:lang="es">diamante</skos:prefLabel>
	<skos:prefLabel xml:lang="it">diamante</skos:prefLabel>
	<skos:prefLabel xml:lang="en">diamond</skos:prefLabel>
	<skos:prefLabel xml:lang="ar">ألماس</skos:prefLabel>
	<skos:related rdf:resource="https://ark.frantiq.fr/ark:/26678/pcrtbrv3wp92hn"/>
	<skos:broader rdf:resource="https://ark.frantiq.fr/ark:/26678/pcrtzVuPZeWdAP"/>
	<skos:inScheme rdf:resource="https://ark.frantiq.fr/ark:/26678/TH_1"/>
	<opentheso:memberOf rdf:resource="https://ark.frantiq.fr/ark:/26678/pcrtv66rn9cbv1"/>
	<opentheso:memberOf rdf:resource="https://ark.frantiq.fr/ark:/26678/pcrtnbDLi2FkAj"/>
	<skos:exactMatch rdf:resource="https://catalogue.bnf.fr/ark:/12148/cb12161401j"/>
	<skos:exactMatch rdf:resource="https://www.wikidata.org/wiki/Q5283"/>
	<skos:exactMatch rdf:resource="http://vocab.getty.edu/aat/300011084"/>
	<dcterms:created rdf:datatype="http://www.w3.org/2001/XMLSchema#date">2007-02-08</dcterms:created>
	<dcterms:modified rdf:datatype="http://www.w3.org/2001/XMLSchema#date">2023-08-02</dcterms:modified>
	<dcterms:identifier>14366</dcterms:identifier>
	<dcterms:contributor>blandine.nouvel</dcterms:contributor>
	<skos:definition xml:lang="en">Precious stone consisting of crystallized pure carbon, very hard but brittle, generally colourless and transparent, used either in jewellery or in industry. (Lar.)</skos:definition>
	<skos:definition xml:lang="fr">Pierre précieuse constituée de carbone pur cristallisé, très dur mais cassant, généralement incolore et transparent, utilisé soit en joaillerie, soit dans l'industrie. (Lar.)</skos:definition>
</rdf:Description>

<rdf:Description rdf:about="https://ark.frantiq.fr/ark:/26678/pcrtIxUJc35jSS">
	<rdf:type rdf:resource="http://www.w3.org/2004/02/skos/core#Concept"/>
	<skos:prefLabel xml:lang="nl">dioriet</skos:prefLabel>
	<skos:prefLabel xml:lang="de">Diorit</skos:prefLabel>
	<skos:prefLabel xml:lang="es">diorita</skos:prefLabel>
	<skos:prefLabel xml:lang="en">diorite</skos:prefLabel>
	<skos:prefLabel xml:lang="fr">diorite</skos:prefLabel>
	<skos:prefLabel xml:lang="it">diorite</skos:prefLabel>
	<skos:prefLabel xml:lang="ar">ديوريت</skos:prefLabel>
	<skos:broader rdf:resource="https://ark.frantiq.fr/ark:/26678/pcrt6BEybyEAjN"/>
	<skos:inScheme rdf:resource="https://ark.frantiq.fr/ark:/26678/TH_1"/>
	<opentheso:memberOf rdf:resource="https://ark.frantiq.fr/ark:/26678/pcrtv66rn9cbv1"/>
	<opentheso:memberOf rdf:resource="https://ark.frantiq.fr/ark:/26678/pcrtnbDLi2FkAj"/>
	<skos:exactMatch rdf:resource="https://www.wikidata.org/wiki/Q187408"/>
	<skos:exactMatch rdf:resource="http://vocab.getty.edu/aat/300011214"/>
	<dcterms:created rdf:datatype="http://www.w3.org/2001/XMLSchema#date">2007-02-08</dcterms:created>
	<dcterms:modified rdf:datatype="http://www.w3.org/2001/XMLSchema#date">2024-11-14</dcterms:modified>
	<dcterms:identifier>14390</dcterms:identifier>
	<dcterms:contributor>blandine.nouvel</dcterms:contributor>
	<dcterms:contributor>justine.vincent</dcterms:contributor>
	<skos:definition xml:lang="fr">Roche magmatique plutonique grenue contenant généralement peu de quartz (2 à 3 %), plus foncée que le granite et est composée de feldspaths, d'amphibole verte, avec un peu de biotite et parfois des pyroxènes. (Lozet &amp;amp; Mathieu, Dictionnaire de science du sol. Ed. Technique et Documentation Lavoisier)</skos:definition>
	<skos:definition xml:lang="en">Grained plutonic magmatic rock generally containing little quartz (2 to 3 %), darker than granite and composed of feldspars, green amphibole, with a little biotite and sometimes pyroxenes (Lozet &amp;amp; Mathieu, Dictionnaire de science du sol. Ed. Technique et Documentation Lavoisier)</skos:definition>
</rdf:Description>

<rdf:Description rdf:about="https://ark.frantiq.fr/ark:/26678/pcrtuxpF5YgM3S">
	<rdf:type rdf:resource="http://www.w3.org/2004/02/skos/core#Concept"/>
	<skos:prefLabel xml:lang="es">droga</skos:prefLabel>
	<skos:prefLabel xml:lang="it">droga</skos:prefLabel>
	<skos:prefLabel xml:lang="de">Droge</skos:prefLabel>
	<skos:prefLabel xml:lang="fr">drogue</skos:prefLabel>
	<skos:prefLabel xml:lang="en">drug</skos:prefLabel>
	<skos:prefLabel xml:lang="nl">drugs</skos:prefLabel>
	<skos:prefLabel xml:lang="ar">مُخَدّر</skos:prefLabel>
	<skos:related rdf:resource="https://ark.frantiq.fr/ark:/26678/pcrtRwq6H6iDlg"/>
	<skos:narrower rdf:resource="https://ark.frantiq.fr/ark:/26678/pcrt0zhHI6jOVx"/>
	<skos:narrower rdf:resource="https://ark.frantiq.fr/ark:/26678/pcrtbRoB6J1AY7"/>
	<skos:narrower rdf:resource="https://ark.frantiq.fr/ark:/26678/pcrtZ6enHsm9bu"/>
	<skos:broader rdf:resource="https://ark.frantiq.fr/ark:/26678/pcrtIMsuG0RWTs"/>
	<skos:inScheme rdf:resource="https://ark.frantiq.fr/ark:/26678/TH_1"/>
	<opentheso:memberOf rdf:resource="https://ark.frantiq.fr/ark:/26678/pcrtv66rn9cbv1"/>
	<opentheso:memberOf rdf:resource="https://ark.frantiq.fr/ark:/26678/pcrtnbDLi2FkAj"/>
	<skos:exactMatch rdf:resource="https://www.wikidata.org/wiki/Q8386"/>
	<skos:exactMatch rdf:resource="http://vocab.getty.edu/aat/300379869"/>
	<dcterms:created rdf:datatype="http://www.w3.org/2001/XMLSchema#date">2007-02-08</dcterms:created>
	<dcterms:modified rdf:datatype="http://www.w3.org/2001/XMLSchema#date">2023-08-02</dcterms:modified>
	<dcterms:identifier>14477</dcterms:identifier>
	<dcterms:contributor>blandine.nouvel</dcterms:contributor>
	<skos:definition xml:lang="en">Substance of organic or inorganic origin with physiologically active properties (sedative, soporific, aphrodisiac, lethal, etc.).</skos:definition>
	<skos:definition xml:lang="fr">Substance d'origine organique ou inorganique douée de propriétés physiologies actives (sédatives, soporifiques, aphrodisiaques, mortelles etc.) (d'ap. CNRTL)</skos:definition>
</rdf:Description>

<rdf:Description rdf:about="https://ark.frantiq.fr/ark:/26678/pcrtWANqEEARhN">
	<rdf:type rdf:resource="http://www.w3.org/2004/02/skos/core#Concept"/>
	<skos:prefLabel xml:lang="fr">dégraissant</skos:prefLabel>
	<skos:prefLabel xml:lang="es">desgrasante</skos:prefLabel>
	<skos:prefLabel xml:lang="de">Magerung</skos:prefLabel>
	<skos:prefLabel xml:lang="it">sgrassante</skos:prefLabel>
	<skos:prefLabel xml:lang="en">temper</skos:prefLabel>
	<skos:prefLabel xml:lang="nl">verschraling</skos:prefLabel>
	<skos:prefLabel xml:lang="ar">مزيل شحم</skos:prefLabel>
	<skos:altLabel xml:lang="es">desengrasante</skos:altLabel>
	<skos:related rdf:resource="https://ark.frantiq.fr/ark:/26678/pcrtr3hwptzwvv"/>
	<skos:broader rdf:resource="https://ark.frantiq.fr/ark:/26678/pcrtZETJwE7RTQ"/>
	<skos:inScheme rdf:resource="https://ark.frantiq.fr/ark:/26678/TH_1"/>
	<opentheso:memberOf rdf:resource="https://ark.frantiq.fr/ark:/26678/pcrtv66rn9cbv1"/>
	<opentheso:memberOf rdf:resource="https://ark.frantiq.fr/ark:/26678/pcrtnbDLi2FkAj"/>
	<skos:exactMatch rdf:resource="https://www.wikidata.org/wiki/Q30765541"/>
	<dcterms:created rdf:datatype="http://www.w3.org/2001/XMLSchema#date">2007-02-08</dcterms:created>
	<dcterms:modified rdf:datatype="http://www.w3.org/2001/XMLSchema#date">2024-11-18</dcterms:modified>
	<dcterms:identifier>14534</dcterms:identifier>
	<dcterms:contributor>blandine.nouvel</dcterms:contributor>
	<dcterms:contributor>justine.vincent</dcterms:contributor>
	<skos:definition xml:lang="en">A non-plastic element of very diverse nature that can be added, in the necessary and sufficient proportion, to improve the consistency of a clay that is too greasy (Balfet et al 1989, p. 49).</skos:definition>
	<skos:definition xml:lang="fr">Élément non plastique de nature très diverse qui peut être ajouté, dans la proportion nécessaire et suffisante, pour aménager la consistance d'une argile trop grasse (Balfet et al 1989, p. 49)</skos:definition>
	<dcterms:source>https://catalogue.frantiq.fr/cgi-bin/koha/opac-detail.pl?biblionumber=241203</dcterms:source>
</rdf:Description>

<rdf:Description rdf:about="https://ark.frantiq.fr/ark:/26678/pcrtJYawSTtElG">
	<rdf:type rdf:resource="http://www.w3.org/2004/02/skos/core#Concept"/>
	<skos:prefLabel xml:lang="it">acqua</skos:prefLabel>
	<skos:prefLabel xml:lang="es">agua</skos:prefLabel>
	<skos:prefLabel xml:lang="fr">eau</skos:prefLabel>
	<skos:prefLabel xml:lang="de">Wasser</skos:prefLabel>
	<skos:prefLabel xml:lang="en">water</skos:prefLabel>
	<skos:prefLabel xml:lang="nl">water</skos:prefLabel>
	<skos:prefLabel xml:lang="ar">ماء</skos:prefLabel>
	<skos:related rdf:resource="https://ark.frantiq.fr/ark:/26678/pcrthAtwVH0f7L"/>
	<skos:related rdf:resource="https://ark.frantiq.fr/ark:/26678/pcrtSKvPhI0dHJ"/>
	<skos:related rdf:resource="https://ark.frantiq.fr/ark:/26678/pcrtyT5Q4Qdi8m"/>
	<skos:related rdf:resource="https://ark.frantiq.fr/ark:/26678/crtYFci9YMvT1"/>
	<skos:related rdf:resource="https://ark.frantiq.fr/ark:/26678/crtdAX11Eumew"/>
	<skos:broader rdf:resource="https://ark.frantiq.fr/ark:/26678/pcrtx37ph91cww"/>
	<skos:inScheme rdf:resource="https://ark.frantiq.fr/ark:/26678/TH_1"/>
	<opentheso:memberOf rdf:resource="https://ark.frantiq.fr/ark:/26678/pcrtv66rn9cbv1"/>
	<opentheso:memberOf rdf:resource="https://ark.frantiq.fr/ark:/26678/pcrtnbDLi2FkAj"/>
	<skos:exactMatch rdf:resource="https://catalogue.bnf.fr/ark:/12148/cb11931913j"/>
	<skos:exactMatch rdf:resource="https://www.wikidata.org/wiki/Q283"/>
	<skos:exactMatch rdf:resource="http://vocab.getty.edu/aat/300011772"/>
	<dcterms:created rdf:datatype="http://www.w3.org/2001/XMLSchema#date">2007-02-08</dcterms:created>
	<dcterms:modified rdf:datatype="http://www.w3.org/2001/XMLSchema#date">2024-11-14</dcterms:modified>
	<dcterms:identifier>14577</dcterms:identifier>
	<dcterms:contributor>blandine.nouvel</dcterms:contributor>
	<dcterms:contributor>justine.vincent</dcterms:contributor>
	<skos:definition xml:lang="fr">Corps liquide constitué de molécules H2O.</skos:definition>
	<skos:definition xml:lang="en">Liquid body made up of H2O molecules.</skos:definition>
</rdf:Description>

<rdf:Description rdf:about="https://ark.frantiq.fr/ark:/26678/pcrto2Udjh8XSP">
	<rdf:type rdf:resource="http://www.w3.org/2004/02/skos/core#Concept"/>
	<skos:prefLabel xml:lang="fr">encens</skos:prefLabel>
	<skos:prefLabel xml:lang="en">incense</skos:prefLabel>
	<skos:prefLabel xml:lang="it">incenso</skos:prefLabel>
	<skos:prefLabel xml:lang="es">incienso</skos:prefLabel>
	<skos:prefLabel xml:lang="de">Weihrauch</skos:prefLabel>
	<skos:prefLabel xml:lang="nl">wierook</skos:prefLabel>
	<skos:prefLabel xml:lang="ar">بخُّور</skos:prefLabel>
	<skos:altLabel xml:lang="en">frankincense</skos:altLabel>
	<skos:altLabel xml:lang="en">olibanum</skos:altLabel>
	<skos:broader rdf:resource="https://ark.frantiq.fr/ark:/26678/pcrtrxL50B7yNx"/>
	<skos:inScheme rdf:resource="https://ark.frantiq.fr/ark:/26678/TH_1"/>
	<opentheso:memberOf rdf:resource="https://ark.frantiq.fr/ark:/26678/pcrtv66rn9cbv1"/>
	<opentheso:memberOf rdf:resource="https://ark.frantiq.fr/ark:/26678/pcrtnbDLi2FkAj"/>
	<skos:exactMatch rdf:resource="https://catalogue.bnf.fr/ark:/12148/cb120448144"/>
	<skos:exactMatch rdf:resource="https://www.wikidata.org/wiki/Q173486"/>
	<skos:exactMatch rdf:resource="https://www.wikidata.org/wiki/Q273131"/>
	<skos:exactMatch rdf:resource="http://vocab.getty.edu/aat/300380405"/>
	<dcterms:created rdf:datatype="http://www.w3.org/2001/XMLSchema#date">2007-02-08</dcterms:created>
	<dcterms:modified rdf:datatype="http://www.w3.org/2001/XMLSchema#date">2023-08-02</dcterms:modified>
	<dcterms:identifier>14597</dcterms:identifier>
	<dcterms:contributor>blandine.nouvel</dcterms:contributor>
	<skos:definition xml:lang="en">Aromatic resin from boswalia (Lar.)</skos:definition>
	<skos:definition xml:lang="fr">Résine aromatique tirée du boswalia (Lar.)</skos:definition>
</rdf:Description>

<rdf:Description rdf:about="https://ark.frantiq.fr/ark:/26678/pcrtXgoFDoG7xA">
	<rdf:type rdf:resource="http://www.w3.org/2004/02/skos/core#Concept"/>
	<skos:prefLabel xml:lang="es">engobe</skos:prefLabel>
	<skos:prefLabel xml:lang="fr">engobe</skos:prefLabel>
	<skos:prefLabel xml:lang="it">ingobbio</skos:prefLabel>
	<skos:prefLabel xml:lang="de">Schlicküberzug</skos:prefLabel>
	<skos:prefLabel xml:lang="nl">slib</skos:prefLabel>
	<skos:prefLabel xml:lang="en">slip</skos:prefLabel>
	<skos:prefLabel xml:lang="ar">غُضار</skos:prefLabel>
	<skos:altLabel xml:lang="es">engobado</skos:altLabel>
	<skos:altLabel xml:lang="de">Engobe</skos:altLabel>
	<skos:altLabel xml:lang="it">ingubbiatura</skos:altLabel>
	<skos:related rdf:resource="https://ark.frantiq.fr/ark:/26678/pcrth5xszphkw6"/>
	<skos:related rdf:resource="https://ark.frantiq.fr/ark:/26678/pcrt518w0nr5tf"/>
	<skos:broader rdf:resource="https://ark.frantiq.fr/ark:/26678/pcrtZETJwE7RTQ"/>
	<skos:inScheme rdf:resource="https://ark.frantiq.fr/ark:/26678/TH_1"/>
	<opentheso:memberOf rdf:resource="https://ark.frantiq.fr/ark:/26678/pcrtv66rn9cbv1"/>
	<opentheso:memberOf rdf:resource="https://ark.frantiq.fr/ark:/26678/pcrtnbDLi2FkAj"/>
	<skos:exactMatch rdf:resource="https://www.wikidata.org/wiki/Q60310"/>
	<skos:exactMatch rdf:resource="http://vocab.getty.edu/aat/300015111"/>
	<skos:exactMatch rdf:resource="http://vocab.getty.edu/aat/300264955"/>
	<dcterms:created rdf:datatype="http://www.w3.org/2001/XMLSchema#date">2007-02-08</dcterms:created>
	<dcterms:modified rdf:datatype="http://www.w3.org/2001/XMLSchema#date">2023-08-02</dcterms:modified>
	<dcterms:identifier>14614</dcterms:identifier>
	<dcterms:contributor>blandine.nouvel</dcterms:contributor>
	<skos:definition xml:lang="en">Earthy coating (clay type) made of slip, applied to the surface of the vase to unify its appearance or give it a different colour from that of the paste (Yon 1981, p. 83).</skos:definition>
	<skos:definition xml:lang="fr">Revêtement de nature terreuse (type argileux) fait de barbotine, étendu à la surface du vase pour unifier son aspect, ou lui donner une coloration différente de celle de la pâte (Yon 1981, p. 83).</skos:definition>
</rdf:Description>

<rdf:Description rdf:about="https://ark.frantiq.fr/ark:/26678/pcrtZFMkWp7vRA">
	<rdf:type rdf:resource="http://www.w3.org/2004/02/skos/core#Concept"/>
	<skos:prefLabel xml:lang="fr">fard</skos:prefLabel>
	<skos:prefLabel xml:lang="it">fard</skos:prefLabel>
	<skos:prefLabel xml:lang="nl">make-up</skos:prefLabel>
	<skos:prefLabel xml:lang="en">rouge (cosmetics)</skos:prefLabel>
	<skos:prefLabel xml:lang="es">rubor</skos:prefLabel>
	<skos:prefLabel xml:lang="de">Schminke</skos:prefLabel>
	<skos:prefLabel xml:lang="ar">مسحوق تجميل</skos:prefLabel>
	<skos:altLabel xml:lang="it">belletto</skos:altLabel>
	<skos:altLabel xml:lang="en">blush</skos:altLabel>
	<skos:altLabel xml:lang="it">blush</skos:altLabel>
	<skos:altLabel xml:lang="en">blusher</skos:altLabel>
	<skos:altLabel xml:lang="fr">maquillage</skos:altLabel>
	<skos:altLabel xml:lang="es">maquillaje</skos:altLabel>
	<skos:related rdf:resource="https://ark.frantiq.fr/ark:/26678/pcrterNa8OcooH"/>
	<skos:broader rdf:resource="https://ark.frantiq.fr/ark:/26678/pcrtLpvrsa9RIz"/>
	<skos:inScheme rdf:resource="https://ark.frantiq.fr/ark:/26678/TH_1"/>
	<opentheso:memberOf rdf:resource="https://ark.frantiq.fr/ark:/26678/pcrtv66rn9cbv1"/>
	<opentheso:memberOf rdf:resource="https://ark.frantiq.fr/ark:/26678/pcrtnbDLi2FkAj"/>
	<skos:exactMatch rdf:resource="https://www.wikidata.org/wiki/Q181791"/>
	<dcterms:created rdf:datatype="http://www.w3.org/2001/XMLSchema#date">2007-02-08</dcterms:created>
	<dcterms:modified rdf:datatype="http://www.w3.org/2001/XMLSchema#date">2024-03-20</dcterms:modified>
	<dcterms:identifier>14710</dcterms:identifier>
	<dcterms:contributor>blandine.nouvel</dcterms:contributor>
	<dcterms:contributor>justine.vincent</dcterms:contributor>
	<skos:definition xml:lang="en">Coloured product applied to different parts of the face to enhance radiance. (cnrtl)</skos:definition>
	<skos:definition xml:lang="fr">Produit coloré qu'on applique sur différentes parties du visage pour en rehausser l'éclat. (cnrtl)</skos:definition>
</rdf:Description>

<rdf:Description rdf:about="https://ark.frantiq.fr/ark:/26678/pcrtqHWkorsw9D">
	<rdf:type rdf:resource="http://www.w3.org/2004/02/skos/core#Concept"/>
	<skos:prefLabel xml:lang="it">faenza</skos:prefLabel>
	<skos:prefLabel xml:lang="en">faience</skos:prefLabel>
	<skos:prefLabel xml:lang="fr">faïence</skos:prefLabel>
	<skos:prefLabel xml:lang="nl">faïence</skos:prefLabel>
	<skos:prefLabel xml:lang="es">fayenza</skos:prefLabel>
	<skos:prefLabel xml:lang="de">Steingut</skos:prefLabel>
	<skos:prefLabel xml:lang="ar">خزف</skos:prefLabel>
	<skos:altLabel xml:lang="en">earthenware</skos:altLabel>
	<skos:altLabel xml:lang="en">faïence</skos:altLabel>
	<skos:altLabel xml:lang="it">faïence</skos:altLabel>
	<skos:altLabel xml:lang="de">Fayence</skos:altLabel>
	<skos:altLabel xml:lang="es">loza</skos:altLabel>
	<skos:altLabel xml:lang="en">tin-glazed pottery</skos:altLabel>
	<skos:related rdf:resource="https://ark.frantiq.fr/ark:/26678/crtlNOi426s1G"/>
	<skos:related rdf:resource="https://ark.frantiq.fr/ark:/26678/pcrtaUOSeoPg5g"/>
	<skos:related rdf:resource="https://ark.frantiq.fr/ark:/26678/crtGFMtrhpRr0"/>
	<skos:related rdf:resource="https://ark.frantiq.fr/ark:/26678/pcrtf7hn86pq11"/>
	<skos:related rdf:resource="https://ark.frantiq.fr/ark:/26678/pcrtSdKu9rjDHO"/>
	<skos:related rdf:resource="https://ark.frantiq.fr/ark:/26678/pcrttazviSjfSr"/>
	<skos:related rdf:resource="https://ark.frantiq.fr/ark:/26678/pcrtgGqgGtQqYs"/>
	<skos:broader rdf:resource="https://ark.frantiq.fr/ark:/26678/pcrtfx4s0yvSLj"/>
	<skos:inScheme rdf:resource="https://ark.frantiq.fr/ark:/26678/TH_1"/>
	<opentheso:memberOf rdf:resource="https://ark.frantiq.fr/ark:/26678/pcrtv66rn9cbv1"/>
	<opentheso:memberOf rdf:resource="https://ark.frantiq.fr/ark:/26678/pcrtnbDLi2FkAj"/>
	<skos:closeMatch rdf:resource="https://ark.mom.fr/ark:/39676/bibp721vgd1px"/>
	<skos:exactMatch rdf:resource="https://www.wikidata.org/wiki/Q209671"/>
	<skos:exactMatch rdf:resource="http://vocab.getty.edu/aat/300010668"/>
	<dcterms:created rdf:datatype="http://www.w3.org/2001/XMLSchema#date">2007-02-08</dcterms:created>
	<dcterms:modified rdf:datatype="http://www.w3.org/2001/XMLSchema#date">2023-08-02</dcterms:modified>
	<dcterms:identifier>14722</dcterms:identifier>
	<dcterms:contributor>blandine.nouvel</dcterms:contributor>
	<skos:definition xml:lang="en">Pottery with an unglazed body covered with a glaze that makes it impermeable (Balfet et al.).</skos:definition>
	<skos:definition xml:lang="fr">Poterie à pâte non vitrifiée recouverte d'un émail qui la rend imperméable (Pour la normalisation de la description des poteries / Balfet et al.).</skos:definition>
	<skos:scopeNote xml:lang="fr">Utiliser pour la faïence  historique  :  terre cuite-traditionnelle à base d'argile, travaillée, cuite et décorée d'une glaçure plombifère opacifiée à l'oxyde d'étain . (Définition technique de la faïence / A. Boquillon, A. Caubet et G. Pierrat-Bonnefois in : les Dossiers d'archéologie n°304, 2005)</skos:scopeNote>
</rdf:Description>

<rdf:Description rdf:about="https://ark.frantiq.fr/ark:/26678/pcrtJWWucnutA0">
	<rdf:type rdf:resource="http://www.w3.org/2004/02/skos/core#Concept"/>
	<skos:prefLabel xml:lang="de">Eisen</skos:prefLabel>
	<skos:prefLabel xml:lang="fr">fer</skos:prefLabel>
	<skos:prefLabel xml:lang="it">ferro</skos:prefLabel>
	<skos:prefLabel xml:lang="es">hierro</skos:prefLabel>
	<skos:prefLabel xml:lang="nl">ijzer</skos:prefLabel>
	<skos:prefLabel xml:lang="en">iron</skos:prefLabel>
	<skos:prefLabel xml:lang="ar">حديد</skos:prefLabel>
	<skos:related rdf:resource="https://ark.frantiq.fr/ark:/26678/pcrt2vSqFSVOQc"/>
	<skos:related rdf:resource="https://ark.frantiq.fr/ark:/26678/crtKNeKtNHY3c"/>
	<skos:broader rdf:resource="https://ark.frantiq.fr/ark:/26678/pcrtkn1hAXHveS"/>
	<skos:inScheme rdf:resource="https://ark.frantiq.fr/ark:/26678/TH_1"/>
	<opentheso:memberOf rdf:resource="https://ark.frantiq.fr/ark:/26678/pcrtv66rn9cbv1"/>
	<opentheso:memberOf rdf:resource="https://ark.frantiq.fr/ark:/26678/pcrtnbDLi2FkAj"/>
	<opentheso:memberOf rdf:resource="https://ark.frantiq.fr/ark:/26678/pcrtv0jq332vcq3gxt5m13d5"/>
	<skos:exactMatch rdf:resource="https://catalogue.bnf.fr/ark:/12148/cb11975665r"/>
	<skos:exactMatch rdf:resource="https://www.wikidata.org/wiki/Q677"/>
	<skos:exactMatch rdf:resource="http://vocab.getty.edu/aat/300011002"/>
	<dcterms:created rdf:datatype="http://www.w3.org/2001/XMLSchema#date">2007-02-08</dcterms:created>
	<dcterms:modified rdf:datatype="http://www.w3.org/2001/XMLSchema#date">2024-03-21</dcterms:modified>
	<dcterms:identifier>14726</dcterms:identifier>
	<dcterms:contributor>blandine.nouvel</dcterms:contributor>
	<dcterms:contributor>irene.weis</dcterms:contributor>
	<skos:definition xml:lang="en">Strong, greyish-white, magnetic, ductile and malleable metal, rarely used in its pure state, with atomic number 26 and symbol Fe.</skos:definition>
	<skos:definition xml:lang="fr">Métal résistant, d'un blanc grisâtre, magnétique, ductile et malléable, très peu utilisé à l'état pur, de numéro atomique 26 et de symbole Fe. (TLFi)</skos:definition>
</rdf:Description>

<rdf:Description rdf:about="https://ark.frantiq.fr/ark:/26678/pcrtTcvLDTNT86">
	<rdf:type rdf:resource="http://www.w3.org/2004/02/skos/core#Concept"/>
	<skos:prefLabel xml:lang="en">cast iron</skos:prefLabel>
	<skos:prefLabel xml:lang="fr">fonte</skos:prefLabel>
	<skos:prefLabel xml:lang="es">fundición</skos:prefLabel>
	<skos:prefLabel xml:lang="it">ghisa</skos:prefLabel>
	<skos:prefLabel xml:lang="nl">het smelten</skos:prefLabel>
	<skos:prefLabel xml:lang="de">Schmelzverfahren</skos:prefLabel>
	<skos:prefLabel xml:lang="ar">صَهر</skos:prefLabel>
	<skos:altLabel xml:lang="es">fundición gris</skos:altLabel>
	<skos:altLabel xml:lang="es">hierro colado</skos:altLabel>
	<skos:altLabel xml:lang="es">hierro fundido</skos:altLabel>
	<skos:broader rdf:resource="https://ark.frantiq.fr/ark:/26678/pcrtzcGlM17go5"/>
	<skos:inScheme rdf:resource="https://ark.frantiq.fr/ark:/26678/TH_1"/>
	<opentheso:memberOf rdf:resource="https://ark.frantiq.fr/ark:/26678/pcrtv66rn9cbv1"/>
	<opentheso:memberOf rdf:resource="https://ark.frantiq.fr/ark:/26678/pcrtnbDLi2FkAj"/>
	<skos:exactMatch rdf:resource="https://catalogue.bnf.fr/ark:/12148/cb124049179"/>
	<skos:exactMatch rdf:resource="https://www.wikidata.org/wiki/Q106080"/>
	<skos:exactMatch rdf:resource="https://www.wikidata.org/wiki/Q483269"/>
	<skos:exactMatch rdf:resource="http://vocab.getty.edu/aat/300053891"/>
	<dcterms:created rdf:datatype="http://www.w3.org/2001/XMLSchema#date">2007-02-08</dcterms:created>
	<dcterms:modified rdf:datatype="http://www.w3.org/2001/XMLSchema#date">2024-11-15</dcterms:modified>
	<dcterms:identifier>14790</dcterms:identifier>
	<dcterms:contributor>blandine.nouvel</dcterms:contributor>
	<dcterms:contributor>justine.vincent</dcterms:contributor>
	<skos:definition xml:lang="en">Alloy of iron and carbon.</skos:definition>
	<skos:definition xml:lang="fr">Alliage de fer et de carbone.</skos:definition>
</rdf:Description>

<rdf:Description rdf:about="https://ark.frantiq.fr/ark:/26678/pcrtVWVfmfl1T2">
	<rdf:type rdf:resource="http://www.w3.org/2004/02/skos/core#Concept"/>
	<skos:prefLabel xml:lang="en">cheese</skos:prefLabel>
	<skos:prefLabel xml:lang="it">formaggio</skos:prefLabel>
	<skos:prefLabel xml:lang="fr">fromage</skos:prefLabel>
	<skos:prefLabel xml:lang="nl">kaas</skos:prefLabel>
	<skos:prefLabel xml:lang="de">Käse</skos:prefLabel>
	<skos:prefLabel xml:lang="es">queso</skos:prefLabel>
	<skos:prefLabel xml:lang="ar">جبن</skos:prefLabel>
	<skos:broader rdf:resource="https://ark.frantiq.fr/ark:/26678/pcrtgcn5U8laUN"/>
	<skos:inScheme rdf:resource="https://ark.frantiq.fr/ark:/26678/TH_1"/>
	<opentheso:memberOf rdf:resource="https://ark.frantiq.fr/ark:/26678/pcrtv66rn9cbv1"/>
	<opentheso:memberOf rdf:resource="https://ark.frantiq.fr/ark:/26678/pcrtnbDLi2FkAj"/>
	<skos:exactMatch rdf:resource="https://catalogue.bnf.fr/ark:/12148/cb119348746"/>
	<skos:exactMatch rdf:resource="https://www.wikidata.org/wiki/Q10943"/>
	<skos:exactMatch rdf:resource="http://vocab.getty.edu/aat/300390514"/>
	<dcterms:created rdf:datatype="http://www.w3.org/2001/XMLSchema#date">2007-02-08</dcterms:created>
	<dcterms:modified rdf:datatype="http://www.w3.org/2001/XMLSchema#date">2023-08-02</dcterms:modified>
	<dcterms:identifier>14837</dcterms:identifier>
	<dcterms:contributor>blandine.nouvel</dcterms:contributor>
	<skos:definition xml:lang="en">Food obtained from dairy products.</skos:definition>
	<skos:definition xml:lang="fr">Aliment obtenu à partir de produits laitiers.</skos:definition>
</rdf:Description>

<rdf:Description rdf:about="https://ark.frantiq.fr/ark:/26678/pcrtTgttY2SfBr">
	<rdf:type rdf:resource="http://www.w3.org/2004/02/skos/core#Concept"/>
	<skos:prefLabel xml:lang="es">canto</skos:prefLabel>
	<skos:prefLabel xml:lang="it">ciottolo</skos:prefLabel>
	<skos:prefLabel xml:lang="fr">galet</skos:prefLabel>
	<skos:prefLabel xml:lang="nl">kei</skos:prefLabel>
	<skos:prefLabel xml:lang="en">pebble</skos:prefLabel>
	<skos:prefLabel xml:lang="de">Pebble</skos:prefLabel>
	<skos:prefLabel xml:lang="ar">حصاة ملساء</skos:prefLabel>
	<skos:altLabel xml:lang="es">canto rodado</skos:altLabel>
	<skos:altLabel xml:lang="de">Geröll</skos:altLabel>
	<skos:altLabel xml:lang="es">guijarro</skos:altLabel>
	<skos:altLabel xml:lang="de">Kiesel</skos:altLabel>
	<skos:related rdf:resource="https://ark.frantiq.fr/ark:/26678/pcrtpjw26EaVTa"/>
	<skos:related rdf:resource="https://ark.frantiq.fr/ark:/26678/pcrta8Bnn8iMwS"/>
	<skos:related rdf:resource="https://ark.frantiq.fr/ark:/26678/pcrtGO1i0Db49w"/>
	<skos:related rdf:resource="https://ark.frantiq.fr/ark:/26678/pcrt0hkf0dk6st"/>
	<skos:narrower rdf:resource="https://ark.frantiq.fr/ark:/26678/pcrtf4mt37h0q8"/>
	<skos:narrower rdf:resource="https://ark.frantiq.fr/ark:/26678/pcrt6867pw8dnx"/>
	<skos:narrower rdf:resource="https://ark.frantiq.fr/ark:/26678/pcrtrsjrghq6f8"/>
	<skos:broader rdf:resource="https://ark.frantiq.fr/ark:/26678/pcrtw8nqd0wpmc"/>
	<skos:inScheme rdf:resource="https://ark.frantiq.fr/ark:/26678/TH_1"/>
	<opentheso:memberOf rdf:resource="https://ark.frantiq.fr/ark:/26678/pcrtv66rn9cbv1"/>
	<opentheso:memberOf rdf:resource="https://ark.frantiq.fr/ark:/26678/pcrtnbDLi2FkAj"/>
	<opentheso:memberOf rdf:resource="https://ark.frantiq.fr/ark:/26678/pcrtv0jq332vcq3gxt5m13d5"/>
	<skos:exactMatch rdf:resource="https://www.wikidata.org/wiki/Q14673"/>
	<skos:exactMatch rdf:resource="http://vocab.getty.edu/aat/300011691"/>
	<dcterms:created rdf:datatype="http://www.w3.org/2001/XMLSchema#date">2007-02-08</dcterms:created>
	<dcterms:modified rdf:datatype="http://www.w3.org/2001/XMLSchema#date">2024-11-19</dcterms:modified>
	<dcterms:identifier>14858</dcterms:identifier>
	<dcterms:contributor>blandine.nouvel</dcterms:contributor>
	<dcterms:contributor>irene.weis</dcterms:contributor>
	<dcterms:contributor>justine.vincent</dcterms:contributor>
	<skos:definition xml:lang="fr">Fragment de roche arrondi par usure mécanique, éolienne, fluviatile, marine ou glaciaire et pouvant servir de matière première à de nombreuses industries lithiques pour le débitage ou pour la confection de galets aménagés (percuteur ou enclume). (d'après La préhistoire)</skos:definition>
	<skos:definition xml:lang="en">A fragment of rock rounded by mechanical, eolian, fluvial, marine or glacial wear and tear that can be used as raw material in many lithic industries for cutting or for making fitted pebbles (striker or anvil). (from La préhistoire)</skos:definition>
</rdf:Description>

<rdf:Description rdf:about="https://ark.frantiq.fr/ark:/26678/pcrtDISmiAdvys">
	<rdf:type rdf:resource="http://www.w3.org/2004/02/skos/core#Concept"/>
	<skos:prefLabel xml:lang="de">Bleiglanz</skos:prefLabel>
	<skos:prefLabel xml:lang="en">galena</skos:prefLabel>
	<skos:prefLabel xml:lang="es">galena</skos:prefLabel>
	<skos:prefLabel xml:lang="it">galena</skos:prefLabel>
	<skos:prefLabel xml:lang="fr">galène</skos:prefLabel>
	<skos:prefLabel xml:lang="nl">loodglans</skos:prefLabel>
	<skos:prefLabel xml:lang="ar">كبريت الرصاص</skos:prefLabel>
	<skos:altLabel xml:lang="de">Galenit</skos:altLabel>
	<skos:altLabel xml:lang="en">lead glance</skos:altLabel>
	<skos:related rdf:resource="https://ark.frantiq.fr/ark:/26678/pcrt5bIL1UtwcT"/>
	<skos:broader rdf:resource="https://ark.frantiq.fr/ark:/26678/pcrty2mcsksa6s"/>
	<skos:inScheme rdf:resource="https://ark.frantiq.fr/ark:/26678/TH_1"/>
	<opentheso:memberOf rdf:resource="https://ark.frantiq.fr/ark:/26678/pcrtv66rn9cbv1"/>
	<opentheso:memberOf rdf:resource="https://ark.frantiq.fr/ark:/26678/pcrtnbDLi2FkAj"/>
	<skos:exactMatch rdf:resource="https://catalogue.bnf.fr/ark:/12148/cb124829509"/>
	<skos:exactMatch rdf:resource="https://www.wikidata.org/wiki/Q37559"/>
	<skos:exactMatch rdf:resource="http://vocab.getty.edu/aat/300266177"/>
	<dcterms:created rdf:datatype="http://www.w3.org/2001/XMLSchema#date">2007-02-08</dcterms:created>
	<dcterms:modified rdf:datatype="http://www.w3.org/2001/XMLSchema#date">2023-08-02</dcterms:modified>
	<dcterms:identifier>14862</dcterms:identifier>
	<dcterms:contributor>blandine.nouvel</dcterms:contributor>
	<skos:definition xml:lang="en">Lead sulphide crystallising in the cubic system (Wikipedia, 2021)</skos:definition>
	<skos:definition xml:lang="fr">Sulfure de plomb cristallisant dans le système cubique (Wikipedia, 2021)</skos:definition>
</rdf:Description>

<rdf:Description rdf:about="https://ark.frantiq.fr/ark:/26678/pcrth6l0mevtSJ">
	<rdf:type rdf:resource="http://www.w3.org/2004/02/skos/core#Concept"/>
	<skos:prefLabel xml:lang="es">garo</skos:prefLabel>
	<skos:prefLabel xml:lang="en">garum</skos:prefLabel>
	<skos:prefLabel xml:lang="fr">garum</skos:prefLabel>
	<skos:prefLabel xml:lang="it">garum</skos:prefLabel>
	<skos:prefLabel xml:lang="nl">garum</skos:prefLabel>
	<skos:prefLabel xml:lang="de">Garum</skos:prefLabel>
	<skos:prefLabel xml:lang="ar">صلصة سمك مُمَلّح</skos:prefLabel>
	<skos:altLabel xml:lang="en">liquamen</skos:altLabel>
	<skos:altLabel xml:lang="fr">liquamen</skos:altLabel>
	<skos:altLabel xml:lang="de">Liquamen</skos:altLabel>
	<iso-thes:broaderPartitive rdf:resource="https://ark.frantiq.fr/ark:/26678/pcrtUTZqItd8SL"/>
	<skos:inScheme rdf:resource="https://ark.frantiq.fr/ark:/26678/TH_1"/>
	<opentheso:memberOf rdf:resource="https://ark.frantiq.fr/ark:/26678/pcrtv66rn9cbv1"/>
	<opentheso:memberOf rdf:resource="https://ark.frantiq.fr/ark:/26678/pcrtnbDLi2FkAj"/>
	<skos:exactMatch rdf:resource="https://www.wikidata.org/wiki/Q950470"/>
	<dcterms:created rdf:datatype="http://www.w3.org/2001/XMLSchema#date">2007-02-08</dcterms:created>
	<dcterms:modified rdf:datatype="http://www.w3.org/2001/XMLSchema#date">2024-03-20</dcterms:modified>
	<dcterms:identifier>14865</dcterms:identifier>
	<dcterms:contributor>blandine.nouvel</dcterms:contributor>
	<dcterms:contributor>justine.vincent</dcterms:contributor>
	<skos:definition xml:lang="fr">Sauce composée de chair ou de viscères de poisson, voire d'huîtres, ayant fermenté longtemps dans une forte quantité de sel. (Wikipedia)</skos:definition>
	<skos:definition xml:lang="en">A sauce made from the flesh or viscera of fish, or even oysters, fermented for a long time in a large quantity of salt (Wikipedia).</skos:definition>
</rdf:Description>

<rdf:Description rdf:about="https://ark.frantiq.fr/ark:/26678/pcrt8yYh5xgMeO">
	<rdf:type rdf:resource="http://www.w3.org/2004/02/skos/core#Concept"/>
	<skos:prefLabel xml:lang="nl">edelsteen</skos:prefLabel>
	<skos:prefLabel xml:lang="es">gema</skos:prefLabel>
	<skos:prefLabel xml:lang="it">gemma</skos:prefLabel>
	<skos:prefLabel xml:lang="fr">gemme</skos:prefLabel>
	<skos:prefLabel xml:lang="en">gemstone</skos:prefLabel>
	<skos:prefLabel xml:lang="de">Schmuckstein</skos:prefLabel>
	<skos:prefLabel xml:lang="ar">جُمانة</skos:prefLabel>
	<skos:altLabel xml:lang="en">fine gem</skos:altLabel>
	<skos:altLabel xml:lang="en">jewel</skos:altLabel>
	<skos:altLabel xml:lang="en">precious stone</skos:altLabel>
	<skos:altLabel xml:lang="en">semiprecious stone</skos:altLabel>
	<skos:related rdf:resource="https://ark.frantiq.fr/ark:/26678/pcrtQgsSx0EwTS"/>
	<skos:related rdf:resource="https://ark.frantiq.fr/ark:/26678/pcrtbNJR98Fv1A"/>
	<skos:related rdf:resource="https://ark.frantiq.fr/ark:/26678/crth1OIw56xOI"/>
	<skos:related rdf:resource="https://ark.frantiq.fr/ark:/26678/pcrt7g5hd66j05pz5sr6k3r5"/>
	<skos:narrower rdf:resource="https://ark.frantiq.fr/ark:/26678/pcrtJt3ZKiNEFK"/>
	<skos:narrower rdf:resource="https://ark.frantiq.fr/ark:/26678/pcrtDoEeaZ6VcU"/>
	<skos:narrower rdf:resource="https://ark.frantiq.fr/ark:/26678/pcrtzVuPZeWdAP"/>
	<skos:broader rdf:resource="https://ark.frantiq.fr/ark:/26678/pcrtIMsuG0RWTs"/>
	<skos:inScheme rdf:resource="https://ark.frantiq.fr/ark:/26678/TH_1"/>
	<opentheso:memberOf rdf:resource="https://ark.frantiq.fr/ark:/26678/pcrtv66rn9cbv1"/>
	<opentheso:memberOf rdf:resource="https://ark.frantiq.fr/ark:/26678/pcrtnbDLi2FkAj"/>
	<skos:exactMatch rdf:resource="https://www.wikidata.org/wiki/Q83437"/>
	<skos:exactMatch rdf:resource="http://vocab.getty.edu/aat/300011172"/>
	<skos:exactMatch rdf:resource="http://vocab.getty.edu/aat/300201964"/>
	<dcterms:created rdf:datatype="http://www.w3.org/2001/XMLSchema#date">2007-02-08</dcterms:created>
	<dcterms:modified rdf:datatype="http://www.w3.org/2001/XMLSchema#date">2024-03-20</dcterms:modified>
	<dcterms:identifier>14869</dcterms:identifier>
	<dcterms:contributor>blandine.nouvel</dcterms:contributor>
	<dcterms:contributor>justine.vincent</dcterms:contributor>
	<skos:definition xml:lang="en">Fine, precious or ornamental stone. (wikipedia)</skos:definition>
	<skos:definition xml:lang="fr">Pierre fine, précieuse ou ornementale. (wikipedia)</skos:definition>
</rdf:Description>

<rdf:Description rdf:about="https://ark.frantiq.fr/ark:/26678/pcrtikYi5ORdK4">
	<rdf:type rdf:resource="http://www.w3.org/2004/02/skos/core#Concept"/>
	<skos:prefLabel xml:lang="en">acorn</skos:prefLabel>
	<skos:prefLabel xml:lang="es">bellota</skos:prefLabel>
	<skos:prefLabel xml:lang="de">Eichel</skos:prefLabel>
	<skos:prefLabel xml:lang="nl">eikel</skos:prefLabel>
	<skos:prefLabel xml:lang="it">ghianda</skos:prefLabel>
	<skos:prefLabel xml:lang="fr">gland</skos:prefLabel>
	<skos:prefLabel xml:lang="ar">جوز البلوط</skos:prefLabel>
	<skos:altLabel xml:lang="es">lande</skos:altLabel>
	<skos:related rdf:resource="https://ark.frantiq.fr/ark:/26678/pcrtDFvOrje3j0"/>
	<skos:related rdf:resource="https://ark.frantiq.fr/ark:/26678/crtOIK9VeDfzl"/>
	<skos:broader rdf:resource="https://ark.frantiq.fr/ark:/26678/pcrtgcn5U8laUN"/>
	<skos:inScheme rdf:resource="https://ark.frantiq.fr/ark:/26678/TH_1"/>
	<opentheso:memberOf rdf:resource="https://ark.frantiq.fr/ark:/26678/pcrtv66rn9cbv1"/>
	<opentheso:memberOf rdf:resource="https://ark.frantiq.fr/ark:/26678/pcrtnbDLi2FkAj"/>
	<skos:exactMatch rdf:resource="https://www.wikidata.org/wiki/Q3914781"/>
	<skos:exactMatch rdf:resource="http://vocab.getty.edu/aat/300251844"/>
	<dcterms:created rdf:datatype="http://www.w3.org/2001/XMLSchema#date">2007-02-08</dcterms:created>
	<dcterms:modified rdf:datatype="http://www.w3.org/2001/XMLSchema#date">2023-08-02</dcterms:modified>
	<dcterms:identifier>14884</dcterms:identifier>
	<dcterms:contributor>blandine.nouvel</dcterms:contributor>
	<skos:definition xml:lang="en">Oak fruit.</skos:definition>
	<skos:definition xml:lang="fr">Fruit du chêne.</skos:definition>
</rdf:Description>

<rdf:Description rdf:about="https://ark.frantiq.fr/ark:/26678/pcrt3pmFUqt27w">
	<rdf:type rdf:resource="http://www.w3.org/2004/02/skos/core#Concept"/>
	<skos:prefLabel xml:lang="fr">glaçure</skos:prefLabel>
	<skos:prefLabel xml:lang="de">Glasur</skos:prefLabel>
	<skos:prefLabel xml:lang="en">glazing</skos:prefLabel>
	<skos:prefLabel xml:lang="nl">glazuur</skos:prefLabel>
	<skos:prefLabel xml:lang="it">vetrina</skos:prefLabel>
	<skos:prefLabel xml:lang="es">vidriado</skos:prefLabel>
	<skos:prefLabel xml:lang="ar">تزجيج</skos:prefLabel>
	<skos:related rdf:resource="https://ark.frantiq.fr/ark:/26678/pcrt1sb2p55pwg"/>
	<skos:related rdf:resource="https://ark.frantiq.fr/ark:/26678/pcrt64s6h0j0cp"/>
	<skos:related rdf:resource="https://ark.frantiq.fr/ark:/26678/pcrt1asKmbn9q8"/>
	<skos:narrower rdf:resource="https://ark.frantiq.fr/ark:/26678/pcrtsTcJvHR17f"/>
	<skos:narrower rdf:resource="https://ark.frantiq.fr/ark:/26678/pcrtjzpz0bA7Mx"/>
	<skos:narrower rdf:resource="https://ark.frantiq.fr/ark:/26678/pcrtL9hSYO73pS"/>
	<skos:narrower rdf:resource="https://ark.frantiq.fr/ark:/26678/pcrt5SnWt4iSF2"/>
	<skos:narrower rdf:resource="https://ark.frantiq.fr/ark:/26678/pcrt2ozTOWS5f0"/>
	<skos:broader rdf:resource="https://ark.frantiq.fr/ark:/26678/pcrtIMsuG0RWTs"/>
	<skos:inScheme rdf:resource="https://ark.frantiq.fr/ark:/26678/TH_1"/>
	<opentheso:memberOf rdf:resource="https://ark.frantiq.fr/ark:/26678/pcrtv66rn9cbv1"/>
	<opentheso:memberOf rdf:resource="https://ark.frantiq.fr/ark:/26678/pcrtnbDLi2FkAj"/>
	<skos:exactMatch rdf:resource="https://www.wikidata.org/wiki/Q335404"/>
	<skos:exactMatch rdf:resource="http://vocab.getty.edu/aat/300015091"/>
	<skos:exactMatch rdf:resource="http://vocab.getty.edu/aat/300015092"/>
	<dcterms:created rdf:datatype="http://www.w3.org/2001/XMLSchema#date">2007-02-08</dcterms:created>
	<dcterms:modified rdf:datatype="http://www.w3.org/2001/XMLSchema#date">2023-08-02</dcterms:modified>
	<dcterms:identifier>14885</dcterms:identifier>
	<dcterms:contributor>blandine.nouvel</dcterms:contributor>
	<skos:definition xml:lang="en">A vitreous, lead-based or alkaline coating that covers an object. (Dic. ceramics PO)</skos:definition>
	<skos:definition xml:lang="fr">Désigne un revêtement de nature vitreuse, plombifère ou alcaline, qui recouvre un objet. (Dic. céramique PO)</skos:definition>
</rdf:Description>

<rdf:Description rdf:about="https://ark.frantiq.fr/ark:/26678/pcrtDnenSUMjFl">
	<rdf:type rdf:resource="http://www.w3.org/2004/02/skos/core#Concept"/>
	<skos:prefLabel xml:lang="nl">graniet</skos:prefLabel>
	<skos:prefLabel xml:lang="de">Granit</skos:prefLabel>
	<skos:prefLabel xml:lang="en">granite</skos:prefLabel>
	<skos:prefLabel xml:lang="fr">granite</skos:prefLabel>
	<skos:prefLabel xml:lang="es">granito</skos:prefLabel>
	<skos:prefLabel xml:lang="it">granito</skos:prefLabel>
	<skos:prefLabel xml:lang="ar">غرانيت</skos:prefLabel>
	<skos:altLabel xml:lang="fr">granit</skos:altLabel>
	<skos:related rdf:resource="https://ark.frantiq.fr/ark:/26678/pcrtXVZBob53by"/>
	<skos:broader rdf:resource="https://ark.frantiq.fr/ark:/26678/pcrt6BEybyEAjN"/>
	<skos:inScheme rdf:resource="https://ark.frantiq.fr/ark:/26678/TH_1"/>
	<opentheso:memberOf rdf:resource="https://ark.frantiq.fr/ark:/26678/pcrtv66rn9cbv1"/>
	<opentheso:memberOf rdf:resource="https://ark.frantiq.fr/ark:/26678/pcrtnbDLi2FkAj"/>
	<opentheso:memberOf rdf:resource="https://ark.frantiq.fr/ark:/26678/pcrtv0jq332vcq3gxt5m13d5"/>
	<skos:exactMatch rdf:resource="https://www.wikidata.org/wiki/Q41177"/>
	<skos:exactMatch rdf:resource="http://vocab.getty.edu/aat/300011183"/>
	<dcterms:created rdf:datatype="http://www.w3.org/2001/XMLSchema#date">2007-02-08</dcterms:created>
	<dcterms:modified rdf:datatype="http://www.w3.org/2001/XMLSchema#date">2024-03-21</dcterms:modified>
	<dcterms:identifier>14909</dcterms:identifier>
	<dcterms:contributor>blandine.nouvel</dcterms:contributor>
	<dcterms:contributor>irene.weis</dcterms:contributor>
	<skos:definition xml:lang="en">Granular plutonic magmatic rock that crystallises slowly at depth, consisting of xenomorphic quartz, feldspars (mainly potassic) such as orthoclase, and biotite in small shiny black flakes. (Lozet &amp;amp; Mathieu, Dictionnaire de science du sol. Ed. Technique et Documentation Lavoisier)</skos:definition>
	<skos:definition xml:lang="fr">Roche magmatique plutonique grenue dont la cristallisation s'est faite lentement en profondeur, constituée de quartz xénomorphe, de feldspaths surtout potassiques comme l'orthose, et de biotite en petites lamelles noires brillantes. (Lozet &amp;amp; Mathieu, Dictionnaire de science du sol. Ed. Technique et Documentation Lavoisier)</skos:definition>
</rdf:Description>

<rdf:Description rdf:about="https://ark.frantiq.fr/ark:/26678/pcrtVLPx3sY5Ku">
	<rdf:type rdf:resource="http://www.w3.org/2004/02/skos/core#Concept"/>
	<skos:prefLabel xml:lang="en">garnet</skos:prefLabel>
	<skos:prefLabel xml:lang="nl">granaat</skos:prefLabel>
	<skos:prefLabel xml:lang="de">Granat</skos:prefLabel>
	<skos:prefLabel xml:lang="es">granate</skos:prefLabel>
	<skos:prefLabel xml:lang="it">granato</skos:prefLabel>
	<skos:prefLabel xml:lang="fr">grenat</skos:prefLabel>
	<skos:prefLabel xml:lang="ar">بِجادي</skos:prefLabel>
	<skos:broader rdf:resource="https://ark.frantiq.fr/ark:/26678/pcrtJt3ZKiNEFK"/>
	<skos:inScheme rdf:resource="https://ark.frantiq.fr/ark:/26678/TH_1"/>
	<opentheso:memberOf rdf:resource="https://ark.frantiq.fr/ark:/26678/pcrtv66rn9cbv1"/>
	<opentheso:memberOf rdf:resource="https://ark.frantiq.fr/ark:/26678/pcrtnbDLi2FkAj"/>
	<skos:exactMatch rdf:resource="https://catalogue.bnf.fr/ark:/12148/cb12050469j"/>
	<skos:exactMatch rdf:resource="https://www.wikidata.org/wiki/Q105368"/>
	<skos:exactMatch rdf:resource="http://vocab.getty.edu/aat/300011097"/>
	<dcterms:created rdf:datatype="http://www.w3.org/2001/XMLSchema#date">2007-02-08</dcterms:created>
	<dcterms:modified rdf:datatype="http://www.w3.org/2001/XMLSchema#date">2024-11-15</dcterms:modified>
	<dcterms:identifier>14922</dcterms:identifier>
	<dcterms:contributor>blandine.nouvel</dcterms:contributor>
	<dcterms:contributor>justine.vincent</dcterms:contributor>
	<skos:definition xml:lang="en">Family of minerals in the nesosilicate group crystallising in the cubic (or isometric) crystal system. (wp)</skos:definition>
	<skos:definition xml:lang="fr">Famille de minéraux du groupe des nésosilicates cristallisant dans le système cristallin cubique (ou isométrique). (wp)</skos:definition>
</rdf:Description>

<rdf:Description rdf:about="https://ark.frantiq.fr/ark:/26678/pcrtR1s94Zuaul">
	<rdf:type rdf:resource="http://www.w3.org/2004/02/skos/core#Concept"/>
	<skos:prefLabel xml:lang="it">arenaria</skos:prefLabel>
	<skos:prefLabel xml:lang="es">gres</skos:prefLabel>
	<skos:prefLabel xml:lang="fr">grès (roche)</skos:prefLabel>
	<skos:prefLabel xml:lang="de">Sandstein</skos:prefLabel>
	<skos:prefLabel xml:lang="en">sandstone</skos:prefLabel>
	<skos:prefLabel xml:lang="nl">zandsteen</skos:prefLabel>
	<skos:prefLabel xml:lang="ar">حُث</skos:prefLabel>
	<skos:related rdf:resource="https://ark.frantiq.fr/ark:/26678/pcrtXk6sdvTjnE"/>
	<skos:related rdf:resource="https://ark.frantiq.fr/ark:/26678/crt3JnkclEfDF"/>
	<skos:related rdf:resource="https://ark.frantiq.fr/ark:/26678/pcrt0712c8ws62"/>
	<skos:narrower rdf:resource="https://ark.frantiq.fr/ark:/26678/pcrtqh9bhz6xcr"/>
	<skos:broader rdf:resource="https://ark.frantiq.fr/ark:/26678/pcrtRiKgPqvJQO"/>
	<skos:inScheme rdf:resource="https://ark.frantiq.fr/ark:/26678/TH_1"/>
	<opentheso:memberOf rdf:resource="https://ark.frantiq.fr/ark:/26678/pcrtv66rn9cbv1"/>
	<opentheso:memberOf rdf:resource="https://ark.frantiq.fr/ark:/26678/pcrtnbDLi2FkAj"/>
	<opentheso:memberOf rdf:resource="https://ark.frantiq.fr/ark:/26678/pcrtv0jq332vcq3gxt5m13d5"/>
	<skos:exactMatch rdf:resource="https://catalogue.bnf.fr/ark:/12148/cb11961094h"/>
	<skos:exactMatch rdf:resource="https://www.wikidata.org/wiki/Q13085"/>
	<skos:exactMatch rdf:resource="http://vocab.getty.edu/aat/300011376"/>
	<dcterms:created rdf:datatype="http://www.w3.org/2001/XMLSchema#date">2007-02-08</dcterms:created>
	<dcterms:modified rdf:datatype="http://www.w3.org/2001/XMLSchema#date">2024-03-21</dcterms:modified>
	<dcterms:identifier>14936</dcterms:identifier>
	<dcterms:contributor>blandine.nouvel</dcterms:contributor>
	<dcterms:contributor>irene.weis</dcterms:contributor>
	<skos:definition xml:lang="fr">Roche sédimentaire détritique, issue de l’agrégation de grains de taille majoritairement sableuse (0,063 mm à 2 mm) et consolidé lors de la diagenèse. (wp)</skos:definition>
</rdf:Description>

<rdf:Description rdf:about="https://ark.frantiq.fr/ark:/26678/pcrttcRKMp4QdV">
	<rdf:type rdf:resource="http://www.w3.org/2004/02/skos/core#Concept"/>
	<skos:prefLabel xml:lang="es"> avellana</skos:prefLabel>
	<skos:prefLabel xml:lang="de">Haselnuss</skos:prefLabel>
	<skos:prefLabel xml:lang="en">hazelnut</skos:prefLabel>
	<skos:prefLabel xml:lang="it">nocciola</skos:prefLabel>
	<skos:prefLabel xml:lang="fr">noisette</skos:prefLabel>
	<skos:prefLabel xml:lang="ar">بُنْدُقة</skos:prefLabel>
	<skos:altLabel xml:lang="en">cobnut</skos:altLabel>
	<skos:altLabel xml:lang="en">filbert</skos:altLabel>
	<skos:related rdf:resource="https://ark.frantiq.fr/ark:/26678/pcrtDFvOrje3j0"/>
	<skos:related rdf:resource="https://ark.frantiq.fr/ark:/26678/pcrtvcqtdq6w0dsv6xpmj4p0"/>
	<skos:broader rdf:resource="https://ark.frantiq.fr/ark:/26678/pcrtgcn5U8laUN"/>
	<skos:inScheme rdf:resource="https://ark.frantiq.fr/ark:/26678/TH_1"/>
	<opentheso:memberOf rdf:resource="https://ark.frantiq.fr/ark:/26678/pcrtv66rn9cbv1"/>
	<opentheso:memberOf rdf:resource="https://ark.frantiq.fr/ark:/26678/pcrtnbDLi2FkAj"/>
	<skos:exactMatch rdf:resource="https://www.wikidata.org/wiki/Q578307"/>
	<skos:exactMatch rdf:resource="http://vocab.getty.edu/aat/300411352"/>
	<dcterms:created rdf:datatype="http://www.w3.org/2001/XMLSchema#date">2015-11-26</dcterms:created>
	<dcterms:modified rdf:datatype="http://www.w3.org/2001/XMLSchema#date">2023-08-02</dcterms:modified>
	<dcterms:identifier>150495</dcterms:identifier>
	<dcterms:contributor>blandine.nouvel</dcterms:contributor>
	<skos:definition xml:lang="en">Fruit of the common hazel (Corylus avellana).</skos:definition>
	<skos:definition xml:lang="fr">Fruit du noisetier commun (Corylus avellana).</skos:definition>
</rdf:Description>

<rdf:Description rdf:about="https://ark.frantiq.fr/ark:/26678/pcrtkdetSDq0bj">
	<rdf:type rdf:resource="http://www.w3.org/2004/02/skos/core#Concept"/>
	<skos:prefLabel xml:lang="es">arcosa</skos:prefLabel>
	<skos:prefLabel xml:lang="it">arcose</skos:prefLabel>
	<skos:prefLabel xml:lang="en">arkose</skos:prefLabel>
	<skos:prefLabel xml:lang="fr">arkose</skos:prefLabel>
	<skos:prefLabel xml:lang="de">Arkose</skos:prefLabel>
	<skos:prefLabel xml:lang="nl">arkoze</skos:prefLabel>
	<skos:prefLabel xml:lang="ar">أَرْكُوز</skos:prefLabel>
	<skos:altLabel xml:lang="en">arkosic sandstone</skos:altLabel>
	<skos:broader rdf:resource="https://ark.frantiq.fr/ark:/26678/pcrtj3ZcwkArSR"/>
	<skos:inScheme rdf:resource="https://ark.frantiq.fr/ark:/26678/TH_1"/>
	<opentheso:memberOf rdf:resource="https://ark.frantiq.fr/ark:/26678/pcrtv66rn9cbv1"/>
	<opentheso:memberOf rdf:resource="https://ark.frantiq.fr/ark:/26678/pcrtnbDLi2FkAj"/>
	<skos:exactMatch rdf:resource="https://www.wikidata.org/wiki/Q673812"/>
	<dcterms:created rdf:datatype="http://www.w3.org/2001/XMLSchema#date">2015-12-18</dcterms:created>
	<dcterms:modified rdf:datatype="http://www.w3.org/2001/XMLSchema#date">2023-08-02</dcterms:modified>
	<dcterms:identifier>150518</dcterms:identifier>
	<dcterms:contributor>blandine.nouvel</dcterms:contributor>
	<skos:definition xml:lang="en">Terrigenous detrital sedimentary rock composed of quartz (up to 60%), feldspar (at least 25%), often a few micas and a cement composed of clay (about 15%). (Wikipedia)</skos:definition>
	<skos:definition xml:lang="fr">Roche sédimentaire détritique terrigène composée de quartz (jusqu'à 60 %), de feldspath (au moins 25 %), souvent de quelques micas et d'un ciment composé d'argile (environ 15 %). (Wikipédia)</skos:definition>
</rdf:Description>

<rdf:Description rdf:about="https://ark.frantiq.fr/ark:/26678/pcrtm6uoPROlPN">
	<rdf:type rdf:resource="http://www.w3.org/2004/02/skos/core#Concept"/>
	<skos:prefLabel xml:lang="en">earth</skos:prefLabel>
	<skos:prefLabel xml:lang="it">terra cruda</skos:prefLabel>
	<skos:prefLabel xml:lang="fr">terre crue</skos:prefLabel>
	<skos:prefLabel xml:lang="es">tierra cruda</skos:prefLabel>
	<skos:prefLabel xml:lang="de">ungebrannter Lehm</skos:prefLabel>
	<skos:prefLabel xml:lang="ar">طين رطب</skos:prefLabel>
	<skos:altLabel xml:lang="fr">terre (matière)</skos:altLabel>
	<skos:related rdf:resource="https://ark.frantiq.fr/ark:/26678/pcrt9FisN8EmXv"/>
	<skos:narrower rdf:resource="https://ark.frantiq.fr/ark:/26678/pcrthELuSjXqGH"/>
	<skos:narrower rdf:resource="https://ark.frantiq.fr/ark:/26678/pcrt52tibSvTjT"/>
	<skos:narrower rdf:resource="https://ark.frantiq.fr/ark:/26678/pcrtK8tO0rlQlM"/>
	<skos:broader rdf:resource="https://ark.frantiq.fr/ark:/26678/pcrtQuZiT5nYY2"/>
	<skos:inScheme rdf:resource="https://ark.frantiq.fr/ark:/26678/TH_1"/>
	<opentheso:memberOf rdf:resource="https://ark.frantiq.fr/ark:/26678/pcrtv66rn9cbv1"/>
	<opentheso:memberOf rdf:resource="https://ark.frantiq.fr/ark:/26678/pcrtnbDLi2FkAj"/>
	<opentheso:memberOf rdf:resource="https://ark.frantiq.fr/ark:/26678/pcrtv0jq332vcq3gxt5m13d5"/>
	<skos:exactMatch rdf:resource="https://www.wikidata.org/wiki/Q2090236"/>
	<dcterms:created rdf:datatype="http://www.w3.org/2001/XMLSchema#date">2015-12-18</dcterms:created>
	<dcterms:modified rdf:datatype="http://www.w3.org/2001/XMLSchema#date">2024-11-15</dcterms:modified>
	<dcterms:identifier>150520</dcterms:identifier>
	<dcterms:contributor>blandine.nouvel</dcterms:contributor>
	<dcterms:contributor>irene.weis</dcterms:contributor>
	<dcterms:contributor>justine.vincent</dcterms:contributor>
	<skos:definition xml:lang="en">Earth with few transformations used as a material (wp)</skos:definition>
	<skos:definition xml:lang="fr">Terre avec peu de transformations utilisée en tant que matériau. (wp)</skos:definition>
</rdf:Description>

<rdf:Description rdf:about="https://ark.frantiq.fr/ark:/26678/pcrt52tibSvTjT">
	<rdf:type rdf:resource="http://www.w3.org/2004/02/skos/core#Concept"/>
	<skos:prefLabel xml:lang="fr">bauge</skos:prefLabel>
	<skos:prefLabel xml:lang="en">cob</skos:prefLabel>
	<skos:prefLabel xml:lang="es">cob</skos:prefLabel>
	<skos:prefLabel xml:lang="de">Lehmwellerbau</skos:prefLabel>
	<skos:prefLabel xml:lang="it">massone</skos:prefLabel>
	<skos:prefLabel xml:lang="ar">طين ممزوج قش و حصى</skos:prefLabel>
	<skos:altLabel xml:lang="es">bajareque</skos:altLabel>
	<skos:altLabel xml:lang="en">clom</skos:altLabel>
	<skos:altLabel xml:lang="en">cobb</skos:altLabel>
	<skos:broader rdf:resource="https://ark.frantiq.fr/ark:/26678/pcrtm6uoPROlPN"/>
	<skos:inScheme rdf:resource="https://ark.frantiq.fr/ark:/26678/TH_1"/>
	<opentheso:memberOf rdf:resource="https://ark.frantiq.fr/ark:/26678/pcrtv66rn9cbv1"/>
	<opentheso:memberOf rdf:resource="https://ark.frantiq.fr/ark:/26678/pcrtnbDLi2FkAj"/>
	<skos:exactMatch rdf:resource="https://www.wikidata.org/wiki/Q54802"/>
	<skos:exactMatch rdf:resource="http://vocab.getty.edu/aat/300010735"/>
	<dcterms:created rdf:datatype="http://www.w3.org/2001/XMLSchema#date">2015-12-18</dcterms:created>
	<dcterms:modified rdf:datatype="http://www.w3.org/2001/XMLSchema#date">2024-10-25</dcterms:modified>
	<dcterms:identifier>150542</dcterms:identifier>
	<dcterms:contributor>blandine.nouvel</dcterms:contributor>
	<dcterms:contributor>patricia.moitrel</dcterms:contributor>
	<skos:definition xml:lang="en">A mixture of clay, straw, water and stones used to build a raw earth wall on a masonry base. It is built in several courses of a maximum height of 60 cm, without any formwork or internal framework, and you have to wait for one course to dry before starting the next (Pactols Group).</skos:definition>
	<skos:definition xml:lang="fr">Mélange de terre argileuse, de paille, d'eau et de cailloux utilisé pour dresser un mur de terre crue sur un soubassement maçonné. Il est monté en plusieurs levées de 60 cm de haut maximum, sans coffrage ou ossature interne et il est nécessaire d'attendre le séchage d'une levée pour entamer la suivante.</skos:definition>
	<skos:historyNote xml:lang="fr">2024-10-18 : réduction de la définition et traduction Deepl.</skos:historyNote>
</rdf:Description>

<rdf:Description rdf:about="https://ark.frantiq.fr/ark:/26678/pcrtJt3ZKiNEFK">
	<rdf:type rdf:resource="http://www.w3.org/2004/02/skos/core#Concept"/>
	<skos:prefLabel xml:lang="de">Halbedelstein</skos:prefLabel>
	<skos:prefLabel xml:lang="nl">halfedelsteen</skos:prefLabel>
	<skos:prefLabel xml:lang="es">piedra semipreciosa</skos:prefLabel>
	<skos:prefLabel xml:lang="fr">pierre fine</skos:prefLabel>
	<skos:prefLabel xml:lang="it">pietra semipreziosa</skos:prefLabel>
	<skos:prefLabel xml:lang="en">semi-precious stone</skos:prefLabel>
	<skos:prefLabel xml:lang="ar">أحجار شبه كريمة</skos:prefLabel>
	<skos:altLabel xml:lang="fr">pierre semi-précieuse</skos:altLabel>
	<skos:related rdf:resource="https://ark.frantiq.fr/ark:/26678/pcrtqmXRwn2Az6"/>
	<skos:related rdf:resource="https://ark.frantiq.fr/ark:/26678/pcrtVtHSyKSdbh"/>
	<skos:related rdf:resource="https://ark.frantiq.fr/ark:/26678/pcrtk2Q3q7YWXG"/>
	<skos:related rdf:resource="https://ark.frantiq.fr/ark:/26678/pcrtuFMPNUEKWb"/>
	<skos:related rdf:resource="https://ark.frantiq.fr/ark:/26678/pcrtgefwJa13yZ"/>
	<skos:related rdf:resource="https://ark.frantiq.fr/ark:/26678/pcrtQAl1Zjr5KF"/>
	<skos:related rdf:resource="https://ark.frantiq.fr/ark:/26678/pcrt3PUAhlWubZ"/>
	<skos:related rdf:resource="https://ark.frantiq.fr/ark:/26678/pcrtpp27tm32r2"/>
	<skos:narrower rdf:resource="https://ark.frantiq.fr/ark:/26678/pcrt0IaUrrrmF5"/>
	<skos:narrower rdf:resource="https://ark.frantiq.fr/ark:/26678/pcrtaJLEkei5LQ"/>
	<skos:narrower rdf:resource="https://ark.frantiq.fr/ark:/26678/pcrtVLPx3sY5Ku"/>
	<skos:narrower rdf:resource="https://ark.frantiq.fr/ark:/26678/pcrt7pgeXjaSI8"/>
	<skos:narrower rdf:resource="https://ark.frantiq.fr/ark:/26678/pcrtFUux6JWTnV"/>
	<skos:narrower rdf:resource="https://ark.frantiq.fr/ark:/26678/pcrtjyrVAHv1m8"/>
	<skos:narrower rdf:resource="https://ark.frantiq.fr/ark:/26678/pcrtv3md53Ugxj"/>
	<skos:broader rdf:resource="https://ark.frantiq.fr/ark:/26678/pcrt8yYh5xgMeO"/>
	<skos:inScheme rdf:resource="https://ark.frantiq.fr/ark:/26678/TH_1"/>
	<opentheso:memberOf rdf:resource="https://ark.frantiq.fr/ark:/26678/pcrtv66rn9cbv1"/>
	<opentheso:memberOf rdf:resource="https://ark.frantiq.fr/ark:/26678/pcrtnbDLi2FkAj"/>
	<skos:exactMatch rdf:resource="https://www.wikidata.org/wiki/Q10967610"/>
	<skos:exactMatch rdf:resource="http://vocab.getty.edu/aat/300011175"/>
	<dcterms:created rdf:datatype="http://www.w3.org/2001/XMLSchema#date">2015-12-21</dcterms:created>
	<dcterms:modified rdf:datatype="http://www.w3.org/2001/XMLSchema#date">2024-03-20</dcterms:modified>
	<dcterms:identifier>150544</dcterms:identifier>
	<dcterms:contributor>blandine.nouvel</dcterms:contributor>
	<dcterms:contributor>justine.vincent</dcterms:contributor>
	<skos:definition xml:lang="en">Gemstone not classified as one of the four precious stones (Wikipedia)</skos:definition>
	<skos:definition xml:lang="fr">Pierre gemme non classée parmi les quatre pierres précieuses. (Wikipedia)</skos:definition>
</rdf:Description>

<rdf:Description rdf:about="https://ark.frantiq.fr/ark:/26678/pcrtDoEeaZ6VcU">
	<rdf:type rdf:resource="http://www.w3.org/2004/02/skos/core#Concept"/>
	<skos:prefLabel xml:lang="it">gemma organica</skos:prefLabel>
	<skos:prefLabel xml:lang="en">organic gemstone</skos:prefLabel>
	<skos:prefLabel xml:lang="de">organische Schmucksteine</skos:prefLabel>
	<skos:prefLabel xml:lang="es">piedra orgánica</skos:prefLabel>
	<skos:prefLabel xml:lang="fr">pierre organique</skos:prefLabel>
	<skos:prefLabel xml:lang="ar">أحجار عضوية</skos:prefLabel>
	<skos:related rdf:resource="https://ark.frantiq.fr/ark:/26678/pcrtSiQAzZxXsv"/>
	<skos:related rdf:resource="https://ark.frantiq.fr/ark:/26678/pcrtknhh7n1sa3"/>
	<skos:narrower rdf:resource="https://ark.frantiq.fr/ark:/26678/pcrtV3BZNic1DR"/>
	<skos:broader rdf:resource="https://ark.frantiq.fr/ark:/26678/pcrt8yYh5xgMeO"/>
	<skos:inScheme rdf:resource="https://ark.frantiq.fr/ark:/26678/TH_1"/>
	<opentheso:memberOf rdf:resource="https://ark.frantiq.fr/ark:/26678/pcrtv66rn9cbv1"/>
	<opentheso:memberOf rdf:resource="https://ark.frantiq.fr/ark:/26678/pcrtnbDLi2FkAj"/>
	<skos:exactMatch rdf:resource="https://www.wikidata.org/wiki/Q110688445"/>
	<dcterms:created rdf:datatype="http://www.w3.org/2001/XMLSchema#date">2015-12-21</dcterms:created>
	<dcterms:modified rdf:datatype="http://www.w3.org/2001/XMLSchema#date">2023-08-02</dcterms:modified>
	<dcterms:identifier>150546</dcterms:identifier>
	<dcterms:contributor>blandine.nouvel</dcterms:contributor>
	<skos:definition xml:lang="en">Gem whose origin is not mineral.</skos:definition>
	<skos:definition xml:lang="fr">Gemme dont l'origine n'est pas minérale.</skos:definition>
</rdf:Description>

<rdf:Description rdf:about="https://ark.frantiq.fr/ark:/26678/pcrtKiepgzdXSQ">
	<rdf:type rdf:resource="http://www.w3.org/2004/02/skos/core#Concept"/>
	<skos:prefLabel xml:lang="es">almendra</skos:prefLabel>
	<skos:prefLabel xml:lang="en">almond</skos:prefLabel>
	<skos:prefLabel xml:lang="fr">amande</skos:prefLabel>
	<skos:prefLabel xml:lang="nl">amandel</skos:prefLabel>
	<skos:prefLabel xml:lang="de">Mandel</skos:prefLabel>
	<skos:prefLabel xml:lang="it">mandorla</skos:prefLabel>
	<skos:prefLabel xml:lang="ar">لَوْزة</skos:prefLabel>
	<skos:related rdf:resource="https://ark.frantiq.fr/ark:/26678/pcrtDFvOrje3j0"/>
	<skos:broader rdf:resource="https://ark.frantiq.fr/ark:/26678/pcrtgcn5U8laUN"/>
	<skos:inScheme rdf:resource="https://ark.frantiq.fr/ark:/26678/TH_1"/>
	<opentheso:memberOf rdf:resource="https://ark.frantiq.fr/ark:/26678/pcrtv66rn9cbv1"/>
	<opentheso:memberOf rdf:resource="https://ark.frantiq.fr/ark:/26678/pcrtnbDLi2FkAj"/>
	<skos:exactMatch rdf:resource="https://catalogue.bnf.fr/ark:/12148/cb12402392x"/>
	<skos:exactMatch rdf:resource="https://www.wikidata.org/wiki/Q184357"/>
	<skos:exactMatch rdf:resource="http://vocab.getty.edu/aat/300404293"/>
	<dcterms:created rdf:datatype="http://www.w3.org/2001/XMLSchema#date">2015-12-25</dcterms:created>
	<dcterms:modified rdf:datatype="http://www.w3.org/2001/XMLSchema#date">2023-08-02</dcterms:modified>
	<dcterms:identifier>150555</dcterms:identifier>
	<dcterms:contributor>blandine.nouvel</dcterms:contributor>
	<skos:definition xml:lang="nl">De amandel is het zaad van de amandelboom (Prunus soorten).</skos:definition>
	<skos:definition xml:lang="it">La mandorla è il seme commestibile del Mandorlo.</skos:definition>
	<skos:definition xml:lang="fr">Fruit de l'amandier (famille des rosacées).</skos:definition>
	<skos:definition xml:lang="es">Fruto del almendro (Prunus dulcis).</skos:definition>
</rdf:Description>

<rdf:Description rdf:about="https://ark.frantiq.fr/ark:/26678/pcrtp5MND6qfnb">
	<rdf:type rdf:resource="http://www.w3.org/2004/02/skos/core#Concept"/>
	<skos:prefLabel xml:lang="it">nichel</skos:prefLabel>
	<skos:prefLabel xml:lang="en">nickel</skos:prefLabel>
	<skos:prefLabel xml:lang="fr">nickel</skos:prefLabel>
	<skos:prefLabel xml:lang="de">Nickel</skos:prefLabel>
	<skos:prefLabel xml:lang="nl">nikkel</skos:prefLabel>
	<skos:prefLabel xml:lang="es">níquel</skos:prefLabel>
	<skos:prefLabel xml:lang="ar">نيكل</skos:prefLabel>
	<skos:altLabel xml:lang="it">nichelio</skos:altLabel>
	<skos:broader rdf:resource="https://ark.frantiq.fr/ark:/26678/pcrtkn1hAXHveS"/>
	<skos:inScheme rdf:resource="https://ark.frantiq.fr/ark:/26678/TH_1"/>
	<opentheso:memberOf rdf:resource="https://ark.frantiq.fr/ark:/26678/pcrtv66rn9cbv1"/>
	<opentheso:memberOf rdf:resource="https://ark.frantiq.fr/ark:/26678/pcrtnbDLi2FkAj"/>
	<skos:exactMatch rdf:resource="https://catalogue.bnf.fr/ark:/12148/cb119445481"/>
	<skos:exactMatch rdf:resource="https://www.wikidata.org/wiki/Q744"/>
	<skos:exactMatch rdf:resource="http://vocab.getty.edu/aat/300011028"/>
	<dcterms:created rdf:datatype="http://www.w3.org/2001/XMLSchema#date">2015-12-25</dcterms:created>
	<dcterms:modified rdf:datatype="http://www.w3.org/2001/XMLSchema#date">2024-12-04</dcterms:modified>
	<dcterms:identifier>150557</dcterms:identifier>
	<dcterms:contributor>blandine.nouvel</dcterms:contributor>
	<dcterms:contributor>justine.vincent</dcterms:contributor>
	<skos:definition xml:lang="en">Corrosion-resistant silvery-white metal, used mainly as an alloy in special steels or as a coating to protect iron or copper objects. (CNRTL)</skos:definition>
	<skos:definition xml:lang="fr">Métal blanc argenté résistant à la corrosion, utilisé principalement en alliage dans des aciers spéciaux ou en revêtement pour protéger des objets en fer ou en cuivre. (CNRTL)</skos:definition>
	<skos:historyNote xml:lang="fr">2024-04-12 : Modification de la définition.</skos:historyNote>
</rdf:Description>

<rdf:Description rdf:about="https://ark.frantiq.fr/ark:/26678/pcrtsEgKPlBjWE">
	<rdf:type rdf:resource="http://www.w3.org/2004/02/skos/core#Concept"/>
	<skos:prefLabel xml:lang="es"></skos:prefLabel>
	<skos:prefLabel xml:lang="it">grison (roccia)</skos:prefLabel>
	<skos:prefLabel xml:lang="fr">grison (roche)</skos:prefLabel>
	<skos:prefLabel xml:lang="de">Grisonstein</skos:prefLabel>
	<skos:prefLabel xml:lang="en">grison (stone)</skos:prefLabel>
	<skos:prefLabel xml:lang="ar">أرقش</skos:prefLabel>
	<skos:altLabel xml:lang="es">grison (roca)</skos:altLabel>
	<skos:broader rdf:resource="https://ark.frantiq.fr/ark:/26678/pcrtj3ZcwkArSR"/>
	<skos:inScheme rdf:resource="https://ark.frantiq.fr/ark:/26678/TH_1"/>
	<opentheso:memberOf rdf:resource="https://ark.frantiq.fr/ark:/26678/pcrtv66rn9cbv1"/>
	<opentheso:memberOf rdf:resource="https://ark.frantiq.fr/ark:/26678/pcrtnbDLi2FkAj"/>
	<skos:exactMatch rdf:resource="https://www.wikidata.org/wiki/Q3116813"/>
	<dcterms:created rdf:datatype="http://www.w3.org/2001/XMLSchema#date">2016-04-20</dcterms:created>
	<dcterms:modified rdf:datatype="http://www.w3.org/2001/XMLSchema#date">2023-08-02</dcterms:modified>
	<dcterms:identifier>150709</dcterms:identifier>
	<dcterms:contributor>blandine.nouvel</dcterms:contributor>
	<skos:definition xml:lang="en">Aggregate of siliceous pebbles welded together by a ferruginous cement giving a rusty-brown colour to the whole. (Wikipedia)</skos:definition>
	<skos:definition xml:lang="fr">Agrégat de cailloux siliceux soudés par un ciment ferrugineux donnant une couleur brun-rouille à l'ensemble. (Wikipédia)</skos:definition>
</rdf:Description>

<rdf:Description rdf:about="https://ark.frantiq.fr/ark:/26678/pcrttvE2YZwZu6">
	<rdf:type rdf:resource="http://www.w3.org/2004/02/skos/core#Concept"/>
	<skos:prefLabel xml:lang="es">aceite</skos:prefLabel>
	<skos:prefLabel xml:lang="fr">huile</skos:prefLabel>
	<skos:prefLabel xml:lang="en">oil</skos:prefLabel>
	<skos:prefLabel xml:lang="de">Öl</skos:prefLabel>
	<skos:prefLabel xml:lang="nl">olie</skos:prefLabel>
	<skos:prefLabel xml:lang="it">olio</skos:prefLabel>
	<skos:prefLabel xml:lang="ar">زيت</skos:prefLabel>
	<skos:altLabel xml:lang="en">cooking oil</skos:altLabel>
	<skos:altLabel xml:lang="fr">huile alimentaire</skos:altLabel>
	<skos:altLabel xml:lang="fr">huile végétale</skos:altLabel>
	<skos:altLabel xml:lang="en">vegetable oil</skos:altLabel>
	<skos:related rdf:resource="https://ark.frantiq.fr/ark:/26678/pcrtUTZqItd8SL"/>
	<skos:related rdf:resource="https://ark.frantiq.fr/ark:/26678/pcrtpJbqFUYwZI"/>
	<skos:related rdf:resource="https://ark.frantiq.fr/ark:/26678/pcrtlKNhumKaYq"/>
	<skos:related rdf:resource="https://ark.frantiq.fr/ark:/26678/pcrtbbb9diaauY"/>
	<skos:related rdf:resource="https://ark.frantiq.fr/ark:/26678/crtnRFSZO3uLv"/>
	<skos:broader rdf:resource="https://ark.frantiq.fr/ark:/26678/pcrtx37ph91cww"/>
	<skos:inScheme rdf:resource="https://ark.frantiq.fr/ark:/26678/TH_1"/>
	<opentheso:memberOf rdf:resource="https://ark.frantiq.fr/ark:/26678/pcrtv66rn9cbv1"/>
	<opentheso:memberOf rdf:resource="https://ark.frantiq.fr/ark:/26678/pcrtnbDLi2FkAj"/>
	<skos:exactMatch rdf:resource="https://www.wikidata.org/wiki/Q42962"/>
	<dcterms:created rdf:datatype="http://www.w3.org/2001/XMLSchema#date">2007-02-08</dcterms:created>
	<dcterms:modified rdf:datatype="http://www.w3.org/2001/XMLSchema#date">2023-08-02</dcterms:modified>
	<dcterms:identifier>15116</dcterms:identifier>
	<dcterms:contributor>blandine.nouvel</dcterms:contributor>
	<skos:definition xml:lang="en">Fatty substance, unctuous and inflammable, of vegetable, animal or mineral origin, generally liquid above 10 centigrade, freezing or solidifying at a lower temperature, used in various applications (CNRTL)</skos:definition>
	<skos:definition xml:lang="fr">Substance grasse, onctueuse et inflammable, d'origine végétale, animale ou minérale, généralement liquide au-dessus de 10&lt;sup&gt;o&lt;/sup&gt;centigrade, se figeant ou se solidifiant à une température inférieure, employée dans différents usages (CNRTL)</skos:definition>
</rdf:Description>

<rdf:Description rdf:about="https://ark.frantiq.fr/ark:/26678/pcrttEcSiJ6kNe">
	<rdf:type rdf:resource="http://www.w3.org/2004/02/skos/core#Concept"/>
	<skos:prefLabel xml:lang="es">hidromiel</skos:prefLabel>
	<skos:prefLabel xml:lang="nl">honingwater</skos:prefLabel>
	<skos:prefLabel xml:lang="en">hydromel</skos:prefLabel>
	<skos:prefLabel xml:lang="fr">hydromel</skos:prefLabel>
	<skos:prefLabel xml:lang="it">idromele</skos:prefLabel>
	<skos:prefLabel xml:lang="de">Met</skos:prefLabel>
	<skos:prefLabel xml:lang="ar">نبيذ العسل</skos:prefLabel>
	<skos:altLabel xml:lang="es">aguamiel</skos:altLabel>
	<skos:altLabel xml:lang="en">mead</skos:altLabel>
	<skos:broader rdf:resource="https://ark.frantiq.fr/ark:/26678/pcrt6z097U6IUf"/>
	<skos:inScheme rdf:resource="https://ark.frantiq.fr/ark:/26678/TH_1"/>
	<opentheso:memberOf rdf:resource="https://ark.frantiq.fr/ark:/26678/pcrtv66rn9cbv1"/>
	<opentheso:memberOf rdf:resource="https://ark.frantiq.fr/ark:/26678/pcrtnbDLi2FkAj"/>
	<skos:exactMatch rdf:resource="https://www.wikidata.org/wiki/Q184442"/>
	<dcterms:created rdf:datatype="http://www.w3.org/2001/XMLSchema#date">2007-02-08</dcterms:created>
	<dcterms:modified rdf:datatype="http://www.w3.org/2001/XMLSchema#date">2023-08-02</dcterms:modified>
	<dcterms:identifier>15127</dcterms:identifier>
	<dcterms:contributor>blandine.nouvel</dcterms:contributor>
	<skos:definition xml:lang="en">Drink, fermented or not, made from water or vinegar and honey (Lar.)</skos:definition>
	<skos:definition xml:lang="fr">Boisson fermentée ou non, faite d'eau ou de vinaigre et de miel (Lar.)</skos:definition>
</rdf:Description>

<rdf:Description rdf:about="https://ark.frantiq.fr/ark:/26678/pcrtuFMPNUEKWb">
	<rdf:type rdf:resource="http://www.w3.org/2004/02/skos/core#Concept"/>
	<skos:prefLabel xml:lang="it">ematite</skos:prefLabel>
	<skos:prefLabel xml:lang="de">Hämatit</skos:prefLabel>
	<skos:prefLabel xml:lang="nl">hematiet</skos:prefLabel>
	<skos:prefLabel xml:lang="es">hematita</skos:prefLabel>
	<skos:prefLabel xml:lang="en">hematite</skos:prefLabel>
	<skos:prefLabel xml:lang="fr">hématite</skos:prefLabel>
	<skos:prefLabel xml:lang="ar">هيماتيت</skos:prefLabel>
	<skos:altLabel xml:lang="en">haematite</skos:altLabel>
	<skos:altLabel xml:lang="es">hematites</skos:altLabel>
	<skos:altLabel xml:lang="ar">حجر الدم</skos:altLabel>
	<skos:related rdf:resource="https://ark.frantiq.fr/ark:/26678/pcrtJt3ZKiNEFK"/>
	<skos:related rdf:resource="https://ark.frantiq.fr/ark:/26678/pcrttnySGIGsj6"/>
	<skos:related rdf:resource="https://ark.frantiq.fr/ark:/26678/pcrtf80pqj28pw"/>
	<skos:broader rdf:resource="https://ark.frantiq.fr/ark:/26678/pcrty2mcsksa6s"/>
	<skos:inScheme rdf:resource="https://ark.frantiq.fr/ark:/26678/TH_1"/>
	<opentheso:memberOf rdf:resource="https://ark.frantiq.fr/ark:/26678/pcrtv66rn9cbv1"/>
	<opentheso:memberOf rdf:resource="https://ark.frantiq.fr/ark:/26678/pcrtnbDLi2FkAj"/>
	<skos:exactMatch rdf:resource="https://catalogue.bnf.fr/ark:/12148/cb13770127j"/>
	<skos:exactMatch rdf:resource="https://www.wikidata.org/wiki/Q103223"/>
	<skos:exactMatch rdf:resource="http://vocab.getty.edu/aat/300011105"/>
	<dcterms:created rdf:datatype="http://www.w3.org/2001/XMLSchema#date">2007-02-08</dcterms:created>
	<dcterms:modified rdf:datatype="http://www.w3.org/2001/XMLSchema#date">2024-11-18</dcterms:modified>
	<dcterms:identifier>15143</dcterms:identifier>
	<dcterms:contributor>blandine.nouvel</dcterms:contributor>
	<dcterms:contributor>justine.vincent</dcterms:contributor>
	<skos:definition xml:lang="en">Mineral species composed of iron oxide with traces of titanium, aluminium, manganese and water, used in ferrous alloys or as a red pigment for parietal painting and cosmetics. (Wikipedia)</skos:definition>
	<skos:definition xml:lang="fr">Espèce minérale composée d'oxyde de fer avec des traces de titane, d'aluminium, de manganèse et d'eau, utilisée dans &lt;span style= background-color: rgb(255, 255, 255); &gt;des alliages ferreux ou comme pigment rouge pour la peinture pariétale et la cosmétique.&lt;/span&gt; (Wikipedia)</skos:definition>
</rdf:Description>

<rdf:Description rdf:about="https://ark.frantiq.fr/ark:/26678/pcrt1zVFrqhSh2">
	<rdf:type rdf:resource="http://www.w3.org/2004/02/skos/core#Concept"/>
	<skos:prefLabel xml:lang="it">avorio</skos:prefLabel>
	<skos:prefLabel xml:lang="de">Elfenbein</skos:prefLabel>
	<skos:prefLabel xml:lang="fr">ivoire</skos:prefLabel>
	<skos:prefLabel xml:lang="nl">ivoor</skos:prefLabel>
	<skos:prefLabel xml:lang="en">ivory</skos:prefLabel>
	<skos:prefLabel xml:lang="es">marfil</skos:prefLabel>
	<skos:prefLabel xml:lang="ar">عاج</skos:prefLabel>
	<skos:related rdf:resource="https://ark.frantiq.fr/ark:/26678/pcrthA4kIWMu84"/>
	<skos:related rdf:resource="https://ark.frantiq.fr/ark:/26678/crtQMTce6O6Z7"/>
	<skos:related rdf:resource="https://ark.frantiq.fr/ark:/26678/pcrtMj9v33qudS"/>
	<skos:broader rdf:resource="https://ark.frantiq.fr/ark:/26678/pcrtf97bQHDGEd"/>
	<skos:inScheme rdf:resource="https://ark.frantiq.fr/ark:/26678/TH_1"/>
	<opentheso:memberOf rdf:resource="https://ark.frantiq.fr/ark:/26678/pcrtv66rn9cbv1"/>
	<opentheso:memberOf rdf:resource="https://ark.frantiq.fr/ark:/26678/pcrtnbDLi2FkAj"/>
	<opentheso:memberOf rdf:resource="https://ark.frantiq.fr/ark:/26678/pcrtv0jq332vcq3gxt5m13d5"/>
	<skos:exactMatch rdf:resource="https://catalogue.bnf.fr/ark:/12148/cb136169195"/>
	<skos:exactMatch rdf:resource="https://www.wikidata.org/wiki/Q82001"/>
	<skos:exactMatch rdf:resource="http://vocab.getty.edu/aat/300011857"/>
	<dcterms:created rdf:datatype="http://www.w3.org/2001/XMLSchema#date">2007-02-08</dcterms:created>
	<dcterms:modified rdf:datatype="http://www.w3.org/2001/XMLSchema#date">2024-12-04</dcterms:modified>
	<dcterms:identifier>15326</dcterms:identifier>
	<dcterms:contributor>blandine.nouvel</dcterms:contributor>
	<dcterms:contributor>patricia.moitrel</dcterms:contributor>
	<skos:definition xml:lang="en">Ivory is a hard, white, opaque substance that is the main material in the teeth and tusks of animals such as elephants, hippopotamuses, walruses, narwhals, sperm whales and warthogs (WP le 19/10/18).</skos:definition>
	<skos:definition xml:lang="fr">Substance dure, blanche, opaque qui est la matière principale des dents et des défenses d'animaux comme l'éléphant, l'hippopotame, le morse, le narval, le cachalot, le phacochère. (WP le 19/10/18)</skos:definition>
	<skos:scopeNote xml:lang="fr">Utiliser ce concept pour l'ivoire comme matière première. Pour l'ivoire sculpté (ou travaillé par l'homme), privilégier le concept  objet en ivoire .</skos:scopeNote>
</rdf:Description>

<rdf:Description rdf:about="https://ark.frantiq.fr/ark:/26678/pcrt7pgeXjaSI8">
	<rdf:type rdf:resource="http://www.w3.org/2004/02/skos/core#Concept"/>
	<skos:prefLabel xml:lang="it">giada</skos:prefLabel>
	<skos:prefLabel xml:lang="en">jade</skos:prefLabel>
	<skos:prefLabel xml:lang="es">jade</skos:prefLabel>
	<skos:prefLabel xml:lang="fr">jade</skos:prefLabel>
	<skos:prefLabel xml:lang="nl">jade</skos:prefLabel>
	<skos:prefLabel xml:lang="de">Jade</skos:prefLabel>
	<skos:prefLabel xml:lang="ar">يَشم</skos:prefLabel>
	<skos:related rdf:resource="https://ark.frantiq.fr/ark:/26678/pcrtSpItdjR86k"/>
	<skos:narrower rdf:resource="https://ark.frantiq.fr/ark:/26678/pcrtslVSzVnfeg"/>
	<skos:broader rdf:resource="https://ark.frantiq.fr/ark:/26678/pcrtJt3ZKiNEFK"/>
	<skos:inScheme rdf:resource="https://ark.frantiq.fr/ark:/26678/TH_1"/>
	<opentheso:memberOf rdf:resource="https://ark.frantiq.fr/ark:/26678/pcrtv66rn9cbv1"/>
	<opentheso:memberOf rdf:resource="https://ark.frantiq.fr/ark:/26678/pcrtnbDLi2FkAj"/>
	<skos:exactMatch rdf:resource="https://www.wikidata.org/wiki/Q175089"/>
	<skos:exactMatch rdf:resource="http://vocab.getty.edu/aat/300011119"/>
	<dcterms:created rdf:datatype="http://www.w3.org/2001/XMLSchema#date">2007-02-08</dcterms:created>
	<dcterms:modified rdf:datatype="http://www.w3.org/2001/XMLSchema#date">2023-08-02</dcterms:modified>
	<dcterms:identifier>15329</dcterms:identifier>
	<dcterms:contributor>blandine.nouvel</dcterms:contributor>
	<skos:definition xml:lang="en">Very hard and tough gemstone used in ornamentation and jewellery (wp)</skos:definition>
	<skos:definition xml:lang="fr">Pierre gemme très dure et tenace employée en ornementation et en joaillerie. (wp)</skos:definition>
</rdf:Description>

<rdf:Description rdf:about="https://ark.frantiq.fr/ark:/26678/pcrtDfHvvnBWz7">
	<rdf:type rdf:resource="http://www.w3.org/2004/02/skos/core#Concept"/>
	<skos:prefLabel xml:lang="fr">laine</skos:prefLabel>
	<skos:prefLabel xml:lang="es">lana</skos:prefLabel>
	<skos:prefLabel xml:lang="it">lana</skos:prefLabel>
	<skos:prefLabel xml:lang="nl">wol</skos:prefLabel>
	<skos:prefLabel xml:lang="de">Wolle</skos:prefLabel>
	<skos:prefLabel xml:lang="en">wool</skos:prefLabel>
	<skos:prefLabel xml:lang="ar">صوف</skos:prefLabel>
	<skos:related rdf:resource="https://ark.frantiq.fr/ark:/26678/pcrthAOjGBEfZk"/>
	<skos:related rdf:resource="https://ark.frantiq.fr/ark:/26678/pcrt5j9z1z718wq4mnx49j43"/>
	<skos:broader rdf:resource="https://ark.frantiq.fr/ark:/26678/pcrtwvFLgSQRs5"/>
	<skos:inScheme rdf:resource="https://ark.frantiq.fr/ark:/26678/TH_1"/>
	<opentheso:memberOf rdf:resource="https://ark.frantiq.fr/ark:/26678/pcrtv66rn9cbv1"/>
	<opentheso:memberOf rdf:resource="https://ark.frantiq.fr/ark:/26678/pcrtnbDLi2FkAj"/>
	<skos:exactMatch rdf:resource="https://catalogue.bnf.fr/ark:/12148/cb119353831"/>
	<skos:exactMatch rdf:resource="https://www.wikidata.org/wiki/Q42329"/>
	<skos:exactMatch rdf:resource="http://vocab.getty.edu/aat/300014074"/>
	<dcterms:created rdf:datatype="http://www.w3.org/2001/XMLSchema#date">2007-02-08</dcterms:created>
	<dcterms:modified rdf:datatype="http://www.w3.org/2001/XMLSchema#date">2023-08-02</dcterms:modified>
	<dcterms:identifier>15385</dcterms:identifier>
	<dcterms:contributor>blandine.nouvel</dcterms:contributor>
	<skos:definition xml:lang="en">Material of animal origin consisting of keratin fibres, mainly from sheep, used in textile production, in particular for its thermal insulation properties. (wp)</skos:definition>
	<skos:definition xml:lang="fr">Matériau d'origine animale qui est constitué de fibres kératiniques, principalement d'ovins et utilisé dans la production textile, notamment pour ses capacités d'isolant thermique. (wp)</skos:definition>
</rdf:Description>

<rdf:Description rdf:about="https://ark.frantiq.fr/ark:/26678/pcrtlSaqkoJ8gu">
	<rdf:type rdf:resource="http://www.w3.org/2004/02/skos/core#Concept"/>
	<skos:prefLabel xml:lang="en">brass</skos:prefLabel>
	<skos:prefLabel xml:lang="nl">geelkoper</skos:prefLabel>
	<skos:prefLabel xml:lang="fr">laiton</skos:prefLabel>
	<skos:prefLabel xml:lang="es">latón</skos:prefLabel>
	<skos:prefLabel xml:lang="de">Messing</skos:prefLabel>
	<skos:prefLabel xml:lang="it">ottone</skos:prefLabel>
	<skos:prefLabel xml:lang="ar">نحاس</skos:prefLabel>
	<skos:altLabel xml:lang="es">azófar</skos:altLabel>
	<skos:altLabel xml:lang="en">latten</skos:altLabel>
	<skos:broader rdf:resource="https://ark.frantiq.fr/ark:/26678/pcrtzcGlM17go5"/>
	<skos:inScheme rdf:resource="https://ark.frantiq.fr/ark:/26678/TH_1"/>
	<opentheso:memberOf rdf:resource="https://ark.frantiq.fr/ark:/26678/pcrtv66rn9cbv1"/>
	<opentheso:memberOf rdf:resource="https://ark.frantiq.fr/ark:/26678/pcrtnbDLi2FkAj"/>
	<skos:exactMatch rdf:resource="https://catalogue.bnf.fr/ark:/12148/cb119830963"/>
	<skos:exactMatch rdf:resource="https://www.wikidata.org/wiki/Q39782"/>
	<skos:exactMatch rdf:resource="http://vocab.getty.edu/aat/300010946"/>
	<dcterms:created rdf:datatype="http://www.w3.org/2001/XMLSchema#date">2007-02-08</dcterms:created>
	<dcterms:modified rdf:datatype="http://www.w3.org/2001/XMLSchema#date">2023-08-02</dcterms:modified>
	<dcterms:identifier>15386</dcterms:identifier>
	<dcterms:contributor>blandine.nouvel</dcterms:contributor>
	<skos:definition xml:lang="en">An alloy of copper and zinc, with a zinc content varying from 5 to 42% in an industrial alloy. (Larousse)</skos:definition>
	<skos:definition xml:lang="fr">Alliage de cuivre et de zinc, dont la teneur en zinc, pour un alliage industriel, varie de 5 à 42 %. (Larousse)</skos:definition>
</rdf:Description>

<rdf:Description rdf:about="https://ark.frantiq.fr/ark:/26678/pcrtFUux6JWTnV">
	<rdf:type rdf:resource="http://www.w3.org/2004/02/skos/core#Concept"/>
	<skos:prefLabel xml:lang="en">lapis lazuli</skos:prefLabel>
	<skos:prefLabel xml:lang="nl">lapis lazuli</skos:prefLabel>
	<skos:prefLabel xml:lang="fr">lapis-lazuli</skos:prefLabel>
	<skos:prefLabel xml:lang="de">Lapislazuli</skos:prefLabel>
	<skos:prefLabel xml:lang="es">lapislázuli</skos:prefLabel>
	<skos:prefLabel xml:lang="it">lapislazzuli</skos:prefLabel>
	<skos:prefLabel xml:lang="ar">لازورد</skos:prefLabel>
	<skos:altLabel xml:lang="en">lapis</skos:altLabel>
	<skos:altLabel xml:lang="it">lapislazuli</skos:altLabel>
	<skos:related rdf:resource="https://ark.frantiq.fr/ark:/26678/pcrtM0mkbZiNnN"/>
	<skos:broader rdf:resource="https://ark.frantiq.fr/ark:/26678/pcrtJt3ZKiNEFK"/>
	<skos:inScheme rdf:resource="https://ark.frantiq.fr/ark:/26678/TH_1"/>
	<opentheso:memberOf rdf:resource="https://ark.frantiq.fr/ark:/26678/pcrtv66rn9cbv1"/>
	<opentheso:memberOf rdf:resource="https://ark.frantiq.fr/ark:/26678/pcrtnbDLi2FkAj"/>
	<skos:exactMatch rdf:resource="https://www.wikidata.org/wiki/Q216798"/>
	<skos:exactMatch rdf:resource="http://vocab.getty.edu/aat/300011122"/>
	<dcterms:created rdf:datatype="http://www.w3.org/2001/XMLSchema#date">2007-02-08</dcterms:created>
	<dcterms:modified rdf:datatype="http://www.w3.org/2001/XMLSchema#date">2023-08-02</dcterms:modified>
	<dcterms:identifier>15417</dcterms:identifier>
	<dcterms:contributor>blandine.nouvel</dcterms:contributor>
	<skos:definition xml:lang="en">Intense blue stone used in ornamentation and jewellery, composed mainly of lazurite, with some calcite, pyrite, etc. (Lar.)</skos:definition>
	<skos:definition xml:lang="fr">Pierre d'un bleu intense, utilisée en ornementation et en joaillerie, composée essentiellement de lazurite, accessoirement de calcite, pyrite, etc. (Lar.)</skos:definition>
</rdf:Description>

<rdf:Description rdf:about="https://ark.frantiq.fr/ark:/26678/pcrt9rIFPQ997Q">
	<rdf:type rdf:resource="http://www.w3.org/2004/02/skos/core#Concept"/>
	<skos:prefLabel xml:lang="nl">ligniet</skos:prefLabel>
	<skos:prefLabel xml:lang="de">Lignit</skos:prefLabel>
	<skos:prefLabel xml:lang="en">lignite</skos:prefLabel>
	<skos:prefLabel xml:lang="fr">lignite</skos:prefLabel>
	<skos:prefLabel xml:lang="it">lignite</skos:prefLabel>
	<skos:prefLabel xml:lang="es">lignito</skos:prefLabel>
	<skos:prefLabel xml:lang="ar">ليغنيت</skos:prefLabel>
	<skos:altLabel xml:lang="en">brown coal</skos:altLabel>
	<skos:related rdf:resource="https://ark.frantiq.fr/ark:/26678/pcrtO40ZLI4giK"/>
	<skos:broader rdf:resource="https://ark.frantiq.fr/ark:/26678/pcrtsrWeYcRkNg"/>
	<skos:inScheme rdf:resource="https://ark.frantiq.fr/ark:/26678/TH_1"/>
	<opentheso:memberOf rdf:resource="https://ark.frantiq.fr/ark:/26678/pcrtv66rn9cbv1"/>
	<opentheso:memberOf rdf:resource="https://ark.frantiq.fr/ark:/26678/pcrtnbDLi2FkAj"/>
	<skos:exactMatch rdf:resource="https://catalogue.bnf.fr/ark:/12148/cb11971410z"/>
	<skos:exactMatch rdf:resource="https://www.wikidata.org/wiki/Q156267"/>
	<skos:exactMatch rdf:resource="http://vocab.getty.edu/aat/300211957"/>
	<dcterms:created rdf:datatype="http://www.w3.org/2001/XMLSchema#date">2007-02-08</dcterms:created>
	<dcterms:modified rdf:datatype="http://www.w3.org/2001/XMLSchema#date">2023-08-02</dcterms:modified>
	<dcterms:identifier>15447</dcterms:identifier>
	<dcterms:contributor>blandine.nouvel</dcterms:contributor>
	<skos:definition xml:lang="en">Brown fossil coal, rich in plant debris, with low calorific value (cnrtl)</skos:definition>
	<skos:definition xml:lang="ar">خشب متفحم</skos:definition>
	<skos:definition xml:lang="fr">Charbon fossile de couleur brune, riche en débris végétaux, à faible pouvoir calorifique (cnrtl)</skos:definition>
</rdf:Description>

<rdf:Description rdf:about="https://ark.frantiq.fr/ark:/26678/pcrt2vlSZd64Zk">
	<rdf:type rdf:resource="http://www.w3.org/2004/02/skos/core#Concept"/>
	<skos:prefLabel xml:lang="nl">leem</skos:prefLabel>
	<skos:prefLabel xml:lang="es">limo</skos:prefLabel>
	<skos:prefLabel xml:lang="it">limo</skos:prefLabel>
	<skos:prefLabel xml:lang="fr">limon</skos:prefLabel>
	<skos:prefLabel xml:lang="de">Schluff</skos:prefLabel>
	<skos:prefLabel xml:lang="en">silt</skos:prefLabel>
	<skos:prefLabel xml:lang="ar">غرين</skos:prefLabel>
	<skos:altLabel xml:lang="de">Silt</skos:altLabel>
	<skos:related rdf:resource="https://ark.frantiq.fr/ark:/26678/pcrtSIsVZPQG1t"/>
	<skos:broader rdf:resource="https://ark.frantiq.fr/ark:/26678/pcrt4Jy2JE8F3U"/>
	<skos:inScheme rdf:resource="https://ark.frantiq.fr/ark:/26678/TH_1"/>
	<opentheso:memberOf rdf:resource="https://ark.frantiq.fr/ark:/26678/pcrtv66rn9cbv1"/>
	<opentheso:memberOf rdf:resource="https://ark.frantiq.fr/ark:/26678/pcrtnbDLi2FkAj"/>
	<opentheso:memberOf rdf:resource="https://ark.frantiq.fr/ark:/26678/pcrtv0jq332vcq3gxt5m13d5"/>
	<skos:exactMatch rdf:resource="https://www.wikidata.org/wiki/Q270699"/>
	<skos:exactMatch rdf:resource="http://vocab.getty.edu/aat/300379483"/>
	<dcterms:created rdf:datatype="http://www.w3.org/2001/XMLSchema#date">2007-02-08</dcterms:created>
	<dcterms:modified rdf:datatype="http://www.w3.org/2001/XMLSchema#date">2024-08-22</dcterms:modified>
	<dcterms:identifier>15454</dcterms:identifier>
	<dcterms:contributor>blandine.nouvel</dcterms:contributor>
	<dcterms:contributor>irene.weis</dcterms:contributor>
	<skos:definition xml:lang="fr">Formation sédimentaire dont les particules sont constituées de débris très fins (taille intermédiaire entre les argiles et les sables c'est-à-dire entre 2 et 63 micromètres) de quartz, de mica et de feldspath, voire de minéraux argileux.</skos:definition>
	<skos:definition xml:lang="en">Sedimentary formation whose particles are made up of very fine debris (intermediate size between clay and sand, i.e. between 2 and 63 micrometres) of quartz, mica and feldspar, and even clay minerals.</skos:definition>
	<skos:historyNote xml:lang="fr">2024-08-22 : révision et traduction de la définition.</skos:historyNote>
</rdf:Description>

<rdf:Description rdf:about="https://ark.frantiq.fr/ark:/26678/pcrtSIsVZPQG1t">
	<rdf:type rdf:resource="http://www.w3.org/2004/02/skos/core#Concept"/>
	<skos:prefLabel xml:lang="en">loess</skos:prefLabel>
	<skos:prefLabel xml:lang="es">loess</skos:prefLabel>
	<skos:prefLabel xml:lang="fr">loess</skos:prefLabel>
	<skos:prefLabel xml:lang="it">loess</skos:prefLabel>
	<skos:prefLabel xml:lang="nl">löss</skos:prefLabel>
	<skos:prefLabel xml:lang="de">Löss</skos:prefLabel>
	<skos:prefLabel xml:lang="ar">طين</skos:prefLabel>
	<skos:altLabel xml:lang="fr">lœss</skos:altLabel>
	<skos:altLabel xml:lang="it">löss</skos:altLabel>
	<skos:related rdf:resource="https://ark.frantiq.fr/ark:/26678/pcrt2vlSZd64Zk"/>
	<skos:broader rdf:resource="https://ark.frantiq.fr/ark:/26678/pcrtjbpmw8qvrn"/>
	<skos:inScheme rdf:resource="https://ark.frantiq.fr/ark:/26678/TH_1"/>
	<opentheso:memberOf rdf:resource="https://ark.frantiq.fr/ark:/26678/pcrtv66rn9cbv1"/>
	<opentheso:memberOf rdf:resource="https://ark.frantiq.fr/ark:/26678/pcrtnbDLi2FkAj"/>
	<opentheso:memberOf rdf:resource="https://ark.frantiq.fr/ark:/26678/pcrtv0jq332vcq3gxt5m13d5"/>
	<skos:exactMatch rdf:resource="https://www.wikidata.org/wiki/Q22723"/>
	<skos:exactMatch rdf:resource="http://vocab.getty.edu/aat/300014336"/>
	<dcterms:created rdf:datatype="http://www.w3.org/2001/XMLSchema#date">2007-02-08</dcterms:created>
	<dcterms:modified rdf:datatype="http://www.w3.org/2001/XMLSchema#date">2024-11-20</dcterms:modified>
	<dcterms:identifier>15474</dcterms:identifier>
	<dcterms:contributor>blandine.nouvel</dcterms:contributor>
	<dcterms:contributor>irene.weis</dcterms:contributor>
	<dcterms:contributor>justine.vincent</dcterms:contributor>
	<dcterms:contributor>patricia.moitrel</dcterms:contributor>
	<skos:definition xml:lang="fr">Roche sédimentaire détritique meuble (&lt;span style= background-color: rgb(255, 255, 255); &gt;grains compris entre 63 µm et 2 mm) &lt;/span&gt;formée par l'accumulation de limons issus de l'érosion éolienne (déflation), dans les régions désertiques et périglaciaires. (wikipedia et Fernandez 2012)</skos:definition>
	<skos:definition xml:lang="en">Loose detrital sedimentary rock (grain size between 63 µm and 2 mm) formed by the accumulation of silts from wind erosion (deflation), in desert and periglacial regions. (wikipedia and Fernandez 2012)</skos:definition>
	<skos:historyNote xml:lang="fr">2024-11-20 : ajout d'une variante.</skos:historyNote>
</rdf:Description>

<rdf:Description rdf:about="https://ark.frantiq.fr/ark:/26678/pcrtQe4n9vGjl0">
	<rdf:type rdf:resource="http://www.w3.org/2004/02/skos/core#Concept"/>
	<skos:prefLabel xml:lang="es">magnesio</skos:prefLabel>
	<skos:prefLabel xml:lang="it">magnesio</skos:prefLabel>
	<skos:prefLabel xml:lang="en">magnesium</skos:prefLabel>
	<skos:prefLabel xml:lang="nl">magnesium</skos:prefLabel>
	<skos:prefLabel xml:lang="de">Magnesium</skos:prefLabel>
	<skos:prefLabel xml:lang="fr">magnésium</skos:prefLabel>
	<skos:prefLabel xml:lang="ar">مغنيسيوم</skos:prefLabel>
	<skos:altLabel xml:lang="ar">معدن صلب</skos:altLabel>
	<skos:broader rdf:resource="https://ark.frantiq.fr/ark:/26678/pcrtkn1hAXHveS"/>
	<skos:inScheme rdf:resource="https://ark.frantiq.fr/ark:/26678/TH_1"/>
	<opentheso:memberOf rdf:resource="https://ark.frantiq.fr/ark:/26678/pcrtv66rn9cbv1"/>
	<opentheso:memberOf rdf:resource="https://ark.frantiq.fr/ark:/26678/pcrtnbDLi2FkAj"/>
	<skos:exactMatch rdf:resource="https://catalogue.bnf.fr/ark:/12148/cb119771902"/>
	<skos:exactMatch rdf:resource="https://www.wikidata.org/wiki/Q660"/>
	<skos:exactMatch rdf:resource="http://vocab.getty.edu/aat/300011024"/>
	<dcterms:created rdf:datatype="http://www.w3.org/2001/XMLSchema#date">2007-02-08</dcterms:created>
	<dcterms:modified rdf:datatype="http://www.w3.org/2001/XMLSchema#date">2024-12-04</dcterms:modified>
	<dcterms:identifier>15548</dcterms:identifier>
	<dcterms:contributor>blandine.nouvel</dcterms:contributor>
	<dcterms:contributor>justine.vincent</dcterms:contributor>
	<skos:definition xml:lang="en">White alkaline-earth metal.</skos:definition>
	<skos:definition xml:lang="fr">Métal blanc alcalino-terreux.</skos:definition>
</rdf:Description>

<rdf:Description rdf:about="https://ark.frantiq.fr/ark:/26678/pcrtevBDzau7qe">
	<rdf:type rdf:resource="http://www.w3.org/2004/02/skos/core#Concept"/>
	<skos:prefLabel xml:lang="nl">robijn</skos:prefLabel>
	<skos:prefLabel xml:lang="es">rubí</skos:prefLabel>
	<skos:prefLabel xml:lang="de">rubin</skos:prefLabel>
	<skos:prefLabel xml:lang="it">rubino</skos:prefLabel>
	<skos:prefLabel xml:lang="fr">rubis</skos:prefLabel>
	<skos:prefLabel xml:lang="en">ruby</skos:prefLabel>
	<skos:related rdf:resource="https://ark.frantiq.fr/ark:/26678/pcrtHv6zSSHk9H"/>
	<skos:broader rdf:resource="https://ark.frantiq.fr/ark:/26678/pcrtzVuPZeWdAP"/>
	<skos:inScheme rdf:resource="https://ark.frantiq.fr/ark:/26678/TH_1"/>
	<opentheso:memberOf rdf:resource="https://ark.frantiq.fr/ark:/26678/pcrtv66rn9cbv1"/>
	<opentheso:memberOf rdf:resource="https://ark.frantiq.fr/ark:/26678/pcrtnbDLi2FkAj"/>
	<skos:exactMatch rdf:resource="https://fr.wikipedia.org/wiki/Rubis"/>
	<skos:exactMatch rdf:resource="https://www.wikidata.org/wiki/Q43088"/>
	<skos:exactMatch rdf:resource="http://vocab.getty.edu/aat/300011082"/>
	<dcterms:created rdf:datatype="http://www.w3.org/2001/XMLSchema#date">2017-08-30</dcterms:created>
	<dcterms:modified rdf:datatype="http://www.w3.org/2001/XMLSchema#date">2023-08-02</dcterms:modified>
	<dcterms:identifier>155679</dcterms:identifier>
	<dcterms:contributor>blandine.nouvel</dcterms:contributor>
	<skos:definition xml:lang="en">Transparent gemstone, bright red with pink or purple undertones (Lar.)</skos:definition>
	<skos:definition xml:lang="fr">Pierre précieuse transparente, d'un rouge vif nuancé de rose ou de pourpre (Lar.)</skos:definition>
</rdf:Description>

<rdf:Description rdf:about="https://ark.frantiq.fr/ark:/26678/pcrt1pRQD1Ircr">
	<rdf:type rdf:resource="http://www.w3.org/2004/02/skos/core#Concept"/>
	<skos:prefLabel xml:lang="fr">saphir</skos:prefLabel>
	<skos:prefLabel xml:lang="de">Saphir</skos:prefLabel>
	<skos:prefLabel xml:lang="en">sapphire</skos:prefLabel>
	<skos:prefLabel xml:lang="it">zaffiro</skos:prefLabel>
	<skos:prefLabel xml:lang="es">zafiro</skos:prefLabel>
	<skos:broader rdf:resource="https://ark.frantiq.fr/ark:/26678/pcrtzVuPZeWdAP"/>
	<skos:inScheme rdf:resource="https://ark.frantiq.fr/ark:/26678/TH_1"/>
	<opentheso:memberOf rdf:resource="https://ark.frantiq.fr/ark:/26678/pcrtv66rn9cbv1"/>
	<opentheso:memberOf rdf:resource="https://ark.frantiq.fr/ark:/26678/pcrtnbDLi2FkAj"/>
	<skos:exactMatch rdf:resource="https://fr.wikipedia.org/wiki/Saphir"/>
	<skos:exactMatch rdf:resource="https://www.wikidata.org/wiki/Q127583"/>
	<skos:exactMatch rdf:resource="http://vocab.getty.edu/aat/300011083"/>
	<dcterms:created rdf:datatype="http://www.w3.org/2001/XMLSchema#date">2017-08-30</dcterms:created>
	<dcterms:modified rdf:datatype="http://www.w3.org/2001/XMLSchema#date">2024-11-15</dcterms:modified>
	<dcterms:identifier>155680</dcterms:identifier>
	<dcterms:contributor>blandine.nouvel</dcterms:contributor>
	<dcterms:contributor>justine.vincent</dcterms:contributor>
	<skos:definition xml:lang="fr">Pierre précieuse, dont la couleur varie du bleu clair au bleu foncé, qui constitue une des variétés du corindon hyalin. (CNRTL)</skos:definition>
	<skos:definition xml:lang="en">Precious stone, varying in colour from light to dark blue, which is one of the varieties of hyaline corundum (CNRTL).</skos:definition>
	<skos:historyNote xml:lang="fr">2024-11-15 : modification de la définition.</skos:historyNote>
</rdf:Description>

<rdf:Description rdf:about="https://ark.frantiq.fr/ark:/26678/pcrtEstKLNLE1q">
	<rdf:type rdf:resource="http://www.w3.org/2004/02/skos/core#Concept"/>
	<skos:prefLabel xml:lang="de">Byssusseide</skos:prefLabel>
	<skos:prefLabel xml:lang="en">sea silk</skos:prefLabel>
	<skos:prefLabel xml:lang="es">seda de mar</skos:prefLabel>
	<skos:prefLabel xml:lang="it">seta marina</skos:prefLabel>
	<skos:prefLabel xml:lang="fr">soie de mer</skos:prefLabel>
	<skos:altLabel xml:lang="es">biso</skos:altLabel>
	<skos:altLabel xml:lang="it">bisso</skos:altLabel>
	<skos:altLabel xml:lang="fr">laine de poisson</skos:altLabel>
	<skos:altLabel xml:lang="de">Muschelseide</skos:altLabel>
	<skos:altLabel xml:lang="es">seda marina</skos:altLabel>
	<skos:altLabel xml:lang="fr">soie marine</skos:altLabel>
	<skos:related rdf:resource="https://ark.frantiq.fr/ark:/26678/pcrtbVQVTAxpc2"/>
	<skos:broader rdf:resource="https://ark.frantiq.fr/ark:/26678/pcrtwvFLgSQRs5"/>
	<skos:inScheme rdf:resource="https://ark.frantiq.fr/ark:/26678/TH_1"/>
	<opentheso:memberOf rdf:resource="https://ark.frantiq.fr/ark:/26678/pcrtv66rn9cbv1"/>
	<opentheso:memberOf rdf:resource="https://ark.frantiq.fr/ark:/26678/pcrtnbDLi2FkAj"/>
	<skos:closeMatch rdf:resource="https://fr.wikipedia.org/wiki/Byssus"/>
	<skos:exactMatch rdf:resource="https://www.wikidata.org/wiki/Q3243230"/>
	<skos:exactMatch rdf:resource="https://www.wikidata.org/wiki/Q780486"/>
	<skos:exactMatch rdf:resource="http://vocab.getty.edu/aat/300380296"/>
	<dcterms:created rdf:datatype="http://www.w3.org/2001/XMLSchema#date">2017-08-30</dcterms:created>
	<dcterms:modified rdf:datatype="http://www.w3.org/2001/XMLSchema#date">2023-08-02</dcterms:modified>
	<dcterms:identifier>155681</dcterms:identifier>
	<dcterms:contributor>blandine.nouvel</dcterms:contributor>
	<skos:definition xml:lang="en">Fabric made in ancient times from the byssus of certain shellfish.</skos:definition>
	<skos:definition xml:lang="fr">Tissu confectionné dans l'Antiquité à partir du byssus de certains coquillages.</skos:definition>
</rdf:Description>

<rdf:Description rdf:about="https://ark.frantiq.fr/ark:/26678/crtSPE6Lx4cPI">
	<rdf:type rdf:resource="http://www.w3.org/2004/02/skos/core#Concept"/>
	<skos:prefLabel xml:lang="de">Beauvaisis-Steingut</skos:prefLabel>
	<skos:prefLabel xml:lang="en">Beauvais stoneware</skos:prefLabel>
	<skos:prefLabel xml:lang="es">cerámica de Beauvaisis</skos:prefLabel>
	<skos:prefLabel xml:lang="it">ceramica di Beauvaisis</skos:prefLabel>
	<skos:prefLabel xml:lang="fr">grès du Beauvaisis</skos:prefLabel>
	<skos:broader rdf:resource="https://ark.frantiq.fr/ark:/26678/pcrtt7G9pnQlu1"/>
	<skos:inScheme rdf:resource="https://ark.frantiq.fr/ark:/26678/TH_1"/>
	<opentheso:memberOf rdf:resource="https://ark.frantiq.fr/ark:/26678/pcrtv66rn9cbv1"/>
	<opentheso:memberOf rdf:resource="https://ark.frantiq.fr/ark:/26678/pcrtnbDLi2FkAj"/>
	<skos:exactMatch rdf:resource="https://www.wikidata.org/wiki/Q88968278"/>
	<dcterms:created rdf:datatype="http://www.w3.org/2001/XMLSchema#date">2017-09-26</dcterms:created>
	<dcterms:modified rdf:datatype="http://www.w3.org/2001/XMLSchema#date">2024-10-25</dcterms:modified>
	<dcterms:identifier>155717</dcterms:identifier>
	<dcterms:contributor>blandine.nouvel</dcterms:contributor>
	<dcterms:contributor>patricia.moitrel</dcterms:contributor>
	<skos:definition xml:lang="en">Ceramic production developed in the Pays de Bray (between Dieppe and Beauvais) from the 14th to the 20th century, using fine clays that vitrify at very high temperatures (between 1150 and 1350°C). It was used for both everyday tableware and decorative ceramics. (Pactols Group)</skos:definition>
	<skos:definition xml:lang="fr">Production céramique développée dans le Pays de Bray (entre Dieppe et Beauvais) du XIVe au XXe siècle, à partir d'argiles fines se vitrifiant à très haute température (entre 1150 à 1350°C). Elle est utilisée pour la vaisselle commune comme pour la céramique décorative (plats décorés, épis de faîtage...).</skos:definition>
</rdf:Description>

<rdf:Description rdf:about="https://ark.frantiq.fr/ark:/26678/pcrtSkipOsBGML">
	<rdf:type rdf:resource="http://www.w3.org/2004/02/skos/core#Concept"/>
	<skos:prefLabel xml:lang="en">marble</skos:prefLabel>
	<skos:prefLabel xml:lang="fr">marbre</skos:prefLabel>
	<skos:prefLabel xml:lang="nl">marmer</skos:prefLabel>
	<skos:prefLabel xml:lang="it">marmo</skos:prefLabel>
	<skos:prefLabel xml:lang="es">mármol</skos:prefLabel>
	<skos:prefLabel xml:lang="de">Marmor</skos:prefLabel>
	<skos:prefLabel xml:lang="ar">مرمر</skos:prefLabel>
	<skos:related rdf:resource="https://ark.frantiq.fr/ark:/26678/pcrtXk6sdvTjnE"/>
	<skos:related rdf:resource="https://ark.frantiq.fr/ark:/26678/pcrtQuZiT5nYY2"/>
	<skos:related rdf:resource="https://ark.frantiq.fr/ark:/26678/pcrtRT5qpNmDqE"/>
	<skos:broader rdf:resource="https://ark.frantiq.fr/ark:/26678/pcrtxybfLE1dkn"/>
	<skos:inScheme rdf:resource="https://ark.frantiq.fr/ark:/26678/TH_1"/>
	<opentheso:memberOf rdf:resource="https://ark.frantiq.fr/ark:/26678/pcrtv66rn9cbv1"/>
	<opentheso:memberOf rdf:resource="https://ark.frantiq.fr/ark:/26678/pcrtnbDLi2FkAj"/>
	<opentheso:memberOf rdf:resource="https://ark.frantiq.fr/ark:/26678/pcrtv0jq332vcq3gxt5m13d5"/>
	<skos:exactMatch rdf:resource="https://catalogue.bnf.fr/ark:/12148/cb11976514t"/>
	<skos:exactMatch rdf:resource="https://www.wikidata.org/wiki/Q40861"/>
	<skos:exactMatch rdf:resource="http://vocab.getty.edu/aat/300011443"/>
	<dcterms:created rdf:datatype="http://www.w3.org/2001/XMLSchema#date">2007-02-08</dcterms:created>
	<dcterms:modified rdf:datatype="http://www.w3.org/2001/XMLSchema#date">2025-01-16</dcterms:modified>
	<dcterms:identifier>15577</dcterms:identifier>
	<dcterms:contributor>blandine.nouvel</dcterms:contributor>
	<dcterms:contributor>irene.weis</dcterms:contributor>
	<skos:definition xml:lang="en">Metamorphosed limestone of various origins and varieties, giving a compact rock, studded with fissures filled with variously coloured matter.(Atelier Silex, May 2021)</skos:definition>
	<skos:definition xml:lang="fr">Calcaire métamorphisé d'origine et de variété diverses, donnant une roche compacte, parsemée de fissures remplies de matières diversement colorées. (Atelier Silex, mai 2021)</skos:definition>
</rdf:Description>

<rdf:Description rdf:about="https://ark.frantiq.fr/ark:/26678/pcrtFxTmoqh7a3">
	<rdf:type rdf:resource="http://www.w3.org/2004/02/skos/core#Concept"/>
	<skos:prefLabel xml:lang="fr">enduit d'étanchéité</skos:prefLabel>
	<skos:prefLabel xml:lang="en">plaster sealing</skos:prefLabel>
	<skos:prefLabel xml:lang="es">sellador</skos:prefLabel>
	<skos:prefLabel xml:lang="it">sigillante</skos:prefLabel>
	<skos:prefLabel xml:lang="de">Versiegelung</skos:prefLabel>
	<skos:altLabel xml:lang="en">plaster seal</skos:altLabel>
	<skos:altLabel xml:lang="en">plaster sealant</skos:altLabel>
	<skos:altLabel xml:lang="es">sellante</skos:altLabel>
	<skos:altLabel xml:lang="it">stucco sigillante</skos:altLabel>
	<skos:related rdf:resource="https://ark.frantiq.fr/ark:/26678/pcrt6htVOpKXb1"/>
	<skos:broader rdf:resource="https://ark.frantiq.fr/ark:/26678/pcrtQuZiT5nYY2"/>
	<skos:inScheme rdf:resource="https://ark.frantiq.fr/ark:/26678/TH_1"/>
	<opentheso:memberOf rdf:resource="https://ark.frantiq.fr/ark:/26678/pcrtv66rn9cbv1"/>
	<opentheso:memberOf rdf:resource="https://ark.frantiq.fr/ark:/26678/pcrtnbDLi2FkAj"/>
	<dcterms:created rdf:datatype="http://www.w3.org/2001/XMLSchema#date">2017-10-31</dcterms:created>
	<dcterms:modified rdf:datatype="http://www.w3.org/2001/XMLSchema#date">2023-08-02</dcterms:modified>
	<dcterms:identifier>155909</dcterms:identifier>
	<dcterms:contributor>blandine.nouvel</dcterms:contributor>
	<skos:definition xml:lang="en">Product used to waterproof a surface.</skos:definition>
	<skos:definition xml:lang="fr">Produit servant à imperméabiliser une surface.</skos:definition>
</rdf:Description>

<rdf:Description rdf:about="https://ark.frantiq.fr/ark:/26678/crtHmI38AHBYS">
	<rdf:type rdf:resource="http://www.w3.org/2004/02/skos/core#Concept"/>
	<skos:prefLabel xml:lang="es">canela</skos:prefLabel>
	<skos:prefLabel xml:lang="it">cannella</skos:prefLabel>
	<skos:prefLabel xml:lang="fr">cannelle</skos:prefLabel>
	<skos:prefLabel xml:lang="en">cinnamon</skos:prefLabel>
	<skos:prefLabel xml:lang="nl">kaneel</skos:prefLabel>
	<skos:prefLabel xml:lang="de">Zimt</skos:prefLabel>
	<skos:altLabel xml:lang="fr">cinnamome</skos:altLabel>
	<skos:broader rdf:resource="https://ark.frantiq.fr/ark:/26678/pcrt0TJJTrHkN1"/>
	<skos:inScheme rdf:resource="https://ark.frantiq.fr/ark:/26678/TH_1"/>
	<opentheso:memberOf rdf:resource="https://ark.frantiq.fr/ark:/26678/pcrtv66rn9cbv1"/>
	<opentheso:memberOf rdf:resource="https://ark.frantiq.fr/ark:/26678/pcrtnbDLi2FkAj"/>
	<skos:exactMatch rdf:resource="https://www.wikidata.org/wiki/Q28165"/>
	<dcterms:created rdf:datatype="http://www.w3.org/2001/XMLSchema#date">2018-02-16</dcterms:created>
	<dcterms:modified rdf:datatype="http://www.w3.org/2001/XMLSchema#date">2023-08-02</dcterms:modified>
	<dcterms:identifier>156070</dcterms:identifier>
	<dcterms:contributor>blandine.nouvel</dcterms:contributor>
	<skos:definition xml:lang="en">Spice obtained from the inner bark of several tree species from the genus Cinnamomum (Wikipedia).</skos:definition>
	<skos:definition xml:lang="fr">Épice provenant de l'écorce intérieure d'une des espèces de cannelier (Wikipédia).</skos:definition>
</rdf:Description>

<rdf:Description rdf:about="https://ark.frantiq.fr/ark:/26678/pcrtwvFLgSQRs5">
	<rdf:type rdf:resource="http://www.w3.org/2004/02/skos/core#Concept"/>
	<skos:prefLabel xml:lang="it">materia organica</skos:prefLabel>
	<skos:prefLabel xml:lang="es">materia orgánica</skos:prefLabel>
	<skos:prefLabel xml:lang="fr">matière organique</skos:prefLabel>
	<skos:prefLabel xml:lang="en">organic matter</skos:prefLabel>
	<skos:prefLabel xml:lang="de">organisches Material</skos:prefLabel>
	<skos:prefLabel xml:lang="nl">organisch materiaal</skos:prefLabel>
	<skos:prefLabel xml:lang="ar">مادة عضوية</skos:prefLabel>
	<skos:altLabel xml:lang="it">materiale organico</skos:altLabel>
	<skos:altLabel xml:lang="fr">matériaux organiques</skos:altLabel>
	<skos:altLabel xml:lang="it">materie organiche</skos:altLabel>
	<skos:altLabel xml:lang="en">natural organic matter</skos:altLabel>
	<skos:altLabel xml:lang="en">organic material</skos:altLabel>
	<skos:related rdf:resource="https://ark.frantiq.fr/ark:/26678/pcrttQ1swNeBVe"/>
	<skos:related rdf:resource="https://ark.frantiq.fr/ark:/26678/pcrtx37ph91cww"/>
	<skos:related rdf:resource="https://ark.frantiq.fr/ark:/26678/pcrttrkqkmfrsq"/>
	<skos:narrower rdf:resource="https://ark.frantiq.fr/ark:/26678/pcrtDfHvvnBWz7"/>
	<skos:narrower rdf:resource="https://ark.frantiq.fr/ark:/26678/pcrtEstKLNLE1q"/>
	<skos:narrower rdf:resource="https://ark.frantiq.fr/ark:/26678/pcrtDffxD420gS"/>
	<skos:narrower rdf:resource="https://ark.frantiq.fr/ark:/26678/pcrttxsm3xSsiz"/>
	<skos:narrower rdf:resource="https://ark.frantiq.fr/ark:/26678/crtqg6iAF3rS7"/>
	<skos:narrower rdf:resource="https://ark.frantiq.fr/ark:/26678/pcrte3NbmKEKON"/>
	<skos:narrower rdf:resource="https://ark.frantiq.fr/ark:/26678/pcrtnHxyjOkhJw"/>
	<skos:narrower rdf:resource="https://ark.frantiq.fr/ark:/26678/pcrtW8Uu5SMsQy"/>
	<skos:narrower rdf:resource="https://ark.frantiq.fr/ark:/26678/pcrtf97bQHDGEd"/>
	<skos:narrower rdf:resource="https://ark.frantiq.fr/ark:/26678/pcrtxGxOl1KuZz"/>
	<skos:narrower rdf:resource="https://ark.frantiq.fr/ark:/26678/pcrtqvm3ztp4h8"/>
	<skos:broader rdf:resource="https://ark.frantiq.fr/ark:/26678/pcrtIMsuG0RWTs"/>
	<skos:inScheme rdf:resource="https://ark.frantiq.fr/ark:/26678/TH_1"/>
	<opentheso:memberOf rdf:resource="https://ark.frantiq.fr/ark:/26678/pcrtv66rn9cbv1"/>
	<opentheso:memberOf rdf:resource="https://ark.frantiq.fr/ark:/26678/pcrtnbDLi2FkAj"/>
	<skos:exactMatch rdf:resource="https://www.wikidata.org/wiki/Q1783121"/>
	<skos:exactMatch rdf:resource="http://vocab.getty.edu/aat/300011792"/>
	<dcterms:created rdf:datatype="http://www.w3.org/2001/XMLSchema#date">2007-02-08</dcterms:created>
	<dcterms:modified rdf:datatype="http://www.w3.org/2001/XMLSchema#date">2023-08-02</dcterms:modified>
	<dcterms:identifier>15616</dcterms:identifier>
	<dcterms:contributor>blandine.nouvel</dcterms:contributor>
	<skos:definition xml:lang="en">Matter produced by living organisms (plants, animals, fungi and other decomposers, including micro-organisms). (wp)</skos:definition>
	<skos:definition xml:lang="fr">Matière fabriquée par les êtres vivants (végétaux, animaux, champignons et autres décomposeurs dont micro-organismes). (wp)</skos:definition>
</rdf:Description>

<rdf:Description rdf:about="https://ark.frantiq.fr/ark:/26678/pcrtIMsuG0RWTs">
	<rdf:type rdf:resource="http://www.w3.org/2004/02/skos/core#Concept"/>
	<skos:prefLabel xml:lang="nl">materialen</skos:prefLabel>
	<skos:prefLabel xml:lang="es">materiales</skos:prefLabel>
	<skos:prefLabel xml:lang="it">materiali</skos:prefLabel>
	<skos:prefLabel xml:lang="de">Materialien</skos:prefLabel>
	<skos:prefLabel xml:lang="en">materials</skos:prefLabel>
	<skos:prefLabel xml:lang="fr">matériaux</skos:prefLabel>
	<skos:prefLabel xml:lang="ar">مواد</skos:prefLabel>
	<skos:topConceptOf rdf:resource="https://ark.frantiq.fr/ark:/26678/TH_1"/>
	<skos:narrower rdf:resource="https://ark.frantiq.fr/ark:/26678/pcrtgcn5U8laUN"/>
	<skos:narrower rdf:resource="https://ark.frantiq.fr/ark:/26678/pcrt6z097U6IUf"/>
	<skos:narrower rdf:resource="https://ark.frantiq.fr/ark:/26678/pcrtO40ZLI4giK"/>
	<skos:narrower rdf:resource="https://ark.frantiq.fr/ark:/26678/pcrtQuZiT5nYY2"/>
	<skos:narrower rdf:resource="https://ark.frantiq.fr/ark:/26678/pcrtLpvrsa9RIz"/>
	<skos:narrower rdf:resource="https://ark.frantiq.fr/ark:/26678/pcrtuxpF5YgM3S"/>
	<skos:narrower rdf:resource="https://ark.frantiq.fr/ark:/26678/pcrt8yYh5xgMeO"/>
	<skos:narrower rdf:resource="https://ark.frantiq.fr/ark:/26678/pcrt3pmFUqt27w"/>
	<skos:narrower rdf:resource="https://ark.frantiq.fr/ark:/26678/pcrtwvFLgSQRs5"/>
	<skos:narrower rdf:resource="https://ark.frantiq.fr/ark:/26678/pcrtkn1hAXHveS"/>
	<skos:narrower rdf:resource="https://ark.frantiq.fr/ark:/26678/pcrtbZkzVXTkJI"/>
	<skos:narrower rdf:resource="https://ark.frantiq.fr/ark:/26678/pcrtGzQPnntJa1"/>
	<skos:narrower rdf:resource="https://ark.frantiq.fr/ark:/26678/pcrtZETJwE7RTQ"/>
	<skos:narrower rdf:resource="https://ark.frantiq.fr/ark:/26678/pcrtSVdwKcS3MI"/>
	<skos:narrower rdf:resource="https://ark.frantiq.fr/ark:/26678/pcrtfx4s0yvSLj"/>
	<skos:narrower rdf:resource="https://ark.frantiq.fr/ark:/26678/pcrthAOjGBEfZk"/>
	<skos:narrower rdf:resource="https://ark.frantiq.fr/ark:/26678/pcrtqGQOorLDxx"/>
	<skos:narrower rdf:resource="https://ark.frantiq.fr/ark:/26678/pcrttS4bFv2ezb"/>
	<skos:narrower rdf:resource="https://ark.frantiq.fr/ark:/26678/pcrt4GqimUgoOq"/>
	<skos:narrower rdf:resource="https://ark.frantiq.fr/ark:/26678/pcrty2mcsksa6s"/>
	<skos:narrower rdf:resource="https://ark.frantiq.fr/ark:/26678/pcrtjbpmw8qvrn"/>
	<skos:narrower rdf:resource="https://ark.frantiq.fr/ark:/26678/pcrtx37ph91cww"/>
	<skos:narrower rdf:resource="https://ark.frantiq.fr/ark:/26678/pcrtvKH7mF2Oas"/>
	<skos:narrower rdf:resource="https://ark.frantiq.fr/ark:/26678/pcrtd1cZp0yBER"/>
	<skos:inScheme rdf:resource="https://ark.frantiq.fr/ark:/26678/TH_1"/>
	<opentheso:memberOf rdf:resource="https://ark.frantiq.fr/ark:/26678/pcrtv66rn9cbv1"/>
	<opentheso:memberOf rdf:resource="https://ark.frantiq.fr/ark:/26678/pcrtnbDLi2FkAj"/>
	<skos:exactMatch rdf:resource="https://catalogue.bnf.fr/ark:/12148/cb11935841g"/>
	<skos:exactMatch rdf:resource="https://vocabs.dariah.eu/bbt/Concept/000003"/>
	<skos:exactMatch rdf:resource="https://www.wikidata.org/wiki/Q214609"/>
	<skos:exactMatch rdf:resource="http://vocab.getty.edu/aat/300010357"/>
	<dcterms:created rdf:datatype="http://www.w3.org/2001/XMLSchema#date">2007-02-08</dcterms:created>
	<dcterms:modified rdf:datatype="http://www.w3.org/2001/XMLSchema#date">2023-08-02</dcterms:modified>
	<dcterms:identifier>15621</dcterms:identifier>
	<dcterms:contributor>blandine.nouvel</dcterms:contributor>
	<skos:definition xml:lang="fr">Cette branche concerne les substances physiques qui composent les objets matériels ou sont utilisés dans leur fabrication. Elle peut inclure les matières premières, transformées ou non, les matériaux façonnés et intégrés à des objets. (d'après le DARIAH Backbone Thesaurus, v. 1.2.8)</skos:definition>
	<skos:scopeNote xml:lang="fr">Concept de niveau supérieur, utiliser de préférence des concepts plus spécifiques.</skos:scopeNote>
	<skos:scopeNote xml:lang="en">This term classifies physical substances that are constituents of material objects or are used in their construction, but whose individual substance is not a factor in the objects’ function (e.g. gold, water, bricks, etc.) The term may include pure raw materials, processed or unprocessed, and also materials that have been modelled and are incorporated into objects. Their main attribute is that they cannot be individualized, that is, they cannot be distinct  units  with clear and distinct boundaries or roles in respect to other units of the same or different kind. (BBT V 1.2.2)</skos:scopeNote>
</rdf:Description>

<rdf:Description rdf:about="https://ark.frantiq.fr/ark:/26678/pcrtyx3UIr91zi">
	<rdf:type rdf:resource="http://www.w3.org/2004/02/skos/core#Concept"/>
	<skos:prefLabel xml:lang="de">Glimmer</skos:prefLabel>
	<skos:prefLabel xml:lang="en">mica</skos:prefLabel>
	<skos:prefLabel xml:lang="es">mica</skos:prefLabel>
	<skos:prefLabel xml:lang="fr">mica</skos:prefLabel>
	<skos:prefLabel xml:lang="it">mica</skos:prefLabel>
	<skos:prefLabel xml:lang="nl">mica</skos:prefLabel>
	<skos:prefLabel xml:lang="ar">ميكا</skos:prefLabel>
	<skos:altLabel xml:lang="en">common mica</skos:altLabel>
	<skos:altLabel xml:lang="en">isinglass</skos:altLabel>
	<skos:altLabel xml:lang="it">miche</skos:altLabel>
	<skos:altLabel xml:lang="en">muscovy glass</skos:altLabel>
	<skos:altLabel xml:lang="en">potash mica</skos:altLabel>
	<skos:altLabel xml:lang="ar">طَلْق</skos:altLabel>
	<skos:broader rdf:resource="https://ark.frantiq.fr/ark:/26678/pcrty2mcsksa6s"/>
	<skos:inScheme rdf:resource="https://ark.frantiq.fr/ark:/26678/TH_1"/>
	<opentheso:memberOf rdf:resource="https://ark.frantiq.fr/ark:/26678/pcrtv66rn9cbv1"/>
	<opentheso:memberOf rdf:resource="https://ark.frantiq.fr/ark:/26678/pcrtnbDLi2FkAj"/>
	<skos:exactMatch rdf:resource="https://catalogue.bnf.fr/ark:/12148/cb11958903b"/>
	<skos:exactMatch rdf:resource="https://www.wikidata.org/wiki/Q114675"/>
	<skos:exactMatch rdf:resource="http://vocab.getty.edu/aat/300011124"/>
	<dcterms:created rdf:datatype="http://www.w3.org/2001/XMLSchema#date">2007-02-08</dcterms:created>
	<dcterms:modified rdf:datatype="http://www.w3.org/2001/XMLSchema#date">2024-11-18</dcterms:modified>
	<dcterms:identifier>15652</dcterms:identifier>
	<dcterms:contributor>blandine.nouvel</dcterms:contributor>
	<dcterms:contributor>justine.vincent</dcterms:contributor>
	<skos:definition xml:lang="en">Name of a family of minerals in the silicate subgroup of the phyllosilicate group, composed mainly of aluminium and potassium silicate, which together with quartz and feldspar form one of the constituents of granite (Wikipedia, 2021).</skos:definition>
	<skos:definition xml:lang="fr">Nom d'une famille de minéraux, du groupe des silicates sous-groupe des phyllosilicates formé principalement de silicate d'aluminium et de potassium, formant avec le quartz et le feldspath l'un des constituants du granite. (Wikipedia, 2021)</skos:definition>
</rdf:Description>

<rdf:Description rdf:about="https://ark.frantiq.fr/ark:/26678/pcrtsPauzzRS5z">
	<rdf:type rdf:resource="http://www.w3.org/2004/02/skos/core#Concept"/>
	<skos:prefLabel xml:lang="en">honey</skos:prefLabel>
	<skos:prefLabel xml:lang="de">Honig</skos:prefLabel>
	<skos:prefLabel xml:lang="nl">honing</skos:prefLabel>
	<skos:prefLabel xml:lang="es">miel</skos:prefLabel>
	<skos:prefLabel xml:lang="fr">miel</skos:prefLabel>
	<skos:prefLabel xml:lang="it">miele</skos:prefLabel>
	<skos:prefLabel xml:lang="ar">عَسَل</skos:prefLabel>
	<skos:related rdf:resource="https://ark.frantiq.fr/ark:/26678/pcrtnpPag9iONJ"/>
	<skos:related rdf:resource="https://ark.frantiq.fr/ark:/26678/pcrtU8RLhLoUoy"/>
	<skos:related rdf:resource="https://ark.frantiq.fr/ark:/26678/pcrt90QbSfsSnc"/>
	<skos:broader rdf:resource="https://ark.frantiq.fr/ark:/26678/pcrtUTZqItd8SL"/>
	<skos:inScheme rdf:resource="https://ark.frantiq.fr/ark:/26678/TH_1"/>
	<opentheso:memberOf rdf:resource="https://ark.frantiq.fr/ark:/26678/pcrtv66rn9cbv1"/>
	<opentheso:memberOf rdf:resource="https://ark.frantiq.fr/ark:/26678/pcrtnbDLi2FkAj"/>
	<skos:exactMatch rdf:resource="https://catalogue.bnf.fr/ark:/12148/cb11932357r"/>
	<skos:exactMatch rdf:resource="https://www.wikidata.org/wiki/Q10987"/>
	<skos:exactMatch rdf:resource="http://vocab.getty.edu/aat/300191621"/>
	<dcterms:created rdf:datatype="http://www.w3.org/2001/XMLSchema#date">2007-02-08</dcterms:created>
	<dcterms:modified rdf:datatype="http://www.w3.org/2001/XMLSchema#date">2023-08-02</dcterms:modified>
	<dcterms:identifier>15658</dcterms:identifier>
	<dcterms:contributor>blandine.nouvel</dcterms:contributor>
	<skos:definition xml:lang="en">A sweet substance produced by bees.</skos:definition>
	<skos:definition xml:lang="fr">Substance sucrée produite par les abeilles.</skos:definition>
</rdf:Description>

<rdf:Description rdf:about="https://ark.frantiq.fr/ark:/26678/pcrt5bIL1UtwcT">
	<rdf:type rdf:resource="http://www.w3.org/2004/02/skos/core#Concept"/>
	<skos:prefLabel xml:lang="nl">erts</skos:prefLabel>
	<skos:prefLabel xml:lang="de">Erz</skos:prefLabel>
	<skos:prefLabel xml:lang="es">mena</skos:prefLabel>
	<skos:prefLabel xml:lang="fr">minerai</skos:prefLabel>
	<skos:prefLabel xml:lang="it">minerale grezzo</skos:prefLabel>
	<skos:prefLabel xml:lang="en">ore</skos:prefLabel>
	<skos:prefLabel xml:lang="ar">رِكاز</skos:prefLabel>
	<skos:altLabel xml:lang="fr">minéraux</skos:altLabel>
	<skos:altLabel xml:lang="ar">معدن خام</skos:altLabel>
	<skos:related rdf:resource="https://ark.frantiq.fr/ark:/26678/pcrtDISmiAdvys"/>
	<skos:related rdf:resource="https://ark.frantiq.fr/ark:/26678/pcrtuVBFofOdjD"/>
	<skos:related rdf:resource="https://ark.frantiq.fr/ark:/26678/pcrttHNINn8k7j"/>
	<skos:related rdf:resource="https://ark.frantiq.fr/ark:/26678/pcrtkn1hAXHveS"/>
	<skos:related rdf:resource="https://ark.frantiq.fr/ark:/26678/crtYQmrPQmygE"/>
	<skos:related rdf:resource="https://ark.frantiq.fr/ark:/26678/pcrty2mcsksa6s"/>
	<skos:broader rdf:resource="https://ark.frantiq.fr/ark:/26678/pcrtSVdwKcS3MI"/>
	<skos:inScheme rdf:resource="https://ark.frantiq.fr/ark:/26678/TH_1"/>
	<opentheso:memberOf rdf:resource="https://ark.frantiq.fr/ark:/26678/pcrtv66rn9cbv1"/>
	<opentheso:memberOf rdf:resource="https://ark.frantiq.fr/ark:/26678/pcrtnbDLi2FkAj"/>
	<opentheso:memberOf rdf:resource="https://ark.frantiq.fr/ark:/26678/pcrtv0jq332vcq3gxt5m13d5"/>
	<skos:exactMatch rdf:resource="https://www.wikidata.org/wiki/Q102798"/>
	<skos:exactMatch rdf:resource="http://vocab.getty.edu/aat/300152583"/>
	<dcterms:created rdf:datatype="http://www.w3.org/2001/XMLSchema#date">2007-02-08</dcterms:created>
	<dcterms:modified rdf:datatype="http://www.w3.org/2001/XMLSchema#date">2024-10-18</dcterms:modified>
	<dcterms:identifier>15666</dcterms:identifier>
	<dcterms:contributor>blandine.nouvel</dcterms:contributor>
	<dcterms:contributor>irene.weis</dcterms:contributor>
	<dcterms:contributor>justine.vincent</dcterms:contributor>
	<skos:definition xml:lang="en">Rock containing useful minerals in sufficiently high proportions to justify exploitation, and requiring processing to be used by industry (Wikipedia).</skos:definition>
	<skos:definition xml:lang="fr">Roche contenant des minéraux utiles en proportion suffisamment intéressante pour justifier l'exploitation, et nécessitant une transformation pour être utilisés par l'industrie (Wikipédia).</skos:definition>
</rdf:Description>

<rdf:Description rdf:about="https://ark.frantiq.fr/ark:/26678/pcrtEWWJvOVoh5">
	<rdf:type rdf:resource="http://www.w3.org/2004/02/skos/core#Concept"/>
	<skos:prefLabel xml:lang="de">Baumörtel</skos:prefLabel>
	<skos:prefLabel xml:lang="it">malta</skos:prefLabel>
	<skos:prefLabel xml:lang="en">mortar (masonry)</skos:prefLabel>
	<skos:prefLabel xml:lang="nl">mortel</skos:prefLabel>
	<skos:prefLabel xml:lang="es">mortero de construccion</skos:prefLabel>
	<skos:prefLabel xml:lang="fr">mortier de construction</skos:prefLabel>
	<skos:prefLabel xml:lang="ar">مِلاط</skos:prefLabel>
	<skos:altLabel xml:lang="it">malta cementizia</skos:altLabel>
	<skos:altLabel xml:lang="en">mortar (cement)</skos:altLabel>
	<skos:altLabel xml:lang="fr">mortier de chaux</skos:altLabel>
	<skos:related rdf:resource="https://ark.frantiq.fr/ark:/26678/pcrtUxTj7SSjjU"/>
	<skos:related rdf:resource="https://ark.frantiq.fr/ark:/26678/pcrtvRM2ZVPsLA"/>
	<skos:related rdf:resource="https://ark.frantiq.fr/ark:/26678/pcrtAOIuwSlK60"/>
	<skos:related rdf:resource="https://ark.frantiq.fr/ark:/26678/pcrtrdsp44jvsk0qqqkndb9g"/>
	<skos:narrower rdf:resource="https://ark.frantiq.fr/ark:/26678/pcrt4nvgWBQ59k"/>
	<skos:narrower rdf:resource="https://ark.frantiq.fr/ark:/26678/pcrttk3hqkx8s7049j925sxn"/>
	<skos:broader rdf:resource="https://ark.frantiq.fr/ark:/26678/pcrtQuZiT5nYY2"/>
	<skos:inScheme rdf:resource="https://ark.frantiq.fr/ark:/26678/TH_1"/>
	<opentheso:memberOf rdf:resource="https://ark.frantiq.fr/ark:/26678/pcrtv66rn9cbv1"/>
	<opentheso:memberOf rdf:resource="https://ark.frantiq.fr/ark:/26678/pcrtnbDLi2FkAj"/>
	<opentheso:memberOf rdf:resource="https://ark.frantiq.fr/ark:/26678/pcrtv0jq332vcq3gxt5m13d5"/>
	<skos:exactMatch rdf:resource="https://www.wikidata.org/wiki/Q189566"/>
	<skos:exactMatch rdf:resource="https://www.wikidata.org/wiki/Q911063"/>
	<dcterms:created rdf:datatype="http://www.w3.org/2001/XMLSchema#date">2007-02-08</dcterms:created>
	<dcterms:modified rdf:datatype="http://www.w3.org/2001/XMLSchema#date">2024-11-26</dcterms:modified>
	<dcterms:identifier>15753</dcterms:identifier>
	<dcterms:contributor>blandine.nouvel</dcterms:contributor>
	<dcterms:contributor>irene.weis</dcterms:contributor>
	<dcterms:contributor>patricia.moitrel</dcterms:contributor>
	<dcterms:contributor>remi.ancel</dcterms:contributor>
	<skos:definition xml:lang="fr">Mélange constitué de ciment ou de chaux, de sable et d'eau (Lar.).</skos:definition>
	<skos:definition xml:lang="en">A mixture of cement or lime, sand and water (Lar.).</skos:definition>
	<skos:historyNote xml:lang="fr">2024-03-29 : réduction de la définition.</skos:historyNote>
</rdf:Description>

<rdf:Description rdf:about="https://ark.frantiq.fr/ark:/26678/pcrtkn1hAXHveS">
	<rdf:type rdf:resource="http://www.w3.org/2004/02/skos/core#Concept"/>
	<skos:prefLabel xml:lang="nl">metaal</skos:prefLabel>
	<skos:prefLabel xml:lang="en">metal</skos:prefLabel>
	<skos:prefLabel xml:lang="es">metal</skos:prefLabel>
	<skos:prefLabel xml:lang="fr">métal</skos:prefLabel>
	<skos:prefLabel xml:lang="de">Metall</skos:prefLabel>
	<skos:prefLabel xml:lang="it">metallo</skos:prefLabel>
	<skos:prefLabel xml:lang="ar">فِلِزّ</skos:prefLabel>
	<skos:related rdf:resource="https://ark.frantiq.fr/ark:/26678/pcrtFQKZJWgr7c"/>
	<skos:related rdf:resource="https://ark.frantiq.fr/ark:/26678/pcrtuVBFofOdjD"/>
	<skos:related rdf:resource="https://ark.frantiq.fr/ark:/26678/pcrt5bIL1UtwcT"/>
	<skos:related rdf:resource="https://ark.frantiq.fr/ark:/26678/pcrtuf9JSs9vo6"/>
	<skos:related rdf:resource="https://ark.frantiq.fr/ark:/26678/pcrt6yec4O2agc"/>
	<skos:related rdf:resource="https://ark.frantiq.fr/ark:/26678/pcrtD8bo5lH0H4"/>
	<skos:narrower rdf:resource="https://ark.frantiq.fr/ark:/26678/pcrtzcGlM17go5"/>
	<skos:narrower rdf:resource="https://ark.frantiq.fr/ark:/26678/pcrtuV4RYc06TP"/>
	<skos:narrower rdf:resource="https://ark.frantiq.fr/ark:/26678/pcrtcWoSlbWLE0"/>
	<skos:narrower rdf:resource="https://ark.frantiq.fr/ark:/26678/pcrt16pnvNar4g"/>
	<skos:narrower rdf:resource="https://ark.frantiq.fr/ark:/26678/pcrtJWWucnutA0"/>
	<skos:narrower rdf:resource="https://ark.frantiq.fr/ark:/26678/pcrtp5MND6qfnb"/>
	<skos:narrower rdf:resource="https://ark.frantiq.fr/ark:/26678/pcrtQe4n9vGjl0"/>
	<skos:narrower rdf:resource="https://ark.frantiq.fr/ark:/26678/pcrtuihSl3eSnW"/>
	<skos:narrower rdf:resource="https://ark.frantiq.fr/ark:/26678/pcrtbLhpWhz8H6"/>
	<skos:narrower rdf:resource="https://ark.frantiq.fr/ark:/26678/pcrtEpGlZykUTy"/>
	<skos:narrower rdf:resource="https://ark.frantiq.fr/ark:/26678/pcrtAhu8O29Xb2"/>
	<skos:narrower rdf:resource="https://ark.frantiq.fr/ark:/26678/pcrtGpmPNJ0jRl"/>
	<skos:narrower rdf:resource="https://ark.frantiq.fr/ark:/26678/pcrtp0jS51rXL1"/>
	<skos:narrower rdf:resource="https://ark.frantiq.fr/ark:/26678/pcrtKASHLmba7X"/>
	<skos:broader rdf:resource="https://ark.frantiq.fr/ark:/26678/pcrtIMsuG0RWTs"/>
	<skos:inScheme rdf:resource="https://ark.frantiq.fr/ark:/26678/TH_1"/>
	<opentheso:memberOf rdf:resource="https://ark.frantiq.fr/ark:/26678/pcrtv66rn9cbv1"/>
	<opentheso:memberOf rdf:resource="https://ark.frantiq.fr/ark:/26678/pcrtnbDLi2FkAj"/>
	<skos:exactMatch rdf:resource="https://catalogue.bnf.fr/ark:/12148/cb11935875s"/>
	<skos:exactMatch rdf:resource="https://www.wikidata.org/wiki/Q11426"/>
	<skos:exactMatch rdf:resource="http://vocab.getty.edu/aat/300010900"/>
	<dcterms:created rdf:datatype="http://www.w3.org/2001/XMLSchema#date">2007-02-08</dcterms:created>
	<dcterms:modified rdf:datatype="http://www.w3.org/2001/XMLSchema#date">2023-08-02</dcterms:modified>
	<dcterms:identifier>15844</dcterms:identifier>
	<dcterms:contributor>blandine.nouvel</dcterms:contributor>
	<skos:definition xml:lang="en">Generic name for any simple body with a particular lustre (metallic lustre), which is a good conductor of heat and electricity and forms basic oxides when combined with oxygen (dic. Robert).</skos:definition>
	<skos:definition xml:lang="fr">Nom générique désignant tout corps simple, doué d'un éclat particulier (éclat métallique), bon conducteur de la chaleur et de l'électricité et formant, par combinaison avec l'oxygène, des oxydes basiques (dic. Robert).</skos:definition>
</rdf:Description>

<rdf:Description rdf:about="https://ark.frantiq.fr/ark:/26678/pcrtgefwJa13yZ">
	<rdf:type rdf:resource="http://www.w3.org/2004/02/skos/core#Concept"/>
	<skos:prefLabel xml:lang="nl">obsidiaan</skos:prefLabel>
	<skos:prefLabel xml:lang="en">obsidian</skos:prefLabel>
	<skos:prefLabel xml:lang="de">Obsidian</skos:prefLabel>
	<skos:prefLabel xml:lang="es">obsidiana</skos:prefLabel>
	<skos:prefLabel xml:lang="fr">obsidienne</skos:prefLabel>
	<skos:prefLabel xml:lang="it">ossidiana</skos:prefLabel>
	<skos:prefLabel xml:lang="ar">السَبج</skos:prefLabel>
	<skos:related rdf:resource="https://ark.frantiq.fr/ark:/26678/pcrtJt3ZKiNEFK"/>
	<skos:related rdf:resource="https://ark.frantiq.fr/ark:/26678/pcrtbAIySxYMnZ"/>
	<skos:related rdf:resource="https://ark.frantiq.fr/ark:/26678/pcrtYdgGceSgwI"/>
	<skos:broader rdf:resource="https://ark.frantiq.fr/ark:/26678/pcrtmxvuuXHSTS"/>
	<skos:inScheme rdf:resource="https://ark.frantiq.fr/ark:/26678/TH_1"/>
	<opentheso:memberOf rdf:resource="https://ark.frantiq.fr/ark:/26678/pcrtv66rn9cbv1"/>
	<opentheso:memberOf rdf:resource="https://ark.frantiq.fr/ark:/26678/pcrtnbDLi2FkAj"/>
	<skos:exactMatch rdf:resource="https://catalogue.bnf.fr/ark:/12148/cb119834052"/>
	<skos:exactMatch rdf:resource="https://www.wikidata.org/wiki/Q53754"/>
	<skos:exactMatch rdf:resource="http://vocab.getty.edu/aat/300011254"/>
	<dcterms:created rdf:datatype="http://www.w3.org/2001/XMLSchema#date">2007-02-08</dcterms:created>
	<dcterms:modified rdf:datatype="http://www.w3.org/2001/XMLSchema#date">2023-08-02</dcterms:modified>
	<dcterms:identifier>15950</dcterms:identifier>
	<dcterms:contributor>blandine.nouvel</dcterms:contributor>
	<skos:definition xml:lang="en">Black volcanic glass with a smooth conchoidal fracture and a chemical composition of rhyolite or sometimes trachyte (Lozet &amp;amp; Mathieu, Dictionnaire de science du sol. Ed. Technique et Documentation Lavoisier)</skos:definition>
	<skos:definition xml:lang="fr">Verre volcanique noir à cassure lisse conchoïdale, à composition chimique de rhyolite ou parfois de trachyte. (Lozet &amp;amp; Mathieu, Dictionnaire de science du sol. Ed. Technique et Documentation Lavoisier)</skos:definition>
</rdf:Description>

<rdf:Description rdf:about="https://ark.frantiq.fr/ark:/26678/pcrttnySGIGsj6">
	<rdf:type rdf:resource="http://www.w3.org/2004/02/skos/core#Concept"/>
	<skos:prefLabel xml:lang="en">ochre</skos:prefLabel>
	<skos:prefLabel xml:lang="de">Ocker</skos:prefLabel>
	<skos:prefLabel xml:lang="it">ocra</skos:prefLabel>
	<skos:prefLabel xml:lang="es">ocre</skos:prefLabel>
	<skos:prefLabel xml:lang="fr">ocre</skos:prefLabel>
	<skos:prefLabel xml:lang="nl">oker</skos:prefLabel>
	<skos:prefLabel xml:lang="ar">مغرة</skos:prefLabel>
	<skos:altLabel xml:lang="en">clay earth pigment</skos:altLabel>
	<skos:related rdf:resource="https://ark.frantiq.fr/ark:/26678/pcrtu5RUM9S618"/>
	<skos:related rdf:resource="https://ark.frantiq.fr/ark:/26678/pcrtuFMPNUEKWb"/>
	<skos:related rdf:resource="https://ark.frantiq.fr/ark:/26678/pcrtGzQPnntJa1"/>
	<skos:broader rdf:resource="https://ark.frantiq.fr/ark:/26678/pcrto44p1SaKFn"/>
	<skos:inScheme rdf:resource="https://ark.frantiq.fr/ark:/26678/TH_1"/>
	<opentheso:memberOf rdf:resource="https://ark.frantiq.fr/ark:/26678/pcrtv66rn9cbv1"/>
	<opentheso:memberOf rdf:resource="https://ark.frantiq.fr/ark:/26678/pcrtnbDLi2FkAj"/>
	<opentheso:memberOf rdf:resource="https://ark.frantiq.fr/ark:/26678/pcrtv0jq332vcq3gxt5m13d5"/>
	<skos:exactMatch rdf:resource="https://www.wikidata.org/wiki/Q194191"/>
	<dcterms:created rdf:datatype="http://www.w3.org/2001/XMLSchema#date">2007-02-08</dcterms:created>
	<dcterms:modified rdf:datatype="http://www.w3.org/2001/XMLSchema#date">2024-03-21</dcterms:modified>
	<dcterms:identifier>15955</dcterms:identifier>
	<dcterms:contributor>blandine.nouvel</dcterms:contributor>
	<dcterms:contributor>irene.weis</dcterms:contributor>
	<skos:definition xml:lang="fr">Roche ferrique composée d'argile pure (kaolinite) colorée par un pigment d'origine minérale (un hydroxyde de fer : l’hématite pour l'ocre rouge, la limonite pour la brune et goethite pour la jaune) (Wikipédia)</skos:definition>
</rdf:Description>

<rdf:Description rdf:about="https://ark.frantiq.fr/ark:/26678/pcrtiaewgLXnZc">
	<rdf:type rdf:resource="http://www.w3.org/2004/02/skos/core#Concept"/>
	<skos:prefLabel xml:lang="es">aceituna</skos:prefLabel>
	<skos:prefLabel xml:lang="nl">olijf</skos:prefLabel>
	<skos:prefLabel xml:lang="it">oliva</skos:prefLabel>
	<skos:prefLabel xml:lang="en">olive</skos:prefLabel>
	<skos:prefLabel xml:lang="fr">olive</skos:prefLabel>
	<skos:prefLabel xml:lang="de">Olive</skos:prefLabel>
	<skos:prefLabel xml:lang="ar">زيتون</skos:prefLabel>
	<skos:related rdf:resource="https://ark.frantiq.fr/ark:/26678/pcrtDFvOrje3j0"/>
	<skos:related rdf:resource="https://ark.frantiq.fr/ark:/26678/crtnRFSZO3uLv"/>
	<skos:related rdf:resource="https://ark.frantiq.fr/ark:/26678/crtXXzLndpZbJ"/>
	<skos:related rdf:resource="https://ark.frantiq.fr/ark:/26678/pcrteZDglJiqWF"/>
	<skos:broader rdf:resource="https://ark.frantiq.fr/ark:/26678/pcrtgcn5U8laUN"/>
	<skos:inScheme rdf:resource="https://ark.frantiq.fr/ark:/26678/TH_1"/>
	<opentheso:memberOf rdf:resource="https://ark.frantiq.fr/ark:/26678/pcrtv66rn9cbv1"/>
	<opentheso:memberOf rdf:resource="https://ark.frantiq.fr/ark:/26678/pcrtnbDLi2FkAj"/>
	<skos:exactMatch rdf:resource="https://www.wikidata.org/wiki/Q1621080"/>
	<skos:exactMatch rdf:resource="http://vocab.getty.edu/aat/300266440"/>
	<dcterms:created rdf:datatype="http://www.w3.org/2001/XMLSchema#date">2007-02-08</dcterms:created>
	<dcterms:modified rdf:datatype="http://www.w3.org/2001/XMLSchema#date">2023-08-02</dcterms:modified>
	<dcterms:identifier>15969</dcterms:identifier>
	<dcterms:contributor>blandine.nouvel</dcterms:contributor>
	<skos:definition xml:lang="en">Fruit of the olive tree.</skos:definition>
	<skos:definition xml:lang="fr">Fruit de l'olivier.</skos:definition>
</rdf:Description>

<rdf:Description rdf:about="https://ark.frantiq.fr/ark:/26678/pcrtbZkzVXTkJI">
	<rdf:type rdf:resource="http://www.w3.org/2004/02/skos/core#Concept"/>
	<skos:prefLabel xml:lang="de">Balsam</skos:prefLabel>
	<skos:prefLabel xml:lang="fr">onguent</skos:prefLabel>
	<skos:prefLabel xml:lang="en">unguent</skos:prefLabel>
	<skos:prefLabel xml:lang="it">unguento</skos:prefLabel>
	<skos:prefLabel xml:lang="es">ungüento</skos:prefLabel>
	<skos:prefLabel xml:lang="nl">zalf</skos:prefLabel>
	<skos:prefLabel xml:lang="ar">مَرْهَم</skos:prefLabel>
	<skos:altLabel xml:lang="fr">baume</skos:altLabel>
	<skos:altLabel xml:lang="en">ointment</skos:altLabel>
	<skos:altLabel xml:lang="es">pomada</skos:altLabel>
	<skos:altLabel xml:lang="fr">pommade</skos:altLabel>
	<skos:related rdf:resource="https://ark.frantiq.fr/ark:/26678/pcrt0rEs0KaVGT"/>
	<skos:broader rdf:resource="https://ark.frantiq.fr/ark:/26678/pcrtIMsuG0RWTs"/>
	<skos:inScheme rdf:resource="https://ark.frantiq.fr/ark:/26678/TH_1"/>
	<opentheso:memberOf rdf:resource="https://ark.frantiq.fr/ark:/26678/pcrtv66rn9cbv1"/>
	<opentheso:memberOf rdf:resource="https://ark.frantiq.fr/ark:/26678/pcrtnbDLi2FkAj"/>
	<skos:exactMatch rdf:resource="https://www.wikidata.org/wiki/Q1776037"/>
	<skos:exactMatch rdf:resource="https://www.wikidata.org/wiki/Q4004659"/>
	<skos:exactMatch rdf:resource="http://vocab.getty.edu/aat/300012891"/>
	<dcterms:created rdf:datatype="http://www.w3.org/2001/XMLSchema#date">2007-02-08</dcterms:created>
	<dcterms:modified rdf:datatype="http://www.w3.org/2001/XMLSchema#date">2023-08-02</dcterms:modified>
	<dcterms:identifier>15978</dcterms:identifier>
	<dcterms:contributor>blandine.nouvel</dcterms:contributor>
	<skos:definition xml:lang="en">Semi-solid preparation intended to be applied most often to the skin (cutaneous and transcutaneous route). (wikipedia)</skos:definition>
	<skos:definition xml:lang="fr">Préparation semi-solide destinée à être appliquée le plus souvent sur la peau (voie cutanée et voie transcutanée). (wikipedia)</skos:definition>
</rdf:Description>

<rdf:Description rdf:about="https://ark.frantiq.fr/ark:/26678/pcrtjyrVAHv1m8">
	<rdf:type rdf:resource="http://www.w3.org/2004/02/skos/core#Concept"/>
	<skos:prefLabel xml:lang="nl">opaal</skos:prefLabel>
	<skos:prefLabel xml:lang="en">opal</skos:prefLabel>
	<skos:prefLabel xml:lang="de">Opal</skos:prefLabel>
	<skos:prefLabel xml:lang="fr">opale</skos:prefLabel>
	<skos:prefLabel xml:lang="it">opale</skos:prefLabel>
	<skos:prefLabel xml:lang="es">ópalo</skos:prefLabel>
	<skos:prefLabel xml:lang="ar">حجر عين الهر</skos:prefLabel>
	<skos:broader rdf:resource="https://ark.frantiq.fr/ark:/26678/pcrtJt3ZKiNEFK"/>
	<skos:inScheme rdf:resource="https://ark.frantiq.fr/ark:/26678/TH_1"/>
	<opentheso:memberOf rdf:resource="https://ark.frantiq.fr/ark:/26678/pcrtv66rn9cbv1"/>
	<opentheso:memberOf rdf:resource="https://ark.frantiq.fr/ark:/26678/pcrtnbDLi2FkAj"/>
	<skos:exactMatch rdf:resource="https://www.wikidata.org/wiki/Q171058"/>
	<skos:exactMatch rdf:resource="http://vocab.getty.edu/aat/300011129"/>
	<dcterms:created rdf:datatype="http://www.w3.org/2001/XMLSchema#date">2007-02-08</dcterms:created>
	<dcterms:modified rdf:datatype="http://www.w3.org/2001/XMLSchema#date">2024-11-15</dcterms:modified>
	<dcterms:identifier>15983</dcterms:identifier>
	<dcterms:contributor>blandine.nouvel</dcterms:contributor>
	<dcterms:contributor>justine.vincent</dcterms:contributor>
	<skos:definition xml:lang="fr">Substance minérale appartenant à la famille de la silice et comprenant toutes les variétés hydratées ou gélatineuses de silice. (Larousse)</skos:definition>
	<skos:definition xml:lang="en">Mineral substance belonging to the silica family and including all hydrated or gelatinous varieties of silica. (Larousse)</skos:definition>
</rdf:Description>

<rdf:Description rdf:about="https://ark.frantiq.fr/ark:/26678/pcrt0zhHI6jOVx">
	<rdf:type rdf:resource="http://www.w3.org/2004/02/skos/core#Concept"/>
	<skos:prefLabel xml:lang="es">opio</skos:prefLabel>
	<skos:prefLabel xml:lang="en">opium</skos:prefLabel>
	<skos:prefLabel xml:lang="fr">opium</skos:prefLabel>
	<skos:prefLabel xml:lang="nl">opium</skos:prefLabel>
	<skos:prefLabel xml:lang="de">Opium</skos:prefLabel>
	<skos:prefLabel xml:lang="it">oppio</skos:prefLabel>
	<skos:prefLabel xml:lang="ar">أفيون</skos:prefLabel>
	<skos:related rdf:resource="https://ark.frantiq.fr/ark:/26678/pcrtemaXFvS9Ms"/>
	<skos:broader rdf:resource="https://ark.frantiq.fr/ark:/26678/pcrtuxpF5YgM3S"/>
	<skos:inScheme rdf:resource="https://ark.frantiq.fr/ark:/26678/TH_1"/>
	<opentheso:memberOf rdf:resource="https://ark.frantiq.fr/ark:/26678/pcrtv66rn9cbv1"/>
	<opentheso:memberOf rdf:resource="https://ark.frantiq.fr/ark:/26678/pcrtnbDLi2FkAj"/>
	<skos:exactMatch rdf:resource="https://catalogue.bnf.fr/ark:/12148/cb11975518z"/>
	<skos:exactMatch rdf:resource="https://www.wikidata.org/wiki/Q46452"/>
	<dcterms:created rdf:datatype="http://www.w3.org/2001/XMLSchema#date">2007-02-08</dcterms:created>
	<dcterms:modified rdf:datatype="http://www.w3.org/2001/XMLSchema#date">2024-03-20</dcterms:modified>
	<dcterms:identifier>15986</dcterms:identifier>
	<dcterms:contributor>blandine.nouvel</dcterms:contributor>
	<dcterms:contributor>justine.vincent</dcterms:contributor>
	<skos:definition xml:lang="en">Psychotropic preparation obtained from the latex of the sleeping poppy (Wikipedia)</skos:definition>
	<skos:definition xml:lang="fr">Préparation psychotrope obtenue à partir du latex du pavot somnifère. (Wikipédia)</skos:definition>
</rdf:Description>

<rdf:Description rdf:about="https://ark.frantiq.fr/ark:/26678/pcrtuihSl3eSnW">
	<rdf:type rdf:resource="http://www.w3.org/2004/02/skos/core#Concept"/>
	<skos:prefLabel xml:lang="en">gold</skos:prefLabel>
	<skos:prefLabel xml:lang="de">Gold</skos:prefLabel>
	<skos:prefLabel xml:lang="nl">goud</skos:prefLabel>
	<skos:prefLabel xml:lang="fr">or</skos:prefLabel>
	<skos:prefLabel xml:lang="es">oro</skos:prefLabel>
	<skos:prefLabel xml:lang="it">oro</skos:prefLabel>
	<skos:prefLabel xml:lang="ar">ذهب</skos:prefLabel>
	<skos:altLabel xml:lang="fr">or (métal)</skos:altLabel>
	<skos:related rdf:resource="https://ark.frantiq.fr/ark:/26678/pcrtz9UOduTM9y"/>
	<skos:related rdf:resource="https://ark.frantiq.fr/ark:/26678/pcrt163rh83f9c"/>
	<skos:related rdf:resource="https://ark.frantiq.fr/ark:/26678/pcrt31pfgqwwcbfvjz0p6dtd"/>
	<skos:related rdf:resource="https://ark.frantiq.fr/ark:/26678/pcrt1wb21fj2vj6r1gjk7221"/>
	<skos:broader rdf:resource="https://ark.frantiq.fr/ark:/26678/pcrtkn1hAXHveS"/>
	<skos:inScheme rdf:resource="https://ark.frantiq.fr/ark:/26678/TH_1"/>
	<opentheso:memberOf rdf:resource="https://ark.frantiq.fr/ark:/26678/pcrtv66rn9cbv1"/>
	<opentheso:memberOf rdf:resource="https://ark.frantiq.fr/ark:/26678/pcrtnbDLi2FkAj"/>
	<opentheso:memberOf rdf:resource="https://ark.frantiq.fr/ark:/26678/pcrtv0jq332vcq3gxt5m13d5"/>
	<skos:exactMatch rdf:resource="https://catalogue.bnf.fr/ark:/12148/cb133184606"/>
	<skos:exactMatch rdf:resource="https://www.wikidata.org/wiki/Q897"/>
	<skos:exactMatch rdf:resource="http://vocab.getty.edu/aat/300011021"/>
	<dcterms:created rdf:datatype="http://www.w3.org/2001/XMLSchema#date">2007-02-08</dcterms:created>
	<dcterms:modified rdf:datatype="http://www.w3.org/2001/XMLSchema#date">2024-03-21</dcterms:modified>
	<dcterms:identifier>15995</dcterms:identifier>
	<dcterms:contributor>blandine.nouvel</dcterms:contributor>
	<dcterms:contributor>irene.weis</dcterms:contributor>
	<skos:definition xml:lang="en">Precious metal, bright yellow, soft, very dense, very malleable and very ductile, unalterable to air, water and acids, generally occurring in its native state in the form of nuggets or flakes (symb. Au, atomic no. 79) (TLFi)</skos:definition>
	<skos:definition xml:lang="fr">Métal précieux, jaune brillant, mou, très dense, très malléable et très ductile, inaltérable à l'air, à l'eau et aux acides, qui se présente généralement à l'état natif sous forme de pépites ou de paillettes (symb. Au, no atomique 79) (TLFi)</skos:definition>
</rdf:Description>

<rdf:Description rdf:about="https://ark.frantiq.fr/ark:/26678/pcrt448yYmVDuT">
	<rdf:type rdf:resource="http://www.w3.org/2004/02/skos/core#Concept"/>
	<skos:prefLabel xml:lang="nl">been</skos:prefLabel>
	<skos:prefLabel xml:lang="en">bone</skos:prefLabel>
	<skos:prefLabel xml:lang="es">hueso</skos:prefLabel>
	<skos:prefLabel xml:lang="de">Knochen</skos:prefLabel>
	<skos:prefLabel xml:lang="fr">matière osseuse</skos:prefLabel>
	<skos:prefLabel xml:lang="it">osso</skos:prefLabel>
	<skos:prefLabel xml:lang="ar">عظم</skos:prefLabel>
	<skos:altLabel xml:lang="en">bone tissue</skos:altLabel>
	<skos:altLabel xml:lang="es">materia ósea</skos:altLabel>
	<skos:altLabel xml:lang="fr">os (matière)</skos:altLabel>
	<skos:related rdf:resource="https://ark.frantiq.fr/ark:/26678/pcrtpy5s63Sdhx"/>
	<skos:related rdf:resource="https://ark.frantiq.fr/ark:/26678/pcrtaI2EMYnfOm"/>
	<skos:related rdf:resource="https://ark.frantiq.fr/ark:/26678/pcrtlflojXmhAi"/>
	<skos:related rdf:resource="https://ark.frantiq.fr/ark:/26678/pcrtEfcf8rSZvm"/>
	<skos:narrower rdf:resource="https://ark.frantiq.fr/ark:/26678/pcrtGg8L8TLNtc"/>
	<skos:broader rdf:resource="https://ark.frantiq.fr/ark:/26678/pcrtf97bQHDGEd"/>
	<skos:inScheme rdf:resource="https://ark.frantiq.fr/ark:/26678/TH_1"/>
	<opentheso:memberOf rdf:resource="https://ark.frantiq.fr/ark:/26678/pcrtv66rn9cbv1"/>
	<opentheso:memberOf rdf:resource="https://ark.frantiq.fr/ark:/26678/pcrtnbDLi2FkAj"/>
	<skos:exactMatch rdf:resource="https://catalogue.bnf.fr/ark:/12148/cb11935812w"/>
	<skos:exactMatch rdf:resource="https://fr.wikipedia.org/wiki/OS"/>
	<skos:exactMatch rdf:resource="https://www.wikidata.org/wiki/Q265868"/>
	<dcterms:created rdf:datatype="http://www.w3.org/2001/XMLSchema#date">2007-02-08</dcterms:created>
	<dcterms:modified rdf:datatype="http://www.w3.org/2001/XMLSchema#date">2023-08-02</dcterms:modified>
	<dcterms:identifier>16029</dcterms:identifier>
	<dcterms:contributor>blandine.nouvel</dcterms:contributor>
	<skos:definition xml:lang="en">An element of hard consistency and whitish colour used to support the soft parts of the body of humans and vertebrates (except certain fish) (cnrtl)</skos:definition>
	<skos:definition xml:lang="fr">Élément de consistance dure et de couleur blanchâtre servant de soutien aux parties molles du corps de l'homme et des vertébrés (à l'exception de certains poissons) (cnrtl)</skos:definition>
</rdf:Description>

<rdf:Description rdf:about="https://ark.frantiq.fr/ark:/26678/pcrtDr6Oi6lHM6">
	<rdf:type rdf:resource="http://www.w3.org/2004/02/skos/core#Concept"/>
	<skos:prefLabel xml:lang="en">bread</skos:prefLabel>
	<skos:prefLabel xml:lang="nl">brood</skos:prefLabel>
	<skos:prefLabel xml:lang="de">Brot</skos:prefLabel>
	<skos:prefLabel xml:lang="fr">pain</skos:prefLabel>
	<skos:prefLabel xml:lang="es">pan</skos:prefLabel>
	<skos:prefLabel xml:lang="it">pane</skos:prefLabel>
	<skos:prefLabel xml:lang="ar">خبز</skos:prefLabel>
	<skos:related rdf:resource="https://ark.frantiq.fr/ark:/26678/pcrt7r77ub1prl"/>
	<skos:broader rdf:resource="https://ark.frantiq.fr/ark:/26678/pcrtgcn5U8laUN"/>
	<skos:inScheme rdf:resource="https://ark.frantiq.fr/ark:/26678/TH_1"/>
	<opentheso:memberOf rdf:resource="https://ark.frantiq.fr/ark:/26678/pcrtv66rn9cbv1"/>
	<opentheso:memberOf rdf:resource="https://ark.frantiq.fr/ark:/26678/pcrtnbDLi2FkAj"/>
	<skos:exactMatch rdf:resource="https://catalogue.bnf.fr/ark:/12148/cb11933895x"/>
	<skos:exactMatch rdf:resource="https://www.wikidata.org/wiki/Q7802"/>
	<skos:exactMatch rdf:resource="http://vocab.getty.edu/aat/300262820"/>
	<dcterms:created rdf:datatype="http://www.w3.org/2001/XMLSchema#date">2007-02-08</dcterms:created>
	<dcterms:modified rdf:datatype="http://www.w3.org/2001/XMLSchema#date">2023-08-02</dcterms:modified>
	<dcterms:identifier>16065</dcterms:identifier>
	<dcterms:contributor>blandine.nouvel</dcterms:contributor>
	<skos:definition xml:lang="en">Food made from flour, salt and water.</skos:definition>
	<skos:definition xml:lang="fr">Aliment fabriqué à partir de farine, de sel et d'eau.</skos:definition>
</rdf:Description>

<rdf:Description rdf:about="https://ark.frantiq.fr/ark:/26678/pcrtMt1immB5H5">
	<rdf:type rdf:resource="http://www.w3.org/2004/02/skos/core#Concept"/>
	<skos:prefLabel xml:lang="fr">parchemin</skos:prefLabel>
	<skos:prefLabel xml:lang="en">parchment</skos:prefLabel>
	<skos:prefLabel xml:lang="it">pergamena</skos:prefLabel>
	<skos:prefLabel xml:lang="de">Pergament</skos:prefLabel>
	<skos:prefLabel xml:lang="es">pergamino</skos:prefLabel>
	<skos:prefLabel xml:lang="nl">perkament</skos:prefLabel>
	<skos:prefLabel xml:lang="ar">لفيفة</skos:prefLabel>
	<skos:altLabel xml:lang="it">cartapecora</skos:altLabel>
	<skos:related rdf:resource="https://ark.frantiq.fr/ark:/26678/pcrtVOeI7bAJTI"/>
	<skos:narrower rdf:resource="https://ark.frantiq.fr/ark:/26678/pcrt2xkdh2n373"/>
	<skos:broader rdf:resource="https://ark.frantiq.fr/ark:/26678/pcrtW8Uu5SMsQy"/>
	<skos:inScheme rdf:resource="https://ark.frantiq.fr/ark:/26678/TH_1"/>
	<opentheso:memberOf rdf:resource="https://ark.frantiq.fr/ark:/26678/pcrtv66rn9cbv1"/>
	<opentheso:memberOf rdf:resource="https://ark.frantiq.fr/ark:/26678/pcrtnbDLi2FkAj"/>
	<skos:exactMatch rdf:resource="https://catalogue.bnf.fr/ark:/12148/cb122648397"/>
	<skos:exactMatch rdf:resource="https://www.wikidata.org/wiki/Q226697"/>
	<skos:exactMatch rdf:resource="http://vocab.getty.edu/aat/300011851"/>
	<dcterms:created rdf:datatype="http://www.w3.org/2001/XMLSchema#date">2007-02-08</dcterms:created>
	<dcterms:modified rdf:datatype="http://www.w3.org/2001/XMLSchema#date">2024-08-23</dcterms:modified>
	<dcterms:identifier>16118</dcterms:identifier>
	<dcterms:contributor>blandine.nouvel</dcterms:contributor>
	<skos:definition xml:lang="en">Animal hide (usually sheep, goat, lamb or calf), scraped, thinned, made rot-proof and softened with pumice stone (cnrtl).</skos:definition>
	<skos:definition xml:lang="fr">Peau d'animal (mouton, chèvre, agneau ou veau généralement), grattée, amincie, rendue imputrescible et doucie à la pierre ponce (cnrtl).</skos:definition>
	<skos:historyNote xml:lang="fr">2024-08-23 : traduction de la définition ; correction du label et arabe.</skos:historyNote>
</rdf:Description>

<rdf:Description rdf:about="https://ark.frantiq.fr/ark:/26678/pcrtOM6tMh4qpF">
	<rdf:type rdf:resource="http://www.w3.org/2004/02/skos/core#Concept"/>
	<skos:prefLabel xml:lang="fr">parfum</skos:prefLabel>
	<skos:prefLabel xml:lang="nl">parfum</skos:prefLabel>
	<skos:prefLabel xml:lang="de">Parfüm</skos:prefLabel>
	<skos:prefLabel xml:lang="en">perfume</skos:prefLabel>
	<skos:prefLabel xml:lang="es">perfume</skos:prefLabel>
	<skos:prefLabel xml:lang="it">profumo</skos:prefLabel>
	<skos:prefLabel xml:lang="ar">عِطر</skos:prefLabel>
	<skos:altLabel xml:lang="fr">arôme</skos:altLabel>
	<skos:altLabel xml:lang="fr">odeur</skos:altLabel>
	<skos:related rdf:resource="https://ark.frantiq.fr/ark:/26678/pcrtGYJ5nOKTlR"/>
	<skos:related rdf:resource="https://ark.frantiq.fr/ark:/26678/pcrtHtkH5XaO98"/>
	<skos:related rdf:resource="https://ark.frantiq.fr/ark:/26678/pcrtZxVQ2PLkIO"/>
	<skos:broader rdf:resource="https://ark.frantiq.fr/ark:/26678/pcrtLpvrsa9RIz"/>
	<skos:inScheme rdf:resource="https://ark.frantiq.fr/ark:/26678/TH_1"/>
	<opentheso:memberOf rdf:resource="https://ark.frantiq.fr/ark:/26678/pcrtv66rn9cbv1"/>
	<opentheso:memberOf rdf:resource="https://ark.frantiq.fr/ark:/26678/pcrtnbDLi2FkAj"/>
	<skos:exactMatch rdf:resource="https://catalogue.bnf.fr/ark:/12148/cb11937402z"/>
	<skos:exactMatch rdf:resource="https://www.wikidata.org/wiki/Q131746"/>
	<skos:exactMatch rdf:resource="http://vocab.getty.edu/aat/300015166"/>
	<dcterms:created rdf:datatype="http://www.w3.org/2001/XMLSchema#date">2007-02-08</dcterms:created>
	<dcterms:modified rdf:datatype="http://www.w3.org/2001/XMLSchema#date">2024-03-20</dcterms:modified>
	<dcterms:identifier>16121</dcterms:identifier>
	<dcterms:contributor>blandine.nouvel</dcterms:contributor>
	<dcterms:contributor>justine.vincent</dcterms:contributor>
	<skos:definition xml:lang="en">Aromatic substance, pleasant to the sense of smell, liquid or solid, of natural or artificial origin(cnrtl)</skos:definition>
	<skos:definition xml:lang="fr">Substance aromatique agréable à l'odorat, liquide ou solide, d'origine naturelle ou artificielle.(cnrtl)</skos:definition>
</rdf:Description>

<rdf:Description rdf:about="https://ark.frantiq.fr/ark:/26678/pcrtnlpDSw0du4">
	<rdf:type rdf:resource="http://www.w3.org/2004/02/skos/core#Concept"/>
	<skos:prefLabel xml:lang="en">cooking stone</skos:prefLabel>
	<skos:prefLabel xml:lang="es">piedra ollar</skos:prefLabel>
	<skos:prefLabel xml:lang="fr">pierre ollaire</skos:prefLabel>
	<skos:prefLabel xml:lang="it">pietra ollare</skos:prefLabel>
	<skos:prefLabel xml:lang="nl">serpentijnsteen</skos:prefLabel>
	<skos:prefLabel xml:lang="de">Speckstein</skos:prefLabel>
	<skos:prefLabel xml:lang="ar">بَصرَة</skos:prefLabel>
	<skos:altLabel xml:lang="en">hearth stone</skos:altLabel>
	<skos:altLabel xml:lang="en">pot boiler</skos:altLabel>
	<skos:broader rdf:resource="https://ark.frantiq.fr/ark:/26678/pcrtnpv5KJIXTy"/>
	<skos:inScheme rdf:resource="https://ark.frantiq.fr/ark:/26678/TH_1"/>
	<opentheso:memberOf rdf:resource="https://ark.frantiq.fr/ark:/26678/pcrtv66rn9cbv1"/>
	<opentheso:memberOf rdf:resource="https://ark.frantiq.fr/ark:/26678/pcrtnbDLi2FkAj"/>
	<skos:exactMatch rdf:resource="https://catalogue.bnf.fr/ark:/12148/cb11965047z"/>
	<skos:exactMatch rdf:resource="https://www.wikidata.org/wiki/Q707896"/>
	<skos:exactMatch rdf:resource="http://vocab.getty.edu/aat/300011665"/>
	<dcterms:created rdf:datatype="http://www.w3.org/2001/XMLSchema#date">2007-02-08</dcterms:created>
	<dcterms:modified rdf:datatype="http://www.w3.org/2001/XMLSchema#date">2024-11-18</dcterms:modified>
	<dcterms:identifier>16235</dcterms:identifier>
	<dcterms:contributor>blandine.nouvel</dcterms:contributor>
	<dcterms:contributor>justine.vincent</dcterms:contributor>
	<skos:definition xml:lang="fr">stéatite contenant de la chlorite, du talc et de la magnésite, caractérisée par sa malléabilité et sa résistance au feu.</skos:definition>
	<skos:definition xml:lang="en">soapstone containing chlorite, talc and magnesite, characterised by its malleability and fire resistance.</skos:definition>
</rdf:Description>

<rdf:Description rdf:about="https://ark.frantiq.fr/ark:/26678/pcrtzVuPZeWdAP">
	<rdf:type rdf:resource="http://www.w3.org/2004/02/skos/core#Concept"/>
	<skos:prefLabel xml:lang="nl">edelgesteente</skos:prefLabel>
	<skos:prefLabel xml:lang="de">Edelstein</skos:prefLabel>
	<skos:prefLabel xml:lang="es">piedra preciosa</skos:prefLabel>
	<skos:prefLabel xml:lang="fr">pierre précieuse</skos:prefLabel>
	<skos:prefLabel xml:lang="it">pietra preziosa</skos:prefLabel>
	<skos:prefLabel xml:lang="en">precious stone</skos:prefLabel>
	<skos:prefLabel xml:lang="ar">حجارة كريمة</skos:prefLabel>
	<skos:narrower rdf:resource="https://ark.frantiq.fr/ark:/26678/pcrtcTqKm5ufUF"/>
	<skos:narrower rdf:resource="https://ark.frantiq.fr/ark:/26678/pcrtevBDzau7qe"/>
	<skos:narrower rdf:resource="https://ark.frantiq.fr/ark:/26678/pcrt1pRQD1Ircr"/>
	<skos:narrower rdf:resource="https://ark.frantiq.fr/ark:/26678/pcrtmbhTSRIoYb"/>
	<skos:broader rdf:resource="https://ark.frantiq.fr/ark:/26678/pcrt8yYh5xgMeO"/>
	<skos:inScheme rdf:resource="https://ark.frantiq.fr/ark:/26678/TH_1"/>
	<opentheso:memberOf rdf:resource="https://ark.frantiq.fr/ark:/26678/pcrtv66rn9cbv1"/>
	<opentheso:memberOf rdf:resource="https://ark.frantiq.fr/ark:/26678/pcrtnbDLi2FkAj"/>
	<skos:exactMatch rdf:resource="https://www.wikidata.org/wiki/Q4990682"/>
	<skos:exactMatch rdf:resource="http://vocab.getty.edu/aat/300133732"/>
	<dcterms:created rdf:datatype="http://www.w3.org/2001/XMLSchema#date">2007-02-08</dcterms:created>
	<dcterms:modified rdf:datatype="http://www.w3.org/2001/XMLSchema#date">2024-11-15</dcterms:modified>
	<dcterms:identifier>16236</dcterms:identifier>
	<dcterms:contributor>blandine.nouvel</dcterms:contributor>
	<dcterms:contributor>justine.vincent</dcterms:contributor>
	<skos:definition xml:lang="en">Historical denomination (officially repealed by French legislation since January 2002) which applies in France to the four gems of diamond, sapphire, ruby and emerald. (ap. Wikipedia)</skos:definition>
	<skos:definition xml:lang="fr">Dénomination historique (&lt;span style= background-color: rgb(255, 255, 255); &gt;officiellement abrogée par la législation française depuis janvier 2002) &lt;/span&gt;qui s'applique en France aux quatre gemmes que sont le diamant, le saphir, le rubis et l'émeraude. (d'ap. Wikipedia)</skos:definition>
</rdf:Description>

<rdf:Description rdf:about="https://ark.frantiq.fr/ark:/26678/pcrtGzQPnntJa1">
	<rdf:type rdf:resource="http://www.w3.org/2004/02/skos/core#Concept"/>
	<skos:prefLabel xml:lang="de">Farbpigment</skos:prefLabel>
	<skos:prefLabel xml:lang="en">pigment</skos:prefLabel>
	<skos:prefLabel xml:lang="fr">pigment</skos:prefLabel>
	<skos:prefLabel xml:lang="nl">pigment</skos:prefLabel>
	<skos:prefLabel xml:lang="es">pigmento</skos:prefLabel>
	<skos:prefLabel xml:lang="it">pigmento</skos:prefLabel>
	<skos:prefLabel xml:lang="ar">صِباغ</skos:prefLabel>
	<skos:altLabel xml:lang="fr">colorant</skos:altLabel>
	<skos:altLabel xml:lang="en">colored material</skos:altLabel>
	<skos:altLabel xml:lang="de">Farbstoff</skos:altLabel>
	<skos:related rdf:resource="https://ark.frantiq.fr/ark:/26678/pcrtu5RUM9S618"/>
	<skos:related rdf:resource="https://ark.frantiq.fr/ark:/26678/pcrttnySGIGsj6"/>
	<skos:related rdf:resource="https://ark.frantiq.fr/ark:/26678/pcrtPpPoKulDjv"/>
	<skos:related rdf:resource="https://ark.frantiq.fr/ark:/26678/pcrtK3vwsfbg8b"/>
	<skos:related rdf:resource="https://ark.frantiq.fr/ark:/26678/pcrt0TJJTrHkN1"/>
	<skos:narrower rdf:resource="https://ark.frantiq.fr/ark:/26678/pcrtM0mkbZiNnN"/>
	<skos:narrower rdf:resource="https://ark.frantiq.fr/ark:/26678/pcrtbbqj7zgqnn"/>
	<skos:narrower rdf:resource="https://ark.frantiq.fr/ark:/26678/pcrtf80pqj28pw"/>
	<skos:narrower rdf:resource="https://ark.frantiq.fr/ark:/26678/pcrt7kSfnJElvj"/>
	<skos:narrower rdf:resource="https://ark.frantiq.fr/ark:/26678/pcrterNa8OcooH"/>
	<skos:narrower rdf:resource="https://ark.frantiq.fr/ark:/26678/pcrttAmNtvNqnf"/>
	<skos:narrower rdf:resource="https://ark.frantiq.fr/ark:/26678/pcrtK2sVvLapYR"/>
	<skos:broader rdf:resource="https://ark.frantiq.fr/ark:/26678/pcrtIMsuG0RWTs"/>
	<skos:inScheme rdf:resource="https://ark.frantiq.fr/ark:/26678/TH_1"/>
	<opentheso:memberOf rdf:resource="https://ark.frantiq.fr/ark:/26678/pcrtv66rn9cbv1"/>
	<opentheso:memberOf rdf:resource="https://ark.frantiq.fr/ark:/26678/pcrtnbDLi2FkAj"/>
	<skos:exactMatch rdf:resource="https://catalogue.bnf.fr/ark:/12148/cb11976099n"/>
	<skos:exactMatch rdf:resource="https://www.wikidata.org/wiki/Q161179"/>
	<skos:exactMatch rdf:resource="http://vocab.getty.edu/aat/300013109"/>
	<dcterms:created rdf:datatype="http://www.w3.org/2001/XMLSchema#date">2007-02-08</dcterms:created>
	<dcterms:modified rdf:datatype="http://www.w3.org/2001/XMLSchema#date">2023-08-02</dcterms:modified>
	<dcterms:identifier>16239</dcterms:identifier>
	<dcterms:contributor>blandine.nouvel</dcterms:contributor>
	<skos:definition xml:lang="fr">Toute substance colorée quelle qu'en soit l'origine, la structure et la nature. (TLFi)</skos:definition>
	<skos:definition xml:lang="en">Any coloured substance, whatever its origin, structure or nature. (TLFi)</skos:definition>
</rdf:Description>

<rdf:Description rdf:about="https://ark.frantiq.fr/ark:/26678/pcrtlZ7VYeGKO3">
	<rdf:type rdf:resource="http://www.w3.org/2004/02/skos/core#Concept"/>
	<skos:prefLabel xml:lang="it">piastrina</skos:prefLabel>
	<skos:prefLabel xml:lang="nl">plaatje</skos:prefLabel>
	<skos:prefLabel xml:lang="es">plaqueta</skos:prefLabel>
	<skos:prefLabel xml:lang="en">plaquette</skos:prefLabel>
	<skos:prefLabel xml:lang="fr">plaquette (matériau)</skos:prefLabel>
	<skos:prefLabel xml:lang="de">Plättchen</skos:prefLabel>
	<skos:prefLabel xml:lang="ar">صفيحة</skos:prefLabel>
	<skos:altLabel xml:lang="fr">plaquette (géologie)</skos:altLabel>
	<skos:related rdf:resource="https://ark.frantiq.fr/ark:/26678/pcrtdt7TJtiVvO"/>
	<skos:broader rdf:resource="https://ark.frantiq.fr/ark:/26678/pcrtw8nqd0wpmc"/>
	<skos:inScheme rdf:resource="https://ark.frantiq.fr/ark:/26678/TH_1"/>
	<opentheso:memberOf rdf:resource="https://ark.frantiq.fr/ark:/26678/pcrtv66rn9cbv1"/>
	<opentheso:memberOf rdf:resource="https://ark.frantiq.fr/ark:/26678/pcrtnbDLi2FkAj"/>
	<skos:exactMatch rdf:resource="https://www.wikidata.org/wiki/Q7201702"/>
	<skos:exactMatch rdf:resource="http://vocab.getty.edu/aat/300190507"/>
	<dcterms:created rdf:datatype="http://www.w3.org/2001/XMLSchema#date">2007-02-08</dcterms:created>
	<dcterms:modified rdf:datatype="http://www.w3.org/2001/XMLSchema#date">2025-01-17</dcterms:modified>
	<dcterms:identifier>16286</dcterms:identifier>
	<dcterms:contributor>blandine.nouvel</dcterms:contributor>
	<dcterms:contributor>justine.vincent</dcterms:contributor>
	<skos:definition xml:lang="en">Sedimentary layer limited to the roof (upper limit of the layer) and the wall (lower limit of the layer) by two thin stratification joints (centimetric thickness, i.e.&lt;=10 cm) (Fernandes et al.: Vade-mecum pour la caractérisation pétroarchéologique des silicites, 2024).</skos:definition>
	<skos:definition xml:lang="fr">Couche sédimentaire limitée au toit (limite supérieure de la couche) et au mur (limite inférieure de la couche) par deux joints de stratification de faible épaisseur (épaisseur centimétrique, soit&lt;=10 cm). (Fernandes et al. : Vade-mecum pour la caractérisation pétroarchéologique des silicites, 2024)</skos:definition>
	<skos:historyNote xml:lang="fr">2025-01-17: mise à jour de la réf. bibliographique de la définition.</skos:historyNote>
</rdf:Description>

<rdf:Description rdf:about="https://ark.frantiq.fr/ark:/26678/pcrtbLhpWhz8H6">
	<rdf:type rdf:resource="http://www.w3.org/2004/02/skos/core#Concept"/>
	<skos:prefLabel xml:lang="de">Platin</skos:prefLabel>
	<skos:prefLabel xml:lang="fr">platine</skos:prefLabel>
	<skos:prefLabel xml:lang="es">platino</skos:prefLabel>
	<skos:prefLabel xml:lang="it">platino</skos:prefLabel>
	<skos:prefLabel xml:lang="en">platinum</skos:prefLabel>
	<skos:prefLabel xml:lang="nl">platinum</skos:prefLabel>
	<skos:prefLabel xml:lang="ar">بلاتين</skos:prefLabel>
	<skos:broader rdf:resource="https://ark.frantiq.fr/ark:/26678/pcrtkn1hAXHveS"/>
	<skos:inScheme rdf:resource="https://ark.frantiq.fr/ark:/26678/TH_1"/>
	<opentheso:memberOf rdf:resource="https://ark.frantiq.fr/ark:/26678/pcrtv66rn9cbv1"/>
	<opentheso:memberOf rdf:resource="https://ark.frantiq.fr/ark:/26678/pcrtnbDLi2FkAj"/>
	<skos:exactMatch rdf:resource="https://catalogue.bnf.fr/ark:/12148/cb11933151c"/>
	<skos:exactMatch rdf:resource="https://www.wikidata.org/wiki/Q880"/>
	<skos:exactMatch rdf:resource="http://vocab.getty.edu/aat/300011031"/>
	<dcterms:created rdf:datatype="http://www.w3.org/2001/XMLSchema#date">2007-02-08</dcterms:created>
	<dcterms:modified rdf:datatype="http://www.w3.org/2001/XMLSchema#date">2024-12-04</dcterms:modified>
	<dcterms:identifier>16295</dcterms:identifier>
	<dcterms:contributor>blandine.nouvel</dcterms:contributor>
	<dcterms:contributor>justine.vincent</dcterms:contributor>
	<skos:definition xml:lang="en">A corrosion-resistant metal found in certain copper and nickel ores, as well as in native deposits.</skos:definition>
	<skos:definition xml:lang="fr">Métal résistant à la corrosion que l'on trouve dans certains minerais de cuivre ou de nickel, ainsi que sous forme de dépôt natif.</skos:definition>
	<skos:historyNote xml:lang="fr">2024-04-12 : modifications de la définition.</skos:historyNote>
</rdf:Description>

<rdf:Description rdf:about="https://ark.frantiq.fr/ark:/26678/pcrtEpGlZykUTy">
	<rdf:type rdf:resource="http://www.w3.org/2004/02/skos/core#Concept"/>
	<skos:prefLabel xml:lang="de">Blei</skos:prefLabel>
	<skos:prefLabel xml:lang="en">lead</skos:prefLabel>
	<skos:prefLabel xml:lang="nl">lood</skos:prefLabel>
	<skos:prefLabel xml:lang="it">piombo</skos:prefLabel>
	<skos:prefLabel xml:lang="fr">plomb</skos:prefLabel>
	<skos:prefLabel xml:lang="es">plomo</skos:prefLabel>
	<skos:prefLabel xml:lang="ar">رصاص</skos:prefLabel>
	<skos:related rdf:resource="https://ark.frantiq.fr/ark:/26678/pcrt0oF1Z1HbOE"/>
	<skos:related rdf:resource="https://ark.frantiq.fr/ark:/26678/pcrt19wqnlF9PM"/>
	<skos:related rdf:resource="https://ark.frantiq.fr/ark:/26678/crtD6yIQ4tlyI"/>
	<skos:related rdf:resource="https://ark.frantiq.fr/ark:/26678/pcrtschzpypSiF"/>
	<skos:related rdf:resource="https://ark.frantiq.fr/ark:/26678/pcrt2ozTOWS5f0"/>
	<skos:broader rdf:resource="https://ark.frantiq.fr/ark:/26678/pcrtkn1hAXHveS"/>
	<skos:inScheme rdf:resource="https://ark.frantiq.fr/ark:/26678/TH_1"/>
	<opentheso:memberOf rdf:resource="https://ark.frantiq.fr/ark:/26678/pcrtv66rn9cbv1"/>
	<opentheso:memberOf rdf:resource="https://ark.frantiq.fr/ark:/26678/pcrtnbDLi2FkAj"/>
	<opentheso:memberOf rdf:resource="https://ark.frantiq.fr/ark:/26678/pcrtv0jq332vcq3gxt5m13d5"/>
	<skos:exactMatch rdf:resource="https://catalogue.bnf.fr/ark:/12148/cb119567697"/>
	<skos:exactMatch rdf:resource="https://www.wikidata.org/wiki/Q708"/>
	<skos:exactMatch rdf:resource="http://vocab.getty.edu/aat/300011022"/>
	<dcterms:created rdf:datatype="http://www.w3.org/2001/XMLSchema#date">2007-02-08</dcterms:created>
	<dcterms:modified rdf:datatype="http://www.w3.org/2001/XMLSchema#date">2024-12-04</dcterms:modified>
	<dcterms:identifier>16297</dcterms:identifier>
	<dcterms:contributor>blandine.nouvel</dcterms:contributor>
	<dcterms:contributor>irene.weis</dcterms:contributor>
	<dcterms:contributor>justine.vincent</dcterms:contributor>
	<skos:definition xml:lang="en">A bluish-grey metal that is very dense, soft, ductile, easily fused, highly malleable and laminable.</skos:definition>
	<skos:definition xml:lang="fr">Métal d'un gris bleuâtre, très dense, mou, ductile, facilement fusible, très malléable et laminable.</skos:definition>
	<skos:historyNote xml:lang="fr">2024-04-12 : modification de la définition.</skos:historyNote>
</rdf:Description>

<rdf:Description rdf:about="https://ark.frantiq.fr/ark:/26678/pcrtxVPISFTEr6">
	<rdf:type rdf:resource="http://www.w3.org/2004/02/skos/core#Concept"/>
	<skos:prefLabel xml:lang="it">gesso</skos:prefLabel>
	<skos:prefLabel xml:lang="en">plaster</skos:prefLabel>
	<skos:prefLabel xml:lang="fr">plâtre</skos:prefLabel>
	<skos:prefLabel xml:lang="nl">pleister</skos:prefLabel>
	<skos:prefLabel xml:lang="de">Verputz</skos:prefLabel>
	<skos:prefLabel xml:lang="es">yeso</skos:prefLabel>
	<skos:prefLabel xml:lang="ar">جبس</skos:prefLabel>
	<skos:altLabel xml:lang="de">Putz</skos:altLabel>
	<skos:related rdf:resource="https://ark.frantiq.fr/ark:/26678/pcrtFidgusMwk8"/>
	<skos:related rdf:resource="https://ark.frantiq.fr/ark:/26678/pcrtOF9oqZo0Pd"/>
	<skos:related rdf:resource="https://ark.frantiq.fr/ark:/26678/pcrtrswcv54832s4j7f06fjb"/>
	<skos:broader rdf:resource="https://ark.frantiq.fr/ark:/26678/pcrtQuZiT5nYY2"/>
	<skos:inScheme rdf:resource="https://ark.frantiq.fr/ark:/26678/TH_1"/>
	<opentheso:memberOf rdf:resource="https://ark.frantiq.fr/ark:/26678/pcrtv66rn9cbv1"/>
	<opentheso:memberOf rdf:resource="https://ark.frantiq.fr/ark:/26678/pcrtnbDLi2FkAj"/>
	<skos:exactMatch rdf:resource="https://catalogue.bnf.fr/ark:/12148/cb11946260j"/>
	<skos:exactMatch rdf:resource="https://www.idref.fr/027416577"/>
	<skos:exactMatch rdf:resource="https://www.wikidata.org/wiki/Q274988"/>
	<skos:exactMatch rdf:resource="http://vocab.getty.edu/aat/300014922"/>
	<skos:exactMatch rdf:resource="http://vocab.getty.edu/aat/300014927"/>
	<dcterms:created rdf:datatype="http://www.w3.org/2001/XMLSchema#date">2007-02-08</dcterms:created>
	<dcterms:modified rdf:datatype="http://www.w3.org/2001/XMLSchema#date">2024-11-15</dcterms:modified>
	<dcterms:identifier>16301</dcterms:identifier>
	<dcterms:contributor>blandine.nouvel</dcterms:contributor>
	<dcterms:contributor>justine.vincent</dcterms:contributor>
	<skos:definition xml:lang="en">Fire-retardant building material used in paste form consisting of a mixture of powder and water (semi-hydrated calcium sulphate), or prepared in sheet form. (Wikipedia)</skos:definition>
	<skos:definition xml:lang="fr">Matériau de construction ignifuge utilisé sous forme de pâte constituée d'un mélange de poudre et d'eau (&lt;span style= background-color: rgb(255, 255, 255); &gt;sulfate de calcium semi hydraté)&lt;/span&gt;, ou préparé sous forme de plaques. (Wikipédia)</skos:definition>
</rdf:Description>

<rdf:Description rdf:about="https://ark.frantiq.fr/ark:/26678/pcrtkbJMkYrMF6">
	<rdf:type rdf:resource="http://www.w3.org/2004/02/skos/core#Concept"/>
	<skos:prefLabel xml:lang="en">potin</skos:prefLabel>
	<skos:prefLabel xml:lang="fr">potin</skos:prefLabel>
	<skos:prefLabel xml:lang="it">potin</skos:prefLabel>
	<skos:prefLabel xml:lang="nl">potin</skos:prefLabel>
	<skos:prefLabel xml:lang="de">Potin</skos:prefLabel>
	<skos:prefLabel xml:lang="es">potín</skos:prefLabel>
	<skos:prefLabel xml:lang="ar">بوتين</skos:prefLabel>
	<skos:altLabel xml:lang="en">billon</skos:altLabel>
	<skos:altLabel xml:lang="it">bronzo bianco</skos:altLabel>
	<skos:altLabel xml:lang="it">lega stagno-rame-piombo</skos:altLabel>
	<skos:broader rdf:resource="https://ark.frantiq.fr/ark:/26678/pcrtzcGlM17go5"/>
	<skos:inScheme rdf:resource="https://ark.frantiq.fr/ark:/26678/TH_1"/>
	<opentheso:memberOf rdf:resource="https://ark.frantiq.fr/ark:/26678/pcrtv66rn9cbv1"/>
	<opentheso:memberOf rdf:resource="https://ark.frantiq.fr/ark:/26678/pcrtnbDLi2FkAj"/>
	<skos:exactMatch rdf:resource="https://www.wikidata.org/wiki/Q1427612"/>
	<dcterms:created rdf:datatype="http://www.w3.org/2001/XMLSchema#date">2007-02-08</dcterms:created>
	<dcterms:modified rdf:datatype="http://www.w3.org/2001/XMLSchema#date">2024-11-15</dcterms:modified>
	<dcterms:identifier>16363</dcterms:identifier>
	<dcterms:contributor>blandine.nouvel</dcterms:contributor>
	<dcterms:contributor>justine.vincent</dcterms:contributor>
	<skos:definition xml:lang="fr">Alliage de cuivre, étain, plomb, auxquels s'ajoutent quelques autres éléments en infimes quantités, qui a donné son nom aux pièces de monnaie gauloise coulées et non frappées. (d'ap. K. Gruel, Gallia, t. 52, 1995)</skos:definition>
	<skos:definition xml:lang="en">An alloy of copper, tin and lead, to which are added a few other elements in minute quantities, which gave its name to cast and unstamped Gaulish coins. (d'ap. K. Gruel, Gallia, t. 52, 1995)</skos:definition>
	<skos:definition xml:lang="ar">نقد غير مختوم مركب من خليط معدني من نحاس، قصدير و رصاص</skos:definition>
	<dcterms:source>https://www.persee.fr/issue/galia_0016-4119_1995_num_52_1</dcterms:source>
</rdf:Description>

<rdf:Description rdf:about="https://ark.frantiq.fr/ark:/26678/pcrtDffxD420gS">
	<rdf:type rdf:resource="http://www.w3.org/2004/02/skos/core#Concept"/>
	<skos:prefLabel xml:lang="en">agricultural product</skos:prefLabel>
	<skos:prefLabel xml:lang="nl">landbouwopbrengst</skos:prefLabel>
	<skos:prefLabel xml:lang="de">landwirtschaftliches Erzeugnis</skos:prefLabel>
	<skos:prefLabel xml:lang="it">prodotto agricolo</skos:prefLabel>
	<skos:prefLabel xml:lang="es">producto agrícola</skos:prefLabel>
	<skos:prefLabel xml:lang="fr">produit agricole</skos:prefLabel>
	<skos:prefLabel xml:lang="ar">منتج زراعي</skos:prefLabel>
	<skos:altLabel xml:lang="en">agricultural good</skos:altLabel>
	<skos:altLabel xml:lang="en">crop</skos:altLabel>
	<skos:altLabel xml:lang="en">farm product</skos:altLabel>
	<skos:altLabel xml:lang="es">producción agrícola</skos:altLabel>
	<skos:altLabel xml:lang="fr">production agricole</skos:altLabel>
	<skos:altLabel xml:lang="it">produzione agricola</skos:altLabel>
	<skos:related rdf:resource="https://ark.frantiq.fr/ark:/26678/pcrtRHA0IiiUOF"/>
	<skos:related rdf:resource="https://ark.frantiq.fr/ark:/26678/pcrtATL3ZnpSP5"/>
	<skos:broader rdf:resource="https://ark.frantiq.fr/ark:/26678/pcrtwvFLgSQRs5"/>
	<skos:inScheme rdf:resource="https://ark.frantiq.fr/ark:/26678/TH_1"/>
	<opentheso:memberOf rdf:resource="https://ark.frantiq.fr/ark:/26678/pcrtv66rn9cbv1"/>
	<opentheso:memberOf rdf:resource="https://ark.frantiq.fr/ark:/26678/pcrtnbDLi2FkAj"/>
	<skos:exactMatch rdf:resource="https://www.wikidata.org/wiki/Q11827455"/>
	<dcterms:created rdf:datatype="http://www.w3.org/2001/XMLSchema#date">2007-02-08</dcterms:created>
	<dcterms:modified rdf:datatype="http://www.w3.org/2001/XMLSchema#date">2024-11-15</dcterms:modified>
	<dcterms:identifier>16416</dcterms:identifier>
	<dcterms:contributor>blandine.nouvel</dcterms:contributor>
	<dcterms:contributor>justine.vincent</dcterms:contributor>
	<skos:definition xml:lang="en">A plant or animal product that can be grown and harvested extensively for profit or subsistence.</skos:definition>
	<skos:definition xml:lang="fr">Produit végétal ou animal qui peut être cultivé et récolté de manière extensive à des fins de profit ou de subsistance.</skos:definition>
	<skos:historyNote xml:lang="fr">2024-11-15 : ajout d'une définition</skos:historyNote>
</rdf:Description>

<rdf:Description rdf:about="https://ark.frantiq.fr/ark:/26678/pcrtZETJwE7RTQ">
	<rdf:type rdf:resource="http://www.w3.org/2004/02/skos/core#Concept"/>
	<skos:prefLabel xml:lang="it">impasto (ceramica)</skos:prefLabel>
	<skos:prefLabel xml:lang="nl">kleipasta</skos:prefLabel>
	<skos:prefLabel xml:lang="es">pasta</skos:prefLabel>
	<skos:prefLabel xml:lang="en">paste</skos:prefLabel>
	<skos:prefLabel xml:lang="fr">pâte (céramique)</skos:prefLabel>
	<skos:prefLabel xml:lang="de">Tonmasse</skos:prefLabel>
	<skos:prefLabel xml:lang="ar">عجينة</skos:prefLabel>
	<skos:altLabel xml:lang="it">impasto argilloso</skos:altLabel>
	<skos:related rdf:resource="https://ark.frantiq.fr/ark:/26678/pcrto44p1SaKFn"/>
	<skos:related rdf:resource="https://ark.frantiq.fr/ark:/26678/pcrtYPpmkDk2rS"/>
	<skos:narrower rdf:resource="https://ark.frantiq.fr/ark:/26678/pcrtbTb5hPcQEn"/>
	<skos:narrower rdf:resource="https://ark.frantiq.fr/ark:/26678/pcrtWANqEEARhN"/>
	<skos:narrower rdf:resource="https://ark.frantiq.fr/ark:/26678/pcrtXgoFDoG7xA"/>
	<skos:narrower rdf:resource="https://ark.frantiq.fr/ark:/26678/pcrt518w0nr5tf"/>
	<skos:broader rdf:resource="https://ark.frantiq.fr/ark:/26678/pcrtIMsuG0RWTs"/>
	<skos:inScheme rdf:resource="https://ark.frantiq.fr/ark:/26678/TH_1"/>
	<opentheso:memberOf rdf:resource="https://ark.frantiq.fr/ark:/26678/pcrtv66rn9cbv1"/>
	<opentheso:memberOf rdf:resource="https://ark.frantiq.fr/ark:/26678/pcrtnbDLi2FkAj"/>
	<skos:exactMatch rdf:resource="https://www.wikidata.org/wiki/Q3411503"/>
	<dcterms:created rdf:datatype="http://www.w3.org/2001/XMLSchema#date">2007-02-08</dcterms:created>
	<dcterms:modified rdf:datatype="http://www.w3.org/2001/XMLSchema#date">2024-11-18</dcterms:modified>
	<dcterms:identifier>16527</dcterms:identifier>
	<dcterms:contributor>blandine.nouvel</dcterms:contributor>
	<dcterms:contributor>justine.vincent</dcterms:contributor>
	<skos:definition xml:lang="en">Pottery material: the paste prepared by kneading with water is intended to be shaped into a plastic state and fixed by firing (Balfet et al 1989, p. 47).</skos:definition>
	<skos:definition xml:lang="fr">Matériau constituant une poterie : la pâte préparée par pétrissage avec de l'eau est destinée à être façonnée à l'état plastique et fixée par la cuisson (Balfet et al 1989, p. 47)</skos:definition>
	<dcterms:source>https://catalogue.frantiq.fr/cgi-bin/koha/opac-detail.pl?biblionumber=241203</dcterms:source>
</rdf:Description>

<rdf:Description rdf:about="https://ark.frantiq.fr/ark:/26678/pcrtDwe0cp16nl">
	<rdf:type rdf:resource="http://www.w3.org/2004/02/skos/core#Concept"/>
	<skos:prefLabel xml:lang="es">cuarzo</skos:prefLabel>
	<skos:prefLabel xml:lang="nl">kwarts</skos:prefLabel>
	<skos:prefLabel xml:lang="en">quartz</skos:prefLabel>
	<skos:prefLabel xml:lang="fr">quartz</skos:prefLabel>
	<skos:prefLabel xml:lang="de">Quarz</skos:prefLabel>
	<skos:prefLabel xml:lang="it">quarzo</skos:prefLabel>
	<skos:prefLabel xml:lang="ar">كوارتز</skos:prefLabel>
	<skos:altLabel xml:lang="ar">مَرو</skos:altLabel>
	<skos:narrower rdf:resource="https://ark.frantiq.fr/ark:/26678/pcrtc2SkvG29we"/>
	<skos:broader rdf:resource="https://ark.frantiq.fr/ark:/26678/pcrty2mcsksa6s"/>
	<skos:inScheme rdf:resource="https://ark.frantiq.fr/ark:/26678/TH_1"/>
	<opentheso:memberOf rdf:resource="https://ark.frantiq.fr/ark:/26678/pcrtv66rn9cbv1"/>
	<opentheso:memberOf rdf:resource="https://ark.frantiq.fr/ark:/26678/pcrtnbDLi2FkAj"/>
	<opentheso:memberOf rdf:resource="https://ark.frantiq.fr/ark:/26678/pcrtv0jq332vcq3gxt5m13d5"/>
	<skos:exactMatch rdf:resource="https://www.wikidata.org/wiki/Q43010"/>
	<skos:exactMatch rdf:resource="http://vocab.getty.edu/aat/300011132"/>
	<dcterms:created rdf:datatype="http://www.w3.org/2001/XMLSchema#date">2007-02-08</dcterms:created>
	<dcterms:modified rdf:datatype="http://www.w3.org/2001/XMLSchema#date">2024-11-18</dcterms:modified>
	<dcterms:identifier>16544</dcterms:identifier>
	<dcterms:contributor>blandine.nouvel</dcterms:contributor>
	<dcterms:contributor>irene.weis</dcterms:contributor>
	<dcterms:contributor>justine.vincent</dcterms:contributor>
	<skos:definition xml:lang="en">Trigonal silica with hexagonal lattice (Raoult and Foucault, 2005).</skos:definition>
	<skos:definition xml:lang="fr">Silice trigonale à réseau hexagonal (Raoult et Foucault, 2005).</skos:definition>
</rdf:Description>

<rdf:Description rdf:about="https://ark.frantiq.fr/ark:/26678/pcrtSVdwKcS3MI">
	<rdf:type rdf:resource="http://www.w3.org/2004/02/skos/core#Concept"/>
	<skos:prefLabel xml:lang="de">Felsgestein</skos:prefLabel>
	<skos:prefLabel xml:lang="nl">gesteente</skos:prefLabel>
	<skos:prefLabel xml:lang="es">roca</skos:prefLabel>
	<skos:prefLabel xml:lang="it">roccia</skos:prefLabel>
	<skos:prefLabel xml:lang="fr">roche</skos:prefLabel>
	<skos:prefLabel xml:lang="en">rock</skos:prefLabel>
	<skos:prefLabel xml:lang="ar">صخر</skos:prefLabel>
	<skos:altLabel xml:lang="es">piedra</skos:altLabel>
	<skos:altLabel xml:lang="fr">pierre</skos:altLabel>
	<skos:altLabel xml:lang="it">pietra</skos:altLabel>
	<skos:altLabel xml:lang="en">stone</skos:altLabel>
	<skos:related rdf:resource="https://ark.frantiq.fr/ark:/26678/pcrtM4y540Y1cl"/>
	<skos:related rdf:resource="https://ark.frantiq.fr/ark:/26678/pcrtiiGa8GYBlS"/>
	<skos:related rdf:resource="https://ark.frantiq.fr/ark:/26678/crtYQmrPQmygE"/>
	<skos:related rdf:resource="https://ark.frantiq.fr/ark:/26678/pcrtvKH7mF2Oas"/>
	<skos:narrower rdf:resource="https://ark.frantiq.fr/ark:/26678/pcrt5bIL1UtwcT"/>
	<skos:narrower rdf:resource="https://ark.frantiq.fr/ark:/26678/pcrtxybfLE1dkn"/>
	<skos:narrower rdf:resource="https://ark.frantiq.fr/ark:/26678/pcrtj3ZcwkArSR"/>
	<skos:narrower rdf:resource="https://ark.frantiq.fr/ark:/26678/pcrtDhZmKFAlZa"/>
	<skos:narrower rdf:resource="https://ark.frantiq.fr/ark:/26678/pcrtr5vk7w9vdz"/>
	<skos:narrower rdf:resource="https://ark.frantiq.fr/ark:/26678/pcrtb4mt1w9s876tsx2cxf61"/>
	<skos:broader rdf:resource="https://ark.frantiq.fr/ark:/26678/pcrtIMsuG0RWTs"/>
	<skos:inScheme rdf:resource="https://ark.frantiq.fr/ark:/26678/TH_1"/>
	<opentheso:memberOf rdf:resource="https://ark.frantiq.fr/ark:/26678/pcrtv66rn9cbv1"/>
	<opentheso:memberOf rdf:resource="https://ark.frantiq.fr/ark:/26678/pcrtnbDLi2FkAj"/>
	<opentheso:memberOf rdf:resource="https://ark.frantiq.fr/ark:/26678/pcrtv0jq332vcq3gxt5m13d5"/>
	<skos:exactMatch rdf:resource="https://catalogue.bnf.fr/ark:/12148/cb119327106"/>
	<skos:exactMatch rdf:resource="https://www.wikidata.org/wiki/Q8063"/>
	<skos:exactMatch rdf:resource="http://vocab.getty.edu/aat/300011692"/>
	<dcterms:created rdf:datatype="http://www.w3.org/2001/XMLSchema#date">2007-02-08</dcterms:created>
	<dcterms:modified rdf:datatype="http://www.w3.org/2001/XMLSchema#date">2024-04-11</dcterms:modified>
	<dcterms:identifier>16689</dcterms:identifier>
	<dcterms:contributor>blandine.nouvel</dcterms:contributor>
	<dcterms:contributor>irene.weis</dcterms:contributor>
	<skos:definition xml:lang="en">Material making up the earth's crust, generally formed from an assemblage of minerals and presenting a certain statistical homogeneity (Dict. de géologie, Foucault et Raoult).</skos:definition>
	<skos:definition xml:lang="fr">Matériaux constitutif de l'écorce terrestre, formé en général d'un assemblage de minéraux et présentant une certaine homogénéité statistique. (Dict. de géologie, Foucault et Raoult)</skos:definition>
</rdf:Description>

<rdf:Description rdf:about="https://ark.frantiq.fr/ark:/26678/pcrtxybfLE1dkn">
	<rdf:type rdf:resource="http://www.w3.org/2004/02/skos/core#Concept"/>
	<skos:prefLabel xml:lang="nl">metamorf gesteente</skos:prefLabel>
	<skos:prefLabel xml:lang="de">Metamorphes Gestein</skos:prefLabel>
	<skos:prefLabel xml:lang="en">metamorphic rock</skos:prefLabel>
	<skos:prefLabel xml:lang="es">roca metamórfica</skos:prefLabel>
	<skos:prefLabel xml:lang="it">roccia metamorfica</skos:prefLabel>
	<skos:prefLabel xml:lang="fr">roche métamorphique</skos:prefLabel>
	<skos:prefLabel xml:lang="ar">صخر متحول</skos:prefLabel>
	<skos:narrower rdf:resource="https://ark.frantiq.fr/ark:/26678/pcrtSkipOsBGML"/>
	<skos:narrower rdf:resource="https://ark.frantiq.fr/ark:/26678/pcrtImRXTwOx0B"/>
	<skos:narrower rdf:resource="https://ark.frantiq.fr/ark:/26678/pcrtT7b3IVuYxG"/>
	<skos:narrower rdf:resource="https://ark.frantiq.fr/ark:/26678/pcrtnpv5KJIXTy"/>
	<skos:narrower rdf:resource="https://ark.frantiq.fr/ark:/26678/pcrtAHm0qJl9tq"/>
	<skos:narrower rdf:resource="https://ark.frantiq.fr/ark:/26678/pcrtQqTsG6TEFy"/>
	<skos:narrower rdf:resource="https://ark.frantiq.fr/ark:/26678/pcrtSpItdjR86k"/>
	<skos:broader rdf:resource="https://ark.frantiq.fr/ark:/26678/pcrtSVdwKcS3MI"/>
	<skos:inScheme rdf:resource="https://ark.frantiq.fr/ark:/26678/TH_1"/>
	<opentheso:memberOf rdf:resource="https://ark.frantiq.fr/ark:/26678/pcrtv66rn9cbv1"/>
	<opentheso:memberOf rdf:resource="https://ark.frantiq.fr/ark:/26678/pcrtnbDLi2FkAj"/>
	<skos:exactMatch rdf:resource="https://catalogue.bnf.fr/ark:/12148/cb119417136"/>
	<skos:exactMatch rdf:resource="https://www.wikidata.org/wiki/Q47069"/>
	<skos:exactMatch rdf:resource="http://vocab.getty.edu/aat/300011437"/>
	<dcterms:created rdf:datatype="http://www.w3.org/2001/XMLSchema#date">2007-02-08</dcterms:created>
	<dcterms:modified rdf:datatype="http://www.w3.org/2001/XMLSchema#date">2023-08-02</dcterms:modified>
	<dcterms:identifier>16691</dcterms:identifier>
	<dcterms:contributor>blandine.nouvel</dcterms:contributor>
	<skos:definition xml:lang="en">Rock formed without fusion from pre-existing rocks, essentially by recrystallisation due to increases in temperature and pressure. (Dict. de géologie, Foucault and Raoult)</skos:definition>
	<skos:definition xml:lang="fr">Roche formée sans fusion à partir de roches préexistantes, et cela essentiellement par des recristallisations dues à des élévations de la température et de la pression. (Dict. de géologie, Foucault et Raoult)</skos:definition>
</rdf:Description>

<rdf:Description rdf:about="https://ark.frantiq.fr/ark:/26678/pcrt4N9jrETRto">
	<rdf:type rdf:resource="http://www.w3.org/2004/02/skos/core#Concept"/>
	<skos:prefLabel xml:lang="de">Kieselgestein</skos:prefLabel>
	<skos:prefLabel xml:lang="es">roca silícea</skos:prefLabel>
	<skos:prefLabel xml:lang="it">roccia silicea</skos:prefLabel>
	<skos:prefLabel xml:lang="fr">roche siliceuse</skos:prefLabel>
	<skos:prefLabel xml:lang="en">siliceous rock</skos:prefLabel>
	<skos:prefLabel xml:lang="nl">siliciumhoudend gesteente</skos:prefLabel>
	<skos:prefLabel xml:lang="ar">صخر سيليسي</skos:prefLabel>
	<skos:altLabel xml:lang="es">roca ácida</skos:altLabel>
	<skos:altLabel xml:lang="es">sílice</skos:altLabel>
	<skos:altLabel xml:lang="it">silicee</skos:altLabel>
	<skos:altLabel xml:lang="fr">silicite</skos:altLabel>
	<skos:altLabel xml:lang="ar">صخر صواني</skos:altLabel>
	<skos:narrower rdf:resource="https://ark.frantiq.fr/ark:/26678/pcrtOBWTai2Xms"/>
	<skos:narrower rdf:resource="https://ark.frantiq.fr/ark:/26678/pcrtIzSUofuocv"/>
	<skos:narrower rdf:resource="https://ark.frantiq.fr/ark:/26678/pcrtLgpv98vu4P"/>
	<skos:narrower rdf:resource="https://ark.frantiq.fr/ark:/26678/pcrt3PUAhlWubZ"/>
	<skos:narrower rdf:resource="https://ark.frantiq.fr/ark:/26678/pcrtEU8K1oF2Eh"/>
	<skos:narrower rdf:resource="https://ark.frantiq.fr/ark:/26678/pcrtmxoAFl0eWR"/>
	<skos:narrower rdf:resource="https://ark.frantiq.fr/ark:/26678/pcrt0712c8ws62"/>
	<skos:narrower rdf:resource="https://ark.frantiq.fr/ark:/26678/pcrt11zbr3964m"/>
	<skos:narrower rdf:resource="https://ark.frantiq.fr/ark:/26678/pcrtt42zqnhf10"/>
	<skos:narrower rdf:resource="https://ark.frantiq.fr/ark:/26678/pcrtszp2f0j63w"/>
	<skos:narrower rdf:resource="https://ark.frantiq.fr/ark:/26678/pcrtcxvd08cn0d"/>
	<skos:narrower rdf:resource="https://ark.frantiq.fr/ark:/26678/pcrtwWYB6o5QwM"/>
	<skos:broader rdf:resource="https://ark.frantiq.fr/ark:/26678/pcrtj3ZcwkArSR"/>
	<skos:inScheme rdf:resource="https://ark.frantiq.fr/ark:/26678/TH_1"/>
	<opentheso:memberOf rdf:resource="https://ark.frantiq.fr/ark:/26678/pcrtv66rn9cbv1"/>
	<opentheso:memberOf rdf:resource="https://ark.frantiq.fr/ark:/26678/pcrtnbDLi2FkAj"/>
	<skos:exactMatch rdf:resource="https://catalogue.bnf.fr/ark:/12148/cb119327764"/>
	<skos:exactMatch rdf:resource="https://www.wikidata.org/wiki/Q1504227"/>
	<dcterms:created rdf:datatype="http://www.w3.org/2001/XMLSchema#date">2007-02-08</dcterms:created>
	<dcterms:modified rdf:datatype="http://www.w3.org/2001/XMLSchema#date">2025-01-30</dcterms:modified>
	<dcterms:identifier>16692</dcterms:identifier>
	<dcterms:contributor>blandine.nouvel</dcterms:contributor>
	<dcterms:contributor>justine.vincent</dcterms:contributor>
	<skos:definition xml:lang="en">General term for a hypersiliceous rock, to be used only prior to any precise characterisation (Fernandes, 2012).</skos:definition>
	<skos:definition xml:lang="fr">Terme général désignant une roche hypersiliceuse, à employer uniquement en amont de toute caractérisation précise (Fernandes, 2012).</skos:definition>
	<dcterms:source>https://doi-org.inshs.bib.cnrs.fr/10.4000/12zm5</dcterms:source>
</rdf:Description>

<rdf:Description rdf:about="https://ark.frantiq.fr/ark:/26678/pcrtrxL50B7yNx">
	<rdf:type rdf:resource="http://www.w3.org/2004/02/skos/core#Concept"/>
	<skos:prefLabel xml:lang="nl">hars</skos:prefLabel>
	<skos:prefLabel xml:lang="de">Harz</skos:prefLabel>
	<skos:prefLabel xml:lang="en">resin</skos:prefLabel>
	<skos:prefLabel xml:lang="es">resina</skos:prefLabel>
	<skos:prefLabel xml:lang="it">resina</skos:prefLabel>
	<skos:prefLabel xml:lang="fr">résine</skos:prefLabel>
	<skos:prefLabel xml:lang="ar">راتينج</skos:prefLabel>
	<skos:altLabel xml:lang="ar">صمغ نباتي</skos:altLabel>
	<skos:related rdf:resource="https://ark.frantiq.fr/ark:/26678/pcrtx31xbt8q47wkx7f60mkp"/>
	<skos:narrower rdf:resource="https://ark.frantiq.fr/ark:/26678/pcrtSiQAzZxXsv"/>
	<skos:narrower rdf:resource="https://ark.frantiq.fr/ark:/26678/pcrto2Udjh8XSP"/>
	<skos:narrower rdf:resource="https://ark.frantiq.fr/ark:/26678/pcrtkf9tnv3kc1"/>
	<skos:broader rdf:resource="https://ark.frantiq.fr/ark:/26678/pcrtnHxyjOkhJw"/>
	<skos:inScheme rdf:resource="https://ark.frantiq.fr/ark:/26678/TH_1"/>
	<opentheso:memberOf rdf:resource="https://ark.frantiq.fr/ark:/26678/pcrtv66rn9cbv1"/>
	<opentheso:memberOf rdf:resource="https://ark.frantiq.fr/ark:/26678/pcrtnbDLi2FkAj"/>
	<skos:exactMatch rdf:resource="https://catalogue.bnf.fr/ark:/12148/cb12259733w"/>
	<skos:exactMatch rdf:resource="https://www.wikidata.org/wiki/Q145205"/>
	<skos:exactMatch rdf:resource="http://vocab.getty.edu/aat/300012882"/>
	<dcterms:created rdf:datatype="http://www.w3.org/2001/XMLSchema#date">2007-02-08</dcterms:created>
	<dcterms:modified rdf:datatype="http://www.w3.org/2001/XMLSchema#date">2024-11-15</dcterms:modified>
	<dcterms:identifier>16764</dcterms:identifier>
	<dcterms:contributor>blandine.nouvel</dcterms:contributor>
	<dcterms:contributor>justine.vincent</dcterms:contributor>
	<skos:definition xml:lang="en">Exudates secreted by certain plants, in particular conifers, with the appearance of a sticky liquid which dries more or less rapidly on contact with air. (wp)</skos:definition>
	<skos:definition xml:lang="fr">Exsudats sécrétées par certains végétaux notamment les conifères, ayant l'aspect d'un liquide poisseux qui sèche plus ou moins rapidement au contact de l'air. (wp)</skos:definition>
</rdf:Description>

<rdf:Description rdf:about="https://ark.frantiq.fr/ark:/26678/pcrt82lj1bBlxj">
	<rdf:type rdf:resource="http://www.w3.org/2004/02/skos/core#Concept"/>
	<skos:prefLabel xml:lang="en">brine</skos:prefLabel>
	<skos:prefLabel xml:lang="nl">pekelnat</skos:prefLabel>
	<skos:prefLabel xml:lang="it">salamoia</skos:prefLabel>
	<skos:prefLabel xml:lang="es">salmuera</skos:prefLabel>
	<skos:prefLabel xml:lang="de">Salzlake</skos:prefLabel>
	<skos:prefLabel xml:lang="fr">saumure</skos:prefLabel>
	<skos:prefLabel xml:lang="ar">مُضاض</skos:prefLabel>
	<skos:related rdf:resource="https://ark.frantiq.fr/ark:/26678/pcrtbSfKuoqH7L"/>
	<skos:broader rdf:resource="https://ark.frantiq.fr/ark:/26678/pcrtgcn5U8laUN"/>
	<skos:inScheme rdf:resource="https://ark.frantiq.fr/ark:/26678/TH_1"/>
	<opentheso:memberOf rdf:resource="https://ark.frantiq.fr/ark:/26678/pcrtv66rn9cbv1"/>
	<opentheso:memberOf rdf:resource="https://ark.frantiq.fr/ark:/26678/pcrtnbDLi2FkAj"/>
	<skos:exactMatch rdf:resource="https://www.wikidata.org/wiki/Q214403"/>
	<dcterms:created rdf:datatype="http://www.w3.org/2001/XMLSchema#date">2007-02-08</dcterms:created>
	<dcterms:modified rdf:datatype="http://www.w3.org/2001/XMLSchema#date">2023-08-02</dcterms:modified>
	<dcterms:identifier>16820</dcterms:identifier>
	<dcterms:contributor>blandine.nouvel</dcterms:contributor>
	<skos:definition xml:lang="en">Aqueous solution of flavoured salt used to preserve meat, fish and vegetables (Lar.)</skos:definition>
	<skos:definition xml:lang="fr">Solution aqueuse de sel aromatisé où l'on conserve des viandes, des poissons et des légumes (Lar.)</skos:definition>
	<skos:definition xml:lang="ar">ماء شديد المُلوحة يستعمل في تقديد و حفظ الأغذية</skos:definition>
</rdf:Description>

<rdf:Description rdf:about="https://ark.frantiq.fr/ark:/26678/pcrtImRXTwOx0B">
	<rdf:type rdf:resource="http://www.w3.org/2004/02/skos/core#Concept"/>
	<skos:prefLabel xml:lang="es">esquisto</skos:prefLabel>
	<skos:prefLabel xml:lang="en">schist</skos:prefLabel>
	<skos:prefLabel xml:lang="nl">schist</skos:prefLabel>
	<skos:prefLabel xml:lang="fr">schiste</skos:prefLabel>
	<skos:prefLabel xml:lang="it">scisto</skos:prefLabel>
	<skos:prefLabel xml:lang="de">Tonschiefer</skos:prefLabel>
	<skos:prefLabel xml:lang="ar">شيست</skos:prefLabel>
	<skos:altLabel xml:lang="it">schisto</skos:altLabel>
	<skos:altLabel xml:lang="ar">نَضيد</skos:altLabel>
	<skos:broader rdf:resource="https://ark.frantiq.fr/ark:/26678/pcrtxybfLE1dkn"/>
	<skos:inScheme rdf:resource="https://ark.frantiq.fr/ark:/26678/TH_1"/>
	<opentheso:memberOf rdf:resource="https://ark.frantiq.fr/ark:/26678/pcrtv66rn9cbv1"/>
	<opentheso:memberOf rdf:resource="https://ark.frantiq.fr/ark:/26678/pcrtnbDLi2FkAj"/>
	<opentheso:memberOf rdf:resource="https://ark.frantiq.fr/ark:/26678/pcrtv0jq332vcq3gxt5m13d5"/>
	<skos:exactMatch rdf:resource="https://www.wikidata.org/wiki/Q15315"/>
	<skos:exactMatch rdf:resource="http://vocab.getty.edu/aat/300011626"/>
	<dcterms:created rdf:datatype="http://www.w3.org/2001/XMLSchema#date">2007-02-08</dcterms:created>
	<dcterms:modified rdf:datatype="http://www.w3.org/2001/XMLSchema#date">2024-11-18</dcterms:modified>
	<dcterms:identifier>16837</dcterms:identifier>
	<dcterms:contributor>blandine.nouvel</dcterms:contributor>
	<dcterms:contributor>irene.weis</dcterms:contributor>
	<dcterms:contributor>justine.vincent</dcterms:contributor>
	<skos:definition xml:lang="en">A rock which has the distinctive feature of having a laminated appearance, and is cut into thin slabs or  sheet rock . (wp)</skos:definition>
	<skos:definition xml:lang="fr">Roche qui a pour particularité d'avoir un aspect feuilleté, et de se débiter en plaques fines ou « feuillet rocheux ». (wp)</skos:definition>
</rdf:Description>

<rdf:Description rdf:about="https://ark.frantiq.fr/ark:/26678/pcrthmVBQESXy2">
	<rdf:type rdf:resource="http://www.w3.org/2004/02/skos/core#Concept"/>
	<skos:prefLabel xml:lang="es">sal</skos:prefLabel>
	<skos:prefLabel xml:lang="it">sale</skos:prefLabel>
	<skos:prefLabel xml:lang="en">salt</skos:prefLabel>
	<skos:prefLabel xml:lang="de">Salz</skos:prefLabel>
	<skos:prefLabel xml:lang="fr">sel</skos:prefLabel>
	<skos:prefLabel xml:lang="nl">zout</skos:prefLabel>
	<skos:prefLabel xml:lang="ar">ملح</skos:prefLabel>
	<skos:related rdf:resource="https://ark.frantiq.fr/ark:/26678/pcrtYHA8kKMYt9"/>
	<skos:related rdf:resource="https://ark.frantiq.fr/ark:/26678/pcrtdKpjA3p734"/>
	<skos:related rdf:resource="https://ark.frantiq.fr/ark:/26678/pcrtfx6Kz0jTNH"/>
	<skos:related rdf:resource="https://ark.frantiq.fr/ark:/26678/pcrtA2yuYDT6Az"/>
	<skos:related rdf:resource="https://ark.frantiq.fr/ark:/26678/pcrtVRGDeMZs50"/>
	<skos:related rdf:resource="https://ark.frantiq.fr/ark:/26678/pcrtgkocmOnXvY"/>
	<skos:related rdf:resource="https://ark.frantiq.fr/ark:/26678/crtKQjUDioQvH"/>
	<skos:related rdf:resource="https://ark.frantiq.fr/ark:/26678/crtlG5yNd23r5"/>
	<skos:related rdf:resource="https://ark.frantiq.fr/ark:/26678/crtqpxMq4B4Ah"/>
	<skos:related rdf:resource="https://ark.frantiq.fr/ark:/26678/pcrttnbgqq8w6f"/>
	<skos:broader rdf:resource="https://ark.frantiq.fr/ark:/26678/pcrtUTZqItd8SL"/>
	<skos:inScheme rdf:resource="https://ark.frantiq.fr/ark:/26678/TH_1"/>
	<opentheso:memberOf rdf:resource="https://ark.frantiq.fr/ark:/26678/pcrtv66rn9cbv1"/>
	<opentheso:memberOf rdf:resource="https://ark.frantiq.fr/ark:/26678/pcrtnbDLi2FkAj"/>
	<skos:exactMatch rdf:resource="https://www.wikidata.org/wiki/Q11254"/>
	<skos:exactMatch rdf:resource="http://vocab.getty.edu/aat/300386506"/>
	<dcterms:created rdf:datatype="http://www.w3.org/2001/XMLSchema#date">2007-02-08</dcterms:created>
	<dcterms:modified rdf:datatype="http://www.w3.org/2001/XMLSchema#date">2024-02-14</dcterms:modified>
	<dcterms:identifier>16883</dcterms:identifier>
	<dcterms:contributor>blandine.nouvel</dcterms:contributor>
	<dcterms:contributor>justine.vincent</dcterms:contributor>
	<skos:definition xml:lang="fr">Solide ionique, utilisé en alimentation comme condiment, agent de conservation ou de préparation et principalement produit à partir de sel gemme ou de sel de mer. (d'après Wikipedia, 2021).</skos:definition>
	<skos:definition xml:lang="en">Ionic solid, used in food as a condiment, preservative or preparation agent and mainly produced from rock salt or sea salt (according to Wikipedia, 2021).</skos:definition>
</rdf:Description>

<rdf:Description rdf:about="https://ark.frantiq.fr/ark:/26678/pcrtT7b3IVuYxG">
	<rdf:type rdf:resource="http://www.w3.org/2004/02/skos/core#Concept"/>
	<skos:prefLabel xml:lang="nl">serpentijn</skos:prefLabel>
	<skos:prefLabel xml:lang="es">serpentina</skos:prefLabel>
	<skos:prefLabel xml:lang="fr">serpentine</skos:prefLabel>
	<skos:prefLabel xml:lang="de">Serpentinit</skos:prefLabel>
	<skos:prefLabel xml:lang="en">serpentinite</skos:prefLabel>
	<skos:prefLabel xml:lang="it">serpentino</skos:prefLabel>
	<skos:prefLabel xml:lang="ar">حَجَر الحية</skos:prefLabel>
	<skos:related rdf:resource="https://ark.frantiq.fr/ark:/26678/pcrtSpItdjR86k"/>
	<skos:broader rdf:resource="https://ark.frantiq.fr/ark:/26678/pcrtxybfLE1dkn"/>
	<skos:inScheme rdf:resource="https://ark.frantiq.fr/ark:/26678/TH_1"/>
	<opentheso:memberOf rdf:resource="https://ark.frantiq.fr/ark:/26678/pcrtv66rn9cbv1"/>
	<opentheso:memberOf rdf:resource="https://ark.frantiq.fr/ark:/26678/pcrtnbDLi2FkAj"/>
	<skos:exactMatch rdf:resource="https://catalogue.bnf.fr/ark:/12148/cb120036224"/>
	<skos:exactMatch rdf:resource="https://www.wikidata.org/wiki/Q335249"/>
	<dcterms:created rdf:datatype="http://www.w3.org/2001/XMLSchema#date">2007-02-08</dcterms:created>
	<dcterms:modified rdf:datatype="http://www.w3.org/2001/XMLSchema#date">2024-11-18</dcterms:modified>
	<dcterms:identifier>16893</dcterms:identifier>
	<dcterms:contributor>blandine.nouvel</dcterms:contributor>
	<dcterms:contributor>justine.vincent</dcterms:contributor>
	<skos:definition xml:lang="en">A family of minerals in the silicate group, comprising dark green metamorphic rocks. (wp)</skos:definition>
	<skos:definition xml:lang="fr">Famille de minéraux du groupe des silicates, comprenant des roches métamorphiques vert sombre. (wp)</skos:definition>
</rdf:Description>

<rdf:Description rdf:about="https://ark.frantiq.fr/ark:/26678/pcrtIzSUofuocv">
	<rdf:type rdf:resource="http://www.w3.org/2004/02/skos/core#Concept"/>
	<skos:prefLabel xml:lang="de">Feuerstein</skos:prefLabel>
	<skos:prefLabel xml:lang="en">flint</skos:prefLabel>
	<skos:prefLabel xml:lang="es">pedernal</skos:prefLabel>
	<skos:prefLabel xml:lang="it">selce</skos:prefLabel>
	<skos:prefLabel xml:lang="fr">silex</skos:prefLabel>
	<skos:prefLabel xml:lang="nl">vuursteen</skos:prefLabel>
	<skos:prefLabel xml:lang="ar">صوان</skos:prefLabel>
	<skos:altLabel xml:lang="de">Hornstein</skos:altLabel>
	<skos:altLabel xml:lang="de">Silex</skos:altLabel>
	<skos:altLabel xml:lang="es">sílex</skos:altLabel>
	<skos:narrower rdf:resource="https://ark.frantiq.fr/ark:/26678/pcrtbjSdl4I8Mo"/>
	<skos:broader rdf:resource="https://ark.frantiq.fr/ark:/26678/pcrt4N9jrETRto"/>
	<skos:inScheme rdf:resource="https://ark.frantiq.fr/ark:/26678/TH_1"/>
	<opentheso:memberOf rdf:resource="https://ark.frantiq.fr/ark:/26678/pcrtv66rn9cbv1"/>
	<opentheso:memberOf rdf:resource="https://ark.frantiq.fr/ark:/26678/pcrtnbDLi2FkAj"/>
	<opentheso:memberOf rdf:resource="https://ark.frantiq.fr/ark:/26678/pcrtv0jq332vcq3gxt5m13d5"/>
	<skos:exactMatch rdf:resource="https://catalogue.bnf.fr/ark:/12148/cb120488232"/>
	<skos:exactMatch rdf:resource="https://www.wikidata.org/wiki/Q83087"/>
	<skos:exactMatch rdf:resource="http://vocab.getty.edu/aat/300011143"/>
	<dcterms:created rdf:datatype="http://www.w3.org/2001/XMLSchema#date">2007-02-08</dcterms:created>
	<dcterms:modified rdf:datatype="http://www.w3.org/2001/XMLSchema#date">2025-01-17</dcterms:modified>
	<dcterms:identifier>16943</dcterms:identifier>
	<dcterms:contributor>blandine.nouvel</dcterms:contributor>
	<dcterms:contributor>irene.weis</dcterms:contributor>
	<skos:definition xml:lang="fr">Terme employé pour les accidents siliceux en milieu carbonaté, désignant les roches hyper siliceuses qui résultent en grand partie d'un remplacement des carbonates et des bioclastes par épigénèse, et se développe dans des formations marines, lacustres et palustres ce qui détermine leur classification en silex « marin », silex « lacustre » ou silex « palustre ». Il est constitué de grains fins, à cassure lustrée. Il est dissocié du sédiment d'origine par un cortex et constitué d'au moins 90 % de silice (le plus souvent de la calcédoine). La phase minérale majeure détermine les variétés : silex à opale CT, silex à quartz microcristallin etc. (Fernandes, 2012).</skos:definition>
	<skos:definition xml:lang="en">Term used for siliceous rocks in carbonate environments, designating hyper-siliceous rocks that are largely the result of replacement of carbonates and bioclasts by epigenesis, and develop in marine, lacustrine and palustrine formations, which determines their classification as  marine ,  lacustrine  or  palustrine  flint. It is made up of fine grains with a lustrous fracture. It is separated from the original sediment by a cortex and consists of at least 90% silica (most often chalcedony). The major mineral phase determines the varieties: CT opal flint, microcrystalline quartz flint, etc. (Fernandes, 2012).</skos:definition>
</rdf:Description>

<rdf:Description rdf:about="https://ark.frantiq.fr/ark:/26678/pcrttxsm3xSsiz">
	<rdf:type rdf:resource="http://www.w3.org/2004/02/skos/core#Concept"/>
	<skos:prefLabel xml:lang="es">seda</skos:prefLabel>
	<skos:prefLabel xml:lang="de">Seide</skos:prefLabel>
	<skos:prefLabel xml:lang="it">seta</skos:prefLabel>
	<skos:prefLabel xml:lang="en">silk</skos:prefLabel>
	<skos:prefLabel xml:lang="fr">soie</skos:prefLabel>
	<skos:prefLabel xml:lang="nl">zijde</skos:prefLabel>
	<skos:prefLabel xml:lang="ar">حرير</skos:prefLabel>
	<skos:related rdf:resource="https://ark.frantiq.fr/ark:/26678/pcrtTYhjuWkfmK"/>
	<skos:related rdf:resource="https://ark.frantiq.fr/ark:/26678/crtRdvPhajbsq"/>
	<skos:broader rdf:resource="https://ark.frantiq.fr/ark:/26678/pcrtwvFLgSQRs5"/>
	<skos:inScheme rdf:resource="https://ark.frantiq.fr/ark:/26678/TH_1"/>
	<opentheso:memberOf rdf:resource="https://ark.frantiq.fr/ark:/26678/pcrtv66rn9cbv1"/>
	<opentheso:memberOf rdf:resource="https://ark.frantiq.fr/ark:/26678/pcrtnbDLi2FkAj"/>
	<skos:exactMatch rdf:resource="https://catalogue.bnf.fr/ark:/12148/cb11941507q"/>
	<skos:exactMatch rdf:resource="https://www.wikidata.org/wiki/Q37681"/>
	<skos:exactMatch rdf:resource="http://vocab.getty.edu/aat/300014072"/>
	<dcterms:created rdf:datatype="http://www.w3.org/2001/XMLSchema#date">2007-02-08</dcterms:created>
	<dcterms:modified rdf:datatype="http://www.w3.org/2001/XMLSchema#date">2023-08-02</dcterms:modified>
	<dcterms:identifier>16971</dcterms:identifier>
	<dcterms:contributor>blandine.nouvel</dcterms:contributor>
	<skos:definition xml:lang="en">Natural protein fibre of animal origin used in the manufacture of textile articles and products. (wp)</skos:definition>
	<skos:definition xml:lang="fr">Fibre protéique naturelle d'origine animale utilisée dans la fabrication d'articles et produits textiles. (wp)</skos:definition>
</rdf:Description>

<rdf:Description rdf:about="https://ark.frantiq.fr/ark:/26678/pcrt6TSfpXkNW6">
	<rdf:type rdf:resource="http://www.w3.org/2004/02/skos/core#Concept"/>
	<skos:prefLabel xml:lang="es">estratos geológicos</skos:prefLabel>
	<skos:prefLabel xml:lang="en">geological strata</skos:prefLabel>
	<skos:prefLabel xml:lang="nl">geologische lagen</skos:prefLabel>
	<skos:prefLabel xml:lang="de">geologische Schichten</skos:prefLabel>
	<skos:prefLabel xml:lang="fr">strate géologique</skos:prefLabel>
	<skos:prefLabel xml:lang="it">strati geologici</skos:prefLabel>
	<skos:prefLabel xml:lang="ar">الطبقات الجيولوجية</skos:prefLabel>
	<skos:altLabel xml:lang="en">geological beds</skos:altLabel>
	<skos:altLabel xml:lang="en">geological lamina</skos:altLabel>
	<skos:altLabel xml:lang="fr">géologie historique</skos:altLabel>
	<skos:altLabel xml:lang="it">stratigrafia geologica</skos:altLabel>
	<skos:related rdf:resource="https://ark.frantiq.fr/ark:/26678/pcrt4vmcwIU4yP"/>
	<skos:broader rdf:resource="https://ark.frantiq.fr/ark:/26678/pcrtr5vk7w9vdz"/>
	<skos:inScheme rdf:resource="https://ark.frantiq.fr/ark:/26678/TH_1"/>
	<opentheso:memberOf rdf:resource="https://ark.frantiq.fr/ark:/26678/pcrtv66rn9cbv1"/>
	<opentheso:memberOf rdf:resource="https://ark.frantiq.fr/ark:/26678/pcrtnbDLi2FkAj"/>
	<skos:exactMatch rdf:resource="https://www.wikidata.org/wiki/Q12758989"/>
	<dcterms:created rdf:datatype="http://www.w3.org/2001/XMLSchema#date">2007-02-08</dcterms:created>
	<dcterms:modified rdf:datatype="http://www.w3.org/2001/XMLSchema#date">2024-11-21</dcterms:modified>
	<dcterms:identifier>17049</dcterms:identifier>
	<dcterms:contributor>blandine.nouvel</dcterms:contributor>
	<dcterms:contributor>justine.vincent</dcterms:contributor>
	<skos:definition xml:lang="en">Layers of rock piled one on top of the other, making up a terrain, each distinguished by petrographic, mineralogical, granulometric, tectonic and palaeontological characteristics.</skos:definition>
	<skos:definition xml:lang="fr">Couches de roches empilées les unes au-dessus des autres, constituant un terrain, qui se distinguent chacune par des caractéristiques pétrographiques, minéralogiques, granulométriques, tectoniques et paléontolologiques.</skos:definition>
</rdf:Description>

<rdf:Description rdf:about="https://ark.frantiq.fr/ark:/26678/pcrtsIGcaQ8O7x">
	<rdf:type rdf:resource="http://www.w3.org/2004/02/skos/core#Concept"/>
	<skos:prefLabel xml:lang="es">estuco</skos:prefLabel>
	<skos:prefLabel xml:lang="nl">pleisterkalk</skos:prefLabel>
	<skos:prefLabel xml:lang="fr">stuc</skos:prefLabel>
	<skos:prefLabel xml:lang="en">stucco</skos:prefLabel>
	<skos:prefLabel xml:lang="it">stucco</skos:prefLabel>
	<skos:prefLabel xml:lang="de">Stuck</skos:prefLabel>
	<skos:prefLabel xml:lang="ar">مِلاط الجبس</skos:prefLabel>
	<skos:altLabel xml:lang="en">render</skos:altLabel>
	<skos:related rdf:resource="https://ark.frantiq.fr/ark:/26678/pcrtERMm8Q0wYw"/>
	<skos:narrower rdf:resource="https://ark.frantiq.fr/ark:/26678/pcrt9SkpOgSbXw"/>
	<skos:broader rdf:resource="https://ark.frantiq.fr/ark:/26678/pcrt4KRB12RYGv"/>
	<skos:inScheme rdf:resource="https://ark.frantiq.fr/ark:/26678/TH_1"/>
	<opentheso:memberOf rdf:resource="https://ark.frantiq.fr/ark:/26678/pcrtv66rn9cbv1"/>
	<opentheso:memberOf rdf:resource="https://ark.frantiq.fr/ark:/26678/pcrtnbDLi2FkAj"/>
	<skos:exactMatch rdf:resource="https://catalogue.bnf.fr/ark:/12148/cb11953328t"/>
	<skos:exactMatch rdf:resource="https://www.wikidata.org/wiki/Q33526"/>
	<skos:exactMatch rdf:resource="http://vocab.getty.edu/aat/300014966"/>
	<dcterms:created rdf:datatype="http://www.w3.org/2001/XMLSchema#date">2007-02-08</dcterms:created>
	<dcterms:modified rdf:datatype="http://www.w3.org/2001/XMLSchema#date">2023-12-08</dcterms:modified>
	<dcterms:identifier>17061</dcterms:identifier>
	<dcterms:contributor>blandine.nouvel</dcterms:contributor>
	<dcterms:contributor>remi.ancel</dcterms:contributor>
	<skos:definition xml:lang="en">Architectural decoration in relief made with a plastic material, generally white, of variable composition (lime and crushed marble, plaster and glue), which can be coloured with pigments, worked by modelling or moulding, and hardening in the air (Nouveau dictionnaire raisonné de l'architecture de Viollet le Duc, 2023).</skos:definition>
	<skos:definition xml:lang="fr">Décor architectural en relief réalisé avec un matériau plastique généralement blanc, de composition variable (chaux et marbre broyé, plâtre et colle), pouvant être coloré par des pigments, travaillé par modelage ou moulage, et durcissant à l'air (Nouveau dictionnaire raisonné de l'architecture de Viollet le Duc, 2023)</skos:definition>
</rdf:Description>

<rdf:Description rdf:about="https://ark.frantiq.fr/ark:/26678/pcrt9SkpOgSbXw">
	<rdf:type rdf:resource="http://www.w3.org/2004/02/skos/core#Concept"/>
	<skos:prefLabel xml:lang="de">bemalter Stuck</skos:prefLabel>
	<skos:prefLabel xml:lang="nl">beschilderd stucwerk</skos:prefLabel>
	<skos:prefLabel xml:lang="es">estuco pintado</skos:prefLabel>
	<skos:prefLabel xml:lang="en">painted stucco</skos:prefLabel>
	<skos:prefLabel xml:lang="it">stucco dipinto</skos:prefLabel>
	<skos:prefLabel xml:lang="fr">stuc peint</skos:prefLabel>
	<skos:prefLabel xml:lang="ar">لوحة جصية</skos:prefLabel>
	<skos:related rdf:resource="https://ark.frantiq.fr/ark:/26678/pcrtmZ7gZV6UUA"/>
	<skos:related rdf:resource="https://ark.frantiq.fr/ark:/26678/pcrtvsFBSmOKN2"/>
	<skos:broader rdf:resource="https://ark.frantiq.fr/ark:/26678/pcrtsIGcaQ8O7x"/>
	<skos:inScheme rdf:resource="https://ark.frantiq.fr/ark:/26678/TH_1"/>
	<opentheso:memberOf rdf:resource="https://ark.frantiq.fr/ark:/26678/pcrtv66rn9cbv1"/>
	<opentheso:memberOf rdf:resource="https://ark.frantiq.fr/ark:/26678/pcrtnbDLi2FkAj"/>
	<dcterms:created rdf:datatype="http://www.w3.org/2001/XMLSchema#date">2007-02-08</dcterms:created>
	<dcterms:modified rdf:datatype="http://www.w3.org/2001/XMLSchema#date">2023-08-02</dcterms:modified>
	<dcterms:identifier>17062</dcterms:identifier>
	<dcterms:contributor>blandine.nouvel</dcterms:contributor>
	<skos:definition xml:lang="en">A decorative wall coating that has been painted.</skos:definition>
	<skos:definition xml:lang="fr">Enduit mural à usage décoratif ayant été peint.</skos:definition>
</rdf:Description>

<rdf:Description rdf:about="https://ark.frantiq.fr/ark:/26678/pcrtnpv5KJIXTy">
	<rdf:type rdf:resource="http://www.w3.org/2004/02/skos/core#Concept"/>
	<skos:prefLabel xml:lang="es">esteatita</skos:prefLabel>
	<skos:prefLabel xml:lang="nl">steatiet</skos:prefLabel>
	<skos:prefLabel xml:lang="de">Steatit</skos:prefLabel>
	<skos:prefLabel xml:lang="en">steatite</skos:prefLabel>
	<skos:prefLabel xml:lang="it">steatite</skos:prefLabel>
	<skos:prefLabel xml:lang="fr">stéatite</skos:prefLabel>
	<skos:prefLabel xml:lang="ar">حجر الطَّلق</skos:prefLabel>
	<skos:altLabel xml:lang="en">soaprock</skos:altLabel>
	<skos:altLabel xml:lang="en">soapstone</skos:altLabel>
	<skos:narrower rdf:resource="https://ark.frantiq.fr/ark:/26678/pcrtnlpDSw0du4"/>
	<skos:broader rdf:resource="https://ark.frantiq.fr/ark:/26678/pcrtxybfLE1dkn"/>
	<skos:inScheme rdf:resource="https://ark.frantiq.fr/ark:/26678/TH_1"/>
	<opentheso:memberOf rdf:resource="https://ark.frantiq.fr/ark:/26678/pcrtv66rn9cbv1"/>
	<opentheso:memberOf rdf:resource="https://ark.frantiq.fr/ark:/26678/pcrtnbDLi2FkAj"/>
	<skos:exactMatch rdf:resource="https://catalogue.bnf.fr/ark:/12148/cb11965047z"/>
	<skos:exactMatch rdf:resource="https://www.wikidata.org/wiki/Q707896"/>
	<skos:exactMatch rdf:resource="http://vocab.getty.edu/aat/300011665"/>
	<dcterms:created rdf:datatype="http://www.w3.org/2001/XMLSchema#date">2007-02-08</dcterms:created>
	<dcterms:modified rdf:datatype="http://www.w3.org/2001/XMLSchema#date">2023-08-02</dcterms:modified>
	<dcterms:identifier>17133</dcterms:identifier>
	<dcterms:contributor>blandine.nouvel</dcterms:contributor>
	<skos:definition xml:lang="en">Very soft rock, mainly composed of talc (wp)</skos:definition>
	<skos:definition xml:lang="fr">Roche très tendre, principalement composée de talc. (wp)</skos:definition>
</rdf:Description>

<rdf:Description rdf:about="https://ark.frantiq.fr/ark:/26678/pcrt1wEGrR9DT3">
	<rdf:type rdf:resource="http://www.w3.org/2004/02/skos/core#Concept"/>
	<skos:prefLabel xml:lang="es">azúcar</skos:prefLabel>
	<skos:prefLabel xml:lang="fr">sucre</skos:prefLabel>
	<skos:prefLabel xml:lang="en">sugar</skos:prefLabel>
	<skos:prefLabel xml:lang="nl">suiker</skos:prefLabel>
	<skos:prefLabel xml:lang="it">zucchero</skos:prefLabel>
	<skos:prefLabel xml:lang="de">Zucker</skos:prefLabel>
	<skos:prefLabel xml:lang="ar">سُكر</skos:prefLabel>
	<skos:related rdf:resource="https://ark.frantiq.fr/ark:/26678/crtLsb4JNRGOS"/>
	<skos:related rdf:resource="https://ark.frantiq.fr/ark:/26678/crt5Y63J4cajj"/>
	<skos:related rdf:resource="https://ark.frantiq.fr/ark:/26678/pcrta3PzVQ4Hnu"/>
	<skos:related rdf:resource="https://ark.frantiq.fr/ark:/26678/pcrtrppzffph84sktxqdz4q5"/>
	<skos:broader rdf:resource="https://ark.frantiq.fr/ark:/26678/pcrtUTZqItd8SL"/>
	<skos:inScheme rdf:resource="https://ark.frantiq.fr/ark:/26678/TH_1"/>
	<opentheso:memberOf rdf:resource="https://ark.frantiq.fr/ark:/26678/pcrtv66rn9cbv1"/>
	<opentheso:memberOf rdf:resource="https://ark.frantiq.fr/ark:/26678/pcrtnbDLi2FkAj"/>
	<skos:exactMatch rdf:resource="https://www.wikidata.org/wiki/Q11002"/>
	<skos:exactMatch rdf:resource="http://vocab.getty.edu/aat/300183931"/>
	<dcterms:created rdf:datatype="http://www.w3.org/2001/XMLSchema#date">2007-02-08</dcterms:created>
	<dcterms:modified rdf:datatype="http://www.w3.org/2001/XMLSchema#date">2024-03-20</dcterms:modified>
	<dcterms:identifier>17143</dcterms:identifier>
	<dcterms:contributor>blandine.nouvel</dcterms:contributor>
	<dcterms:contributor>justine.vincent</dcterms:contributor>
	<skos:definition xml:lang="fr">Substance de saveur douce, extraite principalement de la canne à sucre et de la betterave sucrière. (Wikipedia)</skos:definition>
	<skos:definition xml:lang="en">A sweet-tasting substance extracted mainly from sugar cane and sugar beet. (Wikipedia)</skos:definition>
</rdf:Description>

<rdf:Description rdf:about="https://ark.frantiq.fr/ark:/26678/pcrtfx4s0yvSLj">
	<rdf:type rdf:resource="http://www.w3.org/2004/02/skos/core#Concept"/>
	<skos:prefLabel xml:lang="es">terracota</skos:prefLabel>
	<skos:prefLabel xml:lang="en">terracotta</skos:prefLabel>
	<skos:prefLabel xml:lang="it">terracotta</skos:prefLabel>
	<skos:prefLabel xml:lang="nl">terracotta</skos:prefLabel>
	<skos:prefLabel xml:lang="de">Terrakotta</skos:prefLabel>
	<skos:prefLabel xml:lang="fr">terre cuite</skos:prefLabel>
	<skos:prefLabel xml:lang="ar">فخار مشوي</skos:prefLabel>
	<skos:altLabel xml:lang="en">terra cotta</skos:altLabel>
	<skos:altLabel xml:lang="fr">terra cotta</skos:altLabel>
	<skos:altLabel xml:lang="en">terra-cotta</skos:altLabel>
	<skos:altLabel xml:lang="fr">terracottas</skos:altLabel>
	<skos:related rdf:resource="https://ark.frantiq.fr/ark:/26678/pcrto44p1SaKFn"/>
	<skos:related rdf:resource="https://ark.frantiq.fr/ark:/26678/pcrtL7wUJowBSL"/>
	<skos:related rdf:resource="https://ark.frantiq.fr/ark:/26678/pcrtXpeIEtqsSk"/>
	<skos:related rdf:resource="https://ark.frantiq.fr/ark:/26678/pcrtvzUoe0N6qk"/>
	<skos:related rdf:resource="https://ark.frantiq.fr/ark:/26678/crt9ey83pmtqt"/>
	<skos:related rdf:resource="https://ark.frantiq.fr/ark:/26678/pcrtr3hwptzwvv"/>
	<skos:narrower rdf:resource="https://ark.frantiq.fr/ark:/26678/pcrt1DMOWvDF4j"/>
	<skos:narrower rdf:resource="https://ark.frantiq.fr/ark:/26678/pcrtho8l95no0j"/>
	<skos:narrower rdf:resource="https://ark.frantiq.fr/ark:/26678/pcrtqHWkorsw9D"/>
	<skos:narrower rdf:resource="https://ark.frantiq.fr/ark:/26678/pcrtPEGVkSl8Hk"/>
	<skos:narrower rdf:resource="https://ark.frantiq.fr/ark:/26678/pcrtPLs10mF9zI"/>
	<skos:narrower rdf:resource="https://ark.frantiq.fr/ark:/26678/pcrtaUOSeoPg5g"/>
	<skos:narrower rdf:resource="https://ark.frantiq.fr/ark:/26678/pcrtK43haeM3e3"/>
	<skos:narrower rdf:resource="https://ark.frantiq.fr/ark:/26678/pcrtt7G9pnQlu1"/>
	<skos:narrower rdf:resource="https://ark.frantiq.fr/ark:/26678/pcrtolrabjfp2T"/>
	<skos:narrower rdf:resource="https://ark.frantiq.fr/ark:/26678/pcrtnR5ePytFhO"/>
	<skos:narrower rdf:resource="https://ark.frantiq.fr/ark:/26678/pcrt73gjdrz4rx"/>
	<skos:narrower rdf:resource="https://ark.frantiq.fr/ark:/26678/pcrt1asKmbn9q8"/>
	<skos:narrower rdf:resource="https://ark.frantiq.fr/ark:/26678/pcrtSdKu9rjDHO"/>
	<skos:broader rdf:resource="https://ark.frantiq.fr/ark:/26678/pcrtIMsuG0RWTs"/>
	<skos:inScheme rdf:resource="https://ark.frantiq.fr/ark:/26678/TH_1"/>
	<opentheso:memberOf rdf:resource="https://ark.frantiq.fr/ark:/26678/pcrtv66rn9cbv1"/>
	<opentheso:memberOf rdf:resource="https://ark.frantiq.fr/ark:/26678/pcrtnbDLi2FkAj"/>
	<opentheso:memberOf rdf:resource="https://ark.frantiq.fr/ark:/26678/pcrtv0jq332vcq3gxt5m13d5"/>
	<iso-thes:subordinateArray rdf:resource="https://pactols.frantiq.fr/?idf=F795&amp;idt=TH_1"/>
	<skos:exactMatch rdf:resource="https://catalogue.bnf.fr/ark:/12148/cb119452651"/>
	<skos:exactMatch rdf:resource="https://www.wikidata.org/wiki/Q60424"/>
	<skos:exactMatch rdf:resource="http://vocab.getty.edu/aat/300010669"/>
	<dcterms:created rdf:datatype="http://www.w3.org/2001/XMLSchema#date">2007-02-08</dcterms:created>
	<dcterms:modified rdf:datatype="http://www.w3.org/2001/XMLSchema#date">2024-10-18</dcterms:modified>
	<dcterms:identifier>17266</dcterms:identifier>
	<dcterms:contributor>blandine.nouvel</dcterms:contributor>
	<dcterms:contributor>irene.weis</dcterms:contributor>
	<dcterms:contributor>justine.vincent</dcterms:contributor>
	<skos:definition xml:lang="fr">Matériau céramique, obtenu par la cuisson d'argile, utilisé pour réaliser des poteries, des sculptures et pour la fabrication de matériaux de construction, briques, tuiles ou carreaux (d'après l'article en français  terre cuite  de wikipedia, consulté le 19/10/18).</skos:definition>
	<skos:definition xml:lang="en">Ceramic material, obtained by firing clay, used to make pottery, sculptures and building materials such as bricks, tiles or flagstones (according to the French article  terre cuite  on wikipedia, consulted on 19/10/18).</skos:definition>
	<skos:scopeNote xml:lang="fr">Pour la terre cuite utilisée en contexte architectural, privilégier le concept  terre cuite architecturale</skos:scopeNote>
</rdf:Description>

<rdf:Description rdf:about="https://ark.frantiq.fr/ark:/26678/pcrthAOjGBEfZk">
	<rdf:type rdf:resource="http://www.w3.org/2004/02/skos/core#Concept"/>
	<skos:prefLabel xml:lang="it">tessile</skos:prefLabel>
	<skos:prefLabel xml:lang="nl">textiel</skos:prefLabel>
	<skos:prefLabel xml:lang="es">textil</skos:prefLabel>
	<skos:prefLabel xml:lang="de">Textil</skos:prefLabel>
	<skos:prefLabel xml:lang="en">textile</skos:prefLabel>
	<skos:prefLabel xml:lang="fr">textile</skos:prefLabel>
	<skos:prefLabel xml:lang="ar">نسيج</skos:prefLabel>
	<skos:related rdf:resource="https://ark.frantiq.fr/ark:/26678/pcrtra3VNaUWSW"/>
	<skos:related rdf:resource="https://ark.frantiq.fr/ark:/26678/pcrt3We1mLOmN0"/>
	<skos:related rdf:resource="https://ark.frantiq.fr/ark:/26678/pcrtDfHvvnBWz7"/>
	<skos:related rdf:resource="https://ark.frantiq.fr/ark:/26678/pcrtd1ANdItlam"/>
	<skos:related rdf:resource="https://ark.frantiq.fr/ark:/26678/pcrtNQhoS8U7Ve"/>
	<skos:related rdf:resource="https://ark.frantiq.fr/ark:/26678/pcrtqGQOorLDxx"/>
	<skos:related rdf:resource="https://ark.frantiq.fr/ark:/26678/pcrtu4Do7EDGDg"/>
	<skos:related rdf:resource="https://ark.frantiq.fr/ark:/26678/pcrt5j9z1z718wq4mnx49j43"/>
	<skos:broader rdf:resource="https://ark.frantiq.fr/ark:/26678/pcrtIMsuG0RWTs"/>
	<skos:inScheme rdf:resource="https://ark.frantiq.fr/ark:/26678/TH_1"/>
	<opentheso:memberOf rdf:resource="https://ark.frantiq.fr/ark:/26678/pcrtv66rn9cbv1"/>
	<opentheso:memberOf rdf:resource="https://ark.frantiq.fr/ark:/26678/pcrtnbDLi2FkAj"/>
	<skos:exactMatch rdf:resource="https://www.wikidata.org/wiki/Q28823"/>
	<skos:exactMatch rdf:resource="http://vocab.getty.edu/aat/300014063"/>
	<skos:exactMatch rdf:resource="http://vocab.getty.edu/aat/300231565"/>
	<dcterms:created rdf:datatype="http://www.w3.org/2001/XMLSchema#date">2007-02-08</dcterms:created>
	<dcterms:modified rdf:datatype="http://www.w3.org/2001/XMLSchema#date">2023-08-02</dcterms:modified>
	<dcterms:identifier>17278</dcterms:identifier>
	<dcterms:contributor>blandine.nouvel</dcterms:contributor>
	<skos:definition xml:lang="en">Material of animal, mineral or vegetable origin, natural, artificial or synthetic, suitable for being transformed into yarn and then woven (d'ap. cnrtl)</skos:definition>
	<skos:definition xml:lang="fr">Matière d'origine animale, minérale ou végétale, naturelle, artificielle ou synthétique, propre à être transformée en fil, puis tissée (d'ap. cnrtl)</skos:definition>
</rdf:Description>

<rdf:Description rdf:about="https://ark.frantiq.fr/ark:/26678/pcrtqGQOorLDxx">
	<rdf:type rdf:resource="http://www.w3.org/2004/02/skos/core#Concept"/>
	<skos:prefLabel xml:lang="en">fabric</skos:prefLabel>
	<skos:prefLabel xml:lang="de">Stoff</skos:prefLabel>
	<skos:prefLabel xml:lang="es">tejido</skos:prefLabel>
	<skos:prefLabel xml:lang="it">tessuto</skos:prefLabel>
	<skos:prefLabel xml:lang="fr">tissu</skos:prefLabel>
	<skos:prefLabel xml:lang="nl">weefsel</skos:prefLabel>
	<skos:prefLabel xml:lang="ar">قِماش</skos:prefLabel>
	<skos:altLabel xml:lang="en">cloth</skos:altLabel>
	<skos:altLabel xml:lang="fr">étoffe</skos:altLabel>
	<skos:altLabel xml:lang="it">stoffa</skos:altLabel>
	<skos:altLabel xml:lang="es">tela</skos:altLabel>
	<skos:altLabel xml:lang="en">textile</skos:altLabel>
	<skos:altLabel xml:lang="en">woven fabric</skos:altLabel>
	<skos:related rdf:resource="https://ark.frantiq.fr/ark:/26678/pcrtLhbOznwGk6"/>
	<skos:related rdf:resource="https://ark.frantiq.fr/ark:/26678/pcrthAOjGBEfZk"/>
	<skos:related rdf:resource="https://ark.frantiq.fr/ark:/26678/pcrtR1mzakcqfp"/>
	<skos:related rdf:resource="https://ark.frantiq.fr/ark:/26678/pcrtgkVy7lK4lN"/>
	<skos:related rdf:resource="https://ark.frantiq.fr/ark:/26678/pcrt5j9z1z718wq4mnx49j43"/>
	<skos:broader rdf:resource="https://ark.frantiq.fr/ark:/26678/pcrtIMsuG0RWTs"/>
	<skos:inScheme rdf:resource="https://ark.frantiq.fr/ark:/26678/TH_1"/>
	<opentheso:memberOf rdf:resource="https://ark.frantiq.fr/ark:/26678/pcrtv66rn9cbv1"/>
	<opentheso:memberOf rdf:resource="https://ark.frantiq.fr/ark:/26678/pcrtnbDLi2FkAj"/>
	<skos:exactMatch rdf:resource="https://www.wikidata.org/wiki/Q5849500"/>
	<skos:exactMatch rdf:resource="http://vocab.getty.edu/aat/300162391"/>
	<skos:relatedMatch rdf:resource="https://www.wikidata.org/wiki/Q192296"/>
	<dcterms:created rdf:datatype="http://www.w3.org/2001/XMLSchema#date">2007-02-08</dcterms:created>
	<dcterms:modified rdf:datatype="http://www.w3.org/2001/XMLSchema#date">2024-10-18</dcterms:modified>
	<dcterms:identifier>17305</dcterms:identifier>
	<dcterms:contributor>blandine.nouvel</dcterms:contributor>
	<dcterms:contributor>justine.vincent</dcterms:contributor>
	<skos:definition xml:lang="en">Material obtained by assembling interlaced threads. (Médard, in Batellerie gallo-romaine, 2011, p. 116)</skos:definition>
	<skos:definition xml:lang="fr">Matériau obtenu par l'assemblage de fils entrelacés. (Médard, in Batellerie gallo-romaine, 2011, p. 116)</skos:definition>
</rdf:Description>

<rdf:Description rdf:about="https://ark.frantiq.fr/ark:/26678/pcrtK8tO0rlQlM">
	<rdf:type rdf:resource="http://www.w3.org/2004/02/skos/core#Concept"/>
	<skos:prefLabel xml:lang="es">adobe</skos:prefLabel>
	<skos:prefLabel xml:lang="en">cob</skos:prefLabel>
	<skos:prefLabel xml:lang="it">impasto di argilla e paglia</skos:prefLabel>
	<skos:prefLabel xml:lang="nl">leemmortel</skos:prefLabel>
	<skos:prefLabel xml:lang="de">Lehmputz</skos:prefLabel>
	<skos:prefLabel xml:lang="fr">torchis</skos:prefLabel>
	<skos:prefLabel xml:lang="ar">طين ممزوج بالقش</skos:prefLabel>
	<skos:altLabel xml:lang="it">torchis</skos:altLabel>
	<skos:altLabel xml:lang="en">wattle and daub</skos:altLabel>
	<skos:broader rdf:resource="https://ark.frantiq.fr/ark:/26678/pcrtm6uoPROlPN"/>
	<skos:inScheme rdf:resource="https://ark.frantiq.fr/ark:/26678/TH_1"/>
	<opentheso:memberOf rdf:resource="https://ark.frantiq.fr/ark:/26678/pcrtv66rn9cbv1"/>
	<opentheso:memberOf rdf:resource="https://ark.frantiq.fr/ark:/26678/pcrtnbDLi2FkAj"/>
	<opentheso:memberOf rdf:resource="https://ark.frantiq.fr/ark:/26678/pcrtv0jq332vcq3gxt5m13d5"/>
	<skos:exactMatch rdf:resource="https://www.wikidata.org/wiki/Q1368940"/>
	<skos:exactMatch rdf:resource="http://vocab.getty.edu/aat/300010629"/>
	<skos:exactMatch rdf:resource="http://vocab.getty.edu/aat/300010630"/>
	<dcterms:created rdf:datatype="http://www.w3.org/2001/XMLSchema#date">2007-02-08</dcterms:created>
	<dcterms:modified rdf:datatype="http://www.w3.org/2001/XMLSchema#date">2024-10-25</dcterms:modified>
	<dcterms:identifier>17333</dcterms:identifier>
	<dcterms:contributor>blandine.nouvel</dcterms:contributor>
	<dcterms:contributor>irene.weis</dcterms:contributor>
	<dcterms:contributor>patricia.moitrel</dcterms:contributor>
	<skos:definition xml:lang="en">A mixture of clay-loam soil, plant fibres (straw) or animal fibres (horsehair) and water. Applied to a rafting or lath, it is used as a filling material between the load-bearing elements of a timber frame forming an exterior or interior wall. (Pactols Group)</skos:definition>
	<skos:definition xml:lang="fr">Mélange à base de terre argilo-limoneuse, de fibres végétales (paille) voire animale (crin) et d'eau. Appliqué sur un clayonnage ou un lattis, il sert de matériau de remplissage entre les éléments porteurs d'un pan de bois formant un mur, extérieur ou intérieur.</skos:definition>
</rdf:Description>

<rdf:Description rdf:about="https://ark.frantiq.fr/ark:/26678/pcrtv3md53Ugxj">
	<rdf:type rdf:resource="http://www.w3.org/2004/02/skos/core#Concept"/>
	<skos:prefLabel xml:lang="it">turchese</skos:prefLabel>
	<skos:prefLabel xml:lang="de">Türkis</skos:prefLabel>
	<skos:prefLabel xml:lang="nl">turkoois</skos:prefLabel>
	<skos:prefLabel xml:lang="es">turquesa</skos:prefLabel>
	<skos:prefLabel xml:lang="en">turquoise</skos:prefLabel>
	<skos:prefLabel xml:lang="fr">turquoise</skos:prefLabel>
	<skos:prefLabel xml:lang="ar">فيروز</skos:prefLabel>
	<skos:altLabel xml:lang="es">calaíta</skos:altLabel>
	<skos:related rdf:resource="https://ark.frantiq.fr/ark:/26678/pcrtaJLEkei5LQ"/>
	<skos:broader rdf:resource="https://ark.frantiq.fr/ark:/26678/pcrtJt3ZKiNEFK"/>
	<skos:inScheme rdf:resource="https://ark.frantiq.fr/ark:/26678/TH_1"/>
	<opentheso:memberOf rdf:resource="https://ark.frantiq.fr/ark:/26678/pcrtv66rn9cbv1"/>
	<opentheso:memberOf rdf:resource="https://ark.frantiq.fr/ark:/26678/pcrtnbDLi2FkAj"/>
	<skos:exactMatch rdf:resource="https://catalogue.bnf.fr/ark:/12148/cb125484872"/>
	<skos:exactMatch rdf:resource="https://www.wikidata.org/wiki/Q165254"/>
	<skos:exactMatch rdf:resource="http://vocab.getty.edu/aat/300011164"/>
	<dcterms:created rdf:datatype="http://www.w3.org/2001/XMLSchema#date">2007-02-08</dcterms:created>
	<dcterms:modified rdf:datatype="http://www.w3.org/2001/XMLSchema#date">2023-08-02</dcterms:modified>
	<dcterms:identifier>17425</dcterms:identifier>
	<dcterms:contributor>blandine.nouvel</dcterms:contributor>
	<skos:definition xml:lang="en">A fine, opaque, sky-blue to blue-green stone which is a natural hydrated phosphate of aluminium and copper. (Lar.)</skos:definition>
	<skos:definition xml:lang="fr">Pierre fine de couleur bleu ciel à bleu-vert, opaque, qui est un phosphate hydraté naturel d'aluminium et de cuivre. (Lar.)</skos:definition>
</rdf:Description>

<rdf:Description rdf:about="https://ark.frantiq.fr/ark:/26678/pcrttS4bFv2ezb">
	<rdf:type rdf:resource="http://www.w3.org/2004/02/skos/core#Concept"/>
	<skos:prefLabel xml:lang="es">barniz</skos:prefLabel>
	<skos:prefLabel xml:lang="de">gefirniste Keramik</skos:prefLabel>
	<skos:prefLabel xml:lang="en">glaze</skos:prefLabel>
	<skos:prefLabel xml:lang="it">vernice</skos:prefLabel>
	<skos:prefLabel xml:lang="fr">vernis</skos:prefLabel>
	<skos:prefLabel xml:lang="nl">vernis</skos:prefLabel>
	<skos:prefLabel xml:lang="ar">بَرنيق</skos:prefLabel>
	<skos:altLabel xml:lang="it">smalto</skos:altLabel>
	<skos:related rdf:resource="https://ark.frantiq.fr/ark:/26678/pcrtnR5ePytFhO"/>
	<skos:related rdf:resource="https://ark.frantiq.fr/ark:/26678/pcrtvmf0n3xbgj"/>
	<skos:related rdf:resource="https://ark.frantiq.fr/ark:/26678/pcrtw7wr6cx38h"/>
	<skos:narrower rdf:resource="https://ark.frantiq.fr/ark:/26678/pcrt065IhLltVk"/>
	<skos:narrower rdf:resource="https://ark.frantiq.fr/ark:/26678/pcrtJXS9PmPlFX"/>
	<skos:broader rdf:resource="https://ark.frantiq.fr/ark:/26678/pcrtIMsuG0RWTs"/>
	<skos:inScheme rdf:resource="https://ark.frantiq.fr/ark:/26678/TH_1"/>
	<opentheso:memberOf rdf:resource="https://ark.frantiq.fr/ark:/26678/pcrtv66rn9cbv1"/>
	<opentheso:memberOf rdf:resource="https://ark.frantiq.fr/ark:/26678/pcrtnbDLi2FkAj"/>
	<skos:exactMatch rdf:resource="https://www.wikidata.org/wiki/Q81683"/>
	<skos:exactMatch rdf:resource="http://vocab.getty.edu/aat/300014974"/>
	<dcterms:created rdf:datatype="http://www.w3.org/2001/XMLSchema#date">2007-02-08</dcterms:created>
	<dcterms:modified rdf:datatype="http://www.w3.org/2001/XMLSchema#date">2024-10-18</dcterms:modified>
	<dcterms:identifier>17495</dcterms:identifier>
	<dcterms:contributor>blandine.nouvel</dcterms:contributor>
	<dcterms:contributor>justine.vincent</dcterms:contributor>
	<skos:definition xml:lang="en">More or less viscous liquid, based on a natural or synthetic resin, in solution or dispersion, in a vegetable or mineral essence. (from wikipedia)</skos:definition>
	<skos:definition xml:lang="fr">Liquide plus ou moins visqueux, à base d'une résine naturelle ou synthétique, en solution ou dispersion, dans une essence végétale ou minérale. (d'après wikipedia)</skos:definition>
	<skos:historyNote xml:lang="fr">2024-17-10 : Modification de la définition.</skos:historyNote>
</rdf:Description>

<rdf:Description rdf:about="https://ark.frantiq.fr/ark:/26678/pcrt065IhLltVk">
	<rdf:type rdf:resource="http://www.w3.org/2004/02/skos/core#Concept"/>
	<skos:prefLabel xml:lang="es">barniz negro</skos:prefLabel>
	<skos:prefLabel xml:lang="en">black glaze</skos:prefLabel>
	<skos:prefLabel xml:lang="de">schwarzgefirniste Keramik</skos:prefLabel>
	<skos:prefLabel xml:lang="it">vernice nera</skos:prefLabel>
	<skos:prefLabel xml:lang="fr">vernis noir</skos:prefLabel>
	<skos:prefLabel xml:lang="nl">zwarte vernis</skos:prefLabel>
	<skos:prefLabel xml:lang="ar">برنيق أسود</skos:prefLabel>
	<skos:related rdf:resource="https://ark.frantiq.fr/ark:/26678/pcrtnR5ePytFhO"/>
	<skos:broader rdf:resource="https://ark.frantiq.fr/ark:/26678/pcrttS4bFv2ezb"/>
	<skos:inScheme rdf:resource="https://ark.frantiq.fr/ark:/26678/TH_1"/>
	<opentheso:memberOf rdf:resource="https://ark.frantiq.fr/ark:/26678/pcrtv66rn9cbv1"/>
	<opentheso:memberOf rdf:resource="https://ark.frantiq.fr/ark:/26678/pcrtnbDLi2FkAj"/>
	<dcterms:created rdf:datatype="http://www.w3.org/2001/XMLSchema#date">2007-02-08</dcterms:created>
	<dcterms:modified rdf:datatype="http://www.w3.org/2001/XMLSchema#date">2023-08-02</dcterms:modified>
	<dcterms:identifier>17496</dcterms:identifier>
	<dcterms:contributor>blandine.nouvel</dcterms:contributor>
</rdf:Description>

<rdf:Description rdf:about="https://ark.frantiq.fr/ark:/26678/pcrtJXS9PmPlFX">
	<rdf:type rdf:resource="http://www.w3.org/2004/02/skos/core#Concept"/>
	<skos:prefLabel xml:lang="es">barniz rojo</skos:prefLabel>
	<skos:prefLabel xml:lang="en">red glaze</skos:prefLabel>
	<skos:prefLabel xml:lang="nl">rode vernis</skos:prefLabel>
	<skos:prefLabel xml:lang="de">rotgefirniste Keramik</skos:prefLabel>
	<skos:prefLabel xml:lang="it">vernice rossa</skos:prefLabel>
	<skos:prefLabel xml:lang="fr">vernis rouge</skos:prefLabel>
	<skos:prefLabel xml:lang="ar">برنيق أحمر</skos:prefLabel>
	<skos:related rdf:resource="https://ark.frantiq.fr/ark:/26678/pcrtnR5ePytFhO"/>
	<skos:broader rdf:resource="https://ark.frantiq.fr/ark:/26678/pcrttS4bFv2ezb"/>
	<skos:inScheme rdf:resource="https://ark.frantiq.fr/ark:/26678/TH_1"/>
	<opentheso:memberOf rdf:resource="https://ark.frantiq.fr/ark:/26678/pcrtv66rn9cbv1"/>
	<opentheso:memberOf rdf:resource="https://ark.frantiq.fr/ark:/26678/pcrtnbDLi2FkAj"/>
	<skos:relatedMatch rdf:resource="https://ark.mom.fr/ark:/39676/bibfdb4bqwdf6"/>
	<dcterms:created rdf:datatype="http://www.w3.org/2001/XMLSchema#date">2007-02-08</dcterms:created>
	<dcterms:modified rdf:datatype="http://www.w3.org/2001/XMLSchema#date">2023-08-02</dcterms:modified>
	<dcterms:identifier>17497</dcterms:identifier>
	<dcterms:contributor>blandine.nouvel</dcterms:contributor>
</rdf:Description>

<rdf:Description rdf:about="https://ark.frantiq.fr/ark:/26678/pcrt4GqimUgoOq">
	<rdf:type rdf:resource="http://www.w3.org/2004/02/skos/core#Concept"/>
	<skos:prefLabel xml:lang="nl">glas</skos:prefLabel>
	<skos:prefLabel xml:lang="de">Glas</skos:prefLabel>
	<skos:prefLabel xml:lang="en">glass</skos:prefLabel>
	<skos:prefLabel xml:lang="fr">verre</skos:prefLabel>
	<skos:prefLabel xml:lang="it">vetro</skos:prefLabel>
	<skos:prefLabel xml:lang="es">vidrio</skos:prefLabel>
	<skos:prefLabel xml:lang="ar">زُجاج</skos:prefLabel>
	<skos:related rdf:resource="https://ark.frantiq.fr/ark:/26678/pcrtHX75pcAif1"/>
	<skos:related rdf:resource="https://ark.frantiq.fr/ark:/26678/pcrtYW2UjztJmF"/>
	<skos:related rdf:resource="https://ark.frantiq.fr/ark:/26678/pcrt125sJ3jsbN"/>
	<skos:related rdf:resource="https://ark.frantiq.fr/ark:/26678/pcrtpYS4ijo0m2"/>
	<skos:related rdf:resource="https://ark.frantiq.fr/ark:/26678/crtWAS0j7kGTX"/>
	<skos:broader rdf:resource="https://ark.frantiq.fr/ark:/26678/pcrtIMsuG0RWTs"/>
	<skos:inScheme rdf:resource="https://ark.frantiq.fr/ark:/26678/TH_1"/>
	<opentheso:memberOf rdf:resource="https://ark.frantiq.fr/ark:/26678/pcrtv66rn9cbv1"/>
	<opentheso:memberOf rdf:resource="https://ark.frantiq.fr/ark:/26678/pcrtnbDLi2FkAj"/>
	<opentheso:memberOf rdf:resource="https://ark.frantiq.fr/ark:/26678/pcrtv0jq332vcq3gxt5m13d5"/>
	<skos:exactMatch rdf:resource="https://catalogue.bnf.fr/ark:/12148/cb119383603"/>
	<skos:exactMatch rdf:resource="https://www.wikidata.org/wiki/Q11469"/>
	<skos:exactMatch rdf:resource="http://vocab.getty.edu/aat/300010797"/>
	<dcterms:created rdf:datatype="http://www.w3.org/2001/XMLSchema#date">2007-02-08</dcterms:created>
	<dcterms:modified rdf:datatype="http://www.w3.org/2001/XMLSchema#date">2024-03-21</dcterms:modified>
	<dcterms:identifier>17499</dcterms:identifier>
	<dcterms:contributor>blandine.nouvel</dcterms:contributor>
	<dcterms:contributor>irene.weis</dcterms:contributor>
	<skos:definition xml:lang="en">A hard, brittle and transparent material based on silicon dioxide and fluxes.</skos:definition>
	<skos:definition xml:lang="fr">Matériau dur, fragile (cassant) et transparent, à base de dioxyde de silicium et de fondants. (wp)</skos:definition>
	<skos:scopeNote xml:lang="fr">Utiliser ce terme uniquement pour désigner le matériau, pour les processus de production, privilégier  technologie du verre  ; pour la fabrication du verre, privilégier  verrerie  ; pour le lieu de fabrication, privilégier  atelier de verrier , enfin pour les objets, privilégier le concept  objet en verre  et ses spécifiques.</skos:scopeNote>
</rdf:Description>

<rdf:Description rdf:about="https://ark.frantiq.fr/ark:/26678/pcrtOPqdpwj043">
	<rdf:type rdf:resource="http://www.w3.org/2004/02/skos/core#Concept"/>
	<skos:prefLabel xml:lang="es">carne</skos:prefLabel>
	<skos:prefLabel xml:lang="it">carne</skos:prefLabel>
	<skos:prefLabel xml:lang="de">Fleisch</skos:prefLabel>
	<skos:prefLabel xml:lang="en">meat</skos:prefLabel>
	<skos:prefLabel xml:lang="fr">viande</skos:prefLabel>
	<skos:prefLabel xml:lang="nl">vlees</skos:prefLabel>
	<skos:prefLabel xml:lang="ar">لحم</skos:prefLabel>
	<skos:related rdf:resource="https://ark.frantiq.fr/ark:/26678/pcrttrkqkmfrsq"/>
	<skos:related rdf:resource="https://ark.frantiq.fr/ark:/26678/pcrt8c697b0nfq57nqxb6k5h"/>
	<skos:broader rdf:resource="https://ark.frantiq.fr/ark:/26678/pcrtgcn5U8laUN"/>
	<skos:inScheme rdf:resource="https://ark.frantiq.fr/ark:/26678/TH_1"/>
	<opentheso:memberOf rdf:resource="https://ark.frantiq.fr/ark:/26678/pcrtv66rn9cbv1"/>
	<opentheso:memberOf rdf:resource="https://ark.frantiq.fr/ark:/26678/pcrtnbDLi2FkAj"/>
	<skos:exactMatch rdf:resource="https://www.wikidata.org/wiki/Q10990"/>
	<skos:exactMatch rdf:resource="http://vocab.getty.edu/aat/300389813"/>
	<dcterms:created rdf:datatype="http://www.w3.org/2001/XMLSchema#date">2007-02-08</dcterms:created>
	<dcterms:modified rdf:datatype="http://www.w3.org/2001/XMLSchema#date">2024-03-20</dcterms:modified>
	<dcterms:identifier>17510</dcterms:identifier>
	<dcterms:contributor>blandine.nouvel</dcterms:contributor>
	<dcterms:contributor>justine.vincent</dcterms:contributor>
	<skos:definition xml:lang="en">Animal flesh used as food.</skos:definition>
	<skos:definition xml:lang="fr">Chair animale utilisée comme nourriture.</skos:definition>
</rdf:Description>

<rdf:Description rdf:about="https://ark.frantiq.fr/ark:/26678/pcrt3mTg9h3RFE">
	<rdf:type rdf:resource="http://www.w3.org/2004/02/skos/core#Concept"/>
	<skos:prefLabel xml:lang="fr">vin</skos:prefLabel>
	<skos:prefLabel xml:lang="es">vino</skos:prefLabel>
	<skos:prefLabel xml:lang="it">vino</skos:prefLabel>
	<skos:prefLabel xml:lang="de">Wein</skos:prefLabel>
	<skos:prefLabel xml:lang="nl">wijn</skos:prefLabel>
	<skos:prefLabel xml:lang="en">wine</skos:prefLabel>
	<skos:prefLabel xml:lang="ar">نبيذ</skos:prefLabel>
	<skos:altLabel xml:lang="ar">خَمْر</skos:altLabel>
	<skos:related rdf:resource="https://ark.frantiq.fr/ark:/26678/pcrtihlJWfvH4v"/>
	<skos:related rdf:resource="https://ark.frantiq.fr/ark:/26678/pcrtKpR47IIaTn"/>
	<skos:related rdf:resource="https://ark.frantiq.fr/ark:/26678/pcrtDrDBcuUmry"/>
	<skos:related rdf:resource="https://ark.frantiq.fr/ark:/26678/pcrtuSFhuyLuyh"/>
	<skos:related rdf:resource="https://ark.frantiq.fr/ark:/26678/pcrtbhbct8gbhn"/>
	<skos:broader rdf:resource="https://ark.frantiq.fr/ark:/26678/pcrt6z097U6IUf"/>
	<skos:inScheme rdf:resource="https://ark.frantiq.fr/ark:/26678/TH_1"/>
	<opentheso:memberOf rdf:resource="https://ark.frantiq.fr/ark:/26678/pcrtv66rn9cbv1"/>
	<opentheso:memberOf rdf:resource="https://ark.frantiq.fr/ark:/26678/pcrtnbDLi2FkAj"/>
	<skos:exactMatch rdf:resource="https://catalogue.bnf.fr/ark:/12148/cb11933798p"/>
	<skos:exactMatch rdf:resource="https://www.wikidata.org/wiki/Q282"/>
	<skos:exactMatch rdf:resource="http://vocab.getty.edu/aat/300379442"/>
	<dcterms:created rdf:datatype="http://www.w3.org/2001/XMLSchema#date">2007-02-08</dcterms:created>
	<dcterms:modified rdf:datatype="http://www.w3.org/2001/XMLSchema#date">2023-08-02</dcterms:modified>
	<dcterms:identifier>17543</dcterms:identifier>
	<dcterms:contributor>blandine.nouvel</dcterms:contributor>
	<skos:definition xml:lang="en">Alcoholic beverage produced by fermenting grapes.</skos:definition>
	<skos:definition xml:lang="fr">Boisson alcoolisée obtenue par la fermentation du raisin.</skos:definition>
</rdf:Description>

<rdf:Description rdf:about="https://ark.frantiq.fr/ark:/26678/pcrtAhu8O29Xb2">
	<rdf:type rdf:resource="http://www.w3.org/2004/02/skos/core#Concept"/>
	<skos:prefLabel xml:lang="en">zinc</skos:prefLabel>
	<skos:prefLabel xml:lang="es">zinc</skos:prefLabel>
	<skos:prefLabel xml:lang="fr">zinc</skos:prefLabel>
	<skos:prefLabel xml:lang="it">zinco</skos:prefLabel>
	<skos:prefLabel xml:lang="nl">zink</skos:prefLabel>
	<skos:prefLabel xml:lang="de">Zink</skos:prefLabel>
	<skos:prefLabel xml:lang="ar">خارصين</skos:prefLabel>
	<skos:altLabel xml:lang="ar">توتياء</skos:altLabel>
	<skos:broader rdf:resource="https://ark.frantiq.fr/ark:/26678/pcrtkn1hAXHveS"/>
	<skos:inScheme rdf:resource="https://ark.frantiq.fr/ark:/26678/TH_1"/>
	<opentheso:memberOf rdf:resource="https://ark.frantiq.fr/ark:/26678/pcrtv66rn9cbv1"/>
	<opentheso:memberOf rdf:resource="https://ark.frantiq.fr/ark:/26678/pcrtnbDLi2FkAj"/>
	<opentheso:memberOf rdf:resource="https://ark.frantiq.fr/ark:/26678/pcrtv0jq332vcq3gxt5m13d5"/>
	<skos:exactMatch rdf:resource="https://catalogue.bnf.fr/ark:/12148/cb119731249"/>
	<skos:exactMatch rdf:resource="https://www.wikidata.org/wiki/Q758"/>
	<skos:exactMatch rdf:resource="http://vocab.getty.edu/aat/300011037"/>
	<dcterms:created rdf:datatype="http://www.w3.org/2001/XMLSchema#date">2007-02-08</dcterms:created>
	<dcterms:modified rdf:datatype="http://www.w3.org/2001/XMLSchema#date">2024-12-04</dcterms:modified>
	<dcterms:identifier>17591</dcterms:identifier>
	<dcterms:contributor>blandine.nouvel</dcterms:contributor>
	<dcterms:contributor>irene.weis</dcterms:contributor>
	<dcterms:contributor>justine.vincent</dcterms:contributor>
	<skos:definition xml:lang="en">Shiny, bluish-white, ductile and malleable metal.</skos:definition>
	<skos:definition xml:lang="fr">Métal brillant, d'un blanc bleuâtre, ductile et malléable.</skos:definition>
	<skos:historyNote xml:lang="fr">2024-04-12 : modification de la définition.</skos:historyNote>
</rdf:Description>

<rdf:Description rdf:about="https://ark.frantiq.fr/ark:/26678/pcrtAHm0qJl9tq">
	<rdf:type rdf:resource="http://www.w3.org/2004/02/skos/core#Concept"/>
	<skos:prefLabel xml:lang="nl">eclogiet</skos:prefLabel>
	<skos:prefLabel xml:lang="es">eclogita</skos:prefLabel>
	<skos:prefLabel xml:lang="en">eclogite</skos:prefLabel>
	<skos:prefLabel xml:lang="it">eclogite</skos:prefLabel>
	<skos:prefLabel xml:lang="fr">éclogite</skos:prefLabel>
	<skos:prefLabel xml:lang="de">Eklogit</skos:prefLabel>
	<skos:prefLabel xml:lang="ar">إكلوجيت</skos:prefLabel>
	<skos:broader rdf:resource="https://ark.frantiq.fr/ark:/26678/pcrtxybfLE1dkn"/>
	<skos:inScheme rdf:resource="https://ark.frantiq.fr/ark:/26678/TH_1"/>
	<opentheso:memberOf rdf:resource="https://ark.frantiq.fr/ark:/26678/pcrtv66rn9cbv1"/>
	<opentheso:memberOf rdf:resource="https://ark.frantiq.fr/ark:/26678/pcrtnbDLi2FkAj"/>
	<skos:exactMatch rdf:resource="https://www.wikidata.org/wiki/Q729546"/>
	<skos:exactMatch rdf:resource="http://vocab.getty.edu/aat/300380509"/>
	<dcterms:created rdf:datatype="http://www.w3.org/2001/XMLSchema#date">2007-02-08</dcterms:created>
	<dcterms:modified rdf:datatype="http://www.w3.org/2001/XMLSchema#date">2023-08-02</dcterms:modified>
	<dcterms:identifier>17611</dcterms:identifier>
	<dcterms:contributor>blandine.nouvel</dcterms:contributor>
	<skos:definition xml:lang="en">Metamorphic rock formed in the eclogitic facies, i.e. having undergone the pressure and temperature conditions of this field (wp)</skos:definition>
	<skos:definition xml:lang="ar">صخر عقيقي</skos:definition>
	<skos:definition xml:lang="fr">Roche métamorphique qui s'est formée dans le faciès éclogitique, c'est-à-dire ayant subi les conditions de pression et température de ce champ. (wp)</skos:definition>
</rdf:Description>

<rdf:Description rdf:about="https://ark.frantiq.fr/ark:/26678/pcrt6d15xRmV8x">
	<rdf:type rdf:resource="http://www.w3.org/2004/02/skos/core#Concept"/>
	<skos:prefLabel xml:lang="es">electro</skos:prefLabel>
	<skos:prefLabel xml:lang="en">electrum</skos:prefLabel>
	<skos:prefLabel xml:lang="fr">électrum</skos:prefLabel>
	<skos:prefLabel xml:lang="nl">elektron</skos:prefLabel>
	<skos:prefLabel xml:lang="de">Elektron</skos:prefLabel>
	<skos:prefLabel xml:lang="it">elettro</skos:prefLabel>
	<skos:prefLabel xml:lang="ar">إلكتروم</skos:prefLabel>
	<skos:broader rdf:resource="https://ark.frantiq.fr/ark:/26678/pcrtzcGlM17go5"/>
	<skos:inScheme rdf:resource="https://ark.frantiq.fr/ark:/26678/TH_1"/>
	<opentheso:memberOf rdf:resource="https://ark.frantiq.fr/ark:/26678/pcrtv66rn9cbv1"/>
	<opentheso:memberOf rdf:resource="https://ark.frantiq.fr/ark:/26678/pcrtnbDLi2FkAj"/>
	<skos:exactMatch rdf:resource="https://www.wikidata.org/wiki/Q239481"/>
	<skos:exactMatch rdf:resource="http://vocab.getty.edu/aat/300010965"/>
	<dcterms:created rdf:datatype="http://www.w3.org/2001/XMLSchema#date">2007-02-08</dcterms:created>
	<dcterms:modified rdf:datatype="http://www.w3.org/2001/XMLSchema#date">2023-08-02</dcterms:modified>
	<dcterms:identifier>17651</dcterms:identifier>
	<dcterms:contributor>blandine.nouvel</dcterms:contributor>
	<skos:definition xml:lang="en">Natural gold and silver alloy (Lar.)</skos:definition>
	<skos:definition xml:lang="fr">Alliage naturel d'or et d'argent (Lar.)</skos:definition>
	<skos:definition xml:lang="ar">خليط ذهب و فضة</skos:definition>
</rdf:Description>

<rdf:Description rdf:about="https://ark.frantiq.fr/ark:/26678/pcrtmbhTSRIoYb">
	<rdf:type rdf:resource="http://www.w3.org/2004/02/skos/core#Concept"/>
	<skos:prefLabel xml:lang="en">emerald</skos:prefLabel>
	<skos:prefLabel xml:lang="fr">émeraude</skos:prefLabel>
	<skos:prefLabel xml:lang="es">esmeralda</skos:prefLabel>
	<skos:prefLabel xml:lang="nl">smaragd</skos:prefLabel>
	<skos:prefLabel xml:lang="de">Smaragd</skos:prefLabel>
	<skos:prefLabel xml:lang="it">smeraldo</skos:prefLabel>
	<skos:prefLabel xml:lang="ar">زُمُرّد</skos:prefLabel>
	<skos:broader rdf:resource="https://ark.frantiq.fr/ark:/26678/pcrtzVuPZeWdAP"/>
	<skos:inScheme rdf:resource="https://ark.frantiq.fr/ark:/26678/TH_1"/>
	<opentheso:memberOf rdf:resource="https://ark.frantiq.fr/ark:/26678/pcrtv66rn9cbv1"/>
	<opentheso:memberOf rdf:resource="https://ark.frantiq.fr/ark:/26678/pcrtnbDLi2FkAj"/>
	<skos:exactMatch rdf:resource="https://www.wikidata.org/wiki/Q43513"/>
	<skos:exactMatch rdf:resource="http://vocab.getty.edu/aat/300011074"/>
	<dcterms:created rdf:datatype="http://www.w3.org/2001/XMLSchema#date">2007-02-08</dcterms:created>
	<dcterms:modified rdf:datatype="http://www.w3.org/2001/XMLSchema#date">2023-08-02</dcterms:modified>
	<dcterms:identifier>17670</dcterms:identifier>
	<dcterms:contributor>blandine.nouvel</dcterms:contributor>
	<skos:definition xml:lang="en">Precious stone, transparent and generally of an intense green colour, constituting one of the varieties of beryl (TLFi)</skos:definition>
	<skos:definition xml:lang="fr">Pierre précieuse, transparente et généralement d'un vert intense, constituant une des variétés du béryl. (TLFi)</skos:definition>
</rdf:Description>

<rdf:Description rdf:about="https://ark.frantiq.fr/ark:/26678/pcrt0TJJTrHkN1">
	<rdf:type rdf:resource="http://www.w3.org/2004/02/skos/core#Concept"/>
	<skos:prefLabel xml:lang="fr">épice</skos:prefLabel>
	<skos:prefLabel xml:lang="es">especia</skos:prefLabel>
	<skos:prefLabel xml:lang="de">Gewürze</skos:prefLabel>
	<skos:prefLabel xml:lang="nl">kruiden</skos:prefLabel>
	<skos:prefLabel xml:lang="it">spezia</skos:prefLabel>
	<skos:prefLabel xml:lang="en">spice</skos:prefLabel>
	<skos:prefLabel xml:lang="ar">توابل</skos:prefLabel>
	<skos:related rdf:resource="https://ark.frantiq.fr/ark:/26678/pcrtbSfKuoqH7L"/>
	<skos:related rdf:resource="https://ark.frantiq.fr/ark:/26678/pcrtUTZqItd8SL"/>
	<skos:related rdf:resource="https://ark.frantiq.fr/ark:/26678/pcrtGzQPnntJa1"/>
	<skos:related rdf:resource="https://ark.frantiq.fr/ark:/26678/pcrtOOWRS56wSD"/>
	<skos:related rdf:resource="https://ark.frantiq.fr/ark:/26678/pcrtEYqI4kLNb3"/>
	<skos:narrower rdf:resource="https://ark.frantiq.fr/ark:/26678/crtHmI38AHBYS"/>
	<skos:narrower rdf:resource="https://ark.frantiq.fr/ark:/26678/crtXiS7pEzMh1"/>
	<skos:broader rdf:resource="https://ark.frantiq.fr/ark:/26678/pcrtnHxyjOkhJw"/>
	<skos:inScheme rdf:resource="https://ark.frantiq.fr/ark:/26678/TH_1"/>
	<opentheso:memberOf rdf:resource="https://ark.frantiq.fr/ark:/26678/pcrtv66rn9cbv1"/>
	<opentheso:memberOf rdf:resource="https://ark.frantiq.fr/ark:/26678/pcrtnbDLi2FkAj"/>
	<skos:exactMatch rdf:resource="https://catalogue.bnf.fr/ark:/12148/cb11936422b"/>
	<skos:exactMatch rdf:resource="https://www.wikidata.org/wiki/Q42527"/>
	<skos:exactMatch rdf:resource="http://vocab.getty.edu/aat/300386730"/>
	<dcterms:created rdf:datatype="http://www.w3.org/2001/XMLSchema#date">2007-02-08</dcterms:created>
	<dcterms:modified rdf:datatype="http://www.w3.org/2001/XMLSchema#date">2024-11-15</dcterms:modified>
	<dcterms:identifier>17682</dcterms:identifier>
	<dcterms:contributor>blandine.nouvel</dcterms:contributor>
	<dcterms:contributor>justine.vincent</dcterms:contributor>
	<skos:definition xml:lang="fr">Matière organique d'origine végétale odorante ou piquante utilisée en petite quantité en cuisine, comme conservateur, assaisonnement ou colorant, mais aussi en médecine, en teinturerie ou en distillerie. (Wikipedia)</skos:definition>
	<skos:definition xml:lang="en">A fragrant or pungent organic plant material used in small quantities in cooking as a preservative, seasoning or colouring agent, but also in medicine, dyeing and distilling (Wikipedia).</skos:definition>
</rdf:Description>

<rdf:Description rdf:about="https://ark.frantiq.fr/ark:/26678/pcrtGpmPNJ0jRl">
	<rdf:type rdf:resource="http://www.w3.org/2004/02/skos/core#Concept"/>
	<skos:prefLabel xml:lang="es">estaño</skos:prefLabel>
	<skos:prefLabel xml:lang="fr">étain</skos:prefLabel>
	<skos:prefLabel xml:lang="it">stagno (metallo)</skos:prefLabel>
	<skos:prefLabel xml:lang="en">tin</skos:prefLabel>
	<skos:prefLabel xml:lang="nl">tin</skos:prefLabel>
	<skos:prefLabel xml:lang="de">Zinn</skos:prefLabel>
	<skos:prefLabel xml:lang="ar">قصدير</skos:prefLabel>
	<skos:altLabel xml:lang="it">peltro</skos:altLabel>
	<skos:related rdf:resource="https://ark.frantiq.fr/ark:/26678/pcrtnK3n5OO1RS"/>
	<skos:related rdf:resource="https://ark.frantiq.fr/ark:/26678/pcrtw6rkx2z9fhj1c2dz077r"/>
	<skos:broader rdf:resource="https://ark.frantiq.fr/ark:/26678/pcrtkn1hAXHveS"/>
	<skos:inScheme rdf:resource="https://ark.frantiq.fr/ark:/26678/TH_1"/>
	<opentheso:memberOf rdf:resource="https://ark.frantiq.fr/ark:/26678/pcrtv66rn9cbv1"/>
	<opentheso:memberOf rdf:resource="https://ark.frantiq.fr/ark:/26678/pcrtnbDLi2FkAj"/>
	<opentheso:memberOf rdf:resource="https://ark.frantiq.fr/ark:/26678/pcrtv0jq332vcq3gxt5m13d5"/>
	<skos:exactMatch rdf:resource="https://catalogue.bnf.fr/ark:/12148/cb11952265h"/>
	<skos:exactMatch rdf:resource="https://www.wikidata.org/wiki/Q1096"/>
	<skos:exactMatch rdf:resource="http://vocab.getty.edu/aat/300133748"/>
	<dcterms:created rdf:datatype="http://www.w3.org/2001/XMLSchema#date">2007-02-08</dcterms:created>
	<dcterms:modified rdf:datatype="http://www.w3.org/2001/XMLSchema#date">2024-03-21</dcterms:modified>
	<dcterms:identifier>17710</dcterms:identifier>
	<dcterms:contributor>blandine.nouvel</dcterms:contributor>
	<dcterms:contributor>irene.weis</dcterms:contributor>
	<skos:definition xml:lang="en">Silver-white metal, harder and less dense than lead (Chemical element, symbol Sn, atomic number 50, atomic mass 118.710.) (Lar.)</skos:definition>
	<skos:definition xml:lang="fr">Métal d'un blanc d'argent, plus dur et moins dense que le plomb. (Élément chimique de symbole Sn, de numéro atomique 50, de masse atomique 118,710.) (Lar.)</skos:definition>
</rdf:Description>

<rdf:Description rdf:about="https://ark.frantiq.fr/ark:/26678/crtL2Kjt70xql">
	<rdf:type rdf:resource="http://www.w3.org/2004/02/skos/core#Concept"/>
	<skos:prefLabel xml:lang="nl">varisciet</skos:prefLabel>
	<skos:prefLabel xml:lang="de">Variscit</skos:prefLabel>
	<skos:prefLabel xml:lang="es">variscita</skos:prefLabel>
	<skos:prefLabel xml:lang="fr">variscite</skos:prefLabel>
	<skos:prefLabel xml:lang="it">variscite</skos:prefLabel>
	<skos:prefLabel xml:lang="en">Variscite</skos:prefLabel>
	<skos:altLabel xml:lang="de">Variszit</skos:altLabel>
	<skos:related rdf:resource="https://ark.frantiq.fr/ark:/26678/pcrtaJLEkei5LQ"/>
	<skos:broader rdf:resource="https://ark.frantiq.fr/ark:/26678/pcrt2nbSAPPSwB"/>
	<skos:inScheme rdf:resource="https://ark.frantiq.fr/ark:/26678/TH_1"/>
	<opentheso:memberOf rdf:resource="https://ark.frantiq.fr/ark:/26678/pcrtv66rn9cbv1"/>
	<opentheso:memberOf rdf:resource="https://ark.frantiq.fr/ark:/26678/pcrtnbDLi2FkAj"/>
	<skos:exactMatch rdf:resource="https://www.wikidata.org/wiki/Q415544"/>
	<skos:exactMatch rdf:resource="http://vocab.getty.edu/aat/300386476"/>
	<dcterms:created rdf:datatype="http://www.w3.org/2001/XMLSchema#date">2018-06-30</dcterms:created>
	<dcterms:modified rdf:datatype="http://www.w3.org/2001/XMLSchema#date">2024-11-18</dcterms:modified>
	<dcterms:identifier>177759</dcterms:identifier>
	<dcterms:contributor>blandine.nouvel</dcterms:contributor>
	<dcterms:contributor>justine.vincent</dcterms:contributor>
	<skos:definition xml:lang="en">Mineral species formed from aluminium phosphate.</skos:definition>
	<skos:definition xml:lang="fr">Espèce minérale formée de phosphate d'aluminium.</skos:definition>
</rdf:Description>

<rdf:Description rdf:about="https://ark.frantiq.fr/ark:/26678/crtXiS7pEzMh1">
	<rdf:type rdf:resource="http://www.w3.org/2004/02/skos/core#Concept"/>
	<skos:prefLabel xml:lang="it">pepe</skos:prefLabel>
	<skos:prefLabel xml:lang="en">pepper</skos:prefLabel>
	<skos:prefLabel xml:lang="de">Pfeffer</skos:prefLabel>
	<skos:prefLabel xml:lang="es">pimienta</skos:prefLabel>
	<skos:prefLabel xml:lang="fr">poivre</skos:prefLabel>
	<skos:broader rdf:resource="https://ark.frantiq.fr/ark:/26678/pcrt0TJJTrHkN1"/>
	<skos:inScheme rdf:resource="https://ark.frantiq.fr/ark:/26678/TH_1"/>
	<opentheso:memberOf rdf:resource="https://ark.frantiq.fr/ark:/26678/pcrtv66rn9cbv1"/>
	<opentheso:memberOf rdf:resource="https://ark.frantiq.fr/ark:/26678/pcrtnbDLi2FkAj"/>
	<skos:exactMatch rdf:resource="https://www.wikidata.org/wiki/Q43084"/>
	<dcterms:created rdf:datatype="http://www.w3.org/2001/XMLSchema#date">2018-06-30</dcterms:created>
	<dcterms:modified rdf:datatype="http://www.w3.org/2001/XMLSchema#date">2023-08-02</dcterms:modified>
	<dcterms:identifier>177767</dcterms:identifier>
	<dcterms:contributor>blandine.nouvel</dcterms:contributor>
	<skos:definition xml:lang="en">Spice obtained from the berries of various pepper plant species (Wikipedia)</skos:definition>
	<skos:definition xml:lang="fr">Épice obtenue à partir des baies de différentes espèces de poivriers (Wikipedia)</skos:definition>
</rdf:Description>

<rdf:Description rdf:about="https://ark.frantiq.fr/ark:/26678/crtnOhKKcaFEI">
	<rdf:type rdf:resource="http://www.w3.org/2004/02/skos/core#Concept"/>
	<skos:prefLabel xml:lang="nl">aardolie</skos:prefLabel>
	<skos:prefLabel xml:lang="de">Erdöl</skos:prefLabel>
	<skos:prefLabel xml:lang="fr">pétrole</skos:prefLabel>
	<skos:prefLabel xml:lang="es">petróleo</skos:prefLabel>
	<skos:prefLabel xml:lang="en">petroleum</skos:prefLabel>
	<skos:prefLabel xml:lang="it">petrolio</skos:prefLabel>
	<skos:altLabel xml:lang="en">crude oil</skos:altLabel>
	<skos:altLabel xml:lang="it">nafta</skos:altLabel>
	<skos:altLabel xml:lang="fr">naphte</skos:altLabel>
	<skos:altLabel xml:lang="en">oil</skos:altLabel>
	<skos:related rdf:resource="https://ark.frantiq.fr/ark:/26678/pcrtlKNhumKaYq"/>
	<skos:broader rdf:resource="https://ark.frantiq.fr/ark:/26678/pcrtx37ph91cww"/>
	<skos:inScheme rdf:resource="https://ark.frantiq.fr/ark:/26678/TH_1"/>
	<opentheso:memberOf rdf:resource="https://ark.frantiq.fr/ark:/26678/pcrtv66rn9cbv1"/>
	<opentheso:memberOf rdf:resource="https://ark.frantiq.fr/ark:/26678/pcrtnbDLi2FkAj"/>
	<skos:exactMatch rdf:resource="https://catalogue.bnf.fr/ark:/12148/cb11975899m"/>
	<skos:exactMatch rdf:resource="https://www.wikidata.org/wiki/Q22656"/>
	<skos:exactMatch rdf:resource="http://vocab.getty.edu/aat/300013001"/>
	<dcterms:created rdf:datatype="http://www.w3.org/2001/XMLSchema#date">2018-07-02</dcterms:created>
	<dcterms:modified rdf:datatype="http://www.w3.org/2001/XMLSchema#date">2023-08-02</dcterms:modified>
	<dcterms:identifier>177815</dcterms:identifier>
	<dcterms:contributor>blandine.nouvel</dcterms:contributor>
	<skos:definition xml:lang="en">A naturally occurring mineral oil, composed of a multitude of organic compounds, mainly hydrocarbons, trapped in specific geological formations (Wikipedia).</skos:definition>
	<skos:definition xml:lang="fr">Huile minérale d’origine naturelle, composée d'une multitude de composés organiques, essentiellement des hydrocarbures, piégée dans des formations géologiques particulières (Wikipédia).</skos:definition>
</rdf:Description>

<rdf:Description rdf:about="https://ark.frantiq.fr/ark:/26678/crt9EjSUc0WRF">
	<rdf:type rdf:resource="http://www.w3.org/2004/02/skos/core#Concept"/>
	<skos:prefLabel xml:lang="en">chalk</skos:prefLabel>
	<skos:prefLabel xml:lang="it">chalk</skos:prefLabel>
	<skos:prefLabel xml:lang="fr">craie</skos:prefLabel>
	<skos:prefLabel xml:lang="es">creta</skos:prefLabel>
	<skos:prefLabel xml:lang="de">Kreide</skos:prefLabel>
	<skos:prefLabel xml:lang="nl">Krijtgesteente</skos:prefLabel>
	<skos:related rdf:resource="https://ark.frantiq.fr/ark:/26678/pcrt99qxxgtcx1"/>
	<skos:related rdf:resource="https://ark.frantiq.fr/ark:/26678/pcrt4662dsxgjj"/>
	<skos:narrower rdf:resource="https://ark.frantiq.fr/ark:/26678/pcrtHJ3vzShqFy"/>
	<skos:broader rdf:resource="https://ark.frantiq.fr/ark:/26678/pcrtc1Ueky7Zpg"/>
	<skos:inScheme rdf:resource="https://ark.frantiq.fr/ark:/26678/TH_1"/>
	<opentheso:memberOf rdf:resource="https://ark.frantiq.fr/ark:/26678/pcrtv66rn9cbv1"/>
	<opentheso:memberOf rdf:resource="https://ark.frantiq.fr/ark:/26678/pcrtnbDLi2FkAj"/>
	<skos:exactMatch rdf:resource="https://www.wikidata.org/wiki/Q183670"/>
	<skos:exactMatch rdf:resource="http://vocab.getty.edu/aat/300011727"/>
	<dcterms:created rdf:datatype="http://www.w3.org/2001/XMLSchema#date">2018-07-11</dcterms:created>
	<dcterms:modified rdf:datatype="http://www.w3.org/2001/XMLSchema#date">2023-08-02</dcterms:modified>
	<dcterms:identifier>178055</dcterms:identifier>
	<dcterms:contributor>blandine.nouvel</dcterms:contributor>
	<skos:definition xml:lang="fr">Roche sédimentaire calcaire blanche marine contenant presque exclusivement du carbonate de calcium et un peu d'argile. Formée dans des mers chaudes et peu profondes, elle est constituée essentiellement par l'accumulation d'algues planctoniques. Les principales accumulations de craie en Europe datent du Crétacé, période géologique à laquelle la craie a donné son nom (d'ap. Wikipedia)</skos:definition>
</rdf:Description>

<rdf:Description rdf:about="https://ark.frantiq.fr/ark:/26678/crtAzyiJhxOQN">
	<rdf:type rdf:resource="http://www.w3.org/2004/02/skos/core#Concept"/>
	<skos:prefLabel xml:lang="en">bark (botany)</skos:prefLabel>
	<skos:prefLabel xml:lang="it">corteccia</skos:prefLabel>
	<skos:prefLabel xml:lang="es">corteza</skos:prefLabel>
	<skos:prefLabel xml:lang="fr">écorce</skos:prefLabel>
	<skos:prefLabel xml:lang="de">Rinde</skos:prefLabel>
	<skos:related rdf:resource="https://ark.frantiq.fr/ark:/26678/crtpMHzUJBEF2"/>
	<skos:broader rdf:resource="https://ark.frantiq.fr/ark:/26678/pcrtnHxyjOkhJw"/>
	<skos:inScheme rdf:resource="https://ark.frantiq.fr/ark:/26678/TH_1"/>
	<opentheso:memberOf rdf:resource="https://ark.frantiq.fr/ark:/26678/pcrtv66rn9cbv1"/>
	<opentheso:memberOf rdf:resource="https://ark.frantiq.fr/ark:/26678/pcrtnbDLi2FkAj"/>
	<skos:exactMatch rdf:resource="https://catalogue.bnf.fr/ark:/12148/cb11964939k"/>
	<skos:exactMatch rdf:resource="https://fr.wikipedia.org/wiki/Écorce"/>
	<skos:exactMatch rdf:resource="https://www.wikidata.org/wiki/Q184453"/>
	<skos:exactMatch rdf:resource="http://vocab.getty.edu/aat/300011860"/>
	<dcterms:created rdf:datatype="http://www.w3.org/2001/XMLSchema#date">2018-07-18</dcterms:created>
	<dcterms:modified rdf:datatype="http://www.w3.org/2001/XMLSchema#date">2024-11-15</dcterms:modified>
	<dcterms:identifier>178098</dcterms:identifier>
	<dcterms:contributor>blandine.nouvel</dcterms:contributor>
	<dcterms:contributor>justine.vincent</dcterms:contributor>
	<skos:definition xml:lang="en">Outer covering of the trunk, branches and roots of trees, and more generally of woody plants, used as a building material, source of textile fibres or substance for food or therapeutic use. (wp)</skos:definition>
	<skos:definition xml:lang="fr">Revêtement extérieur du tronc, des branches et des racines des arbres, et plus généralement des plantes ligneuses, utilisé comme matériau de construction, source de fibres textile ou &lt;span style= background-color: rgb(255, 255, 255); &gt;substance à usage alimentaire ou thérapeutique .&lt;/span&gt; (wp)</skos:definition>
</rdf:Description>

<rdf:Description rdf:about="https://ark.frantiq.fr/ark:/26678/crtqg6iAF3rS7">
	<rdf:type rdf:resource="http://www.w3.org/2004/02/skos/core#Concept"/>
	<skos:prefLabel xml:lang="en">peat</skos:prefLabel>
	<skos:prefLabel xml:lang="it">torba</skos:prefLabel>
	<skos:prefLabel xml:lang="de">Torf</skos:prefLabel>
	<skos:prefLabel xml:lang="fr">tourbe</skos:prefLabel>
	<skos:prefLabel xml:lang="es">turba</skos:prefLabel>
	<skos:altLabel xml:lang="it">tappeto erboso</skos:altLabel>
	<skos:altLabel xml:lang="en">turf</skos:altLabel>
	<skos:related rdf:resource="https://ark.frantiq.fr/ark:/26678/pcrtzDfVNkD5St"/>
	<skos:broader rdf:resource="https://ark.frantiq.fr/ark:/26678/pcrtwvFLgSQRs5"/>
	<skos:inScheme rdf:resource="https://ark.frantiq.fr/ark:/26678/TH_1"/>
	<opentheso:memberOf rdf:resource="https://ark.frantiq.fr/ark:/26678/pcrtv66rn9cbv1"/>
	<opentheso:memberOf rdf:resource="https://ark.frantiq.fr/ark:/26678/pcrtnbDLi2FkAj"/>
	<skos:exactMatch rdf:resource="https://catalogue.bnf.fr/ark:/12148/cb11952992b"/>
	<skos:exactMatch rdf:resource="https://www.wikidata.org/wiki/Q184624"/>
	<skos:exactMatch rdf:resource="http://vocab.getty.edu/aat/300014340"/>
	<dcterms:created rdf:datatype="http://www.w3.org/2001/XMLSchema#date">2018-08-16</dcterms:created>
	<dcterms:modified rdf:datatype="http://www.w3.org/2001/XMLSchema#date">2024-11-15</dcterms:modified>
	<dcterms:identifier>178305</dcterms:identifier>
	<dcterms:contributor>blandine.nouvel</dcterms:contributor>
	<dcterms:contributor>justine.vincent</dcterms:contributor>
	<skos:definition xml:lang="fr">Matière organique fossile formée par accumulation sur de longues périodes de temps de matière organique morte, essentiellement des végétaux, dans un milieu saturé en eau, formant ainsi le sols des tourbières. (Wikipedia)</skos:definition>
	<skos:definition xml:lang="en">Fossil organic matter formed by the accumulation over long periods of time of dead organic matter, mainly plant material, in a water-saturated environment, thus forming the soil of peat bogs. (Wikipedia)</skos:definition>
</rdf:Description>

<rdf:Description rdf:about="https://ark.frantiq.fr/ark:/26678/crtXXzLndpZbJ">
	<rdf:type rdf:resource="http://www.w3.org/2004/02/skos/core#Concept"/>
	<skos:prefLabel xml:lang="es">aceite de oliva</skos:prefLabel>
	<skos:prefLabel xml:lang="fr">huile d'olive</skos:prefLabel>
	<skos:prefLabel xml:lang="it">olio di oliva</skos:prefLabel>
	<skos:prefLabel xml:lang="de">Olivenöl</skos:prefLabel>
	<skos:prefLabel xml:lang="en">olive oil</skos:prefLabel>
	<skos:related rdf:resource="https://ark.frantiq.fr/ark:/26678/pcrtiaewgLXnZc"/>
	<skos:broader rdf:resource="https://ark.frantiq.fr/ark:/26678/pcrtnHxyjOkhJw"/>
	<skos:inScheme rdf:resource="https://ark.frantiq.fr/ark:/26678/TH_1"/>
	<opentheso:memberOf rdf:resource="https://ark.frantiq.fr/ark:/26678/pcrtv66rn9cbv1"/>
	<opentheso:memberOf rdf:resource="https://ark.frantiq.fr/ark:/26678/pcrtnbDLi2FkAj"/>
	<skos:exactMatch rdf:resource="https://www.wikidata.org/wiki/Q93165"/>
	<skos:exactMatch rdf:resource="http://vocab.getty.edu/aat/300014323"/>
	<dcterms:created rdf:datatype="http://www.w3.org/2001/XMLSchema#date">2018-10-15</dcterms:created>
	<dcterms:modified rdf:datatype="http://www.w3.org/2001/XMLSchema#date">2023-08-02</dcterms:modified>
	<dcterms:identifier>178388</dcterms:identifier>
	<dcterms:contributor>blandine.nouvel</dcterms:contributor>
	<skos:definition xml:lang="en">Fat from olives.</skos:definition>
	<skos:definition xml:lang="fr">Matière grasse issue de l'olive.</skos:definition>
</rdf:Description>

<rdf:Description rdf:about="https://ark.frantiq.fr/ark:/26678/crtiorG06KeFt">
	<rdf:type rdf:resource="http://www.w3.org/2004/02/skos/core#Concept"/>
	<skos:prefLabel xml:lang="es">fibra vegetal</skos:prefLabel>
	<skos:prefLabel xml:lang="it">fibra vegetale</skos:prefLabel>
	<skos:prefLabel xml:lang="fr">fibre végétale</skos:prefLabel>
	<skos:prefLabel xml:lang="de">pflanzliche Faser</skos:prefLabel>
	<skos:prefLabel xml:lang="en">plant fibre</skos:prefLabel>
	<skos:prefLabel xml:lang="ar">ليف نباتي</skos:prefLabel>
	<skos:altLabel xml:lang="de">Pflanzenfaser</skos:altLabel>
	<skos:altLabel xml:lang="en">plant fiber</skos:altLabel>
	<skos:related rdf:resource="https://ark.frantiq.fr/ark:/26678/pcrtNQhoS8U7Ve"/>
	<skos:narrower rdf:resource="https://ark.frantiq.fr/ark:/26678/pcrtgkVy7lK4lN"/>
	<skos:broader rdf:resource="https://ark.frantiq.fr/ark:/26678/pcrtnHxyjOkhJw"/>
	<skos:inScheme rdf:resource="https://ark.frantiq.fr/ark:/26678/TH_1"/>
	<opentheso:memberOf rdf:resource="https://ark.frantiq.fr/ark:/26678/pcrtv66rn9cbv1"/>
	<opentheso:memberOf rdf:resource="https://ark.frantiq.fr/ark:/26678/pcrtnbDLi2FkAj"/>
	<skos:exactMatch rdf:resource="https://catalogue.bnf.fr/ark:/12148/cb12065541v"/>
	<skos:exactMatch rdf:resource="https://www.wikidata.org/wiki/Q20026824"/>
	<skos:exactMatch rdf:resource="http://vocab.getty.edu/aat/300014031"/>
	<dcterms:created rdf:datatype="http://www.w3.org/2001/XMLSchema#date">2018-10-30</dcterms:created>
	<dcterms:modified rdf:datatype="http://www.w3.org/2001/XMLSchema#date">2024-11-15</dcterms:modified>
	<dcterms:identifier>178473</dcterms:identifier>
	<dcterms:contributor>blandine.nouvel</dcterms:contributor>
	<dcterms:contributor>justine.vincent</dcterms:contributor>
	<skos:definition xml:lang="en">Dead, filiform cell expansion, mainly composed of cellulose, hemicelluloses, lignins and pectins, isolated or in a bundle (wikipedia).</skos:definition>
	<skos:definition xml:lang="fr">Expansion cellulaire filiforme et morte, principalement composée de cellulose, d'hémicelluloses, de lignines, et de pectines, isolée ou composant un faisceau. (wikipedia).</skos:definition>
</rdf:Description>

<rdf:Description rdf:about="https://ark.frantiq.fr/ark:/26678/pcrtPEGVkSl8Hk">
	<rdf:type rdf:resource="http://www.w3.org/2004/02/skos/core#Concept"/>
	<skos:prefLabel xml:lang="en">porcelain</skos:prefLabel>
	<skos:prefLabel xml:lang="fr">porcelaine</skos:prefLabel>
	<skos:prefLabel xml:lang="es">porcelana</skos:prefLabel>
	<skos:prefLabel xml:lang="it">porcellana</skos:prefLabel>
	<skos:prefLabel xml:lang="nl">porselein</skos:prefLabel>
	<skos:prefLabel xml:lang="de">Porzellan</skos:prefLabel>
	<skos:prefLabel xml:lang="ar">بورسلان</skos:prefLabel>
	<skos:altLabel xml:lang="en">china</skos:altLabel>
	<skos:altLabel xml:lang="en">fine china</skos:altLabel>
	<skos:related rdf:resource="https://ark.frantiq.fr/ark:/26678/pcrtf7hn86pq11"/>
	<skos:related rdf:resource="https://ark.frantiq.fr/ark:/26678/pcrtSdKu9rjDHO"/>
	<skos:related rdf:resource="https://ark.frantiq.fr/ark:/26678/pcrtzwzrB48Yro"/>
	<skos:related rdf:resource="https://ark.frantiq.fr/ark:/26678/pcrtmw8sq1KL1L"/>
	<skos:broader rdf:resource="https://ark.frantiq.fr/ark:/26678/pcrtfx4s0yvSLj"/>
	<skos:inScheme rdf:resource="https://ark.frantiq.fr/ark:/26678/TH_1"/>
	<opentheso:memberOf rdf:resource="https://ark.frantiq.fr/ark:/26678/pcrtv66rn9cbv1"/>
	<opentheso:memberOf rdf:resource="https://ark.frantiq.fr/ark:/26678/pcrtnbDLi2FkAj"/>
	<skos:closeMatch rdf:resource="https://ark.mom.fr/ark:/39676/bibp721vgd1px"/>
	<skos:exactMatch rdf:resource="https://catalogue.bnf.fr/ark:/12148/cb11957129k"/>
	<skos:exactMatch rdf:resource="https://www.wikidata.org/wiki/Q130693"/>
	<skos:exactMatch rdf:resource="http://vocab.getty.edu/aat/300010662"/>
	<dcterms:created rdf:datatype="http://www.w3.org/2001/XMLSchema#date">2007-02-08</dcterms:created>
	<dcterms:modified rdf:datatype="http://www.w3.org/2001/XMLSchema#date">2023-08-02</dcterms:modified>
	<dcterms:identifier>18202</dcterms:identifier>
	<dcterms:contributor>blandine.nouvel</dcterms:contributor>
	<skos:definition xml:lang="en">White, translucent, hard, sound and impermeable pottery resulting from a high-temperature firing (around 1400°C for hard porcelain) which causes vitrification and is covered with a transparent glaze called a couverte. (Balfet)</skos:definition>
	<skos:definition xml:lang="fr">Poterie blanche, translucide, dure, sonore et imperméable, résultant d’une cuisson à température élevée (environ 1400°C pour les porcelaines dures) provoquant une vitrification et recouverte d’une glaçure transparente appelée couverte. (Balfet)</skos:definition>
</rdf:Description>

<rdf:Description rdf:about="https://ark.frantiq.fr/ark:/26678/pcrtLgpv98vu4P">
	<rdf:type rdf:resource="http://www.w3.org/2004/02/skos/core#Concept"/>
	<skos:prefLabel xml:lang="es">cuarcita</skos:prefLabel>
	<skos:prefLabel xml:lang="nl">kwartsiet</skos:prefLabel>
	<skos:prefLabel xml:lang="en">quartzite</skos:prefLabel>
	<skos:prefLabel xml:lang="fr">quartzite</skos:prefLabel>
	<skos:prefLabel xml:lang="de">Quarzit</skos:prefLabel>
	<skos:prefLabel xml:lang="it">quarzite</skos:prefLabel>
	<skos:prefLabel xml:lang="ar">كوارتزيت</skos:prefLabel>
	<skos:altLabel xml:lang="es">metacuarcita</skos:altLabel>
	<skos:altLabel xml:lang="ar">حُث صوّاني</skos:altLabel>
	<skos:broader rdf:resource="https://ark.frantiq.fr/ark:/26678/pcrt4N9jrETRto"/>
	<skos:inScheme rdf:resource="https://ark.frantiq.fr/ark:/26678/TH_1"/>
	<opentheso:memberOf rdf:resource="https://ark.frantiq.fr/ark:/26678/pcrtv66rn9cbv1"/>
	<opentheso:memberOf rdf:resource="https://ark.frantiq.fr/ark:/26678/pcrtnbDLi2FkAj"/>
	<skos:exactMatch rdf:resource="https://www.wikidata.org/wiki/Q237883"/>
	<skos:exactMatch rdf:resource="http://vocab.getty.edu/aat/300011623"/>
	<dcterms:created rdf:datatype="http://www.w3.org/2001/XMLSchema#date">2007-02-08</dcterms:created>
	<dcterms:modified rdf:datatype="http://www.w3.org/2001/XMLSchema#date">2025-01-17</dcterms:modified>
	<dcterms:identifier>19605</dcterms:identifier>
	<dcterms:contributor>blandine.nouvel</dcterms:contributor>
	<skos:definition xml:lang="en">Siliceous rock of sedimentary or metamorphic origin, compact, with a conchoidal fracture whose fracture plane intersects the grains, consisting of quartz crystals that are often jagged (Fernandes, 2012) and generally light in colour. (Wikipedia).</skos:definition>
	<skos:definition xml:lang="fr">Roche siliceuse d'origine sédimentaire ou métamorphique, compacte, à cassure conchoïdale dont le plan de cassure recoupe les grains, constituée de cristaux de quartz souvent dentelés (Fernandes, 2012) et à la couleur généralement claire. (Wikipedia).</skos:definition>
</rdf:Description>

<rdf:Description rdf:about="https://ark.frantiq.fr/ark:/26678/pcrtPLs10mF9zI">
	<rdf:type rdf:resource="http://www.w3.org/2004/02/skos/core#Concept"/>
	<skos:prefLabel xml:lang="es">terracota blanca</skos:prefLabel>
	<skos:prefLabel xml:lang="it">terracotta bianca</skos:prefLabel>
	<skos:prefLabel xml:lang="fr">terre cuite blanche</skos:prefLabel>
	<skos:prefLabel xml:lang="de">weisse Terrakotta</skos:prefLabel>
	<skos:prefLabel xml:lang="en">white baked clay</skos:prefLabel>
	<skos:prefLabel xml:lang="nl">witte terracotta</skos:prefLabel>
	<skos:prefLabel xml:lang="ar">فخار مشوي أبيض</skos:prefLabel>
	<skos:altLabel xml:lang="fr">terre cuite à pâte blanche</skos:altLabel>
	<skos:altLabel xml:lang="en">white terracotta</skos:altLabel>
	<skos:related rdf:resource="https://ark.frantiq.fr/ark:/26678/pcrtqEWFq9RGda"/>
	<skos:broader rdf:resource="https://ark.frantiq.fr/ark:/26678/pcrtfx4s0yvSLj"/>
	<skos:inScheme rdf:resource="https://ark.frantiq.fr/ark:/26678/TH_1"/>
	<opentheso:memberOf rdf:resource="https://ark.frantiq.fr/ark:/26678/pcrtv66rn9cbv1"/>
	<opentheso:memberOf rdf:resource="https://ark.frantiq.fr/ark:/26678/pcrtnbDLi2FkAj"/>
	<dcterms:created rdf:datatype="http://www.w3.org/2001/XMLSchema#date">2007-02-08</dcterms:created>
	<dcterms:modified rdf:datatype="http://www.w3.org/2001/XMLSchema#date">2024-11-19</dcterms:modified>
	<dcterms:identifier>21366</dcterms:identifier>
	<dcterms:contributor>blandine.nouvel</dcterms:contributor>
	<dcterms:contributor>justine.vincent</dcterms:contributor>
	<skos:note xml:lang="fr">Matériau céramique conçu à base d'argile blanche.</skos:note>
	<skos:note xml:lang="en">Ceramic material made from white clay.</skos:note>
	<skos:historyNote xml:lang="fr">2024-11-19 : ajout d'une définition.</skos:historyNote>
</rdf:Description>

<rdf:Description rdf:about="https://ark.frantiq.fr/ark:/26678/pcrtp45jEJloXR">
	<rdf:type rdf:resource="http://www.w3.org/2004/02/skos/core#Concept"/>
	<skos:prefLabel xml:lang="es">pórfido</skos:prefLabel>
	<skos:prefLabel xml:lang="nl">porfier</skos:prefLabel>
	<skos:prefLabel xml:lang="it">porfirio</skos:prefLabel>
	<skos:prefLabel xml:lang="de">Porphyr</skos:prefLabel>
	<skos:prefLabel xml:lang="fr">porphyre</skos:prefLabel>
	<skos:prefLabel xml:lang="en">porphyry</skos:prefLabel>
	<skos:prefLabel xml:lang="ar">حجر السمّاق</skos:prefLabel>
	<skos:broader rdf:resource="https://ark.frantiq.fr/ark:/26678/pcrtmxvuuXHSTS"/>
	<skos:inScheme rdf:resource="https://ark.frantiq.fr/ark:/26678/TH_1"/>
	<opentheso:memberOf rdf:resource="https://ark.frantiq.fr/ark:/26678/pcrtv66rn9cbv1"/>
	<opentheso:memberOf rdf:resource="https://ark.frantiq.fr/ark:/26678/pcrtnbDLi2FkAj"/>
	<opentheso:memberOf rdf:resource="https://ark.frantiq.fr/ark:/26678/pcrtv0jq332vcq3gxt5m13d5"/>
	<skos:exactMatch rdf:resource="https://catalogue.bnf.fr/ark:/12148/cb12010154v"/>
	<skos:exactMatch rdf:resource="https://www.wikidata.org/wiki/Q337238"/>
	<skos:exactMatch rdf:resource="http://vocab.getty.edu/aat/300011232"/>
	<dcterms:created rdf:datatype="http://www.w3.org/2001/XMLSchema#date">2007-02-08</dcterms:created>
	<dcterms:modified rdf:datatype="http://www.w3.org/2001/XMLSchema#date">2024-11-18</dcterms:modified>
	<dcterms:identifier>21379</dcterms:identifier>
	<dcterms:contributor>blandine.nouvel</dcterms:contributor>
	<dcterms:contributor>irene.weis</dcterms:contributor>
	<dcterms:contributor>justine.vincent</dcterms:contributor>
	<skos:definition xml:lang="en">Formerly used to define a magmatic rock formed of large crystals in a uniform, very fine-grained base; today this term has been abandoned in petrography (Lozet &amp;amp; Mathieu, Dictionnaire de science du sol. Ed. Technique et Documentation Lavoisier)</skos:definition>
	<skos:definition xml:lang="fr">Anciennement, définissait une roche magmatique formée de grands cristaux dans un fond uniforme à grains très fins; aujourd'hui ce terme a été abandonné en pétrographie. (Lozet &amp;amp; Mathieu, Dictionnaire de science du sol. Ed. Technique et Documentation Lavoisier)</skos:definition>
</rdf:Description>

<rdf:Description rdf:about="https://ark.frantiq.fr/ark:/26678/crtG26Pkhb07S">
	<rdf:type rdf:resource="http://www.w3.org/2004/02/skos/core#Concept"/>
	<skos:prefLabel xml:lang="it">ceramica ad impasto micaceo</skos:prefLabel>
	<skos:prefLabel xml:lang="es">cerámica de pasta micácea</skos:prefLabel>
	<skos:prefLabel xml:lang="fr">céramique à pâte micacée</skos:prefLabel>
	<skos:prefLabel xml:lang="de">glimmerhaltige Keramik</skos:prefLabel>
	<skos:prefLabel xml:lang="en">mica ceramic paste</skos:prefLabel>
	<skos:altLabel xml:lang="es">cerámica micácea</skos:altLabel>
	<skos:altLabel xml:lang="it">ceramica micaea</skos:altLabel>
	<skos:altLabel xml:lang="en">mica clay mix</skos:altLabel>
	<skos:altLabel xml:lang="es">pasta micácea</skos:altLabel>
	<skos:broader rdf:resource="https://ark.frantiq.fr/ark:/26678/pcrtho8l95no0j"/>
	<skos:inScheme rdf:resource="https://ark.frantiq.fr/ark:/26678/TH_1"/>
	<opentheso:memberOf rdf:resource="https://ark.frantiq.fr/ark:/26678/pcrtv66rn9cbv1"/>
	<opentheso:memberOf rdf:resource="https://ark.frantiq.fr/ark:/26678/pcrtnbDLi2FkAj"/>
	<skos:narrowMatch rdf:resource="https://ark.mom.fr/ark:/39676/bibstkhnvpzgq"/>
	<skos:relatedMatch rdf:resource="https://ark.mom.fr/ark:/39676/bib01rm5xgb4w"/>
	<dcterms:created rdf:datatype="http://www.w3.org/2001/XMLSchema#date">2018-11-23</dcterms:created>
	<dcterms:modified rdf:datatype="http://www.w3.org/2001/XMLSchema#date">2023-08-02</dcterms:modified>
	<dcterms:identifier>217694</dcterms:identifier>
	<dcterms:contributor>blandine.nouvel</dcterms:contributor>
	<skos:definition xml:lang="en">ceramic containing a coarse, irregular degreaser with micaceous flakes with a silver sheen (Rivet, RAN, 15, 1982, 243-262)</skos:definition>
	<skos:definition xml:lang="fr">céramique contenant un dégraissant gros et irrégulier renfermant des paillettes micacées à reflet argentées (Rivet, RAN, 15, 1982, 243-262)</skos:definition>
</rdf:Description>

<rdf:Description rdf:about="https://ark.frantiq.fr/ark:/26678/pcrtaUOSeoPg5g">
	<rdf:type rdf:resource="http://www.w3.org/2004/02/skos/core#Concept"/>
	<skos:prefLabel xml:lang="it">maiolica</skos:prefLabel>
	<skos:prefLabel xml:lang="en">Maiolica</skos:prefLabel>
	<skos:prefLabel xml:lang="nl">majolica</skos:prefLabel>
	<skos:prefLabel xml:lang="de">Majolika</skos:prefLabel>
	<skos:prefLabel xml:lang="fr">majolique</skos:prefLabel>
	<skos:prefLabel xml:lang="es">mayólica</skos:prefLabel>
	<skos:prefLabel xml:lang="ar">ماجوليكا</skos:prefLabel>
	<skos:altLabel xml:lang="fr">maïolique</skos:altLabel>
	<skos:related rdf:resource="https://ark.frantiq.fr/ark:/26678/pcrtqHWkorsw9D"/>
	<skos:related rdf:resource="https://ark.frantiq.fr/ark:/26678/pcrtxhiROcXtaM"/>
	<skos:broader rdf:resource="https://ark.frantiq.fr/ark:/26678/pcrtfx4s0yvSLj"/>
	<skos:inScheme rdf:resource="https://ark.frantiq.fr/ark:/26678/TH_1"/>
	<opentheso:memberOf rdf:resource="https://ark.frantiq.fr/ark:/26678/pcrtv66rn9cbv1"/>
	<opentheso:memberOf rdf:resource="https://ark.frantiq.fr/ark:/26678/pcrtnbDLi2FkAj"/>
	<skos:exactMatch rdf:resource="https://catalogue.bnf.fr/ark:/12148/cb11936552j"/>
	<skos:exactMatch rdf:resource="https://www.wikidata.org/wiki/Q622753"/>
	<skos:exactMatch rdf:resource="http://vocab.getty.edu/aat/300021170"/>
	<dcterms:created rdf:datatype="http://www.w3.org/2001/XMLSchema#date">2007-02-08</dcterms:created>
	<dcterms:modified rdf:datatype="http://www.w3.org/2001/XMLSchema#date">2023-08-02</dcterms:modified>
	<dcterms:identifier>21859</dcterms:identifier>
	<dcterms:contributor>blandine.nouvel</dcterms:contributor>
	<skos:definition xml:lang="en">Italian earthenware, particularly from the Renaissance period, with a tin or lead glaze borrowed from Spanish potters (TLFi)</skos:definition>
	<skos:definition xml:lang="fr">Faïence italienne, notamment de l'époque de la Renaissance, dont la glaçure stannifère ou plombifère a été empruntée aux potiers espagnols (TLFi)</skos:definition>
</rdf:Description>

<rdf:Description rdf:about="https://ark.frantiq.fr/ark:/26678/pcrtK43haeM3e3">
	<rdf:type rdf:resource="http://www.w3.org/2004/02/skos/core#Concept"/>
	<skos:prefLabel xml:lang="de">bemalte Keramik</skos:prefLabel>
	<skos:prefLabel xml:lang="nl">beschilderd aardewerk</skos:prefLabel>
	<skos:prefLabel xml:lang="it">ceramica dipinta</skos:prefLabel>
	<skos:prefLabel xml:lang="es">cerámica pintada</skos:prefLabel>
	<skos:prefLabel xml:lang="fr">céramique peinte</skos:prefLabel>
	<skos:prefLabel xml:lang="en">painted ware</skos:prefLabel>
	<skos:prefLabel xml:lang="ar">خزف مطلي</skos:prefLabel>
	<skos:related rdf:resource="https://ark.frantiq.fr/ark:/26678/pcrtmZ7gZV6UUA"/>
	<skos:related rdf:resource="https://ark.frantiq.fr/ark:/26678/pcrt6bb2q2sc9k"/>
	<skos:broader rdf:resource="https://ark.frantiq.fr/ark:/26678/pcrtfx4s0yvSLj"/>
	<skos:inScheme rdf:resource="https://ark.frantiq.fr/ark:/26678/TH_1"/>
	<opentheso:memberOf rdf:resource="https://ark.frantiq.fr/ark:/26678/pcrtv66rn9cbv1"/>
	<opentheso:memberOf rdf:resource="https://ark.frantiq.fr/ark:/26678/pcrtnbDLi2FkAj"/>
	<skos:exactMatch rdf:resource="https://ark.mom.fr/ark:/39676/bibfgtwzspn35"/>
	<dcterms:created rdf:datatype="http://www.w3.org/2001/XMLSchema#date">2007-02-08</dcterms:created>
	<dcterms:modified rdf:datatype="http://www.w3.org/2001/XMLSchema#date">2024-11-19</dcterms:modified>
	<dcterms:identifier>21880</dcterms:identifier>
	<dcterms:contributor>blandine.nouvel</dcterms:contributor>
	<dcterms:contributor>justine.vincent</dcterms:contributor>
	<skos:definition xml:lang="fr">Céramique décorée avec des peintures adaptées.</skos:definition>
	<skos:definition xml:lang="en">Ceramics decorated with appropriate paints.</skos:definition>
	<skos:historyNote xml:lang="fr">2024-11-19 : ajout d'une définition.</skos:historyNote>
</rdf:Description>

<rdf:Description rdf:about="https://ark.frantiq.fr/ark:/26678/pcrty2mcsksa6s">
	<rdf:type rdf:resource="http://www.w3.org/2004/02/skos/core#Concept"/>
	<skos:prefLabel xml:lang="nl">mineraal</skos:prefLabel>
	<skos:prefLabel xml:lang="en">mineral</skos:prefLabel>
	<skos:prefLabel xml:lang="es">mineral</skos:prefLabel>
	<skos:prefLabel xml:lang="de">Mineral</skos:prefLabel>
	<skos:prefLabel xml:lang="fr">minéral</skos:prefLabel>
	<skos:prefLabel xml:lang="it">minerale</skos:prefLabel>
	<skos:prefLabel xml:lang="ar">معدن</skos:prefLabel>
	<skos:related rdf:resource="https://ark.frantiq.fr/ark:/26678/pcrtulsoB7pgV7"/>
	<skos:related rdf:resource="https://ark.frantiq.fr/ark:/26678/pcrt5bIL1UtwcT"/>
	<skos:related rdf:resource="https://ark.frantiq.fr/ark:/26678/pcrtvKH7mF2Oas"/>
	<skos:narrower rdf:resource="https://ark.frantiq.fr/ark:/26678/pcrt5mFxzmQ9rX"/>
	<skos:narrower rdf:resource="https://ark.frantiq.fr/ark:/26678/pcrtDISmiAdvys"/>
	<skos:narrower rdf:resource="https://ark.frantiq.fr/ark:/26678/pcrtuFMPNUEKWb"/>
	<skos:narrower rdf:resource="https://ark.frantiq.fr/ark:/26678/pcrtyx3UIr91zi"/>
	<skos:narrower rdf:resource="https://ark.frantiq.fr/ark:/26678/pcrtDwe0cp16nl"/>
	<skos:narrower rdf:resource="https://ark.frantiq.fr/ark:/26678/pcrt2nbSAPPSwB"/>
	<skos:narrower rdf:resource="https://ark.frantiq.fr/ark:/26678/pcrtF8Wf7AekK2"/>
	<skos:narrower rdf:resource="https://ark.frantiq.fr/ark:/26678/pcrt38v8df6d4c"/>
	<skos:narrower rdf:resource="https://ark.frantiq.fr/ark:/26678/pcrtv4jtvchmgm"/>
	<skos:narrower rdf:resource="https://ark.frantiq.fr/ark:/26678/pcrtqnzx9qwkt5"/>
	<skos:narrower rdf:resource="https://ark.frantiq.fr/ark:/26678/pcrtfpt7p2xkdf"/>
	<skos:narrower rdf:resource="https://ark.frantiq.fr/ark:/26678/pcrt01dd8jnk9r"/>
	<skos:narrower rdf:resource="https://ark.frantiq.fr/ark:/26678/pcrtbrv3wp92hn"/>
	<skos:narrower rdf:resource="https://ark.frantiq.fr/ark:/26678/pcrtpp27tm32r2"/>
	<skos:narrower rdf:resource="https://ark.frantiq.fr/ark:/26678/pcrttr8kcz7mgd"/>
	<skos:narrower rdf:resource="https://ark.frantiq.fr/ark:/26678/pcrtjrbdhj75z0"/>
	<skos:narrower rdf:resource="https://ark.frantiq.fr/ark:/26678/pcrtcb7qm82cts"/>
	<skos:narrower rdf:resource="https://ark.frantiq.fr/ark:/26678/pcrtt9jqbj1ghk"/>
	<skos:narrower rdf:resource="https://ark.frantiq.fr/ark:/26678/pcrtOF9oqZo0Pd"/>
	<skos:narrower rdf:resource="https://ark.frantiq.fr/ark:/26678/pcrtFpNU7SZgo7"/>
	<skos:narrower rdf:resource="https://ark.frantiq.fr/ark:/26678/pcrt5A1NAN3NE3"/>
	<skos:narrower rdf:resource="https://ark.frantiq.fr/ark:/26678/pcrtp201sc1d5bd93jj7mm27"/>
	<skos:narrower rdf:resource="https://ark.frantiq.fr/ark:/26678/pcrtpNOweZVSSH"/>
	<skos:broader rdf:resource="https://ark.frantiq.fr/ark:/26678/pcrtIMsuG0RWTs"/>
	<skos:inScheme rdf:resource="https://ark.frantiq.fr/ark:/26678/TH_1"/>
	<opentheso:memberOf rdf:resource="https://ark.frantiq.fr/ark:/26678/pcrtv66rn9cbv1"/>
	<opentheso:memberOf rdf:resource="https://ark.frantiq.fr/ark:/26678/pcrtnbDLi2FkAj"/>
	<skos:exactMatch rdf:resource="https://www.wikidata.org/wiki/Q7946"/>
	<skos:exactMatch rdf:resource="http://vocab.getty.edu/aat/300011068"/>
	<dcterms:created rdf:datatype="http://www.w3.org/2001/XMLSchema#date">2007-02-08</dcterms:created>
	<dcterms:modified rdf:datatype="http://www.w3.org/2001/XMLSchema#date">2023-08-02</dcterms:modified>
	<dcterms:identifier>22053</dcterms:identifier>
	<dcterms:contributor>blandine.nouvel</dcterms:contributor>
	<skos:definition xml:lang="en">A homogeneous natural solid with an ordered atomic structure and a defined chemical composition (wp)</skos:definition>
	<skos:definition xml:lang="fr">Un solide naturel homogène avec une structure atomique ordonnée et une composition chimique définie. (wp)</skos:definition>
</rdf:Description>

<rdf:Description rdf:about="https://ark.frantiq.fr/ark:/26678/pcrtj3ZcwkArSR">
	<rdf:type rdf:resource="http://www.w3.org/2004/02/skos/core#Concept"/>
	<skos:prefLabel xml:lang="es">roca sedimentaria</skos:prefLabel>
	<skos:prefLabel xml:lang="it">roccia sedimentaria</skos:prefLabel>
	<skos:prefLabel xml:lang="fr">roche sédimentaire</skos:prefLabel>
	<skos:prefLabel xml:lang="nl">sedimentair gesteente</skos:prefLabel>
	<skos:prefLabel xml:lang="en">sedimentary rock</skos:prefLabel>
	<skos:prefLabel xml:lang="de">Sedimentgestein</skos:prefLabel>
	<skos:prefLabel xml:lang="ar">صخور رسوبية</skos:prefLabel>
	<skos:related rdf:resource="https://ark.frantiq.fr/ark:/26678/pcrt2nbSAPPSwB"/>
	<skos:related rdf:resource="https://ark.frantiq.fr/ark:/26678/pcrtjbpmw8qvrn"/>
	<skos:narrower rdf:resource="https://ark.frantiq.fr/ark:/26678/pcrtkdetSDq0bj"/>
	<skos:narrower rdf:resource="https://ark.frantiq.fr/ark:/26678/pcrtsEgKPlBjWE"/>
	<skos:narrower rdf:resource="https://ark.frantiq.fr/ark:/26678/pcrt4N9jrETRto"/>
	<skos:narrower rdf:resource="https://ark.frantiq.fr/ark:/26678/pcrth18FOY3yYX"/>
	<skos:narrower rdf:resource="https://ark.frantiq.fr/ark:/26678/pcrtRiKgPqvJQO"/>
	<skos:narrower rdf:resource="https://ark.frantiq.fr/ark:/26678/pcrtGAARv5y4t4"/>
	<skos:narrower rdf:resource="https://ark.frantiq.fr/ark:/26678/pcrtm4r7mvsvrw"/>
	<skos:narrower rdf:resource="https://ark.frantiq.fr/ark:/26678/pcrtsrWeYcRkNg"/>
	<skos:narrower rdf:resource="https://ark.frantiq.fr/ark:/26678/pcrtu714SnuAFj"/>
	<skos:broader rdf:resource="https://ark.frantiq.fr/ark:/26678/pcrtSVdwKcS3MI"/>
	<skos:inScheme rdf:resource="https://ark.frantiq.fr/ark:/26678/TH_1"/>
	<opentheso:memberOf rdf:resource="https://ark.frantiq.fr/ark:/26678/pcrtv66rn9cbv1"/>
	<opentheso:memberOf rdf:resource="https://ark.frantiq.fr/ark:/26678/pcrtnbDLi2FkAj"/>
	<skos:exactMatch rdf:resource="https://catalogue.bnf.fr/ark:/12148/cb11938323w"/>
	<skos:exactMatch rdf:resource="https://www.wikidata.org/wiki/Q82480"/>
	<skos:exactMatch rdf:resource="http://vocab.getty.edu/aat/300011273"/>
	<dcterms:created rdf:datatype="http://www.w3.org/2001/XMLSchema#date">2007-02-08</dcterms:created>
	<dcterms:modified rdf:datatype="http://www.w3.org/2001/XMLSchema#date">2023-08-02</dcterms:modified>
	<dcterms:identifier>22054</dcterms:identifier>
	<dcterms:contributor>blandine.nouvel</dcterms:contributor>
	<skos:definition xml:lang="en">Exogenous rock resulting from the accumulation of elements (mineral fragments, shell fragments, etc.) and/or precipitation from solutions. (Dict. de géologie, Foucault et Raoult)</skos:definition>
	<skos:definition xml:lang="fr">Roche exogène résultant de l'accumulation d'éléments (fragments minéraux, débris coquilliers, etc.) et/ou de précipitations à partir de solutions. (Dict. de géologie, Foucault et Raoult)</skos:definition>
</rdf:Description>

<rdf:Description rdf:about="https://ark.frantiq.fr/ark:/26678/pcrtDhZmKFAlZa">
	<rdf:type rdf:resource="http://www.w3.org/2004/02/skos/core#Concept"/>
	<skos:prefLabel xml:lang="en">igneous rock</skos:prefLabel>
	<skos:prefLabel xml:lang="de">magmatisches Gestein</skos:prefLabel>
	<skos:prefLabel xml:lang="nl">magmatisch gesteente</skos:prefLabel>
	<skos:prefLabel xml:lang="es">roca magmática</skos:prefLabel>
	<skos:prefLabel xml:lang="it">roccia magmatica</skos:prefLabel>
	<skos:prefLabel xml:lang="fr">roche magmatique</skos:prefLabel>
	<skos:prefLabel xml:lang="ar">صخر اندفاعي</skos:prefLabel>
	<skos:altLabel xml:lang="en">endogeneous rock</skos:altLabel>
	<skos:altLabel xml:lang="en">magmatic rock</skos:altLabel>
	<skos:altLabel xml:lang="fr">roche endogène</skos:altLabel>
	<skos:altLabel xml:lang="ar">صخر ناري</skos:altLabel>
	<skos:narrower rdf:resource="https://ark.frantiq.fr/ark:/26678/pcrt6BEybyEAjN"/>
	<skos:narrower rdf:resource="https://ark.frantiq.fr/ark:/26678/pcrtmxvuuXHSTS"/>
	<skos:narrower rdf:resource="https://ark.frantiq.fr/ark:/26678/pcrt3344f5f89w8bjkpfp2zz"/>
	<skos:broader rdf:resource="https://ark.frantiq.fr/ark:/26678/pcrtSVdwKcS3MI"/>
	<skos:inScheme rdf:resource="https://ark.frantiq.fr/ark:/26678/TH_1"/>
	<opentheso:memberOf rdf:resource="https://ark.frantiq.fr/ark:/26678/pcrtv66rn9cbv1"/>
	<opentheso:memberOf rdf:resource="https://ark.frantiq.fr/ark:/26678/pcrtnbDLi2FkAj"/>
	<skos:exactMatch rdf:resource="https://catalogue.bnf.fr/ark:/12148/cb11949164c"/>
	<skos:exactMatch rdf:resource="https://www.wikidata.org/wiki/Q42045"/>
	<skos:exactMatch rdf:resource="http://vocab.getty.edu/aat/300011178"/>
	<dcterms:created rdf:datatype="http://www.w3.org/2001/XMLSchema#date">2007-02-08</dcterms:created>
	<dcterms:modified rdf:datatype="http://www.w3.org/2001/XMLSchema#date">2023-08-02</dcterms:modified>
	<dcterms:identifier>22055</dcterms:identifier>
	<dcterms:contributor>blandine.nouvel</dcterms:contributor>
	<skos:definition xml:lang="en">Rock resulting from the solidification of magmas (Dict. de géologie, Foucault et Raoult)</skos:definition>
	<skos:definition xml:lang="fr">Roche résultant de la solidification de magmas. (Dict. de géologie, Foucault et Raoult)</skos:definition>
</rdf:Description>

<rdf:Description rdf:about="https://ark.frantiq.fr/ark:/26678/pcrtQAl1Zjr5KF">
	<rdf:type rdf:resource="http://www.w3.org/2004/02/skos/core#Concept"/>
	<skos:prefLabel xml:lang="it">onice</skos:prefLabel>
	<skos:prefLabel xml:lang="es">ónix</skos:prefLabel>
	<skos:prefLabel xml:lang="en">onyx</skos:prefLabel>
	<skos:prefLabel xml:lang="fr">onyx</skos:prefLabel>
	<skos:prefLabel xml:lang="nl">onyx</skos:prefLabel>
	<skos:prefLabel xml:lang="de">Onyx</skos:prefLabel>
	<skos:prefLabel xml:lang="ar">جَزْع</skos:prefLabel>
	<skos:altLabel xml:lang="es">ónice</skos:altLabel>
	<skos:altLabel xml:lang="ar">عقيق يمَاني</skos:altLabel>
	<skos:related rdf:resource="https://ark.frantiq.fr/ark:/26678/pcrtJt3ZKiNEFK"/>
	<skos:broader rdf:resource="https://ark.frantiq.fr/ark:/26678/pcrtOBWTai2Xms"/>
	<skos:inScheme rdf:resource="https://ark.frantiq.fr/ark:/26678/TH_1"/>
	<opentheso:memberOf rdf:resource="https://ark.frantiq.fr/ark:/26678/pcrtv66rn9cbv1"/>
	<opentheso:memberOf rdf:resource="https://ark.frantiq.fr/ark:/26678/pcrtnbDLi2FkAj"/>
	<skos:exactMatch rdf:resource="https://www.wikidata.org/wiki/Q180884"/>
	<skos:exactMatch rdf:resource="http://vocab.getty.edu/aat/300011136"/>
	<dcterms:created rdf:datatype="http://www.w3.org/2001/XMLSchema#date">2007-02-08</dcterms:created>
	<dcterms:modified rdf:datatype="http://www.w3.org/2001/XMLSchema#date">2023-08-02</dcterms:modified>
	<dcterms:identifier>22056</dcterms:identifier>
	<dcterms:contributor>blandine.nouvel</dcterms:contributor>
	<skos:definition xml:lang="fr">Variété d'agate fine, présentant des raies parallèles et concentriques de couleurs différentes et nuancées, dont certaines, semi-transparentes, rappellent celles de l'ongle, et qui est utilisée notamment pour la fabrication des camées. (TLFi)</skos:definition>
</rdf:Description>

<rdf:Description rdf:about="https://ark.frantiq.fr/ark:/26678/pcrt3PUAhlWubZ">
	<rdf:type rdf:resource="http://www.w3.org/2004/02/skos/core#Concept"/>
	<skos:prefLabel xml:lang="it">diaspro</skos:prefLabel>
	<skos:prefLabel xml:lang="es">jaspe</skos:prefLabel>
	<skos:prefLabel xml:lang="fr">jaspe</skos:prefLabel>
	<skos:prefLabel xml:lang="en">jasper</skos:prefLabel>
	<skos:prefLabel xml:lang="nl">jaspis</skos:prefLabel>
	<skos:prefLabel xml:lang="de">Jaspis</skos:prefLabel>
	<skos:prefLabel xml:lang="ar">يَشب</skos:prefLabel>
	<skos:related rdf:resource="https://ark.frantiq.fr/ark:/26678/pcrtJt3ZKiNEFK"/>
	<skos:narrower rdf:resource="https://ark.frantiq.fr/ark:/26678/pcrtX9DGL4v9Ko"/>
	<skos:narrower rdf:resource="https://ark.frantiq.fr/ark:/26678/pcrtb8qzpwp7ck"/>
	<skos:narrower rdf:resource="https://ark.frantiq.fr/ark:/26678/pcrtspv238x81q"/>
	<skos:narrower rdf:resource="https://ark.frantiq.fr/ark:/26678/pcrtXVZBob53by"/>
	<skos:narrower rdf:resource="https://ark.frantiq.fr/ark:/26678/pcrt0HFzFNNK1N"/>
	<skos:broader rdf:resource="https://ark.frantiq.fr/ark:/26678/pcrt4N9jrETRto"/>
	<skos:inScheme rdf:resource="https://ark.frantiq.fr/ark:/26678/TH_1"/>
	<opentheso:memberOf rdf:resource="https://ark.frantiq.fr/ark:/26678/pcrtv66rn9cbv1"/>
	<opentheso:memberOf rdf:resource="https://ark.frantiq.fr/ark:/26678/pcrtnbDLi2FkAj"/>
	<skos:exactMatch rdf:resource="https://www.wikidata.org/wiki/Q201175"/>
	<skos:exactMatch rdf:resource="http://vocab.getty.edu/aat/300011151"/>
	<dcterms:created rdf:datatype="http://www.w3.org/2001/XMLSchema#date">2007-02-08</dcterms:created>
	<dcterms:modified rdf:datatype="http://www.w3.org/2001/XMLSchema#date">2025-01-30</dcterms:modified>
	<dcterms:identifier>22057</dcterms:identifier>
	<dcterms:contributor>blandine.nouvel</dcterms:contributor>
	<dcterms:contributor>justine.vincent</dcterms:contributor>
	<skos:definition xml:lang="fr">Roche sédimentaire silicieuse cryptocristalline, constituée de calcédoine et de quartz opaque à légèrement translucide, contenant parfois des argiles, mais aussi des oxydes de fer responsables de la coloration, et dont les variétés les plus connues sont les radiolites, les lydiennes et les phtanites. (Fernandes, 2012).</skos:definition>
	<skos:definition xml:lang="en">Cryptocrystalline siliceous sedimentary rock, consisting of opaque to slightly translucent chalcedony and quartz, sometimes containing clays, but also iron oxides responsible for colouring, and whose best-known varieties are radiolites, lydiennes and phtanites. (Fernandes, 2012).</skos:definition>
	<skos:historyNote xml:lang="fr">2025-30-01 : modification de la définition.</skos:historyNote>
	<dcterms:source>https://doi-org.inshs.bib.cnrs.fr/10.4000/12zm5</dcterms:source>
</rdf:Description>

<rdf:Description rdf:about="https://ark.frantiq.fr/ark:/26678/pcrtX9DGL4v9Ko">
	<rdf:type rdf:resource="http://www.w3.org/2004/02/skos/core#Concept"/>
	<skos:prefLabel xml:lang="nl">radiolariet</skos:prefLabel>
	<skos:prefLabel xml:lang="de">Radiolarit</skos:prefLabel>
	<skos:prefLabel xml:lang="es">radiolarita</skos:prefLabel>
	<skos:prefLabel xml:lang="en">radiolarite</skos:prefLabel>
	<skos:prefLabel xml:lang="fr">radiolarite</skos:prefLabel>
	<skos:prefLabel xml:lang="it">radiolarite</skos:prefLabel>
	<skos:prefLabel xml:lang="ar">راديولاريت</skos:prefLabel>
	<skos:altLabel xml:lang="it">selce a radiolari</skos:altLabel>
	<skos:broader rdf:resource="https://ark.frantiq.fr/ark:/26678/pcrt3PUAhlWubZ"/>
	<skos:inScheme rdf:resource="https://ark.frantiq.fr/ark:/26678/TH_1"/>
	<opentheso:memberOf rdf:resource="https://ark.frantiq.fr/ark:/26678/pcrtv66rn9cbv1"/>
	<opentheso:memberOf rdf:resource="https://ark.frantiq.fr/ark:/26678/pcrtnbDLi2FkAj"/>
	<skos:exactMatch rdf:resource="https://www.wikidata.org/wiki/Q379386"/>
	<dcterms:created rdf:datatype="http://www.w3.org/2001/XMLSchema#date">2007-02-08</dcterms:created>
	<dcterms:modified rdf:datatype="http://www.w3.org/2001/XMLSchema#date">2025-01-30</dcterms:modified>
	<dcterms:identifier>22058</dcterms:identifier>
	<dcterms:contributor>blandine.nouvel</dcterms:contributor>
	<dcterms:contributor>justine.vincent</dcterms:contributor>
	<skos:definition xml:lang="en">Small (less than 20 microns), cryptocrystalline siliceous sedimentary rock from the Carboniferous, of chemical or biochemical origin (possible presence of radiolarians), very rich in carbonaceous matter (Fernandes, 2012).</skos:definition>
	<skos:definition xml:lang="ar">يَشم يحتوي أوليات</skos:definition>
	<skos:definition xml:lang="fr">Roche sédimentaire siliceuse de petite taille (inférieurs à 20 microns), cryptocristalline du carbonifère, d'origine chimique ou biochimique (présence possible de radiolaires), très riche en matière carbonée. (Fernandes, 2012).</skos:definition>
	<skos:historyNote xml:lang="fr">2025-30-01 : modification de la définition.</skos:historyNote>
	<dcterms:source>https://doi-org.inshs.bib.cnrs.fr/10.4000/12zm5</dcterms:source>
</rdf:Description>

<rdf:Description rdf:about="https://ark.frantiq.fr/ark:/26678/pcrt6BEybyEAjN">
	<rdf:type rdf:resource="http://www.w3.org/2004/02/skos/core#Concept"/>
	<skos:prefLabel xml:lang="en">intrusive rock</skos:prefLabel>
	<skos:prefLabel xml:lang="nl">plutonisch gesteente</skos:prefLabel>
	<skos:prefLabel xml:lang="es">roca plutónica</skos:prefLabel>
	<skos:prefLabel xml:lang="it">roccia plutonica</skos:prefLabel>
	<skos:prefLabel xml:lang="fr">roche plutonique</skos:prefLabel>
	<skos:prefLabel xml:lang="de">Tiefengestein</skos:prefLabel>
	<skos:prefLabel xml:lang="ar">صخر جوفي</skos:prefLabel>
	<skos:altLabel xml:lang="en">plutonic rock</skos:altLabel>
	<skos:altLabel xml:lang="es">roca intrusiva</skos:altLabel>
	<skos:altLabel xml:lang="it">roccia intrusiva</skos:altLabel>
	<skos:narrower rdf:resource="https://ark.frantiq.fr/ark:/26678/pcrtIxUJc35jSS"/>
	<skos:narrower rdf:resource="https://ark.frantiq.fr/ark:/26678/pcrtDnenSUMjFl"/>
	<skos:broader rdf:resource="https://ark.frantiq.fr/ark:/26678/pcrtDhZmKFAlZa"/>
	<skos:inScheme rdf:resource="https://ark.frantiq.fr/ark:/26678/TH_1"/>
	<opentheso:memberOf rdf:resource="https://ark.frantiq.fr/ark:/26678/pcrtv66rn9cbv1"/>
	<opentheso:memberOf rdf:resource="https://ark.frantiq.fr/ark:/26678/pcrtnbDLi2FkAj"/>
	<skos:exactMatch rdf:resource="https://catalogue.bnf.fr/ark:/12148/cb12264521b"/>
	<skos:exactMatch rdf:resource="https://www.wikidata.org/wiki/Q354025"/>
	<skos:exactMatch rdf:resource="https://www.wikidata.org/wiki/Q4054760"/>
	<dcterms:created rdf:datatype="http://www.w3.org/2001/XMLSchema#date">2007-02-08</dcterms:created>
	<dcterms:modified rdf:datatype="http://www.w3.org/2001/XMLSchema#date">2023-08-02</dcterms:modified>
	<dcterms:identifier>22059</dcterms:identifier>
	<dcterms:contributor>blandine.nouvel</dcterms:contributor>
	<skos:definition xml:lang="en">Magmatic rock that has crystallised within the lithosphere (Dict. de géologie, Foucault et Raoult)</skos:definition>
	<skos:definition xml:lang="fr">Roche magmatique ayant cristallisé au sein de la lithosphère (Dict. de géologie, Foucault et Raoult)</skos:definition>
</rdf:Description>

<rdf:Description rdf:about="https://ark.frantiq.fr/ark:/26678/pcrtmxvuuXHSTS">
	<rdf:type rdf:resource="http://www.w3.org/2004/02/skos/core#Concept"/>
	<skos:prefLabel xml:lang="es">roca volcánica</skos:prefLabel>
	<skos:prefLabel xml:lang="it">roccia vulcanica</skos:prefLabel>
	<skos:prefLabel xml:lang="fr">roche volcanique</skos:prefLabel>
	<skos:prefLabel xml:lang="en">volcanic rock</skos:prefLabel>
	<skos:prefLabel xml:lang="nl">vulkanische gesteente</skos:prefLabel>
	<skos:prefLabel xml:lang="de">vulkanisches Gestein</skos:prefLabel>
	<skos:prefLabel xml:lang="ar">صخر بركاني</skos:prefLabel>
	<skos:altLabel xml:lang="de">Ergussgestein</skos:altLabel>
	<skos:altLabel xml:lang="ar">صخر سطحي</skos:altLabel>
	<skos:related rdf:resource="https://ark.frantiq.fr/ark:/26678/pcrtXVZBob53by"/>
	<skos:narrower rdf:resource="https://ark.frantiq.fr/ark:/26678/pcrtctuE9VNJOc"/>
	<skos:narrower rdf:resource="https://ark.frantiq.fr/ark:/26678/pcrtgefwJa13yZ"/>
	<skos:narrower rdf:resource="https://ark.frantiq.fr/ark:/26678/pcrtp45jEJloXR"/>
	<skos:narrower rdf:resource="https://ark.frantiq.fr/ark:/26678/pcrtStScmr2cmH"/>
	<skos:narrower rdf:resource="https://ark.frantiq.fr/ark:/26678/pcrtbnBhdnlQrL"/>
	<skos:narrower rdf:resource="https://ark.frantiq.fr/ark:/26678/pcrtjSXU4udrfP"/>
	<skos:broader rdf:resource="https://ark.frantiq.fr/ark:/26678/pcrtDhZmKFAlZa"/>
	<skos:inScheme rdf:resource="https://ark.frantiq.fr/ark:/26678/TH_1"/>
	<opentheso:memberOf rdf:resource="https://ark.frantiq.fr/ark:/26678/pcrtv66rn9cbv1"/>
	<opentheso:memberOf rdf:resource="https://ark.frantiq.fr/ark:/26678/pcrtnbDLi2FkAj"/>
	<skos:exactMatch rdf:resource="https://catalogue.bnf.fr/ark:/12148/cb11944243g"/>
	<skos:exactMatch rdf:resource="https://catalogue.bnf.fr/ark:/12148/cb12264522p"/>
	<skos:exactMatch rdf:resource="https://www.wikidata.org/wiki/Q108689"/>
	<dcterms:created rdf:datatype="http://www.w3.org/2001/XMLSchema#date">2007-02-08</dcterms:created>
	<dcterms:modified rdf:datatype="http://www.w3.org/2001/XMLSchema#date">2023-08-02</dcterms:modified>
	<dcterms:identifier>22060</dcterms:identifier>
	<dcterms:contributor>blandine.nouvel</dcterms:contributor>
	<skos:definition xml:lang="en">Magmatic rock that has solidified, at least in part, at the surface of the lithosphere (Dict. de géologie, Foucault et Raoult)</skos:definition>
	<skos:definition xml:lang="fr">Roche magmatique s'étant solidifiée, au moins en partie, à la surface de la lithosphère (Dict. de géologie, Foucault et Raoult)</skos:definition>
</rdf:Description>

<rdf:Description rdf:about="https://ark.frantiq.fr/ark:/26678/pcrtt7G9pnQlu1">
	<rdf:type rdf:resource="http://www.w3.org/2004/02/skos/core#Concept"/>
	<skos:prefLabel xml:lang="it">grès</skos:prefLabel>
	<skos:prefLabel xml:lang="es">gres (cerámica)</skos:prefLabel>
	<skos:prefLabel xml:lang="fr">grès (céramique)</skos:prefLabel>
	<skos:prefLabel xml:lang="nl">steengoed</skos:prefLabel>
	<skos:prefLabel xml:lang="de">Steinzeug</skos:prefLabel>
	<skos:prefLabel xml:lang="en">stoneware</skos:prefLabel>
	<skos:prefLabel xml:lang="ar">صَلصال</skos:prefLabel>
	<skos:altLabel xml:lang="it">gres</skos:altLabel>
	<skos:narrower rdf:resource="https://ark.frantiq.fr/ark:/26678/crtSPE6Lx4cPI"/>
	<skos:narrower rdf:resource="https://ark.frantiq.fr/ark:/26678/pcrt9lQWQXyMXK"/>
	<skos:narrower rdf:resource="https://ark.frantiq.fr/ark:/26678/pcrtIq9NE61BMc"/>
	<skos:broader rdf:resource="https://ark.frantiq.fr/ark:/26678/pcrtfx4s0yvSLj"/>
	<skos:inScheme rdf:resource="https://ark.frantiq.fr/ark:/26678/TH_1"/>
	<opentheso:memberOf rdf:resource="https://ark.frantiq.fr/ark:/26678/pcrtv66rn9cbv1"/>
	<opentheso:memberOf rdf:resource="https://ark.frantiq.fr/ark:/26678/pcrtnbDLi2FkAj"/>
	<skos:closeMatch rdf:resource="https://ark.mom.fr/ark:/39676/bibp721vgd1px"/>
	<skos:exactMatch rdf:resource="https://catalogue.bnf.fr/ark:/12148/cb11961607d"/>
	<skos:exactMatch rdf:resource="https://www.wikidata.org/wiki/Q830894"/>
	<skos:exactMatch rdf:resource="http://vocab.getty.edu/aat/300010672"/>
	<dcterms:created rdf:datatype="http://www.w3.org/2001/XMLSchema#date">2007-02-08</dcterms:created>
	<dcterms:modified rdf:datatype="http://www.w3.org/2001/XMLSchema#date">2023-08-02</dcterms:modified>
	<dcterms:identifier>22680</dcterms:identifier>
	<dcterms:contributor>blandine.nouvel</dcterms:contributor>
	<skos:definition xml:lang="en">Opaque, hard, sound and impermeable pottery resulting from a high-temperature firing (around 1200°C) causing semi-vitrification. (Balfet)</skos:definition>
	<skos:definition xml:lang="fr">Poterie opaque, dure, sonore et imperméable résultant d’une cuisson à température élevée (environ 1200°C) provoquant une semi-vitrification. (Balfet)</skos:definition>
	<skos:historyNote xml:lang="fr">Modification de  grès (pot)  en  grès (céramique) , moins restrictif, le 26/09/2017 par PM.</skos:historyNote>
</rdf:Description>

<rdf:Description rdf:about="https://ark.frantiq.fr/ark:/26678/pcrtQqTsG6TEFy">
	<rdf:type rdf:resource="http://www.w3.org/2004/02/skos/core#Concept"/>
	<skos:prefLabel xml:lang="it">ardesia</skos:prefLabel>
	<skos:prefLabel xml:lang="fr">ardoise</skos:prefLabel>
	<skos:prefLabel xml:lang="nl">leisteen</skos:prefLabel>
	<skos:prefLabel xml:lang="es">pizarra</skos:prefLabel>
	<skos:prefLabel xml:lang="de">Schiefer</skos:prefLabel>
	<skos:prefLabel xml:lang="en">slate</skos:prefLabel>
	<skos:prefLabel xml:lang="ar">أردواز</skos:prefLabel>
	<skos:broader rdf:resource="https://ark.frantiq.fr/ark:/26678/pcrtxybfLE1dkn"/>
	<skos:inScheme rdf:resource="https://ark.frantiq.fr/ark:/26678/TH_1"/>
	<opentheso:memberOf rdf:resource="https://ark.frantiq.fr/ark:/26678/pcrtv66rn9cbv1"/>
	<opentheso:memberOf rdf:resource="https://ark.frantiq.fr/ark:/26678/pcrtnbDLi2FkAj"/>
	<opentheso:memberOf rdf:resource="https://ark.frantiq.fr/ark:/26678/pcrtv0jq332vcq3gxt5m13d5"/>
	<skos:exactMatch rdf:resource="https://catalogue.bnf.fr/ark:/12148/cb119316382"/>
	<skos:exactMatch rdf:resource="https://www.wikidata.org/wiki/Q207079"/>
	<skos:exactMatch rdf:resource="http://vocab.getty.edu/aat/300011646"/>
	<dcterms:created rdf:datatype="http://www.w3.org/2001/XMLSchema#date">2007-02-08</dcterms:created>
	<dcterms:modified rdf:datatype="http://www.w3.org/2001/XMLSchema#date">2024-09-06</dcterms:modified>
	<dcterms:identifier>23490</dcterms:identifier>
	<dcterms:contributor>blandine.nouvel</dcterms:contributor>
	<dcterms:contributor>patricia.moitrel</dcterms:contributor>
	<skos:definition xml:lang="en">Metamorphic rock derived from a clay that has undergone little general metamorphism. (wp)</skos:definition>
	<skos:definition xml:lang="fr">Roche métamorphique issue d'une argile ayant subi un métamorphisme général faible. (wp)</skos:definition>
</rdf:Description>

<rdf:Description rdf:about="https://ark.frantiq.fr/ark:/26678/pcrt9JSk28suqb">
	<rdf:type rdf:resource="http://www.w3.org/2004/02/skos/core#Concept"/>
	<skos:prefLabel xml:lang="de">Dachsteinplatte</skos:prefLabel>
	<skos:prefLabel xml:lang="en">flagstone</skos:prefLabel>
	<skos:prefLabel xml:lang="es">laja</skos:prefLabel>
	<skos:prefLabel xml:lang="fr">lauze</skos:prefLabel>
	<skos:prefLabel xml:lang="it">losa</skos:prefLabel>
	<skos:prefLabel xml:lang="nl">stapsteen</skos:prefLabel>
	<skos:prefLabel xml:lang="ar">حجر صفيحي</skos:prefLabel>
	<skos:altLabel xml:lang="es">piedra laja</skos:altLabel>
	<skos:broader rdf:resource="https://ark.frantiq.fr/ark:/26678/pcrtQuZiT5nYY2"/>
	<skos:inScheme rdf:resource="https://ark.frantiq.fr/ark:/26678/TH_1"/>
	<opentheso:memberOf rdf:resource="https://ark.frantiq.fr/ark:/26678/pcrtv66rn9cbv1"/>
	<opentheso:memberOf rdf:resource="https://ark.frantiq.fr/ark:/26678/pcrtnbDLi2FkAj"/>
	<opentheso:memberOf rdf:resource="https://ark.frantiq.fr/ark:/26678/pcrtv0jq332vcq3gxt5m13d5"/>
	<skos:exactMatch rdf:resource="https://www.wikidata.org/wiki/Q1188398"/>
	<skos:exactMatch rdf:resource="http://vocab.getty.edu/aat/300011687"/>
	<dcterms:created rdf:datatype="http://www.w3.org/2001/XMLSchema#date">2007-02-08</dcterms:created>
	<dcterms:modified rdf:datatype="http://www.w3.org/2001/XMLSchema#date">2024-03-21</dcterms:modified>
	<dcterms:identifier>24057</dcterms:identifier>
	<dcterms:contributor>blandine.nouvel</dcterms:contributor>
	<dcterms:contributor>irene.weis</dcterms:contributor>
	<skos:definition xml:lang="en">Flat schist or limestone stone, cut in beds and used as slabs or to cover buildings (ATLIF)</skos:definition>
	<skos:definition xml:lang="fr">Pierre plate de schiste ou de calcaire, détachée par lits et utilisée comme dalle ou pour couvrir les bâtiments (ATLIF)</skos:definition>
</rdf:Description>

<rdf:Description rdf:about="https://ark.frantiq.fr/ark:/26678/pcrtc6RmFQxFuS">
	<rdf:type rdf:resource="http://www.w3.org/2004/02/skos/core#Concept"/>
	<skos:prefLabel xml:lang="it">pece</skos:prefLabel>
	<skos:prefLabel xml:lang="de">Pech</skos:prefLabel>
	<skos:prefLabel xml:lang="nl">pek</skos:prefLabel>
	<skos:prefLabel xml:lang="es">pez</skos:prefLabel>
	<skos:prefLabel xml:lang="en">pitch (resin)</skos:prefLabel>
	<skos:prefLabel xml:lang="fr">poix</skos:prefLabel>
	<skos:prefLabel xml:lang="ar">زِفت</skos:prefLabel>
	<skos:altLabel xml:lang="es">alquitrán</skos:altLabel>
	<skos:related rdf:resource="https://ark.frantiq.fr/ark:/26678/pcrt7G67xbK5BN"/>
	<skos:broader rdf:resource="https://ark.frantiq.fr/ark:/26678/pcrtnHxyjOkhJw"/>
	<skos:inScheme rdf:resource="https://ark.frantiq.fr/ark:/26678/TH_1"/>
	<opentheso:memberOf rdf:resource="https://ark.frantiq.fr/ark:/26678/pcrtv66rn9cbv1"/>
	<opentheso:memberOf rdf:resource="https://ark.frantiq.fr/ark:/26678/pcrtnbDLi2FkAj"/>
	<skos:exactMatch rdf:resource="https://www.wikidata.org/wiki/Q840692"/>
	<dcterms:created rdf:datatype="http://www.w3.org/2001/XMLSchema#date">2007-02-08</dcterms:created>
	<dcterms:modified rdf:datatype="http://www.w3.org/2001/XMLSchema#date">2024-11-15</dcterms:modified>
	<dcterms:identifier>24059</dcterms:identifier>
	<dcterms:contributor>blandine.nouvel</dcterms:contributor>
	<dcterms:contributor>justine.vincent</dcterms:contributor>
	<skos:definition xml:lang="en">A sticky substance produced by distillation, which can be black, such as that made from resins and tars, or lighter, such as that derived from pine resin and used to fix lightweight objects or as a waterproofing coating (Wikipedia).</skos:definition>
	<skos:definition xml:lang="fr">Matière collante produite par distillation, pouvant être noire comme celle constituée à partir de résines et goudrons, ou plus claire comme celle tirée des dérivés de la résine de pin et utilisée pour la fixation de corps légers ou comme enduit imperméabilisant. (Wikipédia).</skos:definition>
	<skos:historyNote xml:lang="fr">2024-11-15 : modification de la définition.</skos:historyNote>
</rdf:Description>

<rdf:Description rdf:about="https://ark.frantiq.fr/ark:/26678/pcrtolrabjfp2T">
	<rdf:type rdf:resource="http://www.w3.org/2004/02/skos/core#Concept"/>
	<skos:prefLabel xml:lang="es">fallo de cocción</skos:prefLabel>
	<skos:prefLabel xml:lang="de">Fehlbrand</skos:prefLabel>
	<skos:prefLabel xml:lang="nl">misbaksel</skos:prefLabel>
	<skos:prefLabel xml:lang="en">misfired pottery</skos:prefLabel>
	<skos:prefLabel xml:lang="fr">raté de cuisson</skos:prefLabel>
	<skos:prefLabel xml:lang="it">scarto di fornace</skos:prefLabel>
	<skos:prefLabel xml:lang="ar">شي مُخفِق</skos:prefLabel>
	<skos:related rdf:resource="https://ark.frantiq.fr/ark:/26678/pcrtx3wq2lIxhn"/>
	<skos:broader rdf:resource="https://ark.frantiq.fr/ark:/26678/pcrtfx4s0yvSLj"/>
	<skos:inScheme rdf:resource="https://ark.frantiq.fr/ark:/26678/TH_1"/>
	<opentheso:memberOf rdf:resource="https://ark.frantiq.fr/ark:/26678/pcrtv66rn9cbv1"/>
	<opentheso:memberOf rdf:resource="https://ark.frantiq.fr/ark:/26678/pcrtnbDLi2FkAj"/>
	<skos:exactMatch rdf:resource="https://www.wikidata.org/wiki/Q27926355"/>
	<dcterms:created rdf:datatype="http://www.w3.org/2001/XMLSchema#date">2007-02-08</dcterms:created>
	<dcterms:modified rdf:datatype="http://www.w3.org/2001/XMLSchema#date">2024-10-25</dcterms:modified>
	<dcterms:identifier>24080</dcterms:identifier>
	<dcterms:contributor>blandine.nouvel</dcterms:contributor>
	<dcterms:contributor>justine.vincent</dcterms:contributor>
	<dcterms:contributor>patricia.moitrel</dcterms:contributor>
	<skos:definition xml:lang="en">Ceramic deteriorated following a firing anomaly (Pactols group)</skos:definition>
	<skos:definition xml:lang="fr">Céramique détériorée suite à une anomalie à la cuisson.</skos:definition>
</rdf:Description>

<rdf:Description rdf:about="https://ark.frantiq.fr/ark:/26678/pcrtOJj49Pe6Vb">
	<rdf:type rdf:resource="http://www.w3.org/2004/02/skos/core#Concept"/>
	<skos:prefLabel xml:lang="es">grèze litée</skos:prefLabel>
	<skos:prefLabel xml:lang="fr">grèze litée</skos:prefLabel>
	<skos:prefLabel xml:lang="it">grèze litée</skos:prefLabel>
	<skos:prefLabel xml:lang="nl">grèze litée</skos:prefLabel>
	<skos:prefLabel xml:lang="en">stratified slope deposit</skos:prefLabel>
	<skos:prefLabel xml:lang="de">stratifizierte Hangablagerungen</skos:prefLabel>
	<skos:prefLabel xml:lang="ar">سرير جليدي</skos:prefLabel>
	<skos:altLabel xml:lang="en">bedded periglacial formations</skos:altLabel>
	<skos:altLabel xml:lang="de">geschichtete Hangsedimente</skos:altLabel>
	<skos:broader rdf:resource="https://ark.frantiq.fr/ark:/26678/pcrtgg4KWVZk74"/>
	<skos:inScheme rdf:resource="https://ark.frantiq.fr/ark:/26678/TH_1"/>
	<opentheso:memberOf rdf:resource="https://ark.frantiq.fr/ark:/26678/pcrtv66rn9cbv1"/>
	<opentheso:memberOf rdf:resource="https://ark.frantiq.fr/ark:/26678/pcrtnbDLi2FkAj"/>
	<skos:exactMatch rdf:resource="https://www.wikidata.org/wiki/Q5803636"/>
	<dcterms:created rdf:datatype="http://www.w3.org/2001/XMLSchema#date">2007-02-08</dcterms:created>
	<dcterms:modified rdf:datatype="http://www.w3.org/2001/XMLSchema#date">2024-10-18</dcterms:modified>
	<dcterms:identifier>24138</dcterms:identifier>
	<dcterms:contributor>blandine.nouvel</dcterms:contributor>
	<dcterms:contributor>justine.vincent</dcterms:contributor>
	<skos:definition xml:lang="en">Periglacial formation (Dict. de géologie / Foucault, Raoult).</skos:definition>
	<skos:definition xml:lang="fr">Modelé périglaciaire (Dict. de géologie / Foucault, Raoult).</skos:definition>
</rdf:Description>

<rdf:Description rdf:about="https://ark.frantiq.fr/ark:/26678/pcrtRT5qpNmDqE">
	<rdf:type rdf:resource="http://www.w3.org/2004/02/skos/core#Concept"/>
	<skos:prefLabel xml:lang="nl">calciet</skos:prefLabel>
	<skos:prefLabel xml:lang="es">calcita</skos:prefLabel>
	<skos:prefLabel xml:lang="en">calcite</skos:prefLabel>
	<skos:prefLabel xml:lang="fr">calcite</skos:prefLabel>
	<skos:prefLabel xml:lang="it">calcite</skos:prefLabel>
	<skos:prefLabel xml:lang="de">Kalkspat</skos:prefLabel>
	<skos:prefLabel xml:lang="ar">كالسيت</skos:prefLabel>
	<skos:altLabel xml:lang="de">Kalzit</skos:altLabel>
	<skos:altLabel xml:lang="ar">كربونات الكالسيوم</skos:altLabel>
	<skos:related rdf:resource="https://ark.frantiq.fr/ark:/26678/pcrtSkipOsBGML"/>
	<skos:broader rdf:resource="https://ark.frantiq.fr/ark:/26678/pcrtqnzx9qwkt5"/>
	<skos:inScheme rdf:resource="https://ark.frantiq.fr/ark:/26678/TH_1"/>
	<opentheso:memberOf rdf:resource="https://ark.frantiq.fr/ark:/26678/pcrtv66rn9cbv1"/>
	<opentheso:memberOf rdf:resource="https://ark.frantiq.fr/ark:/26678/pcrtnbDLi2FkAj"/>
	<skos:exactMatch rdf:resource="https://catalogue.bnf.fr/ark:/12148/cb12218096s"/>
	<skos:exactMatch rdf:resource="https://www.wikidata.org/wiki/Q171917"/>
	<skos:exactMatch rdf:resource="http://vocab.getty.edu/aat/300011078"/>
	<dcterms:created rdf:datatype="http://www.w3.org/2001/XMLSchema#date">2007-02-08</dcterms:created>
	<dcterms:modified rdf:datatype="http://www.w3.org/2001/XMLSchema#date">2024-11-18</dcterms:modified>
	<dcterms:identifier>24139</dcterms:identifier>
	<dcterms:contributor>blandine.nouvel</dcterms:contributor>
	<dcterms:contributor>justine.vincent</dcterms:contributor>
	<skos:definition xml:lang="en">Very common mineral, main constituent of limestone rocks, stalactites and stalagmites. (According to Lozet &amp;amp; Mathieu, Dictionnaire de science du sol. Ed. Technique et Documentation Lavoisier)</skos:definition>
	<skos:definition xml:lang="fr">Minéral très commun, constituant principal des roches calcaires, des stalactites et stalagmites. (D'après Lozet &amp;amp; Mathieu, Dictionnaire de science du sol. Ed. Technique et Documentation Lavoisier)</skos:definition>
</rdf:Description>

<rdf:Description rdf:about="https://ark.frantiq.fr/ark:/26678/pcrt2nbSAPPSwB">
	<rdf:type rdf:resource="http://www.w3.org/2004/02/skos/core#Concept"/>
	<skos:prefLabel xml:lang="nl">fosfaat</skos:prefLabel>
	<skos:prefLabel xml:lang="es">fosfato</skos:prefLabel>
	<skos:prefLabel xml:lang="it">fosfato</skos:prefLabel>
	<skos:prefLabel xml:lang="de">Phosphat</skos:prefLabel>
	<skos:prefLabel xml:lang="en">phosphate</skos:prefLabel>
	<skos:prefLabel xml:lang="fr">phosphate</skos:prefLabel>
	<skos:prefLabel xml:lang="ar">فُسفات</skos:prefLabel>
	<skos:altLabel xml:lang="ar">ملح فُسفوري</skos:altLabel>
	<skos:related rdf:resource="https://ark.frantiq.fr/ark:/26678/pcrtj3ZcwkArSR"/>
	<skos:narrower rdf:resource="https://ark.frantiq.fr/ark:/26678/crtL2Kjt70xql"/>
	<skos:broader rdf:resource="https://ark.frantiq.fr/ark:/26678/pcrty2mcsksa6s"/>
	<skos:inScheme rdf:resource="https://ark.frantiq.fr/ark:/26678/TH_1"/>
	<opentheso:memberOf rdf:resource="https://ark.frantiq.fr/ark:/26678/pcrtv66rn9cbv1"/>
	<opentheso:memberOf rdf:resource="https://ark.frantiq.fr/ark:/26678/pcrtnbDLi2FkAj"/>
	<skos:exactMatch rdf:resource="https://www.wikidata.org/wiki/Q177811"/>
	<dcterms:created rdf:datatype="http://www.w3.org/2001/XMLSchema#date">2007-02-08</dcterms:created>
	<dcterms:modified rdf:datatype="http://www.w3.org/2001/XMLSchema#date">2023-08-02</dcterms:modified>
	<dcterms:identifier>24140</dcterms:identifier>
	<dcterms:contributor>blandine.nouvel</dcterms:contributor>
	<skos:definition xml:lang="en">Any mineral containing tetrahedral phosphate ions (Fernandes, 2012).</skos:definition>
	<skos:definition xml:lang="fr">Tout minéral contenant des ions phosphates tétraédriques (Fernandes, 2012).</skos:definition>
</rdf:Description>

<rdf:Description rdf:about="https://ark.frantiq.fr/ark:/26678/pcrtF8Wf7AekK2">
	<rdf:type rdf:resource="http://www.w3.org/2004/02/skos/core#Concept"/>
	<skos:prefLabel xml:lang="en">silica</skos:prefLabel>
	<skos:prefLabel xml:lang="nl">silica</skos:prefLabel>
	<skos:prefLabel xml:lang="fr">silice</skos:prefLabel>
	<skos:prefLabel xml:lang="it">silice</skos:prefLabel>
	<skos:prefLabel xml:lang="es">silicio</skos:prefLabel>
	<skos:prefLabel xml:lang="de">Siliziumdioxid</skos:prefLabel>
	<skos:prefLabel xml:lang="ar">سيليكا</skos:prefLabel>
	<skos:altLabel xml:lang="it">anidride silicica</skos:altLabel>
	<skos:altLabel xml:lang="it">diossido di silicio</skos:altLabel>
	<skos:altLabel xml:lang="en">silicon dioxide</skos:altLabel>
	<skos:broader rdf:resource="https://ark.frantiq.fr/ark:/26678/pcrty2mcsksa6s"/>
	<skos:inScheme rdf:resource="https://ark.frantiq.fr/ark:/26678/TH_1"/>
	<opentheso:memberOf rdf:resource="https://ark.frantiq.fr/ark:/26678/pcrtv66rn9cbv1"/>
	<opentheso:memberOf rdf:resource="https://ark.frantiq.fr/ark:/26678/pcrtnbDLi2FkAj"/>
	<skos:exactMatch rdf:resource="https://www.wikidata.org/wiki/Q15724995"/>
	<dcterms:created rdf:datatype="http://www.w3.org/2001/XMLSchema#date">2007-02-08</dcterms:created>
	<dcterms:modified rdf:datatype="http://www.w3.org/2001/XMLSchema#date">2024-11-19</dcterms:modified>
	<dcterms:identifier>24141</dcterms:identifier>
	<dcterms:contributor>blandine.nouvel</dcterms:contributor>
	<dcterms:contributor>justine.vincent</dcterms:contributor>
	<skos:definition xml:lang="en">Hard, stable mineral present in rocks in the form of quartz.</skos:definition>
	<skos:definition xml:lang="fr">Minéral dur et stable présent dans les roches sous forme de quartz.</skos:definition>
</rdf:Description>

<rdf:Description rdf:about="https://ark.frantiq.fr/ark:/26678/pcrtc2SkvG29we">
	<rdf:type rdf:resource="http://www.w3.org/2004/02/skos/core#Concept"/>
	<skos:prefLabel xml:lang="nl">bergkristal</skos:prefLabel>
	<skos:prefLabel xml:lang="de">Bergkristall</skos:prefLabel>
	<skos:prefLabel xml:lang="es">cristal de roca</skos:prefLabel>
	<skos:prefLabel xml:lang="fr">cristal de roche</skos:prefLabel>
	<skos:prefLabel xml:lang="it">cristallo di rocca</skos:prefLabel>
	<skos:prefLabel xml:lang="en">rock crystal</skos:prefLabel>
	<skos:prefLabel xml:lang="ar">مهاة</skos:prefLabel>
	<skos:altLabel xml:lang="fr">cristaux</skos:altLabel>
	<skos:altLabel xml:lang="en">quartz</skos:altLabel>
	<skos:altLabel xml:lang="fr">quartz hyalin</skos:altLabel>
	<skos:altLabel xml:lang="it">quarzo ialino</skos:altLabel>
	<skos:broader rdf:resource="https://ark.frantiq.fr/ark:/26678/pcrtDwe0cp16nl"/>
	<skos:inScheme rdf:resource="https://ark.frantiq.fr/ark:/26678/TH_1"/>
	<opentheso:memberOf rdf:resource="https://ark.frantiq.fr/ark:/26678/pcrtv66rn9cbv1"/>
	<opentheso:memberOf rdf:resource="https://ark.frantiq.fr/ark:/26678/pcrtnbDLi2FkAj"/>
	<opentheso:memberOf rdf:resource="https://ark.frantiq.fr/ark:/26678/pcrtv0jq332vcq3gxt5m13d5"/>
	<skos:exactMatch rdf:resource="https://www.wikidata.org/wiki/Q2050687"/>
	<skos:exactMatch rdf:resource="http://vocab.getty.edu/aat/300011152"/>
	<dcterms:created rdf:datatype="http://www.w3.org/2001/XMLSchema#date">2007-02-08</dcterms:created>
	<dcterms:modified rdf:datatype="http://www.w3.org/2001/XMLSchema#date">2024-11-18</dcterms:modified>
	<dcterms:identifier>24142</dcterms:identifier>
	<dcterms:contributor>blandine.nouvel</dcterms:contributor>
	<dcterms:contributor>justine.vincent</dcterms:contributor>
	<dcterms:contributor>patricia.moitrel</dcterms:contributor>
	<skos:definition xml:lang="en">Very hard, colourless, transparent quartz crystal (Raoult and Foucault, 2005).</skos:definition>
	<skos:definition xml:lang="fr">Cristal automorphe de quartz &lt;span style= background-color: rgb(255, 255, 255); &gt;transparent, incolore et très dur. &lt;/span&gt; (Raoult et Foucault, 2005).</skos:definition>
</rdf:Description>

<rdf:Description rdf:about="https://ark.frantiq.fr/ark:/26678/pcrtkgSlgXZbNa">
	<rdf:type rdf:resource="http://www.w3.org/2004/02/skos/core#Concept"/>
	<skos:prefLabel xml:lang="nl">travertijn</skos:prefLabel>
	<skos:prefLabel xml:lang="fr">travertin</skos:prefLabel>
	<skos:prefLabel xml:lang="de">Travertin</skos:prefLabel>
	<skos:prefLabel xml:lang="en">travertine</skos:prefLabel>
	<skos:prefLabel xml:lang="es">travertino</skos:prefLabel>
	<skos:prefLabel xml:lang="it">travertino</skos:prefLabel>
	<skos:prefLabel xml:lang="ar">ترافرتين</skos:prefLabel>
	<skos:altLabel xml:lang="fr">pierre de Tivoli</skos:altLabel>
	<skos:altLabel xml:lang="en">tufa</skos:altLabel>
	<skos:altLabel xml:lang="fr">tuf calcaire</skos:altLabel>
	<skos:related rdf:resource="https://ark.frantiq.fr/ark:/26678/pcrtfx2fwztQ8p"/>
	<skos:broader rdf:resource="https://ark.frantiq.fr/ark:/26678/pcrtc1Ueky7Zpg"/>
	<skos:inScheme rdf:resource="https://ark.frantiq.fr/ark:/26678/TH_1"/>
	<opentheso:memberOf rdf:resource="https://ark.frantiq.fr/ark:/26678/pcrtv66rn9cbv1"/>
	<opentheso:memberOf rdf:resource="https://ark.frantiq.fr/ark:/26678/pcrtnbDLi2FkAj"/>
	<skos:exactMatch rdf:resource="https://www.wikidata.org/wiki/Q187156"/>
	<skos:exactMatch rdf:resource="http://vocab.getty.edu/aat/300011329"/>
	<dcterms:created rdf:datatype="http://www.w3.org/2001/XMLSchema#date">2007-02-08</dcterms:created>
	<dcterms:modified rdf:datatype="http://www.w3.org/2001/XMLSchema#date">2023-08-02</dcterms:modified>
	<dcterms:identifier>24144</dcterms:identifier>
	<dcterms:contributor>blandine.nouvel</dcterms:contributor>
	<skos:definition xml:lang="fr">Roche sédimentaire calcaire qui se forme aux émergences des sources calcaires sur le flanc d'une vallée ou en travers d'un cours d'eau avec rapides et cascades. Peut être une roche grossièrement litée, vacuolaire, jaunâtre et renfermant souvent des débris végétaux parfaitement conservés. (Lozet &amp;amp; Mathieu, Dictionnaire de science du sol. Ed. Technique et documentation Lavoisier)</skos:definition>
</rdf:Description>

<rdf:Description rdf:about="https://ark.frantiq.fr/ark:/26678/pcrtEU8K1oF2Eh">
	<rdf:type rdf:resource="http://www.w3.org/2004/02/skos/core#Concept"/>
	<skos:prefLabel xml:lang="en">chert</skos:prefLabel>
	<skos:prefLabel xml:lang="es">chert</skos:prefLabel>
	<skos:prefLabel xml:lang="fr">chert</skos:prefLabel>
	<skos:prefLabel xml:lang="it">chert</skos:prefLabel>
	<skos:prefLabel xml:lang="nl">hoornkiezel</skos:prefLabel>
	<skos:prefLabel xml:lang="de">Hornstein</skos:prefLabel>
	<skos:prefLabel xml:lang="ar">شرت</skos:prefLabel>
	<skos:altLabel xml:lang="ar">تشكل صخري صواني</skos:altLabel>
	<skos:broader rdf:resource="https://ark.frantiq.fr/ark:/26678/pcrt4N9jrETRto"/>
	<skos:inScheme rdf:resource="https://ark.frantiq.fr/ark:/26678/TH_1"/>
	<opentheso:memberOf rdf:resource="https://ark.frantiq.fr/ark:/26678/pcrtv66rn9cbv1"/>
	<opentheso:memberOf rdf:resource="https://ark.frantiq.fr/ark:/26678/pcrtnbDLi2FkAj"/>
	<skos:exactMatch rdf:resource="https://www.wikidata.org/wiki/Q1070438"/>
	<skos:exactMatch rdf:resource="http://vocab.getty.edu/aat/300011141"/>
	<dcterms:created rdf:datatype="http://www.w3.org/2001/XMLSchema#date">2007-02-08</dcterms:created>
	<dcterms:modified rdf:datatype="http://www.w3.org/2001/XMLSchema#date">2025-01-30</dcterms:modified>
	<dcterms:identifier>24145</dcterms:identifier>
	<dcterms:contributor>blandine.nouvel</dcterms:contributor>
	<dcterms:contributor>justine.vincent</dcterms:contributor>
	<skos:definition xml:lang="en">Varied siliceous rocks in nodules or banks with blurred edges in marine sedimentary rocks most often from the Jurassic period (Fernandes, 2012).</skos:definition>
	<skos:definition xml:lang="fr">Désigne des roches siliceuses variées en nodules ou en bancs et aux bordures floues dans des roches sédimentaires marines appartenant le plus souvent à la période jurassique (Fernandes, 2012).</skos:definition>
	<skos:historyNote xml:lang="fr">2025-30-01 : modification de la définition.</skos:historyNote>
	<dcterms:source>https://doi-org.inshs.bib.cnrs.fr/10.4000/12zm5</dcterms:source>
</rdf:Description>

<rdf:Description rdf:about="https://ark.frantiq.fr/ark:/26678/pcrth18FOY3yYX">
	<rdf:type rdf:resource="http://www.w3.org/2004/02/skos/core#Concept"/>
	<skos:prefLabel xml:lang="nl">fosforiet</skos:prefLabel>
	<skos:prefLabel xml:lang="es">fosforita</skos:prefLabel>
	<skos:prefLabel xml:lang="it">fosforite</skos:prefLabel>
	<skos:prefLabel xml:lang="de">Phosphorit</skos:prefLabel>
	<skos:prefLabel xml:lang="en">phosphorite</skos:prefLabel>
	<skos:prefLabel xml:lang="fr">phosphorite</skos:prefLabel>
	<skos:prefLabel xml:lang="ar">فوسفوريت</skos:prefLabel>
	<skos:altLabel xml:lang="en">phosphate rock</skos:altLabel>
	<skos:altLabel xml:lang="en">rock phosphate</skos:altLabel>
	<skos:broader rdf:resource="https://ark.frantiq.fr/ark:/26678/pcrtj3ZcwkArSR"/>
	<skos:inScheme rdf:resource="https://ark.frantiq.fr/ark:/26678/TH_1"/>
	<opentheso:memberOf rdf:resource="https://ark.frantiq.fr/ark:/26678/pcrtv66rn9cbv1"/>
	<opentheso:memberOf rdf:resource="https://ark.frantiq.fr/ark:/26678/pcrtnbDLi2FkAj"/>
	<skos:exactMatch rdf:resource="https://www.wikidata.org/wiki/Q1424327"/>
	<skos:exactMatch rdf:resource="http://vocab.getty.edu/aat/300390982"/>
	<dcterms:created rdf:datatype="http://www.w3.org/2001/XMLSchema#date">2007-02-08</dcterms:created>
	<dcterms:modified rdf:datatype="http://www.w3.org/2001/XMLSchema#date">2024-11-18</dcterms:modified>
	<dcterms:identifier>24146</dcterms:identifier>
	<dcterms:contributor>blandine.nouvel</dcterms:contributor>
	<dcterms:contributor>justine.vincent</dcterms:contributor>
	<skos:definition xml:lang="en">Phosphate rock of detritic origin (wp)</skos:definition>
	<skos:definition xml:lang="fr">Roche phosphatée d'origine détritique. (wp)</skos:definition>
</rdf:Description>

<rdf:Description rdf:about="https://ark.frantiq.fr/ark:/26678/pcrtgg4KWVZk74">
	<rdf:type rdf:resource="http://www.w3.org/2004/02/skos/core#Concept"/>
	<skos:prefLabel xml:lang="fr">colluvions</skos:prefLabel>
	<skos:prefLabel xml:lang="en">colluvium</skos:prefLabel>
	<skos:prefLabel xml:lang="it">colluvium</skos:prefLabel>
	<skos:prefLabel xml:lang="nl">colluvium</skos:prefLabel>
	<skos:prefLabel xml:lang="es">coluvión</skos:prefLabel>
	<skos:prefLabel xml:lang="de">Kolluvium</skos:prefLabel>
	<skos:prefLabel xml:lang="ar">ركام سطحي</skos:prefLabel>
	<skos:altLabel xml:lang="en">colluvial material</skos:altLabel>
	<skos:altLabel xml:lang="en">colluvial soil</skos:altLabel>
	<skos:altLabel xml:lang="fr">dépôt de pente</skos:altLabel>
	<skos:related rdf:resource="https://ark.frantiq.fr/ark:/26678/pcrtGpkbj7hLSu"/>
	<skos:narrower rdf:resource="https://ark.frantiq.fr/ark:/26678/pcrtOJj49Pe6Vb"/>
	<skos:broader rdf:resource="https://ark.frantiq.fr/ark:/26678/pcrtjbpmw8qvrn"/>
	<skos:inScheme rdf:resource="https://ark.frantiq.fr/ark:/26678/TH_1"/>
	<opentheso:memberOf rdf:resource="https://ark.frantiq.fr/ark:/26678/pcrtv66rn9cbv1"/>
	<opentheso:memberOf rdf:resource="https://ark.frantiq.fr/ark:/26678/pcrtnbDLi2FkAj"/>
	<skos:exactMatch rdf:resource="https://www.wikidata.org/wiki/Q1152275"/>
	<dcterms:created rdf:datatype="http://www.w3.org/2001/XMLSchema#date">2007-02-08</dcterms:created>
	<dcterms:modified rdf:datatype="http://www.w3.org/2001/XMLSchema#date">2023-08-02</dcterms:modified>
	<dcterms:identifier>24147</dcterms:identifier>
	<dcterms:contributor>blandine.nouvel</dcterms:contributor>
	<skos:definition xml:lang="en">Slope sedimentary deposits (scree, sandstone, flint biefs, solifluction flows, etc.) not very far from the formation from which they originate (GDR Silex, 2020).</skos:definition>
	<skos:definition xml:lang="fr">Dépôts sédimentaires de versant (éboulis, grèzes, biefs à silex, coulées de solifluxions…)  peu distants de la formation de laquelle ils sont issus (GDR Silex, 2020)</skos:definition>
</rdf:Description>

<rdf:Description rdf:about="https://ark.frantiq.fr/ark:/26678/pcrt4Jy2JE8F3U">
	<rdf:type rdf:resource="http://www.w3.org/2004/02/skos/core#Concept"/>
	<skos:prefLabel xml:lang="fr">alluvions</skos:prefLabel>
	<skos:prefLabel xml:lang="en">alluvium</skos:prefLabel>
	<skos:prefLabel xml:lang="it">alluvium</skos:prefLabel>
	<skos:prefLabel xml:lang="nl">alluvium</skos:prefLabel>
	<skos:prefLabel xml:lang="de">Alluvium</skos:prefLabel>
	<skos:prefLabel xml:lang="es">aluvión</skos:prefLabel>
	<skos:prefLabel xml:lang="ar">إطماء</skos:prefLabel>
	<skos:altLabel xml:lang="en">alluvial deposit</skos:altLabel>
	<skos:altLabel xml:lang="es">depósito aluvial</skos:altLabel>
	<skos:altLabel xml:lang="fr">terrasse sédimentaire</skos:altLabel>
	<skos:altLabel xml:lang="it">terreno alluvionale</skos:altLabel>
	<skos:altLabel xml:lang="ar">تَكَوُّن الْغَرِين</skos:altLabel>
	<skos:related rdf:resource="https://ark.frantiq.fr/ark:/26678/pcrt8WIZYG4YAf"/>
	<skos:related rdf:resource="https://ark.frantiq.fr/ark:/26678/crtDBkg0LDMOw"/>
	<skos:related rdf:resource="https://ark.frantiq.fr/ark:/26678/pcrt15tbzh4mdg"/>
	<skos:narrower rdf:resource="https://ark.frantiq.fr/ark:/26678/pcrt2vlSZd64Zk"/>
	<skos:broader rdf:resource="https://ark.frantiq.fr/ark:/26678/pcrtjbpmw8qvrn"/>
	<skos:inScheme rdf:resource="https://ark.frantiq.fr/ark:/26678/TH_1"/>
	<opentheso:memberOf rdf:resource="https://ark.frantiq.fr/ark:/26678/pcrtv66rn9cbv1"/>
	<opentheso:memberOf rdf:resource="https://ark.frantiq.fr/ark:/26678/pcrtnbDLi2FkAj"/>
	<skos:exactMatch rdf:resource="https://www.wikidata.org/wiki/Q6185405"/>
	<skos:exactMatch rdf:resource="http://vocab.getty.edu/aat/300264223"/>
	<dcterms:created rdf:datatype="http://www.w3.org/2001/XMLSchema#date">2007-02-08</dcterms:created>
	<dcterms:modified rdf:datatype="http://www.w3.org/2001/XMLSchema#date">2024-08-23</dcterms:modified>
	<dcterms:identifier>24148</dcterms:identifier>
	<dcterms:contributor>blandine.nouvel</dcterms:contributor>
	<skos:definition xml:lang="en">A deposit of debris (sediment), such as sand, mud, clay, pebbles, silt or gravel, transported by running water and which may settle in the bed of the watercourse or accumulate at the point where the slope breaks.</skos:definition>
	<skos:definition xml:lang="fr">Dépôt de débris (sédiments), tels du sable, de la vase, de l'argile, des galets, du limon ou des graviers, transportés par de l'eau courante et qui peuvent se déposer dans le lit du cours d'eau ou s'accumuler au point de rupture de pente.</skos:definition>
	<skos:historyNote xml:lang="fr">2024-08-22 : révision et traduction de la définition. Remplacement de la traduction en arabe qui correspondait à celle de limon par celle proposée de alluvionnements (OpenTrad 2022), non remplacée.</skos:historyNote>
</rdf:Description>

<rdf:Description rdf:about="https://ark.frantiq.fr/ark:/26678/crtSfObTEvbdn">
	<rdf:type rdf:resource="http://www.w3.org/2004/02/skos/core#Concept"/>
	<skos:prefLabel xml:lang="es">café</skos:prefLabel>
	<skos:prefLabel xml:lang="fr">café (boisson)</skos:prefLabel>
	<skos:prefLabel xml:lang="it">caffè</skos:prefLabel>
	<skos:prefLabel xml:lang="en">coffee</skos:prefLabel>
	<skos:prefLabel xml:lang="de">Kaffee</skos:prefLabel>
	<skos:prefLabel xml:lang="nl">koffie</skos:prefLabel>
	<skos:prefLabel xml:lang="ar">قهوة</skos:prefLabel>
	<skos:related rdf:resource="https://ark.frantiq.fr/ark:/26678/pcrtjt2mr1hq3r"/>
	<skos:related rdf:resource="https://ark.frantiq.fr/ark:/26678/pcrtsxjtz27508"/>
	<skos:related rdf:resource="https://ark.frantiq.fr/ark:/26678/pcrt3k3mbd0n2czwp1w1gcr9"/>
	<skos:broader rdf:resource="https://ark.frantiq.fr/ark:/26678/pcrt6z097U6IUf"/>
	<skos:inScheme rdf:resource="https://ark.frantiq.fr/ark:/26678/TH_1"/>
	<opentheso:memberOf rdf:resource="https://ark.frantiq.fr/ark:/26678/pcrtv66rn9cbv1"/>
	<opentheso:memberOf rdf:resource="https://ark.frantiq.fr/ark:/26678/pcrtnbDLi2FkAj"/>
	<skos:exactMatch rdf:resource="https://catalogue.bnf.fr/ark:/12148/cb119310926"/>
	<skos:exactMatch rdf:resource="https://www.wikidata.org/wiki/Q8486"/>
	<skos:exactMatch rdf:resource="http://vocab.getty.edu/aat/300254662"/>
	<dcterms:created rdf:datatype="http://www.w3.org/2001/XMLSchema#date">2018-12-11</dcterms:created>
	<dcterms:modified rdf:datatype="http://www.w3.org/2001/XMLSchema#date">2024-04-02</dcterms:modified>
	<dcterms:identifier>246224</dcterms:identifier>
	<dcterms:contributor>blandine.nouvel</dcterms:contributor>
	<dcterms:contributor>justine.vincent</dcterms:contributor>
	<skos:definition xml:lang="en">A beverage made from the roasted beans of various varieties of coffee plant.</skos:definition>
	<skos:definition xml:lang="fr">Boisson obtenue à partir des graines torréfiées de diverses variétés de caféier.</skos:definition>
</rdf:Description>

<rdf:Description rdf:about="https://ark.frantiq.fr/ark:/26678/pcrtHJ3vzShqFy">
	<rdf:type rdf:resource="http://www.w3.org/2004/02/skos/core#Concept"/>
	<skos:prefLabel xml:lang="nl">Kalktuf</skos:prefLabel>
	<skos:prefLabel xml:lang="de">Kalktuff</skos:prefLabel>
	<skos:prefLabel xml:lang="es">toba calcárea</skos:prefLabel>
	<skos:prefLabel xml:lang="fr">tuffeau</skos:prefLabel>
	<skos:prefLabel xml:lang="it">tuffeau</skos:prefLabel>
	<skos:prefLabel xml:lang="en">tuffeau stone</skos:prefLabel>
	<skos:prefLabel xml:lang="ar">توفا</skos:prefLabel>
	<skos:altLabel xml:lang="fr">tufeau</skos:altLabel>
	<skos:broader rdf:resource="https://ark.frantiq.fr/ark:/26678/crt9EjSUc0WRF"/>
	<skos:inScheme rdf:resource="https://ark.frantiq.fr/ark:/26678/TH_1"/>
	<opentheso:memberOf rdf:resource="https://ark.frantiq.fr/ark:/26678/pcrtv66rn9cbv1"/>
	<opentheso:memberOf rdf:resource="https://ark.frantiq.fr/ark:/26678/pcrtnbDLi2FkAj"/>
	<skos:exactMatch rdf:resource="https://www.wikidata.org/wiki/Q193685"/>
	<skos:exactMatch rdf:resource="http://vocab.getty.edu/aat/300011712"/>
	<dcterms:created rdf:datatype="http://www.w3.org/2001/XMLSchema#date">2018-12-27</dcterms:created>
	<dcterms:modified rdf:datatype="http://www.w3.org/2001/XMLSchema#date">2023-08-02</dcterms:modified>
	<dcterms:identifier>246276</dcterms:identifier>
	<dcterms:contributor>blandine.nouvel</dcterms:contributor>
	<skos:definition xml:lang="fr">Craie micacée ou sableuse à grain fin, de couleur blanche ou crème parfois jaunâtre, et contenant quelques paillettes de mica blanc (muscovite). Elle est extraite de carrières dans des strates de l'ère secondaire au crétacé supérieur, étage turonien. Cette pierre de taille tendre permet de bâtir et de réaliser les décors typiques de l'architecture de la Renaissance que l'on trouve dans les régions autour de la Loire. (Wikipedia)</skos:definition>
</rdf:Description>

<rdf:Description rdf:about="https://ark.frantiq.fr/ark:/26678/pcrtmxoAFl0eWR">
	<rdf:type rdf:resource="http://www.w3.org/2004/02/skos/core#Concept"/>
	<skos:prefLabel xml:lang="es">esponjolita</skos:prefLabel>
	<skos:prefLabel xml:lang="de">Pläner</skos:prefLabel>
	<skos:prefLabel xml:lang="fr">spongolite</skos:prefLabel>
	<skos:prefLabel xml:lang="it">spongolite</skos:prefLabel>
	<skos:prefLabel xml:lang="en">Spongolite</skos:prefLabel>
	<skos:broader rdf:resource="https://ark.frantiq.fr/ark:/26678/pcrt4N9jrETRto"/>
	<skos:inScheme rdf:resource="https://ark.frantiq.fr/ark:/26678/TH_1"/>
	<opentheso:memberOf rdf:resource="https://ark.frantiq.fr/ark:/26678/pcrtv66rn9cbv1"/>
	<opentheso:memberOf rdf:resource="https://ark.frantiq.fr/ark:/26678/pcrtnbDLi2FkAj"/>
	<skos:exactMatch rdf:resource="https://www.wikidata.org/wiki/Q4438015"/>
	<skos:exactMatch rdf:resource="http://vocab.getty.edu/aat/300380347"/>
	<dcterms:created rdf:datatype="http://www.w3.org/2001/XMLSchema#date">2018-12-27</dcterms:created>
	<dcterms:modified rdf:datatype="http://www.w3.org/2001/XMLSchema#date">2023-08-02</dcterms:modified>
	<dcterms:identifier>246277</dcterms:identifier>
	<dcterms:contributor>blandine.nouvel</dcterms:contributor>
	<skos:definition xml:lang="fr">Roche sédimentaire siliceuse essentiellement formée de spicules d’éponges cimentés. (AAT)</skos:definition>
</rdf:Description>

<rdf:Description rdf:about="https://ark.frantiq.fr/ark:/26678/pcrtRiKgPqvJQO">
	<rdf:type rdf:resource="http://www.w3.org/2004/02/skos/core#Concept"/>
	<skos:prefLabel xml:lang="en">clastic rock</skos:prefLabel>
	<skos:prefLabel xml:lang="es">roca detrítica</skos:prefLabel>
	<skos:prefLabel xml:lang="it">roccia detritica</skos:prefLabel>
	<skos:prefLabel xml:lang="fr">roche détritique</skos:prefLabel>
	<skos:prefLabel xml:lang="de">Trümmergesteine</skos:prefLabel>
	<skos:altLabel xml:lang="es">roca clástica</skos:altLabel>
	<skos:altLabel xml:lang="it">roccia sedimentaria clastica</skos:altLabel>
	<skos:narrower rdf:resource="https://ark.frantiq.fr/ark:/26678/pcrto44p1SaKFn"/>
	<skos:narrower rdf:resource="https://ark.frantiq.fr/ark:/26678/pcrtR1s94Zuaul"/>
	<skos:narrower rdf:resource="https://ark.frantiq.fr/ark:/26678/pcrt0gJ3NT8WlW"/>
	<skos:narrower rdf:resource="https://ark.frantiq.fr/ark:/26678/pcrtzzdfgbqjgxghdgkrghbq"/>
	<skos:narrower rdf:resource="https://ark.frantiq.fr/ark:/26678/pcrtsr9r0hqdgqcdmw5mds91"/>
	<skos:narrower rdf:resource="https://ark.frantiq.fr/ark:/26678/pcrtvhmknj8n0n92z5x2xqqk"/>
	<skos:broader rdf:resource="https://ark.frantiq.fr/ark:/26678/pcrtj3ZcwkArSR"/>
	<skos:inScheme rdf:resource="https://ark.frantiq.fr/ark:/26678/TH_1"/>
	<opentheso:memberOf rdf:resource="https://ark.frantiq.fr/ark:/26678/pcrtv66rn9cbv1"/>
	<opentheso:memberOf rdf:resource="https://ark.frantiq.fr/ark:/26678/pcrtnbDLi2FkAj"/>
	<skos:exactMatch rdf:resource="https://www.wikidata.org/wiki/Q612133"/>
	<skos:exactMatch rdf:resource="http://www.wikidata.org/entity/Q3437543"/>
	<dcterms:created rdf:datatype="http://www.w3.org/2001/XMLSchema#date">2018-12-27</dcterms:created>
	<dcterms:modified rdf:datatype="http://www.w3.org/2001/XMLSchema#date">2023-08-02</dcterms:modified>
	<dcterms:identifier>246278</dcterms:identifier>
	<dcterms:contributor>blandine.nouvel</dcterms:contributor>
	<skos:definition xml:lang="fr">Roche sédimentaire composée d'au moins 50 % de débris. Si les débris sont issus de l'érosion d'autres roches, alors on la qualifie de roche détritique terrigène. Si au contraire les débris sont formés par des squelettes d'organismes vivants alors la roche est qualifiée de biodétritique ou biogénique. (Wikipédia)</skos:definition>
</rdf:Description>

<rdf:Description rdf:about="https://ark.frantiq.fr/ark:/26678/pcrt0gJ3NT8WlW">
	<rdf:type rdf:resource="http://www.w3.org/2004/02/skos/core#Concept"/>
	<skos:prefLabel xml:lang="es">limolita</skos:prefLabel>
	<skos:prefLabel xml:lang="de">Schluffstein</skos:prefLabel>
	<skos:prefLabel xml:lang="fr">siltite</skos:prefLabel>
	<skos:prefLabel xml:lang="it">siltite</skos:prefLabel>
	<skos:prefLabel xml:lang="nl">Siltsteen</skos:prefLabel>
	<skos:prefLabel xml:lang="en">siltstone</skos:prefLabel>
	<skos:prefLabel xml:lang="ar">حجر غربني</skos:prefLabel>
	<skos:altLabel xml:lang="en">aleurolite</skos:altLabel>
	<skos:broader rdf:resource="https://ark.frantiq.fr/ark:/26678/pcrtRiKgPqvJQO"/>
	<skos:inScheme rdf:resource="https://ark.frantiq.fr/ark:/26678/TH_1"/>
	<opentheso:memberOf rdf:resource="https://ark.frantiq.fr/ark:/26678/pcrtv66rn9cbv1"/>
	<opentheso:memberOf rdf:resource="https://ark.frantiq.fr/ark:/26678/pcrtnbDLi2FkAj"/>
	<skos:exactMatch rdf:resource="https://www.wikidata.org/wiki/Q565731"/>
	<skos:exactMatch rdf:resource="http://vocab.getty.edu/aat/300011383"/>
	<dcterms:created rdf:datatype="http://www.w3.org/2001/XMLSchema#date">2018-12-27</dcterms:created>
	<dcterms:modified rdf:datatype="http://www.w3.org/2001/XMLSchema#date">2023-08-02</dcterms:modified>
	<dcterms:identifier>246279</dcterms:identifier>
	<dcterms:contributor>blandine.nouvel</dcterms:contributor>
	<skos:definition xml:lang="fr">Roche sédimentaire détritique consolidée principalement composée de silt. (AAT)</skos:definition>
</rdf:Description>

<rdf:Description rdf:about="https://ark.frantiq.fr/ark:/26678/pcrte3NbmKEKON">
	<rdf:type rdf:resource="http://www.w3.org/2004/02/skos/core#Concept"/>
	<skos:prefLabel xml:lang="es">cera</skos:prefLabel>
	<skos:prefLabel xml:lang="it">cera</skos:prefLabel>
	<skos:prefLabel xml:lang="fr">cire</skos:prefLabel>
	<skos:prefLabel xml:lang="de">Wachs</skos:prefLabel>
	<skos:prefLabel xml:lang="nl">was</skos:prefLabel>
	<skos:prefLabel xml:lang="en">wax</skos:prefLabel>
	<skos:prefLabel xml:lang="ar">شمع</skos:prefLabel>
	<skos:altLabel xml:lang="en">beeswax</skos:altLabel>
	<skos:altLabel xml:lang="fr">cire d'abeille</skos:altLabel>
	<skos:broader rdf:resource="https://ark.frantiq.fr/ark:/26678/pcrtwvFLgSQRs5"/>
	<skos:inScheme rdf:resource="https://ark.frantiq.fr/ark:/26678/TH_1"/>
	<opentheso:memberOf rdf:resource="https://ark.frantiq.fr/ark:/26678/pcrtv66rn9cbv1"/>
	<opentheso:memberOf rdf:resource="https://ark.frantiq.fr/ark:/26678/pcrtnbDLi2FkAj"/>
	<skos:exactMatch rdf:resource="https://www.wikidata.org/wiki/Q143739"/>
	<skos:exactMatch rdf:resource="http://vocab.getty.edu/aat/300014588"/>
	<dcterms:created rdf:datatype="http://www.w3.org/2001/XMLSchema#date">2019-01-02</dcterms:created>
	<dcterms:modified rdf:datatype="http://www.w3.org/2001/XMLSchema#date">2024-11-15</dcterms:modified>
	<dcterms:identifier>246297</dcterms:identifier>
	<dcterms:contributor>blandine.nouvel</dcterms:contributor>
	<dcterms:contributor>justine.vincent</dcterms:contributor>
	<skos:definition xml:lang="en">Natural wax secreted by honey bees to build the combs of their hive in order to store honey, pollen and brood (Wikipedia).</skos:definition>
	<skos:definition xml:lang="fr">Cire naturelle sécrétée par les abeilles à miel pour construire les rayons de leur ruche afin d'y stocker le miel, le pollen et leur couvain. (Wikipédia).</skos:definition>
</rdf:Description>

<rdf:Description rdf:about="https://ark.frantiq.fr/ark:/26678/pcrt4KRB12RYGv">
	<rdf:type rdf:resource="http://www.w3.org/2004/02/skos/core#Concept"/>
	<skos:prefLabel xml:lang="fr">enduit</skos:prefLabel>
	<skos:prefLabel xml:lang="it">intonaco</skos:prefLabel>
	<skos:prefLabel xml:lang="en">plaster</skos:prefLabel>
	<skos:prefLabel xml:lang="de">Putz</skos:prefLabel>
	<skos:prefLabel xml:lang="es">revestimiento</skos:prefLabel>
	<skos:altLabel xml:lang="es">argamasa</skos:altLabel>
	<skos:altLabel xml:lang="es">capa</skos:altLabel>
	<skos:related rdf:resource="https://ark.frantiq.fr/ark:/26678/pcrtFidgusMwk8"/>
	<skos:related rdf:resource="https://ark.frantiq.fr/ark:/26678/pcrtg9q416n5wt"/>
	<skos:related rdf:resource="https://ark.frantiq.fr/ark:/26678/pcrtc4Qh2dBShL"/>
	<skos:narrower rdf:resource="https://ark.frantiq.fr/ark:/26678/pcrtKvRuuvDNp2"/>
	<skos:narrower rdf:resource="https://ark.frantiq.fr/ark:/26678/pcrtsIGcaQ8O7x"/>
	<skos:broader rdf:resource="https://ark.frantiq.fr/ark:/26678/pcrtQuZiT5nYY2"/>
	<skos:inScheme rdf:resource="https://ark.frantiq.fr/ark:/26678/TH_1"/>
	<opentheso:memberOf rdf:resource="https://ark.frantiq.fr/ark:/26678/pcrtv66rn9cbv1"/>
	<opentheso:memberOf rdf:resource="https://ark.frantiq.fr/ark:/26678/pcrtnbDLi2FkAj"/>
	<skos:exactMatch rdf:resource="https://www.wikidata.org/wiki/Q52684119"/>
	<dcterms:created rdf:datatype="http://www.w3.org/2001/XMLSchema#date">2019-01-02</dcterms:created>
	<dcterms:modified rdf:datatype="http://www.w3.org/2001/XMLSchema#date">2023-08-02</dcterms:modified>
	<dcterms:identifier>246300</dcterms:identifier>
	<dcterms:contributor>blandine.nouvel</dcterms:contributor>
	<skos:definition xml:lang="en">Wall cladding, usually made of fine mortar, which may be painted (ARSOL).</skos:definition>
	<skos:definition xml:lang="fr">Revêtement d’un mur, constitué en général de mortier fin, et éventuellement peint (ARSOL).</skos:definition>
</rdf:Description>

<rdf:Description rdf:about="https://ark.frantiq.fr/ark:/26678/pcrtnR5ePytFhO">
	<rdf:type rdf:resource="http://www.w3.org/2004/02/skos/core#Concept"/>
	<skos:prefLabel xml:lang="es">cerámica barnizada</skos:prefLabel>
	<skos:prefLabel xml:lang="it">ceramica verniciata</skos:prefLabel>
	<skos:prefLabel xml:lang="fr">céramique vernissée</skos:prefLabel>
	<skos:prefLabel xml:lang="de">glasierte Keramik</skos:prefLabel>
	<skos:prefLabel xml:lang="en">glazed pottery</skos:prefLabel>
	<skos:related rdf:resource="https://ark.frantiq.fr/ark:/26678/pcrtW48HoxU4NZ"/>
	<skos:related rdf:resource="https://ark.frantiq.fr/ark:/26678/pcrtrVMaTXRHGy"/>
	<skos:related rdf:resource="https://ark.frantiq.fr/ark:/26678/pcrtlZIYhsWrEz"/>
	<skos:related rdf:resource="https://ark.frantiq.fr/ark:/26678/pcrtqlWat99dm0"/>
	<skos:related rdf:resource="https://ark.frantiq.fr/ark:/26678/pcrttS4bFv2ezb"/>
	<skos:related rdf:resource="https://ark.frantiq.fr/ark:/26678/pcrt065IhLltVk"/>
	<skos:related rdf:resource="https://ark.frantiq.fr/ark:/26678/pcrtJXS9PmPlFX"/>
	<skos:related rdf:resource="https://ark.frantiq.fr/ark:/26678/pcrtvmf0n3xbgj"/>
	<skos:related rdf:resource="https://ark.frantiq.fr/ark:/26678/pcrtw7wr6cx38h"/>
	<skos:broader rdf:resource="https://ark.frantiq.fr/ark:/26678/pcrtfx4s0yvSLj"/>
	<skos:inScheme rdf:resource="https://ark.frantiq.fr/ark:/26678/TH_1"/>
	<opentheso:memberOf rdf:resource="https://ark.frantiq.fr/ark:/26678/pcrtv66rn9cbv1"/>
	<opentheso:memberOf rdf:resource="https://ark.frantiq.fr/ark:/26678/pcrtnbDLi2FkAj"/>
	<skos:closeMatch rdf:resource="https://ark.mom.fr/ark:/39676/bib2cpwvwc8jg"/>
	<dcterms:created rdf:datatype="http://www.w3.org/2001/XMLSchema#date">2019-01-03</dcterms:created>
	<dcterms:modified rdf:datatype="http://www.w3.org/2001/XMLSchema#date">2024-11-19</dcterms:modified>
	<dcterms:identifier>246310</dcterms:identifier>
	<dcterms:contributor>blandine.nouvel</dcterms:contributor>
	<dcterms:contributor>justine.vincent</dcterms:contributor>
	<skos:definition xml:lang="fr">Terre cuite recouverte d'engobe&amp;amp;nbsp;blanc ou coloré d'oxydes métalliques, puis d'une glaçure transparente plombifère pour la rendre étanche avant cuisson.</skos:definition>
	<skos:definition xml:lang="en">Fired clay covered with white slip or slip coloured with metallic oxides, then with a transparent lead glaze to make it watertight before firing.</skos:definition>
	<skos:historyNote xml:lang="fr">2024-18-11 : ajout d'une définition.</skos:historyNote>
</rdf:Description>

<rdf:Description rdf:about="https://ark.frantiq.fr/ark:/26678/pcrteWLSy9aARp">
	<rdf:type rdf:resource="http://www.w3.org/2004/02/skos/core#Concept"/>
	<skos:prefLabel xml:lang="it">avorio vegetale</skos:prefLabel>
	<skos:prefLabel xml:lang="nl">corozo</skos:prefLabel>
	<skos:prefLabel xml:lang="fr">ivoire végétal</skos:prefLabel>
	<skos:prefLabel xml:lang="de">Steinnuss</skos:prefLabel>
	<skos:prefLabel xml:lang="es">tagua</skos:prefLabel>
	<skos:prefLabel xml:lang="en">vegetable ivory</skos:prefLabel>
	<skos:altLabel xml:lang="fr">corozo</skos:altLabel>
	<skos:altLabel xml:lang="it">corozo</skos:altLabel>
	<skos:altLabel xml:lang="es">marfil vegetal</skos:altLabel>
	<skos:altLabel xml:lang="it">tagua</skos:altLabel>
	<skos:altLabel xml:lang="en">tagua nut</skos:altLabel>
	<skos:broader rdf:resource="https://ark.frantiq.fr/ark:/26678/pcrtnHxyjOkhJw"/>
	<skos:inScheme rdf:resource="https://ark.frantiq.fr/ark:/26678/TH_1"/>
	<opentheso:memberOf rdf:resource="https://ark.frantiq.fr/ark:/26678/pcrtv66rn9cbv1"/>
	<opentheso:memberOf rdf:resource="https://ark.frantiq.fr/ark:/26678/pcrtnbDLi2FkAj"/>
	<skos:exactMatch rdf:resource="https://www.wikidata.org/wiki/Q1668576"/>
	<skos:exactMatch rdf:resource="http://vocab.getty.edu/aat/300379935"/>
	<dcterms:created rdf:datatype="http://www.w3.org/2001/XMLSchema#date">2019-01-03</dcterms:created>
	<dcterms:modified rdf:datatype="http://www.w3.org/2001/XMLSchema#date">2024-11-15</dcterms:modified>
	<dcterms:identifier>246314</dcterms:identifier>
	<dcterms:contributor>blandine.nouvel</dcterms:contributor>
	<dcterms:contributor>justine.vincent</dcterms:contributor>
	<skos:definition xml:lang="en">Albumen from the fruit of the ivory palm in tropical America (species of the genus Phytelephas) and Africa (species of the genus Hyphaene), used to make small figurines or clothing buttons. (Wikipedia)</skos:definition>
	<skos:definition xml:lang="fr">Albumen du fruit du palmier à ivoire d'Amérique tropicale (espèces de genre Phytelephas) mais aussi d'Afrique (espèces du genre Hyphaene), servant à fabriquer de petites figurines ou des boutons de vêtement. (Wikipedia)</skos:definition>
	<skos:historyNote xml:lang="fr">2024-11-15 : modification de la définition.</skos:historyNote>
</rdf:Description>

<rdf:Description rdf:about="https://ark.frantiq.fr/ark:/26678/pcrtSpItdjR86k">
	<rdf:type rdf:resource="http://www.w3.org/2004/02/skos/core#Concept"/>
	<skos:prefLabel xml:lang="en">Greenstone</skos:prefLabel>
	<skos:prefLabel xml:lang="de">Grünstein</skos:prefLabel>
	<skos:prefLabel xml:lang="es">roca verde</skos:prefLabel>
	<skos:prefLabel xml:lang="it">roccia verde</skos:prefLabel>
	<skos:prefLabel xml:lang="fr">roche verte</skos:prefLabel>
	<skos:related rdf:resource="https://ark.frantiq.fr/ark:/26678/pcrt7pgeXjaSI8"/>
	<skos:related rdf:resource="https://ark.frantiq.fr/ark:/26678/pcrtT7b3IVuYxG"/>
	<skos:related rdf:resource="https://ark.frantiq.fr/ark:/26678/pcrtslVSzVnfeg"/>
	<skos:broader rdf:resource="https://ark.frantiq.fr/ark:/26678/pcrtxybfLE1dkn"/>
	<skos:inScheme rdf:resource="https://ark.frantiq.fr/ark:/26678/TH_1"/>
	<opentheso:memberOf rdf:resource="https://ark.frantiq.fr/ark:/26678/pcrtv66rn9cbv1"/>
	<opentheso:memberOf rdf:resource="https://ark.frantiq.fr/ark:/26678/pcrtnbDLi2FkAj"/>
	<opentheso:memberOf rdf:resource="https://ark.frantiq.fr/ark:/26678/pcrtv0jq332vcq3gxt5m13d5"/>
	<skos:exactMatch rdf:resource="https://www.wikidata.org/wiki/Q5604583"/>
	<skos:exactMatch rdf:resource="http://vocab.getty.edu/aat/300386691"/>
	<dcterms:created rdf:datatype="http://www.w3.org/2001/XMLSchema#date">2019-01-04</dcterms:created>
	<dcterms:modified rdf:datatype="http://www.w3.org/2001/XMLSchema#date">2024-03-21</dcterms:modified>
	<dcterms:identifier>246318</dcterms:identifier>
	<dcterms:contributor>blandine.nouvel</dcterms:contributor>
	<dcterms:contributor>irene.weis</dcterms:contributor>
	<skos:definition xml:lang="en">Generic name for green-hued metamorphic minerals and igneous rocks, such as greenschist, chlorastrolite, serpentines, omphacite, chrysoprase, olivine, nephrite, jade and jadeite (although the latter are better known by these names). (Wikipedia on 4.1.2019)</skos:definition>
	<skos:definition xml:lang="fr">&lt;p&gt;Appellation générique de minéraux et roches ignées métamorphiques de teintes vertes, tels le schiste vert, la chlorastrolite, les serpentines, l'omphacite, la chrysoprase, l'olivine, la néphrite, le jade et la jadéite (bien que ces derniers soient mieux connus sous ces noms). (Wikipedia le 4.1.2019)&lt;/p&gt;</skos:definition>
</rdf:Description>

<rdf:Description rdf:about="https://ark.frantiq.fr/ark:/26678/pcrtQhjRUa1GV8">
	<rdf:type rdf:resource="http://www.w3.org/2004/02/skos/core#Concept"/>
	<skos:prefLabel xml:lang="nl">bitumineuze steenkool</skos:prefLabel>
	<skos:prefLabel xml:lang="en">bituminous coal</skos:prefLabel>
	<skos:prefLabel xml:lang="it">carbone bituminoso</skos:prefLabel>
	<skos:prefLabel xml:lang="fr">houille</skos:prefLabel>
	<skos:prefLabel xml:lang="es">hulla</skos:prefLabel>
	<skos:prefLabel xml:lang="de">Steinkohle</skos:prefLabel>
	<skos:prefLabel xml:lang="ar">فحم قاري</skos:prefLabel>
	<skos:altLabel xml:lang="en">black coal</skos:altLabel>
	<skos:altLabel xml:lang="es">carbón bituminoso</skos:altLabel>
	<skos:altLabel xml:lang="it">carbone nero</skos:altLabel>
	<skos:related rdf:resource="https://ark.frantiq.fr/ark:/26678/pcrtO40ZLI4giK"/>
	<skos:broader rdf:resource="https://ark.frantiq.fr/ark:/26678/pcrtsrWeYcRkNg"/>
	<skos:inScheme rdf:resource="https://ark.frantiq.fr/ark:/26678/TH_1"/>
	<opentheso:memberOf rdf:resource="https://ark.frantiq.fr/ark:/26678/pcrtv66rn9cbv1"/>
	<opentheso:memberOf rdf:resource="https://ark.frantiq.fr/ark:/26678/pcrtnbDLi2FkAj"/>
	<opentheso:memberOf rdf:resource="https://ark.frantiq.fr/ark:/26678/pcrtv0jq332vcq3gxt5m13d5"/>
	<skos:exactMatch rdf:resource="https://www.wikidata.org/wiki/Q732607"/>
	<skos:exactMatch rdf:resource="http://vocab.getty.edu/aat/300015143"/>
	<dcterms:created rdf:datatype="http://www.w3.org/2001/XMLSchema#date">2019-01-06</dcterms:created>
	<dcterms:modified rdf:datatype="http://www.w3.org/2001/XMLSchema#date">2024-11-18</dcterms:modified>
	<dcterms:identifier>246330</dcterms:identifier>
	<dcterms:contributor>blandine.nouvel</dcterms:contributor>
	<dcterms:contributor>irene.weis</dcterms:contributor>
	<dcterms:contributor>justine.vincent</dcterms:contributor>
	<skos:definition xml:lang="en">Sedimentary carbonaceous rock corresponding to a specific quality of coal, intermediate between lignite and anthracite (i.e. 80 to 90% carbon), blackish in colour and derived from the carbonisation of plant organisms and can therefore be used as a fossil fuel. (Wikipedia)</skos:definition>
	<skos:definition xml:lang="fr">Roche carbonée sédimentaire correspondant à une qualité spécifique de charbon, intermédiaire entre le lignite et l'anthracite (soit 80 à 90 % de carbone), de couleur noirâtre et provenant de la carbonisation d'organismes végétaux et peut donc servir de combustible fossile. (Wikipédia)</skos:definition>
</rdf:Description>

<rdf:Description rdf:about="https://ark.frantiq.fr/ark:/26678/pcrt4nvgWBQ59k">
	<rdf:type rdf:resource="http://www.w3.org/2004/02/skos/core#Concept"/>
	<skos:prefLabel xml:lang="fr">béton de tuileau</skos:prefLabel>
	<skos:prefLabel xml:lang="it">cemento romano</skos:prefLabel>
	<skos:prefLabel xml:lang="es">mortero hidráulico</skos:prefLabel>
	<skos:prefLabel xml:lang="en">Roman cement</skos:prefLabel>
	<skos:prefLabel xml:lang="de">Ziegelbruch-Mörtel</skos:prefLabel>
	<skos:altLabel xml:lang="fr">ciment hydraulique romain</skos:altLabel>
	<skos:altLabel xml:lang="es">hormigón hidráulico</skos:altLabel>
	<skos:related rdf:resource="https://ark.frantiq.fr/ark:/26678/pcrt6BaMGq7zE1"/>
	<skos:broader rdf:resource="https://ark.frantiq.fr/ark:/26678/pcrtEWWJvOVoh5"/>
	<skos:inScheme rdf:resource="https://ark.frantiq.fr/ark:/26678/TH_1"/>
	<opentheso:memberOf rdf:resource="https://ark.frantiq.fr/ark:/26678/pcrtv66rn9cbv1"/>
	<opentheso:memberOf rdf:resource="https://ark.frantiq.fr/ark:/26678/pcrtnbDLi2FkAj"/>
	<skos:closeMatch rdf:resource="https://www.wikidata.org/wiki/Q3541924"/>
	<dcterms:created rdf:datatype="http://www.w3.org/2001/XMLSchema#date">2019-01-06</dcterms:created>
	<dcterms:modified rdf:datatype="http://www.w3.org/2001/XMLSchema#date">2024-11-15</dcterms:modified>
	<dcterms:identifier>246332</dcterms:identifier>
	<dcterms:contributor>blandine.nouvel</dcterms:contributor>
	<dcterms:contributor>justine.vincent</dcterms:contributor>
	<skos:scopeNote xml:lang="fr">Mortier romain imperméable réalisé en mélangeant de la chaux, de l'eau, du sable de rivière, de la poudre de tuileaux et parfois de la pouzzolane, l'addition de poudre de tuileaux lui donnant une couleur rougeâtre. (Wikipédia)</skos:scopeNote>
	<skos:scopeNote xml:lang="en">Waterproof Roman mortar made by mixing lime, water, river sand, tile powder and sometimes pozzolan, the addition of tile powder giving it a reddish colour (Wikipedia).</skos:scopeNote>
</rdf:Description>

<rdf:Description rdf:about="https://ark.frantiq.fr/ark:/26678/pcrtGAARv5y4t4">
	<rdf:type rdf:resource="http://www.w3.org/2004/02/skos/core#Concept"/>
	<skos:prefLabel xml:lang="es">marga</skos:prefLabel>
	<skos:prefLabel xml:lang="en">marl</skos:prefLabel>
	<skos:prefLabel xml:lang="it">marna</skos:prefLabel>
	<skos:prefLabel xml:lang="fr">marne (roche)</skos:prefLabel>
	<skos:prefLabel xml:lang="de">Mergel</skos:prefLabel>
	<skos:prefLabel xml:lang="nl">Mergel</skos:prefLabel>
	<skos:altLabel xml:lang="en">marlstone</skos:altLabel>
	<skos:broader rdf:resource="https://ark.frantiq.fr/ark:/26678/pcrtj3ZcwkArSR"/>
	<skos:inScheme rdf:resource="https://ark.frantiq.fr/ark:/26678/TH_1"/>
	<opentheso:memberOf rdf:resource="https://ark.frantiq.fr/ark:/26678/pcrtv66rn9cbv1"/>
	<opentheso:memberOf rdf:resource="https://ark.frantiq.fr/ark:/26678/pcrtnbDLi2FkAj"/>
	<opentheso:memberOf rdf:resource="https://ark.frantiq.fr/ark:/26678/pcrtv0jq332vcq3gxt5m13d5"/>
	<skos:exactMatch rdf:resource="https://catalogue.bnf.fr/ark:/12148/cb12142384m"/>
	<skos:exactMatch rdf:resource="https://www.wikidata.org/wiki/Q184053"/>
	<skos:exactMatch rdf:resource="http://vocab.getty.edu/aat/300010451"/>
	<dcterms:created rdf:datatype="http://www.w3.org/2001/XMLSchema#date">2019-01-06</dcterms:created>
	<dcterms:modified rdf:datatype="http://www.w3.org/2001/XMLSchema#date">2024-03-21</dcterms:modified>
	<dcterms:identifier>246337</dcterms:identifier>
	<dcterms:contributor>blandine.nouvel</dcterms:contributor>
	<dcterms:contributor>irene.weis</dcterms:contributor>
	<skos:definition xml:lang="en">Sedimentary rock, mixture of calcite (CaCO3) and clay in roughly equal proportions (Wikipedia)</skos:definition>
	<skos:definition xml:lang="fr">Roche sédimentaire, mélange de calcite (CaCO3) et d'argile dans des proportions à peu près équivalentes (Wikipedia)</skos:definition>
</rdf:Description>

<rdf:Description rdf:about="https://ark.frantiq.fr/ark:/26678/pcrt4dfh8e5Dpz">
	<rdf:type rdf:resource="http://www.w3.org/2004/02/skos/core#Concept"/>
	<skos:prefLabel xml:lang="fr">écaille de tortue</skos:prefLabel>
	<skos:prefLabel xml:lang="es">escama de tortuga</skos:prefLabel>
	<skos:prefLabel xml:lang="it">scaglia di tartaruga</skos:prefLabel>
	<skos:prefLabel xml:lang="de">Schildpatt</skos:prefLabel>
	<skos:prefLabel xml:lang="en">tortoise shell</skos:prefLabel>
	<skos:prefLabel xml:lang="ar">سلحفاة قذيفة</skos:prefLabel>
	<skos:altLabel xml:lang="it">scuto</skos:altLabel>
	<skos:altLabel xml:lang="en">tortoiseshell</skos:altLabel>
	<skos:related rdf:resource="https://ark.frantiq.fr/ark:/26678/pcrtchfdkzkcs7cwsn1rrxmr"/>
	<skos:related rdf:resource="https://ark.frantiq.fr/ark:/26678/pcrthstz3w0h8t"/>
	<skos:broader rdf:resource="https://ark.frantiq.fr/ark:/26678/pcrtf97bQHDGEd"/>
	<skos:inScheme rdf:resource="https://ark.frantiq.fr/ark:/26678/TH_1"/>
	<opentheso:memberOf rdf:resource="https://ark.frantiq.fr/ark:/26678/pcrtv66rn9cbv1"/>
	<opentheso:memberOf rdf:resource="https://ark.frantiq.fr/ark:/26678/pcrtnbDLi2FkAj"/>
	<skos:broadMatch rdf:resource="https://www.wikidata.org/wiki/Q3577344"/>
	<skos:exactMatch rdf:resource="https://www.wikidata.org/wiki/Q2141546"/>
	<skos:exactMatch rdf:resource="http://vocab.getty.edu/aat/300011837"/>
	<dcterms:created rdf:datatype="http://www.w3.org/2001/XMLSchema#date">2019-02-19</dcterms:created>
	<dcterms:modified rdf:datatype="http://www.w3.org/2001/XMLSchema#date">2023-08-02</dcterms:modified>
	<dcterms:identifier>246404</dcterms:identifier>
	<dcterms:contributor>blandine.nouvel</dcterms:contributor>
	<skos:definition xml:lang="en">Tortoiseshell is a material produced from the shells of large species of tortoise, in particular the hawksbill turtle (caret). (Wikipedia)</skos:definition>
	<skos:definition xml:lang="fr">L'écaille de tortue est un matériau produit à partir des carapaces des grandes espèces de tortues, en particulier de la tortue imbriquée (caret) (Wikipédia)</skos:definition>
</rdf:Description>

<rdf:Description rdf:about="https://ark.frantiq.fr/ark:/26678/pcrtnHxyjOkhJw">
	<rdf:type rdf:resource="http://www.w3.org/2004/02/skos/core#Concept"/>
	<skos:prefLabel xml:lang="es">materia vegetal</skos:prefLabel>
	<skos:prefLabel xml:lang="it">materia vegetale</skos:prefLabel>
	<skos:prefLabel xml:lang="fr">matière végétale</skos:prefLabel>
	<skos:prefLabel xml:lang="en">plant material</skos:prefLabel>
	<skos:prefLabel xml:lang="de">Planzenmaterial</skos:prefLabel>
	<skos:altLabel xml:lang="es">materia de origen vegetal</skos:altLabel>
	<skos:altLabel xml:lang="it">materia di origine vegetale</skos:altLabel>
	<skos:altLabel xml:lang="fr">matière d'origine végétale</skos:altLabel>
	<skos:related rdf:resource="https://ark.frantiq.fr/ark:/26678/pcrtvKH7mF2Oas"/>
	<skos:narrower rdf:resource="https://ark.frantiq.fr/ark:/26678/pcrtMr3tb79bV8"/>
	<skos:narrower rdf:resource="https://ark.frantiq.fr/ark:/26678/pcrtrxL50B7yNx"/>
	<skos:narrower rdf:resource="https://ark.frantiq.fr/ark:/26678/pcrt0TJJTrHkN1"/>
	<skos:narrower rdf:resource="https://ark.frantiq.fr/ark:/26678/crtAzyiJhxOQN"/>
	<skos:narrower rdf:resource="https://ark.frantiq.fr/ark:/26678/crtXXzLndpZbJ"/>
	<skos:narrower rdf:resource="https://ark.frantiq.fr/ark:/26678/crtiorG06KeFt"/>
	<skos:narrower rdf:resource="https://ark.frantiq.fr/ark:/26678/pcrtc6RmFQxFuS"/>
	<skos:narrower rdf:resource="https://ark.frantiq.fr/ark:/26678/pcrteWLSy9aARp"/>
	<skos:narrower rdf:resource="https://ark.frantiq.fr/ark:/26678/pcrt6v8xrc8qrd"/>
	<skos:narrower rdf:resource="https://ark.frantiq.fr/ark:/26678/pcrt0k0f3qbw4r"/>
	<skos:narrower rdf:resource="https://ark.frantiq.fr/ark:/26678/pcrtKcuT7Kh6vX"/>
	<skos:narrower rdf:resource="https://ark.frantiq.fr/ark:/26678/pcrtFwQpNgFwZo"/>
	<skos:broader rdf:resource="https://ark.frantiq.fr/ark:/26678/pcrtwvFLgSQRs5"/>
	<skos:inScheme rdf:resource="https://ark.frantiq.fr/ark:/26678/TH_1"/>
	<opentheso:memberOf rdf:resource="https://ark.frantiq.fr/ark:/26678/pcrtv66rn9cbv1"/>
	<opentheso:memberOf rdf:resource="https://ark.frantiq.fr/ark:/26678/pcrtnbDLi2FkAj"/>
	<skos:exactMatch rdf:resource="https://www.wikidata.org/wiki/Q28969364"/>
	<dcterms:created rdf:datatype="http://www.w3.org/2001/XMLSchema#date">2019-02-19</dcterms:created>
	<dcterms:modified rdf:datatype="http://www.w3.org/2001/XMLSchema#date">2023-08-02</dcterms:modified>
	<dcterms:identifier>246405</dcterms:identifier>
	<dcterms:contributor>blandine.nouvel</dcterms:contributor>
	<skos:definition xml:lang="en">Material derived from plants.</skos:definition>
	<skos:definition xml:lang="fr">Matière dérivée des plantes.</skos:definition>
</rdf:Description>

<rdf:Description rdf:about="https://ark.frantiq.fr/ark:/26678/pcrt8ZW1DEoUSn">
	<rdf:type rdf:resource="http://www.w3.org/2004/02/skos/core#Concept"/>
	<skos:prefLabel xml:lang="fr">andouiller</skos:prefLabel>
	<skos:prefLabel xml:lang="de">Geweihsprosse</skos:prefLabel>
	<skos:prefLabel xml:lang="it">palchi</skos:prefLabel>
	<skos:prefLabel xml:lang="ar">punta (cervo)</skos:prefLabel>
	<skos:prefLabel xml:lang="es">punta (ciervo)</skos:prefLabel>
	<skos:prefLabel xml:lang="en">tine</skos:prefLabel>
	<skos:altLabel xml:lang="fr">cor (cervidé)</skos:altLabel>
	<skos:narrower rdf:resource="https://ark.frantiq.fr/ark:/26678/pcrtGET4B08135"/>
	<skos:narrower rdf:resource="https://ark.frantiq.fr/ark:/26678/pcrtakOKgw0Q9M"/>
	<skos:narrower rdf:resource="https://ark.frantiq.fr/ark:/26678/pcrt30jDOWeS57"/>
	<skos:narrower rdf:resource="https://ark.frantiq.fr/ark:/26678/pcrtg0xc91xffk"/>
	<skos:broader rdf:resource="https://ark.frantiq.fr/ark:/26678/pcrtmmQBSGulBN"/>
	<skos:inScheme rdf:resource="https://ark.frantiq.fr/ark:/26678/TH_1"/>
	<opentheso:memberOf rdf:resource="https://ark.frantiq.fr/ark:/26678/pcrtv66rn9cbv1"/>
	<opentheso:memberOf rdf:resource="https://ark.frantiq.fr/ark:/26678/pcrtnbDLi2FkAj"/>
	<skos:exactMatch rdf:resource="https://www.wikidata.org/wiki/Q834007"/>
	<dcterms:created rdf:datatype="http://www.w3.org/2001/XMLSchema#date">2019-02-19</dcterms:created>
	<dcterms:modified rdf:datatype="http://www.w3.org/2001/XMLSchema#date">2023-08-02</dcterms:modified>
	<dcterms:identifier>246406</dcterms:identifier>
	<dcterms:contributor>blandine.nouvel</dcterms:contributor>
	<skos:definition xml:lang="en">Antler branch (cnrtl)</skos:definition>
	<skos:definition xml:lang="fr">Branche des bois de cervidés (cnrtl)</skos:definition>
</rdf:Description>

<rdf:Description rdf:about="https://ark.frantiq.fr/ark:/26678/pcrtGET4B08135">
	<rdf:type rdf:resource="http://www.w3.org/2004/02/skos/core#Concept"/>
	<skos:prefLabel xml:lang="fr">andouiller basilaire (cerf)</skos:prefLabel>
	<skos:prefLabel xml:lang="de">Augsprosse (Hirsch)</skos:prefLabel>
	<skos:prefLabel xml:lang="en">brow tine (red deer)</skos:prefLabel>
	<skos:prefLabel xml:lang="es">luchadera (ciervo)</skos:prefLabel>
	<skos:prefLabel xml:lang="it">pugnale (cervo)</skos:prefLabel>
	<skos:altLabel xml:lang="es">candil basal</skos:altLabel>
	<skos:broader rdf:resource="https://ark.frantiq.fr/ark:/26678/pcrt8ZW1DEoUSn"/>
	<skos:inScheme rdf:resource="https://ark.frantiq.fr/ark:/26678/TH_1"/>
	<opentheso:memberOf rdf:resource="https://ark.frantiq.fr/ark:/26678/pcrtv66rn9cbv1"/>
	<opentheso:memberOf rdf:resource="https://ark.frantiq.fr/ark:/26678/pcrtnbDLi2FkAj"/>
	<dcterms:created rdf:datatype="http://www.w3.org/2001/XMLSchema#date">2019-02-19</dcterms:created>
	<dcterms:modified rdf:datatype="http://www.w3.org/2001/XMLSchema#date">2023-08-02</dcterms:modified>
	<dcterms:identifier>246407</dcterms:identifier>
	<dcterms:contributor>blandine.nouvel</dcterms:contributor>
	<skos:definition xml:lang="en">First andouiller of a deer antler (Averbouh et al., 2016).</skos:definition>
	<skos:definition xml:lang="fr">Premier andouiller d'un bois de cerf (Averbouh et al., 2016).</skos:definition>
</rdf:Description>

<rdf:Description rdf:about="https://ark.frantiq.fr/ark:/26678/pcrtakOKgw0Q9M">
	<rdf:type rdf:resource="http://www.w3.org/2004/02/skos/core#Concept"/>
	<skos:prefLabel xml:lang="fr">andouiller central (cerf)</skos:prefLabel>
	<skos:prefLabel xml:lang="it">mediano (cervo)</skos:prefLabel>
	<skos:prefLabel xml:lang="de">Mittelsprosse (Hirsch)</skos:prefLabel>
	<skos:prefLabel xml:lang="es">punta media</skos:prefLabel>
	<skos:prefLabel xml:lang="en">trez tine (red deer)</skos:prefLabel>
	<skos:altLabel xml:lang="es">candil medio</skos:altLabel>
	<skos:broader rdf:resource="https://ark.frantiq.fr/ark:/26678/pcrt8ZW1DEoUSn"/>
	<skos:inScheme rdf:resource="https://ark.frantiq.fr/ark:/26678/TH_1"/>
	<opentheso:memberOf rdf:resource="https://ark.frantiq.fr/ark:/26678/pcrtv66rn9cbv1"/>
	<opentheso:memberOf rdf:resource="https://ark.frantiq.fr/ark:/26678/pcrtnbDLi2FkAj"/>
	<dcterms:created rdf:datatype="http://www.w3.org/2001/XMLSchema#date">2019-02-19</dcterms:created>
	<dcterms:modified rdf:datatype="http://www.w3.org/2001/XMLSchema#date">2023-08-02</dcterms:modified>
	<dcterms:identifier>246408</dcterms:identifier>
	<dcterms:contributor>blandine.nouvel</dcterms:contributor>
	<skos:definition xml:lang="en">Central antler at the junction of the two staves of a deer antler (Averbouh et al., 2016).</skos:definition>
	<skos:definition xml:lang="fr">Andouiller central à la jonction des deux merrains d'un bois de cerf (Averbouh et al., 2016).</skos:definition>
</rdf:Description>

<rdf:Description rdf:about="https://ark.frantiq.fr/ark:/26678/pcrt30jDOWeS57">
	<rdf:type rdf:resource="http://www.w3.org/2004/02/skos/core#Concept"/>
	<skos:prefLabel xml:lang="fr">andouiller d'oeil (renne)</skos:prefLabel>
	<skos:prefLabel xml:lang="de">Augsprosse (Rentier)</skos:prefLabel>
	<skos:prefLabel xml:lang="en">brow tine (red deer)</skos:prefLabel>
	<skos:prefLabel xml:lang="es">candil de ojo (reno)</skos:prefLabel>
	<skos:prefLabel xml:lang="it">oculare (renna)</skos:prefLabel>
	<skos:altLabel xml:lang="en">first tine</skos:altLabel>
	<skos:broader rdf:resource="https://ark.frantiq.fr/ark:/26678/pcrt8ZW1DEoUSn"/>
	<skos:inScheme rdf:resource="https://ark.frantiq.fr/ark:/26678/TH_1"/>
	<opentheso:memberOf rdf:resource="https://ark.frantiq.fr/ark:/26678/pcrtv66rn9cbv1"/>
	<opentheso:memberOf rdf:resource="https://ark.frantiq.fr/ark:/26678/pcrtnbDLi2FkAj"/>
	<dcterms:created rdf:datatype="http://www.w3.org/2001/XMLSchema#date">2019-02-19</dcterms:created>
	<dcterms:modified rdf:datatype="http://www.w3.org/2001/XMLSchema#date">2023-08-02</dcterms:modified>
	<dcterms:identifier>246409</dcterms:identifier>
	<dcterms:contributor>blandine.nouvel</dcterms:contributor>
	<skos:definition xml:lang="en">First antler of a reindeer (Averbouh et al., 2016).</skos:definition>
	<skos:definition xml:lang="fr">Premier andouiller d'un bois de renne (Averbouh et al., 2016).</skos:definition>
</rdf:Description>

<rdf:Description rdf:about="https://ark.frantiq.fr/ark:/26678/pcrtIDUn8EY3Bx">
	<rdf:type rdf:resource="http://www.w3.org/2004/02/skos/core#Concept"/>
	<skos:prefLabel xml:lang="de">Abwurfstange</skos:prefLabel>
	<skos:prefLabel xml:lang="es">asta de muda</skos:prefLabel>
	<skos:prefLabel xml:lang="fr">bois de chute</skos:prefLabel>
	<skos:prefLabel xml:lang="it">palco da caduta</skos:prefLabel>
	<skos:prefLabel xml:lang="en">shed antler</skos:prefLabel>
	<skos:broader rdf:resource="https://ark.frantiq.fr/ark:/26678/pcrtmmQBSGulBN"/>
	<skos:inScheme rdf:resource="https://ark.frantiq.fr/ark:/26678/TH_1"/>
	<opentheso:memberOf rdf:resource="https://ark.frantiq.fr/ark:/26678/pcrtv66rn9cbv1"/>
	<opentheso:memberOf rdf:resource="https://ark.frantiq.fr/ark:/26678/pcrtnbDLi2FkAj"/>
	<dcterms:created rdf:datatype="http://www.w3.org/2001/XMLSchema#date">2019-02-19</dcterms:created>
	<dcterms:modified rdf:datatype="http://www.w3.org/2001/XMLSchema#date">2023-08-02</dcterms:modified>
	<dcterms:identifier>246410</dcterms:identifier>
	<dcterms:contributor>blandine.nouvel</dcterms:contributor>
	<skos:definition xml:lang="en">Naturally fallen antler (wikipedia).</skos:definition>
	<skos:definition xml:lang="fr">Bois de cervidé tombé naturellement (wikipedia).</skos:definition>
</rdf:Description>

<rdf:Description rdf:about="https://ark.frantiq.fr/ark:/26678/pcrtMBkRt9d0we">
	<rdf:type rdf:resource="http://www.w3.org/2004/02/skos/core#Concept"/>
	<skos:prefLabel xml:lang="en">antler from a hunted animal</skos:prefLabel>
	<skos:prefLabel xml:lang="es">asta de masacre</skos:prefLabel>
	<skos:prefLabel xml:lang="fr">bois de massacre</skos:prefLabel>
	<skos:prefLabel xml:lang="it">palco d'abbattimento</skos:prefLabel>
	<skos:prefLabel xml:lang="de">schädelechtes Geweih</skos:prefLabel>
	<skos:altLabel xml:lang="es">asta de caza</skos:altLabel>
	<skos:broader rdf:resource="https://ark.frantiq.fr/ark:/26678/pcrtmmQBSGulBN"/>
	<skos:inScheme rdf:resource="https://ark.frantiq.fr/ark:/26678/TH_1"/>
	<opentheso:memberOf rdf:resource="https://ark.frantiq.fr/ark:/26678/pcrtv66rn9cbv1"/>
	<opentheso:memberOf rdf:resource="https://ark.frantiq.fr/ark:/26678/pcrtnbDLi2FkAj"/>
	<dcterms:created rdf:datatype="http://www.w3.org/2001/XMLSchema#date">2019-02-19</dcterms:created>
	<dcterms:modified rdf:datatype="http://www.w3.org/2001/XMLSchema#date">2023-08-02</dcterms:modified>
	<dcterms:identifier>246411</dcterms:identifier>
	<dcterms:contributor>blandine.nouvel</dcterms:contributor>
	<skos:definition xml:lang="en">Deer antler, often with frontal bone (cnrtl)</skos:definition>
	<skos:definition xml:lang="fr">Bois de cerf, souvent muni de l'os frontal (cnrtl)</skos:definition>
</rdf:Description>

<rdf:Description rdf:about="https://ark.frantiq.fr/ark:/26678/pcrtQ3dQ0kEMW9">
	<rdf:type rdf:resource="http://www.w3.org/2004/02/skos/core#Concept"/>
	<skos:prefLabel xml:lang="fr">chevillure</skos:prefLabel>
	<skos:prefLabel xml:lang="es">clavija</skos:prefLabel>
	<skos:prefLabel xml:lang="it">forca</skos:prefLabel>
	<skos:prefLabel xml:lang="de">Hintersprosse</skos:prefLabel>
	<skos:prefLabel xml:lang="en">trez tine (red deer)</skos:prefLabel>
	<skos:altLabel xml:lang="it">corna</skos:altLabel>
	<skos:broader rdf:resource="https://ark.frantiq.fr/ark:/26678/pcrtmmQBSGulBN"/>
	<skos:inScheme rdf:resource="https://ark.frantiq.fr/ark:/26678/TH_1"/>
	<opentheso:memberOf rdf:resource="https://ark.frantiq.fr/ark:/26678/pcrtv66rn9cbv1"/>
	<opentheso:memberOf rdf:resource="https://ark.frantiq.fr/ark:/26678/pcrtnbDLi2FkAj"/>
	<dcterms:created rdf:datatype="http://www.w3.org/2001/XMLSchema#date">2019-02-19</dcterms:created>
	<dcterms:modified rdf:datatype="http://www.w3.org/2001/XMLSchema#date">2023-08-02</dcterms:modified>
	<dcterms:identifier>246412</dcterms:identifier>
	<dcterms:contributor>blandine.nouvel</dcterms:contributor>
	<skos:definition xml:lang="en">Third andouiller of the antlers of stag, fallow deer and roe deer; set of andouillers following the third (cnrtl)</skos:definition>
	<skos:definition xml:lang="fr">Troisième andouiller des bois du cerf, du daim, du chevreuil ; ensemble des andouillers venant après le troisième (cnrtl)</skos:definition>
</rdf:Description>

<rdf:Description rdf:about="https://ark.frantiq.fr/ark:/26678/pcrtvMpoEaUF3q">
	<rdf:type rdf:resource="http://www.w3.org/2004/02/skos/core#Concept"/>
	<skos:prefLabel xml:lang="it">daga (cervidi)</skos:prefLabel>
	<skos:prefLabel xml:lang="fr">dague (cervidé)</skos:prefLabel>
	<skos:prefLabel xml:lang="en">pricket (deer)</skos:prefLabel>
	<skos:prefLabel xml:lang="de">Spieß (Hirschartige)</skos:prefLabel>
	<skos:prefLabel xml:lang="es">vara (cérvido)</skos:prefLabel>
	<skos:broader rdf:resource="https://ark.frantiq.fr/ark:/26678/pcrtmmQBSGulBN"/>
	<skos:inScheme rdf:resource="https://ark.frantiq.fr/ark:/26678/TH_1"/>
	<opentheso:memberOf rdf:resource="https://ark.frantiq.fr/ark:/26678/pcrtv66rn9cbv1"/>
	<opentheso:memberOf rdf:resource="https://ark.frantiq.fr/ark:/26678/pcrtnbDLi2FkAj"/>
	<dcterms:created rdf:datatype="http://www.w3.org/2001/XMLSchema#date">2019-02-19</dcterms:created>
	<dcterms:modified rdf:datatype="http://www.w3.org/2001/XMLSchema#date">2023-08-02</dcterms:modified>
	<dcterms:identifier>246413</dcterms:identifier>
	<dcterms:contributor>blandine.nouvel</dcterms:contributor>
	<skos:definition xml:lang="en">Small horn growing in the second year of a young fallow deer or stag.</skos:definition>
	<skos:definition xml:lang="fr">Petite corne poussant la deuxième année d'un jeune daim ou cerf</skos:definition>
</rdf:Description>

<rdf:Description rdf:about="https://ark.frantiq.fr/ark:/26678/pcrtjGSMcDpz8A">
	<rdf:type rdf:resource="http://www.w3.org/2004/02/skos/core#Concept"/>
	<skos:prefLabel xml:lang="es">corona</skos:prefLabel>
	<skos:prefLabel xml:lang="it">corona</skos:prefLabel>
	<skos:prefLabel xml:lang="de">distaler Geweihabschnitt</skos:prefLabel>
	<skos:prefLabel xml:lang="fr">empaumure</skos:prefLabel>
	<skos:prefLabel xml:lang="en">fork segment</skos:prefLabel>
	<skos:altLabel xml:lang="en">palmated antlers</skos:altLabel>
	<skos:altLabel xml:lang="en">palmation</skos:altLabel>
	<skos:broader rdf:resource="https://ark.frantiq.fr/ark:/26678/pcrtmmQBSGulBN"/>
	<skos:inScheme rdf:resource="https://ark.frantiq.fr/ark:/26678/TH_1"/>
	<opentheso:memberOf rdf:resource="https://ark.frantiq.fr/ark:/26678/pcrtv66rn9cbv1"/>
	<opentheso:memberOf rdf:resource="https://ark.frantiq.fr/ark:/26678/pcrtnbDLi2FkAj"/>
	<skos:exactMatch rdf:resource="https://www.wikidata.org/wiki/Q16631991"/>
	<dcterms:created rdf:datatype="http://www.w3.org/2001/XMLSchema#date">2019-02-19</dcterms:created>
	<dcterms:modified rdf:datatype="http://www.w3.org/2001/XMLSchema#date">2023-08-02</dcterms:modified>
	<dcterms:identifier>246414</dcterms:identifier>
	<dcterms:contributor>blandine.nouvel</dcterms:contributor>
	<skos:definition xml:lang="en">Part of the antlers of a deer or roe deer, widening like the palm of the hand and bearing three, four or five antlers, arranged like fingers (cnrtl)</skos:definition>
	<skos:definition xml:lang="fr">Partie des bois du cerf ou du chevreuil, s'élargissant comme la paume de la main et portant trois, quatre ou cinq andouillers, rangés comme des doigts (cnrtl)</skos:definition>
</rdf:Description>

<rdf:Description rdf:about="https://ark.frantiq.fr/ark:/26678/pcrtahNd1oALhh">
	<rdf:type rdf:resource="http://www.w3.org/2004/02/skos/core#Concept"/>
	<skos:prefLabel xml:lang="es">candil</skos:prefLabel>
	<skos:prefLabel xml:lang="fr">épois</skos:prefLabel>
	<skos:prefLabel xml:lang="de">Kronenenden</skos:prefLabel>
	<skos:prefLabel xml:lang="it">punta</skos:prefLabel>
	<skos:prefLabel xml:lang="en">tine tip</skos:prefLabel>
	<skos:altLabel xml:lang="en">antler tip</skos:altLabel>
	<skos:broader rdf:resource="https://ark.frantiq.fr/ark:/26678/pcrtmmQBSGulBN"/>
	<skos:inScheme rdf:resource="https://ark.frantiq.fr/ark:/26678/TH_1"/>
	<opentheso:memberOf rdf:resource="https://ark.frantiq.fr/ark:/26678/pcrtv66rn9cbv1"/>
	<opentheso:memberOf rdf:resource="https://ark.frantiq.fr/ark:/26678/pcrtnbDLi2FkAj"/>
	<dcterms:created rdf:datatype="http://www.w3.org/2001/XMLSchema#date">2019-02-19</dcterms:created>
	<dcterms:modified rdf:datatype="http://www.w3.org/2001/XMLSchema#date">2023-08-02</dcterms:modified>
	<dcterms:identifier>246415</dcterms:identifier>
	<dcterms:contributor>blandine.nouvel</dcterms:contributor>
	<skos:definition xml:lang="en">Horn (andouiller) which finishes the empaumure of a deer antler (cnrtl)</skos:definition>
	<skos:definition xml:lang="fr">Cor (andouiller) qui termine l'empaumure d'un bois de cerf (cnrtl)</skos:definition>
</rdf:Description>

<rdf:Description rdf:about="https://ark.frantiq.fr/ark:/26678/pcrtSd50sRXgiH">
	<rdf:type rdf:resource="http://www.w3.org/2004/02/skos/core#Concept"/>
	<skos:prefLabel xml:lang="es">gotera (cérvido)</skos:prefLabel>
	<skos:prefLabel xml:lang="fr">gouttière (cervidé)</skos:prefLabel>
	<skos:prefLabel xml:lang="en">groove (deer)</skos:prefLabel>
	<skos:prefLabel xml:lang="de">Rinne an der Oberfläche des Geweihs</skos:prefLabel>
	<skos:prefLabel xml:lang="it">solco (cervidi)</skos:prefLabel>
	<skos:altLabel xml:lang="en">antler groove</skos:altLabel>
	<skos:broader rdf:resource="https://ark.frantiq.fr/ark:/26678/pcrtmmQBSGulBN"/>
	<skos:inScheme rdf:resource="https://ark.frantiq.fr/ark:/26678/TH_1"/>
	<opentheso:memberOf rdf:resource="https://ark.frantiq.fr/ark:/26678/pcrtv66rn9cbv1"/>
	<opentheso:memberOf rdf:resource="https://ark.frantiq.fr/ark:/26678/pcrtnbDLi2FkAj"/>
	<dcterms:created rdf:datatype="http://www.w3.org/2001/XMLSchema#date">2019-02-19</dcterms:created>
	<dcterms:modified rdf:datatype="http://www.w3.org/2001/XMLSchema#date">2023-08-02</dcterms:modified>
	<dcterms:identifier>246416</dcterms:identifier>
	<dcterms:contributor>blandine.nouvel</dcterms:contributor>
	<skos:definition xml:lang="en">Long, deep, more or less pronounced longitudinal grooves visible at the base of deer antlers (cnrtl)</skos:definition>
	<skos:definition xml:lang="fr">Rainures longitudinales, plus ou moins marquées, longues et profondes, visibles à la base des bois des cerfs (cnrtl)</skos:definition>
</rdf:Description>

<rdf:Description rdf:about="https://ark.frantiq.fr/ark:/26678/pcrtFEZaa6oTIS">
	<rdf:type rdf:resource="http://www.w3.org/2004/02/skos/core#Concept"/>
	<skos:prefLabel xml:lang="it">medaglione (cervidi)</skos:prefLabel>
	<skos:prefLabel xml:lang="fr">médaillon (cervidé)</skos:prefLabel>
	<skos:prefLabel xml:lang="en">medallion (deer)</skos:prefLabel>
	<skos:prefLabel xml:lang="es">medallón (cérvido)</skos:prefLabel>
	<skos:prefLabel xml:lang="de">Petschaft</skos:prefLabel>
	<skos:altLabel xml:lang="en">antler medallion</skos:altLabel>
	<skos:broader rdf:resource="https://ark.frantiq.fr/ark:/26678/pcrtmmQBSGulBN"/>
	<skos:inScheme rdf:resource="https://ark.frantiq.fr/ark:/26678/TH_1"/>
	<opentheso:memberOf rdf:resource="https://ark.frantiq.fr/ark:/26678/pcrtv66rn9cbv1"/>
	<opentheso:memberOf rdf:resource="https://ark.frantiq.fr/ark:/26678/pcrtnbDLi2FkAj"/>
	<dcterms:created rdf:datatype="http://www.w3.org/2001/XMLSchema#date">2019-02-19</dcterms:created>
	<dcterms:modified rdf:datatype="http://www.w3.org/2001/XMLSchema#date">2023-08-02</dcterms:modified>
	<dcterms:identifier>246417</dcterms:identifier>
	<dcterms:contributor>blandine.nouvel</dcterms:contributor>
	<skos:definition xml:lang="en">The proximal end of the antler which enables it to be attached to the pedicle (Averbouh, 2000).</skos:definition>
	<skos:definition xml:lang="fr">Extrémité proximale du bois de cerf qui lui permet d'être attaché au pédicule (Averbouh, 2000).</skos:definition>
</rdf:Description>

<rdf:Description rdf:about="https://ark.frantiq.fr/ark:/26678/pcrtaSs5GKhSA7">
	<rdf:type rdf:resource="http://www.w3.org/2004/02/skos/core#Concept"/>
	<skos:prefLabel xml:lang="en">beam (red deer)</skos:prefLabel>
	<skos:prefLabel xml:lang="de">Geweihstange (Hirsch)</skos:prefLabel>
	<skos:prefLabel xml:lang="fr">merrain</skos:prefLabel>
	<skos:prefLabel xml:lang="es">percha (ciervo)</skos:prefLabel>
	<skos:prefLabel xml:lang="it">stanga (cervo)</skos:prefLabel>
	<skos:broader rdf:resource="https://ark.frantiq.fr/ark:/26678/pcrtmmQBSGulBN"/>
	<skos:inScheme rdf:resource="https://ark.frantiq.fr/ark:/26678/TH_1"/>
	<opentheso:memberOf rdf:resource="https://ark.frantiq.fr/ark:/26678/pcrtv66rn9cbv1"/>
	<opentheso:memberOf rdf:resource="https://ark.frantiq.fr/ark:/26678/pcrtnbDLi2FkAj"/>
	<dcterms:created rdf:datatype="http://www.w3.org/2001/XMLSchema#date">2019-02-19</dcterms:created>
	<dcterms:modified rdf:datatype="http://www.w3.org/2001/XMLSchema#date">2023-08-02</dcterms:modified>
	<dcterms:identifier>246418</dcterms:identifier>
	<dcterms:contributor>blandine.nouvel</dcterms:contributor>
	<skos:definition xml:lang="en">Central stem of the antlers of deer and other animals with antlers on their heads (cnrtl)</skos:definition>
	<skos:definition xml:lang="fr">Tige centrale de la ramure du cerf et des autres animaux dont la tête est ornée d'un bois (cnrtl)</skos:definition>
</rdf:Description>

<rdf:Description rdf:about="https://ark.frantiq.fr/ark:/26678/pcrtzJhR1OwU8P">
	<rdf:type rdf:resource="http://www.w3.org/2004/02/skos/core#Concept"/>
	<skos:prefLabel xml:lang="en">burr (deer)</skos:prefLabel>
	<skos:prefLabel xml:lang="fr">meule (cervidé)</skos:prefLabel>
	<skos:prefLabel xml:lang="de">Rosenstück</skos:prefLabel>
	<skos:prefLabel xml:lang="es">roseta (cérvido)</skos:prefLabel>
	<skos:prefLabel xml:lang="it">rosetta (cervidi)</skos:prefLabel>
	<skos:altLabel xml:lang="it">rosa (cervidi)</skos:altLabel>
	<skos:broader rdf:resource="https://ark.frantiq.fr/ark:/26678/pcrtmmQBSGulBN"/>
	<skos:inScheme rdf:resource="https://ark.frantiq.fr/ark:/26678/TH_1"/>
	<opentheso:memberOf rdf:resource="https://ark.frantiq.fr/ark:/26678/pcrtv66rn9cbv1"/>
	<opentheso:memberOf rdf:resource="https://ark.frantiq.fr/ark:/26678/pcrtnbDLi2FkAj"/>
	<dcterms:created rdf:datatype="http://www.w3.org/2001/XMLSchema#date">2019-02-19</dcterms:created>
	<dcterms:modified rdf:datatype="http://www.w3.org/2001/XMLSchema#date">2023-08-02</dcterms:modified>
	<dcterms:identifier>246419</dcterms:identifier>
	<dcterms:contributor>blandine.nouvel</dcterms:contributor>
	<skos:definition xml:lang="en">Antler outgrowth at the junction of the stave and the pivots in Cervidae (cnrtl)</skos:definition>
	<skos:definition xml:lang="fr">Excroissance des bois apparaissant à la jonction du merrain et des pivots chez les Cervidés (cnrtl)</skos:definition>
</rdf:Description>

<rdf:Description rdf:about="https://ark.frantiq.fr/ark:/26678/pcrthKDSnMjAR9">
	<rdf:type rdf:resource="http://www.w3.org/2004/02/skos/core#Concept"/>
	<skos:prefLabel xml:lang="de">Geweihschaufel</skos:prefLabel>
	<skos:prefLabel xml:lang="it">pala (cervidi)</skos:prefLabel>
	<skos:prefLabel xml:lang="es">palma (cérvido)</skos:prefLabel>
	<skos:prefLabel xml:lang="en">palm (antler)</skos:prefLabel>
	<skos:prefLabel xml:lang="fr">palme (cervidé)</skos:prefLabel>
	<skos:altLabel xml:lang="es">pala</skos:altLabel>
	<skos:altLabel xml:lang="en">palmate antlers (deer)</skos:altLabel>
	<skos:broader rdf:resource="https://ark.frantiq.fr/ark:/26678/pcrtmmQBSGulBN"/>
	<skos:inScheme rdf:resource="https://ark.frantiq.fr/ark:/26678/TH_1"/>
	<opentheso:memberOf rdf:resource="https://ark.frantiq.fr/ark:/26678/pcrtv66rn9cbv1"/>
	<opentheso:memberOf rdf:resource="https://ark.frantiq.fr/ark:/26678/pcrtnbDLi2FkAj"/>
	<dcterms:created rdf:datatype="http://www.w3.org/2001/XMLSchema#date">2019-02-19</dcterms:created>
	<dcterms:modified rdf:datatype="http://www.w3.org/2001/XMLSchema#date">2023-08-02</dcterms:modified>
	<dcterms:identifier>246421</dcterms:identifier>
	<dcterms:contributor>blandine.nouvel</dcterms:contributor>
	<skos:definition xml:lang="en">Part of the empaumure of a reindeer antler (Averbouh, 2000).</skos:definition>
	<skos:definition xml:lang="fr">Partie de l'empaumure d'un bois de renne (Averbouh, 2000).</skos:definition>
</rdf:Description>

<rdf:Description rdf:about="https://ark.frantiq.fr/ark:/26678/pcrthu1vFbVQHO">
	<rdf:type rdf:resource="http://www.w3.org/2004/02/skos/core#Concept"/>
	<skos:prefLabel xml:lang="en">basal and beam segment (reindeer)</skos:prefLabel>
	<skos:prefLabel xml:lang="de">Geweihstange (Rentier)</skos:prefLabel>
	<skos:prefLabel xml:lang="es">percha (reno)</skos:prefLabel>
	<skos:prefLabel xml:lang="fr">perche (renne)</skos:prefLabel>
	<skos:prefLabel xml:lang="it">stanga (renna)</skos:prefLabel>
	<skos:broader rdf:resource="https://ark.frantiq.fr/ark:/26678/pcrtmmQBSGulBN"/>
	<skos:inScheme rdf:resource="https://ark.frantiq.fr/ark:/26678/TH_1"/>
	<opentheso:memberOf rdf:resource="https://ark.frantiq.fr/ark:/26678/pcrtv66rn9cbv1"/>
	<opentheso:memberOf rdf:resource="https://ark.frantiq.fr/ark:/26678/pcrtnbDLi2FkAj"/>
	<dcterms:created rdf:datatype="http://www.w3.org/2001/XMLSchema#date">2019-02-19</dcterms:created>
	<dcterms:modified rdf:datatype="http://www.w3.org/2001/XMLSchema#date">2023-08-02</dcterms:modified>
	<dcterms:identifier>246422</dcterms:identifier>
	<dcterms:contributor>blandine.nouvel</dcterms:contributor>
	<skos:definition xml:lang="en">Central part of a reindeer antler (Averbouh, 2000).</skos:definition>
	<skos:definition xml:lang="fr">Parties centrale d'un bois de renne (Averbouh, 2000).</skos:definition>
</rdf:Description>

<rdf:Description rdf:about="https://ark.frantiq.fr/ark:/26678/pcrtgym8WF8J02">
	<rdf:type rdf:resource="http://www.w3.org/2004/02/skos/core#Concept"/>
	<skos:prefLabel xml:lang="en">pearling</skos:prefLabel>
	<skos:prefLabel xml:lang="fr">pelure</skos:prefLabel>
	<skos:prefLabel xml:lang="es">perlado</skos:prefLabel>
	<skos:prefLabel xml:lang="it">perlatura</skos:prefLabel>
	<skos:prefLabel xml:lang="de">Perlung</skos:prefLabel>
	<skos:broader rdf:resource="https://ark.frantiq.fr/ark:/26678/pcrtmmQBSGulBN"/>
	<skos:inScheme rdf:resource="https://ark.frantiq.fr/ark:/26678/TH_1"/>
	<opentheso:memberOf rdf:resource="https://ark.frantiq.fr/ark:/26678/pcrtv66rn9cbv1"/>
	<opentheso:memberOf rdf:resource="https://ark.frantiq.fr/ark:/26678/pcrtnbDLi2FkAj"/>
	<dcterms:created rdf:datatype="http://www.w3.org/2001/XMLSchema#date">2019-02-19</dcterms:created>
	<dcterms:modified rdf:datatype="http://www.w3.org/2001/XMLSchema#date">2023-08-02</dcterms:modified>
	<dcterms:identifier>246423</dcterms:identifier>
	<dcterms:contributor>blandine.nouvel</dcterms:contributor>
	<skos:definition xml:lang="en">Small bump forming on the deer's antlers (cnrtl)</skos:definition>
	<skos:definition xml:lang="fr">Petite bosse se formant sur les andouillers du cerf (cnrtl)</skos:definition>
</rdf:Description>

<rdf:Description rdf:about="https://ark.frantiq.fr/ark:/26678/pcrtvmZ325vcRc">
	<rdf:type rdf:resource="http://www.w3.org/2004/02/skos/core#Concept"/>
	<skos:prefLabel xml:lang="en">pedicle</skos:prefLabel>
	<skos:prefLabel xml:lang="es">pedículo (cérvido)</skos:prefLabel>
	<skos:prefLabel xml:lang="fr">pivot (cervidé)</skos:prefLabel>
	<skos:prefLabel xml:lang="it">stelo (cervidi)</skos:prefLabel>
	<skos:prefLabel xml:lang="de">Stirnzapfen</skos:prefLabel>
	<skos:altLabel xml:lang="en">pedicle of the frontal bone</skos:altLabel>
	<skos:altLabel xml:lang="fr">pédicule</skos:altLabel>
	<skos:broader rdf:resource="https://ark.frantiq.fr/ark:/26678/pcrtmmQBSGulBN"/>
	<skos:inScheme rdf:resource="https://ark.frantiq.fr/ark:/26678/TH_1"/>
	<opentheso:memberOf rdf:resource="https://ark.frantiq.fr/ark:/26678/pcrtv66rn9cbv1"/>
	<opentheso:memberOf rdf:resource="https://ark.frantiq.fr/ark:/26678/pcrtnbDLi2FkAj"/>
	<dcterms:created rdf:datatype="http://www.w3.org/2001/XMLSchema#date">2019-02-19</dcterms:created>
	<dcterms:modified rdf:datatype="http://www.w3.org/2001/XMLSchema#date">2023-08-02</dcterms:modified>
	<dcterms:identifier>246424</dcterms:identifier>
	<dcterms:contributor>blandine.nouvel</dcterms:contributor>
	<skos:definition xml:lang="en">Each of the two bony bulges on either side of the frontal process that support the antlers (cnrtl).</skos:definition>
	<skos:definition xml:lang="fr">Chacun des deux bourrelets osseux situés de part et d'autre de l'apophyse du frontal et qui portent les bois [du cervidé] (cnrtl)</skos:definition>
</rdf:Description>

<rdf:Description rdf:about="https://ark.frantiq.fr/ark:/26678/pcrtPkEBaAzwGn">
	<rdf:type rdf:resource="http://www.w3.org/2004/02/skos/core#Concept"/>
	<skos:prefLabel xml:lang="it">solco (osso)</skos:prefLabel>
	<skos:prefLabel xml:lang="es">sulco (hueso)</skos:prefLabel>
	<skos:prefLabel xml:lang="en">sulcus</skos:prefLabel>
	<skos:prefLabel xml:lang="de">Sulcus</skos:prefLabel>
	<skos:prefLabel xml:lang="fr">sulcus (os)</skos:prefLabel>
	<skos:altLabel xml:lang="de">Knochenrinne</skos:altLabel>
	<skos:altLabel xml:lang="fr">sillon (os)</skos:altLabel>
	<skos:broader rdf:resource="https://ark.frantiq.fr/ark:/26678/pcrtmmQBSGulBN"/>
	<skos:inScheme rdf:resource="https://ark.frantiq.fr/ark:/26678/TH_1"/>
	<opentheso:memberOf rdf:resource="https://ark.frantiq.fr/ark:/26678/pcrtv66rn9cbv1"/>
	<opentheso:memberOf rdf:resource="https://ark.frantiq.fr/ark:/26678/pcrtnbDLi2FkAj"/>
	<dcterms:created rdf:datatype="http://www.w3.org/2001/XMLSchema#date">2019-02-19</dcterms:created>
	<dcterms:modified rdf:datatype="http://www.w3.org/2001/XMLSchema#date">2024-11-15</dcterms:modified>
	<dcterms:identifier>246425</dcterms:identifier>
	<dcterms:contributor>blandine.nouvel</dcterms:contributor>
	<dcterms:contributor>justine.vincent</dcterms:contributor>
	<skos:definition xml:lang="fr">&amp;amp;nbsp;Relief creux étroit et allongé entre deux éléments anatomiques.</skos:definition>
	<skos:definition xml:lang="en">Narrow, elongated hollow relief between two anatomical elements.</skos:definition>
	<skos:historyNote xml:lang="fr">&lt;span style= color: rgb(32, 33, 34); &gt;2024-11-15 : ajout d'une définition.&lt;/span&gt;</skos:historyNote>
</rdf:Description>

<rdf:Description rdf:about="https://ark.frantiq.fr/ark:/26678/pcrtMStphi4T4j">
	<rdf:type rdf:resource="http://www.w3.org/2004/02/skos/core#Concept"/>
	<skos:prefLabel xml:lang="en">bez tine (red deer)</skos:prefLabel>
	<skos:prefLabel xml:lang="es">contraluchadera (ciervo)</skos:prefLabel>
	<skos:prefLabel xml:lang="de">Eissprosse (Hirsch)</skos:prefLabel>
	<skos:prefLabel xml:lang="it">invernino (cervo)</skos:prefLabel>
	<skos:prefLabel xml:lang="fr">sur-andouiller</skos:prefLabel>
	<skos:altLabel xml:lang="it">ago</skos:altLabel>
	<skos:altLabel xml:lang="fr">andouiller de fer</skos:altLabel>
	<skos:altLabel xml:lang="es">candil de hierro</skos:altLabel>
	<skos:altLabel xml:lang="fr">second andouiller</skos:altLabel>
	<skos:broader rdf:resource="https://ark.frantiq.fr/ark:/26678/pcrtmmQBSGulBN"/>
	<skos:inScheme rdf:resource="https://ark.frantiq.fr/ark:/26678/TH_1"/>
	<opentheso:memberOf rdf:resource="https://ark.frantiq.fr/ark:/26678/pcrtv66rn9cbv1"/>
	<opentheso:memberOf rdf:resource="https://ark.frantiq.fr/ark:/26678/pcrtnbDLi2FkAj"/>
	<dcterms:created rdf:datatype="http://www.w3.org/2001/XMLSchema#date">2019-02-19</dcterms:created>
	<dcterms:modified rdf:datatype="http://www.w3.org/2001/XMLSchema#date">2023-08-02</dcterms:modified>
	<dcterms:identifier>246426</dcterms:identifier>
	<dcterms:contributor>blandine.nouvel</dcterms:contributor>
	<skos:definition xml:lang="en">Second andouiller (cnrtl)</skos:definition>
	<skos:definition xml:lang="fr">Second andouiller (cnrtl)</skos:definition>
</rdf:Description>

<rdf:Description rdf:about="https://ark.frantiq.fr/ark:/26678/pcrttQ1swNeBVe">
	<rdf:type rdf:resource="http://www.w3.org/2004/02/skos/core#Concept"/>
	<skos:prefLabel xml:lang="fr">cément</skos:prefLabel>
	<skos:prefLabel xml:lang="es">cemento</skos:prefLabel>
	<skos:prefLabel xml:lang="it">cemento dentale</skos:prefLabel>
	<skos:prefLabel xml:lang="en">cementum</skos:prefLabel>
	<skos:prefLabel xml:lang="de">Zahnzement</skos:prefLabel>
	<skos:related rdf:resource="https://ark.frantiq.fr/ark:/26678/pcrtwvFLgSQRs5"/>
	<skos:broader rdf:resource="https://ark.frantiq.fr/ark:/26678/pcrthA4kIWMu84"/>
	<skos:inScheme rdf:resource="https://ark.frantiq.fr/ark:/26678/TH_1"/>
	<opentheso:memberOf rdf:resource="https://ark.frantiq.fr/ark:/26678/pcrtv66rn9cbv1"/>
	<opentheso:memberOf rdf:resource="https://ark.frantiq.fr/ark:/26678/pcrtLminDZvylD"/>
	<opentheso:memberOf rdf:resource="https://ark.frantiq.fr/ark:/26678/pcrtnbDLi2FkAj"/>
	<skos:exactMatch rdf:resource="https://www.wikidata.org/wiki/Q848382"/>
	<dcterms:created rdf:datatype="http://www.w3.org/2001/XMLSchema#date">2019-02-19</dcterms:created>
	<dcterms:modified rdf:datatype="http://www.w3.org/2001/XMLSchema#date">2023-08-02</dcterms:modified>
	<dcterms:identifier>246427</dcterms:identifier>
	<dcterms:contributor>blandine.nouvel</dcterms:contributor>
	<skos:definition xml:lang="fr">Tissu minéralisé engainant les racines [des dents], de l'apex au collet (cnrtl)</skos:definition>
</rdf:Description>

<rdf:Description rdf:about="https://ark.frantiq.fr/ark:/26678/pcrtMj9v33qudS">
	<rdf:type rdf:resource="http://www.w3.org/2004/02/skos/core#Concept"/>
	<skos:prefLabel xml:lang="en">dentin</skos:prefLabel>
	<skos:prefLabel xml:lang="de">Dentin</skos:prefLabel>
	<skos:prefLabel xml:lang="es">dentina</skos:prefLabel>
	<skos:prefLabel xml:lang="it">dentina</skos:prefLabel>
	<skos:prefLabel xml:lang="fr">dentine</skos:prefLabel>
	<skos:altLabel xml:lang="en">dentine</skos:altLabel>
	<skos:related rdf:resource="https://ark.frantiq.fr/ark:/26678/pcrthA4kIWMu84"/>
	<skos:related rdf:resource="https://ark.frantiq.fr/ark:/26678/pcrt1zVFrqhSh2"/>
	<skos:broader rdf:resource="https://ark.frantiq.fr/ark:/26678/pcrtf97bQHDGEd"/>
	<skos:inScheme rdf:resource="https://ark.frantiq.fr/ark:/26678/TH_1"/>
	<opentheso:memberOf rdf:resource="https://ark.frantiq.fr/ark:/26678/pcrtv66rn9cbv1"/>
	<opentheso:memberOf rdf:resource="https://ark.frantiq.fr/ark:/26678/pcrtnbDLi2FkAj"/>
	<skos:exactMatch rdf:resource="https://catalogue.bnf.fr/ark:/12148/cb11931857w"/>
	<skos:exactMatch rdf:resource="https://www.wikidata.org/wiki/Q189637"/>
	<skos:exactMatch rdf:resource="http://vocab.getty.edu/aat/300191881"/>
	<dcterms:created rdf:datatype="http://www.w3.org/2001/XMLSchema#date">2019-02-19</dcterms:created>
	<dcterms:modified rdf:datatype="http://www.w3.org/2001/XMLSchema#date">2024-11-15</dcterms:modified>
	<dcterms:identifier>246428</dcterms:identifier>
	<dcterms:contributor>blandine.nouvel</dcterms:contributor>
	<dcterms:contributor>justine.vincent</dcterms:contributor>
	<skos:definition xml:lang="en">Major substance making up the tooth and, more generally, the dental organ. (from Wikipedia)</skos:definition>
	<skos:definition xml:lang="fr">Substance majoritaire constituant la dent et plus généralement l'organe dentaire. (d'ap. Wikipedia)</skos:definition>
	<skos:scopeNote xml:lang="fr">Terme utilisé pour l'homme exclusivement. Son équivalent pour les autres animaux est l'ivoire.</skos:scopeNote>
</rdf:Description>

<rdf:Description rdf:about="https://ark.frantiq.fr/ark:/26678/pcrtbKNE16SNWh">
	<rdf:type rdf:resource="http://www.w3.org/2004/02/skos/core#Concept"/>
	<skos:prefLabel xml:lang="it">astuccio corneo</skos:prefLabel>
	<skos:prefLabel xml:lang="es">estuche córneo</skos:prefLabel>
	<skos:prefLabel xml:lang="fr">étui corné</skos:prefLabel>
	<skos:prefLabel xml:lang="de">Hornscheide</skos:prefLabel>
	<skos:prefLabel xml:lang="en">horn sheath</skos:prefLabel>
	<skos:altLabel xml:lang="fr">boite cornée</skos:altLabel>
	<skos:altLabel xml:lang="fr">sabot (corne)</skos:altLabel>
	<skos:broader rdf:resource="https://ark.frantiq.fr/ark:/26678/pcrtU6YoUalie6"/>
	<skos:inScheme rdf:resource="https://ark.frantiq.fr/ark:/26678/TH_1"/>
	<opentheso:memberOf rdf:resource="https://ark.frantiq.fr/ark:/26678/pcrtv66rn9cbv1"/>
	<opentheso:memberOf rdf:resource="https://ark.frantiq.fr/ark:/26678/pcrtnbDLi2FkAj"/>
	<dcterms:created rdf:datatype="http://www.w3.org/2001/XMLSchema#date">2019-02-19</dcterms:created>
	<dcterms:modified rdf:datatype="http://www.w3.org/2001/XMLSchema#date">2024-11-15</dcterms:modified>
	<dcterms:identifier>246429</dcterms:identifier>
	<dcterms:contributor>blandine.nouvel</dcterms:contributor>
	<dcterms:contributor>justine.vincent</dcterms:contributor>
	<skos:definition xml:lang="en">A substance similar to animal horns, found in particular under horses' feet. (cnrtl)</skos:definition>
	<skos:definition xml:lang="fr">Substance de même nature que celle des cornes d'animaux, qui se trouve en particulier sous les pieds des chevaux (cnrtl)</skos:definition>
</rdf:Description>

<rdf:Description rdf:about="https://ark.frantiq.fr/ark:/26678/pcrtcyhN8uK1oY">
	<rdf:type rdf:resource="http://www.w3.org/2004/02/skos/core#Concept"/>
	<skos:prefLabel xml:lang="en">compact bone</skos:prefLabel>
	<skos:prefLabel xml:lang="de">kompaktes Knochengewebe</skos:prefLabel>
	<skos:prefLabel xml:lang="es">tejido óseo compacto</skos:prefLabel>
	<skos:prefLabel xml:lang="it">tessuto osseo compatto</skos:prefLabel>
	<skos:prefLabel xml:lang="fr">tissu osseux compact</skos:prefLabel>
	<skos:broader rdf:resource="https://ark.frantiq.fr/ark:/26678/pcrtGg8L8TLNtc"/>
	<skos:inScheme rdf:resource="https://ark.frantiq.fr/ark:/26678/TH_1"/>
	<opentheso:memberOf rdf:resource="https://ark.frantiq.fr/ark:/26678/pcrtv66rn9cbv1"/>
	<opentheso:memberOf rdf:resource="https://ark.frantiq.fr/ark:/26678/pcrtnbDLi2FkAj"/>
	<skos:broadMatch rdf:resource="https://www.wikidata.org/wiki/Q83692"/>
	<dcterms:created rdf:datatype="http://www.w3.org/2001/XMLSchema#date">2019-02-19</dcterms:created>
	<dcterms:modified rdf:datatype="http://www.w3.org/2001/XMLSchema#date">2024-11-15</dcterms:modified>
	<dcterms:identifier>246430</dcterms:identifier>
	<dcterms:contributor>blandine.nouvel</dcterms:contributor>
	<dcterms:contributor>justine.vincent</dcterms:contributor>
	<skos:definition xml:lang="en">Dense bony part forming a sleeve.</skos:definition>
	<skos:definition xml:lang="fr">Partie osseuse dense formant un manchon.</skos:definition>
	<skos:historyNote xml:lang="fr">2024-11-15 : ajout d'une définition.</skos:historyNote>
</rdf:Description>

<rdf:Description rdf:about="https://ark.frantiq.fr/ark:/26678/pcrtZWUH1HnqXo">
	<rdf:type rdf:resource="http://www.w3.org/2004/02/skos/core#Concept"/>
	<skos:prefLabel xml:lang="en">cancellous bone</skos:prefLabel>
	<skos:prefLabel xml:lang="de">spongiöses Knochengewebe</skos:prefLabel>
	<skos:prefLabel xml:lang="es">tejido óseo esponjoso</skos:prefLabel>
	<skos:prefLabel xml:lang="it">tessuto osseo spugnoso</skos:prefLabel>
	<skos:prefLabel xml:lang="fr">tissu osseux spongieux</skos:prefLabel>
	<skos:altLabel xml:lang="en">spongy bone</skos:altLabel>
	<skos:broader rdf:resource="https://ark.frantiq.fr/ark:/26678/pcrtGg8L8TLNtc"/>
	<skos:inScheme rdf:resource="https://ark.frantiq.fr/ark:/26678/TH_1"/>
	<opentheso:memberOf rdf:resource="https://ark.frantiq.fr/ark:/26678/pcrtv66rn9cbv1"/>
	<opentheso:memberOf rdf:resource="https://ark.frantiq.fr/ark:/26678/pcrtnbDLi2FkAj"/>
	<skos:broadMatch rdf:resource="https://www.wikidata.org/wiki/Q83692"/>
	<dcterms:created rdf:datatype="http://www.w3.org/2001/XMLSchema#date">2019-02-19</dcterms:created>
	<dcterms:modified rdf:datatype="http://www.w3.org/2001/XMLSchema#date">2024-11-15</dcterms:modified>
	<dcterms:identifier>246431</dcterms:identifier>
	<dcterms:contributor>blandine.nouvel</dcterms:contributor>
	<dcterms:contributor>justine.vincent</dcterms:contributor>
	<skos:definition xml:lang="en">Bone matrix found mainly in short bones and flat bones (sternum) and in the epiphyses of long bones (wp).</skos:definition>
	<skos:definition xml:lang="fr">Matrice osseuse présente essentiellement dans les os courts et les os plats (sternum) ainsi que dans les épiphyses des os longs. (wp)</skos:definition>
	<skos:historyNote xml:lang="fr">2024-11-15 : modification de la définition.</skos:historyNote>
</rdf:Description>

<rdf:Description rdf:about="https://ark.frantiq.fr/ark:/26678/pcrtM0mkbZiNnN">
	<rdf:type rdf:resource="http://www.w3.org/2004/02/skos/core#Concept"/>
	<skos:prefLabel xml:lang="de">Ägyptisch Blau</skos:prefLabel>
	<skos:prefLabel xml:lang="es">azul egipcio</skos:prefLabel>
	<skos:prefLabel xml:lang="fr">bleu égyptien</skos:prefLabel>
	<skos:prefLabel xml:lang="it">blu egiziano</skos:prefLabel>
	<skos:prefLabel xml:lang="en">Egyptian blue</skos:prefLabel>
	<skos:prefLabel xml:lang="nl">Egyptisch blauw</skos:prefLabel>
	<skos:prefLabel xml:lang="ar">أزرق مصري</skos:prefLabel>
	<skos:altLabel xml:lang="en">calcium copper silicate</skos:altLabel>
	<skos:altLabel xml:lang="fr">fritte de bleu égyptien</skos:altLabel>
	<skos:altLabel xml:lang="es">silicato de cobre</skos:altLabel>
	<skos:related rdf:resource="https://ark.frantiq.fr/ark:/26678/pcrtFUux6JWTnV"/>
	<skos:broader rdf:resource="https://ark.frantiq.fr/ark:/26678/pcrtGzQPnntJa1"/>
	<skos:inScheme rdf:resource="https://ark.frantiq.fr/ark:/26678/TH_1"/>
	<opentheso:memberOf rdf:resource="https://ark.frantiq.fr/ark:/26678/pcrtv66rn9cbv1"/>
	<opentheso:memberOf rdf:resource="https://ark.frantiq.fr/ark:/26678/pcrtnbDLi2FkAj"/>
	<skos:exactMatch rdf:resource="https://www.wikidata.org/wiki/Q253181"/>
	<skos:exactMatch rdf:resource="http://vocab.getty.edu/aat/300013280"/>
	<dcterms:created rdf:datatype="http://www.w3.org/2001/XMLSchema#date">2019-04-16</dcterms:created>
	<dcterms:modified rdf:datatype="http://www.w3.org/2001/XMLSchema#date">2023-08-02</dcterms:modified>
	<dcterms:identifier>246523</dcterms:identifier>
	<dcterms:contributor>blandine.nouvel</dcterms:contributor>
	<skos:definition xml:lang="it">pigmento inorganico (Wikidata)</skos:definition>
	<skos:definition xml:lang="es">pigmento inorgánico usado por los antiguos egipcios (Wikidata)</skos:definition>
	<skos:definition xml:lang="fr">Pigment produit à partir de « verre » (cuisson avec un fondant d'un minerai de cuivre1, sables siliceux, roches calcaires) coloré écrasé en fine poudre. Il est considéré comme le premier pigment synthétique. De couleur bleu, il est utilisé par les anciens Égyptiens notamment sur les sarcophages, sculptures, papyrus, peintures murales à partir de la IVe dynastie. Aussi connu sous le nom de fritte de bleu égyptien et désigné à l'époque de « lapis-lazuli », en référence à la couleur bleue de la pierre (Wikipedia)</skos:definition>
</rdf:Description>

<rdf:Description rdf:about="https://ark.frantiq.fr/ark:/26678/pcrt6BaMGq7zE1">
	<rdf:type rdf:resource="http://www.w3.org/2004/02/skos/core#Concept"/>
	<skos:prefLabel xml:lang="it">terracotta schiacciata</skos:prefLabel>
	<skos:prefLabel xml:lang="es">tiesto</skos:prefLabel>
	<skos:prefLabel xml:lang="en">tile fragment</skos:prefLabel>
	<skos:prefLabel xml:lang="fr">tuileau</skos:prefLabel>
	<skos:prefLabel xml:lang="de">Ziegelbruch</skos:prefLabel>
	<skos:altLabel xml:lang="it">frammento di terracotta</skos:altLabel>
	<skos:altLabel xml:lang="en">roman brick fragment</skos:altLabel>
	<skos:related rdf:resource="https://ark.frantiq.fr/ark:/26678/pcrtE6otPtwi8P"/>
	<skos:related rdf:resource="https://ark.frantiq.fr/ark:/26678/pcrt4nvgWBQ59k"/>
	<skos:broader rdf:resource="https://ark.frantiq.fr/ark:/26678/pcrtQuZiT5nYY2"/>
	<skos:inScheme rdf:resource="https://ark.frantiq.fr/ark:/26678/TH_1"/>
	<opentheso:memberOf rdf:resource="https://ark.frantiq.fr/ark:/26678/pcrtv66rn9cbv1"/>
	<opentheso:memberOf rdf:resource="https://ark.frantiq.fr/ark:/26678/pcrtnbDLi2FkAj"/>
	<skos:exactMatch rdf:resource="https://www.wikidata.org/wiki/Q3541924"/>
	<dcterms:created rdf:datatype="http://www.w3.org/2001/XMLSchema#date">2019-09-30</dcterms:created>
	<dcterms:modified rdf:datatype="http://www.w3.org/2001/XMLSchema#date">2023-08-02</dcterms:modified>
	<dcterms:identifier>246797</dcterms:identifier>
	<dcterms:contributor>blandine.nouvel</dcterms:contributor>
	<skos:definition xml:lang="en">Thin element (the thickness of a tile), the edge of which is used to line a hearth (Lar. 2019)</skos:definition>
	<skos:definition xml:lang="fr">Élément mince (de l'épaisseur d'une tuile) dont la tranche est utilisée pour le revêtement d'un âtre. (Lar. 2019)</skos:definition>
</rdf:Description>

<rdf:Description rdf:about="https://ark.frantiq.fr/ark:/26678/pcrtmoM3SzhDcB">
	<rdf:type rdf:resource="http://www.w3.org/2004/02/skos/core#Concept"/>
	<skos:prefLabel xml:lang="it">madreperla</skos:prefLabel>
	<skos:prefLabel xml:lang="en">mother-of-pearl</skos:prefLabel>
	<skos:prefLabel xml:lang="es">nácar</skos:prefLabel>
	<skos:prefLabel xml:lang="fr">nacre</skos:prefLabel>
	<skos:prefLabel xml:lang="nl">parelmoer</skos:prefLabel>
	<skos:prefLabel xml:lang="de">Perlmutt</skos:prefLabel>
	<skos:prefLabel xml:lang="ru">Перламутр</skos:prefLabel>
	<skos:prefLabel xml:lang="he">אם הפנינה</skos:prefLabel>
	<skos:prefLabel xml:lang="ar">عرق اللؤلؤ</skos:prefLabel>
	<skos:altLabel xml:lang="es">madreperla</skos:altLabel>
	<skos:altLabel xml:lang="en">nacre</skos:altLabel>
	<skos:narrower rdf:resource="https://ark.frantiq.fr/ark:/26678/pcrtupN3PAxWw0"/>
	<skos:broader rdf:resource="https://ark.frantiq.fr/ark:/26678/pcrtf97bQHDGEd"/>
	<skos:inScheme rdf:resource="https://ark.frantiq.fr/ark:/26678/TH_1"/>
	<opentheso:memberOf rdf:resource="https://ark.frantiq.fr/ark:/26678/pcrtv66rn9cbv1"/>
	<opentheso:memberOf rdf:resource="https://ark.frantiq.fr/ark:/26678/pcrtnbDLi2FkAj"/>
	<skos:exactMatch rdf:resource="https://catalogue.bnf.fr/ark:/12148/cb12307892b"/>
	<skos:exactMatch rdf:resource="https://www.wikidata.org/wiki/Q215865"/>
	<skos:exactMatch rdf:resource="http://vocab.getty.edu/aat/300011835"/>
	<dcterms:created rdf:datatype="http://www.w3.org/2001/XMLSchema#date">2007-02-08</dcterms:created>
	<dcterms:modified rdf:datatype="http://www.w3.org/2001/XMLSchema#date">2023-08-02</dcterms:modified>
	<dcterms:identifier>24863</dcterms:identifier>
	<dcterms:contributor>blandine.nouvel</dcterms:contributor>
	<skos:definition xml:lang="fr">Matière calcaire (mélange de conchyoline et de carbonate de calcium), blanche, dure, à reflets irisés, sécrétée par certains mollusques et revêtant l'intérieur de leur coquille, formée de lamelles superposées parallèles, utilisée en bijouterie, en tabletterie et en marqueterie (cnrtl)&lt;/br&gt;revêtement intérieur de certaines coquilles de mollusque aux reflets irisés (Wikidata)</skos:definition>
	<skos:definition xml:lang="de">Natürliches Verbundmaterial (Wikidata)</skos:definition>
	<skos:definition xml:lang="en">organic-inorganic composite material produced by some molluscs (Wikidata)</skos:definition>
	<skos:definition xml:lang="es">sustancia orgánico-inorgánica (Wikidata)</skos:definition>
</rdf:Description>

<rdf:Description rdf:about="https://ark.frantiq.fr/ark:/26678/pcrt2xkdh2n373">
	<rdf:type rdf:resource="http://www.w3.org/2004/02/skos/core#Concept"/>
	<skos:prefLabel xml:lang="de">Kalbsleder</skos:prefLabel>
	<skos:prefLabel xml:lang="es">papel vitela</skos:prefLabel>
	<skos:prefLabel xml:lang="fr">vélin</skos:prefLabel>
	<skos:prefLabel xml:lang="en">vellum</skos:prefLabel>
	<skos:prefLabel xml:lang="it">vellum</skos:prefLabel>
	<skos:altLabel xml:lang="it">cartapecora</skos:altLabel>
	<skos:altLabel xml:lang="it">carta pecudina</skos:altLabel>
	<skos:broader rdf:resource="https://ark.frantiq.fr/ark:/26678/pcrtMt1immB5H5"/>
	<skos:inScheme rdf:resource="https://ark.frantiq.fr/ark:/26678/TH_1"/>
	<opentheso:memberOf rdf:resource="https://ark.frantiq.fr/ark:/26678/pcrtv66rn9cbv1"/>
	<opentheso:memberOf rdf:resource="https://ark.frantiq.fr/ark:/26678/pcrtnbDLi2FkAj"/>
	<skos:exactMatch rdf:resource="https://www.wikidata.org/wiki/Q378274"/>
	<dcterms:created rdf:datatype="http://www.w3.org/2001/XMLSchema#date">2019-11-29</dcterms:created>
	<dcterms:modified rdf:datatype="http://www.w3.org/2001/XMLSchema#date">2023-08-02</dcterms:modified>
	<dcterms:identifier>250848</dcterms:identifier>
	<dcterms:contributor>blandine.nouvel</dcterms:contributor>
	<skos:definition xml:lang="en">Skin of stillborn calf (or other animal, such as lamb or kid), prepared for writing, illustration, printing or binding, smoother and finer than ordinary parchment (cntrl)</skos:definition>
	<skos:definition xml:lang="fr">Peau de veau mort-né (ou d'un autre animal, comme l'agneau ou le chevreau), préparée pour l'écriture, l'illustration, l'imprimerie ou la reliure, plus lisse et plus fine que le parchemin ordinaire (cntrl)</skos:definition>
</rdf:Description>

<rdf:Description rdf:about="https://ark.frantiq.fr/ark:/26678/pcrt6v8xrc8qrd">
	<rdf:type rdf:resource="http://www.w3.org/2004/02/skos/core#Concept"/>
	<skos:prefLabel xml:lang="it">carta</skos:prefLabel>
	<skos:prefLabel xml:lang="es">papel</skos:prefLabel>
	<skos:prefLabel xml:lang="en">paper</skos:prefLabel>
	<skos:prefLabel xml:lang="fr">papier</skos:prefLabel>
	<skos:prefLabel xml:lang="de">Papier</skos:prefLabel>
	<skos:broader rdf:resource="https://ark.frantiq.fr/ark:/26678/pcrtnHxyjOkhJw"/>
	<skos:inScheme rdf:resource="https://ark.frantiq.fr/ark:/26678/TH_1"/>
	<opentheso:memberOf rdf:resource="https://ark.frantiq.fr/ark:/26678/pcrtv66rn9cbv1"/>
	<opentheso:memberOf rdf:resource="https://ark.frantiq.fr/ark:/26678/pcrtnbDLi2FkAj"/>
	<skos:exactMatch rdf:resource="https://www.wikidata.org/wiki/Q11472"/>
	<dcterms:created rdf:datatype="http://www.w3.org/2001/XMLSchema#date">2019-11-29</dcterms:created>
	<dcterms:modified rdf:datatype="http://www.w3.org/2001/XMLSchema#date">2023-08-02</dcterms:modified>
	<dcterms:identifier>250849</dcterms:identifier>
	<dcterms:contributor>blandine.nouvel</dcterms:contributor>
	<skos:definition xml:lang="en">Cellulose-based material made from natural or processed plant fibres, reduced to a homogeneous pulp which is spread out and dried to form a thin sheet (cntrl)</skos:definition>
	<skos:definition xml:lang="fr">Matière à base de cellulose, faite de fibres végétales naturelles ou transformées, réduites en une pâte homogène que l'on étend et sèche pour former une feuille mince. (cntrl)</skos:definition>
</rdf:Description>

<rdf:Description rdf:about="https://ark.frantiq.fr/ark:/26678/pcrtg0xc91xffk">
	<rdf:type rdf:resource="http://www.w3.org/2004/02/skos/core#Concept"/>
	<skos:prefLabel xml:lang="fr">andouiller de glace (renne)</skos:prefLabel>
	<skos:prefLabel xml:lang="en">bez tine</skos:prefLabel>
	<skos:prefLabel xml:lang="es">candil de hielo (reno)</skos:prefLabel>
	<skos:prefLabel xml:lang="de">Eissprosse (Rentier)</skos:prefLabel>
	<skos:prefLabel xml:lang="it">invernino (renna)</skos:prefLabel>
	<skos:broader rdf:resource="https://ark.frantiq.fr/ark:/26678/pcrt8ZW1DEoUSn"/>
	<skos:inScheme rdf:resource="https://ark.frantiq.fr/ark:/26678/TH_1"/>
	<opentheso:memberOf rdf:resource="https://ark.frantiq.fr/ark:/26678/pcrtv66rn9cbv1"/>
	<opentheso:memberOf rdf:resource="https://ark.frantiq.fr/ark:/26678/pcrtnbDLi2FkAj"/>
	<dcterms:created rdf:datatype="http://www.w3.org/2001/XMLSchema#date">2020-02-25</dcterms:created>
	<dcterms:modified rdf:datatype="http://www.w3.org/2001/XMLSchema#date">2023-08-02</dcterms:modified>
	<dcterms:identifier>253745</dcterms:identifier>
	<dcterms:contributor>blandine.nouvel</dcterms:contributor>
	<skos:definition xml:lang="en">Second andouiller of a reindeer antler starting from the base.</skos:definition>
	<skos:definition xml:lang="fr">Deuxième andouiller d'un bois de renne en partant de la base.</skos:definition>
</rdf:Description>

<rdf:Description rdf:about="https://ark.frantiq.fr/ark:/26678/pcrtzOFeK4FZEf">
	<rdf:type rdf:resource="http://www.w3.org/2004/02/skos/core#Concept"/>
	<skos:prefLabel xml:lang="de">Gemüse</skos:prefLabel>
	<skos:prefLabel xml:lang="nl">groente</skos:prefLabel>
	<skos:prefLabel xml:lang="fr">légume</skos:prefLabel>
	<skos:prefLabel xml:lang="it">ortaggio</skos:prefLabel>
	<skos:prefLabel xml:lang="en">vegetables</skos:prefLabel>
	<skos:prefLabel xml:lang="es">verdura</skos:prefLabel>
	<skos:prefLabel xml:lang="ar">خُضار</skos:prefLabel>
	<skos:altLabel xml:lang="it">verdura</skos:altLabel>
	<skos:related rdf:resource="https://ark.frantiq.fr/ark:/26678/pcrtvmAscT0l41"/>
	<skos:broader rdf:resource="https://ark.frantiq.fr/ark:/26678/pcrtgcn5U8laUN"/>
	<skos:inScheme rdf:resource="https://ark.frantiq.fr/ark:/26678/TH_1"/>
	<opentheso:memberOf rdf:resource="https://ark.frantiq.fr/ark:/26678/pcrtv66rn9cbv1"/>
	<opentheso:memberOf rdf:resource="https://ark.frantiq.fr/ark:/26678/pcrtnbDLi2FkAj"/>
	<skos:exactMatch rdf:resource="https://www.wikidata.org/wiki/Q11004"/>
	<dcterms:created rdf:datatype="http://www.w3.org/2001/XMLSchema#date">2007-02-08</dcterms:created>
	<dcterms:modified rdf:datatype="http://www.w3.org/2001/XMLSchema#date">2023-08-02</dcterms:modified>
	<dcterms:identifier>26003</dcterms:identifier>
	<dcterms:contributor>blandine.nouvel</dcterms:contributor>
	<skos:definition xml:lang="en">Edible plant or part of a vegetable species. (Wikipedia)</skos:definition>
	<skos:definition xml:lang="fr">Plante ou une partie comestible d'une espèce potagère. (Wikipedia)</skos:definition>
</rdf:Description>

<rdf:Description rdf:about="https://ark.frantiq.fr/ark:/26678/pcrtr5vk7w9vdz">
	<rdf:type rdf:resource="http://www.w3.org/2004/02/skos/core#Concept"/>
	<skos:prefLabel xml:lang="es">característica física de las rocas</skos:prefLabel>
	<skos:prefLabel xml:lang="fr">caractéristique physique des roches</skos:prefLabel>
	<skos:prefLabel xml:lang="it">caratteristica fisica delle rocce</skos:prefLabel>
	<skos:prefLabel xml:lang="en">physical properties of rocks</skos:prefLabel>
	<skos:prefLabel xml:lang="de">physisches Merkmal</skos:prefLabel>
	<skos:related rdf:resource="https://ark.frantiq.fr/ark:/26678/pcrt45EJYucSHg"/>
	<skos:narrower rdf:resource="https://ark.frantiq.fr/ark:/26678/pcrt6TSfpXkNW6"/>
	<skos:narrower rdf:resource="https://ark.frantiq.fr/ark:/26678/pcrtw8nqd0wpmc"/>
	<skos:narrower rdf:resource="https://ark.frantiq.fr/ark:/26678/pcrtbn5hw6ktqk"/>
	<skos:narrower rdf:resource="https://ark.frantiq.fr/ark:/26678/pcrt094rdqsfbv"/>
	<skos:narrower rdf:resource="https://ark.frantiq.fr/ark:/26678/pcrtkwk6bz94r3"/>
	<skos:narrower rdf:resource="https://ark.frantiq.fr/ark:/26678/pcrtqc4b4zzzmw"/>
	<skos:narrower rdf:resource="https://ark.frantiq.fr/ark:/26678/pcrt40qs0fvnxg"/>
	<skos:narrower rdf:resource="https://ark.frantiq.fr/ark:/26678/pcrtsvkcb5mv2t"/>
	<skos:narrower rdf:resource="https://ark.frantiq.fr/ark:/26678/pcrt5m5pftg21t"/>
	<skos:narrower rdf:resource="https://ark.frantiq.fr/ark:/26678/pcrt0kvts48fht"/>
	<skos:narrower rdf:resource="https://ark.frantiq.fr/ark:/26678/pcrtj6wgmdnp4k"/>
	<skos:narrower rdf:resource="https://ark.frantiq.fr/ark:/26678/pcrtq9kn0538k0"/>
	<skos:narrower rdf:resource="https://ark.frantiq.fr/ark:/26678/pcrtSHAq8xiG3F"/>
	<skos:broader rdf:resource="https://ark.frantiq.fr/ark:/26678/pcrtSVdwKcS3MI"/>
	<skos:inScheme rdf:resource="https://ark.frantiq.fr/ark:/26678/TH_1"/>
	<opentheso:memberOf rdf:resource="https://ark.frantiq.fr/ark:/26678/pcrtv66rn9cbv1"/>
	<opentheso:memberOf rdf:resource="https://ark.frantiq.fr/ark:/26678/pcrtnbDLi2FkAj"/>
	<dcterms:created rdf:datatype="http://www.w3.org/2001/XMLSchema#date">2020-07-08</dcterms:created>
	<dcterms:modified rdf:datatype="http://www.w3.org/2001/XMLSchema#date">2023-08-02</dcterms:modified>
	<dcterms:identifier>264721</dcterms:identifier>
	<dcterms:contributor>blandine.nouvel</dcterms:contributor>
</rdf:Description>

<rdf:Description rdf:about="https://ark.frantiq.fr/ark:/26678/pcrtfkw4vc3pc5">
	<rdf:type rdf:resource="http://www.w3.org/2004/02/skos/core#Concept"/>
	<skos:prefLabel xml:lang="it">ceramica comune tornita</skos:prefLabel>
	<skos:prefLabel xml:lang="es">cerámica común torneada</skos:prefLabel>
	<skos:prefLabel xml:lang="fr">céramique commune tournée</skos:prefLabel>
	<skos:prefLabel xml:lang="en">common wheel thrown ceramics</skos:prefLabel>
	<skos:prefLabel xml:lang="de">gedrehte Gebrauchskeramik</skos:prefLabel>
	<skos:related rdf:resource="https://ark.frantiq.fr/ark:/26678/pcrt3L8yViugRX"/>
	<skos:broader rdf:resource="https://ark.frantiq.fr/ark:/26678/pcrtho8l95no0j"/>
	<skos:inScheme rdf:resource="https://ark.frantiq.fr/ark:/26678/TH_1"/>
	<opentheso:memberOf rdf:resource="https://ark.frantiq.fr/ark:/26678/pcrtv66rn9cbv1"/>
	<opentheso:memberOf rdf:resource="https://ark.frantiq.fr/ark:/26678/pcrtnbDLi2FkAj"/>
	<skos:closeMatch rdf:resource="https://ark.mom.fr/ark:/39676/bib2h4bszv7f0"/>
	<skos:exactMatch rdf:resource="https://ark.mom.fr/ark:/39676/bibqmk2bdtghw"/>
	<dcterms:created rdf:datatype="http://www.w3.org/2001/XMLSchema#date">2020-08-14</dcterms:created>
	<dcterms:modified rdf:datatype="http://www.w3.org/2001/XMLSchema#date">2023-08-02</dcterms:modified>
	<dcterms:identifier>264971</dcterms:identifier>
	<dcterms:contributor>blandine.nouvel</dcterms:contributor>
</rdf:Description>

<rdf:Description rdf:about="https://ark.frantiq.fr/ark:/26678/pcrt5cdhzck93d">
	<rdf:type rdf:resource="http://www.w3.org/2004/02/skos/core#Concept"/>
	<skos:prefLabel xml:lang="de">brauntonige Keramik</skos:prefLabel>
	<skos:prefLabel xml:lang="en">brown ceramic</skos:prefLabel>
	<skos:prefLabel xml:lang="es">cerámica de pasta marrón</skos:prefLabel>
	<skos:prefLabel xml:lang="it">ceramica di impasto bruno</skos:prefLabel>
	<skos:prefLabel xml:lang="fr">céramique à pâte brune</skos:prefLabel>
	<skos:altLabel xml:lang="en">brown ware</skos:altLabel>
	<skos:broader rdf:resource="https://ark.frantiq.fr/ark:/26678/pcrtho8l95no0j"/>
	<skos:inScheme rdf:resource="https://ark.frantiq.fr/ark:/26678/TH_1"/>
	<opentheso:memberOf rdf:resource="https://ark.frantiq.fr/ark:/26678/pcrtv66rn9cbv1"/>
	<opentheso:memberOf rdf:resource="https://ark.frantiq.fr/ark:/26678/pcrtnbDLi2FkAj"/>
	<dcterms:created rdf:datatype="http://www.w3.org/2001/XMLSchema#date">2020-08-14</dcterms:created>
	<dcterms:modified rdf:datatype="http://www.w3.org/2001/XMLSchema#date">2023-08-02</dcterms:modified>
	<dcterms:identifier>264973</dcterms:identifier>
	<dcterms:contributor>blandine.nouvel</dcterms:contributor>
</rdf:Description>

<rdf:Description rdf:about="https://ark.frantiq.fr/ark:/26678/pcrtz14gcmpgjh">
	<rdf:type rdf:resource="http://www.w3.org/2004/02/skos/core#Concept"/>
	<skos:prefLabel xml:lang="es">cerámica de pasta clara</skos:prefLabel>
	<skos:prefLabel xml:lang="it">ceramica di impasto chiaro</skos:prefLabel>
	<skos:prefLabel xml:lang="fr">céramique à pâte claire</skos:prefLabel>
	<skos:prefLabel xml:lang="de">helltonige Keramik</skos:prefLabel>
	<skos:prefLabel xml:lang="en">white ware</skos:prefLabel>
	<skos:altLabel xml:lang="en">pale colored ceramic</skos:altLabel>
	<skos:altLabel xml:lang="en">tan ware</skos:altLabel>
	<skos:related rdf:resource="https://ark.frantiq.fr/ark:/26678/pcrtcccx1cwkd9"/>
	<skos:broader rdf:resource="https://ark.frantiq.fr/ark:/26678/pcrtho8l95no0j"/>
	<skos:inScheme rdf:resource="https://ark.frantiq.fr/ark:/26678/TH_1"/>
	<opentheso:memberOf rdf:resource="https://ark.frantiq.fr/ark:/26678/pcrtv66rn9cbv1"/>
	<opentheso:memberOf rdf:resource="https://ark.frantiq.fr/ark:/26678/pcrtnbDLi2FkAj"/>
	<skos:exactMatch rdf:resource="https://ark.mom.fr/ark:/39676/bibjhq5w25311"/>
	<dcterms:created rdf:datatype="http://www.w3.org/2001/XMLSchema#date">2020-08-14</dcterms:created>
	<dcterms:modified rdf:datatype="http://www.w3.org/2001/XMLSchema#date">2023-08-02</dcterms:modified>
	<dcterms:identifier>264974</dcterms:identifier>
	<dcterms:contributor>blandine.nouvel</dcterms:contributor>
</rdf:Description>

<rdf:Description rdf:about="https://ark.frantiq.fr/ark:/26678/pcrt218fx7941b">
	<rdf:type rdf:resource="http://www.w3.org/2004/02/skos/core#Concept"/>
	<skos:prefLabel xml:lang="es">cerámica de pasta roja</skos:prefLabel>
	<skos:prefLabel xml:lang="it">ceramica di impasto rosso</skos:prefLabel>
	<skos:prefLabel xml:lang="fr">céramique à pâte rouge</skos:prefLabel>
	<skos:prefLabel xml:lang="en">red ware</skos:prefLabel>
	<skos:prefLabel xml:lang="de">rottonige Keramik</skos:prefLabel>
	<skos:altLabel xml:lang="en">reddish brown ceramic</skos:altLabel>
	<skos:altLabel xml:lang="en">red gloss</skos:altLabel>
	<skos:altLabel xml:lang="en">terra sigillata</skos:altLabel>
	<skos:broader rdf:resource="https://ark.frantiq.fr/ark:/26678/pcrtho8l95no0j"/>
	<skos:inScheme rdf:resource="https://ark.frantiq.fr/ark:/26678/TH_1"/>
	<opentheso:memberOf rdf:resource="https://ark.frantiq.fr/ark:/26678/pcrtv66rn9cbv1"/>
	<opentheso:memberOf rdf:resource="https://ark.frantiq.fr/ark:/26678/pcrtnbDLi2FkAj"/>
	<dcterms:created rdf:datatype="http://www.w3.org/2001/XMLSchema#date">2020-08-14</dcterms:created>
	<dcterms:modified rdf:datatype="http://www.w3.org/2001/XMLSchema#date">2023-08-02</dcterms:modified>
	<dcterms:identifier>264976</dcterms:identifier>
	<dcterms:contributor>blandine.nouvel</dcterms:contributor>
</rdf:Description>

<rdf:Description rdf:about="https://ark.frantiq.fr/ark:/26678/pcrtvn284hkmw0">
	<rdf:type rdf:resource="http://www.w3.org/2004/02/skos/core#Concept"/>
	<skos:prefLabel xml:lang="es">cerámica de pasta negra</skos:prefLabel>
	<skos:prefLabel xml:lang="it">ceramica di impasto scuro</skos:prefLabel>
	<skos:prefLabel xml:lang="fr">céramique à pâte sombre</skos:prefLabel>
	<skos:prefLabel xml:lang="en">dark clay ware</skos:prefLabel>
	<skos:prefLabel xml:lang="de">dunkeltonige Keramik</skos:prefLabel>
	<skos:altLabel xml:lang="en">black-burnished ware</skos:altLabel>
	<skos:altLabel xml:lang="en">terra nigra</skos:altLabel>
	<skos:broader rdf:resource="https://ark.frantiq.fr/ark:/26678/pcrtho8l95no0j"/>
	<skos:inScheme rdf:resource="https://ark.frantiq.fr/ark:/26678/TH_1"/>
	<opentheso:memberOf rdf:resource="https://ark.frantiq.fr/ark:/26678/pcrtv66rn9cbv1"/>
	<opentheso:memberOf rdf:resource="https://ark.frantiq.fr/ark:/26678/pcrtnbDLi2FkAj"/>
	<skos:exactMatch rdf:resource="https://ark.mom.fr/ark:/39676/bibw4j422bcjj"/>
	<dcterms:created rdf:datatype="http://www.w3.org/2001/XMLSchema#date">2020-08-14</dcterms:created>
	<dcterms:modified rdf:datatype="http://www.w3.org/2001/XMLSchema#date">2023-08-02</dcterms:modified>
	<dcterms:identifier>264977</dcterms:identifier>
	<dcterms:contributor>blandine.nouvel</dcterms:contributor>
</rdf:Description>

<rdf:Description rdf:about="https://ark.frantiq.fr/ark:/26678/pcrtb1vvxk8fp3">
	<rdf:type rdf:resource="http://www.w3.org/2004/02/skos/core#Concept"/>
	<skos:prefLabel xml:lang="it">caramica di impasto grigio</skos:prefLabel>
	<skos:prefLabel xml:lang="es">cerámica de pasta gris</skos:prefLabel>
	<skos:prefLabel xml:lang="fr">céramique à pâte grise</skos:prefLabel>
	<skos:prefLabel xml:lang="de">grautonige Keramik</skos:prefLabel>
	<skos:prefLabel xml:lang="en">grey ware</skos:prefLabel>
	<skos:broader rdf:resource="https://ark.frantiq.fr/ark:/26678/pcrtho8l95no0j"/>
	<skos:inScheme rdf:resource="https://ark.frantiq.fr/ark:/26678/TH_1"/>
	<opentheso:memberOf rdf:resource="https://ark.frantiq.fr/ark:/26678/pcrtv66rn9cbv1"/>
	<opentheso:memberOf rdf:resource="https://ark.frantiq.fr/ark:/26678/pcrtnbDLi2FkAj"/>
	<skos:exactMatch rdf:resource="https://ark.mom.fr/ark:/39676/bibvqcwgkwxm1"/>
	<dcterms:created rdf:datatype="http://www.w3.org/2001/XMLSchema#date">2020-08-14</dcterms:created>
	<dcterms:modified rdf:datatype="http://www.w3.org/2001/XMLSchema#date">2023-08-02</dcterms:modified>
	<dcterms:identifier>264978</dcterms:identifier>
	<dcterms:contributor>blandine.nouvel</dcterms:contributor>
</rdf:Description>

<rdf:Description rdf:about="https://ark.frantiq.fr/ark:/26678/pcrt73gjdrz4rx">
	<rdf:type rdf:resource="http://www.w3.org/2004/02/skos/core#Concept"/>
	<skos:prefLabel xml:lang="it">caramica fine</skos:prefLabel>
	<skos:prefLabel xml:lang="es">cerámica fina</skos:prefLabel>
	<skos:prefLabel xml:lang="fr">céramique fine</skos:prefLabel>
	<skos:prefLabel xml:lang="de">Feinkeramik</skos:prefLabel>
	<skos:prefLabel xml:lang="en">fine ware</skos:prefLabel>
	<skos:altLabel xml:lang="de">Feinware</skos:altLabel>
	<skos:broader rdf:resource="https://ark.frantiq.fr/ark:/26678/pcrtfx4s0yvSLj"/>
	<skos:inScheme rdf:resource="https://ark.frantiq.fr/ark:/26678/TH_1"/>
	<opentheso:memberOf rdf:resource="https://ark.frantiq.fr/ark:/26678/pcrtv66rn9cbv1"/>
	<opentheso:memberOf rdf:resource="https://ark.frantiq.fr/ark:/26678/pcrtnbDLi2FkAj"/>
	<dcterms:created rdf:datatype="http://www.w3.org/2001/XMLSchema#date">2020-08-14</dcterms:created>
	<dcterms:modified rdf:datatype="http://www.w3.org/2001/XMLSchema#date">2023-08-02</dcterms:modified>
	<dcterms:identifier>264979</dcterms:identifier>
	<dcterms:contributor>blandine.nouvel</dcterms:contributor>
	<skos:definition xml:lang="en">Quality ceramics, often imported, from well-known workshops.</skos:definition>
	<skos:definition xml:lang="fr">Céramique de qualité, souvent importée, provenant d'ateliers connus.</skos:definition>
</rdf:Description>

<rdf:Description rdf:about="https://ark.frantiq.fr/ark:/26678/pcrtbbqj7zgqnn">
	<rdf:type rdf:resource="http://www.w3.org/2004/02/skos/core#Concept"/>
	<skos:prefLabel xml:lang="es">negro de humo</skos:prefLabel>
	<skos:prefLabel xml:lang="it">nerofumo</skos:prefLabel>
	<skos:prefLabel xml:lang="fr">noir de fumée</skos:prefLabel>
	<skos:prefLabel xml:lang="de">rauchschwarz</skos:prefLabel>
	<skos:prefLabel xml:lang="en">smoke carbon residue</skos:prefLabel>
	<skos:altLabel xml:lang="en">smoke carbon residue coloring</skos:altLabel>
	<skos:altLabel xml:lang="en">soot</skos:altLabel>
	<skos:altLabel xml:lang="en">soot colorant</skos:altLabel>
	<skos:related rdf:resource="https://ark.frantiq.fr/ark:/26678/pcrtb45s11kx35"/>
	<skos:related rdf:resource="https://ark.frantiq.fr/ark:/26678/pcrt26v6m1wwnh"/>
	<skos:related rdf:resource="https://ark.frantiq.fr/ark:/26678/pcrt3kpULwWUS2"/>
	<skos:broader rdf:resource="https://ark.frantiq.fr/ark:/26678/pcrtGzQPnntJa1"/>
	<skos:inScheme rdf:resource="https://ark.frantiq.fr/ark:/26678/TH_1"/>
	<opentheso:memberOf rdf:resource="https://ark.frantiq.fr/ark:/26678/pcrtv66rn9cbv1"/>
	<opentheso:memberOf rdf:resource="https://ark.frantiq.fr/ark:/26678/pcrtnbDLi2FkAj"/>
	<skos:exactMatch rdf:resource="https://www.wikidata.org/wiki/Q3342725"/>
	<dcterms:created rdf:datatype="http://www.w3.org/2001/XMLSchema#date">2020-08-15</dcterms:created>
	<dcterms:modified rdf:datatype="http://www.w3.org/2001/XMLSchema#date">2023-08-02</dcterms:modified>
	<dcterms:identifier>265000</dcterms:identifier>
	<dcterms:contributor>blandine.nouvel</dcterms:contributor>
	<skos:definition xml:lang="en">Carbonaceous residue obtained by the incomplete combustion of various carbon-rich organic materials (Wikipedia)</skos:definition>
	<skos:definition xml:lang="fr">Résidu carboné obtenu par la combustion incomplète de diverses matières organiques riches en carbone. (Wikipedia)</skos:definition>
</rdf:Description>

<rdf:Description rdf:about="https://ark.frantiq.fr/ark:/26678/pcrt518w0nr5tf">
	<rdf:type rdf:resource="http://www.w3.org/2004/02/skos/core#Concept"/>
	<skos:prefLabel xml:lang="es">barbotina</skos:prefLabel>
	<skos:prefLabel xml:lang="fr">barbotine</skos:prefLabel>
	<skos:prefLabel xml:lang="it">barbottina</skos:prefLabel>
	<skos:prefLabel xml:lang="de">Schlicker</skos:prefLabel>
	<skos:prefLabel xml:lang="nl">slip</skos:prefLabel>
	<skos:prefLabel xml:lang="en">slip (ceramics)</skos:prefLabel>
	<skos:related rdf:resource="https://ark.frantiq.fr/ark:/26678/pcrtXgoFDoG7xA"/>
	<skos:related rdf:resource="https://ark.frantiq.fr/ark:/26678/pcrth13n5jt6nc"/>
	<skos:related rdf:resource="https://ark.frantiq.fr/ark:/26678/pcrtkvf403bvpk"/>
	<skos:related rdf:resource="https://ark.frantiq.fr/ark:/26678/pcrt6q0qrns6wp"/>
	<skos:broader rdf:resource="https://ark.frantiq.fr/ark:/26678/pcrtZETJwE7RTQ"/>
	<skos:inScheme rdf:resource="https://ark.frantiq.fr/ark:/26678/TH_1"/>
	<opentheso:memberOf rdf:resource="https://ark.frantiq.fr/ark:/26678/pcrtv66rn9cbv1"/>
	<opentheso:memberOf rdf:resource="https://ark.frantiq.fr/ark:/26678/pcrtnbDLi2FkAj"/>
	<skos:exactMatch rdf:resource="https://www.wikidata.org/wiki/Q1971493"/>
	<dcterms:created rdf:datatype="http://www.w3.org/2001/XMLSchema#date">2020-08-16</dcterms:created>
	<dcterms:modified rdf:datatype="http://www.w3.org/2001/XMLSchema#date">2024-11-18</dcterms:modified>
	<dcterms:identifier>265010</dcterms:identifier>
	<dcterms:contributor>blandine.nouvel</dcterms:contributor>
	<dcterms:contributor>justine.vincent</dcterms:contributor>
	<skos:definition xml:lang="en">A more or less fluid clay paste, which makes up engobes and is used for many purposes during the manufacture of vases, in both turned and modelled techniques: keeping the wall of the vase moist and levelling its surface, so that the elements stick together (Yon 1981, p. 32).</skos:definition>
	<skos:definition xml:lang="fr">Pâte argileuse plus ou moins fluide, qui constitue les engobes et qui sert à de multiples usages au cours de la fabrication du vase, aussi bien dans les techniques tournées que dans les techniques modelées : maintenir humide la paroi du vase qu'il travaille, et égaliser sa surface, pour coller les éléments les uns aux autres. (Yon 1981, p. 32)</skos:definition>
	<skos:historyNote xml:lang="fr">2024-18-11 : modification de la définition.</skos:historyNote>
</rdf:Description>

<rdf:Description rdf:about="https://ark.frantiq.fr/ark:/26678/pcrtrdsp44jvsk0qqqkndb9g">
	<rdf:type rdf:resource="http://www.w3.org/2004/02/skos/core#Concept"/>
	<skos:prefLabel xml:lang="es">aglutinante</skos:prefLabel>
	<skos:prefLabel xml:lang="de">Bindemittel</skos:prefLabel>
	<skos:prefLabel xml:lang="en">binder</skos:prefLabel>
	<skos:prefLabel xml:lang="nl">bindmiddel</skos:prefLabel>
	<skos:prefLabel xml:lang="it">legante</skos:prefLabel>
	<skos:prefLabel xml:lang="fr">liant</skos:prefLabel>
	<skos:prefLabel xml:lang="ar">مادة رابطة</skos:prefLabel>
	<skos:related rdf:resource="https://ark.frantiq.fr/ark:/26678/pcrtEWWJvOVoh5"/>
	<skos:broader rdf:resource="https://ark.frantiq.fr/ark:/26678/pcrtQuZiT5nYY2"/>
	<skos:inScheme rdf:resource="https://ark.frantiq.fr/ark:/26678/TH_1"/>
	<opentheso:memberOf rdf:resource="https://ark.frantiq.fr/ark:/26678/pcrtv66rn9cbv1"/>
	<opentheso:memberOf rdf:resource="https://ark.frantiq.fr/ark:/26678/pcrtnbDLi2FkAj"/>
	<skos:exactMatch rdf:resource="https://www.wikidata.org/wiki/Q863583"/>
	<dcterms:created rdf:datatype="http://www.w3.org/2001/XMLSchema#date">2020-09-29</dcterms:created>
	<dcterms:modified rdf:datatype="http://www.w3.org/2001/XMLSchema#date">2023-09-05</dcterms:modified>
	<dcterms:identifier>265137</dcterms:identifier>
	<dcterms:creator>blandine.nouvel</dcterms:creator>
	<dcterms:contributor>justine.vincent</dcterms:contributor>
	<skos:definition xml:lang="en">Material having the property of holding together aggregates (CNRTL).</skos:definition>
	<skos:definition xml:lang="fr">&lt;span style= background-color: rgb(250, 250, 250); &gt;Matériau ayant la propriété de maintenir ensemble des agrégats (CNRTL).&lt;/span&gt;</skos:definition>
</rdf:Description>

<rdf:Description rdf:about="https://ark.frantiq.fr/ark:/26678/pcrt0k0f3qbw4r">
	<rdf:type rdf:resource="http://www.w3.org/2004/02/skos/core#Concept"/>
	<skos:prefLabel xml:lang="es">almidón</skos:prefLabel>
	<skos:prefLabel xml:lang="it">amido</skos:prefLabel>
	<skos:prefLabel xml:lang="fr">amidon</skos:prefLabel>
	<skos:prefLabel xml:lang="en">starch</skos:prefLabel>
	<skos:prefLabel xml:lang="de">Stärke</skos:prefLabel>
	<skos:prefLabel xml:lang="nl">zetmeel</skos:prefLabel>
	<skos:altLabel xml:lang="en">amylum</skos:altLabel>
	<skos:altLabel xml:lang="nl">stijfsel</skos:altLabel>
	<skos:broader rdf:resource="https://ark.frantiq.fr/ark:/26678/pcrtnHxyjOkhJw"/>
	<skos:inScheme rdf:resource="https://ark.frantiq.fr/ark:/26678/TH_1"/>
	<opentheso:memberOf rdf:resource="https://ark.frantiq.fr/ark:/26678/pcrtv66rn9cbv1"/>
	<opentheso:memberOf rdf:resource="https://ark.frantiq.fr/ark:/26678/pcrtnbDLi2FkAj"/>
	<skos:exactMatch rdf:resource="https://www.wikidata.org/wiki/Q41534"/>
	<dcterms:created rdf:datatype="http://www.w3.org/2001/XMLSchema#date">2021-01-21</dcterms:created>
	<dcterms:modified rdf:datatype="http://www.w3.org/2001/XMLSchema#date">2023-08-02</dcterms:modified>
	<dcterms:identifier>266317</dcterms:identifier>
	<dcterms:contributor>blandine.nouvel</dcterms:contributor>
	<skos:definition xml:lang="en">Complex carbohydrate present in the reserve organs of many plants.</skos:definition>
	<skos:definition xml:lang="fr">Glucide complexe présent dans les organes de réserve de nombreuses plantes.</skos:definition>
</rdf:Description>

<rdf:Description rdf:about="https://ark.frantiq.fr/ark:/26678/pcrtsxjtz27508">
	<rdf:type rdf:resource="http://www.w3.org/2004/02/skos/core#Concept"/>
	<skos:prefLabel xml:lang="it">chicco di caffè</skos:prefLabel>
	<skos:prefLabel xml:lang="en">coffee bean</skos:prefLabel>
	<skos:prefLabel xml:lang="fr">grain de café</skos:prefLabel>
	<skos:prefLabel xml:lang="es">grano de café</skos:prefLabel>
	<skos:prefLabel xml:lang="de">Kaffeebohne</skos:prefLabel>
	<skos:prefLabel xml:lang="nl">koffieboon</skos:prefLabel>
	<skos:related rdf:resource="https://ark.frantiq.fr/ark:/26678/pcrtDFvOrje3j0"/>
	<skos:related rdf:resource="https://ark.frantiq.fr/ark:/26678/crtSfObTEvbdn"/>
	<skos:related rdf:resource="https://ark.frantiq.fr/ark:/26678/pcrt3k3mbd0n2czwp1w1gcr9"/>
	<skos:broader rdf:resource="https://ark.frantiq.fr/ark:/26678/pcrtgcn5U8laUN"/>
	<skos:inScheme rdf:resource="https://ark.frantiq.fr/ark:/26678/TH_1"/>
	<opentheso:memberOf rdf:resource="https://ark.frantiq.fr/ark:/26678/pcrtv66rn9cbv1"/>
	<opentheso:memberOf rdf:resource="https://ark.frantiq.fr/ark:/26678/pcrtnbDLi2FkAj"/>
	<skos:exactMatch rdf:resource="https://www.wikidata.org/wiki/Q153697"/>
	<dcterms:created rdf:datatype="http://www.w3.org/2001/XMLSchema#date">2021-01-21</dcterms:created>
	<dcterms:modified rdf:datatype="http://www.w3.org/2001/XMLSchema#date">2023-08-02</dcterms:modified>
	<dcterms:identifier>266323</dcterms:identifier>
	<dcterms:contributor>blandine.nouvel</dcterms:contributor>
	<skos:definition xml:lang="en">Seed of the coffee plant.</skos:definition>
	<skos:definition xml:lang="fr">Graine de la plante de café.</skos:definition>
</rdf:Description>

<rdf:Description rdf:about="https://ark.frantiq.fr/ark:/26678/pcrtbhbct8gbhn">
	<rdf:type rdf:resource="http://www.w3.org/2004/02/skos/core#Concept"/>
	<skos:prefLabel xml:lang="nl">druif</skos:prefLabel>
	<skos:prefLabel xml:lang="en">grape</skos:prefLabel>
	<skos:prefLabel xml:lang="fr">raisin</skos:prefLabel>
	<skos:prefLabel xml:lang="de">Trauben</skos:prefLabel>
	<skos:prefLabel xml:lang="es">uva</skos:prefLabel>
	<skos:prefLabel xml:lang="it">uva</skos:prefLabel>
	<skos:altLabel xml:lang="fr">baie de raisin</skos:altLabel>
	<skos:altLabel xml:lang="it">chicco d'uva</skos:altLabel>
	<skos:altLabel xml:lang="fr">grain de raisin</skos:altLabel>
	<skos:altLabel xml:lang="fr">pépin de raisin</skos:altLabel>
	<skos:altLabel xml:lang="es">racimo de uva</skos:altLabel>
	<skos:altLabel xml:lang="es">semilla de uva</skos:altLabel>
	<skos:related rdf:resource="https://ark.frantiq.fr/ark:/26678/pcrtDFvOrje3j0"/>
	<skos:related rdf:resource="https://ark.frantiq.fr/ark:/26678/pcrtihlJWfvH4v"/>
	<skos:related rdf:resource="https://ark.frantiq.fr/ark:/26678/pcrt3mTg9h3RFE"/>
	<skos:broader rdf:resource="https://ark.frantiq.fr/ark:/26678/pcrtgcn5U8laUN"/>
	<skos:inScheme rdf:resource="https://ark.frantiq.fr/ark:/26678/TH_1"/>
	<opentheso:memberOf rdf:resource="https://ark.frantiq.fr/ark:/26678/pcrtv66rn9cbv1"/>
	<opentheso:memberOf rdf:resource="https://ark.frantiq.fr/ark:/26678/pcrtnbDLi2FkAj"/>
	<skos:exactMatch rdf:resource="https://www.wikidata.org/wiki/Q4013015"/>
	<dcterms:created rdf:datatype="http://www.w3.org/2001/XMLSchema#date">2021-01-21</dcterms:created>
	<dcterms:modified rdf:datatype="http://www.w3.org/2001/XMLSchema#date">2023-08-02</dcterms:modified>
	<dcterms:identifier>266327</dcterms:identifier>
	<dcterms:contributor>blandine.nouvel</dcterms:contributor>
	<skos:definition xml:lang="en">Seed of the grape berry.</skos:definition>
	<skos:definition xml:lang="fr">Graine de la baie de raisin.</skos:definition>
</rdf:Description>

<rdf:Description rdf:about="https://ark.frantiq.fr/ark:/26678/pcrtkf9tnv3kc1">
	<rdf:type rdf:resource="http://www.w3.org/2004/02/skos/core#Concept"/>
	<skos:prefLabel xml:lang="es">mirra</skos:prefLabel>
	<skos:prefLabel xml:lang="it">mirra</skos:prefLabel>
	<skos:prefLabel xml:lang="nl">mirre</skos:prefLabel>
	<skos:prefLabel xml:lang="en">myrrh</skos:prefLabel>
	<skos:prefLabel xml:lang="fr">myrrhe</skos:prefLabel>
	<skos:prefLabel xml:lang="de">Myrrhe</skos:prefLabel>
	<skos:altLabel xml:lang="fr">Commiphora molmol</skos:altLabel>
	<skos:altLabel xml:lang="fr">Commiphora myrrha</skos:altLabel>
	<skos:broader rdf:resource="https://ark.frantiq.fr/ark:/26678/pcrtrxL50B7yNx"/>
	<skos:inScheme rdf:resource="https://ark.frantiq.fr/ark:/26678/TH_1"/>
	<opentheso:memberOf rdf:resource="https://ark.frantiq.fr/ark:/26678/pcrtv66rn9cbv1"/>
	<opentheso:memberOf rdf:resource="https://ark.frantiq.fr/ark:/26678/pcrtnbDLi2FkAj"/>
	<skos:exactMatch rdf:resource="https://www.wikidata.org/wiki/Q203635"/>
	<dcterms:created rdf:datatype="http://www.w3.org/2001/XMLSchema#date">2021-01-21</dcterms:created>
	<dcterms:modified rdf:datatype="http://www.w3.org/2001/XMLSchema#date">2024-11-15</dcterms:modified>
	<dcterms:identifier>266330</dcterms:identifier>
	<dcterms:contributor>blandine.nouvel</dcterms:contributor>
	<dcterms:contributor>justine.vincent</dcterms:contributor>
	<skos:definition xml:lang="fr">Gomme-résine aromatique produite par l'arbre à myrrhe. (Wikipedia, 2021).</skos:definition>
	<skos:definition xml:lang="en">Aromatic gum-resin produced by the myrrh tree (Wikipedia, 2021).</skos:definition>
</rdf:Description>

<rdf:Description rdf:about="https://ark.frantiq.fr/ark:/26678/pcrtw8nqd0wpmc">
	<rdf:type rdf:resource="http://www.w3.org/2004/02/skos/core#Concept"/>
	<skos:prefLabel xml:lang="es">hábito cristalino</skos:prefLabel>
	<skos:prefLabel xml:lang="en">habitus</skos:prefLabel>
	<skos:prefLabel xml:lang="fr">habitus</skos:prefLabel>
	<skos:prefLabel xml:lang="it">habitus</skos:prefLabel>
	<skos:prefLabel xml:lang="de">Habitus</skos:prefLabel>
	<skos:altLabel xml:lang="it">abito cristallino</skos:altLabel>
	<skos:narrower rdf:resource="https://ark.frantiq.fr/ark:/26678/pcrtTgttY2SfBr"/>
	<skos:narrower rdf:resource="https://ark.frantiq.fr/ark:/26678/pcrtlZ7VYeGKO3"/>
	<skos:narrower rdf:resource="https://ark.frantiq.fr/ark:/26678/pcrtv3pfn44gc4"/>
	<skos:narrower rdf:resource="https://ark.frantiq.fr/ark:/26678/pcrtvm1c7n58sx"/>
	<skos:narrower rdf:resource="https://ark.frantiq.fr/ark:/26678/pcrtk3njjx5659"/>
	<skos:narrower rdf:resource="https://ark.frantiq.fr/ark:/26678/pcrt33sf88d6jh"/>
	<skos:narrower rdf:resource="https://ark.frantiq.fr/ark:/26678/pcrtbpgr0h35bn"/>
	<skos:narrower rdf:resource="https://ark.frantiq.fr/ark:/26678/pcrtn97gqkmvfx"/>
	<skos:broader rdf:resource="https://ark.frantiq.fr/ark:/26678/pcrtr5vk7w9vdz"/>
	<skos:inScheme rdf:resource="https://ark.frantiq.fr/ark:/26678/TH_1"/>
	<opentheso:memberOf rdf:resource="https://ark.frantiq.fr/ark:/26678/pcrtv66rn9cbv1"/>
	<opentheso:memberOf rdf:resource="https://ark.frantiq.fr/ark:/26678/pcrtnbDLi2FkAj"/>
	<dcterms:created rdf:datatype="http://www.w3.org/2001/XMLSchema#date">2021-02-12</dcterms:created>
	<dcterms:modified rdf:datatype="http://www.w3.org/2001/XMLSchema#date">2025-01-17</dcterms:modified>
	<dcterms:identifier>266365</dcterms:identifier>
	<dcterms:contributor>blandine.nouvel</dcterms:contributor>
	<skos:definition xml:lang="en">Characterises the morphology of the developed faces of a crystal or rock (Fernandes et al.: Vade-mecum pour la caractérisation pétroarchéologique des silicites, 2024).</skos:definition>
	<skos:definition xml:lang="fr">Caractérise la morphologie des faces développées d'un cristal ou d'une roche (Fernandes et al. : Vade-mecum pour la caractérisation pétroarchéologique des silicites, 2024).</skos:definition>
	<skos:historyNote xml:lang="fr">2025-01-17: mise à jour de la réf. bibliographique de la définition.</skos:historyNote>
</rdf:Description>

<rdf:Description rdf:about="https://ark.frantiq.fr/ark:/26678/pcrtv3pfn44gc4">
	<rdf:type rdf:resource="http://www.w3.org/2004/02/skos/core#Concept"/>
	<skos:prefLabel xml:lang="de">Knoten</skos:prefLabel>
	<skos:prefLabel xml:lang="en">nodule</skos:prefLabel>
	<skos:prefLabel xml:lang="fr">nodule</skos:prefLabel>
	<skos:prefLabel xml:lang="it">nodulo</skos:prefLabel>
	<skos:prefLabel xml:lang="es">nódulo</skos:prefLabel>
	<skos:altLabel xml:lang="de">Knötchen</skos:altLabel>
	<skos:broader rdf:resource="https://ark.frantiq.fr/ark:/26678/pcrtw8nqd0wpmc"/>
	<skos:inScheme rdf:resource="https://ark.frantiq.fr/ark:/26678/TH_1"/>
	<opentheso:memberOf rdf:resource="https://ark.frantiq.fr/ark:/26678/pcrtv66rn9cbv1"/>
	<opentheso:memberOf rdf:resource="https://ark.frantiq.fr/ark:/26678/pcrtnbDLi2FkAj"/>
	<skos:exactMatch rdf:resource="https://www.wikidata.org/wiki/Q2916245"/>
	<dcterms:created rdf:datatype="http://www.w3.org/2001/XMLSchema#date">2021-02-12</dcterms:created>
	<dcterms:modified rdf:datatype="http://www.w3.org/2001/XMLSchema#date">2025-01-17</dcterms:modified>
	<dcterms:identifier>266367</dcterms:identifier>
	<dcterms:contributor>blandine.nouvel</dcterms:contributor>
	<dcterms:contributor>justine.vincent</dcterms:contributor>
	<skos:definition xml:lang="en">Regular or irregular flattened kidney (Fernandes et al.: Vade-mecum pour la caractérisation pétroarchéologique des silicites, 2024).</skos:definition>
	<skos:definition xml:lang="fr">Rognon régulier ou irrégulier aplati (Fernandes et al. : Vade-mecum pour la caractérisation pétroarchéologique des silicites, 2024).</skos:definition>
	<skos:historyNote xml:lang="fr">2025-01-17: mise à jour de la réf. bibliographique de la définition.</skos:historyNote>
</rdf:Description>

<rdf:Description rdf:about="https://ark.frantiq.fr/ark:/26678/pcrtvm1c7n58sx">
	<rdf:type rdf:resource="http://www.w3.org/2004/02/skos/core#Concept"/>
	<skos:prefLabel xml:lang="fr">banc (géologie)</skos:prefLabel>
	<skos:prefLabel xml:lang="it">banco (geologia)</skos:prefLabel>
	<skos:prefLabel xml:lang="es">banco (geología)</skos:prefLabel>
	<skos:prefLabel xml:lang="de">Bank (Geologie)</skos:prefLabel>
	<skos:prefLabel xml:lang="en">bed (geology)</skos:prefLabel>
	<skos:broader rdf:resource="https://ark.frantiq.fr/ark:/26678/pcrtw8nqd0wpmc"/>
	<skos:inScheme rdf:resource="https://ark.frantiq.fr/ark:/26678/TH_1"/>
	<opentheso:memberOf rdf:resource="https://ark.frantiq.fr/ark:/26678/pcrtv66rn9cbv1"/>
	<opentheso:memberOf rdf:resource="https://ark.frantiq.fr/ark:/26678/pcrtnbDLi2FkAj"/>
	<dcterms:created rdf:datatype="http://www.w3.org/2001/XMLSchema#date">2021-02-12</dcterms:created>
	<dcterms:modified rdf:datatype="http://www.w3.org/2001/XMLSchema#date">2025-01-17</dcterms:modified>
	<dcterms:identifier>266369</dcterms:identifier>
	<dcterms:contributor>blandine.nouvel</dcterms:contributor>
	<skos:definition xml:lang="en">Sedimentary layer limited at the roof (upper limit of the layer) and at the wall (lower limit of the layer) by two stratification joints with a thickness greater than or equal to 10 cm (Fernandes et al.: Vade-mecum pour la caractérisation pétroarchéologique des silicites, 2024).</skos:definition>
	<skos:definition xml:lang="fr">Couche sédimentaire limitée au toit (limite supérieure de la couche) et au mur (limite inférieure de la couche) par deux joints de stratification à épaisseur supérieure ou égale à 10 cm (Fernandes et al. : Vade-mecum pour la caractérisation pétroarchéologique des silicites, 2024).</skos:definition>
	<skos:historyNote xml:lang="fr">2025-01-17: mise à jour de la réf. bibliographique de la définition.</skos:historyNote>
</rdf:Description>

<rdf:Description rdf:about="https://ark.frantiq.fr/ark:/26678/pcrtk3njjx5659">
	<rdf:type rdf:resource="http://www.w3.org/2004/02/skos/core#Concept"/>
	<skos:prefLabel xml:lang="fr">dalle (géologie)</skos:prefLabel>
	<skos:prefLabel xml:lang="it">lastra (geologia)</skos:prefLabel>
	<skos:prefLabel xml:lang="es">losa (geología)</skos:prefLabel>
	<skos:prefLabel xml:lang="de">Steinplatte</skos:prefLabel>
	<skos:prefLabel xml:lang="en">stone slab</skos:prefLabel>
	<skos:broader rdf:resource="https://ark.frantiq.fr/ark:/26678/pcrtw8nqd0wpmc"/>
	<skos:inScheme rdf:resource="https://ark.frantiq.fr/ark:/26678/TH_1"/>
	<opentheso:memberOf rdf:resource="https://ark.frantiq.fr/ark:/26678/pcrtv66rn9cbv1"/>
	<opentheso:memberOf rdf:resource="https://ark.frantiq.fr/ark:/26678/pcrtnbDLi2FkAj"/>
	<dcterms:created rdf:datatype="http://www.w3.org/2001/XMLSchema#date">2021-02-12</dcterms:created>
	<dcterms:modified rdf:datatype="http://www.w3.org/2001/XMLSchema#date">2025-01-17</dcterms:modified>
	<dcterms:identifier>266371</dcterms:identifier>
	<dcterms:contributor>blandine.nouvel</dcterms:contributor>
	<skos:definition xml:lang="en">Monolithic rock slab of a sedimentary formation limited at the roof (upper limit of the layer) and at the wall (lower limit of the layer) by two stratification joints with a thickness greater than or equal to 1m (Fernandes et al.: Vade-mecum pour la caractérisation pétroarchéologique des silicites, 2024).</skos:definition>
	<skos:definition xml:lang="fr">Plaque rocheuse monolithe d'une formation sédimentaire limitée au toit (limite supérieure de la couche) et au mur (limite inférieure de la couche) par deux joints de stratification à épaisseur supérieure ou égale à 1m (Fernandes et al. : Vade-mecum pour la caractérisation pétroarchéologique des silicites, 2024).</skos:definition>
	<skos:historyNote xml:lang="fr">2025-01-17: mise à jour de la réf. bibliographique de la définition.</skos:historyNote>
</rdf:Description>

<rdf:Description rdf:about="https://ark.frantiq.fr/ark:/26678/pcrt33sf88d6jh">
	<rdf:type rdf:resource="http://www.w3.org/2004/02/skos/core#Concept"/>
	<skos:prefLabel xml:lang="en">geofact</skos:prefLabel>
	<skos:prefLabel xml:lang="fr">géofact</skos:prefLabel>
	<skos:prefLabel xml:lang="es">geofacto</skos:prefLabel>
	<skos:prefLabel xml:lang="de">Geofakt</skos:prefLabel>
	<skos:prefLabel xml:lang="it">geofatto</skos:prefLabel>
	<skos:narrower rdf:resource="https://ark.frantiq.fr/ark:/26678/pcrtckknjb3bj0"/>
	<skos:narrower rdf:resource="https://ark.frantiq.fr/ark:/26678/pcrthqg1d2ks27"/>
	<skos:broader rdf:resource="https://ark.frantiq.fr/ark:/26678/pcrtw8nqd0wpmc"/>
	<skos:inScheme rdf:resource="https://ark.frantiq.fr/ark:/26678/TH_1"/>
	<opentheso:memberOf rdf:resource="https://ark.frantiq.fr/ark:/26678/pcrtv66rn9cbv1"/>
	<opentheso:memberOf rdf:resource="https://ark.frantiq.fr/ark:/26678/pcrtnbDLi2FkAj"/>
	<skos:exactMatch rdf:resource="https://www.wikidata.org/wiki/Q5534014"/>
	<dcterms:created rdf:datatype="http://www.w3.org/2001/XMLSchema#date">2021-02-12</dcterms:created>
	<dcterms:modified rdf:datatype="http://www.w3.org/2001/XMLSchema#date">2025-01-17</dcterms:modified>
	<dcterms:identifier>266373</dcterms:identifier>
	<dcterms:contributor>blandine.nouvel</dcterms:contributor>
	<dcterms:contributor>justine.vincent</dcterms:contributor>
	<skos:definition xml:lang="fr">Fragment de roche produit et transformé par la nature et qui peut répliquer une forme habituellement façonnée par l'homme (Fernandes et al. : Vade-mecum pour la caractérisation pétroarchéologique des silicites, 2024).</skos:definition>
	<skos:definition xml:lang="en">A fragment of rock produced and transformed by nature that can replicate a form usually shaped by man (Fernandes et al.: Vade-mecum pour la caractérisation pétroarchéologique des silicites, 2024).</skos:definition>
	<skos:scopeNote xml:lang="fr">On distingue les gélifracts (produits par le gel), les téphrofacts (produits par le volcanisme), les ventifacts (produits par les vents).</skos:scopeNote>
	<skos:historyNote xml:lang="fr">2024-11-19 : modification de la définition. 2025-01-17 : mise à jour de la réf. bibliographique dans la définition</skos:historyNote>
</rdf:Description>

<rdf:Description rdf:about="https://ark.frantiq.fr/ark:/26678/pcrtckknjb3bj0">
	<rdf:type rdf:resource="http://www.w3.org/2004/02/skos/core#Concept"/>
	<skos:prefLabel xml:lang="en">gelifact</skos:prefLabel>
	<skos:prefLabel xml:lang="es">gelifact</skos:prefLabel>
	<skos:prefLabel xml:lang="it">gelifact</skos:prefLabel>
	<skos:prefLabel xml:lang="fr">gélifact</skos:prefLabel>
	<skos:prefLabel xml:lang="de">Gelifakt</skos:prefLabel>
	<skos:broader rdf:resource="https://ark.frantiq.fr/ark:/26678/pcrt33sf88d6jh"/>
	<skos:inScheme rdf:resource="https://ark.frantiq.fr/ark:/26678/TH_1"/>
	<opentheso:memberOf rdf:resource="https://ark.frantiq.fr/ark:/26678/pcrtv66rn9cbv1"/>
	<opentheso:memberOf rdf:resource="https://ark.frantiq.fr/ark:/26678/pcrtnbDLi2FkAj"/>
	<dcterms:created rdf:datatype="http://www.w3.org/2001/XMLSchema#date">2021-02-12</dcterms:created>
	<dcterms:modified rdf:datatype="http://www.w3.org/2001/XMLSchema#date">2025-01-17</dcterms:modified>
	<dcterms:identifier>266375</dcterms:identifier>
	<dcterms:contributor>blandine.nouvel</dcterms:contributor>
	<skos:definition xml:lang="en">Natural lithic object or geofact resulting from the fractionation of a rock by gelifraction, i.e. a succession of freezing and thawing phases (Fernandes et al.: Vade-mecum pour la caractérisation pétroarchéologique des silicites, 2024).</skos:definition>
	<skos:definition xml:lang="fr">Objet lithique naturel ou géofact, issu du fractionnement d'une roche par gélifraction, c'est à dire succession de phases de gel et dégel (Fernandes et al. : Vade-mecum pour la caractérisation pétroarchéologique des silicites, 2024).</skos:definition>
	<skos:historyNote xml:lang="fr">2025-01-17: mise à jour de la réf. bibliographique de la définition.</skos:historyNote>
</rdf:Description>

<rdf:Description rdf:about="https://ark.frantiq.fr/ark:/26678/pcrthqg1d2ks27">
	<rdf:type rdf:resource="http://www.w3.org/2004/02/skos/core#Concept"/>
	<skos:prefLabel xml:lang="en">ventifact</skos:prefLabel>
	<skos:prefLabel xml:lang="fr">ventifact</skos:prefLabel>
	<skos:prefLabel xml:lang="it">ventifact</skos:prefLabel>
	<skos:prefLabel xml:lang="es">ventifacto</skos:prefLabel>
	<skos:prefLabel xml:lang="de">Ventifakt</skos:prefLabel>
	<skos:broader rdf:resource="https://ark.frantiq.fr/ark:/26678/pcrt33sf88d6jh"/>
	<skos:inScheme rdf:resource="https://ark.frantiq.fr/ark:/26678/TH_1"/>
	<opentheso:memberOf rdf:resource="https://ark.frantiq.fr/ark:/26678/pcrtv66rn9cbv1"/>
	<opentheso:memberOf rdf:resource="https://ark.frantiq.fr/ark:/26678/pcrtnbDLi2FkAj"/>
	<skos:exactMatch rdf:resource="https://www.wikidata.org/wiki/Q201916"/>
	<dcterms:created rdf:datatype="http://www.w3.org/2001/XMLSchema#date">2021-02-12</dcterms:created>
	<dcterms:modified rdf:datatype="http://www.w3.org/2001/XMLSchema#date">2025-01-17</dcterms:modified>
	<dcterms:identifier>266377</dcterms:identifier>
	<dcterms:contributor>blandine.nouvel</dcterms:contributor>
	<skos:definition xml:lang="en">Rock or fragment of rock abraded, pitted, engraved, grooved or polished by grains of sand or ice crystals carried by the wind (Fernandes et al.: Vade-mecum pour la caractérisation pétroarchéologique des silicites, 2024).</skos:definition>
	<skos:definition xml:lang="fr">Roche ou fragment de roche abrasé, piqueté, gravé, rainuré ou poli par des grains de sable ou&amp;amp;nbsp;des cristaux de glace entrainés par le vent (Fernandes et al. : Vade-mecum pour la caractérisation pétroarchéologique des silicites, 2024).</skos:definition>
	<skos:historyNote xml:lang="fr">2025-01-17: mise à jour de la réf. bibliographique de la définition.</skos:historyNote>
</rdf:Description>

<rdf:Description rdf:about="https://ark.frantiq.fr/ark:/26678/pcrtbpgr0h35bn">
	<rdf:type rdf:resource="http://www.w3.org/2004/02/skos/core#Concept"/>
	<skos:prefLabel xml:lang="de">Ader</skos:prefLabel>
	<skos:prefLabel xml:lang="fr">filon</skos:prefLabel>
	<skos:prefLabel xml:lang="es">filón</skos:prefLabel>
	<skos:prefLabel xml:lang="it">filone</skos:prefLabel>
	<skos:prefLabel xml:lang="en">subvolcanic rock</skos:prefLabel>
	<skos:altLabel xml:lang="en">hypabyssal rock</skos:altLabel>
	<skos:altLabel xml:lang="es">vena</skos:altLabel>
	<skos:altLabel xml:lang="it">vena</skos:altLabel>
	<skos:broader rdf:resource="https://ark.frantiq.fr/ark:/26678/pcrtw8nqd0wpmc"/>
	<skos:inScheme rdf:resource="https://ark.frantiq.fr/ark:/26678/TH_1"/>
	<opentheso:memberOf rdf:resource="https://ark.frantiq.fr/ark:/26678/pcrtv66rn9cbv1"/>
	<opentheso:memberOf rdf:resource="https://ark.frantiq.fr/ark:/26678/pcrtnbDLi2FkAj"/>
	<skos:exactMatch rdf:resource="https://www.wikidata.org/wiki/Q2323389"/>
	<dcterms:created rdf:datatype="http://www.w3.org/2001/XMLSchema#date">2021-02-12</dcterms:created>
	<dcterms:modified rdf:datatype="http://www.w3.org/2001/XMLSchema#date">2025-01-17</dcterms:modified>
	<dcterms:identifier>266379</dcterms:identifier>
	<dcterms:contributor>blandine.nouvel</dcterms:contributor>
	<dcterms:contributor>justine.vincent</dcterms:contributor>
	<skos:definition xml:lang="fr">Lame de roche issue du remplissage d'une fracture ouverte et recoupant des roches de nature variée (roches encaissantes) (Fernandes et al. : Vade-mecum pour la caractérisation pétroarchéologique des silicites, 2024).</skos:definition>
	<skos:definition xml:lang="en">A layer of rock resulting from the filling of an open fracture and intersecting rocks of various types (country rocks) (Fernandes et al.: Vade-mecum pour la caractérisation pétroarchéologique des silicites, 2024).</skos:definition>
	<skos:historyNote xml:lang="fr">2025-01-17: mise à jour de la réf. bibliographique de la définition.</skos:historyNote>
</rdf:Description>

<rdf:Description rdf:about="https://ark.frantiq.fr/ark:/26678/pcrtn97gqkmvfx">
	<rdf:type rdf:resource="http://www.w3.org/2004/02/skos/core#Concept"/>
	<skos:prefLabel xml:lang="it">arnione (geologia)</skos:prefLabel>
	<skos:prefLabel xml:lang="en">concretion (geology)</skos:prefLabel>
	<skos:prefLabel xml:lang="de">Kern (Geologie)</skos:prefLabel>
	<skos:prefLabel xml:lang="es">riñón (geología)</skos:prefLabel>
	<skos:prefLabel xml:lang="fr">rognon (géologie)</skos:prefLabel>
	<skos:altLabel xml:lang="en">nodule (geology)</skos:altLabel>
	<skos:altLabel xml:lang="en">small block of mineral material surrounded in a layer of different rock</skos:altLabel>
	<skos:narrower rdf:resource="https://ark.frantiq.fr/ark:/26678/pcrt58n6q7897s"/>
	<skos:narrower rdf:resource="https://ark.frantiq.fr/ark:/26678/pcrtrmhr3gdwhf"/>
	<skos:narrower rdf:resource="https://ark.frantiq.fr/ark:/26678/pcrtp8m4m99q9m"/>
	<skos:narrower rdf:resource="https://ark.frantiq.fr/ark:/26678/pcrt5fm9qtbrwv"/>
	<skos:broader rdf:resource="https://ark.frantiq.fr/ark:/26678/pcrtw8nqd0wpmc"/>
	<skos:inScheme rdf:resource="https://ark.frantiq.fr/ark:/26678/TH_1"/>
	<opentheso:memberOf rdf:resource="https://ark.frantiq.fr/ark:/26678/pcrtv66rn9cbv1"/>
	<opentheso:memberOf rdf:resource="https://ark.frantiq.fr/ark:/26678/pcrtnbDLi2FkAj"/>
	<skos:exactMatch rdf:resource="https://www.wikidata.org/wiki/Q3439694"/>
	<dcterms:created rdf:datatype="http://www.w3.org/2001/XMLSchema#date">2021-02-12</dcterms:created>
	<dcterms:modified rdf:datatype="http://www.w3.org/2001/XMLSchema#date">2025-01-17</dcterms:modified>
	<dcterms:identifier>266381</dcterms:identifier>
	<dcterms:contributor>blandine.nouvel</dcterms:contributor>
	<dcterms:contributor>justine.vincent</dcterms:contributor>
	<skos:definition xml:lang="en">Mineral mass of variable shape, embedded in a rock of a different nature (Fernandes et al.: Vade-mecum pour la caractérisation pétroarchéologique des silicites, 2024).</skos:definition>
	<skos:definition xml:lang="fr">Masse minérale de forme variable, enrobée dans une roche de nature différente (Fernandes et al. : Vade-mecum pour la caractérisation pétroarchéologique des silicites, 2024).</skos:definition>
	<skos:historyNote xml:lang="fr">2025-01-17: mise à jour de la réf. bibliographique de la définition.</skos:historyNote>
</rdf:Description>

<rdf:Description rdf:about="https://ark.frantiq.fr/ark:/26678/pcrt58n6q7897s">
	<rdf:type rdf:resource="http://www.w3.org/2004/02/skos/core#Concept"/>
	<skos:prefLabel xml:lang="it">arnione regolare</skos:prefLabel>
	<skos:prefLabel xml:lang="de">regelmässiger Kern</skos:prefLabel>
	<skos:prefLabel xml:lang="en">regular concretion</skos:prefLabel>
	<skos:prefLabel xml:lang="es">riñón regular</skos:prefLabel>
	<skos:prefLabel xml:lang="fr">rognon régulier</skos:prefLabel>
	<skos:altLabel xml:lang="en">regular nodule</skos:altLabel>
	<skos:altLabel xml:lang="en">regular, small block of mineral material surrounded in a layer of different rock</skos:altLabel>
	<skos:broader rdf:resource="https://ark.frantiq.fr/ark:/26678/pcrtn97gqkmvfx"/>
	<skos:inScheme rdf:resource="https://ark.frantiq.fr/ark:/26678/TH_1"/>
	<opentheso:memberOf rdf:resource="https://ark.frantiq.fr/ark:/26678/pcrtv66rn9cbv1"/>
	<opentheso:memberOf rdf:resource="https://ark.frantiq.fr/ark:/26678/pcrtnbDLi2FkAj"/>
	<dcterms:created rdf:datatype="http://www.w3.org/2001/XMLSchema#date">2021-02-12</dcterms:created>
	<dcterms:modified rdf:datatype="http://www.w3.org/2001/XMLSchema#date">2025-01-17</dcterms:modified>
	<dcterms:identifier>266383</dcterms:identifier>
	<dcterms:contributor>blandine.nouvel</dcterms:contributor>
	<dcterms:contributor>justine.vincent</dcterms:contributor>
	<skos:definition xml:lang="fr">Masse minérale arrondie de forme régulière, enrobée dans une roche de nature différente. (Fernandes et al. : Vade-mecum pour la caractérisation pétroarchéologique des silicites, 2024).</skos:definition>
	<skos:definition xml:lang="en">A rounded mineral mass of regular shape embedded in a rock of a different nature. (Fernandes et al: Vade-mecum pour la caractérisation pétroarchéologique des silicites, 2024).</skos:definition>
	<skos:historyNote xml:lang="fr">2025-01-17 : mise à jour de la réf. bibliographique dans la définition</skos:historyNote>
</rdf:Description>

<rdf:Description rdf:about="https://ark.frantiq.fr/ark:/26678/pcrtrmhr3gdwhf">
	<rdf:type rdf:resource="http://www.w3.org/2004/02/skos/core#Concept"/>
	<skos:prefLabel xml:lang="it">arnione irregolare</skos:prefLabel>
	<skos:prefLabel xml:lang="en">irregular concretion</skos:prefLabel>
	<skos:prefLabel xml:lang="es">riñón irregular</skos:prefLabel>
	<skos:prefLabel xml:lang="fr">rognon irrégulier</skos:prefLabel>
	<skos:prefLabel xml:lang="de">unregelmässiger Kern</skos:prefLabel>
	<skos:altLabel xml:lang="en">irregular nodule</skos:altLabel>
	<skos:altLabel xml:lang="en">irregular, small block of mineral material surrounded in a layer of different rock</skos:altLabel>
	<skos:broader rdf:resource="https://ark.frantiq.fr/ark:/26678/pcrtn97gqkmvfx"/>
	<skos:inScheme rdf:resource="https://ark.frantiq.fr/ark:/26678/TH_1"/>
	<opentheso:memberOf rdf:resource="https://ark.frantiq.fr/ark:/26678/pcrtv66rn9cbv1"/>
	<opentheso:memberOf rdf:resource="https://ark.frantiq.fr/ark:/26678/pcrtnbDLi2FkAj"/>
	<dcterms:created rdf:datatype="http://www.w3.org/2001/XMLSchema#date">2021-02-12</dcterms:created>
	<dcterms:modified rdf:datatype="http://www.w3.org/2001/XMLSchema#date">2025-01-17</dcterms:modified>
	<dcterms:identifier>266385</dcterms:identifier>
	<dcterms:contributor>blandine.nouvel</dcterms:contributor>
	<dcterms:contributor>justine.vincent</dcterms:contributor>
	<skos:definition xml:lang="fr">Masse minérale arrondie de forme irrégulière, enrobée dans une roche de nature différente. (Fernandes et al. : Vade-mecum pour la caractérisation pétroarchéologique des silicites, 2024).</skos:definition>
	<skos:definition xml:lang="en">A rounded mineral mass of irregular shape embedded in a rock of a different nature. (Fernandes et al: Vade-mecum pour la caractérisation pétroarchéologique des silicites, 2024).</skos:definition>
	<skos:historyNote xml:lang="fr">2025-01-17: mise à jour de la réf. bibliographique de la définition.</skos:historyNote>
</rdf:Description>

<rdf:Description rdf:about="https://ark.frantiq.fr/ark:/26678/pcrtp8m4m99q9m">
	<rdf:type rdf:resource="http://www.w3.org/2004/02/skos/core#Concept"/>
	<skos:prefLabel xml:lang="en">cerebroid concretion</skos:prefLabel>
	<skos:prefLabel xml:lang="de">hirnförmiger Kern</skos:prefLabel>
	<skos:prefLabel xml:lang="it">nodulo cerebroideo</skos:prefLabel>
	<skos:prefLabel xml:lang="fr">rognon cérébroïde</skos:prefLabel>
	<skos:altLabel xml:lang="it">arnione cerebroide</skos:altLabel>
	<skos:altLabel xml:lang="en">cerebroid nodule</skos:altLabel>
	<skos:altLabel xml:lang="en">cerebrum-shaped, small block of mineral material surrounded in a layer of different rock</skos:altLabel>
	<skos:altLabel xml:lang="es">riñón cerebroide</skos:altLabel>
	<skos:broader rdf:resource="https://ark.frantiq.fr/ark:/26678/pcrtn97gqkmvfx"/>
	<skos:inScheme rdf:resource="https://ark.frantiq.fr/ark:/26678/TH_1"/>
	<opentheso:memberOf rdf:resource="https://ark.frantiq.fr/ark:/26678/pcrtv66rn9cbv1"/>
	<opentheso:memberOf rdf:resource="https://ark.frantiq.fr/ark:/26678/pcrtnbDLi2FkAj"/>
	<dcterms:created rdf:datatype="http://www.w3.org/2001/XMLSchema#date">2021-02-12</dcterms:created>
	<dcterms:modified rdf:datatype="http://www.w3.org/2001/XMLSchema#date">2025-01-17</dcterms:modified>
	<dcterms:identifier>266387</dcterms:identifier>
	<dcterms:contributor>blandine.nouvel</dcterms:contributor>
	<dcterms:contributor>justine.vincent</dcterms:contributor>
	<skos:definition xml:lang="en">In petroarchaeology, a kidney with a wrinkled surface reminiscent of a brain (Fernandes et al.: Vade-mecum pour la caractérisation pétroarchéologique des silicites, 2024).</skos:definition>
	<skos:definition xml:lang="fr">En pétroarchéologie, rognon dont la surface ridée rappelle celle du cerveau (Fernandes et al. : Vade-mecum pour la caractérisation pétroarchéologique des silicites, 2024).</skos:definition>
	<skos:historyNote xml:lang="fr">2025-01-17: mise à jour de la réf. bibliographique de la définition.</skos:historyNote>
</rdf:Description>

<rdf:Description rdf:about="https://ark.frantiq.fr/ark:/26678/pcrt5fm9qtbrwv">
	<rdf:type rdf:resource="http://www.w3.org/2004/02/skos/core#Concept"/>
	<skos:prefLabel xml:lang="es"></skos:prefLabel>
	<skos:prefLabel xml:lang="it">nodulo talassinoide</skos:prefLabel>
	<skos:prefLabel xml:lang="fr">rognon thalassinoïde</skos:prefLabel>
	<skos:prefLabel xml:lang="en">thalassinoide concretion</skos:prefLabel>
	<skos:prefLabel xml:lang="de">thalassinoider Kern</skos:prefLabel>
	<skos:altLabel xml:lang="es">riñón thalassinoide</skos:altLabel>
	<skos:altLabel xml:lang="en">thalassinoide nodule</skos:altLabel>
	<skos:altLabel xml:lang="en">thalassinoide-shaped, small block of mineral material surrounded in a layer of different rock</skos:altLabel>
	<skos:broader rdf:resource="https://ark.frantiq.fr/ark:/26678/pcrtn97gqkmvfx"/>
	<skos:inScheme rdf:resource="https://ark.frantiq.fr/ark:/26678/TH_1"/>
	<opentheso:memberOf rdf:resource="https://ark.frantiq.fr/ark:/26678/pcrtv66rn9cbv1"/>
	<opentheso:memberOf rdf:resource="https://ark.frantiq.fr/ark:/26678/pcrtnbDLi2FkAj"/>
	<dcterms:created rdf:datatype="http://www.w3.org/2001/XMLSchema#date">2021-02-12</dcterms:created>
	<dcterms:modified rdf:datatype="http://www.w3.org/2001/XMLSchema#date">2025-01-17</dcterms:modified>
	<dcterms:identifier>266389</dcterms:identifier>
	<dcterms:contributor>blandine.nouvel</dcterms:contributor>
	<dcterms:contributor>justine.vincent</dcterms:contributor>
	<skos:definition xml:lang="en">Fossil traces of burrows forming a network of dichotomous or branched tubes that extend both vertically and horizontally (Fernandes et al.: Vade-mecum pour la caractérisation pétroarchéologique des silicites, 2024).</skos:definition>
	<skos:definition xml:lang="fr">Traces fossiles de terriers formant un réseau de tubes dichotomiques ou ramifiés qui s'étendent à la fois verticalement et horizontalement (Fernandes et al. : Vade-mecum pour la caractérisation pétroarchéologique des silicites, 2024).</skos:definition>
	<skos:historyNote xml:lang="fr">2024-11-19 : modification de la définition.</skos:historyNote>
</rdf:Description>

<rdf:Description rdf:about="https://ark.frantiq.fr/ark:/26678/pcrtf4mt37h0q8">
	<rdf:type rdf:resource="http://www.w3.org/2004/02/skos/core#Concept"/>
	<skos:prefLabel xml:lang="it">ciottolo di mare</skos:prefLabel>
	<skos:prefLabel xml:lang="fr">galet impressionné</skos:prefLabel>
	<skos:prefLabel xml:lang="es">guijarro de mar</skos:prefLabel>
	<skos:prefLabel xml:lang="de">Kiesel mit natürlichen Abdrücken</skos:prefLabel>
	<skos:prefLabel xml:lang="en">shaped pebble</skos:prefLabel>
	<skos:altLabel xml:lang="it">ciottolo levigato per impatto</skos:altLabel>
	<skos:altLabel xml:lang="fr">galet à impression naturelle</skos:altLabel>
	<skos:altLabel xml:lang="es">guijarro pulido por impacto</skos:altLabel>
	<skos:altLabel xml:lang="en">pebble shaped by contact with surrounding pebbles</skos:altLabel>
	<skos:broader rdf:resource="https://ark.frantiq.fr/ark:/26678/pcrtTgttY2SfBr"/>
	<skos:inScheme rdf:resource="https://ark.frantiq.fr/ark:/26678/TH_1"/>
	<opentheso:memberOf rdf:resource="https://ark.frantiq.fr/ark:/26678/pcrtv66rn9cbv1"/>
	<opentheso:memberOf rdf:resource="https://ark.frantiq.fr/ark:/26678/pcrtnbDLi2FkAj"/>
	<dcterms:created rdf:datatype="http://www.w3.org/2001/XMLSchema#date">2021-02-12</dcterms:created>
	<dcterms:modified rdf:datatype="http://www.w3.org/2001/XMLSchema#date">2023-08-02</dcterms:modified>
	<dcterms:identifier>266391</dcterms:identifier>
	<dcterms:contributor>blandine.nouvel</dcterms:contributor>
	<skos:definition xml:lang="en">Marine pebble, with a surface hollowed with small or large cupules as a result of the penetration of neighbouring pebbles or gravel (Fernandes, 2012)</skos:definition>
	<skos:definition xml:lang="fr">Galet de façonnage marin, à surface superficiellement creusée de petites ou grandes cupules suite à la pénétration des galets ou graviers voisins (Fernandes, 2012)</skos:definition>
</rdf:Description>

<rdf:Description rdf:about="https://ark.frantiq.fr/ark:/26678/pcrt6867pw8dnx">
	<rdf:type rdf:resource="http://www.w3.org/2004/02/skos/core#Concept"/>
	<skos:prefLabel xml:lang="it">ciottolo a superficie liscia</skos:prefLabel>
	<skos:prefLabel xml:lang="fr">galet au néocortex lisse</skos:prefLabel>
	<skos:prefLabel xml:lang="es">guijarro con superficie lisa</skos:prefLabel>
	<skos:prefLabel xml:lang="de">Kiesel mit glatter Rinde</skos:prefLabel>
	<skos:prefLabel xml:lang="en">pebble with smooth neo-cortex</skos:prefLabel>
	<skos:broader rdf:resource="https://ark.frantiq.fr/ark:/26678/pcrtTgttY2SfBr"/>
	<skos:inScheme rdf:resource="https://ark.frantiq.fr/ark:/26678/TH_1"/>
	<opentheso:memberOf rdf:resource="https://ark.frantiq.fr/ark:/26678/pcrtv66rn9cbv1"/>
	<opentheso:memberOf rdf:resource="https://ark.frantiq.fr/ark:/26678/pcrtnbDLi2FkAj"/>
	<dcterms:created rdf:datatype="http://www.w3.org/2001/XMLSchema#date">2021-02-12</dcterms:created>
	<dcterms:modified rdf:datatype="http://www.w3.org/2001/XMLSchema#date">2025-01-17</dcterms:modified>
	<dcterms:identifier>266393</dcterms:identifier>
	<dcterms:contributor>blandine.nouvel</dcterms:contributor>
	<skos:definition xml:lang="en">Fragment of rock rounded by mechanical wear and severe weathering, resulting in the disappearance of the original roughness (Fernandes et al.: Vade-mecum pour la caractérisation pétroarchéologique des silicites, 2024).</skos:definition>
	<skos:definition xml:lang="fr">Fragment de roche arrondi par une usure mécanique et une altération forte qui ont entrainé une disparition de la rugosité d'origine (Fernandes et al. : Vade-mecum pour la caractérisation pétroarchéologique des silicites, 2024).</skos:definition>
	<skos:historyNote xml:lang="fr">2025-01-17: mise à jour de la réf. bibliographique de la définition.</skos:historyNote>
</rdf:Description>

<rdf:Description rdf:about="https://ark.frantiq.fr/ark:/26678/pcrtrsjrghq6f8">
	<rdf:type rdf:resource="http://www.w3.org/2004/02/skos/core#Concept"/>
	<skos:prefLabel xml:lang="it">ciottolo a superficie rugosa</skos:prefLabel>
	<skos:prefLabel xml:lang="fr">galet au néocortex rugueux</skos:prefLabel>
	<skos:prefLabel xml:lang="es">guijarro con superficie rugosa</skos:prefLabel>
	<skos:prefLabel xml:lang="de">Kiesel mit rauher Rinde</skos:prefLabel>
	<skos:prefLabel xml:lang="en">pebble with rough neo-cortex</skos:prefLabel>
	<skos:broader rdf:resource="https://ark.frantiq.fr/ark:/26678/pcrtTgttY2SfBr"/>
	<skos:inScheme rdf:resource="https://ark.frantiq.fr/ark:/26678/TH_1"/>
	<opentheso:memberOf rdf:resource="https://ark.frantiq.fr/ark:/26678/pcrtv66rn9cbv1"/>
	<opentheso:memberOf rdf:resource="https://ark.frantiq.fr/ark:/26678/pcrtnbDLi2FkAj"/>
	<dcterms:created rdf:datatype="http://www.w3.org/2001/XMLSchema#date">2021-02-12</dcterms:created>
	<dcterms:modified rdf:datatype="http://www.w3.org/2001/XMLSchema#date">2025-01-17</dcterms:modified>
	<dcterms:identifier>266395</dcterms:identifier>
	<dcterms:contributor>blandine.nouvel</dcterms:contributor>
	<skos:definition xml:lang="en">Fragment of rolled rock, characterised by late but strong alteration that has affected mechanical wear and caused a new roughness to appear on the surfaces (Fernandes et al.: Vade-mecum pour la caractérisation pétroarchéologique des silicites, 2024).</skos:definition>
	<skos:definition xml:lang="fr">Fragment de roche roulé, caractérisé par une altération tardive mais forte qui a impacté l'usure mécanique et provoqué l'apparition d'une nouvelle rugosité sur les surfaces (Fernandes et al. : Vade-mecum pour la caractérisation pétroarchéologique des silicites, 2024).</skos:definition>
	<skos:historyNote xml:lang="fr">2025-01-17: mise à jour de la réf. bibliographique de la définition.</skos:historyNote>
</rdf:Description>

<rdf:Description rdf:about="https://ark.frantiq.fr/ark:/26678/pcrtbn5hw6ktqk">
	<rdf:type rdf:resource="http://www.w3.org/2004/02/skos/core#Concept"/>
	<skos:prefLabel xml:lang="en">DNA sense (molecular biology)</skos:prefLabel>
	<skos:prefLabel xml:lang="de">genetische Polarität</skos:prefLabel>
	<skos:prefLabel xml:lang="it">polarità (genetica)</skos:prefLabel>
	<skos:prefLabel xml:lang="fr">polarité génétique</skos:prefLabel>
	<skos:prefLabel xml:lang="es">sentido (genética)</skos:prefLabel>
	<skos:narrower rdf:resource="https://ark.frantiq.fr/ark:/26678/pcrtcvphm3f016"/>
	<skos:narrower rdf:resource="https://ark.frantiq.fr/ark:/26678/pcrtrb58t07tzv"/>
	<skos:narrower rdf:resource="https://ark.frantiq.fr/ark:/26678/pcrt1z89xc4r6g"/>
	<skos:narrower rdf:resource="https://ark.frantiq.fr/ark:/26678/pcrt36f77fdd1n"/>
	<skos:narrower rdf:resource="https://ark.frantiq.fr/ark:/26678/pcrtk20v37cf0s"/>
	<skos:narrower rdf:resource="https://ark.frantiq.fr/ark:/26678/pcrtd94cn7xznh"/>
	<skos:broader rdf:resource="https://ark.frantiq.fr/ark:/26678/pcrtr5vk7w9vdz"/>
	<skos:inScheme rdf:resource="https://ark.frantiq.fr/ark:/26678/TH_1"/>
	<opentheso:memberOf rdf:resource="https://ark.frantiq.fr/ark:/26678/pcrtv66rn9cbv1"/>
	<opentheso:memberOf rdf:resource="https://ark.frantiq.fr/ark:/26678/pcrtnbDLi2FkAj"/>
	<dcterms:created rdf:datatype="http://www.w3.org/2001/XMLSchema#date">2021-02-12</dcterms:created>
	<dcterms:modified rdf:datatype="http://www.w3.org/2001/XMLSchema#date">2025-01-17</dcterms:modified>
	<dcterms:identifier>266397</dcterms:identifier>
	<dcterms:contributor>blandine.nouvel</dcterms:contributor>
	<skos:definition xml:lang="en">Property of sedimentary rocks that present two surfaces with different characteristics, each of which has a significance in terms of genetic origin (Fernandes et al.: Vade-mecum pour la caractérisation pétroarchéologique des silicites, 2024).</skos:definition>
	<skos:definition xml:lang="fr">Propriété des roches sédimentaires qui présentent deux surfaces aux caractéristiques différentes qui ont chacune une signification en termes d'origine génétique (Fernandes et al. : Vade-mecum pour la caractérisation pétroarchéologique des silicites, 2024).</skos:definition>
	<skos:historyNote xml:lang="fr">2025-01-17: mise à jour de la réf. bibliographique de la définition.</skos:historyNote>
</rdf:Description>

<rdf:Description rdf:about="https://ark.frantiq.fr/ark:/26678/pcrtcvphm3f016">
	<rdf:type rdf:resource="http://www.w3.org/2004/02/skos/core#Concept"/>
	<skos:prefLabel xml:lang="es">ondulitas</skos:prefLabel>
	<skos:prefLabel xml:lang="en">ripple marks</skos:prefLabel>
	<skos:prefLabel xml:lang="fr">ripple marks</skos:prefLabel>
	<skos:prefLabel xml:lang="it">ripple marks</skos:prefLabel>
	<skos:prefLabel xml:lang="de">Strömungsrippeln</skos:prefLabel>
	<skos:altLabel xml:lang="fr">ride de courant</skos:altLabel>
	<skos:altLabel xml:lang="fr">ride de plage</skos:altLabel>
	<skos:altLabel xml:lang="es">ripple marks</skos:altLabel>
	<skos:altLabel xml:lang="it">ripples</skos:altLabel>
	<skos:altLabel xml:lang="es">rizaduras</skos:altLabel>
	<skos:broader rdf:resource="https://ark.frantiq.fr/ark:/26678/pcrtbn5hw6ktqk"/>
	<skos:inScheme rdf:resource="https://ark.frantiq.fr/ark:/26678/TH_1"/>
	<opentheso:memberOf rdf:resource="https://ark.frantiq.fr/ark:/26678/pcrtv66rn9cbv1"/>
	<opentheso:memberOf rdf:resource="https://ark.frantiq.fr/ark:/26678/pcrtnbDLi2FkAj"/>
	<dcterms:created rdf:datatype="http://www.w3.org/2001/XMLSchema#date">2021-02-12</dcterms:created>
	<dcterms:modified rdf:datatype="http://www.w3.org/2001/XMLSchema#date">2025-01-17</dcterms:modified>
	<dcterms:identifier>266399</dcterms:identifier>
	<dcterms:contributor>blandine.nouvel</dcterms:contributor>
	<dcterms:contributor>justine.vincent</dcterms:contributor>
	<skos:definition xml:lang="en">Natural mark left on a rock surface by the action of water currents. (Fernandes et al: Vade-mecum pour la caractérisation pétroarchéologique des silicites, 2024).</skos:definition>
	<skos:definition xml:lang="fr">Marque naturelle laissée sur une des surfaces de la roche par l'action des courants aquatiques. (Fernandes et al. : Vade-mecum pour la caractérisation pétroarchéologique des silicites, 2024).</skos:definition>
	<skos:historyNote xml:lang="fr">2025-01-17: mise à jour de la réf. bibliographique de la définition.</skos:historyNote>
</rdf:Description>

<rdf:Description rdf:about="https://ark.frantiq.fr/ark:/26678/pcrtrb58t07tzv">
	<rdf:type rdf:resource="http://www.w3.org/2004/02/skos/core#Concept"/>
	<skos:prefLabel xml:lang="es">flute marks</skos:prefLabel>
	<skos:prefLabel xml:lang="fr">flute marks</skos:prefLabel>
	<skos:prefLabel xml:lang="it">flute marks</skos:prefLabel>
	<skos:prefLabel xml:lang="de">Kolkmarke</skos:prefLabel>
	<skos:prefLabel xml:lang="en">sole marks</skos:prefLabel>
	<skos:altLabel xml:lang="es">calcos de flujo</skos:altLabel>
	<skos:altLabel xml:lang="de">Fliessmarke</skos:altLabel>
	<skos:altLabel xml:lang="fr">flute cast</skos:altLabel>
	<skos:altLabel xml:lang="en">flute casts</skos:altLabel>
	<skos:altLabel xml:lang="it">flute casts</skos:altLabel>
	<skos:altLabel xml:lang="it">sole marks</skos:altLabel>
	<skos:altLabel xml:lang="it">strutture erosive</skos:altLabel>
	<skos:broader rdf:resource="https://ark.frantiq.fr/ark:/26678/pcrtbn5hw6ktqk"/>
	<skos:inScheme rdf:resource="https://ark.frantiq.fr/ark:/26678/TH_1"/>
	<opentheso:memberOf rdf:resource="https://ark.frantiq.fr/ark:/26678/pcrtv66rn9cbv1"/>
	<opentheso:memberOf rdf:resource="https://ark.frantiq.fr/ark:/26678/pcrtnbDLi2FkAj"/>
	<dcterms:created rdf:datatype="http://www.w3.org/2001/XMLSchema#date">2021-02-12</dcterms:created>
	<dcterms:modified rdf:datatype="http://www.w3.org/2001/XMLSchema#date">2025-01-17</dcterms:modified>
	<dcterms:identifier>266401</dcterms:identifier>
	<dcterms:contributor>blandine.nouvel</dcterms:contributor>
	<dcterms:contributor>justine.vincent</dcterms:contributor>
	<skos:definition xml:lang="fr">Figures sédimentaires formées à la surface des bancs par affouillement du fond marin par des courants d'eau (vortex), reconnaissables par leur forme oblongue, allongée ou triangulaire dont la  queue  indique le sens du courant. (Fernandes et al. : Vademecum pour la caractérisation pétrorarchéologique des silicites, 2024).</skos:definition>
	<skos:definition xml:lang="en">Sedimentary figures formed on the surface of banks by the scouring of the seabed by water currents (vortexes), recognisable by their oblong, elongated or triangular shape with the tail indicating the direction of the current (Fernandes et al: Vademecum pour la caractérisation pétrorarchéologique des silicites, 2024).</skos:definition>
	<skos:historyNote xml:lang="fr">2025-01-17: mise à jour de la réf. bibliographique de la définition.</skos:historyNote>
</rdf:Description>

<rdf:Description rdf:about="https://ark.frantiq.fr/ark:/26678/pcrt1z89xc4r6g">
	<rdf:type rdf:resource="http://www.w3.org/2004/02/skos/core#Concept"/>
	<skos:prefLabel xml:lang="fr">figure en croissant</skos:prefLabel>
	<skos:prefLabel xml:lang="de">Hindernismarke</skos:prefLabel>
	<skos:prefLabel xml:lang="es">marcas de obstáculos en medialuna</skos:prefLabel>
	<skos:prefLabel xml:lang="en">obstacle scour</skos:prefLabel>
	<skos:prefLabel xml:lang="it">obstacle scour</skos:prefLabel>
	<skos:altLabel xml:lang="en">obstacle mark</skos:altLabel>
	<skos:altLabel xml:lang="es">obstacle scour</skos:altLabel>
	<skos:broader rdf:resource="https://ark.frantiq.fr/ark:/26678/pcrtbn5hw6ktqk"/>
	<skos:inScheme rdf:resource="https://ark.frantiq.fr/ark:/26678/TH_1"/>
	<opentheso:memberOf rdf:resource="https://ark.frantiq.fr/ark:/26678/pcrtv66rn9cbv1"/>
	<opentheso:memberOf rdf:resource="https://ark.frantiq.fr/ark:/26678/pcrtnbDLi2FkAj"/>
	<dcterms:created rdf:datatype="http://www.w3.org/2001/XMLSchema#date">2021-02-12</dcterms:created>
	<dcterms:modified rdf:datatype="http://www.w3.org/2001/XMLSchema#date">2025-01-17</dcterms:modified>
	<dcterms:identifier>266403</dcterms:identifier>
	<dcterms:contributor>blandine.nouvel</dcterms:contributor>
	<skos:definition xml:lang="en">Sedimentary figures formed by water currents around an object on the seabed (Fernandes et al.: Vade-mecum pour la caractérisation pétroarchéologique des silicites, 2024).</skos:definition>
	<skos:definition xml:lang="fr">Figures sédimentaires formées par des courants d'eau autour d'un objet posé sur le fond (Fernandes et al. : Vade-mecum pour la caractérisation pétroarchéologique des silicites, 2024).</skos:definition>
	<skos:historyNote xml:lang="fr">2025-01-17: mise à jour de la réf. bibliographique de la définition.</skos:historyNote>
</rdf:Description>

<rdf:Description rdf:about="https://ark.frantiq.fr/ark:/26678/pcrt36f77fdd1n">
	<rdf:type rdf:resource="http://www.w3.org/2004/02/skos/core#Concept"/>
	<skos:prefLabel xml:lang="en">rills marks</skos:prefLabel>
	<skos:prefLabel xml:lang="es">rills marks</skos:prefLabel>
	<skos:prefLabel xml:lang="fr">rills marks</skos:prefLabel>
	<skos:prefLabel xml:lang="it">rills marks</skos:prefLabel>
	<skos:prefLabel xml:lang="de">Rippelmarke</skos:prefLabel>
	<skos:altLabel xml:lang="en">rills</skos:altLabel>
	<skos:broader rdf:resource="https://ark.frantiq.fr/ark:/26678/pcrtbn5hw6ktqk"/>
	<skos:inScheme rdf:resource="https://ark.frantiq.fr/ark:/26678/TH_1"/>
	<opentheso:memberOf rdf:resource="https://ark.frantiq.fr/ark:/26678/pcrtv66rn9cbv1"/>
	<opentheso:memberOf rdf:resource="https://ark.frantiq.fr/ark:/26678/pcrtnbDLi2FkAj"/>
	<dcterms:created rdf:datatype="http://www.w3.org/2001/XMLSchema#date">2021-02-12</dcterms:created>
	<dcterms:modified rdf:datatype="http://www.w3.org/2001/XMLSchema#date">2025-01-17</dcterms:modified>
	<dcterms:identifier>266405</dcterms:identifier>
	<dcterms:contributor>blandine.nouvel</dcterms:contributor>
	<dcterms:contributor>justine.vincent</dcterms:contributor>
	<skos:definition xml:lang="en">Sedimentary figures controlled by runoff on a muddy sediment, forming a hierarchical network with an arborescent, dendritic or fractal character (Fernandes et al.: Vade-mecum pour la caractérisation pétroarchéologique des silicites, 2024).</skos:definition>
	<skos:definition xml:lang="fr">Figures sédimentaires contrôlées par le ruissellement sur un sédiment boueux dessinant un réseau hiérarchisé à caractère arborescent, dendritique ou fractal. (Fernandes et al. : Vade-mecum pour la caractérisation pétroarchéologique des silicites, 2024).</skos:definition>
	<skos:historyNote xml:lang="fr">2025-01-17: mise à jour de la réf. bibliographique de la définition.</skos:historyNote>
</rdf:Description>

<rdf:Description rdf:about="https://ark.frantiq.fr/ark:/26678/pcrtk20v37cf0s">
	<rdf:type rdf:resource="http://www.w3.org/2004/02/skos/core#Concept"/>
	<skos:prefLabel xml:lang="it">fessura da disseccamento</skos:prefLabel>
	<skos:prefLabel xml:lang="fr">figure de dessication</skos:prefLabel>
	<skos:prefLabel xml:lang="es">grieta de desecación</skos:prefLabel>
	<skos:prefLabel xml:lang="en">mud crack</skos:prefLabel>
	<skos:prefLabel xml:lang="de">Trockenriss</skos:prefLabel>
	<skos:altLabel xml:lang="en">cracked mud</skos:altLabel>
	<skos:altLabel xml:lang="en">dessication crack</skos:altLabel>
	<skos:altLabel xml:lang="es">estructura agrietada</skos:altLabel>
	<skos:altLabel xml:lang="es">grieta de lodo</skos:altLabel>
	<skos:altLabel xml:lang="es">grieta de resecación</skos:altLabel>
	<skos:altLabel xml:lang="es">lodo agrietado</skos:altLabel>
	<skos:altLabel xml:lang="es">mud crack</skos:altLabel>
	<skos:altLabel xml:lang="fr">mud crack</skos:altLabel>
	<skos:altLabel xml:lang="it">mud crack</skos:altLabel>
	<skos:altLabel xml:lang="en">mudcrack</skos:altLabel>
	<skos:altLabel xml:lang="it">poligoni da disseccamento</skos:altLabel>
	<skos:altLabel xml:lang="it">strutture da disseccamento</skos:altLabel>
	<skos:broader rdf:resource="https://ark.frantiq.fr/ark:/26678/pcrtbn5hw6ktqk"/>
	<skos:inScheme rdf:resource="https://ark.frantiq.fr/ark:/26678/TH_1"/>
	<opentheso:memberOf rdf:resource="https://ark.frantiq.fr/ark:/26678/pcrtv66rn9cbv1"/>
	<opentheso:memberOf rdf:resource="https://ark.frantiq.fr/ark:/26678/pcrtnbDLi2FkAj"/>
	<dcterms:created rdf:datatype="http://www.w3.org/2001/XMLSchema#date">2021-02-12</dcterms:created>
	<dcterms:modified rdf:datatype="http://www.w3.org/2001/XMLSchema#date">2025-01-17</dcterms:modified>
	<dcterms:identifier>266407</dcterms:identifier>
	<dcterms:contributor>blandine.nouvel</dcterms:contributor>
	<skos:definition xml:lang="en">Sedimentary pattern controlled by water loss (surface evaporation), forming shrinkage cracks in a more or less polygonal network. (Fernandes et al: Vade-mecum pour la caractérisation pétroarchéologique des silicites, 2024).</skos:definition>
	<skos:definition xml:lang="fr">Figure sédimentaire contrôlée par la perte en eau (évaporation de surface), formant des fissures de retrait en réseau plus ou moins polygonal. (Fernandes et al. : Vade-mecum pour la caractérisation pétroarchéologique des silicites, 2024).</skos:definition>
	<skos:historyNote xml:lang="fr">2025-01-17: mise à jour de la réf. bibliographique de la définition.</skos:historyNote>
</rdf:Description>

<rdf:Description rdf:about="https://ark.frantiq.fr/ark:/26678/pcrtd94cn7xznh">
	<rdf:type rdf:resource="http://www.w3.org/2004/02/skos/core#Concept"/>
	<skos:prefLabel xml:lang="es">tool marks</skos:prefLabel>
	<skos:prefLabel xml:lang="fr">tool marks</skos:prefLabel>
	<skos:prefLabel xml:lang="it">tool marks</skos:prefLabel>
	<skos:prefLabel xml:lang="en">tools  marks</skos:prefLabel>
	<skos:prefLabel xml:lang="de">Werkzeugmarken</skos:prefLabel>
	<skos:altLabel xml:lang="es">marcas de herramientas</skos:altLabel>
	<skos:altLabel xml:lang="it">strutture da impatto</skos:altLabel>
	<skos:broader rdf:resource="https://ark.frantiq.fr/ark:/26678/pcrtbn5hw6ktqk"/>
	<skos:inScheme rdf:resource="https://ark.frantiq.fr/ark:/26678/TH_1"/>
	<opentheso:memberOf rdf:resource="https://ark.frantiq.fr/ark:/26678/pcrtv66rn9cbv1"/>
	<opentheso:memberOf rdf:resource="https://ark.frantiq.fr/ark:/26678/pcrtnbDLi2FkAj"/>
	<dcterms:created rdf:datatype="http://www.w3.org/2001/XMLSchema#date">2021-02-12</dcterms:created>
	<dcterms:modified rdf:datatype="http://www.w3.org/2001/XMLSchema#date">2025-01-17</dcterms:modified>
	<dcterms:identifier>266411</dcterms:identifier>
	<dcterms:contributor>blandine.nouvel</dcterms:contributor>
	<dcterms:contributor>justine.vincent</dcterms:contributor>
	<skos:definition xml:lang="en">Sedimentary figures formed by traces of the impact of a solid object (pebbles, boulders, gravel, etc.) transported by a current of water over a muddy bottom and observed in moulding in the overlying layer (Fernandes et al.: Vade-mecum pour la caractérisation pétroarchéologique des silicites, 2024).</skos:definition>
	<skos:definition xml:lang="fr">Figures sédimentaires formées par des traces d'impact d'un objet solide (galets, blocs, graviers…) transporté par un courant d'eau sur un fond boueux et observable en moulage dans la couche sus-jacente (Fernandes et al. : Vade-mecum pour la caractérisation pétroarchéologique des silicites, 2024).</skos:definition>
	<skos:historyNote xml:lang="fr">2025-01-17: mise à jour de la réf. bibliographique de la définition.</skos:historyNote>
</rdf:Description>

<rdf:Description rdf:about="https://ark.frantiq.fr/ark:/26678/pcrt094rdqsfbv">
	<rdf:type rdf:resource="http://www.w3.org/2004/02/skos/core#Concept"/>
	<skos:prefLabel xml:lang="de">Zonalität (Gesteinskunde)</skos:prefLabel>
	<skos:prefLabel xml:lang="fr">zonalité (pétrographie)</skos:prefLabel>
	<skos:prefLabel xml:lang="en">zonality (petrography/lithics)</skos:prefLabel>
	<skos:prefLabel xml:lang="it">zonatura (petrografia)</skos:prefLabel>
	<skos:prefLabel xml:lang="es">zonificación (petrografía)</skos:prefLabel>
	<skos:altLabel xml:lang="it">caratterizzazione zonale</skos:altLabel>
	<skos:related rdf:resource="https://ark.frantiq.fr/ark:/26678/pcrtkwk6bz94r3"/>
	<skos:narrower rdf:resource="https://ark.frantiq.fr/ark:/26678/pcrt21v5j62zkd"/>
	<skos:narrower rdf:resource="https://ark.frantiq.fr/ark:/26678/pcrtj8kv2v5jz0"/>
	<skos:narrower rdf:resource="https://ark.frantiq.fr/ark:/26678/pcrtc64m697d3t"/>
	<skos:narrower rdf:resource="https://ark.frantiq.fr/ark:/26678/pcrt9s23ncq2q9"/>
	<skos:narrower rdf:resource="https://ark.frantiq.fr/ark:/26678/pcrt074z9q8ng3"/>
	<skos:broader rdf:resource="https://ark.frantiq.fr/ark:/26678/pcrtr5vk7w9vdz"/>
	<skos:inScheme rdf:resource="https://ark.frantiq.fr/ark:/26678/TH_1"/>
	<opentheso:memberOf rdf:resource="https://ark.frantiq.fr/ark:/26678/pcrtv66rn9cbv1"/>
	<opentheso:memberOf rdf:resource="https://ark.frantiq.fr/ark:/26678/pcrtnbDLi2FkAj"/>
	<dcterms:created rdf:datatype="http://www.w3.org/2001/XMLSchema#date">2021-02-17</dcterms:created>
	<dcterms:modified rdf:datatype="http://www.w3.org/2001/XMLSchema#date">2024-11-18</dcterms:modified>
	<dcterms:identifier>266413</dcterms:identifier>
	<dcterms:contributor>blandine.nouvel</dcterms:contributor>
	<dcterms:contributor>justine.vincent</dcterms:contributor>
	<skos:definition xml:lang="fr">Succession de zones concentriques identifiées sur une section de roche, présentant des différences de pigmentation, de minéralogie, de structure ou de texture et de porosité, entre le centre et la surface de l'échantillon qui définissent des effets diagénétiques et post-génétiques. (d'ap. Fernandes, 2012)</skos:definition>
	<skos:definition xml:lang="en">Succession of concentric zones identified on a section of rock, showing differences in pigmentation, mineralogy, structure or texture and porosity, between the centre and the surface of the sample that define diagenetic and post-genetic effects. (d'ap. Fernandes, 2012)</skos:definition>
	<skos:historyNote xml:lang="fr">2024-11-18 : modification de la définition.</skos:historyNote>
</rdf:Description>

<rdf:Description rdf:about="https://ark.frantiq.fr/ark:/26678/pcrt21v5j62zkd">
	<rdf:type rdf:resource="http://www.w3.org/2004/02/skos/core#Concept"/>
	<skos:prefLabel xml:lang="es">cara cortical expuesta (petrografía)</skos:prefLabel>
	<skos:prefLabel xml:lang="en">cortical surface exposed (petrography/lithics)</skos:prefLabel>
	<skos:prefLabel xml:lang="de">exponierte Kortexseite</skos:prefLabel>
	<skos:prefLabel xml:lang="fr">face corticale exposée  (pétrographie)</skos:prefLabel>
	<skos:prefLabel xml:lang="it">parte corticale esposta (petrografia)</skos:prefLabel>
	<skos:altLabel xml:lang="fr">zone 1</skos:altLabel>
	<skos:related rdf:resource="https://ark.frantiq.fr/ark:/26678/pcrtqjn0rqg305"/>
	<skos:related rdf:resource="https://ark.frantiq.fr/ark:/26678/pcrtjts6bfc4zq"/>
	<skos:broader rdf:resource="https://ark.frantiq.fr/ark:/26678/pcrt094rdqsfbv"/>
	<skos:inScheme rdf:resource="https://ark.frantiq.fr/ark:/26678/TH_1"/>
	<opentheso:memberOf rdf:resource="https://ark.frantiq.fr/ark:/26678/pcrtv66rn9cbv1"/>
	<opentheso:memberOf rdf:resource="https://ark.frantiq.fr/ark:/26678/pcrtnbDLi2FkAj"/>
	<dcterms:created rdf:datatype="http://www.w3.org/2001/XMLSchema#date">2021-02-17</dcterms:created>
	<dcterms:modified rdf:datatype="http://www.w3.org/2001/XMLSchema#date">2025-01-17</dcterms:modified>
	<dcterms:identifier>266415</dcterms:identifier>
	<dcterms:contributor>blandine.nouvel</dcterms:contributor>
	<skos:definition xml:lang="en">Periphery or upper cortical zone of a rock or rock fragment (Fernandes et al.: Vade-mecum pour la caractérisation pétroarchéologique des silicites, 2024).</skos:definition>
	<skos:definition xml:lang="fr">Périphérie ou zone corticale supérieure d'une roche ou d'un fragment de roche (Fernandes et al. : Vade-mecum pour la caractérisation pétroarchéologique des silicites, 2024).</skos:definition>
	<skos:historyNote xml:lang="fr">2025-01-17: mise à jour de la réf. bibliographique de la définition.</skos:historyNote>
</rdf:Description>

<rdf:Description rdf:about="https://ark.frantiq.fr/ark:/26678/pcrtj8kv2v5jz0">
	<rdf:type rdf:resource="http://www.w3.org/2004/02/skos/core#Concept"/>
	<skos:prefLabel xml:lang="de">Auflagefläche</skos:prefLabel>
	<skos:prefLabel xml:lang="it">piano di appoggio (petrografia)</skos:prefLabel>
	<skos:prefLabel xml:lang="en">striking platform surface (petrography/lithics)</skos:prefLabel>
	<skos:prefLabel xml:lang="es">superficie de apoyo (petrografía)</skos:prefLabel>
	<skos:prefLabel xml:lang="fr">surface d'appui  (pétrographie)</skos:prefLabel>
	<skos:altLabel xml:lang="fr">zone 2</skos:altLabel>
	<skos:related rdf:resource="https://ark.frantiq.fr/ark:/26678/pcrtqjn0rqg305"/>
	<skos:related rdf:resource="https://ark.frantiq.fr/ark:/26678/pcrtjts6bfc4zq"/>
	<skos:broader rdf:resource="https://ark.frantiq.fr/ark:/26678/pcrt094rdqsfbv"/>
	<skos:inScheme rdf:resource="https://ark.frantiq.fr/ark:/26678/TH_1"/>
	<opentheso:memberOf rdf:resource="https://ark.frantiq.fr/ark:/26678/pcrtv66rn9cbv1"/>
	<opentheso:memberOf rdf:resource="https://ark.frantiq.fr/ark:/26678/pcrtnbDLi2FkAj"/>
	<dcterms:created rdf:datatype="http://www.w3.org/2001/XMLSchema#date">2021-02-17</dcterms:created>
	<dcterms:modified rdf:datatype="http://www.w3.org/2001/XMLSchema#date">2025-01-17</dcterms:modified>
	<dcterms:identifier>266417</dcterms:identifier>
	<dcterms:contributor>blandine.nouvel</dcterms:contributor>
	<skos:definition xml:lang="en">Periphery or lower cortical zone of a rock or rock fragment (Fernandes et al.: Vade-mecum pour la caractérisation pétroarchéologique des silicites, 2024).</skos:definition>
	<skos:definition xml:lang="fr">Périphérie ou zone corticale inférieure d'une roche ou d'un fragment de roche (Fernandes et al. : Vade-mecum pour la caractérisation pétroarchéologique des silicites, 2024).</skos:definition>
	<skos:historyNote xml:lang="fr">2025-01-17 : mise à jour de la réf. bibliographique dans la définition.</skos:historyNote>
</rdf:Description>

<rdf:Description rdf:about="https://ark.frantiq.fr/ark:/26678/pcrtc64m697d3t">
	<rdf:type rdf:resource="http://www.w3.org/2004/02/skos/core#Concept"/>
	<skos:prefLabel xml:lang="de">exponierte subkortikale Zone</skos:prefLabel>
	<skos:prefLabel xml:lang="es">sector subcortical expuesto (petrografía)</skos:prefLabel>
	<skos:prefLabel xml:lang="en">sub-cortical surface exposed (petrography/lithics)</skos:prefLabel>
	<skos:prefLabel xml:lang="it">zona sottocorticale esposta (petrografia)</skos:prefLabel>
	<skos:prefLabel xml:lang="fr">zone sous-corticale exposée  (pétrographie)</skos:prefLabel>
	<skos:altLabel xml:lang="fr">zone 3</skos:altLabel>
	<skos:related rdf:resource="https://ark.frantiq.fr/ark:/26678/pcrtjts6bfc4zq"/>
	<skos:broader rdf:resource="https://ark.frantiq.fr/ark:/26678/pcrt094rdqsfbv"/>
	<skos:inScheme rdf:resource="https://ark.frantiq.fr/ark:/26678/TH_1"/>
	<opentheso:memberOf rdf:resource="https://ark.frantiq.fr/ark:/26678/pcrtv66rn9cbv1"/>
	<opentheso:memberOf rdf:resource="https://ark.frantiq.fr/ark:/26678/pcrtnbDLi2FkAj"/>
	<dcterms:created rdf:datatype="http://www.w3.org/2001/XMLSchema#date">2021-02-17</dcterms:created>
	<dcterms:modified rdf:datatype="http://www.w3.org/2001/XMLSchema#date">2025-01-17</dcterms:modified>
	<dcterms:identifier>266419</dcterms:identifier>
	<dcterms:contributor>blandine.nouvel</dcterms:contributor>
	<dcterms:contributor>justine.vincent</dcterms:contributor>
	<skos:definition xml:lang="en">Upper subcortical (or endocortical) zone of a rock or rock fragment (Fernandes et al.: Vade-mecum pour la caractérisation pétroarchéologique des silicites, 2024).</skos:definition>
	<skos:definition xml:lang="fr">Zone sous corticale (ou endocorticale) supérieure d'une roche ou d'un fragment de roche (Fernandes et al. : Vade-mecum pour la caractérisation pétroarchéologique des silicites, 2024).</skos:definition>
	<skos:historyNote xml:lang="fr">2025-01-17 : mise à jour de la réf. bibliographique dans la définition.</skos:historyNote>
</rdf:Description>

<rdf:Description rdf:about="https://ark.frantiq.fr/ark:/26678/pcrt9s23ncq2q9">
	<rdf:type rdf:resource="http://www.w3.org/2004/02/skos/core#Concept"/>
	<skos:prefLabel xml:lang="de">aufliegende subkortikale Zone</skos:prefLabel>
	<skos:prefLabel xml:lang="es">sector subcortical de apoyo (petrografía)</skos:prefLabel>
	<skos:prefLabel xml:lang="en">sub-cortical striking surface (petrography/lithics)</skos:prefLabel>
	<skos:prefLabel xml:lang="it">zona sottocorticale di appoggio (petrografia)</skos:prefLabel>
	<skos:prefLabel xml:lang="fr">zone sous-corticale d'appui  (pétrographie)</skos:prefLabel>
	<skos:altLabel xml:lang="fr">zone 4</skos:altLabel>
	<skos:related rdf:resource="https://ark.frantiq.fr/ark:/26678/pcrtjts6bfc4zq"/>
	<skos:broader rdf:resource="https://ark.frantiq.fr/ark:/26678/pcrt094rdqsfbv"/>
	<skos:inScheme rdf:resource="https://ark.frantiq.fr/ark:/26678/TH_1"/>
	<opentheso:memberOf rdf:resource="https://ark.frantiq.fr/ark:/26678/pcrtv66rn9cbv1"/>
	<opentheso:memberOf rdf:resource="https://ark.frantiq.fr/ark:/26678/pcrtnbDLi2FkAj"/>
	<dcterms:created rdf:datatype="http://www.w3.org/2001/XMLSchema#date">2021-02-17</dcterms:created>
	<dcterms:modified rdf:datatype="http://www.w3.org/2001/XMLSchema#date">2025-01-17</dcterms:modified>
	<dcterms:identifier>266421</dcterms:identifier>
	<dcterms:contributor>blandine.nouvel</dcterms:contributor>
	<dcterms:contributor>justine.vincent</dcterms:contributor>
	<skos:definition xml:lang="en">Lower subcortical (or endocortical) zone of a rock or rock fragment (Fernandes et al.: Vade-mecum pour la caractérisation pétroarchéologique des silicites, 2024).</skos:definition>
	<skos:definition xml:lang="fr">Zone sous corticale (ou endocorticale) inférieure d'une roche ou d'un fragment de roche (Fernandes et al. : Vade-mecum pour la caractérisation pétroarchéologique des silicites, 2024).</skos:definition>
	<skos:historyNote xml:lang="fr">2025-01-17 : mise à jour de la réf. bibliographique dans la définition.</skos:historyNote>
</rdf:Description>

<rdf:Description rdf:about="https://ark.frantiq.fr/ark:/26678/pcrt074z9q8ng3">
	<rdf:type rdf:resource="http://www.w3.org/2004/02/skos/core#Concept"/>
	<skos:prefLabel xml:lang="en">core (petrography/lithics)</skos:prefLabel>
	<skos:prefLabel xml:lang="de">interne Zone</skos:prefLabel>
	<skos:prefLabel xml:lang="it">nucleo (petrografia)</skos:prefLabel>
	<skos:prefLabel xml:lang="es">núcleo (petrografía)</skos:prefLabel>
	<skos:prefLabel xml:lang="fr">zone interne  (pétrographie)</skos:prefLabel>
	<skos:altLabel xml:lang="fr">coeur de la roche</skos:altLabel>
	<skos:altLabel xml:lang="fr">zone 5</skos:altLabel>
	<skos:broader rdf:resource="https://ark.frantiq.fr/ark:/26678/pcrt094rdqsfbv"/>
	<skos:inScheme rdf:resource="https://ark.frantiq.fr/ark:/26678/TH_1"/>
	<opentheso:memberOf rdf:resource="https://ark.frantiq.fr/ark:/26678/pcrtv66rn9cbv1"/>
	<opentheso:memberOf rdf:resource="https://ark.frantiq.fr/ark:/26678/pcrtnbDLi2FkAj"/>
	<dcterms:created rdf:datatype="http://www.w3.org/2001/XMLSchema#date">2021-02-17</dcterms:created>
	<dcterms:modified rdf:datatype="http://www.w3.org/2001/XMLSchema#date">2025-01-17</dcterms:modified>
	<dcterms:identifier>266423</dcterms:identifier>
	<dcterms:contributor>blandine.nouvel</dcterms:contributor>
	<dcterms:contributor>justine.vincent</dcterms:contributor>
	<skos:definition xml:lang="en">Core of rock sample (Fernandes et al.: Vade-mecum pour la caractérisation pétroarchéologique des silicites, 2024).</skos:definition>
	<skos:definition xml:lang="fr">Cœur de l'échantillon rocheux (Fernandes et al. : Vade-mecum pour la caractérisation pétroarchéologique des silicites, 2024).</skos:definition>
	<skos:historyNote xml:lang="fr">2025-01-17 : mise à jour de la réf. bibliographique dans la définition.</skos:historyNote>
</rdf:Description>

<rdf:Description rdf:about="https://ark.frantiq.fr/ark:/26678/pcrtkwk6bz94r3">
	<rdf:type rdf:resource="http://www.w3.org/2004/02/skos/core#Concept"/>
	<skos:prefLabel xml:lang="es">estructura de la roca</skos:prefLabel>
	<skos:prefLabel xml:lang="de">Gesteinstruktur</skos:prefLabel>
	<skos:prefLabel xml:lang="en">stone structure (petrography/lithics)</skos:prefLabel>
	<skos:prefLabel xml:lang="fr">structure de la roche</skos:prefLabel>
	<skos:prefLabel xml:lang="it">struttura della roccia</skos:prefLabel>
	<skos:altLabel xml:lang="en">stone anatomy (petrography/lithics)</skos:altLabel>
	<skos:related rdf:resource="https://ark.frantiq.fr/ark:/26678/pcrt094rdqsfbv"/>
	<skos:narrower rdf:resource="https://ark.frantiq.fr/ark:/26678/pcrt7fsrb8ggkp"/>
	<skos:narrower rdf:resource="https://ark.frantiq.fr/ark:/26678/pcrtx3bv9c7050"/>
	<skos:narrower rdf:resource="https://ark.frantiq.fr/ark:/26678/pcrtv0rphqt1h8"/>
	<skos:narrower rdf:resource="https://ark.frantiq.fr/ark:/26678/pcrtvh6k2wqhg6"/>
	<skos:narrower rdf:resource="https://ark.frantiq.fr/ark:/26678/pcrt969pbxxbzt"/>
	<skos:narrower rdf:resource="https://ark.frantiq.fr/ark:/26678/pcrt2kpf55zh14"/>
	<skos:narrower rdf:resource="https://ark.frantiq.fr/ark:/26678/pcrtndt9zrpjjk"/>
	<skos:narrower rdf:resource="https://ark.frantiq.fr/ark:/26678/pcrtfv2krrfh1d"/>
	<skos:narrower rdf:resource="https://ark.frantiq.fr/ark:/26678/pcrtknmwxc5x5s"/>
	<skos:narrower rdf:resource="https://ark.frantiq.fr/ark:/26678/pcrtrwdpzch5wh"/>
	<skos:narrower rdf:resource="https://ark.frantiq.fr/ark:/26678/pcrth30k691qrk"/>
	<skos:narrower rdf:resource="https://ark.frantiq.fr/ark:/26678/pcrtkgmbfz0x3s"/>
	<skos:narrower rdf:resource="https://ark.frantiq.fr/ark:/26678/pcrtkrm9q3htcj"/>
	<skos:narrower rdf:resource="https://ark.frantiq.fr/ark:/26678/pcrtq764j7snt5"/>
	<skos:narrower rdf:resource="https://ark.frantiq.fr/ark:/26678/pcrtfvk3mp3dhk"/>
	<skos:narrower rdf:resource="https://ark.frantiq.fr/ark:/26678/pcrt3tmh056368"/>
	<skos:narrower rdf:resource="https://ark.frantiq.fr/ark:/26678/pcrtfz97ktt9qf"/>
	<skos:broader rdf:resource="https://ark.frantiq.fr/ark:/26678/pcrtr5vk7w9vdz"/>
	<skos:inScheme rdf:resource="https://ark.frantiq.fr/ark:/26678/TH_1"/>
	<opentheso:memberOf rdf:resource="https://ark.frantiq.fr/ark:/26678/pcrtv66rn9cbv1"/>
	<opentheso:memberOf rdf:resource="https://ark.frantiq.fr/ark:/26678/pcrtnbDLi2FkAj"/>
	<skos:exactMatch rdf:resource="https://www.wikidata.org/wiki/Q20826906"/>
	<dcterms:created rdf:datatype="http://www.w3.org/2001/XMLSchema#date">2021-02-17</dcterms:created>
	<dcterms:modified rdf:datatype="http://www.w3.org/2001/XMLSchema#date">2024-11-21</dcterms:modified>
	<dcterms:identifier>266425</dcterms:identifier>
	<dcterms:contributor>blandine.nouvel</dcterms:contributor>
	<dcterms:contributor>justine.vincent</dcterms:contributor>
	<skos:definition xml:lang="en">General appearance of the rock and its zones on a macroscopic scale (d'ap. Fernandes, 2012).</skos:definition>
	<skos:definition xml:lang="fr">Aspect général de la roche et de ses zones à l'échelle macroscopique (d'ap. Fernandes, 2012).</skos:definition>
</rdf:Description>

<rdf:Description rdf:about="https://ark.frantiq.fr/ark:/26678/pcrtqc4b4zzzmw">
	<rdf:type rdf:resource="http://www.w3.org/2004/02/skos/core#Concept"/>
	<skos:prefLabel xml:lang="it">matrice (petrografia)</skos:prefLabel>
	<skos:prefLabel xml:lang="fr">matrice (pétrographie)</skos:prefLabel>
	<skos:prefLabel xml:lang="de">Matrix (Gesteinskunde)</skos:prefLabel>
	<skos:prefLabel xml:lang="en">matrix (petrography/lithics)</skos:prefLabel>
	<skos:prefLabel xml:lang="es">matriz (petrografía)</skos:prefLabel>
	<skos:altLabel xml:lang="en">groundmass (petrography/lithics)</skos:altLabel>
	<skos:narrower rdf:resource="https://ark.frantiq.fr/ark:/26678/pcrt5bd4f5dv7r"/>
	<skos:narrower rdf:resource="https://ark.frantiq.fr/ark:/26678/pcrt5ddg241ccv"/>
	<skos:narrower rdf:resource="https://ark.frantiq.fr/ark:/26678/pcrtjmqpnw74z9"/>
	<skos:narrower rdf:resource="https://ark.frantiq.fr/ark:/26678/pcrt6pvhc29pfv"/>
	<skos:narrower rdf:resource="https://ark.frantiq.fr/ark:/26678/pcrtk8c4vv2tw8"/>
	<skos:broader rdf:resource="https://ark.frantiq.fr/ark:/26678/pcrtr5vk7w9vdz"/>
	<skos:inScheme rdf:resource="https://ark.frantiq.fr/ark:/26678/TH_1"/>
	<opentheso:memberOf rdf:resource="https://ark.frantiq.fr/ark:/26678/pcrtv66rn9cbv1"/>
	<opentheso:memberOf rdf:resource="https://ark.frantiq.fr/ark:/26678/pcrtnbDLi2FkAj"/>
	<dcterms:created rdf:datatype="http://www.w3.org/2001/XMLSchema#date">2021-02-17</dcterms:created>
	<dcterms:modified rdf:datatype="http://www.w3.org/2001/XMLSchema#date">2025-01-17</dcterms:modified>
	<dcterms:identifier>266427</dcterms:identifier>
	<dcterms:contributor>blandine.nouvel</dcterms:contributor>
	<dcterms:contributor>justine.vincent</dcterms:contributor>
	<skos:definition xml:lang="en">In a composite rock, the matrix is the binding material, made up of small grains, which coats the allochèmes specific to sedimentary rocks. In carbonate rocks, the matrix is made up of crystals of 1 to 8 µm (above 8 µm we talk about cement) (Fernandes et al.: Vade-mecum pour la caractérisation pétroarchéologique des silicites, 2024).</skos:definition>
	<skos:definition xml:lang="fr">Dans une roche composite, la matrice est le matériau liant, constitué de petits grains, qui enrobe les allochèmes spécifiques des roches sédimentaires. Pour les roches carbonatées, la matrice est constituée de cristaux de 1 à 8 µm (au-dessus de 8 µm on parle de ciment) (Fernandes et al. : Vade-mecum pour la caractérisation pétroarchéologique des silicites, 2024).</skos:definition>
	<skos:historyNote xml:lang="fr">2025-01-17 : mise à jour de la réf. bibliographique dans la définition.</skos:historyNote>
</rdf:Description>

<rdf:Description rdf:about="https://ark.frantiq.fr/ark:/26678/pcrt40qs0fvnxg">
	<rdf:type rdf:resource="http://www.w3.org/2004/02/skos/core#Concept"/>
	<skos:prefLabel xml:lang="en">allochem</skos:prefLabel>
	<skos:prefLabel xml:lang="fr">allochème</skos:prefLabel>
	<skos:prefLabel xml:lang="it">allochimico</skos:prefLabel>
	<skos:prefLabel xml:lang="es">aloquímico</skos:prefLabel>
	<skos:prefLabel xml:lang="de">Klast</skos:prefLabel>
	<skos:altLabel xml:lang="fr">allochaemia</skos:altLabel>
	<skos:altLabel xml:lang="it">allochimici</skos:altLabel>
	<skos:altLabel xml:lang="fr">claste</skos:altLabel>
	<skos:altLabel xml:lang="fr">élément figuré (pétrographie)</skos:altLabel>
	<skos:narrower rdf:resource="https://ark.frantiq.fr/ark:/26678/pcrt5nd65vnw7p"/>
	<skos:narrower rdf:resource="https://ark.frantiq.fr/ark:/26678/pcrt24wcqp2cfz"/>
	<skos:narrower rdf:resource="https://ark.frantiq.fr/ark:/26678/pcrt9qq3x37vt0"/>
	<skos:narrower rdf:resource="https://ark.frantiq.fr/ark:/26678/pcrtr06vz24nj3"/>
	<skos:narrower rdf:resource="https://ark.frantiq.fr/ark:/26678/pcrt2fhx0kftpg"/>
	<skos:narrower rdf:resource="https://ark.frantiq.fr/ark:/26678/pcrt1tm77xkqbd"/>
	<skos:narrower rdf:resource="https://ark.frantiq.fr/ark:/26678/pcrt6xvrhrkjz8"/>
	<skos:narrower rdf:resource="https://ark.frantiq.fr/ark:/26678/pcrtwz8jzr2ttd"/>
	<skos:narrower rdf:resource="https://ark.frantiq.fr/ark:/26678/pcrt4rsdrmfk1b"/>
	<skos:narrower rdf:resource="https://ark.frantiq.fr/ark:/26678/pcrtjwwb1xztxh"/>
	<skos:narrower rdf:resource="https://ark.frantiq.fr/ark:/26678/pcrt1kjsnnvmzh"/>
	<skos:narrower rdf:resource="https://ark.frantiq.fr/ark:/26678/pcrt21f986h3tk"/>
	<skos:narrower rdf:resource="https://ark.frantiq.fr/ark:/26678/pcrtqmm7q566vh"/>
	<skos:narrower rdf:resource="https://ark.frantiq.fr/ark:/26678/pcrtv3f379sr9v"/>
	<skos:narrower rdf:resource="https://ark.frantiq.fr/ark:/26678/pcrtb689mtdsz6"/>
	<skos:narrower rdf:resource="https://ark.frantiq.fr/ark:/26678/pcrt8c26426vth"/>
	<skos:broader rdf:resource="https://ark.frantiq.fr/ark:/26678/pcrtr5vk7w9vdz"/>
	<skos:inScheme rdf:resource="https://ark.frantiq.fr/ark:/26678/TH_1"/>
	<opentheso:memberOf rdf:resource="https://ark.frantiq.fr/ark:/26678/pcrtv66rn9cbv1"/>
	<opentheso:memberOf rdf:resource="https://ark.frantiq.fr/ark:/26678/pcrtnbDLi2FkAj"/>
	<iso-thes:subordinateArray rdf:resource="https://pactols.frantiq.fr/?idf=F425&amp;idt=TH_1"/>
	<iso-thes:subordinateArray rdf:resource="https://pactols.frantiq.fr/?idf=F427&amp;idt=TH_1"/>
	<skos:exactMatch rdf:resource="https://www.wikidata.org/wiki/Q4733015"/>
	<dcterms:created rdf:datatype="http://www.w3.org/2001/XMLSchema#date">2021-02-17</dcterms:created>
	<dcterms:modified rdf:datatype="http://www.w3.org/2001/XMLSchema#date">2025-01-30</dcterms:modified>
	<dcterms:identifier>266429</dcterms:identifier>
	<dcterms:contributor>blandine.nouvel</dcterms:contributor>
	<dcterms:contributor>justine.vincent</dcterms:contributor>
	<skos:definition xml:lang="en">Term coined by Folk (1959), reserved for the description of carbonate sedimentary rocks; in petroarchaeology the term is used in equivalence to figurative elements in flints (Fernandes, 2012).</skos:definition>
	<skos:definition xml:lang="fr">Terme créé par Folk (1959), réservé à la description des roches sédimentaires carbonatées ; en pétroarchéologie le terme est utilisé en équivalence d’éléments figurés dans les silex. (Fernandes, 2012)</skos:definition>
	<dcterms:source>https://doi-org.inshs.bib.cnrs.fr/10.4000/12zm5</dcterms:source>
</rdf:Description>

<rdf:Description rdf:about="https://ark.frantiq.fr/ark:/26678/pcrtsvkcb5mv2t">
	<rdf:type rdf:resource="http://www.w3.org/2004/02/skos/core#Concept"/>
	<skos:prefLabel xml:lang="en">natural rock surface</skos:prefLabel>
	<skos:prefLabel xml:lang="de">natürliche Gesteinsoberfläche</skos:prefLabel>
	<skos:prefLabel xml:lang="es">superficie natural de las rocas</skos:prefLabel>
	<skos:prefLabel xml:lang="it">superficie naturale delle rocce</skos:prefLabel>
	<skos:prefLabel xml:lang="fr">surface naturelle des roches</skos:prefLabel>
	<skos:narrower rdf:resource="https://ark.frantiq.fr/ark:/26678/pcrtqjn0rqg305"/>
	<skos:narrower rdf:resource="https://ark.frantiq.fr/ark:/26678/pcrtjts6bfc4zq"/>
	<skos:narrower rdf:resource="https://ark.frantiq.fr/ark:/26678/pcrtzpd0t7gbgz"/>
	<skos:broader rdf:resource="https://ark.frantiq.fr/ark:/26678/pcrtr5vk7w9vdz"/>
	<skos:inScheme rdf:resource="https://ark.frantiq.fr/ark:/26678/TH_1"/>
	<opentheso:memberOf rdf:resource="https://ark.frantiq.fr/ark:/26678/pcrtv66rn9cbv1"/>
	<opentheso:memberOf rdf:resource="https://ark.frantiq.fr/ark:/26678/pcrtnbDLi2FkAj"/>
	<dcterms:created rdf:datatype="http://www.w3.org/2001/XMLSchema#date">2021-02-17</dcterms:created>
	<dcterms:modified rdf:datatype="http://www.w3.org/2001/XMLSchema#date">2025-01-17</dcterms:modified>
	<dcterms:identifier>266431</dcterms:identifier>
	<dcterms:contributor>blandine.nouvel</dcterms:contributor>
	<dcterms:contributor>justine.vincent</dcterms:contributor>
	<skos:definition xml:lang="en">The peripheral part of a rock that has preserved traces of the geological and meteorological processes that structured and shaped it, and that has been partially or totally destroyed by the voluntary action of man (Fernandes et al.: Vade-mecum pour la caractérisation pétroarchéologique des silicites, 2024).</skos:definition>
	<skos:definition xml:lang="fr">Partie périphérique d'une roche qui a conservé les traces des processus géologiques et météoriques qui l'on structurée et façonné, qui disparait partiellement ou en totalité par l'action volontaire de l'homme (Fernandes et al. : Vade-mecum pour la caractérisation pétroarchéologique des silicites, 2024).</skos:definition>
	<skos:historyNote xml:lang="fr">2025-01-17 : mise à jour de la réf. bibliographique dans la définition.</skos:historyNote>
</rdf:Description>

<rdf:Description rdf:about="https://ark.frantiq.fr/ark:/26678/pcrt5m5pftg21t">
	<rdf:type rdf:resource="http://www.w3.org/2004/02/skos/core#Concept"/>
	<skos:prefLabel xml:lang="it">abbattimento della porosità</skos:prefLabel>
	<skos:prefLabel xml:lang="de">Porenzementierung</skos:prefLabel>
	<skos:prefLabel xml:lang="fr">poronécrose</skos:prefLabel>
	<skos:prefLabel xml:lang="en">poronecrosis</skos:prefLabel>
	<skos:prefLabel xml:lang="es">poronecrosis</skos:prefLabel>
	<skos:narrower rdf:resource="https://ark.frantiq.fr/ark:/26678/pcrtqh6z41brjd"/>
	<skos:narrower rdf:resource="https://ark.frantiq.fr/ark:/26678/pcrt1qsxtkgq0f"/>
	<skos:broader rdf:resource="https://ark.frantiq.fr/ark:/26678/pcrtr5vk7w9vdz"/>
	<skos:inScheme rdf:resource="https://ark.frantiq.fr/ark:/26678/TH_1"/>
	<opentheso:memberOf rdf:resource="https://ark.frantiq.fr/ark:/26678/pcrtv66rn9cbv1"/>
	<opentheso:memberOf rdf:resource="https://ark.frantiq.fr/ark:/26678/pcrtnbDLi2FkAj"/>
	<dcterms:created rdf:datatype="http://www.w3.org/2001/XMLSchema#date">2021-02-17</dcterms:created>
	<dcterms:modified rdf:datatype="http://www.w3.org/2001/XMLSchema#date">2024-11-19</dcterms:modified>
	<dcterms:identifier>266433</dcterms:identifier>
	<dcterms:contributor>blandine.nouvel</dcterms:contributor>
	<dcterms:contributor>justine.vincent</dcterms:contributor>
	<skos:definition xml:lang="en">Sealing or lining of porosity by cementing. (Fernandes et al., 2021)</skos:definition>
	<skos:definition xml:lang="fr">Colmatage ou tapissage de la porosité par cimentation. (Fernandes et al., 2021)</skos:definition>
</rdf:Description>

<rdf:Description rdf:about="https://ark.frantiq.fr/ark:/26678/pcrt0kvts48fht">
	<rdf:type rdf:resource="http://www.w3.org/2004/02/skos/core#Concept"/>
	<skos:prefLabel xml:lang="es">porosidad</skos:prefLabel>
	<skos:prefLabel xml:lang="it">porosità</skos:prefLabel>
	<skos:prefLabel xml:lang="de">Porosität</skos:prefLabel>
	<skos:prefLabel xml:lang="fr">porosité</skos:prefLabel>
	<skos:prefLabel xml:lang="en">porosity</skos:prefLabel>
	<skos:altLabel xml:lang="en">void fraction</skos:altLabel>
	<skos:narrower rdf:resource="https://ark.frantiq.fr/ark:/26678/pcrtvq05vjv1z6"/>
	<skos:narrower rdf:resource="https://ark.frantiq.fr/ark:/26678/pcrt02hj78whx8"/>
	<skos:narrower rdf:resource="https://ark.frantiq.fr/ark:/26678/pcrt96jkm5cgpf"/>
	<skos:narrower rdf:resource="https://ark.frantiq.fr/ark:/26678/pcrt776pzvkdkn"/>
	<skos:narrower rdf:resource="https://ark.frantiq.fr/ark:/26678/pcrtv9c4m3q53k"/>
	<skos:narrower rdf:resource="https://ark.frantiq.fr/ark:/26678/pcrt4n7gjb1qfh"/>
	<skos:narrower rdf:resource="https://ark.frantiq.fr/ark:/26678/pcrttkxc1k68td"/>
	<skos:narrower rdf:resource="https://ark.frantiq.fr/ark:/26678/pcrt73m1tx29mm"/>
	<skos:narrower rdf:resource="https://ark.frantiq.fr/ark:/26678/pcrtpsrh8ptqjf"/>
	<skos:narrower rdf:resource="https://ark.frantiq.fr/ark:/26678/pcrtvq01hkvvn3"/>
	<skos:narrower rdf:resource="https://ark.frantiq.fr/ark:/26678/pcrt11wm5hjnm3"/>
	<skos:narrower rdf:resource="https://ark.frantiq.fr/ark:/26678/pcrt375srxkn5s"/>
	<skos:broader rdf:resource="https://ark.frantiq.fr/ark:/26678/pcrtr5vk7w9vdz"/>
	<skos:inScheme rdf:resource="https://ark.frantiq.fr/ark:/26678/TH_1"/>
	<opentheso:memberOf rdf:resource="https://ark.frantiq.fr/ark:/26678/pcrtv66rn9cbv1"/>
	<opentheso:memberOf rdf:resource="https://ark.frantiq.fr/ark:/26678/pcrtnbDLi2FkAj"/>
	<skos:exactMatch rdf:resource="https://www.wikidata.org/wiki/Q622669"/>
	<dcterms:created rdf:datatype="http://www.w3.org/2001/XMLSchema#date">2021-02-17</dcterms:created>
	<dcterms:modified rdf:datatype="http://www.w3.org/2001/XMLSchema#date">2024-11-19</dcterms:modified>
	<dcterms:identifier>266435</dcterms:identifier>
	<dcterms:contributor>blandine.nouvel</dcterms:contributor>
	<dcterms:contributor>justine.vincent</dcterms:contributor>
	<skos:definition xml:lang="fr">Propriété d'un corps solide de comporter des vides (pores) emplis par des fluides, liquide ou gaz. (Fernandes et al., 2021)</skos:definition>
	<skos:definition xml:lang="en">Property of a solid body of having voids (pores) filled by fluids, liquid or gas. (Fernandes et al., 2021)</skos:definition>
</rdf:Description>

<rdf:Description rdf:about="https://ark.frantiq.fr/ark:/26678/pcrt7fsrb8ggkp">
	<rdf:type rdf:resource="http://www.w3.org/2004/02/skos/core#Concept"/>
	<skos:prefLabel xml:lang="es">estructura homogénea</skos:prefLabel>
	<skos:prefLabel xml:lang="en">homogeneous structure</skos:prefLabel>
	<skos:prefLabel xml:lang="de">homogene Struktur</skos:prefLabel>
	<skos:prefLabel xml:lang="fr">structure homogène</skos:prefLabel>
	<skos:prefLabel xml:lang="it">struttura omogenea</skos:prefLabel>
	<skos:broader rdf:resource="https://ark.frantiq.fr/ark:/26678/pcrtkwk6bz94r3"/>
	<skos:inScheme rdf:resource="https://ark.frantiq.fr/ark:/26678/TH_1"/>
	<opentheso:memberOf rdf:resource="https://ark.frantiq.fr/ark:/26678/pcrtv66rn9cbv1"/>
	<opentheso:memberOf rdf:resource="https://ark.frantiq.fr/ark:/26678/pcrtnbDLi2FkAj"/>
	<dcterms:created rdf:datatype="http://www.w3.org/2001/XMLSchema#date">2021-02-17</dcterms:created>
	<dcterms:modified rdf:datatype="http://www.w3.org/2001/XMLSchema#date">2024-11-21</dcterms:modified>
	<dcterms:identifier>266437</dcterms:identifier>
	<dcterms:contributor>blandine.nouvel</dcterms:contributor>
	<dcterms:contributor>justine.vincent</dcterms:contributor>
	<skos:definition xml:lang="en">The rock structure in the area studied is homogeneous (Fernandes et al., 2021).</skos:definition>
	<skos:definition xml:lang="fr">La structure de la roche dans la zone étudiée est homogène. (Fernandes et al., 2021)</skos:definition>
</rdf:Description>

<rdf:Description rdf:about="https://ark.frantiq.fr/ark:/26678/pcrtx3bv9c7050">
	<rdf:type rdf:resource="http://www.w3.org/2004/02/skos/core#Concept"/>
	<skos:prefLabel xml:lang="es">estructura heterogénea</skos:prefLabel>
	<skos:prefLabel xml:lang="en">heterogeneous structure</skos:prefLabel>
	<skos:prefLabel xml:lang="de">heterogene Struktur</skos:prefLabel>
	<skos:prefLabel xml:lang="fr">structure hétérogène</skos:prefLabel>
	<skos:prefLabel xml:lang="it">struttura eterogenea</skos:prefLabel>
	<skos:broader rdf:resource="https://ark.frantiq.fr/ark:/26678/pcrtkwk6bz94r3"/>
	<skos:inScheme rdf:resource="https://ark.frantiq.fr/ark:/26678/TH_1"/>
	<opentheso:memberOf rdf:resource="https://ark.frantiq.fr/ark:/26678/pcrtv66rn9cbv1"/>
	<opentheso:memberOf rdf:resource="https://ark.frantiq.fr/ark:/26678/pcrtnbDLi2FkAj"/>
	<dcterms:created rdf:datatype="http://www.w3.org/2001/XMLSchema#date">2021-02-17</dcterms:created>
	<dcterms:modified rdf:datatype="http://www.w3.org/2001/XMLSchema#date">2024-11-21</dcterms:modified>
	<dcterms:identifier>266439</dcterms:identifier>
	<dcterms:contributor>blandine.nouvel</dcterms:contributor>
	<dcterms:contributor>justine.vincent</dcterms:contributor>
	<skos:definition xml:lang="en">The rock structure in the area studied is heterogeneous (Fernandes et al., 2021).</skos:definition>
	<skos:definition xml:lang="fr">La structure de la roche dans la zone étudiée est hétérogène. (Fernandes et al., 2021)</skos:definition>
</rdf:Description>

<rdf:Description rdf:about="https://ark.frantiq.fr/ark:/26678/pcrtv0rphqt1h8">
	<rdf:type rdf:resource="http://www.w3.org/2004/02/skos/core#Concept"/>
	<skos:prefLabel xml:lang="en">boundstone structure</skos:prefLabel>
	<skos:prefLabel xml:lang="de">Boundstone-Struktur</skos:prefLabel>
	<skos:prefLabel xml:lang="es">estructura boundstone</skos:prefLabel>
	<skos:prefLabel xml:lang="fr">structure boundstone</skos:prefLabel>
	<skos:prefLabel xml:lang="it">struttura boundstone</skos:prefLabel>
	<skos:broader rdf:resource="https://ark.frantiq.fr/ark:/26678/pcrtkwk6bz94r3"/>
	<skos:inScheme rdf:resource="https://ark.frantiq.fr/ark:/26678/TH_1"/>
	<opentheso:memberOf rdf:resource="https://ark.frantiq.fr/ark:/26678/pcrtv66rn9cbv1"/>
	<opentheso:memberOf rdf:resource="https://ark.frantiq.fr/ark:/26678/pcrtnbDLi2FkAj"/>
	<dcterms:created rdf:datatype="http://www.w3.org/2001/XMLSchema#date">2021-02-17</dcterms:created>
	<dcterms:modified rdf:datatype="http://www.w3.org/2001/XMLSchema#date">2023-08-02</dcterms:modified>
	<dcterms:identifier>266441</dcterms:identifier>
	<dcterms:contributor>blandine.nouvel</dcterms:contributor>
	<skos:definition xml:lang="en">The structure of the rock is identical to that of limestones constructed in reef or para-reef environments (d'ap. Dunham, R.J.  Classification of carbonate rocks according to depositional texture . In Ham, W.E. Classification of carbonate rocks. 1962. American Association of Petroleum Geologists Memoir. 1. p. 108-121)</skos:definition>
	<skos:definition xml:lang="fr">La structure de la roche est identique à celle des calcaires construits de milieu récifal ou para-récifal (d'ap. Dunham, R.J.  Classification of carbonate rocks according to depositional texture . In Ham, W.E. Classification of carbonate rocks. 1962. American Association of Petroleum Geologists Memoir. 1. p. 108–121)</skos:definition>
</rdf:Description>

<rdf:Description rdf:about="https://ark.frantiq.fr/ark:/26678/pcrtvh6k2wqhg6">
	<rdf:type rdf:resource="http://www.w3.org/2004/02/skos/core#Concept"/>
	<skos:prefLabel xml:lang="es">estructura de fibras flexibles</skos:prefLabel>
	<skos:prefLabel xml:lang="de">flexible Faserstruktur</skos:prefLabel>
	<skos:prefLabel xml:lang="en">flexible fiber structure</skos:prefLabel>
	<skos:prefLabel xml:lang="fr">structure à fibres flexibles</skos:prefLabel>
	<skos:prefLabel xml:lang="it">struttura a fibre flessibili</skos:prefLabel>
	<skos:broader rdf:resource="https://ark.frantiq.fr/ark:/26678/pcrtkwk6bz94r3"/>
	<skos:inScheme rdf:resource="https://ark.frantiq.fr/ark:/26678/TH_1"/>
	<opentheso:memberOf rdf:resource="https://ark.frantiq.fr/ark:/26678/pcrtv66rn9cbv1"/>
	<opentheso:memberOf rdf:resource="https://ark.frantiq.fr/ark:/26678/pcrtnbDLi2FkAj"/>
	<dcterms:created rdf:datatype="http://www.w3.org/2001/XMLSchema#date">2021-02-17</dcterms:created>
	<dcterms:modified rdf:datatype="http://www.w3.org/2001/XMLSchema#date">2024-11-21</dcterms:modified>
	<dcterms:identifier>266443</dcterms:identifier>
	<dcterms:contributor>blandine.nouvel</dcterms:contributor>
	<dcterms:contributor>justine.vincent</dcterms:contributor>
	<skos:definition xml:lang="fr">La structure de la roche présente des filaments ou tiges courbes, témoins de traces de végétaux ou de bactéries. (Fernandes et al., 2021)</skos:definition>
	<skos:definition xml:lang="en">The structure of the rock shows curved filaments or stems, evidence of traces of plants or bacteria. (Fernandes et al., 2021)</skos:definition>
</rdf:Description>

<rdf:Description rdf:about="https://ark.frantiq.fr/ark:/26678/pcrt969pbxxbzt">
	<rdf:type rdf:resource="http://www.w3.org/2004/02/skos/core#Concept"/>
	<skos:prefLabel xml:lang="en">bioclast structure</skos:prefLabel>
	<skos:prefLabel xml:lang="de">bioklastische Struktur</skos:prefLabel>
	<skos:prefLabel xml:lang="es">estructura bioclástica</skos:prefLabel>
	<skos:prefLabel xml:lang="fr">structure bioclastique</skos:prefLabel>
	<skos:prefLabel xml:lang="it">struttura bioclastica</skos:prefLabel>
	<skos:broader rdf:resource="https://ark.frantiq.fr/ark:/26678/pcrtkwk6bz94r3"/>
	<skos:inScheme rdf:resource="https://ark.frantiq.fr/ark:/26678/TH_1"/>
	<opentheso:memberOf rdf:resource="https://ark.frantiq.fr/ark:/26678/pcrtv66rn9cbv1"/>
	<opentheso:memberOf rdf:resource="https://ark.frantiq.fr/ark:/26678/pcrtnbDLi2FkAj"/>
	<dcterms:created rdf:datatype="http://www.w3.org/2001/XMLSchema#date">2021-02-17</dcterms:created>
	<dcterms:modified rdf:datatype="http://www.w3.org/2001/XMLSchema#date">2024-11-21</dcterms:modified>
	<dcterms:identifier>266445</dcterms:identifier>
	<dcterms:contributor>blandine.nouvel</dcterms:contributor>
	<dcterms:contributor>justine.vincent</dcterms:contributor>
	<skos:definition xml:lang="en">The rock structure contains a significant proportion of bioclasts. (Fernandes et al., 2021)</skos:definition>
	<skos:definition xml:lang="fr">La structure de la roche contient une part significative de bioclastes. (Fernandes et al., 2021)</skos:definition>
</rdf:Description>

<rdf:Description rdf:about="https://ark.frantiq.fr/ark:/26678/pcrt2kpf55zh14">
	<rdf:type rdf:resource="http://www.w3.org/2004/02/skos/core#Concept"/>
	<skos:prefLabel xml:lang="en">bedding structure (geology)</skos:prefLabel>
	<skos:prefLabel xml:lang="es">estructura en capas</skos:prefLabel>
	<skos:prefLabel xml:lang="de">schieferartige Struktur</skos:prefLabel>
	<skos:prefLabel xml:lang="fr">structure litée</skos:prefLabel>
	<skos:prefLabel xml:lang="it">struttura stratificata</skos:prefLabel>
	<skos:altLabel xml:lang="en">bedding surface (geology)</skos:altLabel>
	<skos:altLabel xml:lang="es">estructura estratificada</skos:altLabel>
	<skos:broader rdf:resource="https://ark.frantiq.fr/ark:/26678/pcrtkwk6bz94r3"/>
	<skos:inScheme rdf:resource="https://ark.frantiq.fr/ark:/26678/TH_1"/>
	<opentheso:memberOf rdf:resource="https://ark.frantiq.fr/ark:/26678/pcrtv66rn9cbv1"/>
	<opentheso:memberOf rdf:resource="https://ark.frantiq.fr/ark:/26678/pcrtnbDLi2FkAj"/>
	<dcterms:created rdf:datatype="http://www.w3.org/2001/XMLSchema#date">2021-02-17</dcterms:created>
	<dcterms:modified rdf:datatype="http://www.w3.org/2001/XMLSchema#date">2024-11-21</dcterms:modified>
	<dcterms:identifier>266447</dcterms:identifier>
	<dcterms:contributor>blandine.nouvel</dcterms:contributor>
	<dcterms:contributor>justine.vincent</dcterms:contributor>
	<skos:definition xml:lang="en">The structure of the rock is a succession of superimposed parallel layers or beds of small thickness (millimetre to centimetre). (Fernandes et al., 2021)</skos:definition>
	<skos:definition xml:lang="fr">La structure de la roche présente une succession de couches ou lits superposés parallèles et de faible épaisseur (millimétrique à centimétrique). (Fernandes et al., 2021)</skos:definition>
</rdf:Description>

<rdf:Description rdf:about="https://ark.frantiq.fr/ark:/26678/pcrtndt9zrpjjk">
	<rdf:type rdf:resource="http://www.w3.org/2004/02/skos/core#Concept"/>
	<skos:prefLabel xml:lang="en">acicular structure</skos:prefLabel>
	<skos:prefLabel xml:lang="es">estructura acicular</skos:prefLabel>
	<skos:prefLabel xml:lang="de">nadelförmige Struktur</skos:prefLabel>
	<skos:prefLabel xml:lang="fr">structure à fibre acidulaire</skos:prefLabel>
	<skos:prefLabel xml:lang="it">struttura aciculare</skos:prefLabel>
	<skos:broader rdf:resource="https://ark.frantiq.fr/ark:/26678/pcrtkwk6bz94r3"/>
	<skos:inScheme rdf:resource="https://ark.frantiq.fr/ark:/26678/TH_1"/>
	<opentheso:memberOf rdf:resource="https://ark.frantiq.fr/ark:/26678/pcrtv66rn9cbv1"/>
	<opentheso:memberOf rdf:resource="https://ark.frantiq.fr/ark:/26678/pcrtnbDLi2FkAj"/>
	<dcterms:created rdf:datatype="http://www.w3.org/2001/XMLSchema#date">2021-02-17</dcterms:created>
	<dcterms:modified rdf:datatype="http://www.w3.org/2001/XMLSchema#date">2024-11-21</dcterms:modified>
	<dcterms:identifier>266449</dcterms:identifier>
	<dcterms:contributor>blandine.nouvel</dcterms:contributor>
	<dcterms:contributor>justine.vincent</dcterms:contributor>
	<skos:definition xml:lang="en">The rock structure is characterised by the presence of fine needle-shaped crystals (Fernandes et al., 2021).</skos:definition>
	<skos:definition xml:lang="fr">La structure de la roche est caractérisée par la présence de cristaux en forme de fines aiguilles.(Fernandes et al., 2021)</skos:definition>
</rdf:Description>

<rdf:Description rdf:about="https://ark.frantiq.fr/ark:/26678/pcrtfv2krrfh1d">
	<rdf:type rdf:resource="http://www.w3.org/2004/02/skos/core#Concept"/>
	<skos:prefLabel xml:lang="es">estructura zonal</skos:prefLabel>
	<skos:prefLabel xml:lang="fr">structure zonée</skos:prefLabel>
	<skos:prefLabel xml:lang="it">struttura zonata</skos:prefLabel>
	<skos:prefLabel xml:lang="de">zonale Struktur</skos:prefLabel>
	<skos:prefLabel xml:lang="en">zonal structure</skos:prefLabel>
	<skos:broader rdf:resource="https://ark.frantiq.fr/ark:/26678/pcrtkwk6bz94r3"/>
	<skos:inScheme rdf:resource="https://ark.frantiq.fr/ark:/26678/TH_1"/>
	<opentheso:memberOf rdf:resource="https://ark.frantiq.fr/ark:/26678/pcrtv66rn9cbv1"/>
	<opentheso:memberOf rdf:resource="https://ark.frantiq.fr/ark:/26678/pcrtnbDLi2FkAj"/>
	<dcterms:created rdf:datatype="http://www.w3.org/2001/XMLSchema#date">2021-02-17</dcterms:created>
	<dcterms:modified rdf:datatype="http://www.w3.org/2001/XMLSchema#date">2024-11-21</dcterms:modified>
	<dcterms:identifier>266451</dcterms:identifier>
	<dcterms:contributor>blandine.nouvel</dcterms:contributor>
	<dcterms:contributor>justine.vincent</dcterms:contributor>
	<skos:definition xml:lang="en">The structure of the rock shows concentric bands with different colourimetric or granulometric aspects. (Fernandes et al., 2021)</skos:definition>
	<skos:definition xml:lang="fr">La structure de la roche présente des bandes concentriques d'aspects colorimétriques ou granulométriques différents. (Fernandes et al., 2021)</skos:definition>
</rdf:Description>

<rdf:Description rdf:about="https://ark.frantiq.fr/ark:/26678/pcrtknmwxc5x5s">
	<rdf:type rdf:resource="http://www.w3.org/2004/02/skos/core#Concept"/>
	<skos:prefLabel xml:lang="en">bioturbation structure</skos:prefLabel>
	<skos:prefLabel xml:lang="de">Bioturbation (Struktur)</skos:prefLabel>
	<skos:prefLabel xml:lang="it">bioturbazione (struttura)</skos:prefLabel>
	<skos:prefLabel xml:lang="es">estructura de bioturbación</skos:prefLabel>
	<skos:prefLabel xml:lang="fr">structure bioturbée</skos:prefLabel>
	<skos:altLabel xml:lang="it">struttura biogenica</skos:altLabel>
	<skos:broader rdf:resource="https://ark.frantiq.fr/ark:/26678/pcrtkwk6bz94r3"/>
	<skos:inScheme rdf:resource="https://ark.frantiq.fr/ark:/26678/TH_1"/>
	<opentheso:memberOf rdf:resource="https://ark.frantiq.fr/ark:/26678/pcrtv66rn9cbv1"/>
	<opentheso:memberOf rdf:resource="https://ark.frantiq.fr/ark:/26678/pcrtnbDLi2FkAj"/>
	<dcterms:created rdf:datatype="http://www.w3.org/2001/XMLSchema#date">2021-02-17</dcterms:created>
	<dcterms:modified rdf:datatype="http://www.w3.org/2001/XMLSchema#date">2024-11-21</dcterms:modified>
	<dcterms:identifier>266453</dcterms:identifier>
	<dcterms:contributor>blandine.nouvel</dcterms:contributor>
	<dcterms:contributor>justine.vincent</dcterms:contributor>
	<skos:definition xml:lang="en">The rock structure shows patches of destructuring caused by living organisms (burrows, tracks, galleries...). &gt;(Fernandes et al., 2021)</skos:definition>
	<skos:definition xml:lang="fr">La structure de la roche présente des plages de déstructurations provoquées par des organismes vivants (terriers, pistes, galeries…). &lt;span style= color: rgb(102, 102, 102); &gt;(Fernandes et al., 2021)&lt;/span&gt;</skos:definition>
</rdf:Description>

<rdf:Description rdf:about="https://ark.frantiq.fr/ark:/26678/pcrtrwdpzch5wh">
	<rdf:type rdf:resource="http://www.w3.org/2004/02/skos/core#Concept"/>
	<skos:prefLabel xml:lang="es">estructura granular</skos:prefLabel>
	<skos:prefLabel xml:lang="de">granulare Struktur</skos:prefLabel>
	<skos:prefLabel xml:lang="en">granular structure</skos:prefLabel>
	<skos:prefLabel xml:lang="fr">structure granoclassée</skos:prefLabel>
	<skos:prefLabel xml:lang="it">struttura granulare</skos:prefLabel>
	<skos:broader rdf:resource="https://ark.frantiq.fr/ark:/26678/pcrtkwk6bz94r3"/>
	<skos:inScheme rdf:resource="https://ark.frantiq.fr/ark:/26678/TH_1"/>
	<opentheso:memberOf rdf:resource="https://ark.frantiq.fr/ark:/26678/pcrtv66rn9cbv1"/>
	<opentheso:memberOf rdf:resource="https://ark.frantiq.fr/ark:/26678/pcrtnbDLi2FkAj"/>
	<dcterms:created rdf:datatype="http://www.w3.org/2001/XMLSchema#date">2021-02-17</dcterms:created>
	<dcterms:modified rdf:datatype="http://www.w3.org/2001/XMLSchema#date">2024-11-21</dcterms:modified>
	<dcterms:identifier>266455</dcterms:identifier>
	<dcterms:contributor>blandine.nouvel</dcterms:contributor>
	<dcterms:contributor>justine.vincent</dcterms:contributor>
	<skos:definition xml:lang="en">The rock structure shows a distribution of grains by increasing or decreasing size. (Fernandes et al., 2021)</skos:definition>
	<skos:definition xml:lang="fr">La structure de la roche présente une répartition des grains par taille croissante ou décroissante.&lt;span style= color: rgb(102, 102, 102); &gt;(Fernandes et al., 2021)&lt;/span&gt;</skos:definition>
</rdf:Description>

<rdf:Description rdf:about="https://ark.frantiq.fr/ark:/26678/pcrth30k691qrk">
	<rdf:type rdf:resource="http://www.w3.org/2004/02/skos/core#Concept"/>
	<skos:prefLabel xml:lang="es">estructura oolítica</skos:prefLabel>
	<skos:prefLabel xml:lang="en">oolithic structure</skos:prefLabel>
	<skos:prefLabel xml:lang="de">oolithische Struktur</skos:prefLabel>
	<skos:prefLabel xml:lang="fr">structure oolithique</skos:prefLabel>
	<skos:prefLabel xml:lang="it">struttura oolitica</skos:prefLabel>
	<skos:altLabel xml:lang="en">oölithic structure</skos:altLabel>
	<skos:related rdf:resource="https://ark.frantiq.fr/ark:/26678/pcrt11g9hx0p5s"/>
	<skos:broader rdf:resource="https://ark.frantiq.fr/ark:/26678/pcrtkwk6bz94r3"/>
	<skos:inScheme rdf:resource="https://ark.frantiq.fr/ark:/26678/TH_1"/>
	<opentheso:memberOf rdf:resource="https://ark.frantiq.fr/ark:/26678/pcrtv66rn9cbv1"/>
	<opentheso:memberOf rdf:resource="https://ark.frantiq.fr/ark:/26678/pcrtnbDLi2FkAj"/>
	<dcterms:created rdf:datatype="http://www.w3.org/2001/XMLSchema#date">2021-02-17</dcterms:created>
	<dcterms:modified rdf:datatype="http://www.w3.org/2001/XMLSchema#date">2024-11-21</dcterms:modified>
	<dcterms:identifier>266457</dcterms:identifier>
	<dcterms:contributor>blandine.nouvel</dcterms:contributor>
	<dcterms:contributor>justine.vincent</dcterms:contributor>
	<skos:definition xml:lang="en">The rock structure is predominantly made up of oolites. (Fernandes et al., 2021)</skos:definition>
	<skos:definition xml:lang="fr">La structure de la roche est majoritairement constituée par des oolithes. &lt;span style= color: rgb(102, 102, 102); &gt;(Fernandes et al., 2021)&lt;/span&gt;</skos:definition>
</rdf:Description>

<rdf:Description rdf:about="https://ark.frantiq.fr/ark:/26678/pcrtkgmbfz0x3s">
	<rdf:type rdf:resource="http://www.w3.org/2004/02/skos/core#Concept"/>
	<skos:prefLabel xml:lang="es">estructura laminar</skos:prefLabel>
	<skos:prefLabel xml:lang="de">geschichtete Struktur</skos:prefLabel>
	<skos:prefLabel xml:lang="en">laminated structure</skos:prefLabel>
	<skos:prefLabel xml:lang="fr">structure laminée</skos:prefLabel>
	<skos:prefLabel xml:lang="it">struttura laminata</skos:prefLabel>
	<skos:altLabel xml:lang="es">estructura laminada</skos:altLabel>
	<skos:altLabel xml:lang="es">laminación</skos:altLabel>
	<skos:altLabel xml:lang="en">laminated sediments</skos:altLabel>
	<skos:altLabel xml:lang="it">laminazione</skos:altLabel>
	<skos:broader rdf:resource="https://ark.frantiq.fr/ark:/26678/pcrtkwk6bz94r3"/>
	<skos:inScheme rdf:resource="https://ark.frantiq.fr/ark:/26678/TH_1"/>
	<opentheso:memberOf rdf:resource="https://ark.frantiq.fr/ark:/26678/pcrtv66rn9cbv1"/>
	<opentheso:memberOf rdf:resource="https://ark.frantiq.fr/ark:/26678/pcrtnbDLi2FkAj"/>
	<dcterms:created rdf:datatype="http://www.w3.org/2001/XMLSchema#date">2021-02-17</dcterms:created>
	<dcterms:modified rdf:datatype="http://www.w3.org/2001/XMLSchema#date">2023-08-02</dcterms:modified>
	<dcterms:identifier>266459</dcterms:identifier>
	<dcterms:contributor>blandine.nouvel</dcterms:contributor>
	<skos:definition xml:lang="en">The rock structure comprises a succession of very thin (sub-millimetre to millimetre) bedded levels . (Fernandes et al., 2021)</skos:definition>
	<skos:definition xml:lang="fr">La structure de la roche comporte une succession de niveaux lités de très faible épaisseur (inframillimétrique à millimétrique) &lt;span style= color: rgb(102, 102, 102); &gt;(Fernandes et al., 2021)&lt;/span&gt;</skos:definition>
</rdf:Description>

<rdf:Description rdf:about="https://ark.frantiq.fr/ark:/26678/pcrtkrm9q3htcj">
	<rdf:type rdf:resource="http://www.w3.org/2004/02/skos/core#Concept"/>
	<skos:prefLabel xml:lang="de">Fenster-Struktur</skos:prefLabel>
	<skos:prefLabel xml:lang="fr">structure fenestrée</skos:prefLabel>
	<skos:prefLabel xml:lang="it">struttura fenestrale</skos:prefLabel>
	<skos:prefLabel xml:lang="es">ventana tectónica</skos:prefLabel>
	<skos:prefLabel xml:lang="en">window (geology)</skos:prefLabel>
	<skos:altLabel xml:lang="es">fenster</skos:altLabel>
	<skos:altLabel xml:lang="en">fenster (geology)</skos:altLabel>
	<skos:broader rdf:resource="https://ark.frantiq.fr/ark:/26678/pcrtkwk6bz94r3"/>
	<skos:inScheme rdf:resource="https://ark.frantiq.fr/ark:/26678/TH_1"/>
	<opentheso:memberOf rdf:resource="https://ark.frantiq.fr/ark:/26678/pcrtv66rn9cbv1"/>
	<opentheso:memberOf rdf:resource="https://ark.frantiq.fr/ark:/26678/pcrtnbDLi2FkAj"/>
	<dcterms:created rdf:datatype="http://www.w3.org/2001/XMLSchema#date">2021-02-17</dcterms:created>
	<dcterms:modified rdf:datatype="http://www.w3.org/2001/XMLSchema#date">2024-11-21</dcterms:modified>
	<dcterms:identifier>266461</dcterms:identifier>
	<dcterms:contributor>blandine.nouvel</dcterms:contributor>
	<dcterms:contributor>justine.vincent</dcterms:contributor>
	<skos:definition xml:lang="en">The rock structure shows degassing cavities forming more or less spherical vacuoles, flattened in the sedimentation plane. (Fernandes et al., 2021)</skos:definition>
	<skos:definition xml:lang="fr">La structure de la roche présente des cavités de dégazage formant des vacuoles plus ou moins sphériques, aplaties dans le plan de sédimentation. &lt;span style= color: rgb(102, 102, 102); &gt;(Fernandes et al., 2021)&lt;/span&gt;</skos:definition>
</rdf:Description>

<rdf:Description rdf:about="https://ark.frantiq.fr/ark:/26678/pcrtq764j7snt5">
	<rdf:type rdf:resource="http://www.w3.org/2004/02/skos/core#Concept"/>
	<skos:prefLabel xml:lang="en">breccia structure</skos:prefLabel>
	<skos:prefLabel xml:lang="de">Brekzienstruktur</skos:prefLabel>
	<skos:prefLabel xml:lang="es">estructura brechada</skos:prefLabel>
	<skos:prefLabel xml:lang="fr">structure bréchique</skos:prefLabel>
	<skos:prefLabel xml:lang="it">struttura brecciosa</skos:prefLabel>
	<skos:altLabel xml:lang="it">breccia (conglomerato roccioso)</skos:altLabel>
	<skos:altLabel xml:lang="es">brechamiento</skos:altLabel>
	<skos:related rdf:resource="https://ark.frantiq.fr/ark:/26678/pcrtvhmknj8n0n92z5x2xqqk"/>
	<skos:broader rdf:resource="https://ark.frantiq.fr/ark:/26678/pcrtkwk6bz94r3"/>
	<skos:inScheme rdf:resource="https://ark.frantiq.fr/ark:/26678/TH_1"/>
	<opentheso:memberOf rdf:resource="https://ark.frantiq.fr/ark:/26678/pcrtv66rn9cbv1"/>
	<opentheso:memberOf rdf:resource="https://ark.frantiq.fr/ark:/26678/pcrtnbDLi2FkAj"/>
	<dcterms:created rdf:datatype="http://www.w3.org/2001/XMLSchema#date">2021-02-17</dcterms:created>
	<dcterms:modified rdf:datatype="http://www.w3.org/2001/XMLSchema#date">2024-11-21</dcterms:modified>
	<dcterms:identifier>266463</dcterms:identifier>
	<dcterms:contributor>blandine.nouvel</dcterms:contributor>
	<dcterms:contributor>justine.vincent</dcterms:contributor>
	<skos:definition xml:lang="en">The structure of the breccia-like rock (Slansky, 1992), composed mainly of angular figurative elements (Fernandes et al. 2021).</skos:definition>
	<skos:definition xml:lang="fr">La structure de la roche à caractère de brèche (Slansky, 1992), composée majoritairement d'éléments figurés anguleux. (Fernandes et al. 2021)</skos:definition>
</rdf:Description>

<rdf:Description rdf:about="https://ark.frantiq.fr/ark:/26678/pcrtfvk3mp3dhk">
	<rdf:type rdf:resource="http://www.w3.org/2004/02/skos/core#Concept"/>
	<skos:prefLabel xml:lang="en">conglomerate structure (geology)</skos:prefLabel>
	<skos:prefLabel xml:lang="es">estructura conglomerada</skos:prefLabel>
	<skos:prefLabel xml:lang="de">Konglomeratstruktur</skos:prefLabel>
	<skos:prefLabel xml:lang="fr">structure conglomératique</skos:prefLabel>
	<skos:prefLabel xml:lang="it">struttura conglomerata</skos:prefLabel>
	<skos:broader rdf:resource="https://ark.frantiq.fr/ark:/26678/pcrtkwk6bz94r3"/>
	<skos:inScheme rdf:resource="https://ark.frantiq.fr/ark:/26678/TH_1"/>
	<opentheso:memberOf rdf:resource="https://ark.frantiq.fr/ark:/26678/pcrtv66rn9cbv1"/>
	<opentheso:memberOf rdf:resource="https://ark.frantiq.fr/ark:/26678/pcrtnbDLi2FkAj"/>
	<dcterms:created rdf:datatype="http://www.w3.org/2001/XMLSchema#date">2021-02-17</dcterms:created>
	<dcterms:modified rdf:datatype="http://www.w3.org/2001/XMLSchema#date">2024-11-21</dcterms:modified>
	<dcterms:identifier>266465</dcterms:identifier>
	<dcterms:contributor>blandine.nouvel</dcterms:contributor>
	<dcterms:contributor>justine.vincent</dcterms:contributor>
	<skos:definition xml:lang="en">The rock structure is a conglomerate composed mainly of rounded fragments (Fernandes et al., 2021).</skos:definition>
	<skos:definition xml:lang="fr">La structure de la roche présente un conglomérat composé majoritairement de fragments arrondis. (Fernandes et al., 2021)</skos:definition>
</rdf:Description>

<rdf:Description rdf:about="https://ark.frantiq.fr/ark:/26678/pcrt3tmh056368">
	<rdf:type rdf:resource="http://www.w3.org/2004/02/skos/core#Concept"/>
	<skos:prefLabel xml:lang="en">annular structure (geology)</skos:prefLabel>
	<skos:prefLabel xml:lang="es">estructura anular</skos:prefLabel>
	<skos:prefLabel xml:lang="de">Ringstruktur</skos:prefLabel>
	<skos:prefLabel xml:lang="fr">structure annulaire</skos:prefLabel>
	<skos:prefLabel xml:lang="it">struttura anulare</skos:prefLabel>
	<skos:broader rdf:resource="https://ark.frantiq.fr/ark:/26678/pcrtkwk6bz94r3"/>
	<skos:inScheme rdf:resource="https://ark.frantiq.fr/ark:/26678/TH_1"/>
	<opentheso:memberOf rdf:resource="https://ark.frantiq.fr/ark:/26678/pcrtv66rn9cbv1"/>
	<opentheso:memberOf rdf:resource="https://ark.frantiq.fr/ark:/26678/pcrtnbDLi2FkAj"/>
	<dcterms:created rdf:datatype="http://www.w3.org/2001/XMLSchema#date">2021-02-17</dcterms:created>
	<dcterms:modified rdf:datatype="http://www.w3.org/2001/XMLSchema#date">2024-11-21</dcterms:modified>
	<dcterms:identifier>266467</dcterms:identifier>
	<dcterms:contributor>blandine.nouvel</dcterms:contributor>
	<dcterms:contributor>justine.vincent</dcterms:contributor>
	<skos:definition xml:lang="en">The structure of the rock is a succession of concentric rings. (Fernandes et al., 2021)</skos:definition>
	<skos:definition xml:lang="fr">La structure de la roche présente une succession d'anneaux concentriques. (Fernandes et al., 2021)</skos:definition>
</rdf:Description>

<rdf:Description rdf:about="https://ark.frantiq.fr/ark:/26678/pcrtfz97ktt9qf">
	<rdf:type rdf:resource="http://www.w3.org/2004/02/skos/core#Concept"/>
	<skos:prefLabel xml:lang="en">clastic rock</skos:prefLabel>
	<skos:prefLabel xml:lang="es">estructura clástica</skos:prefLabel>
	<skos:prefLabel xml:lang="de">klastische Struktur</skos:prefLabel>
	<skos:prefLabel xml:lang="fr">structure clastique</skos:prefLabel>
	<skos:prefLabel xml:lang="it">struttura clastica</skos:prefLabel>
	<skos:altLabel xml:lang="en">clastic structure</skos:altLabel>
	<skos:broader rdf:resource="https://ark.frantiq.fr/ark:/26678/pcrtkwk6bz94r3"/>
	<skos:inScheme rdf:resource="https://ark.frantiq.fr/ark:/26678/TH_1"/>
	<opentheso:memberOf rdf:resource="https://ark.frantiq.fr/ark:/26678/pcrtv66rn9cbv1"/>
	<opentheso:memberOf rdf:resource="https://ark.frantiq.fr/ark:/26678/pcrtnbDLi2FkAj"/>
	<dcterms:created rdf:datatype="http://www.w3.org/2001/XMLSchema#date">2021-02-17</dcterms:created>
	<dcterms:modified rdf:datatype="http://www.w3.org/2001/XMLSchema#date">2024-11-21</dcterms:modified>
	<dcterms:identifier>266469</dcterms:identifier>
	<dcterms:contributor>blandine.nouvel</dcterms:contributor>
	<dcterms:contributor>justine.vincent</dcterms:contributor>
	<skos:definition xml:lang="en">The rock structure is made up of rock debris, grains or fossils. (Fernandes et al., 2021)</skos:definition>
	<skos:definition xml:lang="fr">La structure de la roche est constituée de débris de roches, de grains ou de fossiles. (Fernandes et al., 2021)</skos:definition>
</rdf:Description>

<rdf:Description rdf:about="https://ark.frantiq.fr/ark:/26678/pcrt5bd4f5dv7r">
	<rdf:type rdf:resource="http://www.w3.org/2004/02/skos/core#Concept"/>
	<skos:prefLabel xml:lang="fr">matrice micro-méso cristalline</skos:prefLabel>
	<skos:prefLabel xml:lang="es">matriz micro y mesocristalina</skos:prefLabel>
	<skos:prefLabel xml:lang="en">micro meso crystalline rock matrix</skos:prefLabel>
	<skos:prefLabel xml:lang="de">mikro-mesokristalline Matrix</skos:prefLabel>
	<skos:prefLabel xml:lang="it">struttura micro e mesocristallina</skos:prefLabel>
	<skos:broader rdf:resource="https://ark.frantiq.fr/ark:/26678/pcrtqc4b4zzzmw"/>
	<skos:inScheme rdf:resource="https://ark.frantiq.fr/ark:/26678/TH_1"/>
	<opentheso:memberOf rdf:resource="https://ark.frantiq.fr/ark:/26678/pcrtv66rn9cbv1"/>
	<opentheso:memberOf rdf:resource="https://ark.frantiq.fr/ark:/26678/pcrtnbDLi2FkAj"/>
	<dcterms:created rdf:datatype="http://www.w3.org/2001/XMLSchema#date">2021-02-17</dcterms:created>
	<dcterms:modified rdf:datatype="http://www.w3.org/2001/XMLSchema#date">2023-08-02</dcterms:modified>
	<dcterms:identifier>266471</dcterms:identifier>
	<dcterms:contributor>blandine.nouvel</dcterms:contributor>
	<skos:definition xml:lang="en">Matrix with crystals from 1 µm to 630 µm. (Fernandes P.: Itinéraires et transformations du silex : une pétroarchéologie refondée, application au Paléolithique moyen, thesis Prehistory, Univ. Bordeaux, 2012)</skos:definition>
	<skos:definition xml:lang="fr">Matrice à cristaux de 1 µm à 630 µm (Fernandes P. :  Itinéraires et transformations du silex : une pétroarchéologie refondée, application au Paléolithique moyen, thèse Préhistoire, Univ. Bordeaux, 2012)</skos:definition>
</rdf:Description>

<rdf:Description rdf:about="https://ark.frantiq.fr/ark:/26678/pcrt5ddg241ccv">
	<rdf:type rdf:resource="http://www.w3.org/2004/02/skos/core#Concept"/>
	<skos:prefLabel xml:lang="en">cryptocrystalline matrix</skos:prefLabel>
	<skos:prefLabel xml:lang="de">kryptokristalline Matrix</skos:prefLabel>
	<skos:prefLabel xml:lang="fr">matrice cryptocristalline</skos:prefLabel>
	<skos:prefLabel xml:lang="es">matriz criptocristalina</skos:prefLabel>
	<skos:prefLabel xml:lang="it">struttura criptocristallina</skos:prefLabel>
	<skos:broader rdf:resource="https://ark.frantiq.fr/ark:/26678/pcrtqc4b4zzzmw"/>
	<skos:inScheme rdf:resource="https://ark.frantiq.fr/ark:/26678/TH_1"/>
	<opentheso:memberOf rdf:resource="https://ark.frantiq.fr/ark:/26678/pcrtv66rn9cbv1"/>
	<opentheso:memberOf rdf:resource="https://ark.frantiq.fr/ark:/26678/pcrtnbDLi2FkAj"/>
	<dcterms:created rdf:datatype="http://www.w3.org/2001/XMLSchema#date">2021-02-17</dcterms:created>
	<dcterms:modified rdf:datatype="http://www.w3.org/2001/XMLSchema#date">2024-11-19</dcterms:modified>
	<dcterms:identifier>266473</dcterms:identifier>
	<dcterms:contributor>blandine.nouvel</dcterms:contributor>
	<dcterms:contributor>justine.vincent</dcterms:contributor>
	<skos:definition xml:lang="en">Matrix with crystals smaller than 1 µm (Slansky, 1992)</skos:definition>
	<skos:definition xml:lang="fr">Matrice à cristaux de moins de 1 µm. (Slansky, 1992)</skos:definition>
</rdf:Description>

<rdf:Description rdf:about="https://ark.frantiq.fr/ark:/26678/pcrtjmqpnw74z9">
	<rdf:type rdf:resource="http://www.w3.org/2004/02/skos/core#Concept"/>
	<skos:prefLabel xml:lang="it">matrice microcristallina</skos:prefLabel>
	<skos:prefLabel xml:lang="fr">matrice microcristalline</skos:prefLabel>
	<skos:prefLabel xml:lang="es">matriz microcristalina</skos:prefLabel>
	<skos:prefLabel xml:lang="en">micro crystalline matrix</skos:prefLabel>
	<skos:prefLabel xml:lang="de">mikrokristalline Matrix</skos:prefLabel>
	<skos:broader rdf:resource="https://ark.frantiq.fr/ark:/26678/pcrtqc4b4zzzmw"/>
	<skos:inScheme rdf:resource="https://ark.frantiq.fr/ark:/26678/TH_1"/>
	<opentheso:memberOf rdf:resource="https://ark.frantiq.fr/ark:/26678/pcrtv66rn9cbv1"/>
	<opentheso:memberOf rdf:resource="https://ark.frantiq.fr/ark:/26678/pcrtnbDLi2FkAj"/>
	<dcterms:created rdf:datatype="http://www.w3.org/2001/XMLSchema#date">2021-02-17</dcterms:created>
	<dcterms:modified rdf:datatype="http://www.w3.org/2001/XMLSchema#date">2024-11-19</dcterms:modified>
	<dcterms:identifier>266475</dcterms:identifier>
	<dcterms:contributor>blandine.nouvel</dcterms:contributor>
	<dcterms:contributor>justine.vincent</dcterms:contributor>
	<skos:definition xml:lang="en">Matrix with crystals larger than 1 µm and less than 4 µm. (Slansky, 1992)</skos:definition>
	<skos:definition xml:lang="fr">Matrice à cristaux de plus de 1 µm et moins de 4 µm. (Slansky, 1992)</skos:definition>
</rdf:Description>

<rdf:Description rdf:about="https://ark.frantiq.fr/ark:/26678/pcrt6pvhc29pfv">
	<rdf:type rdf:resource="http://www.w3.org/2004/02/skos/core#Concept"/>
	<skos:prefLabel xml:lang="it">matrice mesocristallina</skos:prefLabel>
	<skos:prefLabel xml:lang="fr">matrice mésocristalline</skos:prefLabel>
	<skos:prefLabel xml:lang="es">matriz mesocristalina</skos:prefLabel>
	<skos:prefLabel xml:lang="en">meso crystalline matrix</skos:prefLabel>
	<skos:prefLabel xml:lang="de">mesokristalline Matrix</skos:prefLabel>
	<skos:broader rdf:resource="https://ark.frantiq.fr/ark:/26678/pcrtqc4b4zzzmw"/>
	<skos:inScheme rdf:resource="https://ark.frantiq.fr/ark:/26678/TH_1"/>
	<opentheso:memberOf rdf:resource="https://ark.frantiq.fr/ark:/26678/pcrtv66rn9cbv1"/>
	<opentheso:memberOf rdf:resource="https://ark.frantiq.fr/ark:/26678/pcrtnbDLi2FkAj"/>
	<dcterms:created rdf:datatype="http://www.w3.org/2001/XMLSchema#date">2021-02-17</dcterms:created>
	<dcterms:modified rdf:datatype="http://www.w3.org/2001/XMLSchema#date">2023-08-02</dcterms:modified>
	<dcterms:identifier>266477</dcterms:identifier>
	<dcterms:contributor>blandine.nouvel</dcterms:contributor>
	<skos:definition xml:lang="en">Matrix with crystals from 4 µm to 630 µm. (Slansky, 1992)</skos:definition>
	<skos:definition xml:lang="fr">Matrice à cristaux de 4 µm à 630 µm (Slansky, 1992)</skos:definition>
</rdf:Description>

<rdf:Description rdf:about="https://ark.frantiq.fr/ark:/26678/pcrtk8c4vv2tw8">
	<rdf:type rdf:resource="http://www.w3.org/2004/02/skos/core#Concept"/>
	<skos:prefLabel xml:lang="en">macro crystalline matrix</skos:prefLabel>
	<skos:prefLabel xml:lang="de">makrokristalline Matrix</skos:prefLabel>
	<skos:prefLabel xml:lang="it">matrice macrocristallina</skos:prefLabel>
	<skos:prefLabel xml:lang="fr">matrice macrocristalline</skos:prefLabel>
	<skos:prefLabel xml:lang="es">matriz macrocristalina</skos:prefLabel>
	<skos:broader rdf:resource="https://ark.frantiq.fr/ark:/26678/pcrtqc4b4zzzmw"/>
	<skos:inScheme rdf:resource="https://ark.frantiq.fr/ark:/26678/TH_1"/>
	<opentheso:memberOf rdf:resource="https://ark.frantiq.fr/ark:/26678/pcrtv66rn9cbv1"/>
	<opentheso:memberOf rdf:resource="https://ark.frantiq.fr/ark:/26678/pcrtnbDLi2FkAj"/>
	<dcterms:created rdf:datatype="http://www.w3.org/2001/XMLSchema#date">2021-02-17</dcterms:created>
	<dcterms:modified rdf:datatype="http://www.w3.org/2001/XMLSchema#date">2024-11-19</dcterms:modified>
	<dcterms:identifier>266479</dcterms:identifier>
	<dcterms:contributor>blandine.nouvel</dcterms:contributor>
	<dcterms:contributor>justine.vincent</dcterms:contributor>
	<skos:definition xml:lang="en">Matrix or cement of more than 630 µm and less than 2 mm (Slansky, 1992).</skos:definition>
	<skos:definition xml:lang="fr">Matrice ou ciment de plus de 630 µm et moins de 2 mm. (Slansky, 1992)</skos:definition>
</rdf:Description>

<rdf:Description rdf:about="https://ark.frantiq.fr/ark:/26678/pcrt5nd65vnw7p">
	<rdf:type rdf:resource="http://www.w3.org/2004/02/skos/core#Concept"/>
	<skos:prefLabel xml:lang="en">grain morphology (geology)</skos:prefLabel>
	<skos:prefLabel xml:lang="de">Kornmorphologie</skos:prefLabel>
	<skos:prefLabel xml:lang="it">morfologia dei granuli</skos:prefLabel>
	<skos:prefLabel xml:lang="es">morfología del grano</skos:prefLabel>
	<skos:prefLabel xml:lang="fr">morphologie des grains</skos:prefLabel>
	<skos:narrower rdf:resource="https://ark.frantiq.fr/ark:/26678/pcrtjg8pxcjgdt"/>
	<skos:narrower rdf:resource="https://ark.frantiq.fr/ark:/26678/pcrt7qtb4j1twt"/>
	<skos:broader rdf:resource="https://ark.frantiq.fr/ark:/26678/pcrt40qs0fvnxg"/>
	<skos:inScheme rdf:resource="https://ark.frantiq.fr/ark:/26678/TH_1"/>
	<opentheso:memberOf rdf:resource="https://ark.frantiq.fr/ark:/26678/pcrtv66rn9cbv1"/>
	<opentheso:memberOf rdf:resource="https://ark.frantiq.fr/ark:/26678/pcrtnbDLi2FkAj"/>
	<dcterms:created rdf:datatype="http://www.w3.org/2001/XMLSchema#date">2021-02-17</dcterms:created>
	<dcterms:modified rdf:datatype="http://www.w3.org/2001/XMLSchema#date">2023-08-02</dcterms:modified>
	<dcterms:identifier>266485</dcterms:identifier>
	<dcterms:contributor>blandine.nouvel</dcterms:contributor>
	<skos:definition xml:lang="en">Morphological characteristics of the grains that make up rocks.</skos:definition>
	<skos:definition xml:lang="fr">Caractéristique morphologique des grains composant les roches</skos:definition>
</rdf:Description>

<rdf:Description rdf:about="https://ark.frantiq.fr/ark:/26678/pcrt24wcqp2cfz">
	<rdf:type rdf:resource="http://www.w3.org/2004/02/skos/core#Concept"/>
	<skos:prefLabel xml:lang="fr">allochème minéral</skos:prefLabel>
	<skos:prefLabel xml:lang="it">allochimico minerale</skos:prefLabel>
	<skos:prefLabel xml:lang="es">aloquímico mineral</skos:prefLabel>
	<skos:prefLabel xml:lang="en">mineral allochem</skos:prefLabel>
	<skos:prefLabel xml:lang="de">minerales Allochem</skos:prefLabel>
	<skos:broader rdf:resource="https://ark.frantiq.fr/ark:/26678/pcrt40qs0fvnxg"/>
	<skos:inScheme rdf:resource="https://ark.frantiq.fr/ark:/26678/TH_1"/>
	<opentheso:memberOf rdf:resource="https://ark.frantiq.fr/ark:/26678/pcrtv66rn9cbv1"/>
	<opentheso:memberOf rdf:resource="https://ark.frantiq.fr/ark:/26678/pcrtnbDLi2FkAj"/>
	<dcterms:created rdf:datatype="http://www.w3.org/2001/XMLSchema#date">2021-02-17</dcterms:created>
	<dcterms:modified rdf:datatype="http://www.w3.org/2001/XMLSchema#date">2025-01-30</dcterms:modified>
	<dcterms:identifier>266487</dcterms:identifier>
	<dcterms:contributor>blandine.nouvel</dcterms:contributor>
	<dcterms:contributor>justine.vincent</dcterms:contributor>
	<skos:definition xml:lang="en">In a rock, figurative elements exclusively of minerals. (Fernandes P., 2012)</skos:definition>
	<skos:definition xml:lang="fr">Dans une roche, éléments figurés exclusivement de minéraux. (Fernandes P., 2012)</skos:definition>
	<dcterms:source>https://doi-org.inshs.bib.cnrs.fr/10.4000/12zm5</dcterms:source>
</rdf:Description>

<rdf:Description rdf:about="https://ark.frantiq.fr/ark:/26678/pcrt9qq3x37vt0">
	<rdf:type rdf:resource="http://www.w3.org/2004/02/skos/core#Concept"/>
	<skos:prefLabel xml:lang="fr">allochème lithoclastique</skos:prefLabel>
	<skos:prefLabel xml:lang="it">allochimico litoclastico</skos:prefLabel>
	<skos:prefLabel xml:lang="es">aloquímico litoclástico</skos:prefLabel>
	<skos:prefLabel xml:lang="en">lithoclastic allochem</skos:prefLabel>
	<skos:prefLabel xml:lang="de">lithoklastisches Allochem</skos:prefLabel>
	<skos:broader rdf:resource="https://ark.frantiq.fr/ark:/26678/pcrt40qs0fvnxg"/>
	<skos:inScheme rdf:resource="https://ark.frantiq.fr/ark:/26678/TH_1"/>
	<opentheso:memberOf rdf:resource="https://ark.frantiq.fr/ark:/26678/pcrtv66rn9cbv1"/>
	<opentheso:memberOf rdf:resource="https://ark.frantiq.fr/ark:/26678/pcrtnbDLi2FkAj"/>
	<dcterms:created rdf:datatype="http://www.w3.org/2001/XMLSchema#date">2021-02-17</dcterms:created>
	<dcterms:modified rdf:datatype="http://www.w3.org/2001/XMLSchema#date">2025-01-30</dcterms:modified>
	<dcterms:identifier>266489</dcterms:identifier>
	<dcterms:contributor>blandine.nouvel</dcterms:contributor>
	<dcterms:contributor>justine.vincent</dcterms:contributor>
	<skos:definition xml:lang="en">Fragment embedded in a sediment or rock. (Fernandes, 2012)</skos:definition>
	<skos:definition xml:lang="fr">Fragment inclus dans un sédiment ou une roche. (Fernandes, 2012)</skos:definition>
	<dcterms:source>https://doi-org.inshs.bib.cnrs.fr/10.4000/12zm5</dcterms:source>
</rdf:Description>

<rdf:Description rdf:about="https://ark.frantiq.fr/ark:/26678/pcrtr06vz24nj3">
	<rdf:type rdf:resource="http://www.w3.org/2004/02/skos/core#Concept"/>
	<skos:prefLabel xml:lang="fr">allochème clastique</skos:prefLabel>
	<skos:prefLabel xml:lang="it">allochimico clastico</skos:prefLabel>
	<skos:prefLabel xml:lang="es">aloquímico clástico</skos:prefLabel>
	<skos:prefLabel xml:lang="en">clastic allochem</skos:prefLabel>
	<skos:prefLabel xml:lang="de">klastisches Allochem</skos:prefLabel>
	<skos:broader rdf:resource="https://ark.frantiq.fr/ark:/26678/pcrt40qs0fvnxg"/>
	<skos:inScheme rdf:resource="https://ark.frantiq.fr/ark:/26678/TH_1"/>
	<opentheso:memberOf rdf:resource="https://ark.frantiq.fr/ark:/26678/pcrtv66rn9cbv1"/>
	<opentheso:memberOf rdf:resource="https://ark.frantiq.fr/ark:/26678/pcrtnbDLi2FkAj"/>
	<dcterms:created rdf:datatype="http://www.w3.org/2001/XMLSchema#date">2021-02-17</dcterms:created>
	<dcterms:modified rdf:datatype="http://www.w3.org/2001/XMLSchema#date">2025-01-30</dcterms:modified>
	<dcterms:identifier>266491</dcterms:identifier>
	<dcterms:contributor>blandine.nouvel</dcterms:contributor>
	<dcterms:contributor>justine.vincent</dcterms:contributor>
	<skos:definition xml:lang="en">Figurative elements of different natures present in the rock matrix (Fernandes, 2012)</skos:definition>
	<skos:definition xml:lang="fr">Éléments figurés de nature différente présents dans la matrice de la roche.&amp;amp;nbsp;(Fernandes, 2012)</skos:definition>
	<dcterms:source>https://doi-org.inshs.bib.cnrs.fr/10.4000/12zm5</dcterms:source>
</rdf:Description>

<rdf:Description rdf:about="https://ark.frantiq.fr/ark:/26678/pcrt2fhx0kftpg">
	<rdf:type rdf:resource="http://www.w3.org/2004/02/skos/core#Concept"/>
	<skos:prefLabel xml:lang="fr">allochème bioclastique</skos:prefLabel>
	<skos:prefLabel xml:lang="it">allochimico bioclastico</skos:prefLabel>
	<skos:prefLabel xml:lang="es">aloquímico bioclástico</skos:prefLabel>
	<skos:prefLabel xml:lang="en">bioclastic allochem</skos:prefLabel>
	<skos:prefLabel xml:lang="de">bioklastisches Allochem</skos:prefLabel>
	<skos:broader rdf:resource="https://ark.frantiq.fr/ark:/26678/pcrt40qs0fvnxg"/>
	<skos:inScheme rdf:resource="https://ark.frantiq.fr/ark:/26678/TH_1"/>
	<opentheso:memberOf rdf:resource="https://ark.frantiq.fr/ark:/26678/pcrtv66rn9cbv1"/>
	<opentheso:memberOf rdf:resource="https://ark.frantiq.fr/ark:/26678/pcrtnbDLi2FkAj"/>
	<dcterms:created rdf:datatype="http://www.w3.org/2001/XMLSchema#date">2021-02-17</dcterms:created>
	<dcterms:modified rdf:datatype="http://www.w3.org/2001/XMLSchema#date">2025-01-30</dcterms:modified>
	<dcterms:identifier>266493</dcterms:identifier>
	<dcterms:contributor>blandine.nouvel</dcterms:contributor>
	<dcterms:contributor>justine.vincent</dcterms:contributor>
	<skos:definition xml:lang="en">In a rock, figurative elements made up exclusively of fossil remains (Fernandes, 2012)</skos:definition>
	<skos:definition xml:lang="fr">Dans une roche, éléments figurés exclusivement constitués par des restes de fossiles (Fernandes, 2012)</skos:definition>
	<dcterms:source>https://doi-org.inshs.bib.cnrs.fr/10.4000/12zm5</dcterms:source>
</rdf:Description>

<rdf:Description rdf:about="https://ark.frantiq.fr/ark:/26678/pcrt1tm77xkqbd">
	<rdf:type rdf:resource="http://www.w3.org/2004/02/skos/core#Concept"/>
	<skos:prefLabel xml:lang="fr">allochème à organisme massif</skos:prefLabel>
	<skos:prefLabel xml:lang="de">Allochem mit massiven Organismen</skos:prefLabel>
	<skos:prefLabel xml:lang="it">allochimico con organismo a corpo massivo</skos:prefLabel>
	<skos:prefLabel xml:lang="es">aloquímico con organismo masivo</skos:prefLabel>
	<skos:prefLabel xml:lang="en">massive organism allochem</skos:prefLabel>
	<skos:broader rdf:resource="https://ark.frantiq.fr/ark:/26678/pcrt40qs0fvnxg"/>
	<skos:inScheme rdf:resource="https://ark.frantiq.fr/ark:/26678/TH_1"/>
	<opentheso:memberOf rdf:resource="https://ark.frantiq.fr/ark:/26678/pcrtv66rn9cbv1"/>
	<opentheso:memberOf rdf:resource="https://ark.frantiq.fr/ark:/26678/pcrtnbDLi2FkAj"/>
	<dcterms:created rdf:datatype="http://www.w3.org/2001/XMLSchema#date">2021-02-17</dcterms:created>
	<dcterms:modified rdf:datatype="http://www.w3.org/2001/XMLSchema#date">2023-08-02</dcterms:modified>
	<dcterms:identifier>266495</dcterms:identifier>
	<dcterms:contributor>blandine.nouvel</dcterms:contributor>
	<skos:definition xml:lang="en">Allochaeum made up of colonial corals or certain algae such as Lithothamnias (Purser, Sédimentation et diagenèse des carbonates néritiques récents, Paris: Technip, 1980)</skos:definition>
	<skos:definition xml:lang="fr">Allochème constitué de coraux coloniaux ou certaines algues telles que les Lithothamniées (Purser, Sédimentation et diagenèse des carbonates néritiques récents, Paris : Technip, 1980)</skos:definition>
</rdf:Description>

<rdf:Description rdf:about="https://ark.frantiq.fr/ark:/26678/pcrt6xvrhrkjz8">
	<rdf:type rdf:resource="http://www.w3.org/2004/02/skos/core#Concept"/>
	<skos:prefLabel xml:lang="fr">allochème à organisme mou</skos:prefLabel>
	<skos:prefLabel xml:lang="de">Allochem mit Weichteil-Organismen</skos:prefLabel>
	<skos:prefLabel xml:lang="it">allochimico con organismo a corpo molle</skos:prefLabel>
	<skos:prefLabel xml:lang="es">aloquímico con organismo de cuerpo blando</skos:prefLabel>
	<skos:prefLabel xml:lang="en">soft tissue organism allochem</skos:prefLabel>
	<skos:broader rdf:resource="https://ark.frantiq.fr/ark:/26678/pcrt40qs0fvnxg"/>
	<skos:inScheme rdf:resource="https://ark.frantiq.fr/ark:/26678/TH_1"/>
	<opentheso:memberOf rdf:resource="https://ark.frantiq.fr/ark:/26678/pcrtv66rn9cbv1"/>
	<opentheso:memberOf rdf:resource="https://ark.frantiq.fr/ark:/26678/pcrtnbDLi2FkAj"/>
	<dcterms:created rdf:datatype="http://www.w3.org/2001/XMLSchema#date">2021-02-17</dcterms:created>
	<dcterms:modified rdf:datatype="http://www.w3.org/2001/XMLSchema#date">2023-08-02</dcterms:modified>
	<dcterms:identifier>266497</dcterms:identifier>
	<dcterms:contributor>blandine.nouvel</dcterms:contributor>
	<skos:definition xml:lang="en">Allocheme made up of plants or animals with an internal skeleton that disintegrates after death and releases microparticles (Purser, Sédimentation et diagenèse des carbonates néritiques récents, Paris: Technip, 1980).</skos:definition>
	<skos:definition xml:lang="fr">Allochème constitué de végétaux ou d'animaux à squelette interne qui se désintègre après la mort et libèrent des microparticules (Purser, Sédimentation et diagenèse des carbonates néritiques récents, Paris : Technip, 1980)</skos:definition>
</rdf:Description>

<rdf:Description rdf:about="https://ark.frantiq.fr/ark:/26678/pcrtwz8jzr2ttd">
	<rdf:type rdf:resource="http://www.w3.org/2004/02/skos/core#Concept"/>
	<skos:prefLabel xml:lang="fr">allochème à organisme à squelette creux</skos:prefLabel>
	<skos:prefLabel xml:lang="de">Allochem mit Hohlknochenorganismen</skos:prefLabel>
	<skos:prefLabel xml:lang="it">allochimico con organismo a corpo cavo</skos:prefLabel>
	<skos:prefLabel xml:lang="es">aloquímico con organismo de cuerpo hueco</skos:prefLabel>
	<skos:prefLabel xml:lang="en">hollow skeleton organism allochem</skos:prefLabel>
	<skos:altLabel xml:lang="en">bryozoan</skos:altLabel>
	<skos:altLabel xml:lang="en">skeletal allochem</skos:altLabel>
	<skos:broader rdf:resource="https://ark.frantiq.fr/ark:/26678/pcrt40qs0fvnxg"/>
	<skos:inScheme rdf:resource="https://ark.frantiq.fr/ark:/26678/TH_1"/>
	<opentheso:memberOf rdf:resource="https://ark.frantiq.fr/ark:/26678/pcrtv66rn9cbv1"/>
	<opentheso:memberOf rdf:resource="https://ark.frantiq.fr/ark:/26678/pcrtnbDLi2FkAj"/>
	<dcterms:created rdf:datatype="http://www.w3.org/2001/XMLSchema#date">2021-02-17</dcterms:created>
	<dcterms:modified rdf:datatype="http://www.w3.org/2001/XMLSchema#date">2023-08-02</dcterms:modified>
	<dcterms:identifier>266499</dcterms:identifier>
	<dcterms:contributor>blandine.nouvel</dcterms:contributor>
	<skos:definition xml:lang="en">Allochaeum made up of gastropods, lamellibranchs, brachiopods, foraminifera, echinoderms (Purser, Sédimentation et diagenèse des carbonates néritiques récents, Paris: Technip, 1980)</skos:definition>
	<skos:definition xml:lang="fr">Allochème constitué de gastropodes, lamellibranches, brachiopodes, foraminifères, échinodermes (Purser, Sédimentation et diagenèse des carbonates néritiques récents, Paris : Technip, 1980)</skos:definition>
</rdf:Description>

<rdf:Description rdf:about="https://ark.frantiq.fr/ark:/26678/pcrt4rsdrmfk1b">
	<rdf:type rdf:resource="http://www.w3.org/2004/02/skos/core#Concept"/>
	<skos:prefLabel xml:lang="fr">allochème à squelette branchu</skos:prefLabel>
	<skos:prefLabel xml:lang="de">Allochem mit verzweigtem Skelett</skos:prefLabel>
	<skos:prefLabel xml:lang="it">allochimico con organismo a scheletro ramificato</skos:prefLabel>
	<skos:prefLabel xml:lang="es">aloquímico con organismo de esqueleto ramificado</skos:prefLabel>
	<skos:prefLabel xml:lang="en">branching form allochem</skos:prefLabel>
	<skos:altLabel xml:lang="en">bryozoan</skos:altLabel>
	<skos:altLabel xml:lang="en">skeletal allochem</skos:altLabel>
	<skos:broader rdf:resource="https://ark.frantiq.fr/ark:/26678/pcrt40qs0fvnxg"/>
	<skos:inScheme rdf:resource="https://ark.frantiq.fr/ark:/26678/TH_1"/>
	<opentheso:memberOf rdf:resource="https://ark.frantiq.fr/ark:/26678/pcrtv66rn9cbv1"/>
	<opentheso:memberOf rdf:resource="https://ark.frantiq.fr/ark:/26678/pcrtnbDLi2FkAj"/>
	<dcterms:created rdf:datatype="http://www.w3.org/2001/XMLSchema#date">2021-02-17</dcterms:created>
	<dcterms:modified rdf:datatype="http://www.w3.org/2001/XMLSchema#date">2023-08-02</dcterms:modified>
	<dcterms:identifier>266501</dcterms:identifier>
	<dcterms:contributor>blandine.nouvel</dcterms:contributor>
	<skos:definition xml:lang="en">An allocheme made up of organisms such as polyparians, red algae and bryozoans (Purser, Sédimentation et diagenèse des carbonates néritiques récents, Paris: Technip, 1980).</skos:definition>
	<skos:definition xml:lang="fr">Allochème constitué d'organismes comme le polypier, l'algue rouge, le bryozoaire (Purser, Sédimentation et diagenèse des carbonates néritiques récents, Paris : Technip, 1980)</skos:definition>
</rdf:Description>

<rdf:Description rdf:about="https://ark.frantiq.fr/ark:/26678/pcrtjwwb1xztxh">
	<rdf:type rdf:resource="http://www.w3.org/2004/02/skos/core#Concept"/>
	<skos:prefLabel xml:lang="fr">allochème issu d'une épigénie</skos:prefLabel>
	<skos:prefLabel xml:lang="en">allochem through epigenesis</skos:prefLabel>
	<skos:prefLabel xml:lang="it">allochimico derivato da un'epigenesi</skos:prefLabel>
	<skos:prefLabel xml:lang="es">aloquímico por epigénesis</skos:prefLabel>
	<skos:prefLabel xml:lang="de">durch Epigenese entstandenes Allochem</skos:prefLabel>
	<skos:related rdf:resource="https://ark.frantiq.fr/ark:/26678/pcrt0c5wnff3d6"/>
	<skos:broader rdf:resource="https://ark.frantiq.fr/ark:/26678/pcrt40qs0fvnxg"/>
	<skos:inScheme rdf:resource="https://ark.frantiq.fr/ark:/26678/TH_1"/>
	<opentheso:memberOf rdf:resource="https://ark.frantiq.fr/ark:/26678/pcrtv66rn9cbv1"/>
	<opentheso:memberOf rdf:resource="https://ark.frantiq.fr/ark:/26678/pcrtnbDLi2FkAj"/>
	<dcterms:created rdf:datatype="http://www.w3.org/2001/XMLSchema#date">2021-02-17</dcterms:created>
	<dcterms:modified rdf:datatype="http://www.w3.org/2001/XMLSchema#date">2025-01-30</dcterms:modified>
	<dcterms:identifier>266503</dcterms:identifier>
	<dcterms:contributor>blandine.nouvel</dcterms:contributor>
	<dcterms:contributor>justine.vincent</dcterms:contributor>
	<skos:definition xml:lang="en">Allocheme consisting of elements replacing one mineral by another without modifying its shape or structure. (Fernandes et al. 2021)</skos:definition>
	<skos:definition xml:lang="fr">Allochème constitué d'éléments de remplacement d'un minéral par un autre sans modification de sa forme et de sa structure. (Fernandes et al. 2021)</skos:definition>
	<dcterms:source>https://doi-org.inshs.bib.cnrs.fr/10.4000/12zm5</dcterms:source>
</rdf:Description>

<rdf:Description rdf:about="https://ark.frantiq.fr/ark:/26678/pcrt1kjsnnvmzh">
	<rdf:type rdf:resource="http://www.w3.org/2004/02/skos/core#Concept"/>
	<skos:prefLabel xml:lang="fr">allochème homogène</skos:prefLabel>
	<skos:prefLabel xml:lang="it">allochimico omogeneo</skos:prefLabel>
	<skos:prefLabel xml:lang="es">aloquímico homogéneo</skos:prefLabel>
	<skos:prefLabel xml:lang="de">homogenes Allochem</skos:prefLabel>
	<skos:prefLabel xml:lang="en">homogenous allochem</skos:prefLabel>
	<skos:broader rdf:resource="https://ark.frantiq.fr/ark:/26678/pcrt40qs0fvnxg"/>
	<skos:inScheme rdf:resource="https://ark.frantiq.fr/ark:/26678/TH_1"/>
	<opentheso:memberOf rdf:resource="https://ark.frantiq.fr/ark:/26678/pcrtv66rn9cbv1"/>
	<opentheso:memberOf rdf:resource="https://ark.frantiq.fr/ark:/26678/pcrtnbDLi2FkAj"/>
	<dcterms:created rdf:datatype="http://www.w3.org/2001/XMLSchema#date">2021-02-17</dcterms:created>
	<dcterms:modified rdf:datatype="http://www.w3.org/2001/XMLSchema#date">2025-01-30</dcterms:modified>
	<dcterms:identifier>266505</dcterms:identifier>
	<dcterms:contributor>blandine.nouvel</dcterms:contributor>
	<dcterms:contributor>justine.vincent</dcterms:contributor>
	<skos:definition xml:lang="fr">Les éléments figurés observés dans la roche sont similaires en termes de nature et leur répartition est régulière en tous points de l'échantillon. (Fernandes et al., 2021)</skos:definition>
	<dcterms:source>https://doi-org.inshs.bib.cnrs.fr/10.4000/12zm5</dcterms:source>
</rdf:Description>

<rdf:Description rdf:about="https://ark.frantiq.fr/ark:/26678/pcrt21f986h3tk">
	<rdf:type rdf:resource="http://www.w3.org/2004/02/skos/core#Concept"/>
	<skos:prefLabel xml:lang="fr">allochème hétérogène</skos:prefLabel>
	<skos:prefLabel xml:lang="it">allochimico eterogeneo</skos:prefLabel>
	<skos:prefLabel xml:lang="es">aloquímico heterogéneo</skos:prefLabel>
	<skos:prefLabel xml:lang="en">heterogeneous allochem</skos:prefLabel>
	<skos:prefLabel xml:lang="de">heterogenes Allochem</skos:prefLabel>
	<skos:broader rdf:resource="https://ark.frantiq.fr/ark:/26678/pcrt40qs0fvnxg"/>
	<skos:inScheme rdf:resource="https://ark.frantiq.fr/ark:/26678/TH_1"/>
	<opentheso:memberOf rdf:resource="https://ark.frantiq.fr/ark:/26678/pcrtv66rn9cbv1"/>
	<opentheso:memberOf rdf:resource="https://ark.frantiq.fr/ark:/26678/pcrtnbDLi2FkAj"/>
	<dcterms:created rdf:datatype="http://www.w3.org/2001/XMLSchema#date">2021-02-17</dcterms:created>
	<dcterms:modified rdf:datatype="http://www.w3.org/2001/XMLSchema#date">2025-01-30</dcterms:modified>
	<dcterms:identifier>266507</dcterms:identifier>
	<dcterms:contributor>blandine.nouvel</dcterms:contributor>
	<dcterms:contributor>justine.vincent</dcterms:contributor>
	<skos:definition xml:lang="en">The figurative elements observed in the rock are of different natures and their distribution is irregular within the sample (Fernandes et al., 2021).</skos:definition>
	<skos:definition xml:lang="fr">Les éléments figurés observés dans la roche sont de natures différentes et leur répartition est irrégulière au sein de l’échantillon. (Fernandes et al., 2021)</skos:definition>
	<dcterms:source>https://doi-org.inshs.bib.cnrs.fr/10.4000/12zm5</dcterms:source>
</rdf:Description>

<rdf:Description rdf:about="https://ark.frantiq.fr/ark:/26678/pcrtqmm7q566vh">
	<rdf:type rdf:resource="http://www.w3.org/2004/02/skos/core#Concept"/>
	<skos:prefLabel xml:lang="fr">allochème orienté</skos:prefLabel>
	<skos:prefLabel xml:lang="it">allochimico orientato</skos:prefLabel>
	<skos:prefLabel xml:lang="es">aloquímico orientado</skos:prefLabel>
	<skos:prefLabel xml:lang="en">preferential oriented allochem</skos:prefLabel>
	<skos:prefLabel xml:lang="de">preferentiell ausgerichtetes Allochem</skos:prefLabel>
	<skos:broader rdf:resource="https://ark.frantiq.fr/ark:/26678/pcrt40qs0fvnxg"/>
	<skos:inScheme rdf:resource="https://ark.frantiq.fr/ark:/26678/TH_1"/>
	<opentheso:memberOf rdf:resource="https://ark.frantiq.fr/ark:/26678/pcrtv66rn9cbv1"/>
	<opentheso:memberOf rdf:resource="https://ark.frantiq.fr/ark:/26678/pcrtnbDLi2FkAj"/>
	<dcterms:created rdf:datatype="http://www.w3.org/2001/XMLSchema#date">2021-02-17</dcterms:created>
	<dcterms:modified rdf:datatype="http://www.w3.org/2001/XMLSchema#date">2023-08-02</dcterms:modified>
	<dcterms:identifier>266509</dcterms:identifier>
	<dcterms:contributor>blandine.nouvel</dcterms:contributor>
</rdf:Description>

<rdf:Description rdf:about="https://ark.frantiq.fr/ark:/26678/pcrtv3f379sr9v">
	<rdf:type rdf:resource="http://www.w3.org/2004/02/skos/core#Concept"/>
	<skos:prefLabel xml:lang="fr">allochème laminé</skos:prefLabel>
	<skos:prefLabel xml:lang="it">allochimico stratificato</skos:prefLabel>
	<skos:prefLabel xml:lang="es">aloquímico laminar</skos:prefLabel>
	<skos:prefLabel xml:lang="de">geschichtetes Allochem</skos:prefLabel>
	<skos:prefLabel xml:lang="en">laminated allochem</skos:prefLabel>
	<skos:broader rdf:resource="https://ark.frantiq.fr/ark:/26678/pcrt40qs0fvnxg"/>
	<skos:inScheme rdf:resource="https://ark.frantiq.fr/ark:/26678/TH_1"/>
	<opentheso:memberOf rdf:resource="https://ark.frantiq.fr/ark:/26678/pcrtv66rn9cbv1"/>
	<opentheso:memberOf rdf:resource="https://ark.frantiq.fr/ark:/26678/pcrtnbDLi2FkAj"/>
	<dcterms:created rdf:datatype="http://www.w3.org/2001/XMLSchema#date">2021-02-17</dcterms:created>
	<dcterms:modified rdf:datatype="http://www.w3.org/2001/XMLSchema#date">2025-01-30</dcterms:modified>
	<dcterms:identifier>266511</dcterms:identifier>
	<dcterms:contributor>blandine.nouvel</dcterms:contributor>
	<dcterms:contributor>justine.vincent</dcterms:contributor>
	<skos:definition xml:lang="en">The figurative elements present in the rock are arranged in thin submillimetre layers called laminae (Fernandes et al., 2021).</skos:definition>
	<skos:definition xml:lang="fr">Les éléments figurés présents dans la roche sont disposés en fines couches inframillimétriques appelées lamines. (Fernandes et al., 2021)</skos:definition>
	<dcterms:source>https://doi-org.inshs.bib.cnrs.fr/10.4000/12zm5</dcterms:source>
</rdf:Description>

<rdf:Description rdf:about="https://ark.frantiq.fr/ark:/26678/pcrtb689mtdsz6">
	<rdf:type rdf:resource="http://www.w3.org/2004/02/skos/core#Concept"/>
	<skos:prefLabel xml:lang="fr">allochème granoclassé</skos:prefLabel>
	<skos:prefLabel xml:lang="it">allochimico granulare</skos:prefLabel>
	<skos:prefLabel xml:lang="es">aloquímico granular</skos:prefLabel>
	<skos:prefLabel xml:lang="en">granular allochem</skos:prefLabel>
	<skos:prefLabel xml:lang="de">granulares Allochem</skos:prefLabel>
	<skos:broader rdf:resource="https://ark.frantiq.fr/ark:/26678/pcrt40qs0fvnxg"/>
	<skos:inScheme rdf:resource="https://ark.frantiq.fr/ark:/26678/TH_1"/>
	<opentheso:memberOf rdf:resource="https://ark.frantiq.fr/ark:/26678/pcrtv66rn9cbv1"/>
	<opentheso:memberOf rdf:resource="https://ark.frantiq.fr/ark:/26678/pcrtnbDLi2FkAj"/>
	<dcterms:created rdf:datatype="http://www.w3.org/2001/XMLSchema#date">2021-02-17</dcterms:created>
	<dcterms:modified rdf:datatype="http://www.w3.org/2001/XMLSchema#date">2025-01-30</dcterms:modified>
	<dcterms:identifier>266513</dcterms:identifier>
	<dcterms:contributor>blandine.nouvel</dcterms:contributor>
	<dcterms:contributor>justine.vincent</dcterms:contributor>
	<skos:definition xml:lang="en">The grains of rock are distributed in increasing or decreasing size, depending on the speed of the currents that governed their arrangement. (Fernandes et al., 2021)</skos:definition>
	<skos:definition xml:lang="fr">Les grains de la roche sont répartis par taille croissante ou décroissante, selon la vitesse des courants qui ont présidé à leur disposition. (Fernandes et al., 2021)</skos:definition>
	<dcterms:source>https://doi-org.inshs.bib.cnrs.fr/10.4000/12zm5</dcterms:source>
</rdf:Description>

<rdf:Description rdf:about="https://ark.frantiq.fr/ark:/26678/pcrt8c26426vth">
	<rdf:type rdf:resource="http://www.w3.org/2004/02/skos/core#Concept"/>
	<skos:prefLabel xml:lang="fr">allochème bimodal</skos:prefLabel>
	<skos:prefLabel xml:lang="it">allochimico bimodale</skos:prefLabel>
	<skos:prefLabel xml:lang="es">aloquímico bimodal</skos:prefLabel>
	<skos:prefLabel xml:lang="en">bimodal allochem</skos:prefLabel>
	<skos:prefLabel xml:lang="de">bimodales Allochem</skos:prefLabel>
	<skos:broader rdf:resource="https://ark.frantiq.fr/ark:/26678/pcrt40qs0fvnxg"/>
	<skos:inScheme rdf:resource="https://ark.frantiq.fr/ark:/26678/TH_1"/>
	<opentheso:memberOf rdf:resource="https://ark.frantiq.fr/ark:/26678/pcrtv66rn9cbv1"/>
	<opentheso:memberOf rdf:resource="https://ark.frantiq.fr/ark:/26678/pcrtnbDLi2FkAj"/>
	<dcterms:created rdf:datatype="http://www.w3.org/2001/XMLSchema#date">2021-02-17</dcterms:created>
	<dcterms:modified rdf:datatype="http://www.w3.org/2001/XMLSchema#date">2025-01-30</dcterms:modified>
	<dcterms:identifier>266515</dcterms:identifier>
	<dcterms:contributor>blandine.nouvel</dcterms:contributor>
	<dcterms:contributor>justine.vincent</dcterms:contributor>
	<skos:definition xml:lang="en">The elements in the rock show two grain sizes at all points in the sample. (Slansky, 1992)</skos:definition>
	<skos:definition xml:lang="fr">Les éléments figurés dans la roche présentent deux tailles de grains en tous points de l'échantillon. (Slansky, 1992)</skos:definition>
</rdf:Description>

<rdf:Description rdf:about="https://ark.frantiq.fr/ark:/26678/pcrtjg8pxcjgdt">
	<rdf:type rdf:resource="http://www.w3.org/2004/02/skos/core#Concept"/>
	<skos:prefLabel xml:lang="es">esfericidad de los granos</skos:prefLabel>
	<skos:prefLabel xml:lang="en">grain sphericity</skos:prefLabel>
	<skos:prefLabel xml:lang="it">sfericità dei granuli</skos:prefLabel>
	<skos:prefLabel xml:lang="de">Sphärizität der Körner</skos:prefLabel>
	<skos:prefLabel xml:lang="fr">sphéricité des grains</skos:prefLabel>
	<skos:broader rdf:resource="https://ark.frantiq.fr/ark:/26678/pcrt5nd65vnw7p"/>
	<skos:inScheme rdf:resource="https://ark.frantiq.fr/ark:/26678/TH_1"/>
	<opentheso:memberOf rdf:resource="https://ark.frantiq.fr/ark:/26678/pcrtv66rn9cbv1"/>
	<opentheso:memberOf rdf:resource="https://ark.frantiq.fr/ark:/26678/pcrtnbDLi2FkAj"/>
	<dcterms:created rdf:datatype="http://www.w3.org/2001/XMLSchema#date">2021-02-17</dcterms:created>
	<dcterms:modified rdf:datatype="http://www.w3.org/2001/XMLSchema#date">2023-08-02</dcterms:modified>
	<dcterms:identifier>266517</dcterms:identifier>
	<dcterms:contributor>blandine.nouvel</dcterms:contributor>
	<skos:definition xml:lang="en">Spherical shape of the rock grains (or clasts) as assessed according to the chart drawn up by Krumbein and Sloss, 1955.</skos:definition>
	<skos:definition xml:lang="fr">Forme sphérique des grains de la roche (ou le claste) telle qu' évaluée selon la charte établie par Krumbein et Sloss, 1955</skos:definition>
</rdf:Description>

<rdf:Description rdf:about="https://ark.frantiq.fr/ark:/26678/pcrt7qtb4j1twt">
	<rdf:type rdf:resource="http://www.w3.org/2004/02/skos/core#Concept"/>
	<skos:prefLabel xml:lang="fr">arrondi des grains</skos:prefLabel>
	<skos:prefLabel xml:lang="it">arrotondamento dei granuli</skos:prefLabel>
	<skos:prefLabel xml:lang="en">grain curvature</skos:prefLabel>
	<skos:prefLabel xml:lang="es">redondez de los granos</skos:prefLabel>
	<skos:prefLabel xml:lang="de">Rundung der Körner</skos:prefLabel>
	<skos:broader rdf:resource="https://ark.frantiq.fr/ark:/26678/pcrt5nd65vnw7p"/>
	<skos:inScheme rdf:resource="https://ark.frantiq.fr/ark:/26678/TH_1"/>
	<opentheso:memberOf rdf:resource="https://ark.frantiq.fr/ark:/26678/pcrtv66rn9cbv1"/>
	<opentheso:memberOf rdf:resource="https://ark.frantiq.fr/ark:/26678/pcrtnbDLi2FkAj"/>
	<dcterms:created rdf:datatype="http://www.w3.org/2001/XMLSchema#date">2021-02-17</dcterms:created>
	<dcterms:modified rdf:datatype="http://www.w3.org/2001/XMLSchema#date">2023-08-02</dcterms:modified>
	<dcterms:identifier>266519</dcterms:identifier>
	<dcterms:contributor>blandine.nouvel</dcterms:contributor>
	<skos:definition xml:lang="en">Edge wear of a grain or clast as assessed according to the chart established by Krumbein and Sloss, 1955.</skos:definition>
	<skos:definition xml:lang="fr">Usure des arêtes d'un grain ou d’un claste telle qu'évaluée selon la charte établie par Krumbein et Sloss, 1955.</skos:definition>
</rdf:Description>

<rdf:Description rdf:about="https://ark.frantiq.fr/ark:/26678/pcrtqjn0rqg305">
	<rdf:type rdf:resource="http://www.w3.org/2004/02/skos/core#Concept"/>
	<skos:prefLabel xml:lang="en">cortex</skos:prefLabel>
	<skos:prefLabel xml:lang="fr">cortex</skos:prefLabel>
	<skos:prefLabel xml:lang="it">cortex</skos:prefLabel>
	<skos:prefLabel xml:lang="es">córtex</skos:prefLabel>
	<skos:prefLabel xml:lang="de">Kortex</skos:prefLabel>
	<skos:altLabel xml:lang="de">Rinde</skos:altLabel>
	<skos:related rdf:resource="https://ark.frantiq.fr/ark:/26678/pcrt21v5j62zkd"/>
	<skos:related rdf:resource="https://ark.frantiq.fr/ark:/26678/pcrtj8kv2v5jz0"/>
	<skos:broader rdf:resource="https://ark.frantiq.fr/ark:/26678/pcrtsvkcb5mv2t"/>
	<skos:inScheme rdf:resource="https://ark.frantiq.fr/ark:/26678/TH_1"/>
	<opentheso:memberOf rdf:resource="https://ark.frantiq.fr/ark:/26678/pcrtv66rn9cbv1"/>
	<opentheso:memberOf rdf:resource="https://ark.frantiq.fr/ark:/26678/pcrtnbDLi2FkAj"/>
	<dcterms:created rdf:datatype="http://www.w3.org/2001/XMLSchema#date">2021-02-17</dcterms:created>
	<dcterms:modified rdf:datatype="http://www.w3.org/2001/XMLSchema#date">2024-11-21</dcterms:modified>
	<dcterms:identifier>266521</dcterms:identifier>
	<dcterms:contributor>blandine.nouvel</dcterms:contributor>
	<dcterms:contributor>justine.vincent</dcterms:contributor>
	<skos:definition xml:lang="en">Altered surface zone enveloping certain boulders, particularly flints. (Brézillon, 1968)</skos:definition>
	<skos:definition xml:lang="fr">Zone superficielle altérée enveloppant certains blocs de roche et notamment les silex. (Brézillon, 1968)</skos:definition>
</rdf:Description>

<rdf:Description rdf:about="https://ark.frantiq.fr/ark:/26678/pcrtjts6bfc4zq">
	<rdf:type rdf:resource="http://www.w3.org/2004/02/skos/core#Concept"/>
	<skos:prefLabel xml:lang="en">neo-cortex</skos:prefLabel>
	<skos:prefLabel xml:lang="it">neocortex</skos:prefLabel>
	<skos:prefLabel xml:lang="es">neocórtex</skos:prefLabel>
	<skos:prefLabel xml:lang="fr">néo-cortex</skos:prefLabel>
	<skos:prefLabel xml:lang="de">Neokortex</skos:prefLabel>
	<skos:related rdf:resource="https://ark.frantiq.fr/ark:/26678/pcrt21v5j62zkd"/>
	<skos:related rdf:resource="https://ark.frantiq.fr/ark:/26678/pcrtj8kv2v5jz0"/>
	<skos:related rdf:resource="https://ark.frantiq.fr/ark:/26678/pcrtc64m697d3t"/>
	<skos:related rdf:resource="https://ark.frantiq.fr/ark:/26678/pcrt9s23ncq2q9"/>
	<skos:broader rdf:resource="https://ark.frantiq.fr/ark:/26678/pcrtsvkcb5mv2t"/>
	<skos:inScheme rdf:resource="https://ark.frantiq.fr/ark:/26678/TH_1"/>
	<opentheso:memberOf rdf:resource="https://ark.frantiq.fr/ark:/26678/pcrtv66rn9cbv1"/>
	<opentheso:memberOf rdf:resource="https://ark.frantiq.fr/ark:/26678/pcrtnbDLi2FkAj"/>
	<dcterms:created rdf:datatype="http://www.w3.org/2001/XMLSchema#date">2021-02-17</dcterms:created>
	<dcterms:modified rdf:datatype="http://www.w3.org/2001/XMLSchema#date">2024-11-21</dcterms:modified>
	<dcterms:identifier>266523</dcterms:identifier>
	<dcterms:contributor>blandine.nouvel</dcterms:contributor>
	<dcterms:contributor>justine.vincent</dcterms:contributor>
	<skos:definition xml:lang="en">The peripheral zone of a flint, resulting from a series of mechanical and physico-chemical transformations located on its surface after its expulsion from the parent rock and before its abandonment in the archaeological site (Fernandes, 2012).</skos:definition>
	<skos:definition xml:lang="fr">Zone périphérique d'un silex, résultant d'un ensemble de transformations mécaniques et physico-chimiques localisées à sa surface après son expulsion de la roche mère et avant son abandon dans le site archéologique. (Fernandes, 2012).</skos:definition>
</rdf:Description>

<rdf:Description rdf:about="https://ark.frantiq.fr/ark:/26678/pcrtzpd0t7gbgz">
	<rdf:type rdf:resource="http://www.w3.org/2004/02/skos/core#Concept"/>
	<skos:prefLabel xml:lang="fr">lithoclase</skos:prefLabel>
	<skos:prefLabel xml:lang="en">lithoclast</skos:prefLabel>
	<skos:prefLabel xml:lang="de">Lithoklast</skos:prefLabel>
	<skos:prefLabel xml:lang="es">litoclasa</skos:prefLabel>
	<skos:prefLabel xml:lang="it">litoclasi</skos:prefLabel>
	<skos:broader rdf:resource="https://ark.frantiq.fr/ark:/26678/pcrtsvkcb5mv2t"/>
	<skos:inScheme rdf:resource="https://ark.frantiq.fr/ark:/26678/TH_1"/>
	<opentheso:memberOf rdf:resource="https://ark.frantiq.fr/ark:/26678/pcrtv66rn9cbv1"/>
	<opentheso:memberOf rdf:resource="https://ark.frantiq.fr/ark:/26678/pcrtnbDLi2FkAj"/>
	<dcterms:created rdf:datatype="http://www.w3.org/2001/XMLSchema#date">2021-02-17</dcterms:created>
	<dcterms:modified rdf:datatype="http://www.w3.org/2001/XMLSchema#date">2024-11-21</dcterms:modified>
	<dcterms:identifier>266525</dcterms:identifier>
	<dcterms:contributor>blandine.nouvel</dcterms:contributor>
	<dcterms:contributor>justine.vincent</dcterms:contributor>
	<skos:definition xml:lang="en">Fracture plane in a rock, with or without displacement of fragments. (Fernandes et al., 2021)</skos:definition>
	<skos:definition xml:lang="fr">Plan de cassure dans une roche, avec ou sans déplacement des fragments. (Fernandes et al., 2021)</skos:definition>
</rdf:Description>

<rdf:Description rdf:about="https://ark.frantiq.fr/ark:/26678/pcrtvq05vjv1z6">
	<rdf:type rdf:resource="http://www.w3.org/2004/02/skos/core#Concept"/>
	<skos:prefLabel xml:lang="es">porosidad primaria</skos:prefLabel>
	<skos:prefLabel xml:lang="it">porosità primaria</skos:prefLabel>
	<skos:prefLabel xml:lang="fr">porosité primaire</skos:prefLabel>
	<skos:prefLabel xml:lang="de">primäre Porosität</skos:prefLabel>
	<skos:prefLabel xml:lang="en">primary porosity</skos:prefLabel>
	<skos:broader rdf:resource="https://ark.frantiq.fr/ark:/26678/pcrt0kvts48fht"/>
	<skos:inScheme rdf:resource="https://ark.frantiq.fr/ark:/26678/TH_1"/>
	<opentheso:memberOf rdf:resource="https://ark.frantiq.fr/ark:/26678/pcrtv66rn9cbv1"/>
	<opentheso:memberOf rdf:resource="https://ark.frantiq.fr/ark:/26678/pcrtnbDLi2FkAj"/>
	<dcterms:created rdf:datatype="http://www.w3.org/2001/XMLSchema#date">2021-02-18</dcterms:created>
	<dcterms:modified rdf:datatype="http://www.w3.org/2001/XMLSchema#date">2023-08-02</dcterms:modified>
	<dcterms:identifier>266527</dcterms:identifier>
	<dcterms:contributor>blandine.nouvel</dcterms:contributor>
	<skos:definition xml:lang="en">Porosity created at the time of deposition and preserved during diagenesis (Fernandes et al., 2021).</skos:definition>
	<skos:definition xml:lang="fr">Porosité créée au moment du dépôt et conservé lors de la diagenèse. (Fernandes et al., 2021)</skos:definition>
</rdf:Description>

<rdf:Description rdf:about="https://ark.frantiq.fr/ark:/26678/pcrt02hj78whx8">
	<rdf:type rdf:resource="http://www.w3.org/2004/02/skos/core#Concept"/>
	<skos:prefLabel xml:lang="en">fracture porosity</skos:prefLabel>
	<skos:prefLabel xml:lang="es">porosidad de fractura</skos:prefLabel>
	<skos:prefLabel xml:lang="it">porosità della fessura</skos:prefLabel>
	<skos:prefLabel xml:lang="fr">porosité de fissure</skos:prefLabel>
	<skos:prefLabel xml:lang="de">Rissporosität</skos:prefLabel>
	<skos:broader rdf:resource="https://ark.frantiq.fr/ark:/26678/pcrt0kvts48fht"/>
	<skos:inScheme rdf:resource="https://ark.frantiq.fr/ark:/26678/TH_1"/>
	<opentheso:memberOf rdf:resource="https://ark.frantiq.fr/ark:/26678/pcrtv66rn9cbv1"/>
	<opentheso:memberOf rdf:resource="https://ark.frantiq.fr/ark:/26678/pcrtnbDLi2FkAj"/>
	<dcterms:created rdf:datatype="http://www.w3.org/2001/XMLSchema#date">2021-02-18</dcterms:created>
	<dcterms:modified rdf:datatype="http://www.w3.org/2001/XMLSchema#date">2023-08-02</dcterms:modified>
	<dcterms:identifier>266529</dcterms:identifier>
	<dcterms:contributor>blandine.nouvel</dcterms:contributor>
	<skos:definition xml:lang="en">Porosity due to the existence of cracks and open diaclases caused by the rupture or shattering of a rock (Fernandes et al., 2021).</skos:definition>
	<skos:definition xml:lang="fr">Porosité due à l'existence de fissures et diaclases ouvertes dues à la rupture ou l'éclatement d'une roche. (Fernandes et al., 2021)</skos:definition>
</rdf:Description>

<rdf:Description rdf:about="https://ark.frantiq.fr/ark:/26678/pcrt96jkm5cgpf">
	<rdf:type rdf:resource="http://www.w3.org/2004/02/skos/core#Concept"/>
	<skos:prefLabel xml:lang="en">channel porosity</skos:prefLabel>
	<skos:prefLabel xml:lang="es">porosidad de canal</skos:prefLabel>
	<skos:prefLabel xml:lang="it">porosità del canale</skos:prefLabel>
	<skos:prefLabel xml:lang="fr">porosité de chenaux</skos:prefLabel>
	<skos:prefLabel xml:lang="de">Rinnenporosität</skos:prefLabel>
	<skos:broader rdf:resource="https://ark.frantiq.fr/ark:/26678/pcrt0kvts48fht"/>
	<skos:inScheme rdf:resource="https://ark.frantiq.fr/ark:/26678/TH_1"/>
	<opentheso:memberOf rdf:resource="https://ark.frantiq.fr/ark:/26678/pcrtv66rn9cbv1"/>
	<opentheso:memberOf rdf:resource="https://ark.frantiq.fr/ark:/26678/pcrtnbDLi2FkAj"/>
	<dcterms:created rdf:datatype="http://www.w3.org/2001/XMLSchema#date">2021-02-18</dcterms:created>
	<dcterms:modified rdf:datatype="http://www.w3.org/2001/XMLSchema#date">2024-11-21</dcterms:modified>
	<dcterms:identifier>266531</dcterms:identifier>
	<dcterms:contributor>blandine.nouvel</dcterms:contributor>
	<dcterms:contributor>justine.vincent</dcterms:contributor>
	<skos:definition xml:lang="en">Porosity created between two parts of the same rock that are no longer in contact but whose boundaries are irregular, often the result of biological activity in the sediments. (Fernandes et al., 2021)</skos:definition>
	<skos:definition xml:lang="fr">Porosité créé entre deux parties d'une même roche qui ne sont plus en contact mais dont les limites sont irrégulières, qui est souvent le résultat d'activité biologique dans les sédiments. (Fernandes et al., 2021)</skos:definition>
</rdf:Description>

<rdf:Description rdf:about="https://ark.frantiq.fr/ark:/26678/pcrt776pzvkdkn">
	<rdf:type rdf:resource="http://www.w3.org/2004/02/skos/core#Concept"/>
	<skos:prefLabel xml:lang="en">moldic porosity</skos:prefLabel>
	<skos:prefLabel xml:lang="de">moldische Porosität</skos:prefLabel>
	<skos:prefLabel xml:lang="es">porosidad móldica</skos:prefLabel>
	<skos:prefLabel xml:lang="it">porosità moldic</skos:prefLabel>
	<skos:prefLabel xml:lang="fr">porosité moldique</skos:prefLabel>
	<skos:altLabel xml:lang="it">porosità di tipo moldic</skos:altLabel>
	<skos:broader rdf:resource="https://ark.frantiq.fr/ark:/26678/pcrt0kvts48fht"/>
	<skos:inScheme rdf:resource="https://ark.frantiq.fr/ark:/26678/TH_1"/>
	<opentheso:memberOf rdf:resource="https://ark.frantiq.fr/ark:/26678/pcrtv66rn9cbv1"/>
	<opentheso:memberOf rdf:resource="https://ark.frantiq.fr/ark:/26678/pcrtnbDLi2FkAj"/>
	<dcterms:created rdf:datatype="http://www.w3.org/2001/XMLSchema#date">2021-02-18</dcterms:created>
	<dcterms:modified rdf:datatype="http://www.w3.org/2001/XMLSchema#date">2023-08-02</dcterms:modified>
	<dcterms:identifier>266533</dcterms:identifier>
	<dcterms:contributor>blandine.nouvel</dcterms:contributor>
	<skos:definition xml:lang="en">Mould porosity caused by the dissolution of a particular constituent of the rock (Fernandes et al., 2021).</skos:definition>
	<skos:definition xml:lang="fr">Porosité de moulage provoquée par la dissolution d’un constituant particulier de la roche. (Fernandes et al., 2021)</skos:definition>
</rdf:Description>

<rdf:Description rdf:about="https://ark.frantiq.fr/ark:/26678/pcrtv9c4m3q53k">
	<rdf:type rdf:resource="http://www.w3.org/2004/02/skos/core#Concept"/>
	<skos:prefLabel xml:lang="en">fenestral porosity</skos:prefLabel>
	<skos:prefLabel xml:lang="de">Fensterporosität</skos:prefLabel>
	<skos:prefLabel xml:lang="es">porosidad fenestral</skos:prefLabel>
	<skos:prefLabel xml:lang="it">porosità fenestrale</skos:prefLabel>
	<skos:prefLabel xml:lang="fr">porosité fenestrae</skos:prefLabel>
	<skos:broader rdf:resource="https://ark.frantiq.fr/ark:/26678/pcrt0kvts48fht"/>
	<skos:inScheme rdf:resource="https://ark.frantiq.fr/ark:/26678/TH_1"/>
	<opentheso:memberOf rdf:resource="https://ark.frantiq.fr/ark:/26678/pcrtv66rn9cbv1"/>
	<opentheso:memberOf rdf:resource="https://ark.frantiq.fr/ark:/26678/pcrtnbDLi2FkAj"/>
	<dcterms:created rdf:datatype="http://www.w3.org/2001/XMLSchema#date">2021-02-18</dcterms:created>
	<dcterms:modified rdf:datatype="http://www.w3.org/2001/XMLSchema#date">2024-11-21</dcterms:modified>
	<dcterms:identifier>266535</dcterms:identifier>
	<dcterms:contributor>blandine.nouvel</dcterms:contributor>
	<dcterms:contributor>justine.vincent</dcterms:contributor>
	<skos:definition xml:lang="en">Porosity characterised by the presence of isolated pores (Fernandes et al., 2021).</skos:definition>
	<skos:definition xml:lang="fr">Porosité caractérisée par la présence de pores isolés. (Fernandes et al., 2021)</skos:definition>
</rdf:Description>

<rdf:Description rdf:about="https://ark.frantiq.fr/ark:/26678/pcrt4n7gjb1qfh">
	<rdf:type rdf:resource="http://www.w3.org/2004/02/skos/core#Concept"/>
	<skos:prefLabel xml:lang="es">porosidad vacuolar</skos:prefLabel>
	<skos:prefLabel xml:lang="it">porosità vacuolare</skos:prefLabel>
	<skos:prefLabel xml:lang="fr">porosité vacuolaire</skos:prefLabel>
	<skos:prefLabel xml:lang="en">vacuole-shaped matrix porosity</skos:prefLabel>
	<skos:prefLabel xml:lang="de">vakuolare Porosität</skos:prefLabel>
	<skos:broader rdf:resource="https://ark.frantiq.fr/ark:/26678/pcrt0kvts48fht"/>
	<skos:inScheme rdf:resource="https://ark.frantiq.fr/ark:/26678/TH_1"/>
	<opentheso:memberOf rdf:resource="https://ark.frantiq.fr/ark:/26678/pcrtv66rn9cbv1"/>
	<opentheso:memberOf rdf:resource="https://ark.frantiq.fr/ark:/26678/pcrtnbDLi2FkAj"/>
	<dcterms:created rdf:datatype="http://www.w3.org/2001/XMLSchema#date">2021-02-18</dcterms:created>
	<dcterms:modified rdf:datatype="http://www.w3.org/2001/XMLSchema#date">2024-11-21</dcterms:modified>
	<dcterms:identifier>266537</dcterms:identifier>
	<dcterms:contributor>blandine.nouvel</dcterms:contributor>
	<dcterms:contributor>justine.vincent</dcterms:contributor>
	<skos:definition xml:lang="en">Porosity made up of voids left by the partial or total dissolution of certain figurative elements. (Fernandes et al., 2021)</skos:definition>
	<skos:definition xml:lang="fr">Porosité constituée par les vides laissés par la dissolution partielle ou totale de certains éléments figurés. (Fernandes et al., 2021)</skos:definition>
</rdf:Description>

<rdf:Description rdf:about="https://ark.frantiq.fr/ark:/26678/pcrttkxc1k68td">
	<rdf:type rdf:resource="http://www.w3.org/2004/02/skos/core#Concept"/>
	<skos:prefLabel xml:lang="en">intraparticle porosity</skos:prefLabel>
	<skos:prefLabel xml:lang="de">intrapartikuläre Porosität</skos:prefLabel>
	<skos:prefLabel xml:lang="es">porosidad intrapartícula</skos:prefLabel>
	<skos:prefLabel xml:lang="it">porosità intraparticellare</skos:prefLabel>
	<skos:prefLabel xml:lang="fr">porosité intraparticulaire</skos:prefLabel>
	<skos:altLabel xml:lang="fr">boxwork</skos:altLabel>
	<skos:altLabel xml:lang="de">Boxwork</skos:altLabel>
	<skos:broader rdf:resource="https://ark.frantiq.fr/ark:/26678/pcrt0kvts48fht"/>
	<skos:inScheme rdf:resource="https://ark.frantiq.fr/ark:/26678/TH_1"/>
	<opentheso:memberOf rdf:resource="https://ark.frantiq.fr/ark:/26678/pcrtv66rn9cbv1"/>
	<opentheso:memberOf rdf:resource="https://ark.frantiq.fr/ark:/26678/pcrtnbDLi2FkAj"/>
	<dcterms:created rdf:datatype="http://www.w3.org/2001/XMLSchema#date">2021-02-18</dcterms:created>
	<dcterms:modified rdf:datatype="http://www.w3.org/2001/XMLSchema#date">2023-08-02</dcterms:modified>
	<dcterms:identifier>266539</dcterms:identifier>
	<dcterms:contributor>blandine.nouvel</dcterms:contributor>
	<skos:definition xml:lang="en">Porosity linked to the differential dissolution of certain minerals while retaining their original shape. (Fernandes et al., 2021)</skos:definition>
	<skos:definition xml:lang="fr">Porosité liée à  la dissolution différentielle de certains minéraux en conservant leur forme originale. (Fernandes et al., 2021)</skos:definition>
</rdf:Description>

<rdf:Description rdf:about="https://ark.frantiq.fr/ark:/26678/pcrt73m1tx29mm">
	<rdf:type rdf:resource="http://www.w3.org/2004/02/skos/core#Concept"/>
	<skos:prefLabel xml:lang="en">geode porosity</skos:prefLabel>
	<skos:prefLabel xml:lang="de">geodische Porosität</skos:prefLabel>
	<skos:prefLabel xml:lang="es">porosidad geódica</skos:prefLabel>
	<skos:prefLabel xml:lang="it">porosità geodica</skos:prefLabel>
	<skos:prefLabel xml:lang="fr">porosité géodique</skos:prefLabel>
	<skos:broader rdf:resource="https://ark.frantiq.fr/ark:/26678/pcrt0kvts48fht"/>
	<skos:inScheme rdf:resource="https://ark.frantiq.fr/ark:/26678/TH_1"/>
	<opentheso:memberOf rdf:resource="https://ark.frantiq.fr/ark:/26678/pcrtv66rn9cbv1"/>
	<opentheso:memberOf rdf:resource="https://ark.frantiq.fr/ark:/26678/pcrtnbDLi2FkAj"/>
	<dcterms:created rdf:datatype="http://www.w3.org/2001/XMLSchema#date">2021-02-18</dcterms:created>
	<dcterms:modified rdf:datatype="http://www.w3.org/2001/XMLSchema#date">2023-08-02</dcterms:modified>
	<dcterms:identifier>266541</dcterms:identifier>
	<dcterms:contributor>blandine.nouvel</dcterms:contributor>
	<skos:definition xml:lang="en">Pores resulting from the development of geodes in rocks (Fernandes et al., 2021).</skos:definition>
	<skos:definition xml:lang="fr">Pores résultants du développement de géodes dans les roches. (Fernandes et al., 2021)</skos:definition>
</rdf:Description>

<rdf:Description rdf:about="https://ark.frantiq.fr/ark:/26678/pcrtpsrh8ptqjf">
	<rdf:type rdf:resource="http://www.w3.org/2004/02/skos/core#Concept"/>
	<skos:prefLabel xml:lang="en">intraclast porosity</skos:prefLabel>
	<skos:prefLabel xml:lang="de">intraklastische Porosität</skos:prefLabel>
	<skos:prefLabel xml:lang="es">porosidad intragranular</skos:prefLabel>
	<skos:prefLabel xml:lang="it">porosità intraclastica</skos:prefLabel>
	<skos:prefLabel xml:lang="fr">porosité intraclastique</skos:prefLabel>
	<skos:altLabel xml:lang="de">intragranulare Porosität</skos:altLabel>
	<skos:altLabel xml:lang="es">porosidad intraclástica</skos:altLabel>
	<skos:altLabel xml:lang="it">porosità intragranulare</skos:altLabel>
	<skos:altLabel xml:lang="fr">porosité intragranulaire</skos:altLabel>
	<skos:broader rdf:resource="https://ark.frantiq.fr/ark:/26678/pcrt0kvts48fht"/>
	<skos:inScheme rdf:resource="https://ark.frantiq.fr/ark:/26678/TH_1"/>
	<opentheso:memberOf rdf:resource="https://ark.frantiq.fr/ark:/26678/pcrtv66rn9cbv1"/>
	<opentheso:memberOf rdf:resource="https://ark.frantiq.fr/ark:/26678/pcrtnbDLi2FkAj"/>
	<dcterms:created rdf:datatype="http://www.w3.org/2001/XMLSchema#date">2021-02-18</dcterms:created>
	<dcterms:modified rdf:datatype="http://www.w3.org/2001/XMLSchema#date">2024-11-21</dcterms:modified>
	<dcterms:identifier>266543</dcterms:identifier>
	<dcterms:contributor>blandine.nouvel</dcterms:contributor>
	<dcterms:contributor>justine.vincent</dcterms:contributor>
	<skos:definition xml:lang="en">Corresponds to the voids formed within the figurative elements of a rock (Fernandes et al., 2021).</skos:definition>
	<skos:definition xml:lang="fr">Correspond aux vides formés à l'intérieur des éléments figurés d'une roche. (Fernandes et al., 2021)</skos:definition>
</rdf:Description>

<rdf:Description rdf:about="https://ark.frantiq.fr/ark:/26678/pcrtvq01hkvvn3">
	<rdf:type rdf:resource="http://www.w3.org/2004/02/skos/core#Concept"/>
	<skos:prefLabel xml:lang="en">interclast porosity</skos:prefLabel>
	<skos:prefLabel xml:lang="de">interklastische Porosität</skos:prefLabel>
	<skos:prefLabel xml:lang="es">porosidad intergranular</skos:prefLabel>
	<skos:prefLabel xml:lang="it">porosità interclastica</skos:prefLabel>
	<skos:prefLabel xml:lang="fr">porosité interclastique</skos:prefLabel>
	<skos:altLabel xml:lang="de">intergranulare Porosität</skos:altLabel>
	<skos:altLabel xml:lang="es">porosidad interclástica</skos:altLabel>
	<skos:altLabel xml:lang="it">porosità intergranulare</skos:altLabel>
	<skos:altLabel xml:lang="fr">porosité intergranulaire</skos:altLabel>
	<skos:broader rdf:resource="https://ark.frantiq.fr/ark:/26678/pcrt0kvts48fht"/>
	<skos:inScheme rdf:resource="https://ark.frantiq.fr/ark:/26678/TH_1"/>
	<opentheso:memberOf rdf:resource="https://ark.frantiq.fr/ark:/26678/pcrtv66rn9cbv1"/>
	<opentheso:memberOf rdf:resource="https://ark.frantiq.fr/ark:/26678/pcrtnbDLi2FkAj"/>
	<dcterms:created rdf:datatype="http://www.w3.org/2001/XMLSchema#date">2021-02-18</dcterms:created>
	<dcterms:modified rdf:datatype="http://www.w3.org/2001/XMLSchema#date">2023-08-02</dcterms:modified>
	<dcterms:identifier>266545</dcterms:identifier>
	<dcterms:contributor>blandine.nouvel</dcterms:contributor>
	<skos:definition xml:lang="en">Space left free between the figurative elements of a rock (Fernandes et al., 2021).</skos:definition>
	<skos:definition xml:lang="fr">Espace laissé libre entre les éléments figurés d'une roche. (Fernandes et al., 2021)</skos:definition>
</rdf:Description>

<rdf:Description rdf:about="https://ark.frantiq.fr/ark:/26678/pcrt11wm5hjnm3">
	<rdf:type rdf:resource="http://www.w3.org/2004/02/skos/core#Concept"/>
	<skos:prefLabel xml:lang="es">porosidad secundaria</skos:prefLabel>
	<skos:prefLabel xml:lang="it">porosità secondaria</skos:prefLabel>
	<skos:prefLabel xml:lang="fr">porosité secondaire</skos:prefLabel>
	<skos:prefLabel xml:lang="en">secondary porosity</skos:prefLabel>
	<skos:prefLabel xml:lang="de">sekundäre Porosität</skos:prefLabel>
	<skos:broader rdf:resource="https://ark.frantiq.fr/ark:/26678/pcrt0kvts48fht"/>
	<skos:inScheme rdf:resource="https://ark.frantiq.fr/ark:/26678/TH_1"/>
	<opentheso:memberOf rdf:resource="https://ark.frantiq.fr/ark:/26678/pcrtv66rn9cbv1"/>
	<opentheso:memberOf rdf:resource="https://ark.frantiq.fr/ark:/26678/pcrtnbDLi2FkAj"/>
	<dcterms:created rdf:datatype="http://www.w3.org/2001/XMLSchema#date">2021-02-18</dcterms:created>
	<dcterms:modified rdf:datatype="http://www.w3.org/2001/XMLSchema#date">2024-11-21</dcterms:modified>
	<dcterms:identifier>266547</dcterms:identifier>
	<dcterms:contributor>blandine.nouvel</dcterms:contributor>
	<dcterms:contributor>justine.vincent</dcterms:contributor>
	<skos:definition xml:lang="en">Porosity formed in sediments after deposition. (Fernandes et al., 2021)</skos:definition>
	<skos:definition xml:lang="fr">Porosité formée dans les sédiments après leur dépôt. (Fernandes et al., 2021)</skos:definition>
</rdf:Description>

<rdf:Description rdf:about="https://ark.frantiq.fr/ark:/26678/pcrt375srxkn5s">
	<rdf:type rdf:resource="http://www.w3.org/2004/02/skos/core#Concept"/>
	<skos:prefLabel xml:lang="en">intercrystalline porosity</skos:prefLabel>
	<skos:prefLabel xml:lang="de">interkristalline Porosität</skos:prefLabel>
	<skos:prefLabel xml:lang="es">porosidad intercristalina</skos:prefLabel>
	<skos:prefLabel xml:lang="it">porosità intercristallina</skos:prefLabel>
	<skos:prefLabel xml:lang="fr">porosité intercristalline</skos:prefLabel>
	<skos:broader rdf:resource="https://ark.frantiq.fr/ark:/26678/pcrt0kvts48fht"/>
	<skos:inScheme rdf:resource="https://ark.frantiq.fr/ark:/26678/TH_1"/>
	<opentheso:memberOf rdf:resource="https://ark.frantiq.fr/ark:/26678/pcrtv66rn9cbv1"/>
	<opentheso:memberOf rdf:resource="https://ark.frantiq.fr/ark:/26678/pcrtnbDLi2FkAj"/>
	<dcterms:created rdf:datatype="http://www.w3.org/2001/XMLSchema#date">2021-02-18</dcterms:created>
	<dcterms:modified rdf:datatype="http://www.w3.org/2001/XMLSchema#date">2024-11-21</dcterms:modified>
	<dcterms:identifier>266549</dcterms:identifier>
	<dcterms:contributor>blandine.nouvel</dcterms:contributor>
	<dcterms:contributor>justine.vincent</dcterms:contributor>
	<skos:definition xml:lang="en">Microporosity consisting of the pores between the crystals of a rock (Fernandes et al., 2021).</skos:definition>
	<skos:definition xml:lang="fr">Microporosité constituée par les pores situés entre les cristaux d'une roche. (Fernandes et al., 2021)</skos:definition>
</rdf:Description>

<rdf:Description rdf:about="https://ark.frantiq.fr/ark:/26678/pcrtqh6z41brjd">
	<rdf:type rdf:resource="http://www.w3.org/2004/02/skos/core#Concept"/>
	<skos:prefLabel xml:lang="en">pore lining (geology)</skos:prefLabel>
	<skos:prefLabel xml:lang="de">Porenauskleidung</skos:prefLabel>
	<skos:prefLabel xml:lang="fr">pore tapissé</skos:prefLabel>
	<skos:prefLabel xml:lang="es">poro revestido</skos:prefLabel>
	<skos:prefLabel xml:lang="it">poro rivestito</skos:prefLabel>
	<skos:broader rdf:resource="https://ark.frantiq.fr/ark:/26678/pcrt5m5pftg21t"/>
	<skos:inScheme rdf:resource="https://ark.frantiq.fr/ark:/26678/TH_1"/>
	<opentheso:memberOf rdf:resource="https://ark.frantiq.fr/ark:/26678/pcrtv66rn9cbv1"/>
	<opentheso:memberOf rdf:resource="https://ark.frantiq.fr/ark:/26678/pcrtnbDLi2FkAj"/>
	<dcterms:created rdf:datatype="http://www.w3.org/2001/XMLSchema#date">2021-02-18</dcterms:created>
	<dcterms:modified rdf:datatype="http://www.w3.org/2001/XMLSchema#date">2025-01-17</dcterms:modified>
	<dcterms:identifier>266551</dcterms:identifier>
	<dcterms:contributor>blandine.nouvel</dcterms:contributor>
	<skos:definition xml:lang="en">Mineral growth along the wall of voids in a rock; the core (or lumen) of the pore is not filled (Fernandes et al.: Vade-mecum pour la caractérisation pétroarchéologique des silicites, 2024).</skos:definition>
	<skos:definition xml:lang="fr">Croissance minérale le long de la paroi des vides dans une roche ; le cœur (ou lumière) du pore n'est pas rempli (Fernandes et al. : Vade-mecum pour la caractérisation pétroarchéologique des silicites, 2024).</skos:definition>
	<skos:historyNote xml:lang="fr">2025-01-17 : mise à jour de la réf. bibliographique dans la définition</skos:historyNote>
</rdf:Description>

<rdf:Description rdf:about="https://ark.frantiq.fr/ark:/26678/pcrt1qsxtkgq0f">
	<rdf:type rdf:resource="http://www.w3.org/2004/02/skos/core#Concept"/>
	<skos:prefLabel xml:lang="en">filled pore space (geology)</skos:prefLabel>
	<skos:prefLabel xml:lang="fr">pore colmaté</skos:prefLabel>
	<skos:prefLabel xml:lang="de">Porenverfüllung</skos:prefLabel>
	<skos:prefLabel xml:lang="it">poro colmato</skos:prefLabel>
	<skos:prefLabel xml:lang="es">poro tapado</skos:prefLabel>
	<skos:altLabel xml:lang="es">poro colmado</skos:altLabel>
	<skos:broader rdf:resource="https://ark.frantiq.fr/ark:/26678/pcrt5m5pftg21t"/>
	<skos:inScheme rdf:resource="https://ark.frantiq.fr/ark:/26678/TH_1"/>
	<opentheso:memberOf rdf:resource="https://ark.frantiq.fr/ark:/26678/pcrtv66rn9cbv1"/>
	<opentheso:memberOf rdf:resource="https://ark.frantiq.fr/ark:/26678/pcrtnbDLi2FkAj"/>
	<dcterms:created rdf:datatype="http://www.w3.org/2001/XMLSchema#date">2021-02-18</dcterms:created>
	<dcterms:modified rdf:datatype="http://www.w3.org/2001/XMLSchema#date">2023-08-02</dcterms:modified>
	<dcterms:identifier>266553</dcterms:identifier>
	<dcterms:contributor>blandine.nouvel</dcterms:contributor>
	<skos:definition xml:lang="en">Mineral growth that completely closes the pore of a rock. Mineral growth usually occurs from the edge (wall) to the core (lumen) of the pore (Fernandes et al., 2021).</skos:definition>
	<skos:definition xml:lang="fr">Croissance minérale qui vient totalement boucher le pore d'une roche. La croissance minérale s’effectue classiquement du bord (paroi) vers le cœur (lumière) du pore. (Fernandes et al., 2021)</skos:definition>
</rdf:Description>

<rdf:Description rdf:about="https://ark.frantiq.fr/ark:/26678/pcrtj6wgmdnp4k">
	<rdf:type rdf:resource="http://www.w3.org/2004/02/skos/core#Concept"/>
	<skos:prefLabel xml:lang="de">Auflösungszone</skos:prefLabel>
	<skos:prefLabel xml:lang="en">hydrolysis alteration zone</skos:prefLabel>
	<skos:prefLabel xml:lang="fr">plage de dissolution</skos:prefLabel>
	<skos:prefLabel xml:lang="es">rango de disolución</skos:prefLabel>
	<skos:prefLabel xml:lang="it">zona di dissoluzione</skos:prefLabel>
	<skos:broader rdf:resource="https://ark.frantiq.fr/ark:/26678/pcrtr5vk7w9vdz"/>
	<skos:inScheme rdf:resource="https://ark.frantiq.fr/ark:/26678/TH_1"/>
	<opentheso:memberOf rdf:resource="https://ark.frantiq.fr/ark:/26678/pcrtv66rn9cbv1"/>
	<opentheso:memberOf rdf:resource="https://ark.frantiq.fr/ark:/26678/pcrtnbDLi2FkAj"/>
	<dcterms:created rdf:datatype="http://www.w3.org/2001/XMLSchema#date">2021-02-24</dcterms:created>
	<dcterms:modified rdf:datatype="http://www.w3.org/2001/XMLSchema#date">2023-08-02</dcterms:modified>
	<dcterms:identifier>266609</dcterms:identifier>
	<dcterms:contributor>blandine.nouvel</dcterms:contributor>
	<skos:definition xml:lang="en">A concave area on the surface of a crystal or rock, usually caused by hydrolysis (Fernandes, 2012).</skos:definition>
	<skos:definition xml:lang="fr">Zone concave à la surface d’un cristal ou d’une roche, qui est généralement due à une hydrolyse (Fernandes, 2012).</skos:definition>
</rdf:Description>

<rdf:Description rdf:about="https://ark.frantiq.fr/ark:/26678/pcrtq9kn0538k0">
	<rdf:type rdf:resource="http://www.w3.org/2004/02/skos/core#Concept"/>
	<skos:prefLabel xml:lang="en">chemical composition of rocks</skos:prefLabel>
	<skos:prefLabel xml:lang="de">chemische Komponente des Gesteins</skos:prefLabel>
	<skos:prefLabel xml:lang="it">componente chimico delle rocce</skos:prefLabel>
	<skos:prefLabel xml:lang="es">componente químico de las rocas</skos:prefLabel>
	<skos:prefLabel xml:lang="fr">composant chimique des roches</skos:prefLabel>
	<skos:narrower rdf:resource="https://ark.frantiq.fr/ark:/26678/pcrtvd560z43dq"/>
	<skos:narrower rdf:resource="https://ark.frantiq.fr/ark:/26678/pcrt9bqtk5n9vs"/>
	<skos:narrower rdf:resource="https://ark.frantiq.fr/ark:/26678/pcrtc1qqps1k4g"/>
	<skos:broader rdf:resource="https://ark.frantiq.fr/ark:/26678/pcrtr5vk7w9vdz"/>
	<skos:inScheme rdf:resource="https://ark.frantiq.fr/ark:/26678/TH_1"/>
	<opentheso:memberOf rdf:resource="https://ark.frantiq.fr/ark:/26678/pcrtv66rn9cbv1"/>
	<opentheso:memberOf rdf:resource="https://ark.frantiq.fr/ark:/26678/pcrtnbDLi2FkAj"/>
	<dcterms:created rdf:datatype="http://www.w3.org/2001/XMLSchema#date">2021-03-12</dcterms:created>
	<dcterms:modified rdf:datatype="http://www.w3.org/2001/XMLSchema#date">2023-08-02</dcterms:modified>
	<dcterms:identifier>266660</dcterms:identifier>
	<dcterms:contributor>blandine.nouvel</dcterms:contributor>
</rdf:Description>

<rdf:Description rdf:about="https://ark.frantiq.fr/ark:/26678/pcrtvd560z43dq">
	<rdf:type rdf:resource="http://www.w3.org/2004/02/skos/core#Concept"/>
	<skos:prefLabel xml:lang="de">Pellet</skos:prefLabel>
	<skos:prefLabel xml:lang="fr">pelletoïde</skos:prefLabel>
	<skos:prefLabel xml:lang="en">pellet (petrology)</skos:prefLabel>
	<skos:prefLabel xml:lang="es">peloide</skos:prefLabel>
	<skos:prefLabel xml:lang="it">peloide</skos:prefLabel>
	<skos:narrower rdf:resource="https://ark.frantiq.fr/ark:/26678/pcrtcfbz4mzqtc"/>
	<skos:narrower rdf:resource="https://ark.frantiq.fr/ark:/26678/pcrtxt48rvckxp"/>
	<skos:narrower rdf:resource="https://ark.frantiq.fr/ark:/26678/pcrt1pj0md5g5q"/>
	<skos:broader rdf:resource="https://ark.frantiq.fr/ark:/26678/pcrtq9kn0538k0"/>
	<skos:inScheme rdf:resource="https://ark.frantiq.fr/ark:/26678/TH_1"/>
	<opentheso:memberOf rdf:resource="https://ark.frantiq.fr/ark:/26678/pcrtv66rn9cbv1"/>
	<opentheso:memberOf rdf:resource="https://ark.frantiq.fr/ark:/26678/pcrtnbDLi2FkAj"/>
	<dcterms:created rdf:datatype="http://www.w3.org/2001/XMLSchema#date">2021-03-12</dcterms:created>
	<dcterms:modified rdf:datatype="http://www.w3.org/2001/XMLSchema#date">2025-01-30</dcterms:modified>
	<dcterms:identifier>266662</dcterms:identifier>
	<dcterms:contributor>blandine.nouvel</dcterms:contributor>
	<dcterms:contributor>justine.vincent</dcterms:contributor>
	<skos:definition xml:lang="en">Structure made up of non-skeletal grains, without nuclei (between 100 and 500 µm) with a more or less regular morphology, rather ovoid, sometimes rod-shaped. (Fernandes et al, 2021)</skos:definition>
	<skos:definition xml:lang="fr">Structure constituée de grains non squelettiques, sans nucléus (entre 100 et 500 µm) à la morphologie plus ou moins régulière, plutôt ovoïde parfois en bâtonnet. (Fernandes et al, 2021)</skos:definition>
	<dcterms:source>https://doi-org.inshs.bib.cnrs.fr/10.4000/12zm5</dcterms:source>
</rdf:Description>

<rdf:Description rdf:about="https://ark.frantiq.fr/ark:/26678/pcrt9bqtk5n9vs">
	<rdf:type rdf:resource="http://www.w3.org/2004/02/skos/core#Concept"/>
	<skos:prefLabel xml:lang="en">aggregate</skos:prefLabel>
	<skos:prefLabel xml:lang="it">aggregato</skos:prefLabel>
	<skos:prefLabel xml:lang="es">agregado</skos:prefLabel>
	<skos:prefLabel xml:lang="de">Agregat</skos:prefLabel>
	<skos:prefLabel xml:lang="fr">agrégat</skos:prefLabel>
	<skos:narrower rdf:resource="https://ark.frantiq.fr/ark:/26678/pcrt277j912tkp"/>
	<skos:narrower rdf:resource="https://ark.frantiq.fr/ark:/26678/pcrtg4q8hhzgqb"/>
	<skos:narrower rdf:resource="https://ark.frantiq.fr/ark:/26678/pcrt558wf1f6dg"/>
	<skos:broader rdf:resource="https://ark.frantiq.fr/ark:/26678/pcrtq9kn0538k0"/>
	<skos:inScheme rdf:resource="https://ark.frantiq.fr/ark:/26678/TH_1"/>
	<opentheso:memberOf rdf:resource="https://ark.frantiq.fr/ark:/26678/pcrtv66rn9cbv1"/>
	<opentheso:memberOf rdf:resource="https://ark.frantiq.fr/ark:/26678/pcrtnbDLi2FkAj"/>
	<skos:exactMatch rdf:resource="https://www.wikidata.org/wiki/Q866298"/>
	<dcterms:created rdf:datatype="http://www.w3.org/2001/XMLSchema#date">2021-03-12</dcterms:created>
	<dcterms:modified rdf:datatype="http://www.w3.org/2001/XMLSchema#date">2025-01-30</dcterms:modified>
	<dcterms:identifier>266664</dcterms:identifier>
	<dcterms:contributor>blandine.nouvel</dcterms:contributor>
	<dcterms:contributor>justine.vincent</dcterms:contributor>
	<skos:definition xml:lang="fr">Fragment de roche rugueux (obtenu par concassage) ou arrondi (obtenu par érosion naturelle comme pour les galets), ou un matériau granulaire artificiel (par exemple le laitier métallurgique), d'une taille inférieure à 150 mm. (wikipedia)</skos:definition>
	<skos:definition xml:lang="en">Rough rock fragment (obtained by crushing) or rounded rock fragment (obtained by natural erosion, as in the case of pebbles), or an artificial granular material (e.g. metallurgical slag), smaller than 150 mm in size (wikipedia).</skos:definition>
	<skos:historyNote xml:lang="fr">2025-30-01 : modification de la définition.</skos:historyNote>
</rdf:Description>

<rdf:Description rdf:about="https://ark.frantiq.fr/ark:/26678/pcrtc1qqps1k4g">
	<rdf:type rdf:resource="http://www.w3.org/2004/02/skos/core#Concept"/>
	<skos:prefLabel xml:lang="de">eiförmig</skos:prefLabel>
	<skos:prefLabel xml:lang="en">ooid</skos:prefLabel>
	<skos:prefLabel xml:lang="es">ooide</skos:prefLabel>
	<skos:prefLabel xml:lang="it">ooide</skos:prefLabel>
	<skos:prefLabel xml:lang="fr">ooïde</skos:prefLabel>
	<skos:narrower rdf:resource="https://ark.frantiq.fr/ark:/26678/pcrt11g9hx0p5s"/>
	<skos:narrower rdf:resource="https://ark.frantiq.fr/ark:/26678/pcrtz6cz5t6ngd"/>
	<skos:narrower rdf:resource="https://ark.frantiq.fr/ark:/26678/pcrtdn47j0pbjt"/>
	<skos:narrower rdf:resource="https://ark.frantiq.fr/ark:/26678/pcrtmk1p11fm4k"/>
	<skos:narrower rdf:resource="https://ark.frantiq.fr/ark:/26678/pcrtq7hgb8vqh2"/>
	<skos:narrower rdf:resource="https://ark.frantiq.fr/ark:/26678/pcrtxrcv4dz28t"/>
	<skos:broader rdf:resource="https://ark.frantiq.fr/ark:/26678/pcrtq9kn0538k0"/>
	<skos:inScheme rdf:resource="https://ark.frantiq.fr/ark:/26678/TH_1"/>
	<opentheso:memberOf rdf:resource="https://ark.frantiq.fr/ark:/26678/pcrtv66rn9cbv1"/>
	<opentheso:memberOf rdf:resource="https://ark.frantiq.fr/ark:/26678/pcrtnbDLi2FkAj"/>
	<skos:exactMatch rdf:resource="https://www.wikidata.org/wiki/Q642735"/>
	<dcterms:created rdf:datatype="http://www.w3.org/2001/XMLSchema#date">2021-03-12</dcterms:created>
	<dcterms:modified rdf:datatype="http://www.w3.org/2001/XMLSchema#date">2025-01-30</dcterms:modified>
	<dcterms:identifier>266666</dcterms:identifier>
	<dcterms:contributor>blandine.nouvel</dcterms:contributor>
	<dcterms:contributor>justine.vincent</dcterms:contributor>
	<skos:definition xml:lang="fr">Grain de forme sphéroïdale et de nature généralement calcaire avec nucléus, subdivisés en six groupes (oolithes, sphérulithes, spastholithe, pseud-oolithe, grain composite et bahamites) et se caractérisant par un classement granulométrique presque parfait associé à des stratifications entrecroisées. (Fernandes et al., 2021)</skos:definition>
	<skos:definition xml:lang="en">Spheroidal grain of a generally calcareous nature with nuclei, subdivided into six groups (oolites, spherulites, spastholite, pseudo-oolite, composite grain and bahamites) and characterised by an almost perfect granulometric classification associated with criss-cross stratification. (Fernandes et al., 2021)</skos:definition>
	<skos:historyNote xml:lang="fr">2025-30-01 : modification de la définition.</skos:historyNote>
	<dcterms:source>https://doi-org.inshs.bib.cnrs.fr/10.4000/12zm5</dcterms:source>
</rdf:Description>

<rdf:Description rdf:about="https://ark.frantiq.fr/ark:/26678/pcrtcfbz4mzqtc">
	<rdf:type rdf:resource="http://www.w3.org/2004/02/skos/core#Concept"/>
	<skos:prefLabel xml:lang="en">coated grain</skos:prefLabel>
	<skos:prefLabel xml:lang="fr">coated grain</skos:prefLabel>
	<skos:prefLabel xml:lang="it">coated grain</skos:prefLabel>
	<skos:prefLabel xml:lang="es">granos con envueltas</skos:prefLabel>
	<skos:prefLabel xml:lang="de">Rindenkorn</skos:prefLabel>
	<skos:altLabel xml:lang="es">coated grain</skos:altLabel>
	<skos:altLabel xml:lang="it">granuli rivestiti</skos:altLabel>
	<skos:narrower rdf:resource="https://ark.frantiq.fr/ark:/26678/pcrt78g8rrd958"/>
	<skos:narrower rdf:resource="https://ark.frantiq.fr/ark:/26678/pcrt12db2x701r"/>
	<skos:narrower rdf:resource="https://ark.frantiq.fr/ark:/26678/pcrtnc6zr3n8dr"/>
	<skos:broader rdf:resource="https://ark.frantiq.fr/ark:/26678/pcrtvd560z43dq"/>
	<skos:inScheme rdf:resource="https://ark.frantiq.fr/ark:/26678/TH_1"/>
	<opentheso:memberOf rdf:resource="https://ark.frantiq.fr/ark:/26678/pcrtv66rn9cbv1"/>
	<opentheso:memberOf rdf:resource="https://ark.frantiq.fr/ark:/26678/pcrtnbDLi2FkAj"/>
	<dcterms:created rdf:datatype="http://www.w3.org/2001/XMLSchema#date">2021-03-12</dcterms:created>
	<dcterms:modified rdf:datatype="http://www.w3.org/2001/XMLSchema#date">2025-01-30</dcterms:modified>
	<dcterms:identifier>266668</dcterms:identifier>
	<dcterms:contributor>blandine.nouvel</dcterms:contributor>
	<dcterms:contributor>justine.vincent</dcterms:contributor>
	<skos:definition xml:lang="en">A generic term for all figurative elements with a chemical or biochemical film (Fernandes et al, 2021).</skos:definition>
	<skos:definition xml:lang="fr">Terme générique qui correspond à l’ensemble des éléments figurés qui présentent un film d’origine chimique ou biochimique. (Fernandes et al, 2021)</skos:definition>
	<dcterms:source>https://doi-org.inshs.bib.cnrs.fr/10.4000/12zm5</dcterms:source>
</rdf:Description>

<rdf:Description rdf:about="https://ark.frantiq.fr/ark:/26678/pcrtxt48rvckxp">
	<rdf:type rdf:resource="http://www.w3.org/2004/02/skos/core#Concept"/>
	<skos:prefLabel xml:lang="es">pellet</skos:prefLabel>
	<skos:prefLabel xml:lang="fr">pellet</skos:prefLabel>
	<skos:prefLabel xml:lang="it">pellet</skos:prefLabel>
	<skos:prefLabel xml:lang="de">Pellet</skos:prefLabel>
	<skos:prefLabel xml:lang="en">pellet (petrology)</skos:prefLabel>
	<skos:related rdf:resource="https://ark.frantiq.fr/ark:/26678/pcrt0Ffns3pZ28"/>
	<skos:broader rdf:resource="https://ark.frantiq.fr/ark:/26678/pcrtvd560z43dq"/>
	<skos:inScheme rdf:resource="https://ark.frantiq.fr/ark:/26678/TH_1"/>
	<opentheso:memberOf rdf:resource="https://ark.frantiq.fr/ark:/26678/pcrtv66rn9cbv1"/>
	<opentheso:memberOf rdf:resource="https://ark.frantiq.fr/ark:/26678/pcrtnbDLi2FkAj"/>
	<dcterms:created rdf:datatype="http://www.w3.org/2001/XMLSchema#date">2021-03-12</dcterms:created>
	<dcterms:modified rdf:datatype="http://www.w3.org/2001/XMLSchema#date">2025-01-30</dcterms:modified>
	<dcterms:identifier>266670</dcterms:identifier>
	<dcterms:contributor>blandine.nouvel</dcterms:contributor>
	<dcterms:contributor>justine.vincent</dcterms:contributor>
	<skos:definition xml:lang="en">Aggregation of ovoid micritic elements of 40 to 100 µm, not very compact, without internal structure and initially rich in organic matter. (Fernandes et al, 2021)</skos:definition>
	<skos:definition xml:lang="fr">Agrégation d'éléments micritiques ovoïdes de 40 à 100 µm, peu compacts, dépourvus de structure interne et initialement riches en matières organiques. (Fernandes et al, 2021)</skos:definition>
	<skos:historyNote xml:lang="fr">2025-30-01 : modification de la définition.</skos:historyNote>
	<dcterms:source>https://doi-org.inshs.bib.cnrs.fr/10.4000/12zm5</dcterms:source>
</rdf:Description>

<rdf:Description rdf:about="https://ark.frantiq.fr/ark:/26678/pcrt1pj0md5g5q">
	<rdf:type rdf:resource="http://www.w3.org/2004/02/skos/core#Concept"/>
	<skos:prefLabel xml:lang="it">ghiaietto</skos:prefLabel>
	<skos:prefLabel xml:lang="en">gravel</skos:prefLabel>
	<skos:prefLabel xml:lang="fr">gravele</skos:prefLabel>
	<skos:prefLabel xml:lang="es">gravilla</skos:prefLabel>
	<skos:prefLabel xml:lang="de">Kies</skos:prefLabel>
	<skos:altLabel xml:lang="fr">gravelle</skos:altLabel>
	<skos:altLabel xml:lang="fr">graviers</skos:altLabel>
	<skos:broader rdf:resource="https://ark.frantiq.fr/ark:/26678/pcrtvd560z43dq"/>
	<skos:inScheme rdf:resource="https://ark.frantiq.fr/ark:/26678/TH_1"/>
	<opentheso:memberOf rdf:resource="https://ark.frantiq.fr/ark:/26678/pcrtv66rn9cbv1"/>
	<opentheso:memberOf rdf:resource="https://ark.frantiq.fr/ark:/26678/pcrtnbDLi2FkAj"/>
	<opentheso:memberOf rdf:resource="https://ark.frantiq.fr/ark:/26678/pcrtv0jq332vcq3gxt5m13d5"/>
	<dcterms:created rdf:datatype="http://www.w3.org/2001/XMLSchema#date">2021-03-12</dcterms:created>
	<dcterms:modified rdf:datatype="http://www.w3.org/2001/XMLSchema#date">2025-01-30</dcterms:modified>
	<dcterms:identifier>266672</dcterms:identifier>
	<dcterms:contributor>blandine.nouvel</dcterms:contributor>
	<dcterms:contributor>justine.vincent</dcterms:contributor>
	<dcterms:contributor>patricia.moitrel</dcterms:contributor>
	<skos:definition xml:lang="en">Small rounded or blunt limestone grain used in the composition of certain detrital limestones (Larousse).</skos:definition>
	<skos:definition xml:lang="fr">Petit grain calcaire arrondi ou émoussé entrant dans la composition de certains calcaires détritiques (Larousse).</skos:definition>
</rdf:Description>

<rdf:Description rdf:about="https://ark.frantiq.fr/ark:/26678/pcrt78g8rrd958">
	<rdf:type rdf:resource="http://www.w3.org/2004/02/skos/core#Concept"/>
	<skos:prefLabel xml:lang="en">oncolite</skos:prefLabel>
	<skos:prefLabel xml:lang="it">oncolite</skos:prefLabel>
	<skos:prefLabel xml:lang="fr">oncolithe</skos:prefLabel>
	<skos:prefLabel xml:lang="es">oncolito</skos:prefLabel>
	<skos:prefLabel xml:lang="de">Onkolith</skos:prefLabel>
	<skos:altLabel xml:lang="fr">oncolite</skos:altLabel>
	<skos:broader rdf:resource="https://ark.frantiq.fr/ark:/26678/pcrtcfbz4mzqtc"/>
	<skos:inScheme rdf:resource="https://ark.frantiq.fr/ark:/26678/TH_1"/>
	<opentheso:memberOf rdf:resource="https://ark.frantiq.fr/ark:/26678/pcrtv66rn9cbv1"/>
	<opentheso:memberOf rdf:resource="https://ark.frantiq.fr/ark:/26678/pcrtnbDLi2FkAj"/>
	<skos:exactMatch rdf:resource="https://www.wikidata.org/wiki/Q1194827"/>
	<dcterms:created rdf:datatype="http://www.w3.org/2001/XMLSchema#date">2021-03-12</dcterms:created>
	<dcterms:modified rdf:datatype="http://www.w3.org/2001/XMLSchema#date">2025-01-30</dcterms:modified>
	<dcterms:identifier>266674</dcterms:identifier>
	<dcterms:contributor>blandine.nouvel</dcterms:contributor>
	<dcterms:contributor>justine.vincent</dcterms:contributor>
	<skos:definition xml:lang="en">Ooids originating from shallow marine or fluvial environments, formed by encrustation of algal or microbial origin, with an irregular external morphology marked by concavities. (Fernandes et al, 2021)</skos:definition>
	<skos:definition xml:lang="fr">Ooïdes issus de milieux marins ou fluviatiles peu profonds, formés par encroûtement d'origine algaire ou microbienne dont la morphologie externe irrégulière est marquée de concavités. (Fernandes et al, 2021)</skos:definition>
	<skos:historyNote xml:lang="fr">2025-30-01 : modification de la définition.</skos:historyNote>
	<dcterms:source>https://doi-org.inshs.bib.cnrs.fr/10.4000/12zm5</dcterms:source>
</rdf:Description>

<rdf:Description rdf:about="https://ark.frantiq.fr/ark:/26678/pcrt12db2x701r">
	<rdf:type rdf:resource="http://www.w3.org/2004/02/skos/core#Concept"/>
	<skos:prefLabel xml:lang="en">pisolite</skos:prefLabel>
	<skos:prefLabel xml:lang="it">pisolite</skos:prefLabel>
	<skos:prefLabel xml:lang="de">Pisolith</skos:prefLabel>
	<skos:prefLabel xml:lang="fr">pisolithe</skos:prefLabel>
	<skos:prefLabel xml:lang="es">pisolito</skos:prefLabel>
	<skos:broader rdf:resource="https://ark.frantiq.fr/ark:/26678/pcrtcfbz4mzqtc"/>
	<skos:inScheme rdf:resource="https://ark.frantiq.fr/ark:/26678/TH_1"/>
	<opentheso:memberOf rdf:resource="https://ark.frantiq.fr/ark:/26678/pcrtv66rn9cbv1"/>
	<opentheso:memberOf rdf:resource="https://ark.frantiq.fr/ark:/26678/pcrtnbDLi2FkAj"/>
	<skos:exactMatch rdf:resource="https://www.wikidata.org/wiki/Q1760214"/>
	<dcterms:created rdf:datatype="http://www.w3.org/2001/XMLSchema#date">2021-03-12</dcterms:created>
	<dcterms:modified rdf:datatype="http://www.w3.org/2001/XMLSchema#date">2025-01-30</dcterms:modified>
	<dcterms:identifier>266676</dcterms:identifier>
	<dcterms:contributor>blandine.nouvel</dcterms:contributor>
	<dcterms:contributor>justine.vincent</dcterms:contributor>
	<skos:definition xml:lang="en">Large spherical element with a diameter greater than 2 mm, generally calcareous, with a concentric structure, resulting from direct precipitation or precipitation induced by algae (Fernandes et al, 2021).</skos:definition>
	<skos:definition xml:lang="fr">Grand élément sphérique de diamètre supérieur à 2 mm, généralement calcaire, à structure concentrique, issue de la précipitation directe ou induite par des algues. (Fernandes et al, 2021)</skos:definition>
	<dcterms:source>https://doi-org.inshs.bib.cnrs.fr/10.4000/12zm5</dcterms:source>
</rdf:Description>

<rdf:Description rdf:about="https://ark.frantiq.fr/ark:/26678/pcrtnc6zr3n8dr">
	<rdf:type rdf:resource="http://www.w3.org/2004/02/skos/core#Concept"/>
	<skos:prefLabel xml:lang="en">vadoid</skos:prefLabel>
	<skos:prefLabel xml:lang="es">vadoid</skos:prefLabel>
	<skos:prefLabel xml:lang="fr">vadoid</skos:prefLabel>
	<skos:prefLabel xml:lang="it">vadoid</skos:prefLabel>
	<skos:prefLabel xml:lang="de">Vadoid</skos:prefLabel>
	<skos:broader rdf:resource="https://ark.frantiq.fr/ark:/26678/pcrtcfbz4mzqtc"/>
	<skos:inScheme rdf:resource="https://ark.frantiq.fr/ark:/26678/TH_1"/>
	<opentheso:memberOf rdf:resource="https://ark.frantiq.fr/ark:/26678/pcrtv66rn9cbv1"/>
	<opentheso:memberOf rdf:resource="https://ark.frantiq.fr/ark:/26678/pcrtnbDLi2FkAj"/>
	<dcterms:created rdf:datatype="http://www.w3.org/2001/XMLSchema#date">2021-03-12</dcterms:created>
	<dcterms:modified rdf:datatype="http://www.w3.org/2001/XMLSchema#date">2025-01-30</dcterms:modified>
	<dcterms:identifier>266678</dcterms:identifier>
	<dcterms:contributor>blandine.nouvel</dcterms:contributor>
	<dcterms:contributor>justine.vincent</dcterms:contributor>
	<skos:definition xml:lang="en">More or less rounded element resulting from epigenetic replacement of an organic body developed in a vadose zone. Common form in pedogenetic silcrete (Fernandes et al, 2021).</skos:definition>
	<skos:definition xml:lang="fr">Elément plus ou moins arrondis issu d’un remplacement épigénitique d’un corps organique développé dans une zone vadose. Forme fréquente dans les silcrètes pédogénétiques.(Fernandes et al, 2021)</skos:definition>
	<dcterms:source>https://doi-org.inshs.bib.cnrs.fr/10.4000/12zm5</dcterms:source>
</rdf:Description>

<rdf:Description rdf:about="https://ark.frantiq.fr/ark:/26678/pcrt277j912tkp">
	<rdf:type rdf:resource="http://www.w3.org/2004/02/skos/core#Concept"/>
	<skos:prefLabel xml:lang="es">granos agregados</skos:prefLabel>
	<skos:prefLabel xml:lang="de">Klumpen</skos:prefLabel>
	<skos:prefLabel xml:lang="en">lump</skos:prefLabel>
	<skos:prefLabel xml:lang="fr">lump</skos:prefLabel>
	<skos:prefLabel xml:lang="it">lump</skos:prefLabel>
	<skos:altLabel xml:lang="it">granuli aggregati</skos:altLabel>
	<skos:altLabel xml:lang="es">lump</skos:altLabel>
	<skos:broader rdf:resource="https://ark.frantiq.fr/ark:/26678/pcrt9bqtk5n9vs"/>
	<skos:inScheme rdf:resource="https://ark.frantiq.fr/ark:/26678/TH_1"/>
	<opentheso:memberOf rdf:resource="https://ark.frantiq.fr/ark:/26678/pcrtv66rn9cbv1"/>
	<opentheso:memberOf rdf:resource="https://ark.frantiq.fr/ark:/26678/pcrtnbDLi2FkAj"/>
	<dcterms:created rdf:datatype="http://www.w3.org/2001/XMLSchema#date">2021-03-12</dcterms:created>
	<dcterms:modified rdf:datatype="http://www.w3.org/2001/XMLSchema#date">2025-01-30</dcterms:modified>
	<dcterms:identifier>266680</dcterms:identifier>
	<dcterms:contributor>blandine.nouvel</dcterms:contributor>
	<dcterms:contributor>justine.vincent</dcterms:contributor>
	<skos:definition xml:lang="fr">Agrégat à morphologie irrégulière lié à l'agglutination de grains ou de graviers. (Fernandes et al., 2021)</skos:definition>
	<skos:definition xml:lang="en">Aggregate with irregular morphology due to the agglutination of grains or gravel. (Fernandes et al., 2021)</skos:definition>
	<dcterms:source>https://doi-org.inshs.bib.cnrs.fr/10.4000/12zm5</dcterms:source>
</rdf:Description>

<rdf:Description rdf:about="https://ark.frantiq.fr/ark:/26678/pcrtg4q8hhzgqb">
	<rdf:type rdf:resource="http://www.w3.org/2004/02/skos/core#Concept"/>
	<skos:prefLabel xml:lang="en">mudball</skos:prefLabel>
	<skos:prefLabel xml:lang="es">mudball</skos:prefLabel>
	<skos:prefLabel xml:lang="fr">mudball</skos:prefLabel>
	<skos:prefLabel xml:lang="it">mudball</skos:prefLabel>
	<skos:prefLabel xml:lang="de">Schlammgeröll</skos:prefLabel>
	<skos:altLabel xml:lang="it">aggregati di fango</skos:altLabel>
	<skos:broader rdf:resource="https://ark.frantiq.fr/ark:/26678/pcrt9bqtk5n9vs"/>
	<skos:inScheme rdf:resource="https://ark.frantiq.fr/ark:/26678/TH_1"/>
	<opentheso:memberOf rdf:resource="https://ark.frantiq.fr/ark:/26678/pcrtv66rn9cbv1"/>
	<opentheso:memberOf rdf:resource="https://ark.frantiq.fr/ark:/26678/pcrtnbDLi2FkAj"/>
	<dcterms:created rdf:datatype="http://www.w3.org/2001/XMLSchema#date">2021-03-12</dcterms:created>
	<dcterms:modified rdf:datatype="http://www.w3.org/2001/XMLSchema#date">2025-01-30</dcterms:modified>
	<dcterms:identifier>266682</dcterms:identifier>
	<dcterms:contributor>blandine.nouvel</dcterms:contributor>
	<dcterms:contributor>justine.vincent</dcterms:contributor>
	<skos:definition xml:lang="en">A multi-millimetre to multi-centimetre, more or less spherical mass of mud in sedimentary rock. (Fernandes et al., 2021)</skos:definition>
	<skos:definition xml:lang="fr">Masse de boue plurimillimétrique à pluricentimétrique, plus ou moins sphérique dans une roche sédimentaire. (Fernandes et al., 2021)</skos:definition>
	<dcterms:source>https://doi-org.inshs.bib.cnrs.fr/10.4000/12zm5</dcterms:source>
</rdf:Description>

<rdf:Description rdf:about="https://ark.frantiq.fr/ark:/26678/pcrt558wf1f6dg">
	<rdf:type rdf:resource="http://www.w3.org/2004/02/skos/core#Concept"/>
	<skos:prefLabel xml:lang="en">grapestone</skos:prefLabel>
	<skos:prefLabel xml:lang="es">grapestone</skos:prefLabel>
	<skos:prefLabel xml:lang="fr">grapestone</skos:prefLabel>
	<skos:prefLabel xml:lang="it">grapestone</skos:prefLabel>
	<skos:prefLabel xml:lang="de">traubenförmiges Gestein</skos:prefLabel>
	<skos:altLabel xml:lang="it">agglomerato a grappolo</skos:altLabel>
	<skos:altLabel xml:lang="it">granuli aggregati</skos:altLabel>
	<skos:broader rdf:resource="https://ark.frantiq.fr/ark:/26678/pcrt9bqtk5n9vs"/>
	<skos:inScheme rdf:resource="https://ark.frantiq.fr/ark:/26678/TH_1"/>
	<opentheso:memberOf rdf:resource="https://ark.frantiq.fr/ark:/26678/pcrtv66rn9cbv1"/>
	<opentheso:memberOf rdf:resource="https://ark.frantiq.fr/ark:/26678/pcrtnbDLi2FkAj"/>
	<dcterms:created rdf:datatype="http://www.w3.org/2001/XMLSchema#date">2021-03-12</dcterms:created>
	<dcterms:modified rdf:datatype="http://www.w3.org/2001/XMLSchema#date">2025-01-30</dcterms:modified>
	<dcterms:identifier>266684</dcterms:identifier>
	<dcterms:contributor>blandine.nouvel</dcterms:contributor>
	<dcterms:contributor>justine.vincent</dcterms:contributor>
	<skos:definition xml:lang="en">Aggregate composed of peloids, bioclasts and cemented coated grain. (Fernandes et al., 2021)</skos:definition>
	<skos:definition xml:lang="fr">Agrégat composé de peloïdes, de bioclastes et de coated grain cimentés. (Fernandes et al., 2021)</skos:definition>
	<dcterms:source>https://doi-org.inshs.bib.cnrs.fr/10.4000/12zm5</dcterms:source>
</rdf:Description>

<rdf:Description rdf:about="https://ark.frantiq.fr/ark:/26678/pcrt11g9hx0p5s">
	<rdf:type rdf:resource="http://www.w3.org/2004/02/skos/core#Concept"/>
	<skos:prefLabel xml:lang="en">oolite</skos:prefLabel>
	<skos:prefLabel xml:lang="it">oolite</skos:prefLabel>
	<skos:prefLabel xml:lang="de">Oolith</skos:prefLabel>
	<skos:prefLabel xml:lang="fr">oolithe</skos:prefLabel>
	<skos:prefLabel xml:lang="es">oolito</skos:prefLabel>
	<skos:altLabel xml:lang="fr">oolite</skos:altLabel>
	<skos:altLabel xml:lang="en">oölite</skos:altLabel>
	<skos:related rdf:resource="https://ark.frantiq.fr/ark:/26678/pcrth30k691qrk"/>
	<skos:broader rdf:resource="https://ark.frantiq.fr/ark:/26678/pcrtc1qqps1k4g"/>
	<skos:inScheme rdf:resource="https://ark.frantiq.fr/ark:/26678/TH_1"/>
	<opentheso:memberOf rdf:resource="https://ark.frantiq.fr/ark:/26678/pcrtv66rn9cbv1"/>
	<opentheso:memberOf rdf:resource="https://ark.frantiq.fr/ark:/26678/pcrtnbDLi2FkAj"/>
	<skos:exactMatch rdf:resource="https://www.wikidata.org/wiki/Q632078"/>
	<dcterms:created rdf:datatype="http://www.w3.org/2001/XMLSchema#date">2021-03-12</dcterms:created>
	<dcterms:modified rdf:datatype="http://www.w3.org/2001/XMLSchema#date">2025-01-30</dcterms:modified>
	<dcterms:identifier>266686</dcterms:identifier>
	<dcterms:contributor>blandine.nouvel</dcterms:contributor>
	<dcterms:contributor>justine.vincent</dcterms:contributor>
	<skos:definition xml:lang="en">Element of chemical origin that composes oolitic rocks, in the form of small spheres with a nucleus (bioclast or lithoclast) 0.5 to 2 mm in diameter characterised by the predominance of concentric cortical laminations of primary origin. (Fernandes et al., 2021)</skos:definition>
	<skos:definition xml:lang="fr">Elément d'origine chimique qui compose les roches oolithiques, se présentant sous forme de petites sphères à nucléus (bioclaste ou lithoclaste) de 0,5 à 2 mm de diamètre caractérisées par la prédominance de laminations corticales concentriques d'origine primaire. (Fernandes et al., 2021)</skos:definition>
	<dcterms:source>https://doi-org.inshs.bib.cnrs.fr/10.4000/12zm5</dcterms:source>
</rdf:Description>

<rdf:Description rdf:about="https://ark.frantiq.fr/ark:/26678/pcrtz6cz5t6ngd">
	<rdf:type rdf:resource="http://www.w3.org/2004/02/skos/core#Concept"/>
	<skos:prefLabel xml:lang="es">espastolito</skos:prefLabel>
	<skos:prefLabel xml:lang="fr">spastholithe</skos:prefLabel>
	<skos:prefLabel xml:lang="en">spastolite</skos:prefLabel>
	<skos:prefLabel xml:lang="it">spastolite</skos:prefLabel>
	<skos:prefLabel xml:lang="de">Spastolith</skos:prefLabel>
	<skos:altLabel xml:lang="fr">spastholite</skos:altLabel>
	<skos:broader rdf:resource="https://ark.frantiq.fr/ark:/26678/pcrtc1qqps1k4g"/>
	<skos:inScheme rdf:resource="https://ark.frantiq.fr/ark:/26678/TH_1"/>
	<opentheso:memberOf rdf:resource="https://ark.frantiq.fr/ark:/26678/pcrtv66rn9cbv1"/>
	<opentheso:memberOf rdf:resource="https://ark.frantiq.fr/ark:/26678/pcrtnbDLi2FkAj"/>
	<dcterms:created rdf:datatype="http://www.w3.org/2001/XMLSchema#date">2021-03-12</dcterms:created>
	<dcterms:modified rdf:datatype="http://www.w3.org/2001/XMLSchema#date">2025-01-30</dcterms:modified>
	<dcterms:identifier>266688</dcterms:identifier>
	<dcterms:contributor>blandine.nouvel</dcterms:contributor>
	<dcterms:contributor>justine.vincent</dcterms:contributor>
	<skos:definition xml:lang="en">Deformed oolite, often flattened. (Fernandes et al., 2021)</skos:definition>
	<skos:definition xml:lang="fr">Oolithe défomrée, souvent aplatie. (Fernandes et al., 2021)</skos:definition>
	<dcterms:source>https://doi-org.inshs.bib.cnrs.fr/10.4000/12zm5</dcterms:source>
</rdf:Description>

<rdf:Description rdf:about="https://ark.frantiq.fr/ark:/26678/pcrtdn47j0pbjt">
	<rdf:type rdf:resource="http://www.w3.org/2004/02/skos/core#Concept"/>
	<skos:prefLabel xml:lang="es">esferulito</skos:prefLabel>
	<skos:prefLabel xml:lang="it">sferolite</skos:prefLabel>
	<skos:prefLabel xml:lang="de">Sphärulith</skos:prefLabel>
	<skos:prefLabel xml:lang="en">spherulite</skos:prefLabel>
	<skos:prefLabel xml:lang="fr">sphérulithe</skos:prefLabel>
	<skos:altLabel xml:lang="es">esferulita</skos:altLabel>
	<skos:altLabel xml:lang="it">sferulite</skos:altLabel>
	<skos:broader rdf:resource="https://ark.frantiq.fr/ark:/26678/pcrtc1qqps1k4g"/>
	<skos:inScheme rdf:resource="https://ark.frantiq.fr/ark:/26678/TH_1"/>
	<opentheso:memberOf rdf:resource="https://ark.frantiq.fr/ark:/26678/pcrtv66rn9cbv1"/>
	<opentheso:memberOf rdf:resource="https://ark.frantiq.fr/ark:/26678/pcrtnbDLi2FkAj"/>
	<skos:exactMatch rdf:resource="https://www.wikidata.org/wiki/Q46262"/>
	<dcterms:created rdf:datatype="http://www.w3.org/2001/XMLSchema#date">2021-03-12</dcterms:created>
	<dcterms:modified rdf:datatype="http://www.w3.org/2001/XMLSchema#date">2025-01-30</dcterms:modified>
	<dcterms:identifier>266690</dcterms:identifier>
	<dcterms:contributor>blandine.nouvel</dcterms:contributor>
	<dcterms:contributor>justine.vincent</dcterms:contributor>
	<skos:definition xml:lang="en">Oolite with a radial cortex structure. (Fernandes et al., 2021)</skos:definition>
	<skos:definition xml:lang="fr">Oolithe dont le cortex montre une structure radiaire. (Fernandes et al., 2021)</skos:definition>
	<dcterms:source>https://doi-org.inshs.bib.cnrs.fr/10.4000/12zm5</dcterms:source>
</rdf:Description>

<rdf:Description rdf:about="https://ark.frantiq.fr/ark:/26678/pcrtmk1p11fm4k">
	<rdf:type rdf:resource="http://www.w3.org/2004/02/skos/core#Concept"/>
	<skos:prefLabel xml:lang="de">Bahamit</skos:prefLabel>
	<skos:prefLabel xml:lang="es">bahamita</skos:prefLabel>
	<skos:prefLabel xml:lang="en">bahamite</skos:prefLabel>
	<skos:prefLabel xml:lang="it">bahamite</skos:prefLabel>
	<skos:prefLabel xml:lang="fr">bahamithe</skos:prefLabel>
	<skos:altLabel xml:lang="fr">bahamite</skos:altLabel>
	<skos:broader rdf:resource="https://ark.frantiq.fr/ark:/26678/pcrtc1qqps1k4g"/>
	<skos:inScheme rdf:resource="https://ark.frantiq.fr/ark:/26678/TH_1"/>
	<opentheso:memberOf rdf:resource="https://ark.frantiq.fr/ark:/26678/pcrtv66rn9cbv1"/>
	<opentheso:memberOf rdf:resource="https://ark.frantiq.fr/ark:/26678/pcrtnbDLi2FkAj"/>
	<dcterms:created rdf:datatype="http://www.w3.org/2001/XMLSchema#date">2021-03-12</dcterms:created>
	<dcterms:modified rdf:datatype="http://www.w3.org/2001/XMLSchema#date">2025-01-30</dcterms:modified>
	<dcterms:identifier>266692</dcterms:identifier>
	<dcterms:contributor>blandine.nouvel</dcterms:contributor>
	<dcterms:contributor>justine.vincent</dcterms:contributor>
	<skos:definition xml:lang="fr">Ooïde à cortex, dépourvu de structure concentrique ou radiaire, parfois assimilé aux pseudo-oolithes par l'école française et résultant probablement d'un processus diagénétique syn-sédimentaire. (Fernandes et al., 2021)</skos:definition>
	<skos:definition xml:lang="en">Ooid with cortex, lacking concentric or radial structure, sometimes assimilated to pseudo-oolites by the French school and probably resulting from a syn-sedimentary diagenetic process. (Fernandes et al., 2021)</skos:definition>
	<skos:historyNote xml:lang="fr">2025-30-01 : modification de la définition.</skos:historyNote>
	<dcterms:source>https://doi-org.inshs.bib.cnrs.fr/10.4000/12zm5</dcterms:source>
</rdf:Description>

<rdf:Description rdf:about="https://ark.frantiq.fr/ark:/26678/pcrtq7hgb8vqh2">
	<rdf:type rdf:resource="http://www.w3.org/2004/02/skos/core#Concept"/>
	<skos:prefLabel xml:lang="es">pseudoolito</skos:prefLabel>
	<skos:prefLabel xml:lang="en">pseudo-oolite</skos:prefLabel>
	<skos:prefLabel xml:lang="it">pseudo-oolite</skos:prefLabel>
	<skos:prefLabel xml:lang="de">Pseudo-Oolith</skos:prefLabel>
	<skos:prefLabel xml:lang="fr">pseudo-oolithe</skos:prefLabel>
	<skos:altLabel xml:lang="fr">pseudo-oolite</skos:altLabel>
	<skos:broader rdf:resource="https://ark.frantiq.fr/ark:/26678/pcrtc1qqps1k4g"/>
	<skos:inScheme rdf:resource="https://ark.frantiq.fr/ark:/26678/TH_1"/>
	<opentheso:memberOf rdf:resource="https://ark.frantiq.fr/ark:/26678/pcrtv66rn9cbv1"/>
	<opentheso:memberOf rdf:resource="https://ark.frantiq.fr/ark:/26678/pcrtnbDLi2FkAj"/>
	<dcterms:created rdf:datatype="http://www.w3.org/2001/XMLSchema#date">2021-03-12</dcterms:created>
	<dcterms:modified rdf:datatype="http://www.w3.org/2001/XMLSchema#date">2025-01-30</dcterms:modified>
	<dcterms:identifier>266694</dcterms:identifier>
	<dcterms:contributor>blandine.nouvel</dcterms:contributor>
	<dcterms:contributor>justine.vincent</dcterms:contributor>
	<skos:definition xml:lang="en">Nucleated but indeterminate element with a shape similar to that of ooids (Fernandes et al., 2021).</skos:definition>
	<skos:definition xml:lang="fr">Elément nucléé mais indéterminé, d'une forme proche de celle des ooïdes. (Fernandes et al., 2021)</skos:definition>
	<dcterms:source>https://doi-org.inshs.bib.cnrs.fr/10.4000/12zm5</dcterms:source>
</rdf:Description>

<rdf:Description rdf:about="https://ark.frantiq.fr/ark:/26678/pcrtxrcv4dz28t">
	<rdf:type rdf:resource="http://www.w3.org/2004/02/skos/core#Concept"/>
	<skos:prefLabel xml:lang="de">Aggregat</skos:prefLabel>
	<skos:prefLabel xml:lang="en">aggregate</skos:prefLabel>
	<skos:prefLabel xml:lang="fr">grain composite</skos:prefLabel>
	<skos:prefLabel xml:lang="es">granos compuestos</skos:prefLabel>
	<skos:prefLabel xml:lang="it">granuli compositi</skos:prefLabel>
	<skos:altLabel xml:lang="en">composite grain (geology)</skos:altLabel>
	<skos:broader rdf:resource="https://ark.frantiq.fr/ark:/26678/pcrtc1qqps1k4g"/>
	<skos:inScheme rdf:resource="https://ark.frantiq.fr/ark:/26678/TH_1"/>
	<opentheso:memberOf rdf:resource="https://ark.frantiq.fr/ark:/26678/pcrtv66rn9cbv1"/>
	<opentheso:memberOf rdf:resource="https://ark.frantiq.fr/ark:/26678/pcrtnbDLi2FkAj"/>
	<dcterms:created rdf:datatype="http://www.w3.org/2001/XMLSchema#date">2021-03-12</dcterms:created>
	<dcterms:modified rdf:datatype="http://www.w3.org/2001/XMLSchema#date">2025-01-30</dcterms:modified>
	<dcterms:identifier>266696</dcterms:identifier>
	<dcterms:contributor>blandine.nouvel</dcterms:contributor>
	<dcterms:contributor>justine.vincent</dcterms:contributor>
	<skos:definition xml:lang="en">Multi-nuclear oolite (Fernandes et al., 2021)</skos:definition>
	<skos:definition xml:lang="fr">Oolithe plurinuclée. (Fernandes et al., 2021)</skos:definition>
	<dcterms:source>https://doi-org.inshs.bib.cnrs.fr/10.4000/12zm5</dcterms:source>
</rdf:Description>

<rdf:Description rdf:about="https://ark.frantiq.fr/ark:/26678/pcrtzwhr6nrsvxm73pzkq2dq">
	<rdf:type rdf:resource="http://www.w3.org/2004/02/skos/core#Concept"/>
	<skos:prefLabel xml:lang="en">alabaster</skos:prefLabel>
	<skos:prefLabel xml:lang="de">Alabaster</skos:prefLabel>
	<skos:prefLabel xml:lang="it">alabastro gessoso</skos:prefLabel>
	<skos:prefLabel xml:lang="es">alabastro yesoso</skos:prefLabel>
	<skos:prefLabel xml:lang="fr">albâtre gypseux</skos:prefLabel>
	<skos:altLabel xml:lang="fr">alabastrites</skos:altLabel>
	<skos:altLabel xml:lang="en">gypsym type alabaster</skos:altLabel>
	<skos:related rdf:resource="https://ark.frantiq.fr/ark:/26678/pcrtyJc250eY3m"/>
	<skos:broader rdf:resource="https://ark.frantiq.fr/ark:/26678/pcrtOF9oqZo0Pd"/>
	<skos:inScheme rdf:resource="https://ark.frantiq.fr/ark:/26678/TH_1"/>
	<opentheso:memberOf rdf:resource="https://ark.frantiq.fr/ark:/26678/pcrtv66rn9cbv1"/>
	<opentheso:memberOf rdf:resource="https://ark.frantiq.fr/ark:/26678/pcrtnbDLi2FkAj"/>
	<dcterms:created rdf:datatype="http://www.w3.org/2001/XMLSchema#date">2021-04-01</dcterms:created>
	<dcterms:modified rdf:datatype="http://www.w3.org/2001/XMLSchema#date">2024-11-18</dcterms:modified>
	<dcterms:identifier>266742</dcterms:identifier>
	<dcterms:contributor>blandine.nouvel</dcterms:contributor>
	<dcterms:contributor>justine.vincent</dcterms:contributor>
	<skos:definition xml:lang="en">Mineral produced by the recrystallisation of gypsum (wp)</skos:definition>
	<skos:definition xml:lang="fr">Minéral qui provient de la recristallisation du gypse. (wp)</skos:definition>
</rdf:Description>

<rdf:Description rdf:about="https://ark.frantiq.fr/ark:/26678/pcrtjbpmw8qvrn">
	<rdf:type rdf:resource="http://www.w3.org/2004/02/skos/core#Concept"/>
	<skos:prefLabel xml:lang="en">sediment</skos:prefLabel>
	<skos:prefLabel xml:lang="de">Sediment</skos:prefLabel>
	<skos:prefLabel xml:lang="fr">sédiment</skos:prefLabel>
	<skos:prefLabel xml:lang="es">sedimento</skos:prefLabel>
	<skos:prefLabel xml:lang="it">sedimento</skos:prefLabel>
	<skos:altLabel xml:lang="en">mobile sediment</skos:altLabel>
	<skos:altLabel xml:lang="en">non consolidated detrital sediment</skos:altLabel>
	<skos:altLabel xml:lang="fr">sédiment détritique non consolidé</skos:altLabel>
	<skos:altLabel xml:lang="fr">sédiment meuble</skos:altLabel>
	<skos:altLabel xml:lang="es">sedimento detrítico no consolidado</skos:altLabel>
	<skos:altLabel xml:lang="it">sedimento detritico non consolidato</skos:altLabel>
	<skos:related rdf:resource="https://ark.frantiq.fr/ark:/26678/pcrt4vmcwIU4yP"/>
	<skos:related rdf:resource="https://ark.frantiq.fr/ark:/26678/pcrtj3ZcwkArSR"/>
	<skos:narrower rdf:resource="https://ark.frantiq.fr/ark:/26678/pcrtSIsVZPQG1t"/>
	<skos:narrower rdf:resource="https://ark.frantiq.fr/ark:/26678/pcrtgg4KWVZk74"/>
	<skos:narrower rdf:resource="https://ark.frantiq.fr/ark:/26678/pcrt4Jy2JE8F3U"/>
	<skos:broader rdf:resource="https://ark.frantiq.fr/ark:/26678/pcrtIMsuG0RWTs"/>
	<skos:inScheme rdf:resource="https://ark.frantiq.fr/ark:/26678/TH_1"/>
	<opentheso:memberOf rdf:resource="https://ark.frantiq.fr/ark:/26678/pcrtv66rn9cbv1"/>
	<opentheso:memberOf rdf:resource="https://ark.frantiq.fr/ark:/26678/pcrtnbDLi2FkAj"/>
	<skos:exactMatch rdf:resource="https://www.wikidata.org/wiki/Q180184"/>
	<dcterms:created rdf:datatype="http://www.w3.org/2001/XMLSchema#date">2021-04-21</dcterms:created>
	<dcterms:modified rdf:datatype="http://www.w3.org/2001/XMLSchema#date">2024-11-14</dcterms:modified>
	<dcterms:identifier>266794</dcterms:identifier>
	<dcterms:contributor>blandine.nouvel</dcterms:contributor>
	<dcterms:contributor>justine.vincent</dcterms:contributor>
	<skos:definition xml:lang="en">A collection of particles that were previously suspended in water, the atmosphere or ice and that have finally settled under the effect of gravity, often in successive layers or strata. (Wikipedia)</skos:definition>
	<skos:definition xml:lang="fr">Ensemble de particules antérieurement en suspension dans l'eau, l'atmosphère ou la glace et qui a fini par se déposer sous l'effet de la pesanteur, souvent en couches ou strates successives. (Wikipedia)</skos:definition>
</rdf:Description>

<rdf:Description rdf:about="https://ark.frantiq.fr/ark:/26678/pcrt0712c8ws62">
	<rdf:type rdf:resource="http://www.w3.org/2004/02/skos/core#Concept"/>
	<skos:prefLabel xml:lang="it">arenaria silicizzata</skos:prefLabel>
	<skos:prefLabel xml:lang="es">arenisca silicificada</skos:prefLabel>
	<skos:prefLabel xml:lang="nl">gesilicificeerde zandsteen</skos:prefLabel>
	<skos:prefLabel xml:lang="fr">grès silicifié</skos:prefLabel>
	<skos:prefLabel xml:lang="en">silicified sandstone</skos:prefLabel>
	<skos:prefLabel xml:lang="de">verkieselter Sandstein</skos:prefLabel>
	<skos:related rdf:resource="https://ark.frantiq.fr/ark:/26678/pcrtR1s94Zuaul"/>
	<skos:broader rdf:resource="https://ark.frantiq.fr/ark:/26678/pcrt4N9jrETRto"/>
	<skos:inScheme rdf:resource="https://ark.frantiq.fr/ark:/26678/TH_1"/>
	<opentheso:memberOf rdf:resource="https://ark.frantiq.fr/ark:/26678/pcrtv66rn9cbv1"/>
	<opentheso:memberOf rdf:resource="https://ark.frantiq.fr/ark:/26678/pcrtnbDLi2FkAj"/>
	<dcterms:created rdf:datatype="http://www.w3.org/2001/XMLSchema#date">2021-07-12</dcterms:created>
	<dcterms:modified rdf:datatype="http://www.w3.org/2001/XMLSchema#date">2023-08-02</dcterms:modified>
	<dcterms:identifier>266930</dcterms:identifier>
	<dcterms:contributor>blandine.nouvel</dcterms:contributor>
</rdf:Description>

<rdf:Description rdf:about="https://ark.frantiq.fr/ark:/26678/pcrtxn3nfsg0pd">
	<rdf:type rdf:resource="http://www.w3.org/2004/02/skos/core#Concept"/>
	<skos:prefLabel xml:lang="fr">calcaire silicifié</skos:prefLabel>
	<skos:prefLabel xml:lang="it">calcare silicizzato</skos:prefLabel>
	<skos:prefLabel xml:lang="es">caliza silicificada</skos:prefLabel>
	<skos:prefLabel xml:lang="nl">silicaatkalksteen</skos:prefLabel>
	<skos:prefLabel xml:lang="en">silicified limestone</skos:prefLabel>
	<skos:prefLabel xml:lang="de">verkieselter Kalkstein</skos:prefLabel>
	<skos:altLabel xml:lang="fr">calcaire siliceux</skos:altLabel>
	<skos:broader rdf:resource="https://ark.frantiq.fr/ark:/26678/pcrtc1Ueky7Zpg"/>
	<skos:inScheme rdf:resource="https://ark.frantiq.fr/ark:/26678/TH_1"/>
	<opentheso:memberOf rdf:resource="https://ark.frantiq.fr/ark:/26678/pcrtv66rn9cbv1"/>
	<opentheso:memberOf rdf:resource="https://ark.frantiq.fr/ark:/26678/pcrtnbDLi2FkAj"/>
	<dcterms:created rdf:datatype="http://www.w3.org/2001/XMLSchema#date">2021-07-12</dcterms:created>
	<dcterms:modified rdf:datatype="http://www.w3.org/2001/XMLSchema#date">2023-08-02</dcterms:modified>
	<dcterms:identifier>266932</dcterms:identifier>
	<dcterms:contributor>blandine.nouvel</dcterms:contributor>
	<skos:definition xml:lang="fr">Calcaire partiellement imprégné ou remplacé par une ou plusieurs phases silicieuses et contenant de 10 à 50% de silice (Fernandes, 2012)</skos:definition>
</rdf:Description>

<rdf:Description rdf:about="https://ark.frantiq.fr/ark:/26678/pcrt11zbr3964m">
	<rdf:type rdf:resource="http://www.w3.org/2004/02/skos/core#Concept"/>
	<skos:prefLabel xml:lang="es">cinerita silicificada</skos:prefLabel>
	<skos:prefLabel xml:lang="fr">cinérite silicifiée</skos:prefLabel>
	<skos:prefLabel xml:lang="it">cinerite silicizzata</skos:prefLabel>
	<skos:prefLabel xml:lang="nl">gesilicifieerde cineriet</skos:prefLabel>
	<skos:prefLabel xml:lang="en">silicified cinerite</skos:prefLabel>
	<skos:prefLabel xml:lang="de">verkieselter Cinerit</skos:prefLabel>
	<skos:broader rdf:resource="https://ark.frantiq.fr/ark:/26678/pcrt4N9jrETRto"/>
	<skos:inScheme rdf:resource="https://ark.frantiq.fr/ark:/26678/TH_1"/>
	<opentheso:memberOf rdf:resource="https://ark.frantiq.fr/ark:/26678/pcrtv66rn9cbv1"/>
	<opentheso:memberOf rdf:resource="https://ark.frantiq.fr/ark:/26678/pcrtnbDLi2FkAj"/>
	<dcterms:created rdf:datatype="http://www.w3.org/2001/XMLSchema#date">2021-07-12</dcterms:created>
	<dcterms:modified rdf:datatype="http://www.w3.org/2001/XMLSchema#date">2025-01-30</dcterms:modified>
	<dcterms:identifier>266934</dcterms:identifier>
	<dcterms:contributor>blandine.nouvel</dcterms:contributor>
	<dcterms:contributor>justine.vincent</dcterms:contributor>
	<skos:definition xml:lang="en">Volcanic ash consolidated by silica and more or less compact (Fernandes, 2012).</skos:definition>
	<skos:definition xml:lang="fr">Cendres volcaniques consolidées par de la silice et plus ou moins compactes (Fernandes, 2012).</skos:definition>
	<dcterms:source>https://doi-org.inshs.bib.cnrs.fr/10.4000/12zm5</dcterms:source>
</rdf:Description>

<rdf:Description rdf:about="https://ark.frantiq.fr/ark:/26678/pcrtb8qzpwp7ck">
	<rdf:type rdf:resource="http://www.w3.org/2004/02/skos/core#Concept"/>
	<skos:prefLabel xml:lang="en">black jasper</skos:prefLabel>
	<skos:prefLabel xml:lang="es">lidita</skos:prefLabel>
	<skos:prefLabel xml:lang="it">lidite</skos:prefLabel>
	<skos:prefLabel xml:lang="fr">lydienne</skos:prefLabel>
	<skos:prefLabel xml:lang="de">schwarzer Jasper</skos:prefLabel>
	<skos:altLabel xml:lang="it">lydite</skos:altLabel>
	<skos:altLabel xml:lang="it">pietra lidia</skos:altLabel>
	<skos:broader rdf:resource="https://ark.frantiq.fr/ark:/26678/pcrt3PUAhlWubZ"/>
	<skos:inScheme rdf:resource="https://ark.frantiq.fr/ark:/26678/TH_1"/>
	<opentheso:memberOf rdf:resource="https://ark.frantiq.fr/ark:/26678/pcrtv66rn9cbv1"/>
	<opentheso:memberOf rdf:resource="https://ark.frantiq.fr/ark:/26678/pcrtnbDLi2FkAj"/>
	<skos:narrowMatch rdf:resource="https://www.wikidata.org/wiki/Q201175"/>
	<dcterms:created rdf:datatype="http://www.w3.org/2001/XMLSchema#date">2021-07-12</dcterms:created>
	<dcterms:modified rdf:datatype="http://www.w3.org/2001/XMLSchema#date">2025-01-30</dcterms:modified>
	<dcterms:identifier>266936</dcterms:identifier>
	<dcterms:contributor>blandine.nouvel</dcterms:contributor>
	<dcterms:contributor>justine.vincent</dcterms:contributor>
	<skos:definition xml:lang="en">Siliceous sedimentary rock with grey or black radiolarians and a calcareous matrix, known mainly from Carboniferous series (Fernandes, 2012).</skos:definition>
	<skos:definition xml:lang="fr">Roche sédimentaire silicieuse à radiolaires de couleur grise ou noire, à matrice calcédonieuse, surtout connue dans les séries carbonifères (Fernandes, 2012).</skos:definition>
	<dcterms:source>https://doi-org.inshs.bib.cnrs.fr/10.4000/12zm5</dcterms:source>
</rdf:Description>

<rdf:Description rdf:about="https://ark.frantiq.fr/ark:/26678/pcrtspv238x81q">
	<rdf:type rdf:resource="http://www.w3.org/2004/02/skos/core#Concept"/>
	<skos:prefLabel xml:lang="es">ftanita</skos:prefLabel>
	<skos:prefLabel xml:lang="it">ftanite</skos:prefLabel>
	<skos:prefLabel xml:lang="nl">phtaniet</skos:prefLabel>
	<skos:prefLabel xml:lang="en">phtanit</skos:prefLabel>
	<skos:prefLabel xml:lang="fr">phtanite</skos:prefLabel>
	<skos:prefLabel xml:lang="de">Phthanit</skos:prefLabel>
	<skos:broader rdf:resource="https://ark.frantiq.fr/ark:/26678/pcrt3PUAhlWubZ"/>
	<skos:inScheme rdf:resource="https://ark.frantiq.fr/ark:/26678/TH_1"/>
	<opentheso:memberOf rdf:resource="https://ark.frantiq.fr/ark:/26678/pcrtv66rn9cbv1"/>
	<opentheso:memberOf rdf:resource="https://ark.frantiq.fr/ark:/26678/pcrtnbDLi2FkAj"/>
	<dcterms:created rdf:datatype="http://www.w3.org/2001/XMLSchema#date">2021-07-12</dcterms:created>
	<dcterms:modified rdf:datatype="http://www.w3.org/2001/XMLSchema#date">2025-01-30</dcterms:modified>
	<dcterms:identifier>266938</dcterms:identifier>
	<dcterms:contributor>blandine.nouvel</dcterms:contributor>
	<dcterms:contributor>justine.vincent</dcterms:contributor>
	<skos:definition xml:lang="fr">Roche sédimentaire silicieuse de petite taille (inférieurs à 20 microns), cryptocristalline du carbonifère (Fernandes, 2012).</skos:definition>
	<skos:historyNote xml:lang="fr">2025-30-01 : modifcation de la définition.</skos:historyNote>
	<dcterms:source>https://doi-org.inshs.bib.cnrs.fr/10.4000/12zm5</dcterms:source>
</rdf:Description>

<rdf:Description rdf:about="https://ark.frantiq.fr/ark:/26678/pcrtt42zqnhf10">
	<rdf:type rdf:resource="http://www.w3.org/2004/02/skos/core#Concept"/>
	<skos:prefLabel xml:lang="en">jasperoid</skos:prefLabel>
	<skos:prefLabel xml:lang="it">jasperoid</skos:prefLabel>
	<skos:prefLabel xml:lang="de">Jasperoid</skos:prefLabel>
	<skos:prefLabel xml:lang="es">jasperoide</skos:prefLabel>
	<skos:prefLabel xml:lang="fr">jaspéroïde</skos:prefLabel>
	<skos:broader rdf:resource="https://ark.frantiq.fr/ark:/26678/pcrt4N9jrETRto"/>
	<skos:inScheme rdf:resource="https://ark.frantiq.fr/ark:/26678/TH_1"/>
	<opentheso:memberOf rdf:resource="https://ark.frantiq.fr/ark:/26678/pcrtv66rn9cbv1"/>
	<opentheso:memberOf rdf:resource="https://ark.frantiq.fr/ark:/26678/pcrtnbDLi2FkAj"/>
	<skos:exactMatch rdf:resource="https://www.wikidata.org/wiki/Q2201550"/>
	<dcterms:created rdf:datatype="http://www.w3.org/2001/XMLSchema#date">2021-07-12</dcterms:created>
	<dcterms:modified rdf:datatype="http://www.w3.org/2001/XMLSchema#date">2025-01-30</dcterms:modified>
	<dcterms:identifier>266940</dcterms:identifier>
	<dcterms:contributor>blandine.nouvel</dcterms:contributor>
	<dcterms:contributor>justine.vincent</dcterms:contributor>
	<skos:definition xml:lang="en">Rock formed by metasomatism under the influence of hydrothermal circulation near hot magmatic intrusions in the Earth's crust. (Fernandes, 2012).</skos:definition>
	<skos:definition xml:lang="fr">Roche formée par métasomatisme sous l'influence de la circulation hydrothermale près des intrusions magmatiques chaudes dans la croûte terrestre. (Fernandes, 2012).</skos:definition>
	<skos:scopeNote xml:lang="en">Not to be confused with jaspoids.</skos:scopeNote>
	<skos:scopeNote xml:lang="fr">Ne pas confondre avec les jaspoïdes.</skos:scopeNote>
	<skos:historyNote xml:lang="fr">2025-30-01 : modification de la définition.</skos:historyNote>
	<dcterms:source>https://doi-org.inshs.bib.cnrs.fr/10.4000/12zm5</dcterms:source>
</rdf:Description>

<rdf:Description rdf:about="https://ark.frantiq.fr/ark:/26678/pcrtx37ph91cww">
	<rdf:type rdf:resource="http://www.w3.org/2004/02/skos/core#Concept"/>
	<skos:prefLabel xml:lang="en">natural material</skos:prefLabel>
	<skos:prefLabel xml:lang="it">sostanza naturale</skos:prefLabel>
	<skos:prefLabel xml:lang="nl">stof</skos:prefLabel>
	<skos:prefLabel xml:lang="fr">substance naturelle (matière)</skos:prefLabel>
	<skos:prefLabel xml:lang="de">Substanz</skos:prefLabel>
	<skos:prefLabel xml:lang="es">sustancia natural</skos:prefLabel>
	<skos:altLabel xml:lang="es">materia natural</skos:altLabel>
	<skos:altLabel xml:lang="it">materia naturale</skos:altLabel>
	<skos:altLabel xml:lang="fr">matière naturelle</skos:altLabel>
	<skos:altLabel xml:lang="en">natural substance</skos:altLabel>
	<skos:related rdf:resource="https://ark.frantiq.fr/ark:/26678/pcrtwvFLgSQRs5"/>
	<skos:narrower rdf:resource="https://ark.frantiq.fr/ark:/26678/pcrtnsH1xdYgZe"/>
	<skos:narrower rdf:resource="https://ark.frantiq.fr/ark:/26678/pcrtJYawSTtElG"/>
	<skos:narrower rdf:resource="https://ark.frantiq.fr/ark:/26678/pcrttvE2YZwZu6"/>
	<skos:narrower rdf:resource="https://ark.frantiq.fr/ark:/26678/crtnOhKKcaFEI"/>
	<skos:broader rdf:resource="https://ark.frantiq.fr/ark:/26678/pcrtIMsuG0RWTs"/>
	<skos:inScheme rdf:resource="https://ark.frantiq.fr/ark:/26678/TH_1"/>
	<opentheso:memberOf rdf:resource="https://ark.frantiq.fr/ark:/26678/pcrtv66rn9cbv1"/>
	<opentheso:memberOf rdf:resource="https://ark.frantiq.fr/ark:/26678/pcrtnbDLi2FkAj"/>
	<dcterms:created rdf:datatype="http://www.w3.org/2001/XMLSchema#date">2021-07-12</dcterms:created>
	<dcterms:modified rdf:datatype="http://www.w3.org/2001/XMLSchema#date">2024-10-18</dcterms:modified>
	<dcterms:identifier>266942</dcterms:identifier>
	<dcterms:contributor>blandine.nouvel</dcterms:contributor>
	<dcterms:contributor>justine.vincent</dcterms:contributor>
	<skos:definition xml:lang="fr">&lt;span style= color: rgb(4, 12, 40); &gt;Toute substance trouvée dans la nature.&lt;/span&gt;</skos:definition>
	<skos:definition xml:lang="en">Any substance found in nature.</skos:definition>
</rdf:Description>

<rdf:Description rdf:about="https://ark.frantiq.fr/ark:/26678/pcrtszp2f0j63w">
	<rdf:type rdf:resource="http://www.w3.org/2004/02/skos/core#Concept"/>
	<skos:prefLabel xml:lang="es">silcreta</skos:prefLabel>
	<skos:prefLabel xml:lang="en">silcrete</skos:prefLabel>
	<skos:prefLabel xml:lang="it">silcrete</skos:prefLabel>
	<skos:prefLabel xml:lang="de">Silcrete</skos:prefLabel>
	<skos:prefLabel xml:lang="fr">silcrète</skos:prefLabel>
	<skos:narrower rdf:resource="https://ark.frantiq.fr/ark:/26678/pcrtdpxq48r9pj"/>
	<skos:narrower rdf:resource="https://ark.frantiq.fr/ark:/26678/pcrt9bvd56q20k"/>
	<skos:broader rdf:resource="https://ark.frantiq.fr/ark:/26678/pcrt4N9jrETRto"/>
	<skos:inScheme rdf:resource="https://ark.frantiq.fr/ark:/26678/TH_1"/>
	<opentheso:memberOf rdf:resource="https://ark.frantiq.fr/ark:/26678/pcrtv66rn9cbv1"/>
	<opentheso:memberOf rdf:resource="https://ark.frantiq.fr/ark:/26678/pcrtnbDLi2FkAj"/>
	<skos:exactMatch rdf:resource="https://www.wikidata.org/wiki/Q1422939"/>
	<dcterms:created rdf:datatype="http://www.w3.org/2001/XMLSchema#date">2021-07-12</dcterms:created>
	<dcterms:modified rdf:datatype="http://www.w3.org/2001/XMLSchema#date">2023-08-02</dcterms:modified>
	<dcterms:identifier>266944</dcterms:identifier>
	<dcterms:contributor>blandine.nouvel</dcterms:contributor>
	<skos:definition xml:lang="fr">&lt;p&gt;Roche siliceuse issue de formations continentales superficielles ou sub-superficielles. Son origine fait suite à un apport hydrique vadose de silice et à sa précipitation dans un sol (silcrète pédogénétique) ou dans une formation située dans la zone phréatique (silcrète phréatique). (Fernandes, 2012).&lt;/p&gt;</skos:definition>
</rdf:Description>

<rdf:Description rdf:about="https://ark.frantiq.fr/ark:/26678/pcrtdpxq48r9pj">
	<rdf:type rdf:resource="http://www.w3.org/2004/02/skos/core#Concept"/>
	<skos:prefLabel xml:lang="de">Evaporit</skos:prefLabel>
	<skos:prefLabel xml:lang="es">evaporita</skos:prefLabel>
	<skos:prefLabel xml:lang="en">evaporite</skos:prefLabel>
	<skos:prefLabel xml:lang="it">evaporite</skos:prefLabel>
	<skos:prefLabel xml:lang="fr">évaporite</skos:prefLabel>
	<skos:broader rdf:resource="https://ark.frantiq.fr/ark:/26678/pcrtszp2f0j63w"/>
	<skos:inScheme rdf:resource="https://ark.frantiq.fr/ark:/26678/TH_1"/>
	<opentheso:memberOf rdf:resource="https://ark.frantiq.fr/ark:/26678/pcrtv66rn9cbv1"/>
	<opentheso:memberOf rdf:resource="https://ark.frantiq.fr/ark:/26678/pcrtnbDLi2FkAj"/>
	<skos:exactMatch rdf:resource="https://www.wikidata.org/wiki/Q491689"/>
	<dcterms:created rdf:datatype="http://www.w3.org/2001/XMLSchema#date">2021-07-12</dcterms:created>
	<dcterms:modified rdf:datatype="http://www.w3.org/2001/XMLSchema#date">2023-08-02</dcterms:modified>
	<dcterms:identifier>266946</dcterms:identifier>
	<dcterms:contributor>blandine.nouvel</dcterms:contributor>
	<skos:definition xml:lang="fr">Roche sédimentaire issue de la précipitation chimique par évaporation de substances dissoutes dans des solutions. Elle se forme dans des milieux confinés : dans des bassins sédimentaires fermés à la suite d'une régression marine, dans des dépressions côtières (lagunes, chotts,...) ou dans des bassins endoréiques (lacs salins, sebkraa,...). Les chlorures, les sulfates, les carbonates hydratés alcalins et les borates en sont les principales famille minérales (Fernandes 2012).</skos:definition>
</rdf:Description>

<rdf:Description rdf:about="https://ark.frantiq.fr/ark:/26678/pcrt9bvd56q20k">
	<rdf:type rdf:resource="http://www.w3.org/2004/02/skos/core#Concept"/>
	<skos:prefLabel xml:lang="en">gritstone</skos:prefLabel>
	<skos:prefLabel xml:lang="it">macina (roccia)</skos:prefLabel>
	<skos:prefLabel xml:lang="fr">meulière</skos:prefLabel>
	<skos:prefLabel xml:lang="nl">molensteen</skos:prefLabel>
	<skos:prefLabel xml:lang="de">Mühlstein</skos:prefLabel>
	<skos:prefLabel xml:lang="es">piedra molar (roca)</skos:prefLabel>
	<skos:altLabel xml:lang="en">grindstone</skos:altLabel>
	<skos:altLabel xml:lang="en">grit</skos:altLabel>
	<skos:altLabel xml:lang="en">millstone</skos:altLabel>
	<skos:altLabel xml:lang="fr">pierre de meulière</skos:altLabel>
	<skos:altLabel xml:lang="it">pietra molare</skos:altLabel>
	<skos:broader rdf:resource="https://ark.frantiq.fr/ark:/26678/pcrtszp2f0j63w"/>
	<skos:inScheme rdf:resource="https://ark.frantiq.fr/ark:/26678/TH_1"/>
	<opentheso:memberOf rdf:resource="https://ark.frantiq.fr/ark:/26678/pcrtv66rn9cbv1"/>
	<opentheso:memberOf rdf:resource="https://ark.frantiq.fr/ark:/26678/pcrtnbDLi2FkAj"/>
	<skos:exactMatch rdf:resource="https://www.wikidata.org/wiki/Q1048392"/>
	<dcterms:created rdf:datatype="http://www.w3.org/2001/XMLSchema#date">2021-07-12</dcterms:created>
	<dcterms:modified rdf:datatype="http://www.w3.org/2001/XMLSchema#date">2023-08-02</dcterms:modified>
	<dcterms:identifier>266948</dcterms:identifier>
	<dcterms:contributor>blandine.nouvel</dcterms:contributor>
	<skos:definition xml:lang="fr">Roche silicseuse en masse irrégulière, arrondie ou anguleuse, massive,, homogène ou alvéolaire. Constituée de calcédonite, de quartz et plus rarement d'opale. Il est possible d'y observer des fossiles d'environnement palustre à lacustre (gastéropodes, algues, végétaux,...). Ce type d'accident siliceux est commun dans les milieux oligocènes du Bassin parisien (Fernandes, 2012).</skos:definition>
</rdf:Description>

<rdf:Description rdf:about="https://ark.frantiq.fr/ark:/26678/pcrtcxvd08cn0d">
	<rdf:type rdf:resource="http://www.w3.org/2004/02/skos/core#Concept"/>
	<skos:prefLabel xml:lang="de">hydrothermales Kieselgestein</skos:prefLabel>
	<skos:prefLabel xml:lang="en">hydrothermal siliceous rock</skos:prefLabel>
	<skos:prefLabel xml:lang="es">sílice hidrotermal</skos:prefLabel>
	<skos:prefLabel xml:lang="fr">silice hydrothermale</skos:prefLabel>
	<skos:prefLabel xml:lang="it">silice idrotermale</skos:prefLabel>
	<skos:altLabel xml:lang="en">hydrothermal chert</skos:altLabel>
	<skos:narrower rdf:resource="https://ark.frantiq.fr/ark:/26678/pcrtm3j41zv11k"/>
	<skos:broader rdf:resource="https://ark.frantiq.fr/ark:/26678/pcrt4N9jrETRto"/>
	<skos:inScheme rdf:resource="https://ark.frantiq.fr/ark:/26678/TH_1"/>
	<opentheso:memberOf rdf:resource="https://ark.frantiq.fr/ark:/26678/pcrtv66rn9cbv1"/>
	<opentheso:memberOf rdf:resource="https://ark.frantiq.fr/ark:/26678/pcrtnbDLi2FkAj"/>
	<dcterms:created rdf:datatype="http://www.w3.org/2001/XMLSchema#date">2021-07-12</dcterms:created>
	<dcterms:modified rdf:datatype="http://www.w3.org/2001/XMLSchema#date">2023-08-02</dcterms:modified>
	<dcterms:identifier>266950</dcterms:identifier>
	<dcterms:contributor>blandine.nouvel</dcterms:contributor>
	<skos:definition xml:lang="fr">Type de dépôt siliceux résultant de phénomènes hydrothermiques qui se produisent généralement à la faveur des grands accidents tectoniques qui bordent les bassins sédimentaires. La diagenèse de ces roches est dictée par la géométrie, la chimie et la porosité de la roche mère (GDR Silex, 2021).</skos:definition>
</rdf:Description>

<rdf:Description rdf:about="https://ark.frantiq.fr/ark:/26678/pcrtm3j41zv11k">
	<rdf:type rdf:resource="http://www.w3.org/2004/02/skos/core#Concept"/>
	<skos:prefLabel xml:lang="es">geiserita</skos:prefLabel>
	<skos:prefLabel xml:lang="it">geyserite</skos:prefLabel>
	<skos:prefLabel xml:lang="de">Kieselsinter</skos:prefLabel>
	<skos:prefLabel xml:lang="en">siliceous sinter</skos:prefLabel>
	<skos:prefLabel xml:lang="fr">sinter</skos:prefLabel>
	<skos:altLabel xml:lang="de">Geyserit</skos:altLabel>
	<skos:altLabel xml:lang="en">geyserite</skos:altLabel>
	<skos:altLabel xml:lang="fr">geysérite</skos:altLabel>
	<skos:altLabel xml:lang="it">precipitato siliceo</skos:altLabel>
	<skos:broader rdf:resource="https://ark.frantiq.fr/ark:/26678/pcrtcxvd08cn0d"/>
	<skos:inScheme rdf:resource="https://ark.frantiq.fr/ark:/26678/TH_1"/>
	<opentheso:memberOf rdf:resource="https://ark.frantiq.fr/ark:/26678/pcrtv66rn9cbv1"/>
	<opentheso:memberOf rdf:resource="https://ark.frantiq.fr/ark:/26678/pcrtnbDLi2FkAj"/>
	<skos:exactMatch rdf:resource="https://www.wikidata.org/wiki/Q1976078"/>
	<dcterms:created rdf:datatype="http://www.w3.org/2001/XMLSchema#date">2021-07-12</dcterms:created>
	<dcterms:modified rdf:datatype="http://www.w3.org/2001/XMLSchema#date">2023-08-02</dcterms:modified>
	<dcterms:identifier>266952</dcterms:identifier>
	<dcterms:contributor>blandine.nouvel</dcterms:contributor>
	<skos:definition xml:lang="fr">Roche résultant de l'arrivée en surface des fluides hydrothermaux (geysers). La précipitation rapide de ces fluides siliceux à haute température entraîne le dépôt de roches généralement peu structurées, opalescentes (opale A) et accompagnées d'un peu d'alumine (Fernandes, 2012).</skos:definition>
</rdf:Description>

<rdf:Description rdf:about="https://ark.frantiq.fr/ark:/26678/pcrtf80pqj28pw">
	<rdf:type rdf:resource="http://www.w3.org/2004/02/skos/core#Concept"/>
	<skos:prefLabel xml:lang="de">Eisenoxid</skos:prefLabel>
	<skos:prefLabel xml:lang="nl">ijzeroxide</skos:prefLabel>
	<skos:prefLabel xml:lang="en">iron oxide</skos:prefLabel>
	<skos:prefLabel xml:lang="it">ossido di ferro</skos:prefLabel>
	<skos:prefLabel xml:lang="es">óxido de hierro</skos:prefLabel>
	<skos:prefLabel xml:lang="fr">oxyde de fer</skos:prefLabel>
	<skos:related rdf:resource="https://ark.frantiq.fr/ark:/26678/pcrtuFMPNUEKWb"/>
	<skos:broader rdf:resource="https://ark.frantiq.fr/ark:/26678/pcrtGzQPnntJa1"/>
	<skos:inScheme rdf:resource="https://ark.frantiq.fr/ark:/26678/TH_1"/>
	<opentheso:memberOf rdf:resource="https://ark.frantiq.fr/ark:/26678/pcrtv66rn9cbv1"/>
	<opentheso:memberOf rdf:resource="https://ark.frantiq.fr/ark:/26678/pcrtnbDLi2FkAj"/>
	<skos:exactMatch rdf:resource="https://www.wikidata.org/wiki/Q721849"/>
	<dcterms:created rdf:datatype="http://www.w3.org/2001/XMLSchema#date">2021-07-23</dcterms:created>
	<dcterms:modified rdf:datatype="http://www.w3.org/2001/XMLSchema#date">2023-08-02</dcterms:modified>
	<dcterms:identifier>266956</dcterms:identifier>
	<dcterms:contributor>blandine.nouvel</dcterms:contributor>
	<skos:definition xml:lang="en">Mineral that impregnates the porosity of flint (Fernandes, 2012).</skos:definition>
	<skos:definition xml:lang="fr">Minéral pigmentant en imprégnation la porosité des silex (Fernandes, 2012).</skos:definition>
</rdf:Description>

<rdf:Description rdf:about="https://ark.frantiq.fr/ark:/26678/pcrt38v8df6d4c">
	<rdf:type rdf:resource="http://www.w3.org/2004/02/skos/core#Concept"/>
	<skos:prefLabel xml:lang="es">pirita</skos:prefLabel>
	<skos:prefLabel xml:lang="it">pirita</skos:prefLabel>
	<skos:prefLabel xml:lang="nl">pyriet</skos:prefLabel>
	<skos:prefLabel xml:lang="de">Pyrit</skos:prefLabel>
	<skos:prefLabel xml:lang="en">pyrite</skos:prefLabel>
	<skos:prefLabel xml:lang="fr">pyrite</skos:prefLabel>
	<skos:altLabel xml:lang="en">iron pyrite</skos:altLabel>
	<skos:broader rdf:resource="https://ark.frantiq.fr/ark:/26678/pcrty2mcsksa6s"/>
	<skos:inScheme rdf:resource="https://ark.frantiq.fr/ark:/26678/TH_1"/>
	<opentheso:memberOf rdf:resource="https://ark.frantiq.fr/ark:/26678/pcrtv66rn9cbv1"/>
	<opentheso:memberOf rdf:resource="https://ark.frantiq.fr/ark:/26678/pcrtnbDLi2FkAj"/>
	<skos:exactMatch rdf:resource="https://www.wikidata.org/wiki/Q50769"/>
	<dcterms:created rdf:datatype="http://www.w3.org/2001/XMLSchema#date">2021-07-23</dcterms:created>
	<dcterms:modified rdf:datatype="http://www.w3.org/2001/XMLSchema#date">2023-08-02</dcterms:modified>
	<dcterms:identifier>266960</dcterms:identifier>
	<dcterms:contributor>blandine.nouvel</dcterms:contributor>
	<skos:definition xml:lang="en">Iron sulphide (Fe Se), which often occurs in cubes or concretions in black flints from a reducing environment (Fernandes, 2012).</skos:definition>
	<skos:definition xml:lang="fr">Sulfure de fer (Fe Se) qui se présente souvent en cubes ou en concrétions dans les silex de teinte noire et issu d’un environnement réducteur (Fernandes, 2012).</skos:definition>
</rdf:Description>

<rdf:Description rdf:about="https://ark.frantiq.fr/ark:/26678/pcrtv4jtvchmgm">
	<rdf:type rdf:resource="http://www.w3.org/2004/02/skos/core#Concept"/>
	<skos:prefLabel xml:lang="nl">glauconiet</skos:prefLabel>
	<skos:prefLabel xml:lang="es">glauconita</skos:prefLabel>
	<skos:prefLabel xml:lang="en">glauconite</skos:prefLabel>
	<skos:prefLabel xml:lang="fr">glauconite</skos:prefLabel>
	<skos:prefLabel xml:lang="it">glauconite</skos:prefLabel>
	<skos:prefLabel xml:lang="de">Glaukonit</skos:prefLabel>
	<skos:broader rdf:resource="https://ark.frantiq.fr/ark:/26678/pcrty2mcsksa6s"/>
	<skos:inScheme rdf:resource="https://ark.frantiq.fr/ark:/26678/TH_1"/>
	<opentheso:memberOf rdf:resource="https://ark.frantiq.fr/ark:/26678/pcrtv66rn9cbv1"/>
	<opentheso:memberOf rdf:resource="https://ark.frantiq.fr/ark:/26678/pcrtnbDLi2FkAj"/>
	<skos:exactMatch rdf:resource="https://www.wikidata.org/wiki/Q423034"/>
	<dcterms:created rdf:datatype="http://www.w3.org/2001/XMLSchema#date">2021-07-23</dcterms:created>
	<dcterms:modified rdf:datatype="http://www.w3.org/2001/XMLSchema#date">2024-11-18</dcterms:modified>
	<dcterms:identifier>266962</dcterms:identifier>
	<dcterms:contributor>blandine.nouvel</dcterms:contributor>
	<dcterms:contributor>justine.vincent</dcterms:contributor>
	<skos:note xml:lang="en">Green mineral from the silicate group, making up glauconite, found in sedimentary rocks accumulated in the sea (sands, gaizes, clays, carbonate rocks, phosphorites).</skos:note>
	<skos:note xml:lang="fr">Minéral vert du groupe des silicates, composant la glauconie répandu dans les roches sédimentaires accumulées dans la mer (sables, gaizes, argiles, roches carbonatées, phosphorites).</skos:note>
	<skos:historyNote xml:lang="fr">2024-18-11 : modification de la définition.</skos:historyNote>
</rdf:Description>

<rdf:Description rdf:about="https://ark.frantiq.fr/ark:/26678/pcrtqnzx9qwkt5">
	<rdf:type rdf:resource="http://www.w3.org/2004/02/skos/core#Concept"/>
	<skos:prefLabel xml:lang="nl">carbonaat</skos:prefLabel>
	<skos:prefLabel xml:lang="en">carbonate</skos:prefLabel>
	<skos:prefLabel xml:lang="fr">carbonate</skos:prefLabel>
	<skos:prefLabel xml:lang="es">carbonato</skos:prefLabel>
	<skos:prefLabel xml:lang="it">carbonato</skos:prefLabel>
	<skos:prefLabel xml:lang="de">Karbonat</skos:prefLabel>
	<skos:narrower rdf:resource="https://ark.frantiq.fr/ark:/26678/pcrtRT5qpNmDqE"/>
	<skos:narrower rdf:resource="https://ark.frantiq.fr/ark:/26678/pcrtk5md9510q7"/>
	<skos:narrower rdf:resource="https://ark.frantiq.fr/ark:/26678/pcrtgb1xs84qs8"/>
	<skos:broader rdf:resource="https://ark.frantiq.fr/ark:/26678/pcrty2mcsksa6s"/>
	<skos:inScheme rdf:resource="https://ark.frantiq.fr/ark:/26678/TH_1"/>
	<opentheso:memberOf rdf:resource="https://ark.frantiq.fr/ark:/26678/pcrtv66rn9cbv1"/>
	<opentheso:memberOf rdf:resource="https://ark.frantiq.fr/ark:/26678/pcrtnbDLi2FkAj"/>
	<skos:exactMatch rdf:resource="https://www.wikidata.org/wiki/Q181699"/>
	<dcterms:created rdf:datatype="http://www.w3.org/2001/XMLSchema#date">2021-07-23</dcterms:created>
	<dcterms:modified rdf:datatype="http://www.w3.org/2001/XMLSchema#date">2023-08-02</dcterms:modified>
	<dcterms:identifier>266964</dcterms:identifier>
	<dcterms:contributor>blandine.nouvel</dcterms:contributor>
	<skos:definition xml:lang="en">A family of minerals, generally rhombohedral or orthorhombic, characterised by the ion (CO3)²; two of them are more or less common in flint: calcite and dolomite (Fernandes, 2012).</skos:definition>
	<skos:definition xml:lang="fr">Famille de minéraux, généralement rhomboédriques ou orthorhombiques, caractérisés par l’ion (CO3)²  ; deux d’entre eux sont plus ou moins fréquents dans les silex : la calcite et la dolomite (Fernandes, 2012)</skos:definition>
</rdf:Description>

<rdf:Description rdf:about="https://ark.frantiq.fr/ark:/26678/pcrtk5md9510q7">
	<rdf:type rdf:resource="http://www.w3.org/2004/02/skos/core#Concept"/>
	<skos:prefLabel xml:lang="nl">dolomiet</skos:prefLabel>
	<skos:prefLabel xml:lang="de">Dolomit</skos:prefLabel>
	<skos:prefLabel xml:lang="es">dolomita</skos:prefLabel>
	<skos:prefLabel xml:lang="en">dolomite</skos:prefLabel>
	<skos:prefLabel xml:lang="fr">dolomite</skos:prefLabel>
	<skos:prefLabel xml:lang="it">dolomite</skos:prefLabel>
	<skos:related rdf:resource="https://ark.frantiq.fr/ark:/26678/pcrtbxntxs7hfz99qvswk8k1"/>
	<skos:broader rdf:resource="https://ark.frantiq.fr/ark:/26678/pcrtqnzx9qwkt5"/>
	<skos:inScheme rdf:resource="https://ark.frantiq.fr/ark:/26678/TH_1"/>
	<opentheso:memberOf rdf:resource="https://ark.frantiq.fr/ark:/26678/pcrtv66rn9cbv1"/>
	<opentheso:memberOf rdf:resource="https://ark.frantiq.fr/ark:/26678/pcrtnbDLi2FkAj"/>
	<skos:exactMatch rdf:resource="https://www.wikidata.org/wiki/Q1134814"/>
	<dcterms:created rdf:datatype="http://www.w3.org/2001/XMLSchema#date">2021-07-23</dcterms:created>
	<dcterms:modified rdf:datatype="http://www.w3.org/2001/XMLSchema#date">2024-11-18</dcterms:modified>
	<dcterms:identifier>266966</dcterms:identifier>
	<dcterms:contributor>blandine.nouvel</dcterms:contributor>
	<dcterms:contributor>justine.vincent</dcterms:contributor>
	<skos:definition xml:lang="en">A mineral (anhydrous double carbonate of calcium and magnesium) with a rhombohedral habitus, it is the main phase in dolomites. In flint, it is a significant accessory phase of its protolith (Fernandes, 2012).</skos:definition>
	<skos:definition xml:lang="fr">Minéral (Carbonate double anhydre de calcium et magnésium) d'habitus rhomboédrique, il est la phase principale des dolomies. Dans le silex, il s'agit d'une phase accessoire significative de son protolithe. (Fernandes, 2012)</skos:definition>
</rdf:Description>

<rdf:Description rdf:about="https://ark.frantiq.fr/ark:/26678/pcrtgb1xs84qs8">
	<rdf:type rdf:resource="http://www.w3.org/2004/02/skos/core#Concept"/>
	<skos:prefLabel xml:lang="nl">ankeriet</skos:prefLabel>
	<skos:prefLabel xml:lang="de">Ankerit</skos:prefLabel>
	<skos:prefLabel xml:lang="es">ankerita</skos:prefLabel>
	<skos:prefLabel xml:lang="en">ankerite</skos:prefLabel>
	<skos:prefLabel xml:lang="it">ankerite</skos:prefLabel>
	<skos:prefLabel xml:lang="fr">ankérite</skos:prefLabel>
	<skos:broader rdf:resource="https://ark.frantiq.fr/ark:/26678/pcrtqnzx9qwkt5"/>
	<skos:inScheme rdf:resource="https://ark.frantiq.fr/ark:/26678/TH_1"/>
	<opentheso:memberOf rdf:resource="https://ark.frantiq.fr/ark:/26678/pcrtv66rn9cbv1"/>
	<opentheso:memberOf rdf:resource="https://ark.frantiq.fr/ark:/26678/pcrtnbDLi2FkAj"/>
	<skos:exactMatch rdf:resource="https://www.wikidata.org/wiki/Q120481"/>
	<dcterms:created rdf:datatype="http://www.w3.org/2001/XMLSchema#date">2021-07-23</dcterms:created>
	<dcterms:modified rdf:datatype="http://www.w3.org/2001/XMLSchema#date">2023-08-02</dcterms:modified>
	<dcterms:identifier>266968</dcterms:identifier>
	<dcterms:contributor>blandine.nouvel</dcterms:contributor>
	<skos:definition xml:lang="en">Rhombohedral ferrous carbonate, similar to dolomite (Fernandes, 2012).</skos:definition>
	<skos:definition xml:lang="fr">Carbonate ferreux rhomboédrique, proche de la dolomite (Fernandes, 2012).</skos:definition>
</rdf:Description>

<rdf:Description rdf:about="https://ark.frantiq.fr/ark:/26678/pcrtfpt7p2xkdf">
	<rdf:type rdf:resource="http://www.w3.org/2004/02/skos/core#Concept"/>
	<skos:prefLabel xml:lang="es">moscovita</skos:prefLabel>
	<skos:prefLabel xml:lang="de">Muscovit</skos:prefLabel>
	<skos:prefLabel xml:lang="en">muscovite</skos:prefLabel>
	<skos:prefLabel xml:lang="fr">muscovite</skos:prefLabel>
	<skos:prefLabel xml:lang="it">muscovite</skos:prefLabel>
	<skos:prefLabel xml:lang="nl">muskoviet</skos:prefLabel>
	<skos:altLabel xml:lang="en">common mica</skos:altLabel>
	<skos:altLabel xml:lang="en">isinglass</skos:altLabel>
	<skos:broader rdf:resource="https://ark.frantiq.fr/ark:/26678/pcrty2mcsksa6s"/>
	<skos:inScheme rdf:resource="https://ark.frantiq.fr/ark:/26678/TH_1"/>
	<opentheso:memberOf rdf:resource="https://ark.frantiq.fr/ark:/26678/pcrtv66rn9cbv1"/>
	<opentheso:memberOf rdf:resource="https://ark.frantiq.fr/ark:/26678/pcrtnbDLi2FkAj"/>
	<skos:exactMatch rdf:resource="https://www.wikidata.org/wiki/Q106532"/>
	<dcterms:created rdf:datatype="http://www.w3.org/2001/XMLSchema#date">2021-07-23</dcterms:created>
	<dcterms:modified rdf:datatype="http://www.w3.org/2001/XMLSchema#date">2023-08-02</dcterms:modified>
	<dcterms:identifier>266970</dcterms:identifier>
	<dcterms:contributor>blandine.nouvel</dcterms:contributor>
	<skos:definition xml:lang="en">Hydrated aluminium-potassium silicate, elongated monoclinic and lamellar (Fernandes, 2012).</skos:definition>
	<skos:definition xml:lang="fr">Silicate hydraté d’aluminium et de potassium, monoclinique allongé et lamellaire (Fernandes, 2012).</skos:definition>
</rdf:Description>

<rdf:Description rdf:about="https://ark.frantiq.fr/ark:/26678/pcrt01dd8jnk9r">
	<rdf:type rdf:resource="http://www.w3.org/2004/02/skos/core#Concept"/>
	<skos:prefLabel xml:lang="nl">biotiet</skos:prefLabel>
	<skos:prefLabel xml:lang="de">Biotit</skos:prefLabel>
	<skos:prefLabel xml:lang="es">biotita</skos:prefLabel>
	<skos:prefLabel xml:lang="en">biotite</skos:prefLabel>
	<skos:prefLabel xml:lang="fr">biotite</skos:prefLabel>
	<skos:prefLabel xml:lang="it">biotite</skos:prefLabel>
	<skos:broader rdf:resource="https://ark.frantiq.fr/ark:/26678/pcrty2mcsksa6s"/>
	<skos:inScheme rdf:resource="https://ark.frantiq.fr/ark:/26678/TH_1"/>
	<opentheso:memberOf rdf:resource="https://ark.frantiq.fr/ark:/26678/pcrtv66rn9cbv1"/>
	<opentheso:memberOf rdf:resource="https://ark.frantiq.fr/ark:/26678/pcrtnbDLi2FkAj"/>
	<skos:exactMatch rdf:resource="https://www.wikidata.org/wiki/Q105794"/>
	<dcterms:created rdf:datatype="http://www.w3.org/2001/XMLSchema#date">2021-07-23</dcterms:created>
	<dcterms:modified rdf:datatype="http://www.w3.org/2001/XMLSchema#date">2023-08-02</dcterms:modified>
	<dcterms:identifier>266972</dcterms:identifier>
	<dcterms:contributor>blandine.nouvel</dcterms:contributor>
	<skos:definition xml:lang="en">Hydrated silicate of aluminium and iron or magnesium (Fernandes, 2012).</skos:definition>
	<skos:definition xml:lang="fr">Silicate hydraté d’aluminium et de fer ou de magnésium (Fernandes, 2012).</skos:definition>
</rdf:Description>

<rdf:Description rdf:about="https://ark.frantiq.fr/ark:/26678/pcrtbrv3wp92hn">
	<rdf:type rdf:resource="http://www.w3.org/2004/02/skos/core#Concept"/>
	<skos:prefLabel xml:lang="en">zircon</skos:prefLabel>
	<skos:prefLabel xml:lang="fr">zircon</skos:prefLabel>
	<skos:prefLabel xml:lang="es">zircón</skos:prefLabel>
	<skos:prefLabel xml:lang="it">zircone</skos:prefLabel>
	<skos:prefLabel xml:lang="de">Zirkon</skos:prefLabel>
	<skos:prefLabel xml:lang="nl">zirkoon</skos:prefLabel>
	<skos:altLabel xml:lang="es">circón</skos:altLabel>
	<skos:related rdf:resource="https://ark.frantiq.fr/ark:/26678/pcrtcTqKm5ufUF"/>
	<skos:broader rdf:resource="https://ark.frantiq.fr/ark:/26678/pcrty2mcsksa6s"/>
	<skos:inScheme rdf:resource="https://ark.frantiq.fr/ark:/26678/TH_1"/>
	<opentheso:memberOf rdf:resource="https://ark.frantiq.fr/ark:/26678/pcrtv66rn9cbv1"/>
	<opentheso:memberOf rdf:resource="https://ark.frantiq.fr/ark:/26678/pcrtnbDLi2FkAj"/>
	<skos:exactMatch rdf:resource="https://www.wikidata.org/wiki/Q178928"/>
	<dcterms:created rdf:datatype="http://www.w3.org/2001/XMLSchema#date">2021-07-23</dcterms:created>
	<dcterms:modified rdf:datatype="http://www.w3.org/2001/XMLSchema#date">2024-11-19</dcterms:modified>
	<dcterms:identifier>266974</dcterms:identifier>
	<dcterms:contributor>blandine.nouvel</dcterms:contributor>
	<dcterms:contributor>justine.vincent</dcterms:contributor>
	<skos:definition xml:lang="en">Zirconium silicate is a quadratic gemstone, ranging in colour from highly variable to colourless, and popular as a substitute for diamonds.</skos:definition>
	<skos:definition xml:lang="fr">Le silicate de zirconium est une pierre précieuse quadratique, de couleur très variable à incolore et &lt;span style= background-color: rgb(255, 255, 255); &gt;apprécié comme substitut des diamants&lt;/span&gt;.</skos:definition>
	<skos:historyNote xml:lang="fr">2024-11-19 : modification de la définition.</skos:historyNote>
</rdf:Description>

<rdf:Description rdf:about="https://ark.frantiq.fr/ark:/26678/pcrtpp27tm32r2">
	<rdf:type rdf:resource="http://www.w3.org/2004/02/skos/core#Concept"/>
	<skos:prefLabel xml:lang="nl">toermalijn</skos:prefLabel>
	<skos:prefLabel xml:lang="it">tormalina</skos:prefLabel>
	<skos:prefLabel xml:lang="en">tourmaline</skos:prefLabel>
	<skos:prefLabel xml:lang="fr">tourmaline</skos:prefLabel>
	<skos:prefLabel xml:lang="de">Turmalin</skos:prefLabel>
	<skos:prefLabel xml:lang="es">turmalina</skos:prefLabel>
	<skos:related rdf:resource="https://ark.frantiq.fr/ark:/26678/pcrtJt3ZKiNEFK"/>
	<skos:broader rdf:resource="https://ark.frantiq.fr/ark:/26678/pcrty2mcsksa6s"/>
	<skos:inScheme rdf:resource="https://ark.frantiq.fr/ark:/26678/TH_1"/>
	<opentheso:memberOf rdf:resource="https://ark.frantiq.fr/ark:/26678/pcrtv66rn9cbv1"/>
	<opentheso:memberOf rdf:resource="https://ark.frantiq.fr/ark:/26678/pcrtnbDLi2FkAj"/>
	<skos:exactMatch rdf:resource="https://www.wikidata.org/wiki/Q179911"/>
	<dcterms:created rdf:datatype="http://www.w3.org/2001/XMLSchema#date">2021-07-23</dcterms:created>
	<dcterms:modified rdf:datatype="http://www.w3.org/2001/XMLSchema#date">2024-11-19</dcterms:modified>
	<dcterms:identifier>266976</dcterms:identifier>
	<dcterms:contributor>blandine.nouvel</dcterms:contributor>
	<dcterms:contributor>justine.vincent</dcterms:contributor>
	<skos:definition xml:lang="fr">Minéral borosilicate de la famille des cyclosilicates rhomboédriques en prismes allongés à pléochroïsme inverse, utilisé en joaillerie pour les variétés colorées. (Fernandes, 2012).</skos:definition>
	<skos:definition xml:lang="en">Borosilicate mineral of the rhombohedral cyclosilicate family in elongated prisms with reverse pleochroism, used in jewellery for coloured varieties (Fernandes, 2012).</skos:definition>
</rdf:Description>

<rdf:Description rdf:about="https://ark.frantiq.fr/ark:/26678/pcrttr8kcz7mgd">
	<rdf:type rdf:resource="http://www.w3.org/2004/02/skos/core#Concept"/>
	<skos:prefLabel xml:lang="nl">carbonaat extraclast</skos:prefLabel>
	<skos:prefLabel xml:lang="en">carbonate extraclast</skos:prefLabel>
	<skos:prefLabel xml:lang="fr">extraclaste carbonaté</skos:prefLabel>
	<skos:prefLabel xml:lang="es">extraclasto carbonatado</skos:prefLabel>
	<skos:prefLabel xml:lang="it">extraclasto di carbonato</skos:prefLabel>
	<skos:prefLabel xml:lang="de">Karbonat-Extraklast</skos:prefLabel>
	<skos:broader rdf:resource="https://ark.frantiq.fr/ark:/26678/pcrty2mcsksa6s"/>
	<skos:inScheme rdf:resource="https://ark.frantiq.fr/ark:/26678/TH_1"/>
	<opentheso:memberOf rdf:resource="https://ark.frantiq.fr/ark:/26678/pcrtv66rn9cbv1"/>
	<opentheso:memberOf rdf:resource="https://ark.frantiq.fr/ark:/26678/pcrtnbDLi2FkAj"/>
	<dcterms:created rdf:datatype="http://www.w3.org/2001/XMLSchema#date">2021-07-23</dcterms:created>
	<dcterms:modified rdf:datatype="http://www.w3.org/2001/XMLSchema#date">2024-11-18</dcterms:modified>
	<dcterms:identifier>266978</dcterms:identifier>
	<dcterms:contributor>blandine.nouvel</dcterms:contributor>
	<dcterms:contributor>justine.vincent</dcterms:contributor>
	<skos:definition xml:lang="fr">Fragment allogène de roche carbonatée. (Fernandes, 2012)</skos:definition>
	<skos:definition xml:lang="en">Allogenic fragment of carbonate rock. (Fernandes, 2012)</skos:definition>
</rdf:Description>

<rdf:Description rdf:about="https://ark.frantiq.fr/ark:/26678/pcrtjrbdhj75z0">
	<rdf:type rdf:resource="http://www.w3.org/2004/02/skos/core#Concept"/>
	<skos:prefLabel xml:lang="es">cuarcita</skos:prefLabel>
	<skos:prefLabel xml:lang="en">quartzine</skos:prefLabel>
	<skos:prefLabel xml:lang="fr">quartzine</skos:prefLabel>
	<skos:prefLabel xml:lang="de">Quarzin</skos:prefLabel>
	<skos:prefLabel xml:lang="it">quarzite</skos:prefLabel>
	<skos:related rdf:resource="https://ark.frantiq.fr/ark:/26678/pcrtcb7qm82cts"/>
	<skos:broader rdf:resource="https://ark.frantiq.fr/ark:/26678/pcrty2mcsksa6s"/>
	<skos:inScheme rdf:resource="https://ark.frantiq.fr/ark:/26678/TH_1"/>
	<opentheso:memberOf rdf:resource="https://ark.frantiq.fr/ark:/26678/pcrtv66rn9cbv1"/>
	<opentheso:memberOf rdf:resource="https://ark.frantiq.fr/ark:/26678/pcrtnbDLi2FkAj"/>
	<skos:exactMatch rdf:resource="https://www.wikidata.org/wiki/Q1722152"/>
	<dcterms:created rdf:datatype="http://www.w3.org/2001/XMLSchema#date">2021-07-23</dcterms:created>
	<dcterms:modified rdf:datatype="http://www.w3.org/2001/XMLSchema#date">2024-11-19</dcterms:modified>
	<dcterms:identifier>266980</dcterms:identifier>
	<dcterms:contributor>blandine.nouvel</dcterms:contributor>
	<dcterms:contributor>justine.vincent</dcterms:contributor>
	<skos:definition xml:lang="en">Fibrous microcrystalline habitus of quartz, distinct from chalcedony by its positive elongation and forming aggregates of crystals with varied morphologies (spherulites, dendrites, fibres, etc.) (Fernandes, 2012).</skos:definition>
	<skos:definition xml:lang="fr">Habitus microcristallin fibreux du quartz, distinct de la calcédoine par son allongement positif et formant des agrégats de cristaux à morphologies variées (sphérolites, dendrites, fibres…) (Fernandes, 2012).</skos:definition>
</rdf:Description>

<rdf:Description rdf:about="https://ark.frantiq.fr/ark:/26678/pcrtcb7qm82cts">
	<rdf:type rdf:resource="http://www.w3.org/2004/02/skos/core#Concept"/>
	<skos:prefLabel xml:lang="es">calcedonia</skos:prefLabel>
	<skos:prefLabel xml:lang="nl">calcedoniet</skos:prefLabel>
	<skos:prefLabel xml:lang="it">calcedonio</skos:prefLabel>
	<skos:prefLabel xml:lang="de">Calcedonit</skos:prefLabel>
	<skos:prefLabel xml:lang="fr">calcédonite</skos:prefLabel>
	<skos:prefLabel xml:lang="en">chalcedony</skos:prefLabel>
	<skos:related rdf:resource="https://ark.frantiq.fr/ark:/26678/pcrtOBWTai2Xms"/>
	<skos:related rdf:resource="https://ark.frantiq.fr/ark:/26678/pcrtjrbdhj75z0"/>
	<skos:narrower rdf:resource="https://ark.frantiq.fr/ark:/26678/pcrtc02b47wn5t"/>
	<skos:broader rdf:resource="https://ark.frantiq.fr/ark:/26678/pcrty2mcsksa6s"/>
	<skos:inScheme rdf:resource="https://ark.frantiq.fr/ark:/26678/TH_1"/>
	<opentheso:memberOf rdf:resource="https://ark.frantiq.fr/ark:/26678/pcrtv66rn9cbv1"/>
	<opentheso:memberOf rdf:resource="https://ark.frantiq.fr/ark:/26678/pcrtnbDLi2FkAj"/>
	<dcterms:created rdf:datatype="http://www.w3.org/2001/XMLSchema#date">2021-07-23</dcterms:created>
	<dcterms:modified rdf:datatype="http://www.w3.org/2001/XMLSchema#date">2024-11-18</dcterms:modified>
	<dcterms:identifier>266982</dcterms:identifier>
	<dcterms:contributor>blandine.nouvel</dcterms:contributor>
	<dcterms:contributor>justine.vincent</dcterms:contributor>
	<skos:definition xml:lang="fr">Minéral sulfate-carbonate de plomb et de cuivre richement coloré bleu-vert ayant une structure cristalline orthorhombique. (Wikipedia)</skos:definition>
	<skos:definition xml:lang="en">Lead and copper sulphate-carbonate mineral with a rich blue-green colour and an orthorhombic crystal structure (Wikipedia)</skos:definition>
	<skos:historyNote xml:lang="fr">2024-11-18 : modification de la définition.</skos:historyNote>
</rdf:Description>

<rdf:Description rdf:about="https://ark.frantiq.fr/ark:/26678/pcrtc02b47wn5t">
	<rdf:type rdf:resource="http://www.w3.org/2004/02/skos/core#Concept"/>
	<skos:prefLabel xml:lang="es">pseudocalcedonia</skos:prefLabel>
	<skos:prefLabel xml:lang="it">pseudo-calcedonio</skos:prefLabel>
	<skos:prefLabel xml:lang="fr">pseudo-calcédonite</skos:prefLabel>
	<skos:prefLabel xml:lang="en">pseudo-chalcedony</skos:prefLabel>
	<skos:prefLabel xml:lang="nl">pseudokaledoniet</skos:prefLabel>
	<skos:prefLabel xml:lang="de">Pseudokaledonit</skos:prefLabel>
	<skos:hiddenLabel xml:lang="fr">pseudocalcédonite</skos:hiddenLabel>
	<skos:broader rdf:resource="https://ark.frantiq.fr/ark:/26678/pcrtcb7qm82cts"/>
	<skos:inScheme rdf:resource="https://ark.frantiq.fr/ark:/26678/TH_1"/>
	<opentheso:memberOf rdf:resource="https://ark.frantiq.fr/ark:/26678/pcrtv66rn9cbv1"/>
	<opentheso:memberOf rdf:resource="https://ark.frantiq.fr/ark:/26678/pcrtnbDLi2FkAj"/>
	<dcterms:created rdf:datatype="http://www.w3.org/2001/XMLSchema#date">2021-07-23</dcterms:created>
	<dcterms:modified rdf:datatype="http://www.w3.org/2001/XMLSchema#date">2023-08-02</dcterms:modified>
	<dcterms:identifier>266984</dcterms:identifier>
	<dcterms:contributor>blandine.nouvel</dcterms:contributor>
	<skos:definition xml:lang="en">Fibrous microcrystalline habitus of negative-elongation quartz (Fernandes, 2012).</skos:definition>
	<skos:definition xml:lang="fr">Habitus microcristallin fibreux du quartz à allongement négatif (Fernandes, 2012).</skos:definition>
</rdf:Description>

<rdf:Description rdf:about="https://ark.frantiq.fr/ark:/26678/pcrtt9jqbj1ghk">
	<rdf:type rdf:resource="http://www.w3.org/2004/02/skos/core#Concept"/>
	<skos:prefLabel xml:lang="nl">moganiet</skos:prefLabel>
	<skos:prefLabel xml:lang="de">Mogánit</skos:prefLabel>
	<skos:prefLabel xml:lang="es">moganita</skos:prefLabel>
	<skos:prefLabel xml:lang="en">moganite</skos:prefLabel>
	<skos:prefLabel xml:lang="fr">moganite</skos:prefLabel>
	<skos:prefLabel xml:lang="it">moganite</skos:prefLabel>
	<skos:altLabel xml:lang="fr">IMA 1999-035</skos:altLabel>
	<skos:altLabel xml:lang="fr">lutécite</skos:altLabel>
	<skos:broader rdf:resource="https://ark.frantiq.fr/ark:/26678/pcrty2mcsksa6s"/>
	<skos:inScheme rdf:resource="https://ark.frantiq.fr/ark:/26678/TH_1"/>
	<opentheso:memberOf rdf:resource="https://ark.frantiq.fr/ark:/26678/pcrtv66rn9cbv1"/>
	<opentheso:memberOf rdf:resource="https://ark.frantiq.fr/ark:/26678/pcrtnbDLi2FkAj"/>
	<skos:exactMatch rdf:resource="https://www.wikidata.org/wiki/Q415243"/>
	<dcterms:created rdf:datatype="http://www.w3.org/2001/XMLSchema#date">2021-07-23</dcterms:created>
	<dcterms:modified rdf:datatype="http://www.w3.org/2001/XMLSchema#date">2024-11-18</dcterms:modified>
	<dcterms:identifier>266986</dcterms:identifier>
	<dcterms:contributor>blandine.nouvel</dcterms:contributor>
	<dcterms:contributor>justine.vincent</dcterms:contributor>
	<skos:definition xml:lang="en">Mineral species composed of silica, considered to be a polymorph of quartz.</skos:definition>
	<skos:definition xml:lang="fr">Espèce minérale formée de silice, considérée comme un polymorphe du quartz.</skos:definition>
	<dcterms:isReplacedBy rdf:resource="https://ark.frantiq.fr/ark:/26678/pcrtt9jqbj1ghk"/>
</rdf:Description>

<rdf:Description rdf:about="https://ark.frantiq.fr/ark:/26678/pcrtm4r7mvsvrw">
	<rdf:type rdf:resource="http://www.w3.org/2004/02/skos/core#Concept"/>
	<skos:prefLabel xml:lang="en">carbonate rock</skos:prefLabel>
	<skos:prefLabel xml:lang="de">Karbonatgestein</skos:prefLabel>
	<skos:prefLabel xml:lang="es">roca carbonatada</skos:prefLabel>
	<skos:prefLabel xml:lang="it">roccia carbonatica</skos:prefLabel>
	<skos:prefLabel xml:lang="fr">roche carbonatée</skos:prefLabel>
	<skos:narrower rdf:resource="https://ark.frantiq.fr/ark:/26678/pcrtc1Ueky7Zpg"/>
	<skos:narrower rdf:resource="https://ark.frantiq.fr/ark:/26678/pcrt45bjq160pt"/>
	<skos:narrower rdf:resource="https://ark.frantiq.fr/ark:/26678/pcrttmkgbwr8c7"/>
	<skos:narrower rdf:resource="https://ark.frantiq.fr/ark:/26678/pcrtfx2fwztQ8p"/>
	<skos:narrower rdf:resource="https://ark.frantiq.fr/ark:/26678/pcrtbxntxs7hfz99qvswk8k1"/>
	<skos:broader rdf:resource="https://ark.frantiq.fr/ark:/26678/pcrtj3ZcwkArSR"/>
	<skos:inScheme rdf:resource="https://ark.frantiq.fr/ark:/26678/TH_1"/>
	<opentheso:memberOf rdf:resource="https://ark.frantiq.fr/ark:/26678/pcrtv66rn9cbv1"/>
	<opentheso:memberOf rdf:resource="https://ark.frantiq.fr/ark:/26678/pcrtnbDLi2FkAj"/>
	<skos:exactMatch rdf:resource="https://www.wikidata.org/wiki/Q777913"/>
	<dcterms:created rdf:datatype="http://www.w3.org/2001/XMLSchema#date">2021-07-23</dcterms:created>
	<dcterms:modified rdf:datatype="http://www.w3.org/2001/XMLSchema#date">2023-08-02</dcterms:modified>
	<dcterms:identifier>266988</dcterms:identifier>
	<dcterms:contributor>blandine.nouvel</dcterms:contributor>
	<skos:definition xml:lang="fr">Roches sédimentaires résultant de la compaction de sédiments carbonatés et composés d'au moins 50 % de carbonates. (Wikipedia)</skos:definition>
</rdf:Description>

<rdf:Description rdf:about="https://ark.frantiq.fr/ark:/26678/pcrt45bjq160pt">
	<rdf:type rdf:resource="http://www.w3.org/2004/02/skos/core#Concept"/>
	<skos:prefLabel xml:lang="es">micrita</skos:prefLabel>
	<skos:prefLabel xml:lang="en">micrite</skos:prefLabel>
	<skos:prefLabel xml:lang="fr">micrite</skos:prefLabel>
	<skos:prefLabel xml:lang="it">micrite</skos:prefLabel>
	<skos:prefLabel xml:lang="de">Mikrit</skos:prefLabel>
	<skos:related rdf:resource="https://ark.frantiq.fr/ark:/26678/pcrtqh9bhz6xcr"/>
	<skos:broader rdf:resource="https://ark.frantiq.fr/ark:/26678/pcrtm4r7mvsvrw"/>
	<skos:inScheme rdf:resource="https://ark.frantiq.fr/ark:/26678/TH_1"/>
	<opentheso:memberOf rdf:resource="https://ark.frantiq.fr/ark:/26678/pcrtv66rn9cbv1"/>
	<opentheso:memberOf rdf:resource="https://ark.frantiq.fr/ark:/26678/pcrtnbDLi2FkAj"/>
	<skos:exactMatch rdf:resource="https://www.wikidata.org/wiki/Q1761229"/>
	<dcterms:created rdf:datatype="http://www.w3.org/2001/XMLSchema#date">2021-07-23</dcterms:created>
	<dcterms:modified rdf:datatype="http://www.w3.org/2001/XMLSchema#date">2023-08-02</dcterms:modified>
	<dcterms:identifier>266990</dcterms:identifier>
	<dcterms:contributor>blandine.nouvel</dcterms:contributor>
	<skos:definition xml:lang="fr">Calcite finement cristalline constituant tout ou partie de certaines roches carbonatées, dont par extension elles ont pris le nom (micrite) (Fernandes, 2012).</skos:definition>
</rdf:Description>

<rdf:Description rdf:about="https://ark.frantiq.fr/ark:/26678/pcrttmkgbwr8c7">
	<rdf:type rdf:resource="http://www.w3.org/2004/02/skos/core#Concept"/>
	<skos:prefLabel xml:lang="nl">calcareeniet</skos:prefLabel>
	<skos:prefLabel xml:lang="de">Calcareenit</skos:prefLabel>
	<skos:prefLabel xml:lang="es">calcarenita</skos:prefLabel>
	<skos:prefLabel xml:lang="en">calcarenite</skos:prefLabel>
	<skos:prefLabel xml:lang="it">calcarenite</skos:prefLabel>
	<skos:prefLabel xml:lang="fr">calcarénite</skos:prefLabel>
	<skos:broader rdf:resource="https://ark.frantiq.fr/ark:/26678/pcrtm4r7mvsvrw"/>
	<skos:inScheme rdf:resource="https://ark.frantiq.fr/ark:/26678/TH_1"/>
	<opentheso:memberOf rdf:resource="https://ark.frantiq.fr/ark:/26678/pcrtv66rn9cbv1"/>
	<opentheso:memberOf rdf:resource="https://ark.frantiq.fr/ark:/26678/pcrtnbDLi2FkAj"/>
	<skos:exactMatch rdf:resource="https://www.wikidata.org/wiki/Q2286246"/>
	<dcterms:created rdf:datatype="http://www.w3.org/2001/XMLSchema#date">2021-07-23</dcterms:created>
	<dcterms:modified rdf:datatype="http://www.w3.org/2001/XMLSchema#date">2023-08-02</dcterms:modified>
	<dcterms:identifier>266992</dcterms:identifier>
	<dcterms:contributor>blandine.nouvel</dcterms:contributor>
	<skos:definition xml:lang="fr">Roche sédimentaire carbonatée consolidée dont les éléments ont des dimensions comprises entre 63 µm et 2 mm (Fernandes, 2012).</skos:definition>
</rdf:Description>

<rdf:Description rdf:about="https://ark.frantiq.fr/ark:/26678/pcrtqh9bhz6xcr">
	<rdf:type rdf:resource="http://www.w3.org/2004/02/skos/core#Concept"/>
	<skos:prefLabel xml:lang="it">arenaria carbonatica</skos:prefLabel>
	<skos:prefLabel xml:lang="es">arenisca carbonatada</skos:prefLabel>
	<skos:prefLabel xml:lang="en">carbonate sandstone</skos:prefLabel>
	<skos:prefLabel xml:lang="fr">grès carbonaté</skos:prefLabel>
	<skos:prefLabel xml:lang="de">karbonatischer Sandstein</skos:prefLabel>
	<skos:related rdf:resource="https://ark.frantiq.fr/ark:/26678/pcrt45bjq160pt"/>
	<skos:broader rdf:resource="https://ark.frantiq.fr/ark:/26678/pcrtR1s94Zuaul"/>
	<skos:inScheme rdf:resource="https://ark.frantiq.fr/ark:/26678/TH_1"/>
	<opentheso:memberOf rdf:resource="https://ark.frantiq.fr/ark:/26678/pcrtv66rn9cbv1"/>
	<opentheso:memberOf rdf:resource="https://ark.frantiq.fr/ark:/26678/pcrtnbDLi2FkAj"/>
	<dcterms:created rdf:datatype="http://www.w3.org/2001/XMLSchema#date">2021-07-23</dcterms:created>
	<dcterms:modified rdf:datatype="http://www.w3.org/2001/XMLSchema#date">2023-08-02</dcterms:modified>
	<dcterms:identifier>266994</dcterms:identifier>
	<dcterms:contributor>blandine.nouvel</dcterms:contributor>
</rdf:Description>

<rdf:Description rdf:about="https://ark.frantiq.fr/ark:/26678/pcrtsrWeYcRkNg">
	<rdf:type rdf:resource="http://www.w3.org/2004/02/skos/core#Concept"/>
	<skos:prefLabel xml:lang="es">carbón</skos:prefLabel>
	<skos:prefLabel xml:lang="it">carbone</skos:prefLabel>
	<skos:prefLabel xml:lang="fr">charbon</skos:prefLabel>
	<skos:prefLabel xml:lang="en">coal</skos:prefLabel>
	<skos:prefLabel xml:lang="de">Kohle</skos:prefLabel>
	<skos:prefLabel xml:lang="nl">kool</skos:prefLabel>
	<skos:prefLabel xml:lang="ar">فحم</skos:prefLabel>
	<skos:narrower rdf:resource="https://ark.frantiq.fr/ark:/26678/pcrt9rIFPQ997Q"/>
	<skos:narrower rdf:resource="https://ark.frantiq.fr/ark:/26678/pcrtQhjRUa1GV8"/>
	<skos:narrower rdf:resource="https://ark.frantiq.fr/ark:/26678/pcrt1jTyJEx22Y"/>
	<skos:broader rdf:resource="https://ark.frantiq.fr/ark:/26678/pcrtj3ZcwkArSR"/>
	<skos:inScheme rdf:resource="https://ark.frantiq.fr/ark:/26678/TH_1"/>
	<opentheso:memberOf rdf:resource="https://ark.frantiq.fr/ark:/26678/pcrtv66rn9cbv1"/>
	<opentheso:memberOf rdf:resource="https://ark.frantiq.fr/ark:/26678/pcrtnbDLi2FkAj"/>
	<opentheso:memberOf rdf:resource="https://ark.frantiq.fr/ark:/26678/pcrtv0jq332vcq3gxt5m13d5"/>
	<skos:exactMatch rdf:resource="https://catalogue.bnf.fr/ark:/12148/cb11941871n"/>
	<skos:exactMatch rdf:resource="https://www.wikidata.org/wiki/Q24489"/>
	<dcterms:created rdf:datatype="http://www.w3.org/2001/XMLSchema#date">2007-02-08</dcterms:created>
	<dcterms:modified rdf:datatype="http://www.w3.org/2001/XMLSchema#date">2024-04-11</dcterms:modified>
	<dcterms:identifier>26893</dcterms:identifier>
	<dcterms:contributor>blandine.nouvel</dcterms:contributor>
	<dcterms:contributor>irene.weis</dcterms:contributor>
	<skos:definition xml:lang="en">Carbon-rich, combustible sedimentary rock, black or dark brown in colour, formed from the partial degradation of plant organic matter. (wp)</skos:definition>
	<skos:definition xml:lang="fr">Roche sédimentaire combustible, riche en carbone, de couleur noire ou marron foncé, formée à partir de la dégradation partielle de la matière organique des végétaux. (wp)</skos:definition>
</rdf:Description>

<rdf:Description rdf:about="https://ark.frantiq.fr/ark:/26678/pcrtStScmr2cmH">
	<rdf:type rdf:resource="http://www.w3.org/2004/02/skos/core#Concept"/>
	<skos:prefLabel xml:lang="nl">afaniet</skos:prefLabel>
	<skos:prefLabel xml:lang="es">afanita</skos:prefLabel>
	<skos:prefLabel xml:lang="it">afanite</skos:prefLabel>
	<skos:prefLabel xml:lang="de">Aphanit</skos:prefLabel>
	<skos:prefLabel xml:lang="en">aphanite</skos:prefLabel>
	<skos:prefLabel xml:lang="fr">aphanite</skos:prefLabel>
	<skos:prefLabel xml:lang="ar">أفانيت</skos:prefLabel>
	<skos:broader rdf:resource="https://ark.frantiq.fr/ark:/26678/pcrtmxvuuXHSTS"/>
	<skos:inScheme rdf:resource="https://ark.frantiq.fr/ark:/26678/TH_1"/>
	<opentheso:memberOf rdf:resource="https://ark.frantiq.fr/ark:/26678/pcrtv66rn9cbv1"/>
	<opentheso:memberOf rdf:resource="https://ark.frantiq.fr/ark:/26678/pcrtnbDLi2FkAj"/>
	<skos:exactMatch rdf:resource="https://www.wikidata.org/wiki/Q618416"/>
	<dcterms:created rdf:datatype="http://www.w3.org/2001/XMLSchema#date">2007-02-08</dcterms:created>
	<dcterms:modified rdf:datatype="http://www.w3.org/2001/XMLSchema#date">2023-08-02</dcterms:modified>
	<dcterms:identifier>26948</dcterms:identifier>
	<dcterms:contributor>blandine.nouvel</dcterms:contributor>
	<skos:definition xml:lang="en">A magmatic rock with a very fine-grained structure. Its crystals are so small that they cannot be seen with the naked eye (Wikipedia).</skos:definition>
	<skos:definition xml:lang="ar">صخر صلب دقيق البلورات</skos:definition>
	<skos:definition xml:lang="fr">Roche magmatique dont la structure est à grain très fin. Les cristaux qui la composent sont si petits qu'ils ne peuvent être observés à l'œil nu. (Wikipédia)</skos:definition>
</rdf:Description>

<rdf:Description rdf:about="https://ark.frantiq.fr/ark:/26678/pcrt1asKmbn9q8">
	<rdf:type rdf:resource="http://www.w3.org/2004/02/skos/core#Concept"/>
	<skos:prefLabel xml:lang="it">ceramica invetriata</skos:prefLabel>
	<skos:prefLabel xml:lang="es">cerámica vidriada</skos:prefLabel>
	<skos:prefLabel xml:lang="fr">céramique glaçurée</skos:prefLabel>
	<skos:prefLabel xml:lang="nl">geglazuurd aardewerk</skos:prefLabel>
	<skos:prefLabel xml:lang="de">glasierte Keramik</skos:prefLabel>
	<skos:prefLabel xml:lang="en">glazed ware</skos:prefLabel>
	<skos:prefLabel xml:lang="ar">خزف مُزَجَّج</skos:prefLabel>
	<skos:altLabel xml:lang="es">cerámica vitrificada</skos:altLabel>
	<skos:altLabel xml:lang="en">glazed ceramic</skos:altLabel>
	<skos:related rdf:resource="https://ark.frantiq.fr/ark:/26678/pcrtYqRY0jHNjP"/>
	<skos:related rdf:resource="https://ark.frantiq.fr/ark:/26678/pcrt3pmFUqt27w"/>
	<skos:related rdf:resource="https://ark.frantiq.fr/ark:/26678/pcrt1sb2p55pwg"/>
	<skos:related rdf:resource="https://ark.frantiq.fr/ark:/26678/pcrt64s6h0j0cp"/>
	<skos:narrower rdf:resource="https://ark.frantiq.fr/ark:/26678/pcrtxk63t9cg4vz559qr94zk"/>
	<skos:broader rdf:resource="https://ark.frantiq.fr/ark:/26678/pcrtfx4s0yvSLj"/>
	<skos:inScheme rdf:resource="https://ark.frantiq.fr/ark:/26678/TH_1"/>
	<opentheso:memberOf rdf:resource="https://ark.frantiq.fr/ark:/26678/pcrtv66rn9cbv1"/>
	<opentheso:memberOf rdf:resource="https://ark.frantiq.fr/ark:/26678/pcrtnbDLi2FkAj"/>
	<skos:exactMatch rdf:resource="https://ark.mom.fr/ark:/39676/bibhrsscjs0sg"/>
	<skos:exactMatch rdf:resource="https://www.wikidata.org/wiki/Q3664976"/>
	<dcterms:created rdf:datatype="http://www.w3.org/2001/XMLSchema#date">2007-02-08</dcterms:created>
	<dcterms:modified rdf:datatype="http://www.w3.org/2001/XMLSchema#date">2024-10-25</dcterms:modified>
	<dcterms:identifier>27378</dcterms:identifier>
	<dcterms:contributor>blandine.nouvel</dcterms:contributor>
	<dcterms:contributor>justine.vincent</dcterms:contributor>
	<dcterms:contributor>patricia.moitrel</dcterms:contributor>
	<skos:definition xml:lang="en">Type of ceramic characterised by the presence of a glaze (Pactols group)</skos:definition>
	<skos:definition xml:lang="fr">Type de céramique caractérisé par la présence d'une glaçure.</skos:definition>
	<skos:scopeNote xml:lang="fr">&amp;amp;nbsp;Ne pas confondre avec la céramique à glaçure plombifère d'époque romaine.</skos:scopeNote>
	<skos:historyNote xml:lang="fr">2024-10-18 : modification de la définition.</skos:historyNote>
</rdf:Description>

<rdf:Description rdf:about="https://ark.frantiq.fr/ark:/26678/pcrtbnBhdnlQrL">
	<rdf:type rdf:resource="http://www.w3.org/2004/02/skos/core#Concept"/>
	<skos:prefLabel xml:lang="nl">doleriet</skos:prefLabel>
	<skos:prefLabel xml:lang="de">Dolerit</skos:prefLabel>
	<skos:prefLabel xml:lang="es">dolerita</skos:prefLabel>
	<skos:prefLabel xml:lang="en">dolerite</skos:prefLabel>
	<skos:prefLabel xml:lang="it">dolerite</skos:prefLabel>
	<skos:prefLabel xml:lang="fr">dolérite</skos:prefLabel>
	<skos:prefLabel xml:lang="ar">دوليريت</skos:prefLabel>
	<skos:altLabel xml:lang="es">diabasa</skos:altLabel>
	<skos:altLabel xml:lang="en">diabase</skos:altLabel>
	<skos:altLabel xml:lang="en">microgabbro</skos:altLabel>
	<skos:broader rdf:resource="https://ark.frantiq.fr/ark:/26678/pcrtmxvuuXHSTS"/>
	<skos:inScheme rdf:resource="https://ark.frantiq.fr/ark:/26678/TH_1"/>
	<opentheso:memberOf rdf:resource="https://ark.frantiq.fr/ark:/26678/pcrtv66rn9cbv1"/>
	<opentheso:memberOf rdf:resource="https://ark.frantiq.fr/ark:/26678/pcrtnbDLi2FkAj"/>
	<skos:exactMatch rdf:resource="https://www.wikidata.org/wiki/Q1235463"/>
	<skos:exactMatch rdf:resource="http://vocab.getty.edu/aat/300311591"/>
	<dcterms:created rdf:datatype="http://www.w3.org/2001/XMLSchema#date">2007-02-08</dcterms:created>
	<dcterms:modified rdf:datatype="http://www.w3.org/2001/XMLSchema#date">2024-11-14</dcterms:modified>
	<dcterms:identifier>27422</dcterms:identifier>
	<dcterms:contributor>blandine.nouvel</dcterms:contributor>
	<dcterms:contributor>justine.vincent</dcterms:contributor>
	<skos:definition xml:lang="en">Magmatic rock intermediate between garnet gabbros and microlithic basalts. Generally greenish or reddish in colour due to alteration, may contain olivine (Lozet &amp;amp; Mathieu, Dictionnaire de science du sol. Ed. Technique et Documentation Lavoisier)</skos:definition>
	<skos:definition xml:lang="ar">صخر بركاني بازلتي</skos:definition>
	<skos:definition xml:lang="fr">Roche magmatique intermédiaire entre les gabbros grenus et les basaltes microlithiques. Teinte généralement verdâtre ou rougeâtre par altération, pouvant renfermer de l'olivine. (Lozet &amp;amp; Mathieu, Dictionnaire de science du sol. Ed. Technique et Documentation Lavoisier)</skos:definition>
</rdf:Description>

<rdf:Description rdf:about="https://ark.frantiq.fr/ark:/26678/pcrtAoNmnP9BYF">
	<rdf:type rdf:resource="http://www.w3.org/2004/02/skos/core#Concept"/>
	<skos:prefLabel xml:lang="fr">émail dentaire</skos:prefLabel>
	<skos:prefLabel xml:lang="es">esmalte dental</skos:prefLabel>
	<skos:prefLabel xml:lang="it">smalto dentale</skos:prefLabel>
	<skos:prefLabel xml:lang="nl">tandglazuur</skos:prefLabel>
	<skos:prefLabel xml:lang="en">tooth enamel</skos:prefLabel>
	<skos:prefLabel xml:lang="de">Zahnschmelz</skos:prefLabel>
	<skos:prefLabel xml:lang="ar">شَنَب</skos:prefLabel>
	<skos:altLabel xml:lang="ar">ميناء الأسنان</skos:altLabel>
	<skos:related rdf:resource="https://ark.frantiq.fr/ark:/26678/pcrthA4kIWMu84"/>
	<skos:broader rdf:resource="https://ark.frantiq.fr/ark:/26678/pcrtf97bQHDGEd"/>
	<skos:inScheme rdf:resource="https://ark.frantiq.fr/ark:/26678/TH_1"/>
	<opentheso:memberOf rdf:resource="https://ark.frantiq.fr/ark:/26678/pcrtv66rn9cbv1"/>
	<opentheso:memberOf rdf:resource="https://ark.frantiq.fr/ark:/26678/pcrtnbDLi2FkAj"/>
	<skos:exactMatch rdf:resource="https://www.wikidata.org/wiki/Q143942"/>
	<skos:exactMatch rdf:resource="http://vocab.getty.edu/aat/300191879"/>
	<dcterms:created rdf:datatype="http://www.w3.org/2001/XMLSchema#date">2007-02-08</dcterms:created>
	<dcterms:modified rdf:datatype="http://www.w3.org/2001/XMLSchema#date">2023-08-02</dcterms:modified>
	<dcterms:identifier>27436</dcterms:identifier>
	<dcterms:contributor>blandine.nouvel</dcterms:contributor>
	<skos:definition xml:lang="en">Extremely hard, translucent substance, 95% mineral matter, which covers the ivory of the dental crown (cnrtl)</skos:definition>
	<skos:definition xml:lang="fr">Substance extrêmement dure, translucide, composée à 95 % de matières minérales, qui recouvre l'ivoire de la couronne dentaire (cnrtl)</skos:definition>
</rdf:Description>

<rdf:Description rdf:about="https://ark.frantiq.fr/ark:/26678/pcrt1jTyJEx22Y">
	<rdf:type rdf:resource="http://www.w3.org/2004/02/skos/core#Concept"/>
	<skos:prefLabel xml:lang="nl">grafiet</skos:prefLabel>
	<skos:prefLabel xml:lang="it">grafite</skos:prefLabel>
	<skos:prefLabel xml:lang="es">grafito</skos:prefLabel>
	<skos:prefLabel xml:lang="de">Graphit</skos:prefLabel>
	<skos:prefLabel xml:lang="en">graphite</skos:prefLabel>
	<skos:prefLabel xml:lang="fr">graphite</skos:prefLabel>
	<skos:prefLabel xml:lang="ar">أَسرَب</skos:prefLabel>
	<skos:related rdf:resource="https://ark.frantiq.fr/ark:/26678/pcrtuia0lxRySc"/>
	<skos:related rdf:resource="https://ark.frantiq.fr/ark:/26678/pcrtq29n54kbvk"/>
	<skos:broader rdf:resource="https://ark.frantiq.fr/ark:/26678/pcrtsrWeYcRkNg"/>
	<skos:inScheme rdf:resource="https://ark.frantiq.fr/ark:/26678/TH_1"/>
	<opentheso:memberOf rdf:resource="https://ark.frantiq.fr/ark:/26678/pcrtv66rn9cbv1"/>
	<opentheso:memberOf rdf:resource="https://ark.frantiq.fr/ark:/26678/pcrtnbDLi2FkAj"/>
	<skos:exactMatch rdf:resource="https://catalogue.bnf.fr/ark:/12148/cb12152787z"/>
	<skos:exactMatch rdf:resource="https://www.wikidata.org/wiki/Q5309"/>
	<skos:exactMatch rdf:resource="http://vocab.getty.edu/aat/300011098"/>
	<dcterms:created rdf:datatype="http://www.w3.org/2001/XMLSchema#date">2007-02-08</dcterms:created>
	<dcterms:modified rdf:datatype="http://www.w3.org/2001/XMLSchema#date">2023-08-02</dcterms:modified>
	<dcterms:identifier>27459</dcterms:identifier>
	<dcterms:contributor>blandine.nouvel</dcterms:contributor>
	<skos:definition xml:lang="en">Mineral species which, along with diamond, lonsdaleite and chaoite, is one of the natural allotropes of carbon (wp)</skos:definition>
	<skos:definition xml:lang="fr">Espèce minérale qui est, avec le diamant, la lonsdaléite et la chaoite, l'un des allotropes naturels du carbone. (wp)</skos:definition>
</rdf:Description>

<rdf:Description rdf:about="https://ark.frantiq.fr/ark:/26678/pcrtOF9oqZo0Pd">
	<rdf:type rdf:resource="http://www.w3.org/2004/02/skos/core#Concept"/>
	<skos:prefLabel xml:lang="es">aljez</skos:prefLabel>
	<skos:prefLabel xml:lang="it">gesso</skos:prefLabel>
	<skos:prefLabel xml:lang="nl">gips</skos:prefLabel>
	<skos:prefLabel xml:lang="de">Gips</skos:prefLabel>
	<skos:prefLabel xml:lang="fr">gypse</skos:prefLabel>
	<skos:prefLabel xml:lang="en">gypsum</skos:prefLabel>
	<skos:prefLabel xml:lang="ar">جِبس </skos:prefLabel>
	<skos:altLabel xml:lang="fr">sélénite</skos:altLabel>
	<skos:related rdf:resource="https://ark.frantiq.fr/ark:/26678/pcrtxVPISFTEr6"/>
	<skos:narrower rdf:resource="https://ark.frantiq.fr/ark:/26678/pcrtzwhr6nrsvxm73pzkq2dq"/>
	<skos:broader rdf:resource="https://ark.frantiq.fr/ark:/26678/pcrty2mcsksa6s"/>
	<skos:inScheme rdf:resource="https://ark.frantiq.fr/ark:/26678/TH_1"/>
	<opentheso:memberOf rdf:resource="https://ark.frantiq.fr/ark:/26678/pcrtv66rn9cbv1"/>
	<opentheso:memberOf rdf:resource="https://ark.frantiq.fr/ark:/26678/pcrtnbDLi2FkAj"/>
	<opentheso:memberOf rdf:resource="https://ark.frantiq.fr/ark:/26678/pcrtv0jq332vcq3gxt5m13d5"/>
	<skos:exactMatch rdf:resource="https://catalogue.bnf.fr/ark:/12148/cb11958210p"/>
	<skos:exactMatch rdf:resource="https://www.idref.fr/02757010X"/>
	<skos:exactMatch rdf:resource="https://www.wikidata.org/wiki/Q82658"/>
	<skos:exactMatch rdf:resource="http://vocab.getty.edu/aat/300011099"/>
	<dcterms:created rdf:datatype="http://www.w3.org/2001/XMLSchema#date">2007-02-08</dcterms:created>
	<dcterms:modified rdf:datatype="http://www.w3.org/2001/XMLSchema#date">2024-11-18</dcterms:modified>
	<dcterms:identifier>27473</dcterms:identifier>
	<dcterms:contributor>blandine.nouvel</dcterms:contributor>
	<dcterms:contributor>irene.weis</dcterms:contributor>
	<dcterms:contributor>justine.vincent</dcterms:contributor>
	<skos:definition xml:lang="en">Mineral species composed of calcium sulphate dihydrate (wp)</skos:definition>
	<skos:definition xml:lang="fr">Espèce minérale composée de sulfate dihydraté de calcium. (wp)</skos:definition>
</rdf:Description>

<rdf:Description rdf:about="https://ark.frantiq.fr/ark:/26678/pcrtslVSzVnfeg">
	<rdf:type rdf:resource="http://www.w3.org/2004/02/skos/core#Concept"/>
	<skos:prefLabel xml:lang="it">giadeite</skos:prefLabel>
	<skos:prefLabel xml:lang="nl">jadeïet</skos:prefLabel>
	<skos:prefLabel xml:lang="de">Jadeit</skos:prefLabel>
	<skos:prefLabel xml:lang="es">jadeíta</skos:prefLabel>
	<skos:prefLabel xml:lang="en">jadeite</skos:prefLabel>
	<skos:prefLabel xml:lang="fr">jadéite</skos:prefLabel>
	<skos:prefLabel xml:lang="ar">جاديت</skos:prefLabel>
	<skos:related rdf:resource="https://ark.frantiq.fr/ark:/26678/pcrtSpItdjR86k"/>
	<skos:broader rdf:resource="https://ark.frantiq.fr/ark:/26678/pcrt7pgeXjaSI8"/>
	<skos:inScheme rdf:resource="https://ark.frantiq.fr/ark:/26678/TH_1"/>
	<opentheso:memberOf rdf:resource="https://ark.frantiq.fr/ark:/26678/pcrtv66rn9cbv1"/>
	<opentheso:memberOf rdf:resource="https://ark.frantiq.fr/ark:/26678/pcrtnbDLi2FkAj"/>
	<skos:exactMatch rdf:resource="https://www.wikidata.org/wiki/Q422173"/>
	<skos:exactMatch rdf:resource="http://vocab.getty.edu/aat/300011121"/>
	<dcterms:created rdf:datatype="http://www.w3.org/2001/XMLSchema#date">2007-02-08</dcterms:created>
	<dcterms:modified rdf:datatype="http://www.w3.org/2001/XMLSchema#date">2023-08-02</dcterms:modified>
	<dcterms:identifier>27495</dcterms:identifier>
	<dcterms:contributor>blandine.nouvel</dcterms:contributor>
	<skos:definition xml:lang="fr">minéral (TLFi)&lt;/br&gt;Espèce minérale de la famille des silicates, classe des inosilicates, groupe des pyroxènes dont la composition chimique idéale est NaAlSi2O6. (wp)</skos:definition>
	<skos:definition xml:lang="en">Mineral species of the silicate family, inosilicate class, pyroxene group, whose ideal chemical composition is NaAlSi2O6. (wp)</skos:definition>
</rdf:Description>

<rdf:Description rdf:about="https://ark.frantiq.fr/ark:/26678/pcrtV3BZNic1DR">
	<rdf:type rdf:resource="http://www.w3.org/2004/02/skos/core#Concept"/>
	<skos:prefLabel xml:lang="es">azabache</skos:prefLabel>
	<skos:prefLabel xml:lang="de">Gagat</skos:prefLabel>
	<skos:prefLabel xml:lang="it">giaietto</skos:prefLabel>
	<skos:prefLabel xml:lang="nl">git</skos:prefLabel>
	<skos:prefLabel xml:lang="fr">jais</skos:prefLabel>
	<skos:prefLabel xml:lang="en">jet (lignite)</skos:prefLabel>
	<skos:prefLabel xml:lang="ar"> فحم أحفوري</skos:prefLabel>
	<skos:altLabel xml:lang="it">gagate</skos:altLabel>
	<skos:altLabel xml:lang="es">gagates</skos:altLabel>
	<skos:altLabel xml:lang="fr">jayet</skos:altLabel>
	<skos:broader rdf:resource="https://ark.frantiq.fr/ark:/26678/pcrtDoEeaZ6VcU"/>
	<skos:inScheme rdf:resource="https://ark.frantiq.fr/ark:/26678/TH_1"/>
	<opentheso:memberOf rdf:resource="https://ark.frantiq.fr/ark:/26678/pcrtv66rn9cbv1"/>
	<opentheso:memberOf rdf:resource="https://ark.frantiq.fr/ark:/26678/pcrtnbDLi2FkAj"/>
	<skos:exactMatch rdf:resource="https://www.wikidata.org/wiki/Q543694"/>
	<skos:exactMatch rdf:resource="http://vocab.getty.edu/aat/300045514"/>
	<dcterms:created rdf:datatype="http://www.w3.org/2001/XMLSchema#date">2007-02-08</dcterms:created>
	<dcterms:modified rdf:datatype="http://www.w3.org/2001/XMLSchema#date">2023-08-02</dcterms:modified>
	<dcterms:identifier>27496</dcterms:identifier>
	<dcterms:contributor>blandine.nouvel</dcterms:contributor>
	<skos:definition xml:lang="en">Fossil gem formed by the action of oceanic pressure on sedimentary rock composed of the fossil remains of plants. (wp)</skos:definition>
	<skos:definition xml:lang="ar">ليغنيت أسود برّاق</skos:definition>
	<skos:definition xml:lang="fr">Gemme fossile formée par l'action de la pression océanique sur une roche sédimentaire composée de restes fossiles de plantes. (wp)</skos:definition>
</rdf:Description>

<rdf:Description rdf:about="https://ark.frantiq.fr/ark:/26678/pcrtAWl3eAUQlA">
	<rdf:type rdf:resource="http://www.w3.org/2004/02/skos/core#Concept"/>
	<skos:prefLabel xml:lang="fr">lait</skos:prefLabel>
	<skos:prefLabel xml:lang="it">latte</skos:prefLabel>
	<skos:prefLabel xml:lang="es">leche</skos:prefLabel>
	<skos:prefLabel xml:lang="nl">melk</skos:prefLabel>
	<skos:prefLabel xml:lang="de">Milch</skos:prefLabel>
	<skos:prefLabel xml:lang="en">milk</skos:prefLabel>
	<skos:prefLabel xml:lang="ar">حليب</skos:prefLabel>
	<skos:related rdf:resource="https://ark.frantiq.fr/ark:/26678/pcrtwjkf1r9cgjwxj7mz9qcn"/>
	<skos:broader rdf:resource="https://ark.frantiq.fr/ark:/26678/pcrt6z097U6IUf"/>
	<skos:inScheme rdf:resource="https://ark.frantiq.fr/ark:/26678/TH_1"/>
	<opentheso:memberOf rdf:resource="https://ark.frantiq.fr/ark:/26678/pcrtv66rn9cbv1"/>
	<opentheso:memberOf rdf:resource="https://ark.frantiq.fr/ark:/26678/pcrtnbDLi2FkAj"/>
	<skos:exactMatch rdf:resource="https://www.wikidata.org/wiki/Q8495"/>
	<skos:exactMatch rdf:resource="http://vocab.getty.edu/aat/300191622"/>
	<dcterms:created rdf:datatype="http://www.w3.org/2001/XMLSchema#date">2007-02-08</dcterms:created>
	<dcterms:modified rdf:datatype="http://www.w3.org/2001/XMLSchema#date">2023-08-02</dcterms:modified>
	<dcterms:identifier>27500</dcterms:identifier>
	<dcterms:contributor>blandine.nouvel</dcterms:contributor>
	<skos:definition xml:lang="en">Biological edible liquid produced by female mammals.</skos:definition>
	<skos:definition xml:lang="fr">Liquide biologique comestible produit par les mammifères femelles.</skos:definition>
</rdf:Description>

<rdf:Description rdf:about="https://ark.frantiq.fr/ark:/26678/pcrtvKH7mF2Oas">
	<rdf:type rdf:resource="http://www.w3.org/2004/02/skos/core#Concept"/>
	<skos:prefLabel xml:lang="nl">grondstof</skos:prefLabel>
	<skos:prefLabel xml:lang="es">materia prima</skos:prefLabel>
	<skos:prefLabel xml:lang="it">materia prima</skos:prefLabel>
	<skos:prefLabel xml:lang="fr">matière première</skos:prefLabel>
	<skos:prefLabel xml:lang="en">raw material</skos:prefLabel>
	<skos:prefLabel xml:lang="de">Rohmaterial</skos:prefLabel>
	<skos:prefLabel xml:lang="ar">مادة أولية</skos:prefLabel>
	<skos:altLabel xml:lang="fr">matériau de base</skos:altLabel>
	<skos:altLabel xml:lang="en">primary commodity</skos:altLabel>
	<skos:altLabel xml:lang="en">primary material</skos:altLabel>
	<skos:altLabel xml:lang="en">unprocessed material</skos:altLabel>
	<skos:related rdf:resource="https://ark.frantiq.fr/ark:/26678/pcrtHDkQbAT5WW"/>
	<skos:related rdf:resource="https://ark.frantiq.fr/ark:/26678/pcrtSVdwKcS3MI"/>
	<skos:related rdf:resource="https://ark.frantiq.fr/ark:/26678/crtYQmrPQmygE"/>
	<skos:related rdf:resource="https://ark.frantiq.fr/ark:/26678/pcrty2mcsksa6s"/>
	<skos:related rdf:resource="https://ark.frantiq.fr/ark:/26678/pcrtnHxyjOkhJw"/>
	<skos:related rdf:resource="https://ark.frantiq.fr/ark:/26678/pcrtf97bQHDGEd"/>
	<skos:broader rdf:resource="https://ark.frantiq.fr/ark:/26678/pcrtIMsuG0RWTs"/>
	<skos:inScheme rdf:resource="https://ark.frantiq.fr/ark:/26678/TH_1"/>
	<opentheso:memberOf rdf:resource="https://ark.frantiq.fr/ark:/26678/pcrtv66rn9cbv1"/>
	<opentheso:memberOf rdf:resource="https://ark.frantiq.fr/ark:/26678/pcrtnbDLi2FkAj"/>
	<skos:exactMatch rdf:resource="https://catalogue.bnf.fr/ark:/12148/cb11950813f"/>
	<skos:exactMatch rdf:resource="https://www.wikidata.org/wiki/Q192355"/>
	<skos:exactMatch rdf:resource="http://vocab.getty.edu/aat/300015351"/>
	<dcterms:created rdf:datatype="http://www.w3.org/2001/XMLSchema#date">2007-02-08</dcterms:created>
	<dcterms:modified rdf:datatype="http://www.w3.org/2001/XMLSchema#date">2024-04-23</dcterms:modified>
	<dcterms:identifier>27525</dcterms:identifier>
	<dcterms:contributor>blandine.nouvel</dcterms:contributor>
	<dcterms:contributor>emmanuelle.bryas</dcterms:contributor>
	<skos:definition xml:lang="fr">Matériau d'origine naturelle utilisé brut ou transformé pour fabriquer un bien ou un produit.</skos:definition>
	<skos:definition xml:lang="en">Material of natural origin used raw or processed to manufacture a good or product.</skos:definition>
	<skos:historyNote xml:lang="fr">2024-04-22 : simplification de la définition et traduction</skos:historyNote>
</rdf:Description>

<rdf:Description rdf:about="https://ark.frantiq.fr/ark:/26678/pcrtFpNU7SZgo7">
	<rdf:type rdf:resource="http://www.w3.org/2004/02/skos/core#Concept"/>
	<skos:prefLabel xml:lang="en">natron</skos:prefLabel>
	<skos:prefLabel xml:lang="fr">natron</skos:prefLabel>
	<skos:prefLabel xml:lang="it">natron</skos:prefLabel>
	<skos:prefLabel xml:lang="nl">natron</skos:prefLabel>
	<skos:prefLabel xml:lang="es">natrón</skos:prefLabel>
	<skos:prefLabel xml:lang="de">Soda</skos:prefLabel>
	<skos:prefLabel xml:lang="ar">نطرون</skos:prefLabel>
	<skos:altLabel xml:lang="fr">natronite</skos:altLabel>
	<skos:altLabel xml:lang="ar">كربونات الصوديوم</skos:altLabel>
	<skos:broader rdf:resource="https://ark.frantiq.fr/ark:/26678/pcrty2mcsksa6s"/>
	<skos:inScheme rdf:resource="https://ark.frantiq.fr/ark:/26678/TH_1"/>
	<opentheso:memberOf rdf:resource="https://ark.frantiq.fr/ark:/26678/pcrtv66rn9cbv1"/>
	<opentheso:memberOf rdf:resource="https://ark.frantiq.fr/ark:/26678/pcrtnbDLi2FkAj"/>
	<skos:exactMatch rdf:resource="https://www.wikidata.org/wiki/Q427329"/>
	<skos:exactMatch rdf:resource="http://vocab.getty.edu/aat/300379923"/>
	<dcterms:created rdf:datatype="http://www.w3.org/2001/XMLSchema#date">2007-02-08</dcterms:created>
	<dcterms:modified rdf:datatype="http://www.w3.org/2001/XMLSchema#date">2024-11-18</dcterms:modified>
	<dcterms:identifier>27529</dcterms:identifier>
	<dcterms:contributor>blandine.nouvel</dcterms:contributor>
	<dcterms:contributor>justine.vincent</dcterms:contributor>
	<skos:definition xml:lang="en">Rock or mineral composed mainly of decahydrated sodium carbonate.</skos:definition>
	<skos:definition xml:lang="fr">Roche ou minéral composé principalement de carbonate de sodium décahydrate.</skos:definition>
</rdf:Description>

<rdf:Description rdf:about="https://ark.frantiq.fr/ark:/26678/pcrtKcuT7Kh6vX">
	<rdf:type rdf:resource="http://www.w3.org/2004/02/skos/core#Concept"/>
	<skos:prefLabel xml:lang="es">cartonaje</skos:prefLabel>
	<skos:prefLabel xml:lang="en">cartonnage</skos:prefLabel>
	<skos:prefLabel xml:lang="it">cartonnage</skos:prefLabel>
	<skos:prefLabel xml:lang="fr">cartonnage de momie</skos:prefLabel>
	<skos:prefLabel xml:lang="de">Mumienkartonnage</skos:prefLabel>
	<skos:prefLabel xml:lang="nl">mummiecartonnage</skos:prefLabel>
	<skos:prefLabel xml:lang="ar">غلاف المومياء</skos:prefLabel>
	<skos:altLabel xml:lang="en">cartonnage mummy masks</skos:altLabel>
	<skos:altLabel xml:lang="fr">enveloppe de cartonnage</skos:altLabel>
	<skos:altLabel xml:lang="en">mummy cartonnage</skos:altLabel>
	<skos:related rdf:resource="https://ark.frantiq.fr/ark:/26678/pcrtxAh3LEGcFT"/>
	<skos:broader rdf:resource="https://ark.frantiq.fr/ark:/26678/pcrtnHxyjOkhJw"/>
	<skos:inScheme rdf:resource="https://ark.frantiq.fr/ark:/26678/TH_1"/>
	<opentheso:memberOf rdf:resource="https://ark.frantiq.fr/ark:/26678/pcrtv66rn9cbv1"/>
	<opentheso:memberOf rdf:resource="https://ark.frantiq.fr/ark:/26678/pcrtnbDLi2FkAj"/>
	<skos:exactMatch rdf:resource="https://www.wikidata.org/wiki/Q2940633"/>
	<skos:exactMatch rdf:resource="http://vocab.getty.edu/aat/300379687"/>
	<dcterms:created rdf:datatype="http://www.w3.org/2001/XMLSchema#date">2007-02-08</dcterms:created>
	<dcterms:modified rdf:datatype="http://www.w3.org/2001/XMLSchema#date">2024-11-15</dcterms:modified>
	<dcterms:identifier>27545</dcterms:identifier>
	<dcterms:contributor>blandine.nouvel</dcterms:contributor>
	<dcterms:contributor>justine.vincent</dcterms:contributor>
	<skos:definition xml:lang="fr">Aggloméré de vieux papyrus ou de tissus qui était utilisé par les Egyptiens pour fabriquer des enveloppes de momies solides et bon marché. (BiAA)</skos:definition>
	<skos:definition xml:lang="en">An agglomerate of old papyrus or cloth used by the Egyptians to make strong, cheap mummy wrappings. (BiAA)</skos:definition>
</rdf:Description>

<rdf:Description rdf:about="https://ark.frantiq.fr/ark:/26678/pcrtW8Uu5SMsQy">
	<rdf:type rdf:resource="http://www.w3.org/2004/02/skos/core#Concept"/>
	<skos:prefLabel xml:lang="de">Fell</skos:prefLabel>
	<skos:prefLabel xml:lang="en">hide</skos:prefLabel>
	<skos:prefLabel xml:lang="nl">huid</skos:prefLabel>
	<skos:prefLabel xml:lang="fr">peau</skos:prefLabel>
	<skos:prefLabel xml:lang="it">pelle</skos:prefLabel>
	<skos:prefLabel xml:lang="es">piel</skos:prefLabel>
	<skos:prefLabel xml:lang="ar">جلد</skos:prefLabel>
	<skos:altLabel xml:lang="en">skin</skos:altLabel>
	<skos:related rdf:resource="https://ark.frantiq.fr/ark:/26678/pcrtgb2sTfcBKy"/>
	<skos:related rdf:resource="https://ark.frantiq.fr/ark:/26678/pcrt4ySXFux6Td"/>
	<skos:related rdf:resource="https://ark.frantiq.fr/ark:/26678/pcrtnvdQmt8WEf"/>
	<skos:narrower rdf:resource="https://ark.frantiq.fr/ark:/26678/pcrtn5zR6bBN39"/>
	<skos:narrower rdf:resource="https://ark.frantiq.fr/ark:/26678/pcrtMt1immB5H5"/>
	<skos:broader rdf:resource="https://ark.frantiq.fr/ark:/26678/pcrtwvFLgSQRs5"/>
	<skos:inScheme rdf:resource="https://ark.frantiq.fr/ark:/26678/TH_1"/>
	<opentheso:memberOf rdf:resource="https://ark.frantiq.fr/ark:/26678/pcrtv66rn9cbv1"/>
	<opentheso:memberOf rdf:resource="https://ark.frantiq.fr/ark:/26678/pcrtnbDLi2FkAj"/>
	<skos:exactMatch rdf:resource="https://catalogue.bnf.fr/ark:/12148/cb11965434q"/>
	<skos:exactMatch rdf:resource="https://www.wikidata.org/wiki/Q1074"/>
	<skos:exactMatch rdf:resource="http://vocab.getty.edu/aat/300011840"/>
	<dcterms:created rdf:datatype="http://www.w3.org/2001/XMLSchema#date">2007-02-08</dcterms:created>
	<dcterms:modified rdf:datatype="http://www.w3.org/2001/XMLSchema#date">2024-11-15</dcterms:modified>
	<dcterms:identifier>27549</dcterms:identifier>
	<dcterms:contributor>blandine.nouvel</dcterms:contributor>
	<dcterms:contributor>justine.vincent</dcterms:contributor>
	<skos:definition xml:lang="en">The outer covering of the body of vertebrate animals, consisting of a deep part (the dermis) and a superficial layer (the epidermis). (Le Robert)</skos:definition>
	<skos:definition xml:lang="fr">Enveloppe extérieure du corps des animaux vertébrés, constituée par une partie profonde (le derme) et par une couche superficielle (l'épiderme). (Le Robert)</skos:definition>
	<skos:historyNote xml:lang="fr">2024-11-15 : modification de la définition.</skos:historyNote>
</rdf:Description>

<rdf:Description rdf:about="https://ark.frantiq.fr/ark:/26678/pcrtf97bQHDGEd">
	<rdf:type rdf:resource="http://www.w3.org/2004/02/skos/core#Concept"/>
	<skos:prefLabel xml:lang="en">animal bones and teeth</skos:prefLabel>
	<skos:prefLabel xml:lang="de">Knochengewinnung</skos:prefLabel>
	<skos:prefLabel xml:lang="it">materia dura animale</skos:prefLabel>
	<skos:prefLabel xml:lang="es">materia dura de origen animal</skos:prefLabel>
	<skos:prefLabel xml:lang="fr">matière dure animale</skos:prefLabel>
	<skos:prefLabel xml:lang="nl">verzameling van beenderen</skos:prefLabel>
	<skos:prefLabel xml:lang="ar">(جمع (عظم</skos:prefLabel>
	<skos:related rdf:resource="https://ark.frantiq.fr/ark:/26678/pcrtvKH7mF2Oas"/>
	<skos:narrower rdf:resource="https://ark.frantiq.fr/ark:/26678/pcrtmmQBSGulBN"/>
	<skos:narrower rdf:resource="https://ark.frantiq.fr/ark:/26678/pcrtknhh7n1sa3"/>
	<skos:narrower rdf:resource="https://ark.frantiq.fr/ark:/26678/pcrtU6YoUalie6"/>
	<skos:narrower rdf:resource="https://ark.frantiq.fr/ark:/26678/pcrt1zVFrqhSh2"/>
	<skos:narrower rdf:resource="https://ark.frantiq.fr/ark:/26678/pcrt448yYmVDuT"/>
	<skos:narrower rdf:resource="https://ark.frantiq.fr/ark:/26678/pcrt4dfh8e5Dpz"/>
	<skos:narrower rdf:resource="https://ark.frantiq.fr/ark:/26678/pcrtMj9v33qudS"/>
	<skos:narrower rdf:resource="https://ark.frantiq.fr/ark:/26678/pcrtmoM3SzhDcB"/>
	<skos:narrower rdf:resource="https://ark.frantiq.fr/ark:/26678/pcrtAoNmnP9BYF"/>
	<skos:broader rdf:resource="https://ark.frantiq.fr/ark:/26678/pcrtwvFLgSQRs5"/>
	<skos:inScheme rdf:resource="https://ark.frantiq.fr/ark:/26678/TH_1"/>
	<opentheso:memberOf rdf:resource="https://ark.frantiq.fr/ark:/26678/pcrtv66rn9cbv1"/>
	<opentheso:memberOf rdf:resource="https://ark.frantiq.fr/ark:/26678/pcrtnbDLi2FkAj"/>
	<dcterms:created rdf:datatype="http://www.w3.org/2001/XMLSchema#date">2007-06-06</dcterms:created>
	<dcterms:modified rdf:datatype="http://www.w3.org/2001/XMLSchema#date">2023-08-02</dcterms:modified>
	<dcterms:identifier>27630</dcterms:identifier>
	<dcterms:contributor>blandine.nouvel</dcterms:contributor>
	<skos:definition xml:lang="en">All hard materials of animal origin (bone, antler, ivory, fossil test, shell, etc.) collected or acquired by man (E.David).</skos:definition>
	<skos:definition xml:lang="fr">Toutes matières dures d'origine animale (os, bois de cervidés, ivoire, test fossile, coquillage, etc.) collectées ou acquises par l'homme (E.David).</skos:definition>
</rdf:Description>

<rdf:Description rdf:about="https://ark.frantiq.fr/ark:/26678/pcrtXVZBob53by">
	<rdf:type rdf:resource="http://www.w3.org/2004/02/skos/core#Concept"/>
	<skos:prefLabel xml:lang="de">Rhyolit</skos:prefLabel>
	<skos:prefLabel xml:lang="fr">rhyolite</skos:prefLabel>
	<skos:prefLabel xml:lang="en">Rhyolite</skos:prefLabel>
	<skos:prefLabel xml:lang="es">riolita</skos:prefLabel>
	<skos:prefLabel xml:lang="it">riolite</skos:prefLabel>
	<skos:prefLabel xml:lang="nl">ryoliet</skos:prefLabel>
	<skos:prefLabel xml:lang="ar">ريوليت</skos:prefLabel>
	<skos:altLabel xml:lang="fr">rhyolithe</skos:altLabel>
	<skos:related rdf:resource="https://ark.frantiq.fr/ark:/26678/pcrtDnenSUMjFl"/>
	<skos:related rdf:resource="https://ark.frantiq.fr/ark:/26678/pcrtmxvuuXHSTS"/>
	<skos:broader rdf:resource="https://ark.frantiq.fr/ark:/26678/pcrt3PUAhlWubZ"/>
	<skos:inScheme rdf:resource="https://ark.frantiq.fr/ark:/26678/TH_1"/>
	<opentheso:memberOf rdf:resource="https://ark.frantiq.fr/ark:/26678/pcrtv66rn9cbv1"/>
	<opentheso:memberOf rdf:resource="https://ark.frantiq.fr/ark:/26678/pcrtnbDLi2FkAj"/>
	<skos:exactMatch rdf:resource="https://www.wikidata.org/wiki/Q190727"/>
	<skos:exactMatch rdf:resource="http://vocab.getty.edu/aat/300011211"/>
	<dcterms:created rdf:datatype="http://www.w3.org/2001/XMLSchema#date">2007-07-04</dcterms:created>
	<dcterms:modified rdf:datatype="http://www.w3.org/2001/XMLSchema#date">2025-01-30</dcterms:modified>
	<dcterms:identifier>27632</dcterms:identifier>
	<dcterms:contributor>blandine.nouvel</dcterms:contributor>
	<dcterms:contributor>justine.vincent</dcterms:contributor>
	<skos:definition xml:lang="en">Sedimentary volcanic rock rich in siliceous tests of radiolarians, red or green in colour (Fernandes, 2012).</skos:definition>
	<skos:definition xml:lang="ar">صخر بركاني غني بالسيليكا</skos:definition>
	<skos:definition xml:lang="fr">Roche volcanique sédimentaire riche en tests siliceux de radiolaires, de couleur rouge ou verte (Fernandes, 2012).</skos:definition>
	<skos:historyNote xml:lang="fr">2025-30-01 : modification de la définition.</skos:historyNote>
	<dcterms:source>https://doi-org.inshs.bib.cnrs.fr/10.4000/12zm5</dcterms:source>
</rdf:Description>

<rdf:Description rdf:about="https://ark.frantiq.fr/ark:/26678/pcrtfx2fwztQ8p">
	<rdf:type rdf:resource="http://www.w3.org/2004/02/skos/core#Concept"/>
	<skos:prefLabel xml:lang="es">toba</skos:prefLabel>
	<skos:prefLabel xml:lang="fr">tuf</skos:prefLabel>
	<skos:prefLabel xml:lang="en">tuff</skos:prefLabel>
	<skos:prefLabel xml:lang="de">Tuff</skos:prefLabel>
	<skos:prefLabel xml:lang="it">tufo</skos:prefLabel>
	<skos:prefLabel xml:lang="nl">tufsteen</skos:prefLabel>
	<skos:prefLabel xml:lang="ar">فُلَيس</skos:prefLabel>
	<skos:altLabel xml:lang="es">toba volcánica</skos:altLabel>
	<skos:altLabel xml:lang="en">tuffaceous sandstone</skos:altLabel>
	<skos:altLabel xml:lang="en">volcanic sandstone</skos:altLabel>
	<skos:related rdf:resource="https://ark.frantiq.fr/ark:/26678/pcrtkgSlgXZbNa"/>
	<skos:broader rdf:resource="https://ark.frantiq.fr/ark:/26678/pcrtm4r7mvsvrw"/>
	<skos:inScheme rdf:resource="https://ark.frantiq.fr/ark:/26678/TH_1"/>
	<opentheso:memberOf rdf:resource="https://ark.frantiq.fr/ark:/26678/pcrtv66rn9cbv1"/>
	<opentheso:memberOf rdf:resource="https://ark.frantiq.fr/ark:/26678/pcrtnbDLi2FkAj"/>
	<opentheso:memberOf rdf:resource="https://ark.frantiq.fr/ark:/26678/pcrtv0jq332vcq3gxt5m13d5"/>
	<skos:exactMatch rdf:resource="https://www.wikidata.org/wiki/Q484924"/>
	<skos:exactMatch rdf:resource="https://www.wikidata.org/wiki/Q565256"/>
	<skos:exactMatch rdf:resource="http://vocab.getty.edu/aat/300011264"/>
	<dcterms:created rdf:datatype="http://www.w3.org/2001/XMLSchema#date">2009-03-02</dcterms:created>
	<dcterms:modified rdf:datatype="http://www.w3.org/2001/XMLSchema#date">2024-03-21</dcterms:modified>
	<dcterms:identifier>28355</dcterms:identifier>
	<dcterms:contributor>blandine.nouvel</dcterms:contributor>
	<dcterms:contributor>irene.weis</dcterms:contributor>
	<skos:definition xml:lang="fr">Couche indurée que l'on rencontre dans des sols légers et à faible ou moyenne profondeur. Ces couches sont constituées de matériaux continus et cimentés, soit du carbonate de calcium pour le tuf calcaire, soit de l'oxyde de fer pour le tuf ferrugineux, soit de l'humus pour le tuf humique, soit des cendres volcaniques pour le tuf volcanique. (Lozet &amp;amp; Mathieu, Dictionnaire de Science du Sol. Ed. Technique et documentation Lavoisier)</skos:definition>
	<skos:scopeNote xml:lang="fr">Pour le tuf calcaire, utiliser  travertin .</skos:scopeNote>
</rdf:Description>

<rdf:Description rdf:about="https://ark.frantiq.fr/ark:/26678/pcrtSdKu9rjDHO">
	<rdf:type rdf:resource="http://www.w3.org/2004/02/skos/core#Concept"/>
	<skos:prefLabel xml:lang="it">biscotto</skos:prefLabel>
	<skos:prefLabel xml:lang="en">biscuit</skos:prefLabel>
	<skos:prefLabel xml:lang="fr">biscuit</skos:prefLabel>
	<skos:prefLabel xml:lang="nl">biscuit</skos:prefLabel>
	<skos:prefLabel xml:lang="de">Biskuitware</skos:prefLabel>
	<skos:prefLabel xml:lang="es">bizcocho</skos:prefLabel>
	<skos:prefLabel xml:lang="ar">بورسلان بِسكويت</skos:prefLabel>
	<skos:related rdf:resource="https://ark.frantiq.fr/ark:/26678/pcrtqHWkorsw9D"/>
	<skos:related rdf:resource="https://ark.frantiq.fr/ark:/26678/pcrtPEGVkSl8Hk"/>
	<skos:broader rdf:resource="https://ark.frantiq.fr/ark:/26678/pcrtfx4s0yvSLj"/>
	<skos:inScheme rdf:resource="https://ark.frantiq.fr/ark:/26678/TH_1"/>
	<opentheso:memberOf rdf:resource="https://ark.frantiq.fr/ark:/26678/pcrtv66rn9cbv1"/>
	<opentheso:memberOf rdf:resource="https://ark.frantiq.fr/ark:/26678/pcrtnbDLi2FkAj"/>
	<skos:exactMatch rdf:resource="https://catalogue.bnf.fr/ark:/12148/cb123123981"/>
	<skos:exactMatch rdf:resource="https://www.wikidata.org/wiki/Q804070"/>
	<dcterms:created rdf:datatype="http://www.w3.org/2001/XMLSchema#date">2009-03-02</dcterms:created>
	<dcterms:modified rdf:datatype="http://www.w3.org/2001/XMLSchema#date">2023-08-02</dcterms:modified>
	<dcterms:identifier>28356</dcterms:identifier>
	<dcterms:contributor>blandine.nouvel</dcterms:contributor>
	<skos:definition xml:lang="fr">Poterie cuite une première fois en vue de recevoir au cours d’une cuisson un revêtement de glaçure. On parle surtout de biscuit dans le cas de faïence et de porcelaine. Par extension peut désigner des poteries de même type, mais destinées à rester sans glaçure. (Balfet)</skos:definition>
</rdf:Description>

<rdf:Description rdf:about="https://ark.frantiq.fr/ark:/26678/pcrtd1cZp0yBER">
	<rdf:type rdf:resource="http://www.w3.org/2004/02/skos/core#Concept"/>
	<skos:prefLabel xml:lang="en">frit</skos:prefLabel>
	<skos:prefLabel xml:lang="nl">frit</skos:prefLabel>
	<skos:prefLabel xml:lang="es">frita</skos:prefLabel>
	<skos:prefLabel xml:lang="it">fritta</skos:prefLabel>
	<skos:prefLabel xml:lang="fr">fritte</skos:prefLabel>
	<skos:prefLabel xml:lang="de">Fritte</skos:prefLabel>
	<skos:prefLabel xml:lang="ar">مسحوق مُزَجَّج</skos:prefLabel>
	<skos:related rdf:resource="https://ark.frantiq.fr/ark:/26678/pcrtYUUgSfW5wk"/>
	<skos:related rdf:resource="https://ark.frantiq.fr/ark:/26678/pcrtTSjUc9rzm8"/>
	<skos:related rdf:resource="https://ark.frantiq.fr/ark:/26678/pcrtcc11bvc83q"/>
	<skos:broader rdf:resource="https://ark.frantiq.fr/ark:/26678/pcrtIMsuG0RWTs"/>
	<skos:inScheme rdf:resource="https://ark.frantiq.fr/ark:/26678/TH_1"/>
	<opentheso:memberOf rdf:resource="https://ark.frantiq.fr/ark:/26678/pcrtv66rn9cbv1"/>
	<opentheso:memberOf rdf:resource="https://ark.frantiq.fr/ark:/26678/pcrtnbDLi2FkAj"/>
	<skos:exactMatch rdf:resource="https://www.wikidata.org/wiki/Q383361"/>
	<skos:exactMatch rdf:resource="http://vocab.getty.edu/aat/300343495"/>
	<dcterms:created rdf:datatype="http://www.w3.org/2001/XMLSchema#date">2009-03-06</dcterms:created>
	<dcterms:modified rdf:datatype="http://www.w3.org/2001/XMLSchema#date">2024-03-20</dcterms:modified>
	<dcterms:identifier>28380</dcterms:identifier>
	<dcterms:contributor>blandine.nouvel</dcterms:contributor>
	<dcterms:contributor>justine.vincent</dcterms:contributor>
	<skos:definition xml:lang="fr">Matériau composé d'un mélange de sable et de matériaux réfractaires fondus à la chaleur mais pas entièrement vitrifiés, souvent utilisé dans la fabrication des glaçures et des émaux.</skos:definition>
	<skos:definition xml:lang="en">A material composed of a mixture of sand and refractory materials fused by heat but not entirely vitrified, often used in the manufacture of glazes and enamels.</skos:definition>
	<skos:definition xml:lang="ar">خليط من الرمل و القلى المصهورة يدخل في صناعة الزجاج و الخزف ـ المعجم المزدوج</skos:definition>
</rdf:Description>

<rdf:Description rdf:about="https://ark.frantiq.fr/ark:/26678/pcrt0HFzFNNK1N">
	<rdf:type rdf:resource="http://www.w3.org/2004/02/skos/core#Concept"/>
	<skos:prefLabel xml:lang="es">arena</skos:prefLabel>
	<skos:prefLabel xml:lang="it">sabbia</skos:prefLabel>
	<skos:prefLabel xml:lang="fr">sable</skos:prefLabel>
	<skos:prefLabel xml:lang="en">sand</skos:prefLabel>
	<skos:prefLabel xml:lang="de">Sand</skos:prefLabel>
	<skos:prefLabel xml:lang="nl">zand</skos:prefLabel>
	<skos:prefLabel xml:lang="ar">رمل</skos:prefLabel>
	<skos:related rdf:resource="https://ark.frantiq.fr/ark:/26678/pcrth13n5jt6nc"/>
	<skos:related rdf:resource="https://ark.frantiq.fr/ark:/26678/pcrtkvf403bvpk"/>
	<skos:broader rdf:resource="https://ark.frantiq.fr/ark:/26678/pcrt3PUAhlWubZ"/>
	<skos:inScheme rdf:resource="https://ark.frantiq.fr/ark:/26678/TH_1"/>
	<opentheso:memberOf rdf:resource="https://ark.frantiq.fr/ark:/26678/pcrtv66rn9cbv1"/>
	<opentheso:memberOf rdf:resource="https://ark.frantiq.fr/ark:/26678/pcrtnbDLi2FkAj"/>
	<skos:exactMatch rdf:resource="https://catalogue.bnf.fr/ark:/12148/cb11951122q"/>
	<skos:exactMatch rdf:resource="https://www.wikidata.org/wiki/Q34679"/>
	<skos:exactMatch rdf:resource="http://vocab.getty.edu/aat/300014341"/>
	<dcterms:created rdf:datatype="http://www.w3.org/2001/XMLSchema#date">2009-03-18</dcterms:created>
	<dcterms:modified rdf:datatype="http://www.w3.org/2001/XMLSchema#date">2025-01-30</dcterms:modified>
	<dcterms:identifier>28644</dcterms:identifier>
	<dcterms:contributor>blandine.nouvel</dcterms:contributor>
	<dcterms:contributor>justine.vincent</dcterms:contributor>
	<skos:definition xml:lang="en">Loose detrital sedimentary rock of various types with grains between 63 µm and 2 mm (Fernandes, 2012).</skos:definition>
	<skos:definition xml:lang="fr">Roche sédimentaire détritique meuble de natures diverses dont les grains sont compris entre 63 µm et 2 mm (Fernandes, 2012).</skos:definition>
	<dcterms:source>https://doi-org.inshs.bib.cnrs.fr/10.4000/12zm5</dcterms:source>
</rdf:Description>

<rdf:Description rdf:about="https://ark.frantiq.fr/ark:/26678/pcrtxGxOl1KuZz">
	<rdf:type rdf:resource="http://www.w3.org/2004/02/skos/core#Concept"/>
	<skos:prefLabel xml:lang="es">jabón</skos:prefLabel>
	<skos:prefLabel xml:lang="it">sapone</skos:prefLabel>
	<skos:prefLabel xml:lang="fr">savon</skos:prefLabel>
	<skos:prefLabel xml:lang="de">Seife</skos:prefLabel>
	<skos:prefLabel xml:lang="en">soap</skos:prefLabel>
	<skos:prefLabel xml:lang="nl">zeep</skos:prefLabel>
	<skos:prefLabel xml:lang="ar">صابون</skos:prefLabel>
	<skos:altLabel xml:lang="fr">pain de savon</skos:altLabel>
	<skos:broader rdf:resource="https://ark.frantiq.fr/ark:/26678/pcrtwvFLgSQRs5"/>
	<skos:inScheme rdf:resource="https://ark.frantiq.fr/ark:/26678/TH_1"/>
	<opentheso:memberOf rdf:resource="https://ark.frantiq.fr/ark:/26678/pcrtv66rn9cbv1"/>
	<opentheso:memberOf rdf:resource="https://ark.frantiq.fr/ark:/26678/pcrtnbDLi2FkAj"/>
	<skos:exactMatch rdf:resource="https://catalogue.bnf.fr/ark:/12148/cb119396082"/>
	<skos:exactMatch rdf:resource="https://www.wikidata.org/wiki/Q34396"/>
	<skos:exactMatch rdf:resource="http://vocab.getty.edu/aat/300014329"/>
	<dcterms:created rdf:datatype="http://www.w3.org/2001/XMLSchema#date">2014-12-15</dcterms:created>
	<dcterms:modified rdf:datatype="http://www.w3.org/2001/XMLSchema#date">2024-11-15</dcterms:modified>
	<dcterms:identifier>29781</dcterms:identifier>
	<dcterms:contributor>blandine.nouvel</dcterms:contributor>
	<dcterms:contributor>justine.vincent</dcterms:contributor>
	<skos:definition xml:lang="fr">Produit liquide ou solide composé de molécules amphiphiles obtenues par réaction chimique entre un corps gras et une base forte. (wikipedia)</skos:definition>
	<skos:definition xml:lang="en">Liquid or solid product composed of amphiphilic molecules obtained by chemical reaction between a fatty substance and a strong base (wikipedia).</skos:definition>
	<skos:historyNote xml:lang="fr">2024-11-15 : ajout d'une définition.</skos:historyNote>
</rdf:Description>

<rdf:Description rdf:about="https://ark.frantiq.fr/ark:/26678/pcrt5A1NAN3NE3">
	<rdf:type rdf:resource="http://www.w3.org/2004/02/skos/core#Concept"/>
	<skos:prefLabel xml:lang="de">Alaune</skos:prefLabel>
	<skos:prefLabel xml:lang="it">allume di potassio</skos:prefLabel>
	<skos:prefLabel xml:lang="nl">aluin</skos:prefLabel>
	<skos:prefLabel xml:lang="en">alum</skos:prefLabel>
	<skos:prefLabel xml:lang="es">alumbre</skos:prefLabel>
	<skos:prefLabel xml:lang="fr">alun</skos:prefLabel>
	<skos:prefLabel xml:lang="ar">الشبَّ</skos:prefLabel>
	<skos:altLabel xml:lang="fr">pierre d'alun</skos:altLabel>
	<skos:altLabel xml:lang="it">potassio-allume</skos:altLabel>
	<skos:related rdf:resource="https://ark.frantiq.fr/ark:/26678/pcrtXiL6nBw86Y"/>
	<skos:related rdf:resource="https://ark.frantiq.fr/ark:/26678/pcrtEYqI4kLNb3"/>
	<skos:broader rdf:resource="https://ark.frantiq.fr/ark:/26678/pcrty2mcsksa6s"/>
	<skos:inScheme rdf:resource="https://ark.frantiq.fr/ark:/26678/TH_1"/>
	<opentheso:memberOf rdf:resource="https://ark.frantiq.fr/ark:/26678/pcrtv66rn9cbv1"/>
	<opentheso:memberOf rdf:resource="https://ark.frantiq.fr/ark:/26678/pcrtnbDLi2FkAj"/>
	<skos:exactMatch rdf:resource="https://catalogue.bnf.fr/ark:/12148/cb12527843w"/>
	<skos:exactMatch rdf:resource="https://www.wikidata.org/wiki/Q190527"/>
	<skos:exactMatch rdf:resource="http://vocab.getty.edu/aat/300183621"/>
	<dcterms:created rdf:datatype="http://www.w3.org/2001/XMLSchema#date">2010-06-30</dcterms:created>
	<dcterms:modified rdf:datatype="http://www.w3.org/2001/XMLSchema#date">2024-11-18</dcterms:modified>
	<dcterms:identifier>35139</dcterms:identifier>
	<dcterms:contributor>blandine.nouvel</dcterms:contributor>
	<dcterms:contributor>justine.vincent</dcterms:contributor>
	<skos:definition xml:lang="en">Natural stone extracted from alunite mines (Syria), or from surface outcrops (Egypt, Bohemia and Saxony), or in volcanic areas (around Naples, Greece, Guadeloupe), used in medicine, dyeing and leatherwork (Wikipedia).</skos:definition>
	<skos:definition xml:lang="fr">Pierre naturelle extraite de mines d'alunites (Syrie), ou d'affleurements de surface (Égypte, Bohême et Saxe), ou dans des zones volcaniques (autour de Naples, Grèce, Guadeloupe), utilisé notamment en médecine, en teinturerie et peausserie. (Wikipedia)</skos:definition>
	<skos:historyNote xml:lang="fr">2024-11-18 : modification de la définition.</skos:historyNote>
</rdf:Description>

<rdf:Description rdf:about="https://ark.frantiq.fr/ark:/26678/pcrtgkVy7lK4lN">
	<rdf:type rdf:resource="http://www.w3.org/2004/02/skos/core#Concept"/>
	<skos:prefLabel xml:lang="de">Baumwolle</skos:prefLabel>
	<skos:prefLabel xml:lang="fr">coton</skos:prefLabel>
	<skos:prefLabel xml:lang="es">cotón</skos:prefLabel>
	<skos:prefLabel xml:lang="it">cotone</skos:prefLabel>
	<skos:prefLabel xml:lang="en">cotton</skos:prefLabel>
	<skos:prefLabel xml:lang="nl">katoen</skos:prefLabel>
	<skos:prefLabel xml:lang="ar">قُطن</skos:prefLabel>
	<skos:related rdf:resource="https://ark.frantiq.fr/ark:/26678/pcrtqGQOorLDxx"/>
	<skos:broader rdf:resource="https://ark.frantiq.fr/ark:/26678/crtiorG06KeFt"/>
	<skos:inScheme rdf:resource="https://ark.frantiq.fr/ark:/26678/TH_1"/>
	<opentheso:memberOf rdf:resource="https://ark.frantiq.fr/ark:/26678/pcrtv66rn9cbv1"/>
	<opentheso:memberOf rdf:resource="https://ark.frantiq.fr/ark:/26678/pcrtnbDLi2FkAj"/>
	<opentheso:memberOf rdf:resource="https://ark.frantiq.fr/ark:/26678/pcrtv0jq332vcq3gxt5m13d5"/>
	<skos:exactMatch rdf:resource="https://catalogue.bnf.fr/ark:/12148/cb11975914p"/>
	<skos:exactMatch rdf:resource="https://www.wikidata.org/wiki/Q11457"/>
	<skos:exactMatch rdf:resource="http://vocab.getty.edu/aat/300183670"/>
	<dcterms:created rdf:datatype="http://www.w3.org/2001/XMLSchema#date">2011-01-27</dcterms:created>
	<dcterms:modified rdf:datatype="http://www.w3.org/2001/XMLSchema#date">2024-11-15</dcterms:modified>
	<dcterms:identifier>35252</dcterms:identifier>
	<dcterms:contributor>blandine.nouvel</dcterms:contributor>
	<dcterms:contributor>justine.vincent</dcterms:contributor>
	<dcterms:contributor>patricia.moitrel</dcterms:contributor>
	<skos:definition xml:lang="fr">Fibre végétale qui entoure les graines des cotonniers « véritables » (Gossypium sp.), arbustes de la famille des Malvacées, constituée de cellulose presque pure et généralement transformée en fil qui est tissé pour fabriquer des tissus. (wp)</skos:definition>
	<skos:definition xml:lang="en">Plant fibre that surrounds the seeds of  true  cotton plants (Gossypium sp.), shrubs in the Malvaceae family, made up of almost pure cellulose and generally transformed into yarn that is woven to make fabrics. (wp)</skos:definition>
</rdf:Description>

<rdf:Description rdf:about="https://ark.frantiq.fr/ark:/26678/pcrt8brfm4pd4t">
	<rdf:type rdf:resource="http://www.w3.org/2004/02/skos/core#Concept"/>
	<skos:prefLabel xml:lang="fr">bois d'élan</skos:prefLabel>
	<skos:prefLabel xml:lang="en">elk antler</skos:prefLabel>
	<skos:related rdf:resource="https://ark.frantiq.fr/ark:/26678/pcrtlSEevAHx0F"/>
	<skos:broader rdf:resource="https://ark.frantiq.fr/ark:/26678/pcrtmmQBSGulBN"/>
	<skos:inScheme rdf:resource="https://ark.frantiq.fr/ark:/26678/TH_1"/>
	<opentheso:memberOf rdf:resource="https://ark.frantiq.fr/ark:/26678/pcrtv66rn9cbv1"/>
	<opentheso:memberOf rdf:resource="https://ark.frantiq.fr/ark:/26678/pcrtnbDLi2FkAj"/>
	<dcterms:created rdf:datatype="http://www.w3.org/2001/XMLSchema#date">2022-12-08</dcterms:created>
	<dcterms:modified rdf:datatype="http://www.w3.org/2001/XMLSchema#date">2022-12-08</dcterms:modified>
	<dcterms:identifier>353950</dcterms:identifier>
	<skos:definition xml:lang="en">Broad, flat antlers of the largest deer.</skos:definition>
	<skos:definition xml:lang="fr">Bois du plus grand des cervidés, larges et plats.</skos:definition>
</rdf:Description>

<rdf:Description rdf:about="https://ark.frantiq.fr/ark:/26678/pcrtjs2wjn65hq">
	<rdf:type rdf:resource="http://www.w3.org/2004/02/skos/core#Concept"/>
	<skos:prefLabel xml:lang="en">egg</skos:prefLabel>
	<skos:prefLabel xml:lang="de">Ei</skos:prefLabel>
	<skos:prefLabel xml:lang="es">huevo</skos:prefLabel>
	<skos:prefLabel xml:lang="fr">œuf</skos:prefLabel>
	<skos:prefLabel xml:lang="it">uovo</skos:prefLabel>
	<skos:prefLabel xml:lang="ar">بيضه</skos:prefLabel>
	<skos:hiddenLabel xml:lang="fr">oeuf</skos:hiddenLabel>
	<skos:altLabel xml:lang="ar">beyḍah</skos:altLabel>
	<skos:altLabel xml:lang="fr">ovum</skos:altLabel>
	<skos:related rdf:resource="https://ark.frantiq.fr/ark:/26678/pcrt7ySVpWQ2aW"/>
	<skos:broader rdf:resource="https://ark.frantiq.fr/ark:/26678/pcrtgcn5U8laUN"/>
	<skos:inScheme rdf:resource="https://ark.frantiq.fr/ark:/26678/TH_1"/>
	<opentheso:memberOf rdf:resource="https://ark.frantiq.fr/ark:/26678/pcrtv66rn9cbv1"/>
	<opentheso:memberOf rdf:resource="https://ark.frantiq.fr/ark:/26678/pcrtnbDLi2FkAj"/>
	<skos:exactMatch rdf:resource="https://www.wikidata.org/wiki/Q93189"/>
	<dcterms:created rdf:datatype="http://www.w3.org/2001/XMLSchema#date">2022-12-08</dcterms:created>
	<dcterms:modified rdf:datatype="http://www.w3.org/2001/XMLSchema#date">2024-03-20</dcterms:modified>
	<dcterms:identifier>353967</dcterms:identifier>
	<dcterms:contributor>justine.vincent</dcterms:contributor>
	<skos:definition xml:lang="fr">Corps arrondi et dur que produisent les femelles des ovipares, constitué d'une coquille calcaire renfermant le germe de l'embryon et les substances de réserve destinées à nourrir celui-ci pendant l'incubation, ces derniers pouvant constituer un aliment.</skos:definition>
	<skos:definition xml:lang="en">Hard, rounded body produced by oviparous females, consisting of a calcareous shell containing the embryo germ and the reserve substances intended to nourish the embryo during incubation, the latter possibly constituting food.</skos:definition>
</rdf:Description>

<rdf:Description rdf:about="https://ark.frantiq.fr/ark:/26678/pcrtqvm3ztp4h8">
	<rdf:type rdf:resource="http://www.w3.org/2004/02/skos/core#Concept"/>
	<skos:prefLabel xml:lang="de">Daune</skos:prefLabel>
	<skos:prefLabel xml:lang="nl">dons</skos:prefLabel>
	<skos:prefLabel xml:lang="fr">duvet (plumage)</skos:prefLabel>
	<skos:prefLabel xml:lang="en">fluff</skos:prefLabel>
	<skos:prefLabel xml:lang="it">piumino (zoologia)</skos:prefLabel>
	<skos:prefLabel xml:lang="es">plumón</skos:prefLabel>
	<skos:altLabel xml:lang="en">down feather</skos:altLabel>
	<skos:related rdf:resource="https://ark.frantiq.fr/ark:/26678/pcrtpwtt5txd4f"/>
	<skos:broader rdf:resource="https://ark.frantiq.fr/ark:/26678/pcrtwvFLgSQRs5"/>
	<skos:inScheme rdf:resource="https://ark.frantiq.fr/ark:/26678/TH_1"/>
	<opentheso:memberOf rdf:resource="https://ark.frantiq.fr/ark:/26678/pcrtv66rn9cbv1"/>
	<opentheso:memberOf rdf:resource="https://ark.frantiq.fr/ark:/26678/pcrtnbDLi2FkAj"/>
	<skos:exactMatch rdf:resource="https://www.wikidata.org/wiki/Q953515"/>
	<dcterms:created rdf:datatype="http://www.w3.org/2001/XMLSchema#date">2022-12-08</dcterms:created>
	<dcterms:modified rdf:datatype="http://www.w3.org/2001/XMLSchema#date">2022-12-09</dcterms:modified>
	<dcterms:identifier>353973</dcterms:identifier>
	<skos:definition xml:lang="en">Plumage made up of the light feathers of birds and the first feathers of chicks, used as a raw material to make clothing in particular.</skos:definition>
	<skos:definition xml:lang="fr">Plumage formé de plumes légères chez les oiseaux et premières plumes des poussins, utilisé comme matière première pour fabriquer notamment des vêtements.</skos:definition>
</rdf:Description>

<rdf:Description rdf:about="https://ark.frantiq.fr/ark:/26678/pcrt9c0c2gpn8g">
	<rdf:type rdf:resource="http://www.w3.org/2004/02/skos/core#Concept"/>
	<skos:prefLabel xml:lang="it">artiglio</skos:prefLabel>
	<skos:prefLabel xml:lang="en">claw</skos:prefLabel>
	<skos:prefLabel xml:lang="fr">griffe</skos:prefLabel>
	<skos:prefLabel xml:lang="de">Klaue</skos:prefLabel>
	<skos:prefLabel xml:lang="nl">klauw</skos:prefLabel>
	<skos:prefLabel xml:lang="es">uña larga y afilada</skos:prefLabel>
	<skos:prefLabel xml:lang="ar">مخلب</skos:prefLabel>
	<skos:altLabel xml:lang="fr">serre</skos:altLabel>
	<skos:broader rdf:resource="https://ark.frantiq.fr/ark:/26678/pcrtU6YoUalie6"/>
	<skos:inScheme rdf:resource="https://ark.frantiq.fr/ark:/26678/TH_1"/>
	<opentheso:memberOf rdf:resource="https://ark.frantiq.fr/ark:/26678/pcrtv66rn9cbv1"/>
	<opentheso:memberOf rdf:resource="https://ark.frantiq.fr/ark:/26678/pcrtnbDLi2FkAj"/>
	<skos:exactMatch rdf:resource="https://www.wikidata.org/wiki/Q217605"/>
	<dcterms:created rdf:datatype="http://www.w3.org/2001/XMLSchema#date">2022-12-08</dcterms:created>
	<dcterms:modified rdf:datatype="http://www.w3.org/2001/XMLSchema#date">2022-12-09</dcterms:modified>
	<dcterms:identifier>353976</dcterms:identifier>
	<skos:definition xml:lang="en">The pointed, curved nail of certain animals (mammals, birds, reptiles) used by humans as a tool or for adornment.</skos:definition>
	<skos:definition xml:lang="fr">&lt;p&gt;Ongle pointu et recourbé de certains animaux (mammifères, oiseaux, reptiles) que l'homme utilise comme outil ou élément de parure.&lt;/p&gt;</skos:definition>
</rdf:Description>

<rdf:Description rdf:about="https://ark.frantiq.fr/ark:/26678/pcrtzzdfgbqjgxghdgkrghbq">
	<rdf:type rdf:resource="http://www.w3.org/2004/02/skos/core#Concept"/>
	<skos:prefLabel xml:lang="es">molasa</skos:prefLabel>
	<skos:prefLabel xml:lang="it">molassa</skos:prefLabel>
	<skos:prefLabel xml:lang="en">molasse</skos:prefLabel>
	<skos:prefLabel xml:lang="fr">molasse</skos:prefLabel>
	<skos:prefLabel xml:lang="de">Molasse</skos:prefLabel>
	<skos:broader rdf:resource="https://ark.frantiq.fr/ark:/26678/pcrtRiKgPqvJQO"/>
	<skos:inScheme rdf:resource="https://ark.frantiq.fr/ark:/26678/TH_1"/>
	<opentheso:memberOf rdf:resource="https://ark.frantiq.fr/ark:/26678/pcrtv66rn9cbv1"/>
	<opentheso:memberOf rdf:resource="https://ark.frantiq.fr/ark:/26678/pcrtnbDLi2FkAj"/>
	<skos:exactMatch rdf:resource="https://www.wikidata.org/wiki/Q304080"/>
	<dcterms:created rdf:datatype="http://www.w3.org/2001/XMLSchema#date">2023-04-18</dcterms:created>
	<dcterms:modified rdf:datatype="http://www.w3.org/2001/XMLSchema#date">2023-04-19</dcterms:modified>
	<dcterms:identifier>354408</dcterms:identifier>
	<skos:definition xml:lang="fr">&lt;span style= color: rgb(77, 81, 86); &gt;Ensemble de roches sédimentaires, essentiellement détritiques, et post-orogéniques, s'accumulant dans un bassin d'avant-pays, en périphérie des chaînes de montagnes; peut être utilisé comme matériau de construction. (wikipedia)&lt;/span&gt;</skos:definition>
</rdf:Description>

<rdf:Description rdf:about="https://ark.frantiq.fr/ark:/26678/pcrt3344f5f89w8bjkpfp2zz">
	<rdf:type rdf:resource="http://www.w3.org/2004/02/skos/core#Concept"/>
	<skos:prefLabel xml:lang="es">piroclasto</skos:prefLabel>
	<skos:prefLabel xml:lang="de">Pyroklast</skos:prefLabel>
	<skos:prefLabel xml:lang="it">tefra</skos:prefLabel>
	<skos:prefLabel xml:lang="en">tephra</skos:prefLabel>
	<skos:prefLabel xml:lang="fr">téphra</skos:prefLabel>
	<skos:altLabel xml:lang="fr">ejecta</skos:altLabel>
	<skos:broader rdf:resource="https://ark.frantiq.fr/ark:/26678/pcrtDhZmKFAlZa"/>
	<skos:inScheme rdf:resource="https://ark.frantiq.fr/ark:/26678/TH_1"/>
	<opentheso:memberOf rdf:resource="https://ark.frantiq.fr/ark:/26678/pcrtv66rn9cbv1"/>
	<skos:exactMatch rdf:resource="https://www.wikidata.org/wiki/Q209245"/>
	<dcterms:created rdf:datatype="http://www.w3.org/2001/XMLSchema#date">2023-11-10</dcterms:created>
	<dcterms:modified rdf:datatype="http://www.w3.org/2001/XMLSchema#date">2023-11-28</dcterms:modified>
	<dcterms:identifier>354562</dcterms:identifier>
	<dcterms:creator>justine.vincent</dcterms:creator>
	<dcterms:contributor>blandine.nouvel</dcterms:contributor>
	<dcterms:contributor>justine.vincent</dcterms:contributor>
	<skos:definition xml:lang="en">A collection of solid and liquid matter from magma and volcanic vent rocks, carried along by gases and ejected with them during volcanic eruptions (Foucault and Raoult, Dictionnaire de géologie, 1980), used as a stratigraphic marker in archaeology.</skos:definition>
	<skos:definition xml:lang="fr">&lt;p&gt;Ensemble des matières solides et liquides provenant du magma et des roches de la cheminée volcanique, entraînées par les gaz et éjectées avec eux lors des éruptions volcaniques (Foucault et Raoult, Dictionnaire de géologie, 1980), utilisé comme marqueur stratigraphique en archéologie.&lt;/p&gt;</skos:definition>
</rdf:Description>

<rdf:Description rdf:about="https://ark.frantiq.fr/ark:/26678/pcrtSHAq8xiG3F">
	<rdf:type rdf:resource="http://www.w3.org/2004/02/skos/core#Concept"/>
	<skos:prefLabel xml:lang="nl">druipsteen</skos:prefLabel>
	<skos:prefLabel xml:lang="es">espeleotema</skos:prefLabel>
	<skos:prefLabel xml:lang="de">Speläothem</skos:prefLabel>
	<skos:prefLabel xml:lang="it">speleotema</skos:prefLabel>
	<skos:prefLabel xml:lang="en">speleothem</skos:prefLabel>
	<skos:prefLabel xml:lang="fr">spéléothème</skos:prefLabel>
	<skos:prefLabel xml:lang="ar">التوضعات الكلسية المتحجرة</skos:prefLabel>
	<skos:altLabel xml:lang="fr">concrétion</skos:altLabel>
	<skos:related rdf:resource="https://ark.frantiq.fr/ark:/26678/pcrtxKnfzXYMxK"/>
	<skos:broader rdf:resource="https://ark.frantiq.fr/ark:/26678/pcrtr5vk7w9vdz"/>
	<skos:inScheme rdf:resource="https://ark.frantiq.fr/ark:/26678/TH_1"/>
	<opentheso:memberOf rdf:resource="https://ark.frantiq.fr/ark:/26678/pcrtv66rn9cbv1"/>
	<opentheso:memberOf rdf:resource="https://ark.frantiq.fr/ark:/26678/pcrtnbDLi2FkAj"/>
	<skos:exactMatch rdf:resource="https://www.wikidata.org/wiki/Q154507"/>
	<skos:exactMatch rdf:resource="http://vocab.getty.edu/aat/300380015"/>
	<dcterms:created rdf:datatype="http://www.w3.org/2001/XMLSchema#date">2011-02-25</dcterms:created>
	<dcterms:modified rdf:datatype="http://www.w3.org/2001/XMLSchema#date">2023-08-02</dcterms:modified>
	<dcterms:identifier>35457</dcterms:identifier>
	<dcterms:contributor>blandine.nouvel</dcterms:contributor>
	<skos:definition xml:lang="en">Mineral deposit precipitated in a natural underground cavity (cave, chasm, etc.). (WP)</skos:definition>
	<skos:definition xml:lang="fr">Dépôt minéral précipité dans une cavité naturelle souterraine (grotte, gouffre, ..). (WP)</skos:definition>
</rdf:Description>

<rdf:Description rdf:about="https://ark.frantiq.fr/ark:/26678/pcrtwWYB6o5QwM">
	<rdf:type rdf:resource="http://www.w3.org/2004/02/skos/core#Concept"/>
	<skos:prefLabel xml:lang="nl">Libisch glas</skos:prefLabel>
	<skos:prefLabel xml:lang="en">Libyan desert glass</skos:prefLabel>
	<skos:prefLabel xml:lang="de">Libysches Wüstenglas</skos:prefLabel>
	<skos:prefLabel xml:lang="fr">verre libyque</skos:prefLabel>
	<skos:prefLabel xml:lang="it">vetro del deserto libico</skos:prefLabel>
	<skos:prefLabel xml:lang="es">vidrio líbico</skos:prefLabel>
	<skos:prefLabel xml:lang="ar">زجاج طبيعي</skos:prefLabel>
	<skos:altLabel xml:lang="en">Great Sand Sea glass</skos:altLabel>
	<skos:broader rdf:resource="https://ark.frantiq.fr/ark:/26678/pcrt4N9jrETRto"/>
	<skos:inScheme rdf:resource="https://ark.frantiq.fr/ark:/26678/TH_1"/>
	<opentheso:memberOf rdf:resource="https://ark.frantiq.fr/ark:/26678/pcrtv66rn9cbv1"/>
	<opentheso:memberOf rdf:resource="https://ark.frantiq.fr/ark:/26678/pcrtnbDLi2FkAj"/>
	<skos:exactMatch rdf:resource="https://www.wikidata.org/wiki/Q1778748"/>
	<dcterms:created rdf:datatype="http://www.w3.org/2001/XMLSchema#date">2011-02-25</dcterms:created>
	<dcterms:modified rdf:datatype="http://www.w3.org/2001/XMLSchema#date">2023-08-02</dcterms:modified>
	<dcterms:identifier>35461</dcterms:identifier>
	<dcterms:contributor>blandine.nouvel</dcterms:contributor>
	<skos:definition xml:lang="ar">زجاج طبيعي يعثر عليه في صحراء ليبيا</skos:definition>
	<skos:definition xml:lang="fr">Sorte de verre naturel présent sur 6 500 km² du désert Libyque dont l'origine pourrait être liée à l'impact d'une comète (Wikipédia).</skos:definition>
</rdf:Description>

<rdf:Description rdf:about="https://ark.frantiq.fr/ark:/26678/pcrtp201sc1d5bd93jj7mm27">
	<rdf:type rdf:resource="http://www.w3.org/2004/02/skos/core#Concept"/>
	<skos:prefLabel xml:lang="fr">antimoine</skos:prefLabel>
	<skos:prefLabel xml:lang="de">Antimon (gediegen)</skos:prefLabel>
	<skos:prefLabel xml:lang="it">antimonio nativo</skos:prefLabel>
	<skos:prefLabel xml:lang="es">Antimonio nativo</skos:prefLabel>
	<skos:prefLabel xml:lang="en">antimony (native)</skos:prefLabel>
	<skos:prefLabel xml:lang="nl">antimoon</skos:prefLabel>
	<skos:prefLabel xml:lang="ar">إثمد</skos:prefLabel>
	<skos:altLabel xml:lang="fr">antimoine natif</skos:altLabel>
	<skos:broader rdf:resource="https://ark.frantiq.fr/ark:/26678/pcrty2mcsksa6s"/>
	<skos:inScheme rdf:resource="https://ark.frantiq.fr/ark:/26678/TH_1"/>
	<opentheso:memberOf rdf:resource="https://ark.frantiq.fr/ark:/26678/pcrtv66rn9cbv1"/>
	<opentheso:memberOf rdf:resource="https://ark.frantiq.fr/ark:/26678/pcrtv0jq332vcq3gxt5m13d5"/>
	<skos:exactMatch rdf:resource="https://www.wikidata.org/wiki/Q1134295"/>
	<dcterms:created rdf:datatype="http://www.w3.org/2001/XMLSchema#date">2024-06-03</dcterms:created>
	<dcterms:modified rdf:datatype="http://www.w3.org/2001/XMLSchema#date">2024-06-04</dcterms:modified>
	<dcterms:identifier>354698</dcterms:identifier>
	<dcterms:creator>patricia.moitrel</dcterms:creator>
	<dcterms:contributor>blandine.nouvel</dcterms:contributor>
	<dcterms:contributor>patricia.moitrel</dcterms:contributor>
	<skos:definition xml:lang="fr">Corps simple, solide (symbole Sb) d'un blanc argenté et bleuâtre, cristallin, très fragile, ni malléable, ni ductile, présentant à la fois des propriétés de métal et de métalloïde, et entrant dans la composition de nombreux alliages et de préparations pharmaceutiques  (TLFI / Trésor de la langue française informatisé).</skos:definition>
	<skos:definition xml:lang="en">&lt;p&gt;Simple solid body (symbol Sb), silvery-white and bluish, crystalline, very brittle, neither malleable nor ductile, having both metal and metalloid properties, and used in the composition of many alloys and pharmaceutical preparations  (TLFI / Trésor de la langue française informatisé).&lt;/p&gt;</skos:definition>
</rdf:Description>

<rdf:Description rdf:about="https://ark.frantiq.fr/ark:/26678/pcrtbxntxs7hfz99qvswk8k1">
	<rdf:type rdf:resource="http://www.w3.org/2004/02/skos/core#Concept"/>
	<skos:prefLabel xml:lang="it">dolomia</skos:prefLabel>
	<skos:prefLabel xml:lang="es">dolomía</skos:prefLabel>
	<skos:prefLabel xml:lang="fr">dolomie</skos:prefLabel>
	<skos:prefLabel xml:lang="de">Dolomit (Gestein)</skos:prefLabel>
	<skos:prefLabel xml:lang="nl">dolosteen</skos:prefLabel>
	<skos:prefLabel xml:lang="en">dolostone</skos:prefLabel>
	<skos:related rdf:resource="https://ark.frantiq.fr/ark:/26678/pcrtk5md9510q7"/>
	<skos:broader rdf:resource="https://ark.frantiq.fr/ark:/26678/pcrtm4r7mvsvrw"/>
	<skos:inScheme rdf:resource="https://ark.frantiq.fr/ark:/26678/TH_1"/>
	<opentheso:memberOf rdf:resource="https://ark.frantiq.fr/ark:/26678/pcrtv66rn9cbv1"/>
	<skos:exactMatch rdf:resource="https://www.wikidata.org/wiki/Q1134814"/>
	<dcterms:created rdf:datatype="http://www.w3.org/2001/XMLSchema#date">2024-06-25</dcterms:created>
	<dcterms:modified rdf:datatype="http://www.w3.org/2001/XMLSchema#date">2024-06-25</dcterms:modified>
	<dcterms:identifier>354718</dcterms:identifier>
	<dcterms:creator>aurelie.devillechaise-Gmail</dcterms:creator>
	<dcterms:contributor>blandine.nouvel</dcterms:contributor>
	<skos:definition xml:lang="fr">&lt;p&gt;Roche sédimentaire carbonatée composée d'au moins 50% de dolomite, qui cristallise en prismes losangiques (Wikipédia).&lt;/p&gt;</skos:definition>
</rdf:Description>

<rdf:Description rdf:about="https://ark.frantiq.fr/ark:/26678/pcrtsr9r0hqdgqcdmw5mds91">
	<rdf:type rdf:resource="http://www.w3.org/2004/02/skos/core#Concept"/>
	<skos:prefLabel xml:lang="fr">poudingue</skos:prefLabel>
	<skos:prefLabel xml:lang="nl">puddingsteen</skos:prefLabel>
	<skos:prefLabel xml:lang="de">Puddingstein</skos:prefLabel>
	<skos:prefLabel xml:lang="en">pudding stone</skos:prefLabel>
	<skos:prefLabel xml:lang="es">pudinga</skos:prefLabel>
	<skos:broader rdf:resource="https://ark.frantiq.fr/ark:/26678/pcrtRiKgPqvJQO"/>
	<skos:inScheme rdf:resource="https://ark.frantiq.fr/ark:/26678/TH_1"/>
	<opentheso:memberOf rdf:resource="https://ark.frantiq.fr/ark:/26678/pcrtv66rn9cbv1"/>
	<skos:exactMatch rdf:resource="https://www.wikidata.org/wiki/Q262815"/>
	<dcterms:created rdf:datatype="http://www.w3.org/2001/XMLSchema#date">2024-06-25</dcterms:created>
	<dcterms:modified rdf:datatype="http://www.w3.org/2001/XMLSchema#date">2024-06-25</dcterms:modified>
	<dcterms:identifier>354719</dcterms:identifier>
	<dcterms:creator>aurelie.devillechaise-Gmail</dcterms:creator>
	<dcterms:contributor>blandine.nouvel</dcterms:contributor>
	<skos:definition xml:lang="fr">Roche sédimentaire détritique consolidée, faisant partie des conglomérats, &lt;span style= color: rgb(32, 33, 34); &gt;constituée de débris arrondis, qui sont d'anciens&amp;amp;nbsp;galets ayant subi un transport sur une certaine distance dans des rivières ou sur un littoral (Wikipédia).&lt;/span&gt;</skos:definition>
</rdf:Description>

<rdf:Description rdf:about="https://ark.frantiq.fr/ark:/26678/pcrtvhmknj8n0n92z5x2xqqk">
	<rdf:type rdf:resource="http://www.w3.org/2004/02/skos/core#Concept"/>
	<skos:prefLabel xml:lang="en">breccia</skos:prefLabel>
	<skos:prefLabel xml:lang="it">breccia</skos:prefLabel>
	<skos:prefLabel xml:lang="nl">breccie</skos:prefLabel>
	<skos:prefLabel xml:lang="es">brecha</skos:prefLabel>
	<skos:prefLabel xml:lang="fr">brèche (roche)</skos:prefLabel>
	<skos:prefLabel xml:lang="de">Brekzie</skos:prefLabel>
	<skos:prefLabel xml:lang="ar">مدملكات</skos:prefLabel>
	<skos:related rdf:resource="https://ark.frantiq.fr/ark:/26678/pcrtq764j7snt5"/>
	<skos:broader rdf:resource="https://ark.frantiq.fr/ark:/26678/pcrtRiKgPqvJQO"/>
	<skos:inScheme rdf:resource="https://ark.frantiq.fr/ark:/26678/TH_1"/>
	<opentheso:memberOf rdf:resource="https://ark.frantiq.fr/ark:/26678/pcrtv66rn9cbv1"/>
	<skos:exactMatch rdf:resource="https://www.wikidata.org/wiki/Q191250"/>
	<skos:exactMatch rdf:resource="http://vocab.getty.edu/page/aat/300011425"/>
	<dcterms:created rdf:datatype="http://www.w3.org/2001/XMLSchema#date">2024-06-25</dcterms:created>
	<dcterms:modified rdf:datatype="http://www.w3.org/2001/XMLSchema#date">2024-07-02</dcterms:modified>
	<dcterms:identifier>354720</dcterms:identifier>
	<dcterms:creator>aurelie.devillechaise-Gmail</dcterms:creator>
	<dcterms:contributor>blandine.nouvel</dcterms:contributor>
	<dcterms:contributor>patricia.moitrel</dcterms:contributor>
	<skos:definition xml:lang="fr">Roche sédimentaire détritique consolidée, faisant partie des conglomérats, constituée de débris anguleux unis par un ciment naturel.</skos:definition>
	<skos:definition xml:lang="en">Consolidated detritic sedimentary rock, part of the conglomerates, made up of angular debris united by a natural cement.</skos:definition>
</rdf:Description>

<rdf:Description rdf:about="https://ark.frantiq.fr/ark:/26678/pcrttk3hqkx8s7049j925sxn">
	<rdf:type rdf:resource="http://www.w3.org/2004/02/skos/core#Concept"/>
	<skos:prefLabel xml:lang="nl">beton</skos:prefLabel>
	<skos:prefLabel xml:lang="de">Beton</skos:prefLabel>
	<skos:prefLabel xml:lang="fr">béton de ciment</skos:prefLabel>
	<skos:prefLabel xml:lang="it">calcestruzzo</skos:prefLabel>
	<skos:prefLabel xml:lang="en">concrete</skos:prefLabel>
	<skos:prefLabel xml:lang="es">concreto</skos:prefLabel>
	<skos:prefLabel xml:lang="ar">خرسانة</skos:prefLabel>
	<skos:altLabel xml:lang="fr">béton</skos:altLabel>
	<skos:broader rdf:resource="https://ark.frantiq.fr/ark:/26678/pcrtEWWJvOVoh5"/>
	<skos:inScheme rdf:resource="https://ark.frantiq.fr/ark:/26678/TH_1"/>
	<opentheso:memberOf rdf:resource="https://ark.frantiq.fr/ark:/26678/pcrtv66rn9cbv1"/>
	<opentheso:memberOf rdf:resource="https://ark.frantiq.fr/ark:/26678/pcrtv0jq332vcq3gxt5m13d5"/>
	<skos:exactMatch rdf:resource="https://www.wikidata.org/wiki/Q22657"/>
	<dcterms:created rdf:datatype="http://www.w3.org/2001/XMLSchema#date">2024-10-25</dcterms:created>
	<dcterms:modified rdf:datatype="http://www.w3.org/2001/XMLSchema#date">2024-11-26</dcterms:modified>
	<dcterms:identifier>354849</dcterms:identifier>
	<dcterms:creator>patricia.moitrel</dcterms:creator>
	<dcterms:contributor>blandine.nouvel</dcterms:contributor>
	<dcterms:contributor>patricia.moitrel</dcterms:contributor>
	<skos:definition xml:lang="fr">Mélange de ciment, de granulats, d'eau et d'adjuvants.</skos:definition>
</rdf:Description>

<rdf:Description rdf:about="https://ark.frantiq.fr/ark:/26678/pcrtb4mt1w9s876tsx2cxf61">
	<rdf:type rdf:resource="http://www.w3.org/2004/02/skos/core#Concept"/>
	<skos:prefLabel xml:lang="en">monolith</skos:prefLabel>
	<skos:prefLabel xml:lang="de">Monolith</skos:prefLabel>
	<skos:prefLabel xml:lang="fr">monolithe</skos:prefLabel>
	<skos:prefLabel xml:lang="es">monolito</skos:prefLabel>
	<skos:prefLabel xml:lang="it">monolito</skos:prefLabel>
	<skos:prefLabel xml:lang="ar">مونوليث</skos:prefLabel>
	<skos:broader rdf:resource="https://ark.frantiq.fr/ark:/26678/pcrtSVdwKcS3MI"/>
	<skos:inScheme rdf:resource="https://ark.frantiq.fr/ark:/26678/TH_1"/>
	<opentheso:memberOf rdf:resource="https://ark.frantiq.fr/ark:/26678/pcrtv66rn9cbv1"/>
	<opentheso:memberOf rdf:resource="https://ark.frantiq.fr/ark:/26678/pcrtv0jq332vcq3gxt5m13d5"/>
	<skos:exactMatch rdf:resource="https://www.wikidata.org/wiki/Q653208"/>
	<dcterms:created rdf:datatype="http://www.w3.org/2001/XMLSchema#date">2024-10-29</dcterms:created>
	<dcterms:modified rdf:datatype="http://www.w3.org/2001/XMLSchema#date">2024-12-03</dcterms:modified>
	<dcterms:identifier>354852</dcterms:identifier>
	<dcterms:creator>justine.vincent</dcterms:creator>
	<dcterms:contributor>justine.vincent</dcterms:contributor>
	<dcterms:contributor>patricia.moitrel</dcterms:contributor>
	<skos:definition xml:lang="fr">Bloc de pierre de grande dimension constitué d'un seul élément, ou élément de construction taillé dans un unique bloc de pierre.</skos:definition>
	<skos:definition xml:lang="en">A large block of stone consisting of a single element, or a building element cut from a single block of stone.</skos:definition>
</rdf:Description>

<rdf:Description rdf:about="https://ark.frantiq.fr/ark:/26678/pcrtB8FNASjQrB">
	<rdf:type rdf:resource="http://www.w3.org/2004/02/skos/core#Concept"/>
	<skos:prefLabel xml:lang="fr">argile blanche</skos:prefLabel>
	<skos:prefLabel xml:lang="es">caolinita</skos:prefLabel>
	<skos:prefLabel xml:lang="it">caolinite</skos:prefLabel>
	<skos:prefLabel xml:lang="nl">kaolin</skos:prefLabel>
	<skos:prefLabel xml:lang="de">Kaolinit</skos:prefLabel>
	<skos:prefLabel xml:lang="en">kaolinite</skos:prefLabel>
	<skos:prefLabel xml:lang="ar">صلصال أبيض</skos:prefLabel>
	<skos:altLabel xml:lang="fr">kaolin</skos:altLabel>
	<skos:altLabel xml:lang="fr">kaolinite</skos:altLabel>
	<skos:broader rdf:resource="https://ark.frantiq.fr/ark:/26678/pcrto44p1SaKFn"/>
	<skos:inScheme rdf:resource="https://ark.frantiq.fr/ark:/26678/TH_1"/>
	<opentheso:memberOf rdf:resource="https://ark.frantiq.fr/ark:/26678/pcrtv66rn9cbv1"/>
	<opentheso:memberOf rdf:resource="https://ark.frantiq.fr/ark:/26678/pcrtnbDLi2FkAj"/>
	<skos:exactMatch rdf:resource="https://catalogue.bnf.fr/ark:/12148/cb16708810n"/>
	<skos:exactMatch rdf:resource="https://www.wikidata.org/wiki/Q223197"/>
	<skos:exactMatch rdf:resource="http://vocab.getty.edu/aat/300010445"/>
	<skos:exactMatch rdf:resource="http://vocab.getty.edu/aat/300013815"/>
	<dcterms:created rdf:datatype="http://www.w3.org/2001/XMLSchema#date">2012-06-08</dcterms:created>
	<dcterms:modified rdf:datatype="http://www.w3.org/2001/XMLSchema#date">2023-08-02</dcterms:modified>
	<dcterms:identifier>35660</dcterms:identifier>
	<dcterms:contributor>blandine.nouvel</dcterms:contributor>
</rdf:Description>

<rdf:Description rdf:about="https://ark.frantiq.fr/ark:/26678/pcrtskMRAe4usI">
	<rdf:type rdf:resource="http://www.w3.org/2004/02/skos/core#Concept"/>
	<skos:prefLabel xml:lang="es">arcilla refractaria</skos:prefLabel>
	<skos:prefLabel xml:lang="fr">argile réfractaire</skos:prefLabel>
	<skos:prefLabel xml:lang="it">argilla refrattaria</skos:prefLabel>
	<skos:prefLabel xml:lang="en">refractory clay</skos:prefLabel>
	<skos:prefLabel xml:lang="de">Schamott</skos:prefLabel>
	<skos:prefLabel xml:lang="nl">vuurvaste klei</skos:prefLabel>
	<skos:prefLabel xml:lang="ar">صلصال مقاوم للحرارة </skos:prefLabel>
	<skos:broader rdf:resource="https://ark.frantiq.fr/ark:/26678/pcrto44p1SaKFn"/>
	<skos:inScheme rdf:resource="https://ark.frantiq.fr/ark:/26678/TH_1"/>
	<opentheso:memberOf rdf:resource="https://ark.frantiq.fr/ark:/26678/pcrtv66rn9cbv1"/>
	<opentheso:memberOf rdf:resource="https://ark.frantiq.fr/ark:/26678/pcrtnbDLi2FkAj"/>
	<skos:exactMatch rdf:resource="https://www.wikidata.org/wiki/Q2523928"/>
	<skos:exactMatch rdf:resource="http://vocab.getty.edu/aat/300010457"/>
	<dcterms:created rdf:datatype="http://www.w3.org/2001/XMLSchema#date">2012-06-08</dcterms:created>
	<dcterms:modified rdf:datatype="http://www.w3.org/2001/XMLSchema#date">2023-08-02</dcterms:modified>
	<dcterms:identifier>35661</dcterms:identifier>
	<dcterms:contributor>blandine.nouvel</dcterms:contributor>
	<skos:definition xml:lang="fr">Argile qui résiste à des températures de 1 600 à 1 700° et davantage et où il entre du calcaire, du fer oxydé, du fer sulfuré. (CNRTL)</skos:definition>
</rdf:Description>

<rdf:Description rdf:about="https://ark.frantiq.fr/ark:/26678/pcrtpNOweZVSSH">
	<rdf:type rdf:resource="http://www.w3.org/2004/02/skos/core#Concept"/>
	<skos:prefLabel xml:lang="es">feldespato</skos:prefLabel>
	<skos:prefLabel xml:lang="en">feldspars</skos:prefLabel>
	<skos:prefLabel xml:lang="de">Feldspat</skos:prefLabel>
	<skos:prefLabel xml:lang="fr">feldspath</skos:prefLabel>
	<skos:prefLabel xml:lang="it">feldspato</skos:prefLabel>
	<skos:prefLabel xml:lang="nl">veldspaat</skos:prefLabel>
	<skos:prefLabel xml:lang="ar">فلدسبات</skos:prefLabel>
	<skos:altLabel xml:lang="ar">صُفَّاح الحقول</skos:altLabel>
	<skos:broader rdf:resource="https://ark.frantiq.fr/ark:/26678/pcrty2mcsksa6s"/>
	<skos:inScheme rdf:resource="https://ark.frantiq.fr/ark:/26678/TH_1"/>
	<opentheso:memberOf rdf:resource="https://ark.frantiq.fr/ark:/26678/pcrtv66rn9cbv1"/>
	<opentheso:memberOf rdf:resource="https://ark.frantiq.fr/ark:/26678/pcrtnbDLi2FkAj"/>
	<skos:exactMatch rdf:resource="https://catalogue.bnf.fr/ark:/12148/cb11971186c"/>
	<skos:exactMatch rdf:resource="https://www.wikidata.org/wiki/Q170258"/>
	<skos:exactMatch rdf:resource="http://vocab.getty.edu/aat/300011087"/>
	<dcterms:created rdf:datatype="http://www.w3.org/2001/XMLSchema#date">2012-06-15</dcterms:created>
	<dcterms:modified rdf:datatype="http://www.w3.org/2001/XMLSchema#date">2024-11-18</dcterms:modified>
	<dcterms:identifier>35688</dcterms:identifier>
	<dcterms:contributor>blandine.nouvel</dcterms:contributor>
	<dcterms:contributor>justine.vincent</dcterms:contributor>
	<skos:definition xml:lang="en">Mineral of the tectosilicate family, very common in magmatic rocks. (Raoult and Foucault, 2005)</skos:definition>
	<skos:definition xml:lang="fr">Minéral de la famille des tectosilicates, très fréquent dans les roches magmatiques. (Raoult et Foucault, 2005)</skos:definition>
</rdf:Description>

<rdf:Description rdf:about="https://ark.frantiq.fr/ark:/26678/pcrtp0jS51rXL1">
	<rdf:type rdf:resource="http://www.w3.org/2004/02/skos/core#Concept"/>
	<skos:prefLabel xml:lang="es">galio</skos:prefLabel>
	<skos:prefLabel xml:lang="it">gallio</skos:prefLabel>
	<skos:prefLabel xml:lang="en">gallium</skos:prefLabel>
	<skos:prefLabel xml:lang="fr">gallium</skos:prefLabel>
	<skos:prefLabel xml:lang="nl">gallium</skos:prefLabel>
	<skos:prefLabel xml:lang="de">Gallium</skos:prefLabel>
	<skos:prefLabel xml:lang="ar">غاليوم</skos:prefLabel>
	<skos:altLabel xml:lang="ar">فِلِز نادر أبيض مُزرق</skos:altLabel>
	<skos:broader rdf:resource="https://ark.frantiq.fr/ark:/26678/pcrtkn1hAXHveS"/>
	<skos:inScheme rdf:resource="https://ark.frantiq.fr/ark:/26678/TH_1"/>
	<opentheso:memberOf rdf:resource="https://ark.frantiq.fr/ark:/26678/pcrtv66rn9cbv1"/>
	<opentheso:memberOf rdf:resource="https://ark.frantiq.fr/ark:/26678/pcrtnbDLi2FkAj"/>
	<skos:exactMatch rdf:resource="https://catalogue.bnf.fr/ark:/12148/cb11955437j"/>
	<skos:exactMatch rdf:resource="https://www.wikidata.org/wiki/Q861"/>
	<dcterms:created rdf:datatype="http://www.w3.org/2001/XMLSchema#date">2012-06-19</dcterms:created>
	<dcterms:modified rdf:datatype="http://www.w3.org/2001/XMLSchema#date">2023-08-02</dcterms:modified>
	<dcterms:identifier>35698</dcterms:identifier>
	<dcterms:contributor>blandine.nouvel</dcterms:contributor>
	<skos:definition xml:lang="en">A rare single metallic body very similar to zinc, used in particular in thermometers for very high temperatures. (TLFi)</skos:definition>
	<skos:definition xml:lang="fr">Corps simple métallique, rare, présentant beaucoup d'analogie avec le zinc, utilisé notamment dans les thermomètres pour de très hautes températures. (TLFi)</skos:definition>
</rdf:Description>

<rdf:Description rdf:about="https://ark.frantiq.fr/ark:/26678/pcrtsTcJvHR17f">
	<rdf:type rdf:resource="http://www.w3.org/2004/02/skos/core#Concept"/>
	<skos:prefLabel xml:lang="nl">alkaliglazuur</skos:prefLabel>
	<skos:prefLabel xml:lang="en">alkaline glaze</skos:prefLabel>
	<skos:prefLabel xml:lang="es">barniz alcalino</skos:prefLabel>
	<skos:prefLabel xml:lang="fr">glaçure alcaline</skos:prefLabel>
	<skos:prefLabel xml:lang="de">Laugenglasur</skos:prefLabel>
	<skos:prefLabel xml:lang="it">vetrina alcalina</skos:prefLabel>
	<skos:prefLabel xml:lang="ar">تزجيج قلوي</skos:prefLabel>
	<skos:altLabel xml:lang="es">vidriado alcalino</skos:altLabel>
	<skos:broader rdf:resource="https://ark.frantiq.fr/ark:/26678/pcrt3pmFUqt27w"/>
	<skos:inScheme rdf:resource="https://ark.frantiq.fr/ark:/26678/TH_1"/>
	<opentheso:memberOf rdf:resource="https://ark.frantiq.fr/ark:/26678/pcrtv66rn9cbv1"/>
	<opentheso:memberOf rdf:resource="https://ark.frantiq.fr/ark:/26678/pcrtnbDLi2FkAj"/>
	<skos:exactMatch rdf:resource="https://www.wikidata.org/wiki/Q111686681"/>
	<dcterms:created rdf:datatype="http://www.w3.org/2001/XMLSchema#date">2012-06-19</dcterms:created>
	<dcterms:modified rdf:datatype="http://www.w3.org/2001/XMLSchema#date">2023-08-02</dcterms:modified>
	<dcterms:identifier>35699</dcterms:identifier>
	<dcterms:contributor>blandine.nouvel</dcterms:contributor>
	<skos:definition xml:lang="en">Glaze with sodium, potassium or lithium salts.</skos:definition>
	<skos:definition xml:lang="fr">Glaçure aux sels de sodium, de potassium ou de lithium.</skos:definition>
</rdf:Description>

<rdf:Description rdf:about="https://ark.frantiq.fr/ark:/26678/pcrtjzpz0bA7Mx">
	<rdf:type rdf:resource="http://www.w3.org/2004/02/skos/core#Concept"/>
	<skos:prefLabel xml:lang="es">barniz al manganeso</skos:prefLabel>
	<skos:prefLabel xml:lang="fr">glaçure au manganèse</skos:prefLabel>
	<skos:prefLabel xml:lang="nl">mangaanglazuur</skos:prefLabel>
	<skos:prefLabel xml:lang="en">manganese glaze</skos:prefLabel>
	<skos:prefLabel xml:lang="de">Manganglasur</skos:prefLabel>
	<skos:prefLabel xml:lang="it">vetrina al manganese</skos:prefLabel>
	<skos:prefLabel xml:lang="ar">تزجيج بالمنغنيز</skos:prefLabel>
	<skos:altLabel xml:lang="es">esmalte al manganeso</skos:altLabel>
	<skos:altLabel xml:lang="en">manganese dioxide glaze</skos:altLabel>
	<skos:related rdf:resource="https://ark.frantiq.fr/ark:/26678/pcrtKASHLmba7X"/>
	<skos:broader rdf:resource="https://ark.frantiq.fr/ark:/26678/pcrt3pmFUqt27w"/>
	<skos:inScheme rdf:resource="https://ark.frantiq.fr/ark:/26678/TH_1"/>
	<opentheso:memberOf rdf:resource="https://ark.frantiq.fr/ark:/26678/pcrtv66rn9cbv1"/>
	<opentheso:memberOf rdf:resource="https://ark.frantiq.fr/ark:/26678/pcrtnbDLi2FkAj"/>
	<dcterms:created rdf:datatype="http://www.w3.org/2001/XMLSchema#date">2012-06-19</dcterms:created>
	<dcterms:modified rdf:datatype="http://www.w3.org/2001/XMLSchema#date">2023-08-02</dcterms:modified>
	<dcterms:identifier>35700</dcterms:identifier>
	<dcterms:contributor>blandine.nouvel</dcterms:contributor>
	<skos:definition xml:lang="en">Glaze containing ferro-manganic compounds.</skos:definition>
	<skos:definition xml:lang="fr">Glaçure comportant des composés ferro-manganiques.</skos:definition>
</rdf:Description>

<rdf:Description rdf:about="https://ark.frantiq.fr/ark:/26678/pcrtL9hSYO73pS">
	<rdf:type rdf:resource="http://www.w3.org/2004/02/skos/core#Concept"/>
	<skos:prefLabel xml:lang="es">esmalte salino</skos:prefLabel>
	<skos:prefLabel xml:lang="fr">glaçure salifère</skos:prefLabel>
	<skos:prefLabel xml:lang="en">salt glaze</skos:prefLabel>
	<skos:prefLabel xml:lang="de">Salzglasur</skos:prefLabel>
	<skos:prefLabel xml:lang="it">vetrina salifera</skos:prefLabel>
	<skos:prefLabel xml:lang="nl">zouthoudende glazuur</skos:prefLabel>
	<skos:prefLabel xml:lang="ar">تزجيج ملحي</skos:prefLabel>
	<skos:altLabel xml:lang="es">esmalte a la sal</skos:altLabel>
	<skos:altLabel xml:lang="fr">glaçure au sel</skos:altLabel>
	<skos:altLabel xml:lang="en">salt-glaze</skos:altLabel>
	<skos:broader rdf:resource="https://ark.frantiq.fr/ark:/26678/pcrt3pmFUqt27w"/>
	<skos:inScheme rdf:resource="https://ark.frantiq.fr/ark:/26678/TH_1"/>
	<opentheso:memberOf rdf:resource="https://ark.frantiq.fr/ark:/26678/pcrtv66rn9cbv1"/>
	<opentheso:memberOf rdf:resource="https://ark.frantiq.fr/ark:/26678/pcrtnbDLi2FkAj"/>
	<skos:exactMatch rdf:resource="https://www.wikidata.org/wiki/Q2159609"/>
	<skos:exactMatch rdf:resource="http://vocab.getty.edu/aat/300048635"/>
	<dcterms:created rdf:datatype="http://www.w3.org/2001/XMLSchema#date">2012-06-19</dcterms:created>
	<dcterms:modified rdf:datatype="http://www.w3.org/2001/XMLSchema#date">2023-08-02</dcterms:modified>
	<dcterms:identifier>35701</dcterms:identifier>
	<dcterms:contributor>blandine.nouvel</dcterms:contributor>
	<skos:definition xml:lang="en">Glaze created by adding salt or soda to the ceramic during the firing process.</skos:definition>
	<skos:definition xml:lang="fr">Glaçure créée créé en ajoutant du sel ou de la soude à la céramique pendant le processus de cuisson.</skos:definition>
</rdf:Description>

<rdf:Description rdf:about="https://ark.frantiq.fr/ark:/26678/pcrt5SnWt4iSF2">
	<rdf:type rdf:resource="http://www.w3.org/2004/02/skos/core#Concept"/>
	<skos:prefLabel xml:lang="es">barniz al estaño</skos:prefLabel>
	<skos:prefLabel xml:lang="fr">glaçure stannifère</skos:prefLabel>
	<skos:prefLabel xml:lang="en">tin-glaze</skos:prefLabel>
	<skos:prefLabel xml:lang="nl">tinhoudende glazuur</skos:prefLabel>
	<skos:prefLabel xml:lang="it">vetrina stannifera</skos:prefLabel>
	<skos:prefLabel xml:lang="de">Zinnglasur</skos:prefLabel>
	<skos:prefLabel xml:lang="ar">تزجيج قصديري</skos:prefLabel>
	<skos:altLabel xml:lang="es">esmalte estannífero</skos:altLabel>
	<skos:altLabel xml:lang="fr">glaçure de faïence</skos:altLabel>
	<skos:altLabel xml:lang="fr">glaçure stannique</skos:altLabel>
	<skos:broader rdf:resource="https://ark.frantiq.fr/ark:/26678/pcrt3pmFUqt27w"/>
	<skos:inScheme rdf:resource="https://ark.frantiq.fr/ark:/26678/TH_1"/>
	<opentheso:memberOf rdf:resource="https://ark.frantiq.fr/ark:/26678/pcrtv66rn9cbv1"/>
	<opentheso:memberOf rdf:resource="https://ark.frantiq.fr/ark:/26678/pcrtnbDLi2FkAj"/>
	<skos:exactMatch rdf:resource="https://www.wikidata.org/wiki/Q104418745"/>
	<dcterms:created rdf:datatype="http://www.w3.org/2001/XMLSchema#date">2012-06-19</dcterms:created>
	<dcterms:modified rdf:datatype="http://www.w3.org/2001/XMLSchema#date">2023-08-02</dcterms:modified>
	<dcterms:identifier>35702</dcterms:identifier>
	<dcterms:contributor>blandine.nouvel</dcterms:contributor>
	<skos:definition xml:lang="en">Opaque glaze obtained by using tin or tin oxide as a flux or opacifier (D'Anna et al.).</skos:definition>
	<skos:definition xml:lang="fr">Glaçure opaque obtenue en utilisant de l'étain ou de l'oxyde d'étain comme fondant ou opacifiant (D'Anna et al.)</skos:definition>
</rdf:Description>

<rdf:Description rdf:about="https://ark.frantiq.fr/ark:/26678/pcrt2ozTOWS5f0">
	<rdf:type rdf:resource="http://www.w3.org/2004/02/skos/core#Concept"/>
	<skos:prefLabel xml:lang="es">barniz de plomo</skos:prefLabel>
	<skos:prefLabel xml:lang="de">Bleiglasur</skos:prefLabel>
	<skos:prefLabel xml:lang="fr">glaçure plombifère</skos:prefLabel>
	<skos:prefLabel xml:lang="en">lead-glaze</skos:prefLabel>
	<skos:prefLabel xml:lang="nl">loodhoudende glazuur</skos:prefLabel>
	<skos:prefLabel xml:lang="it">vetrina piombifera</skos:prefLabel>
	<skos:prefLabel xml:lang="ar">تزجيج رصاصي</skos:prefLabel>
	<skos:altLabel xml:lang="es">esmalte plúmbeo</skos:altLabel>
	<skos:related rdf:resource="https://ark.frantiq.fr/ark:/26678/pcrt0oF1Z1HbOE"/>
	<skos:related rdf:resource="https://ark.frantiq.fr/ark:/26678/pcrtEpGlZykUTy"/>
	<skos:broader rdf:resource="https://ark.frantiq.fr/ark:/26678/pcrt3pmFUqt27w"/>
	<skos:inScheme rdf:resource="https://ark.frantiq.fr/ark:/26678/TH_1"/>
	<opentheso:memberOf rdf:resource="https://ark.frantiq.fr/ark:/26678/pcrtv66rn9cbv1"/>
	<opentheso:memberOf rdf:resource="https://ark.frantiq.fr/ark:/26678/pcrtnbDLi2FkAj"/>
	<skos:exactMatch rdf:resource="https://www.wikidata.org/wiki/Q63346318"/>
	<skos:exactMatch rdf:resource="http://vocab.getty.edu/aat/300233430"/>
	<dcterms:created rdf:datatype="http://www.w3.org/2001/XMLSchema#date">2012-06-19</dcterms:created>
	<dcterms:modified rdf:datatype="http://www.w3.org/2001/XMLSchema#date">2023-08-02</dcterms:modified>
	<dcterms:identifier>35703</dcterms:identifier>
	<dcterms:contributor>blandine.nouvel</dcterms:contributor>
	<skos:definition xml:lang="en">Lead-based glaze.</skos:definition>
	<skos:definition xml:lang="fr">Glaçure à base de plomb.</skos:definition>
</rdf:Description>

<rdf:Description rdf:about="https://ark.frantiq.fr/ark:/26678/pcrt9lQWQXyMXK">
	<rdf:type rdf:resource="http://www.w3.org/2004/02/skos/core#Concept"/>
	<skos:prefLabel xml:lang="it">arenaria renania</skos:prefLabel>
	<skos:prefLabel xml:lang="es">arenisca rética</skos:prefLabel>
	<skos:prefLabel xml:lang="fr">grès rhénan</skos:prefLabel>
	<skos:prefLabel xml:lang="en">Rhaetian sandstone</skos:prefLabel>
	<skos:prefLabel xml:lang="de">Rheinisches Steingut</skos:prefLabel>
	<skos:prefLabel xml:lang="nl">steengoed uit het Rijnland</skos:prefLabel>
	<skos:prefLabel xml:lang="ar">صَلصال رايني</skos:prefLabel>
	<skos:altLabel xml:lang="fr">grès allemand</skos:altLabel>
	<skos:broader rdf:resource="https://ark.frantiq.fr/ark:/26678/pcrtt7G9pnQlu1"/>
	<skos:inScheme rdf:resource="https://ark.frantiq.fr/ark:/26678/TH_1"/>
	<opentheso:memberOf rdf:resource="https://ark.frantiq.fr/ark:/26678/pcrtv66rn9cbv1"/>
	<opentheso:memberOf rdf:resource="https://ark.frantiq.fr/ark:/26678/pcrtnbDLi2FkAj"/>
	<skos:exactMatch rdf:resource="https://www.wikidata.org/wiki/Q90563901"/>
	<dcterms:created rdf:datatype="http://www.w3.org/2001/XMLSchema#date">2012-06-19</dcterms:created>
	<dcterms:modified rdf:datatype="http://www.w3.org/2001/XMLSchema#date">2023-08-02</dcterms:modified>
	<dcterms:identifier>35707</dcterms:identifier>
	<dcterms:contributor>blandine.nouvel</dcterms:contributor>
	<skos:definition xml:lang="en">Ceramic material from the Rhine Graben region (wikidata)</skos:definition>
	<skos:definition xml:lang="fr">Matériau céramique provenant de la région du fossé rhénan. (wikidata)</skos:definition>
</rdf:Description>

<rdf:Description rdf:about="https://ark.frantiq.fr/ark:/26678/pcrtIq9NE61BMc">
	<rdf:type rdf:resource="http://www.w3.org/2004/02/skos/core#Concept"/>
	<skos:prefLabel xml:lang="it">arenaria azzurra</skos:prefLabel>
	<skos:prefLabel xml:lang="es">arenisca azul</skos:prefLabel>
	<skos:prefLabel xml:lang="nl">azuren steengoed</skos:prefLabel>
	<skos:prefLabel xml:lang="de">blau glasiertes Steingut</skos:prefLabel>
	<skos:prefLabel xml:lang="en">blue sandstone</skos:prefLabel>
	<skos:prefLabel xml:lang="fr">grès azuré</skos:prefLabel>
	<skos:prefLabel xml:lang="ar">صَلصال آزوري</skos:prefLabel>
	<skos:broader rdf:resource="https://ark.frantiq.fr/ark:/26678/pcrtt7G9pnQlu1"/>
	<skos:inScheme rdf:resource="https://ark.frantiq.fr/ark:/26678/TH_1"/>
	<opentheso:memberOf rdf:resource="https://ark.frantiq.fr/ark:/26678/pcrtv66rn9cbv1"/>
	<opentheso:memberOf rdf:resource="https://ark.frantiq.fr/ark:/26678/pcrtnbDLi2FkAj"/>
	<skos:exactMatch rdf:resource="https://www.wikidata.org/wiki/Q90565196"/>
	<dcterms:created rdf:datatype="http://www.w3.org/2001/XMLSchema#date">2012-06-19</dcterms:created>
	<dcterms:modified rdf:datatype="http://www.w3.org/2001/XMLSchema#date">2024-10-18</dcterms:modified>
	<dcterms:identifier>35708</dcterms:identifier>
	<dcterms:contributor>blandine.nouvel</dcterms:contributor>
	<dcterms:contributor>justine.vincent</dcterms:contributor>
	<skos:definition xml:lang="en">Ceramic material with a blue glaze (from wikidata)</skos:definition>
	<skos:definition xml:lang="fr">Matériau céramique recouvert d'un vernis bleu. (d'après wikidata)</skos:definition>
</rdf:Description>

<rdf:Description rdf:about="https://ark.frantiq.fr/ark:/26678/pcrtKASHLmba7X">
	<rdf:type rdf:resource="http://www.w3.org/2004/02/skos/core#Concept"/>
	<skos:prefLabel xml:lang="nl">mangaan</skos:prefLabel>
	<skos:prefLabel xml:lang="de">Mangan</skos:prefLabel>
	<skos:prefLabel xml:lang="en">manganese</skos:prefLabel>
	<skos:prefLabel xml:lang="it">manganese</skos:prefLabel>
	<skos:prefLabel xml:lang="fr">manganèse</skos:prefLabel>
	<skos:prefLabel xml:lang="es">manganeso</skos:prefLabel>
	<skos:prefLabel xml:lang="ar">منغنيز</skos:prefLabel>
	<skos:altLabel xml:lang="ar">معدن شديد الصلابة</skos:altLabel>
	<skos:related rdf:resource="https://ark.frantiq.fr/ark:/26678/pcrtjzpz0bA7Mx"/>
	<skos:broader rdf:resource="https://ark.frantiq.fr/ark:/26678/pcrtkn1hAXHveS"/>
	<skos:inScheme rdf:resource="https://ark.frantiq.fr/ark:/26678/TH_1"/>
	<opentheso:memberOf rdf:resource="https://ark.frantiq.fr/ark:/26678/pcrtv66rn9cbv1"/>
	<opentheso:memberOf rdf:resource="https://ark.frantiq.fr/ark:/26678/pcrtnbDLi2FkAj"/>
	<opentheso:memberOf rdf:resource="https://ark.frantiq.fr/ark:/26678/pcrtv0jq332vcq3gxt5m13d5"/>
	<skos:exactMatch rdf:resource="https://catalogue.bnf.fr/ark:/12148/cb11938451d"/>
	<skos:exactMatch rdf:resource="https://www.wikidata.org/wiki/Q731"/>
	<skos:exactMatch rdf:resource="http://vocab.getty.edu/aat/300011025"/>
	<dcterms:created rdf:datatype="http://www.w3.org/2001/XMLSchema#date">2012-06-20</dcterms:created>
	<dcterms:modified rdf:datatype="http://www.w3.org/2001/XMLSchema#date">2024-12-04</dcterms:modified>
	<dcterms:identifier>35717</dcterms:identifier>
	<dcterms:contributor>blandine.nouvel</dcterms:contributor>
	<dcterms:contributor>irene.weis</dcterms:contributor>
	<dcterms:contributor>justine.vincent</dcterms:contributor>
	<skos:definition xml:lang="en">Grey-white transition metal that resembles iron.</skos:definition>
	<skos:definition xml:lang="fr">Métal de transition gris-blanc qui ressemble au fer.</skos:definition>
</rdf:Description>

<rdf:Description rdf:about="https://ark.frantiq.fr/ark:/26678/pcrt7kSfnJElvj">
	<rdf:type rdf:resource="http://www.w3.org/2004/02/skos/core#Concept"/>
	<skos:prefLabel xml:lang="nl">menie</skos:prefLabel>
	<skos:prefLabel xml:lang="es">minio</skos:prefLabel>
	<skos:prefLabel xml:lang="it">minio</skos:prefLabel>
	<skos:prefLabel xml:lang="en">minium</skos:prefLabel>
	<skos:prefLabel xml:lang="fr">minium</skos:prefLabel>
	<skos:prefLabel xml:lang="de">Minium</skos:prefLabel>
	<skos:prefLabel xml:lang="ar">زِنجَفَر</skos:prefLabel>
	<skos:related rdf:resource="https://ark.frantiq.fr/ark:/26678/pcrtHv6zSSHk9H"/>
	<skos:broader rdf:resource="https://ark.frantiq.fr/ark:/26678/pcrtGzQPnntJa1"/>
	<skos:inScheme rdf:resource="https://ark.frantiq.fr/ark:/26678/TH_1"/>
	<opentheso:memberOf rdf:resource="https://ark.frantiq.fr/ark:/26678/pcrtv66rn9cbv1"/>
	<opentheso:memberOf rdf:resource="https://ark.frantiq.fr/ark:/26678/pcrtnbDLi2FkAj"/>
	<skos:exactMatch rdf:resource="https://www.wikidata.org/wiki/Q408757"/>
	<skos:exactMatch rdf:resource="http://vocab.getty.edu/aat/300311178"/>
	<dcterms:created rdf:datatype="http://www.w3.org/2001/XMLSchema#date">2012-06-20</dcterms:created>
	<dcterms:modified rdf:datatype="http://www.w3.org/2001/XMLSchema#date">2024-10-18</dcterms:modified>
	<dcterms:identifier>35720</dcterms:identifier>
	<dcterms:contributor>blandine.nouvel</dcterms:contributor>
	<dcterms:contributor>justine.vincent</dcterms:contributor>
	<skos:definition xml:lang="fr">Pigment rouge à rouge orangé constitué par un oxyde de plomb. (cnrtl)</skos:definition>
	<skos:definition xml:lang="en">Red to orange-red lead oxide pigment (cnrtl)</skos:definition>
	<skos:definition xml:lang="ar">أكسيد الرصاص الأحمر ـ المعجم المزدوج</skos:definition>
</rdf:Description>

<rdf:Description rdf:about="https://ark.frantiq.fr/ark:/26678/pcrtjSXU4udrfP">
	<rdf:type rdf:resource="http://www.w3.org/2004/02/skos/core#Concept"/>
	<skos:prefLabel xml:lang="nl">pegmatiet</skos:prefLabel>
	<skos:prefLabel xml:lang="de">Pegmatit</skos:prefLabel>
	<skos:prefLabel xml:lang="es">pegmatita</skos:prefLabel>
	<skos:prefLabel xml:lang="en">pegmatite</skos:prefLabel>
	<skos:prefLabel xml:lang="fr">pegmatite</skos:prefLabel>
	<skos:prefLabel xml:lang="it">pegmatite</skos:prefLabel>
	<skos:prefLabel xml:lang="ar">بغماتيت</skos:prefLabel>
	<skos:broader rdf:resource="https://ark.frantiq.fr/ark:/26678/pcrtmxvuuXHSTS"/>
	<skos:inScheme rdf:resource="https://ark.frantiq.fr/ark:/26678/TH_1"/>
	<opentheso:memberOf rdf:resource="https://ark.frantiq.fr/ark:/26678/pcrtv66rn9cbv1"/>
	<opentheso:memberOf rdf:resource="https://ark.frantiq.fr/ark:/26678/pcrtnbDLi2FkAj"/>
	<skos:exactMatch rdf:resource="https://www.wikidata.org/wiki/Q105630"/>
	<skos:exactMatch rdf:resource="http://vocab.getty.edu/aat/300011187"/>
	<dcterms:created rdf:datatype="http://www.w3.org/2001/XMLSchema#date">2012-06-29</dcterms:created>
	<dcterms:modified rdf:datatype="http://www.w3.org/2001/XMLSchema#date">2024-11-14</dcterms:modified>
	<dcterms:identifier>35735</dcterms:identifier>
	<dcterms:contributor>blandine.nouvel</dcterms:contributor>
	<dcterms:contributor>justine.vincent</dcterms:contributor>
	<skos:definition xml:lang="en">deep quartzite magmatic rock of the granite family formed of quartz and alkaline feldspars, which differs from granite by a structure of gigantic crystals, from 1 cm to sometimes more than 1 m. (Lozet &amp;amp; Mathieu, Dictionnaire de science du sol. Ed. Technique et Documentation Lavoisier)</skos:definition>
	<skos:definition xml:lang="ar">صخر ذو بلورات كبيرة</skos:definition>
	<skos:definition xml:lang="fr">roche magmatique quartzitique de profondeur de la famille du granite formée de quartz et de feldspaths alcalins, qui diffère du granite par une structure à cristaux gigantesques, de 1 cm à parfois plus d'1 m. (Lozet &amp;amp; Mathieu, Dictionnaire de science du sol. Ed. Technique et Documentation Lavoisier)</skos:definition>
</rdf:Description>

<rdf:Description rdf:about="https://ark.frantiq.fr/ark:/26678/pcrterNa8OcooH">
	<rdf:type rdf:resource="http://www.w3.org/2004/02/skos/core#Concept"/>
	<skos:prefLabel xml:lang="it">bianco di piombo</skos:prefLabel>
	<skos:prefLabel xml:lang="es">blanco de plomo</skos:prefLabel>
	<skos:prefLabel xml:lang="de">Bleiweiß</skos:prefLabel>
	<skos:prefLabel xml:lang="fr">céruse</skos:prefLabel>
	<skos:prefLabel xml:lang="nl">loodwit</skos:prefLabel>
	<skos:prefLabel xml:lang="en">white lead</skos:prefLabel>
	<skos:prefLabel xml:lang="ar">إسبيداج</skos:prefLabel>
	<skos:altLabel xml:lang="es">albayalde</skos:altLabel>
	<skos:altLabel xml:lang="it">biacca</skos:altLabel>
	<skos:altLabel xml:lang="fr">blanc d'argent</skos:altLabel>
	<skos:altLabel xml:lang="fr">blanc de plomb</skos:altLabel>
	<skos:altLabel xml:lang="fr">blanc de Saturne</skos:altLabel>
	<skos:altLabel xml:lang="en">hydrocerussite</skos:altLabel>
	<skos:related rdf:resource="https://ark.frantiq.fr/ark:/26678/pcrtTrvqZaQ5Bt"/>
	<skos:related rdf:resource="https://ark.frantiq.fr/ark:/26678/pcrtZFMkWp7vRA"/>
	<skos:broader rdf:resource="https://ark.frantiq.fr/ark:/26678/pcrtGzQPnntJa1"/>
	<skos:inScheme rdf:resource="https://ark.frantiq.fr/ark:/26678/TH_1"/>
	<opentheso:memberOf rdf:resource="https://ark.frantiq.fr/ark:/26678/pcrtv66rn9cbv1"/>
	<opentheso:memberOf rdf:resource="https://ark.frantiq.fr/ark:/26678/pcrtnbDLi2FkAj"/>
	<skos:exactMatch rdf:resource="https://www.wikidata.org/wiki/Q656004"/>
	<skos:exactMatch rdf:resource="http://vocab.getty.edu/aat/300013754"/>
	<dcterms:created rdf:datatype="http://www.w3.org/2001/XMLSchema#date">2012-06-29</dcterms:created>
	<dcterms:modified rdf:datatype="http://www.w3.org/2001/XMLSchema#date">2024-10-18</dcterms:modified>
	<dcterms:identifier>35740</dcterms:identifier>
	<dcterms:contributor>blandine.nouvel</dcterms:contributor>
	<dcterms:contributor>justine.vincent</dcterms:contributor>
	<skos:definition xml:lang="fr">Carbonate de plomb et plus particulièrement substance blanche fabriquée à partir de carbonate de plomb, utilisée surtout en peinture et autrefois comme fard, mais dont l'emploi est interdit depuis le début du XXe siècle, à cause de sa toxicité (cnrtl)</skos:definition>
	<skos:definition xml:lang="en">Lead carbonate and more specifically a white substance made from lead carbonate, used mainly in paint and formerly as make-up, but banned since the early 20th century because of its toxicity (cnrtl)</skos:definition>
	<skos:definition xml:lang="ar">كربونات الرصاص ـ المعجم المزدوج</skos:definition>
</rdf:Description>

<rdf:Description rdf:about="https://ark.frantiq.fr/ark:/26678/pcrtbRoB6J1AY7">
	<rdf:type rdf:resource="http://www.w3.org/2004/02/skos/core#Concept"/>
	<skos:prefLabel xml:lang="es">nicotina</skos:prefLabel>
	<skos:prefLabel xml:lang="it">nicotina</skos:prefLabel>
	<skos:prefLabel xml:lang="en">nicotine</skos:prefLabel>
	<skos:prefLabel xml:lang="fr">nicotine</skos:prefLabel>
	<skos:prefLabel xml:lang="nl">nicotine</skos:prefLabel>
	<skos:prefLabel xml:lang="de">Nikotin</skos:prefLabel>
	<skos:prefLabel xml:lang="ar">نيكوتين</skos:prefLabel>
	<skos:related rdf:resource="https://ark.frantiq.fr/ark:/26678/pcrtXLoNEjBvnw"/>
	<skos:broader rdf:resource="https://ark.frantiq.fr/ark:/26678/pcrtuxpF5YgM3S"/>
	<skos:inScheme rdf:resource="https://ark.frantiq.fr/ark:/26678/TH_1"/>
	<opentheso:memberOf rdf:resource="https://ark.frantiq.fr/ark:/26678/pcrtv66rn9cbv1"/>
	<opentheso:memberOf rdf:resource="https://ark.frantiq.fr/ark:/26678/pcrtnbDLi2FkAj"/>
	<skos:exactMatch rdf:resource="https://www.wikidata.org/wiki/Q28086552"/>
	<dcterms:created rdf:datatype="http://www.w3.org/2001/XMLSchema#date">2013-09-18</dcterms:created>
	<dcterms:modified rdf:datatype="http://www.w3.org/2001/XMLSchema#date">2023-08-02</dcterms:modified>
	<dcterms:identifier>36429</dcterms:identifier>
	<dcterms:contributor>blandine.nouvel</dcterms:contributor>
	<skos:definition xml:lang="en">Alkaloid found in plants of the Solanaceae family. (Wikipedia)</skos:definition>
	<skos:definition xml:lang="fr">Alcaloïde présent dans les plantes de la famille des solanacées. (Wikipédia)</skos:definition>
</rdf:Description>

<rdf:Description rdf:about="https://ark.frantiq.fr/ark:/26678/pcrtZ6enHsm9bu">
	<rdf:type rdf:resource="http://www.w3.org/2004/02/skos/core#Concept"/>
	<skos:prefLabel xml:lang="it">cocaina</skos:prefLabel>
	<skos:prefLabel xml:lang="es">cocaína</skos:prefLabel>
	<skos:prefLabel xml:lang="en">cocaine</skos:prefLabel>
	<skos:prefLabel xml:lang="fr">cocaïne</skos:prefLabel>
	<skos:prefLabel xml:lang="nl">cocaïne</skos:prefLabel>
	<skos:prefLabel xml:lang="de">Kokain</skos:prefLabel>
	<skos:prefLabel xml:lang="ar">كوكائين</skos:prefLabel>
	<skos:related rdf:resource="https://ark.frantiq.fr/ark:/26678/pcrtzRLONNn2X7"/>
	<skos:broader rdf:resource="https://ark.frantiq.fr/ark:/26678/pcrtuxpF5YgM3S"/>
	<skos:inScheme rdf:resource="https://ark.frantiq.fr/ark:/26678/TH_1"/>
	<opentheso:memberOf rdf:resource="https://ark.frantiq.fr/ark:/26678/pcrtv66rn9cbv1"/>
	<opentheso:memberOf rdf:resource="https://ark.frantiq.fr/ark:/26678/pcrtnbDLi2FkAj"/>
	<skos:exactMatch rdf:resource="https://catalogue.bnf.fr/ark:/12148/cb11967516j"/>
	<skos:exactMatch rdf:resource="https://www.wikidata.org/wiki/Q41576"/>
	<dcterms:created rdf:datatype="http://www.w3.org/2001/XMLSchema#date">2013-09-18</dcterms:created>
	<dcterms:modified rdf:datatype="http://www.w3.org/2001/XMLSchema#date">2024-03-20</dcterms:modified>
	<dcterms:identifier>36431</dcterms:identifier>
	<dcterms:contributor>blandine.nouvel</dcterms:contributor>
	<dcterms:contributor>justine.vincent</dcterms:contributor>
	<skos:definition xml:lang="en">Tropanic alkaloid extracted from coca, known for its psychotropic effects.</skos:definition>
	<skos:definition xml:lang="fr">Alcaloïde tropanique extrait de la coca, connu pour ses effets psychotropes.</skos:definition>
</rdf:Description>

<rdf:Description rdf:about="https://ark.frantiq.fr/ark:/26678/pcrttAmNtvNqnf">
	<rdf:type rdf:resource="http://www.w3.org/2004/02/skos/core#Concept"/>
	<skos:prefLabel xml:lang="en">carmine</skos:prefLabel>
	<skos:prefLabel xml:lang="it">cocciniglia</skos:prefLabel>
	<skos:prefLabel xml:lang="fr">cochenille</skos:prefLabel>
	<skos:prefLabel xml:lang="es">cochinilla</skos:prefLabel>
	<skos:prefLabel xml:lang="de">Karmin</skos:prefLabel>
	<skos:prefLabel xml:lang="ar">قرمزي</skos:prefLabel>
	<skos:altLabel xml:lang="fr">Acide carminique</skos:altLabel>
	<skos:altLabel xml:lang="fr">carmin de cochenille</skos:altLabel>
	<skos:altLabel xml:lang="en">carmine dye</skos:altLabel>
	<skos:altLabel xml:lang="en">cochineal</skos:altLabel>
	<skos:altLabel xml:lang="en">cochineal extractcarminic acid</skos:altLabel>
	<skos:altLabel xml:lang="es">cochinilla del carmín</skos:altLabel>
	<skos:altLabel xml:lang="de">Karminsäure</skos:altLabel>
	<skos:altLabel xml:lang="de">Koschenille</skos:altLabel>
	<skos:related rdf:resource="https://ark.frantiq.fr/ark:/26678/pcrtEBpIym4SMO"/>
	<skos:broader rdf:resource="https://ark.frantiq.fr/ark:/26678/pcrtGzQPnntJa1"/>
	<skos:inScheme rdf:resource="https://ark.frantiq.fr/ark:/26678/TH_1"/>
	<opentheso:memberOf rdf:resource="https://ark.frantiq.fr/ark:/26678/pcrtv66rn9cbv1"/>
	<opentheso:memberOf rdf:resource="https://ark.frantiq.fr/ark:/26678/pcrtnbDLi2FkAj"/>
	<skos:exactMatch rdf:resource="https://www.wikidata.org/wiki/Q320617"/>
	<skos:exactMatch rdf:resource="https://www.wikidata.org/wiki/Q340228"/>
	<skos:exactMatch rdf:resource="http://vocab.getty.edu/aat/300013587"/>
	<dcterms:created rdf:datatype="http://www.w3.org/2001/XMLSchema#date">2013-09-23</dcterms:created>
	<dcterms:modified rdf:datatype="http://www.w3.org/2001/XMLSchema#date">2023-08-02</dcterms:modified>
	<dcterms:identifier>36468</dcterms:identifier>
	<dcterms:contributor>blandine.nouvel</dcterms:contributor>
	<skos:definition xml:lang="en">Deep purple dye extracted from the female cochineal (dactylopius coccus). (Wikipedia)</skos:definition>
	<skos:definition xml:lang="fr">Teinture d'un pourpre profond extraite de la femelle cochenille (dactylopius coccus). (Wikipédia)</skos:definition>
</rdf:Description>

<rdf:Description rdf:about="https://ark.frantiq.fr/ark:/26678/pcrtu714SnuAFj">
	<rdf:type rdf:resource="http://www.w3.org/2004/02/skos/core#Concept"/>
	<skos:prefLabel xml:lang="nl">bauxiet</skos:prefLabel>
	<skos:prefLabel xml:lang="de">Bauxit</skos:prefLabel>
	<skos:prefLabel xml:lang="es">bauxita</skos:prefLabel>
	<skos:prefLabel xml:lang="en">bauxite</skos:prefLabel>
	<skos:prefLabel xml:lang="fr">bauxite</skos:prefLabel>
	<skos:prefLabel xml:lang="it">bauxite</skos:prefLabel>
	<skos:prefLabel xml:lang="ar">بوكسيت</skos:prefLabel>
	<skos:altLabel xml:lang="it">baussite</skos:altLabel>
	<skos:broader rdf:resource="https://ark.frantiq.fr/ark:/26678/pcrtj3ZcwkArSR"/>
	<skos:inScheme rdf:resource="https://ark.frantiq.fr/ark:/26678/TH_1"/>
	<opentheso:memberOf rdf:resource="https://ark.frantiq.fr/ark:/26678/pcrtv66rn9cbv1"/>
	<opentheso:memberOf rdf:resource="https://ark.frantiq.fr/ark:/26678/pcrtnbDLi2FkAj"/>
	<skos:exactMatch rdf:resource="https://catalogue.bnf.fr/ark:/12148/cb119407803"/>
	<skos:exactMatch rdf:resource="https://www.wikidata.org/wiki/Q102078"/>
	<skos:exactMatch rdf:resource="http://vocab.getty.edu/aat/300387544"/>
	<dcterms:created rdf:datatype="http://www.w3.org/2001/XMLSchema#date">2013-09-24</dcterms:created>
	<dcterms:modified rdf:datatype="http://www.w3.org/2001/XMLSchema#date">2024-11-18</dcterms:modified>
	<dcterms:identifier>36507</dcterms:identifier>
	<dcterms:contributor>blandine.nouvel</dcterms:contributor>
	<dcterms:contributor>justine.vincent</dcterms:contributor>
	<skos:definition xml:lang="fr">Roche sédimentaire ou résiduelle, à forte teneur en alumine et en oxydes de fer, constituant le principal minerai permettant la production d'aluminium (d'ap. Foucault et Raoult, 2005).</skos:definition>
	<skos:definition xml:lang="en">Sedimentary or residual rock with a high alumina and iron oxide content, the main ore used in aluminium production (after Foucault and Raoult, 2005).</skos:definition>
	<skos:definition xml:lang="ar">صخر غني بالألومنيوم</skos:definition>
</rdf:Description>

<rdf:Description rdf:about="https://ark.frantiq.fr/ark:/26678/pcrtupN3PAxWw0">
	<rdf:type rdf:resource="http://www.w3.org/2004/02/skos/core#Concept"/>
	<skos:prefLabel xml:lang="nl">parel</skos:prefLabel>
	<skos:prefLabel xml:lang="en">pearl</skos:prefLabel>
	<skos:prefLabel xml:lang="es">perla</skos:prefLabel>
	<skos:prefLabel xml:lang="it">perla</skos:prefLabel>
	<skos:prefLabel xml:lang="fr">perle de nacre</skos:prefLabel>
	<skos:prefLabel xml:lang="de">Perlmuttperle</skos:prefLabel>
	<skos:prefLabel xml:lang="ar">صدفة أم اللؤلؤ</skos:prefLabel>
	<skos:related rdf:resource="https://ark.frantiq.fr/ark:/26678/pcrtcOdrZSUYkk"/>
	<skos:related rdf:resource="https://ark.frantiq.fr/ark:/26678/pcrtT4hbrNQwkc"/>
	<skos:broader rdf:resource="https://ark.frantiq.fr/ark:/26678/pcrtmoM3SzhDcB"/>
	<skos:inScheme rdf:resource="https://ark.frantiq.fr/ark:/26678/TH_1"/>
	<opentheso:memberOf rdf:resource="https://ark.frantiq.fr/ark:/26678/pcrtv66rn9cbv1"/>
	<opentheso:memberOf rdf:resource="https://ark.frantiq.fr/ark:/26678/pcrtnbDLi2FkAj"/>
	<skos:exactMatch rdf:resource="https://catalogue.bnf.fr/ark:/12148/cb12049526h"/>
	<skos:exactMatch rdf:resource="https://www.wikidata.org/wiki/Q43436"/>
	<skos:exactMatch rdf:resource="http://vocab.getty.edu/aat/300011827"/>
	<dcterms:created rdf:datatype="http://www.w3.org/2001/XMLSchema#date">2013-09-24</dcterms:created>
	<dcterms:modified rdf:datatype="http://www.w3.org/2001/XMLSchema#date">2023-08-02</dcterms:modified>
	<dcterms:identifier>36515</dcterms:identifier>
	<dcterms:contributor>blandine.nouvel</dcterms:contributor>
	<skos:definition xml:lang="en">Small concretion, generally spherical, of a silvery white colour with iridescent reflections, which is formed by the secretion of concentric layers of mother-of-pearl around a parasitic body which has entered the shell of certain marine (oyster) or freshwater molluscs, and which is sought after for the manufacture of jewellery or ornaments. (TLF)</skos:definition>
	<skos:definition xml:lang="fr">Petite concrétion, généralement sphérique, d'un blanc argentin à reflets irisés, qui se forme par sécrétion de couches concentriques de nacre autour d'un corps parasite entré dans la coquille de certains mollusques marins (huîtres) ou d'eau douce, et qui est recherchée pour la fabrication des bijoux ou des parures. (TLF)</skos:definition>
</rdf:Description>

<rdf:Description rdf:about="https://ark.frantiq.fr/ark:/26678/pcrtK2sVvLapYR">
	<rdf:type rdf:resource="http://www.w3.org/2004/02/skos/core#Concept"/>
	<skos:prefLabel xml:lang="it">porpora</skos:prefLabel>
	<skos:prefLabel xml:lang="fr">pourpre (teinture)</skos:prefLabel>
	<skos:prefLabel xml:lang="en">purple</skos:prefLabel>
	<skos:prefLabel xml:lang="es">púrpura</skos:prefLabel>
	<skos:prefLabel xml:lang="de">Purpur (Farbstoff)</skos:prefLabel>
	<skos:prefLabel xml:lang="ar">(أرجواني (صباغ</skos:prefLabel>
	<skos:related rdf:resource="https://ark.frantiq.fr/ark:/26678/pcrtvb5yPkXYYL"/>
	<skos:related rdf:resource="https://ark.frantiq.fr/ark:/26678/pcrtEBpIym4SMO"/>
	<skos:broader rdf:resource="https://ark.frantiq.fr/ark:/26678/pcrtGzQPnntJa1"/>
	<skos:inScheme rdf:resource="https://ark.frantiq.fr/ark:/26678/TH_1"/>
	<opentheso:memberOf rdf:resource="https://ark.frantiq.fr/ark:/26678/pcrtv66rn9cbv1"/>
	<opentheso:memberOf rdf:resource="https://ark.frantiq.fr/ark:/26678/pcrtnbDLi2FkAj"/>
	<skos:exactMatch rdf:resource="https://www.wikidata.org/wiki/Q3257809"/>
	<skos:exactMatch rdf:resource="https://www.wikidata.org/wiki/Q5180360"/>
	<skos:exactMatch rdf:resource="http://vocab.getty.edu/aat/300013087"/>
	<dcterms:created rdf:datatype="http://www.w3.org/2001/XMLSchema#date">2013-10-09</dcterms:created>
	<dcterms:modified rdf:datatype="http://www.w3.org/2001/XMLSchema#date">2024-11-18</dcterms:modified>
	<dcterms:identifier>36821</dcterms:identifier>
	<dcterms:contributor>blandine.nouvel</dcterms:contributor>
	<dcterms:contributor>justine.vincent</dcterms:contributor>
	<skos:definition xml:lang="en">A deep purplish-red dye of animal origin already used by the Phoenicians and Aegeans. (Wikipedia)</skos:definition>
	<skos:definition xml:lang="fr">Teinture rouge violacée profond d'origine animale déjà en usage chez les Phéniciens et les Égéens. (Wikipedia)</skos:definition>
	<skos:historyNote xml:lang="fr">2024-18-11 : modification de la définition.</skos:historyNote>
</rdf:Description>

<rdf:Description rdf:about="https://ark.frantiq.fr/ark:/26678/pcrtFwQpNgFwZo">
	<rdf:type rdf:resource="http://www.w3.org/2004/02/skos/core#Concept"/>
	<skos:prefLabel xml:lang="es">macroalga</skos:prefLabel>
	<skos:prefLabel xml:lang="en">seaweed</skos:prefLabel>
	<skos:prefLabel xml:lang="de">Seetang</skos:prefLabel>
	<skos:prefLabel xml:lang="fr">varech</skos:prefLabel>
	<skos:prefLabel xml:lang="it">varech</skos:prefLabel>
	<skos:prefLabel xml:lang="ar">فَوْقس</skos:prefLabel>
	<skos:altLabel xml:lang="en">algae</skos:altLabel>
	<skos:altLabel xml:lang="fr">goémon</skos:altLabel>
	<skos:altLabel xml:lang="de">marine Makroalgen</skos:altLabel>
	<skos:related rdf:resource="https://ark.frantiq.fr/ark:/26678/pcrtlLaVIacMMt"/>
	<skos:related rdf:resource="https://ark.frantiq.fr/ark:/26678/pcrtP3aHTZILi9"/>
	<skos:broader rdf:resource="https://ark.frantiq.fr/ark:/26678/pcrtnHxyjOkhJw"/>
	<skos:inScheme rdf:resource="https://ark.frantiq.fr/ark:/26678/TH_1"/>
	<opentheso:memberOf rdf:resource="https://ark.frantiq.fr/ark:/26678/pcrtv66rn9cbv1"/>
	<opentheso:memberOf rdf:resource="https://ark.frantiq.fr/ark:/26678/pcrtnbDLi2FkAj"/>
	<skos:exactMatch rdf:resource="https://catalogue.bnf.fr/ark:/12148/cb11940267h"/>
	<skos:exactMatch rdf:resource="https://www.wikidata.org/wiki/Q237169"/>
	<dcterms:created rdf:datatype="http://www.w3.org/2001/XMLSchema#date">2013-10-11</dcterms:created>
	<dcterms:modified rdf:datatype="http://www.w3.org/2001/XMLSchema#date">2023-08-02</dcterms:modified>
	<dcterms:identifier>36826</dcterms:identifier>
	<dcterms:contributor>blandine.nouvel</dcterms:contributor>
	<skos:definition xml:lang="en">An indeterminate mixture of brown, red or green seaweed left behind by receding tides and harvested along sea coasts, particularly in Brittany, mainly for use as fertiliser. (Wikipedia)</skos:definition>
	<skos:definition xml:lang="ar">طحالب بحرية بُنيَّة اللون</skos:definition>
	<skos:definition xml:lang="fr">Mélange indéterminé d'algues brunes, rouges ou vertes, laissées par le retrait des marées, et que l'on récolte le long des côtes maritimes, notamment en Bretagne, essentiellement à l'usage d'engrais. (Wikipédia)</skos:definition>
</rdf:Description>

<rdf:Description rdf:about="https://ark.frantiq.fr/ark:/26678/pcrta0mEYU6AUY">
	<rdf:type rdf:resource="http://www.w3.org/2004/02/skos/core#Concept"/>
	<skos:prefLabel xml:lang="it">ceramica comune non tornita</skos:prefLabel>
	<skos:prefLabel xml:lang="es">cerámica común no torneada</skos:prefLabel>
	<skos:prefLabel xml:lang="fr">céramique commune non tournée</skos:prefLabel>
	<skos:prefLabel xml:lang="en">hand-built pottery</skos:prefLabel>
	<skos:prefLabel xml:lang="de">handgefertigte Gebrauchsware</skos:prefLabel>
	<skos:prefLabel xml:lang="ar">خزف غير مُصنَّع بالدولاب</skos:prefLabel>
	<skos:broader rdf:resource="https://ark.frantiq.fr/ark:/26678/pcrtho8l95no0j"/>
	<skos:inScheme rdf:resource="https://ark.frantiq.fr/ark:/26678/TH_1"/>
	<opentheso:memberOf rdf:resource="https://ark.frantiq.fr/ark:/26678/pcrtv66rn9cbv1"/>
	<opentheso:memberOf rdf:resource="https://ark.frantiq.fr/ark:/26678/pcrtnbDLi2FkAj"/>
	<skos:broadMatch rdf:resource="https://ark.mom.fr/ark:/39676/bib9z4b0wqmdk"/>
	<skos:closeMatch rdf:resource="https://ark.mom.fr/ark:/39676/bibcdhc232x3v"/>
	<dcterms:created rdf:datatype="http://www.w3.org/2001/XMLSchema#date">2013-10-16</dcterms:created>
	<dcterms:modified rdf:datatype="http://www.w3.org/2001/XMLSchema#date">2023-08-02</dcterms:modified>
	<dcterms:identifier>37039</dcterms:identifier>
	<dcterms:contributor>blandine.nouvel</dcterms:contributor>
	<skos:definition xml:lang="en">Ceramic characterised by the fact that the centrifugal force of the potter's wheel was not used to produce the shape (after P. Argelin, Lattara 6).</skos:definition>
	<skos:definition xml:lang="fr">Céramique caractérisée par la non utilisation de la force centrifuge du tour de potier dans l’élaboration de la forme. (d'après P. Argelin, Lattara 6)</skos:definition>
</rdf:Description>

<rdf:Description rdf:about="https://ark.frantiq.fr/ark:/26678/pcrtbjSdl4I8Mo">
	<rdf:type rdf:resource="http://www.w3.org/2004/02/skos/core#Concept"/>
	<skos:prefLabel xml:lang="en">chocolate flint</skos:prefLabel>
	<skos:prefLabel xml:lang="de">dunkelbrauner Silex</skos:prefLabel>
	<skos:prefLabel xml:lang="es">pedernal color chocolate</skos:prefLabel>
	<skos:prefLabel xml:lang="it">selce color cioccolato</skos:prefLabel>
	<skos:prefLabel xml:lang="fr">silex chocolat</skos:prefLabel>
	<skos:prefLabel xml:lang="ar">صوان  بنِّي داكن</skos:prefLabel>
	<skos:broader rdf:resource="https://ark.frantiq.fr/ark:/26678/pcrtIzSUofuocv"/>
	<skos:inScheme rdf:resource="https://ark.frantiq.fr/ark:/26678/TH_1"/>
	<opentheso:memberOf rdf:resource="https://ark.frantiq.fr/ark:/26678/pcrtv66rn9cbv1"/>
	<opentheso:memberOf rdf:resource="https://ark.frantiq.fr/ark:/26678/pcrtnbDLi2FkAj"/>
	<dcterms:created rdf:datatype="http://www.w3.org/2001/XMLSchema#date">2014-03-21</dcterms:created>
	<dcterms:modified rdf:datatype="http://www.w3.org/2001/XMLSchema#date">2023-08-02</dcterms:modified>
	<dcterms:identifier>38506</dcterms:identifier>
	<dcterms:contributor>blandine.nouvel</dcterms:contributor>
	<skos:definition xml:lang="fr">Silex noir à grain très fin.</skos:definition>
</rdf:Description>

</rdf:RDF>